<?xml version="1.0" encoding="UTF-8"?>
<rdf:RDF xmlns:rdf="http://www.w3.org/1999/02/22-rdf-syntax-ns#" xmlns:rdfs="http://www.w3.org/2000/01/rdf-schema#" xmlns:skos="http://www.w3.org/2004/02/skos/core#" xmlns:dc="http://purl.org/dc/elements/1.1/" xmlns:dct="http://purl.org/dc/terms/">
  <rdf:Description rdf:about="http://www.usgs.gov/science/USGSThesaurus">
    <rdf:type rdf:resource="http://www.w3.org/2004/02/skos/core#ConceptScheme"/>
    <dc:title xml:lang="en">USGS Thesaurus</dc:title>
    <dc:description xml:lang="en">Topics and methods of scientific study carried out by USGS, with product types, scientific disciplines, geologic time, and types of institutional structure and activities.  Broad and shallow, used to help people find scientific information.</dc:description>
    <dc:creator xml:lang="en">U.S. Geological Survey</dc:creator>
    <dc:date rdf:datatype="http://www.w3.org/2001/XMLSchema#dateTime">2014-10-16</dc:date>
    <dc:language>en</dc:language>
    <dc:rights xml:lang="en">Public domain</dc:rights>
    <dct:subject xml:lang="en">hierarchical</dct:subject>
    <dct:subject xml:lang="en">transitive</dct:subject>
    <dct:subject xml:lang="en">disciplines</dct:subject>
    <dct:subject xml:lang="en">methods</dct:subject>
    <dct:subject xml:lang="en">organizational functions</dct:subject>
    <dct:subject xml:lang="en">temporal</dct:subject>
    <dct:subject xml:lang="en">theme</dct:subject>
    <dct:subject xml:lang="en">distinct labels</dct:subject>
  </rdf:Description>
  <rdf:Description about="http://www.usgs.gov/science/USGSThesaurus/Categories">
    <rdf:type rdf:resource="http://www.w3.org/2004/02/skos/core#Concept"/>
    <skos:prefLabel xml:lang="en">Categories</skos:prefLabel>
    <skos:scopeNote xml:lang="en">Thematic terms for categorizing information resources.  This thesaurus is intended to support finding and understanding scientific information.</skos:scopeNote>
    <skos:narrower rdf:resource="http://www.usgs.gov/science/USGSThesaurus/institutional%20structures%20and%20activities"/>
    <skos:narrower rdf:resource="http://www.usgs.gov/science/USGSThesaurus/methods"/>
    <skos:narrower rdf:resource="http://www.usgs.gov/science/USGSThesaurus/product%20types"/>
    <skos:narrower rdf:resource="http://www.usgs.gov/science/USGSThesaurus/sciences"/>
    <skos:narrower rdf:resource="http://www.usgs.gov/science/USGSThesaurus/time%20periods"/>
    <skos:narrower rdf:resource="http://www.usgs.gov/science/USGSThesaurus/topics"/>
    <skos:inScheme rdf:resource="http://www.usgs.gov/science/USGSThesaurus"/>
  </rdf:Description>
  <rdf:Description about="http://www.usgs.gov/science/USGSThesaurus/institutional%20structures%20and%20activities">
    <rdf:type rdf:resource="http://www.w3.org/2004/02/skos/core#Concept"/>
    <skos:prefLabel xml:lang="en">institutional structures and activities</skos:prefLabel>
    <skos:scopeNote xml:lang="en">Organizational characteristics, services, activities and physical infrastructure, primarily focused on those of the USGS</skos:scopeNote>
    <skos:broader rdf:resource="http://www.usgs.gov/science/USGSThesaurus/Categories"/>
    <skos:narrower rdf:resource="http://www.usgs.gov/science/USGSThesaurus/employment%20and%20volunteer%20opportunities"/>
    <skos:narrower rdf:resource="http://www.usgs.gov/science/USGSThesaurus/facilities"/>
    <skos:narrower rdf:resource="http://www.usgs.gov/science/USGSThesaurus/organizational%20structure"/>
    <skos:narrower rdf:resource="http://www.usgs.gov/science/USGSThesaurus/science%20programs"/>
    <skos:narrower rdf:resource="http://www.usgs.gov/science/USGSThesaurus/user%20services"/>
    <skos:inScheme rdf:resource="http://www.usgs.gov/science/USGSThesaurus"/>
  </rdf:Description>
  <rdf:Description about="http://www.usgs.gov/science/USGSThesaurus/employment%20and%20volunteer%20opportunities">
    <rdf:type rdf:resource="http://www.w3.org/2004/02/skos/core#Concept"/>
    <skos:prefLabel xml:lang="en">employment and volunteer opportunities</skos:prefLabel>
    <skos:scopeNote xml:lang="en"></skos:scopeNote>
    <skos:broader rdf:resource="http://www.usgs.gov/science/USGSThesaurus/institutional%20structures%20and%20activities"/>
    <skos:inScheme rdf:resource="http://www.usgs.gov/science/USGSThesaurus"/>
  </rdf:Description>
  <rdf:Description about="http://www.usgs.gov/science/USGSThesaurus/facilities">
    <rdf:type rdf:resource="http://www.w3.org/2004/02/skos/core#Concept"/>
    <skos:prefLabel xml:lang="en">facilities</skos:prefLabel>
    <skos:scopeNote xml:lang="en">Location, character, and general use of the physical offices used to carry out research, monitoring, and administration</skos:scopeNote>
    <skos:broader rdf:resource="http://www.usgs.gov/science/USGSThesaurus/institutional%20structures%20and%20activities"/>
    <skos:narrower rdf:resource="http://www.usgs.gov/science/USGSThesaurus/field%20offices"/>
    <skos:narrower rdf:resource="http://www.usgs.gov/science/USGSThesaurus/laboratories"/>
    <skos:narrower rdf:resource="http://www.usgs.gov/science/USGSThesaurus/libraries%20and%20archives"/>
    <skos:narrower rdf:resource="http://www.usgs.gov/science/USGSThesaurus/national%20centers"/>
    <skos:related rdf:resource="http://www.usgs.gov/science/USGSThesaurus/science%20centers"/>
    <skos:inScheme rdf:resource="http://www.usgs.gov/science/USGSThesaurus"/>
  </rdf:Description>
  <rdf:Description about="http://www.usgs.gov/science/USGSThesaurus/field%20offices">
    <rdf:type rdf:resource="http://www.w3.org/2004/02/skos/core#Concept"/>
    <skos:prefLabel xml:lang="en">field offices</skos:prefLabel>
    <skos:scopeNote xml:lang="en">Small branch of a science center not located at the headquarters of the science center</skos:scopeNote>
    <skos:altLabel xml:lang="en">field stations</skos:altLabel>
    <skos:broader rdf:resource="http://www.usgs.gov/science/USGSThesaurus/facilities"/>
    <skos:inScheme rdf:resource="http://www.usgs.gov/science/USGSThesaurus"/>
  </rdf:Description>
  <rdf:Description about="http://www.usgs.gov/science/USGSThesaurus/laboratories">
    <rdf:type rdf:resource="http://www.w3.org/2004/02/skos/core#Concept"/>
    <skos:prefLabel xml:lang="en">laboratories</skos:prefLabel>
    <skos:scopeNote xml:lang="en"></skos:scopeNote>
    <skos:altLabel xml:lang="en">nuclear reactors</skos:altLabel>
    <skos:broader rdf:resource="http://www.usgs.gov/science/USGSThesaurus/facilities"/>
    <skos:inScheme rdf:resource="http://www.usgs.gov/science/USGSThesaurus"/>
  </rdf:Description>
  <rdf:Description about="http://www.usgs.gov/science/USGSThesaurus/libraries%20and%20archives">
    <rdf:type rdf:resource="http://www.w3.org/2004/02/skos/core#Concept"/>
    <skos:prefLabel xml:lang="en">libraries and archives</skos:prefLabel>
    <skos:scopeNote xml:lang="en"></skos:scopeNote>
    <skos:broader rdf:resource="http://www.usgs.gov/science/USGSThesaurus/facilities"/>
    <skos:narrower rdf:resource="http://www.usgs.gov/science/USGSThesaurus/sample%20repositories"/>
    <skos:inScheme rdf:resource="http://www.usgs.gov/science/USGSThesaurus"/>
  </rdf:Description>
  <rdf:Description about="http://www.usgs.gov/science/USGSThesaurus/sample%20repositories">
    <rdf:type rdf:resource="http://www.w3.org/2004/02/skos/core#Concept"/>
    <skos:prefLabel xml:lang="en">sample repositories</skos:prefLabel>
    <skos:scopeNote xml:lang="en">Organized and curated collections of physical materials such as drill cores, rock samples, thin sections, and biological samples.</skos:scopeNote>
    <skos:altLabel xml:lang="en">core repositories</skos:altLabel>
    <skos:altLabel xml:lang="en">sample collections</skos:altLabel>
    <skos:broader rdf:resource="http://www.usgs.gov/science/USGSThesaurus/libraries%20and%20archives"/>
    <skos:inScheme rdf:resource="http://www.usgs.gov/science/USGSThesaurus"/>
  </rdf:Description>
  <rdf:Description about="http://www.usgs.gov/science/USGSThesaurus/national%20centers">
    <rdf:type rdf:resource="http://www.w3.org/2004/02/skos/core#Concept"/>
    <skos:prefLabel xml:lang="en">national centers</skos:prefLabel>
    <skos:scopeNote xml:lang="en">Research and monitoring office with a mission of nationwide scope</skos:scopeNote>
    <skos:broader rdf:resource="http://www.usgs.gov/science/USGSThesaurus/facilities"/>
    <skos:inScheme rdf:resource="http://www.usgs.gov/science/USGSThesaurus"/>
  </rdf:Description>
  <rdf:Description about="http://www.usgs.gov/science/USGSThesaurus/organizational%20structure">
    <rdf:type rdf:resource="http://www.w3.org/2004/02/skos/core#Concept"/>
    <skos:prefLabel xml:lang="en">organizational structure</skos:prefLabel>
    <skos:scopeNote xml:lang="en"></skos:scopeNote>
    <skos:broader rdf:resource="http://www.usgs.gov/science/USGSThesaurus/institutional%20structures%20and%20activities"/>
    <skos:narrower rdf:resource="http://www.usgs.gov/science/USGSThesaurus/mission%20directorates"/>
    <skos:narrower rdf:resource="http://www.usgs.gov/science/USGSThesaurus/regional%20offices"/>
    <skos:narrower rdf:resource="http://www.usgs.gov/science/USGSThesaurus/science%20centers"/>
    <skos:narrower rdf:resource="http://www.usgs.gov/science/USGSThesaurus/science%20discipline%20offices"/>
    <skos:narrower rdf:resource="http://www.usgs.gov/science/USGSThesaurus/support%20offices"/>
    <skos:inScheme rdf:resource="http://www.usgs.gov/science/USGSThesaurus"/>
  </rdf:Description>
  <rdf:Description about="http://www.usgs.gov/science/USGSThesaurus/mission%20directorates">
    <rdf:type rdf:resource="http://www.w3.org/2004/02/skos/core#Concept"/>
    <skos:prefLabel xml:lang="en">mission directorates</skos:prefLabel>
    <skos:scopeNote xml:lang="en">Offices charged with coordinating a variety of scientific activities focused on strategic objectives that may cross traditional scientific discipline boundaries.</skos:scopeNote>
    <skos:altLabel xml:lang="en">multidisciplinary directorates</skos:altLabel>
    <skos:altLabel xml:lang="en">interdisciplinary directorates</skos:altLabel>
    <skos:broader rdf:resource="http://www.usgs.gov/science/USGSThesaurus/organizational%20structure"/>
    <skos:inScheme rdf:resource="http://www.usgs.gov/science/USGSThesaurus"/>
  </rdf:Description>
  <rdf:Description about="http://www.usgs.gov/science/USGSThesaurus/regional%20offices">
    <rdf:type rdf:resource="http://www.w3.org/2004/02/skos/core#Concept"/>
    <skos:prefLabel xml:lang="en">regional offices</skos:prefLabel>
    <skos:scopeNote xml:lang="en">Multidisciplinary management offices overseeing specified geographic area</skos:scopeNote>
    <skos:broader rdf:resource="http://www.usgs.gov/science/USGSThesaurus/organizational%20structure"/>
    <skos:inScheme rdf:resource="http://www.usgs.gov/science/USGSThesaurus"/>
  </rdf:Description>
  <rdf:Description about="http://www.usgs.gov/science/USGSThesaurus/science%20centers">
    <rdf:type rdf:resource="http://www.w3.org/2004/02/skos/core#Concept"/>
    <skos:prefLabel xml:lang="en">science centers</skos:prefLabel>
    <skos:scopeNote xml:lang="en">Organizational units that carry out research or monitoring</skos:scopeNote>
    <skos:altLabel xml:lang="en">geophysical observatories</skos:altLabel>
    <skos:altLabel xml:lang="en">volcano observatories</skos:altLabel>
    <skos:broader rdf:resource="http://www.usgs.gov/science/USGSThesaurus/organizational%20structure"/>
    <skos:related rdf:resource="http://www.usgs.gov/science/USGSThesaurus/facilities"/>
    <skos:inScheme rdf:resource="http://www.usgs.gov/science/USGSThesaurus"/>
  </rdf:Description>
  <rdf:Description about="http://www.usgs.gov/science/USGSThesaurus/science%20discipline%20offices">
    <rdf:type rdf:resource="http://www.w3.org/2004/02/skos/core#Concept"/>
    <skos:prefLabel xml:lang="en">science discipline offices</skos:prefLabel>
    <skos:scopeNote xml:lang="en">Offices coordinating activities focused on traditional academic categories</skos:scopeNote>
    <skos:altLabel xml:lang="en">divisions</skos:altLabel>
    <skos:broader rdf:resource="http://www.usgs.gov/science/USGSThesaurus/organizational%20structure"/>
    <skos:related rdf:resource="http://www.usgs.gov/science/USGSThesaurus/science%20programs"/>
    <skos:inScheme rdf:resource="http://www.usgs.gov/science/USGSThesaurus"/>
  </rdf:Description>
  <rdf:Description about="http://www.usgs.gov/science/USGSThesaurus/support%20offices">
    <rdf:type rdf:resource="http://www.w3.org/2004/02/skos/core#Concept"/>
    <skos:prefLabel xml:lang="en">support offices</skos:prefLabel>
    <skos:scopeNote xml:lang="en">Organizational units that carry out administrative functions rather than research or monitoring</skos:scopeNote>
    <skos:broader rdf:resource="http://www.usgs.gov/science/USGSThesaurus/organizational%20structure"/>
    <skos:inScheme rdf:resource="http://www.usgs.gov/science/USGSThesaurus"/>
  </rdf:Description>
  <rdf:Description about="http://www.usgs.gov/science/USGSThesaurus/science%20programs">
    <rdf:type rdf:resource="http://www.w3.org/2004/02/skos/core#Concept"/>
    <skos:prefLabel xml:lang="en">science programs</skos:prefLabel>
    <skos:scopeNote xml:lang="en">Broadly organized scientific research and monitoring activities</skos:scopeNote>
    <skos:broader rdf:resource="http://www.usgs.gov/science/USGSThesaurus/institutional%20structures%20and%20activities"/>
    <skos:narrower rdf:resource="http://www.usgs.gov/science/USGSThesaurus/citizen%20science%20programs"/>
    <skos:narrower rdf:resource="http://www.usgs.gov/science/USGSThesaurus/external%20research%20support"/>
    <skos:narrower rdf:resource="http://www.usgs.gov/science/USGSThesaurus/interagency%20programs"/>
    <skos:narrower rdf:resource="http://www.usgs.gov/science/USGSThesaurus/interdisciplinary%20programs"/>
    <skos:narrower rdf:resource="http://www.usgs.gov/science/USGSThesaurus/international%20programs"/>
    <skos:narrower rdf:resource="http://www.usgs.gov/science/USGSThesaurus/partnerships"/>
    <skos:related rdf:resource="http://www.usgs.gov/science/USGSThesaurus/science%20discipline%20offices"/>
    <skos:inScheme rdf:resource="http://www.usgs.gov/science/USGSThesaurus"/>
  </rdf:Description>
  <rdf:Description about="http://www.usgs.gov/science/USGSThesaurus/citizen%20science%20programs">
    <rdf:type rdf:resource="http://www.w3.org/2004/02/skos/core#Concept"/>
    <skos:prefLabel xml:lang="en">citizen science programs</skos:prefLabel>
    <skos:scopeNote xml:lang="en">Observation or monitoring activities that include contributions from amateur or non-professional scientists or other citizen volunteers.</skos:scopeNote>
    <skos:altLabel xml:lang="en">public participation in scientific research</skos:altLabel>
    <skos:altLabel xml:lang="en">crowd sourcing (science)</skos:altLabel>
    <skos:broader rdf:resource="http://www.usgs.gov/science/USGSThesaurus/science%20programs"/>
    <skos:inScheme rdf:resource="http://www.usgs.gov/science/USGSThesaurus"/>
  </rdf:Description>
  <rdf:Description about="http://www.usgs.gov/science/USGSThesaurus/external%20research%20support">
    <rdf:type rdf:resource="http://www.w3.org/2004/02/skos/core#Concept"/>
    <skos:prefLabel xml:lang="en">external research support</skos:prefLabel>
    <skos:scopeNote xml:lang="en">Research carried out by external organizations or individuals through contracts or grants</skos:scopeNote>
    <skos:altLabel xml:lang="en">research grants</skos:altLabel>
    <skos:altLabel xml:lang="en">contract research programs</skos:altLabel>
    <skos:broader rdf:resource="http://www.usgs.gov/science/USGSThesaurus/science%20programs"/>
    <skos:inScheme rdf:resource="http://www.usgs.gov/science/USGSThesaurus"/>
  </rdf:Description>
  <rdf:Description about="http://www.usgs.gov/science/USGSThesaurus/interagency%20programs">
    <rdf:type rdf:resource="http://www.w3.org/2004/02/skos/core#Concept"/>
    <skos:prefLabel xml:lang="en">interagency programs</skos:prefLabel>
    <skos:scopeNote xml:lang="en">Ongoing organizational activities in which USGS works directly with other government agencies</skos:scopeNote>
    <skos:broader rdf:resource="http://www.usgs.gov/science/USGSThesaurus/science%20programs"/>
    <skos:inScheme rdf:resource="http://www.usgs.gov/science/USGSThesaurus"/>
  </rdf:Description>
  <rdf:Description about="http://www.usgs.gov/science/USGSThesaurus/interdisciplinary%20programs">
    <rdf:type rdf:resource="http://www.w3.org/2004/02/skos/core#Concept"/>
    <skos:prefLabel xml:lang="en">interdisciplinary programs</skos:prefLabel>
    <skos:scopeNote xml:lang="en">Major research and monitoring activities focused on topics that cross or integrate multiple traditional academic categories</skos:scopeNote>
    <skos:broader rdf:resource="http://www.usgs.gov/science/USGSThesaurus/science%20programs"/>
    <skos:inScheme rdf:resource="http://www.usgs.gov/science/USGSThesaurus"/>
  </rdf:Description>
  <rdf:Description about="http://www.usgs.gov/science/USGSThesaurus/international%20programs">
    <rdf:type rdf:resource="http://www.w3.org/2004/02/skos/core#Concept"/>
    <skos:prefLabel xml:lang="en">international programs</skos:prefLabel>
    <skos:scopeNote xml:lang="en">Organizational activities that USGS undertakes with cooperation and support of foreign governments or multinational organizations</skos:scopeNote>
    <skos:broader rdf:resource="http://www.usgs.gov/science/USGSThesaurus/science%20programs"/>
    <skos:inScheme rdf:resource="http://www.usgs.gov/science/USGSThesaurus"/>
  </rdf:Description>
  <rdf:Description about="http://www.usgs.gov/science/USGSThesaurus/partnerships">
    <rdf:type rdf:resource="http://www.w3.org/2004/02/skos/core#Concept"/>
    <skos:prefLabel xml:lang="en">partnerships</skos:prefLabel>
    <skos:scopeNote xml:lang="en">Formal collaborative relationships between USGS and other organizations</skos:scopeNote>
    <skos:altLabel xml:lang="en">cooperative agreements</skos:altLabel>
    <skos:broader rdf:resource="http://www.usgs.gov/science/USGSThesaurus/science%20programs"/>
    <skos:inScheme rdf:resource="http://www.usgs.gov/science/USGSThesaurus"/>
  </rdf:Description>
  <rdf:Description about="http://www.usgs.gov/science/USGSThesaurus/user%20services">
    <rdf:type rdf:resource="http://www.w3.org/2004/02/skos/core#Concept"/>
    <skos:prefLabel xml:lang="en">user services</skos:prefLabel>
    <skos:scopeNote xml:lang="en"></skos:scopeNote>
    <skos:broader rdf:resource="http://www.usgs.gov/science/USGSThesaurus/institutional%20structures%20and%20activities"/>
    <skos:narrower rdf:resource="http://www.usgs.gov/science/USGSThesaurus/community%20relations"/>
    <skos:narrower rdf:resource="http://www.usgs.gov/science/USGSThesaurus/customer%20support%20and%20user%20feedback"/>
    <skos:narrower rdf:resource="http://www.usgs.gov/science/USGSThesaurus/educational%20services"/>
    <skos:narrower rdf:resource="http://www.usgs.gov/science/USGSThesaurus/information%20services"/>
    <skos:narrower rdf:resource="http://www.usgs.gov/science/USGSThesaurus/media%20relations"/>
    <skos:narrower rdf:resource="http://www.usgs.gov/science/USGSThesaurus/standards%20development"/>
    <skos:inScheme rdf:resource="http://www.usgs.gov/science/USGSThesaurus"/>
  </rdf:Description>
  <rdf:Description about="http://www.usgs.gov/science/USGSThesaurus/community%20relations">
    <rdf:type rdf:resource="http://www.w3.org/2004/02/skos/core#Concept"/>
    <skos:prefLabel xml:lang="en">community relations</skos:prefLabel>
    <skos:scopeNote xml:lang="en"></skos:scopeNote>
    <skos:broader rdf:resource="http://www.usgs.gov/science/USGSThesaurus/user%20services"/>
    <skos:inScheme rdf:resource="http://www.usgs.gov/science/USGSThesaurus"/>
  </rdf:Description>
  <rdf:Description about="http://www.usgs.gov/science/USGSThesaurus/customer%20support%20and%20user%20feedback">
    <rdf:type rdf:resource="http://www.w3.org/2004/02/skos/core#Concept"/>
    <skos:prefLabel xml:lang="en">customer support and user feedback</skos:prefLabel>
    <skos:scopeNote xml:lang="en">Web sites focusing on assistance to users of USGS information products</skos:scopeNote>
    <skos:altLabel xml:lang="en">technical support</skos:altLabel>
    <skos:altLabel xml:lang="en">product support</skos:altLabel>
    <skos:broader rdf:resource="http://www.usgs.gov/science/USGSThesaurus/user%20services"/>
    <skos:inScheme rdf:resource="http://www.usgs.gov/science/USGSThesaurus"/>
  </rdf:Description>
  <rdf:Description about="http://www.usgs.gov/science/USGSThesaurus/educational%20services">
    <rdf:type rdf:resource="http://www.w3.org/2004/02/skos/core#Concept"/>
    <skos:prefLabel xml:lang="en">educational services</skos:prefLabel>
    <skos:scopeNote xml:lang="en"></skos:scopeNote>
    <skos:broader rdf:resource="http://www.usgs.gov/science/USGSThesaurus/user%20services"/>
    <skos:narrower rdf:resource="http://www.usgs.gov/science/USGSThesaurus/K-12%20resources"/>
    <skos:narrower rdf:resource="http://www.usgs.gov/science/USGSThesaurus/college%20resources"/>
    <skos:narrower rdf:resource="http://www.usgs.gov/science/USGSThesaurus/internship%20programs"/>
    <skos:narrower rdf:resource="http://www.usgs.gov/science/USGSThesaurus/lifelong%20learning%20resources"/>
    <skos:inScheme rdf:resource="http://www.usgs.gov/science/USGSThesaurus"/>
  </rdf:Description>
  <rdf:Description about="http://www.usgs.gov/science/USGSThesaurus/K-12%20resources">
    <rdf:type rdf:resource="http://www.w3.org/2004/02/skos/core#Concept"/>
    <skos:prefLabel xml:lang="en">K-12 resources</skos:prefLabel>
    <skos:scopeNote xml:lang="en"></skos:scopeNote>
    <skos:broader rdf:resource="http://www.usgs.gov/science/USGSThesaurus/educational%20services"/>
    <skos:inScheme rdf:resource="http://www.usgs.gov/science/USGSThesaurus"/>
  </rdf:Description>
  <rdf:Description about="http://www.usgs.gov/science/USGSThesaurus/college%20resources">
    <rdf:type rdf:resource="http://www.w3.org/2004/02/skos/core#Concept"/>
    <skos:prefLabel xml:lang="en">college resources</skos:prefLabel>
    <skos:scopeNote xml:lang="en"></skos:scopeNote>
    <skos:broader rdf:resource="http://www.usgs.gov/science/USGSThesaurus/educational%20services"/>
    <skos:inScheme rdf:resource="http://www.usgs.gov/science/USGSThesaurus"/>
  </rdf:Description>
  <rdf:Description about="http://www.usgs.gov/science/USGSThesaurus/internship%20programs">
    <rdf:type rdf:resource="http://www.w3.org/2004/02/skos/core#Concept"/>
    <skos:prefLabel xml:lang="en">internship programs</skos:prefLabel>
    <skos:scopeNote xml:lang="en"></skos:scopeNote>
    <skos:broader rdf:resource="http://www.usgs.gov/science/USGSThesaurus/educational%20services"/>
    <skos:inScheme rdf:resource="http://www.usgs.gov/science/USGSThesaurus"/>
  </rdf:Description>
  <rdf:Description about="http://www.usgs.gov/science/USGSThesaurus/lifelong%20learning%20resources">
    <rdf:type rdf:resource="http://www.w3.org/2004/02/skos/core#Concept"/>
    <skos:prefLabel xml:lang="en">lifelong learning resources</skos:prefLabel>
    <skos:scopeNote xml:lang="en"></skos:scopeNote>
    <skos:broader rdf:resource="http://www.usgs.gov/science/USGSThesaurus/educational%20services"/>
    <skos:inScheme rdf:resource="http://www.usgs.gov/science/USGSThesaurus"/>
  </rdf:Description>
  <rdf:Description about="http://www.usgs.gov/science/USGSThesaurus/information%20services">
    <rdf:type rdf:resource="http://www.w3.org/2004/02/skos/core#Concept"/>
    <skos:prefLabel xml:lang="en">information services</skos:prefLabel>
    <skos:scopeNote xml:lang="en"></skos:scopeNote>
    <!--FOR clearinghouses USE information services WITH catalogs and indexes-->
    <skos:altLabel xml:lang="en">clearinghouses</skos:altLabel>
    <skos:broader rdf:resource="http://www.usgs.gov/science/USGSThesaurus/user%20services"/>
    <skos:narrower rdf:resource="http://www.usgs.gov/science/USGSThesaurus/data%20services"/>
    <skos:narrower rdf:resource="http://www.usgs.gov/science/USGSThesaurus/map%20interfaces"/>
    <skos:narrower rdf:resource="http://www.usgs.gov/science/USGSThesaurus/news%20services"/>
    <skos:narrower rdf:resource="http://www.usgs.gov/science/USGSThesaurus/publishing"/>
    <skos:narrower rdf:resource="http://www.usgs.gov/science/USGSThesaurus/reference%20services"/>
    <skos:narrower rdf:resource="http://www.usgs.gov/science/USGSThesaurus/sales%20and%20distribution%20services"/>
    <skos:narrower rdf:resource="http://www.usgs.gov/science/USGSThesaurus/search%20services"/>
    <skos:inScheme rdf:resource="http://www.usgs.gov/science/USGSThesaurus"/>
  </rdf:Description>
  <rdf:Description about="http://www.usgs.gov/science/USGSThesaurus/data%20services">
    <rdf:type rdf:resource="http://www.w3.org/2004/02/skos/core#Concept"/>
    <skos:prefLabel xml:lang="en">data services</skos:prefLabel>
    <skos:scopeNote xml:lang="en"></skos:scopeNote>
    <skos:altLabel xml:lang="en">data downloading</skos:altLabel>
    <skos:broader rdf:resource="http://www.usgs.gov/science/USGSThesaurus/information%20services"/>
    <skos:narrower rdf:resource="http://www.usgs.gov/science/USGSThesaurus/application%20programming%20interfaces"/>
    <skos:inScheme rdf:resource="http://www.usgs.gov/science/USGSThesaurus"/>
  </rdf:Description>
  <rdf:Description about="http://www.usgs.gov/science/USGSThesaurus/application%20programming%20interfaces">
    <rdf:type rdf:resource="http://www.w3.org/2004/02/skos/core#Concept"/>
    <skos:prefLabel xml:lang="en">application programming interfaces</skos:prefLabel>
    <skos:scopeNote xml:lang="en">Internet services providing subsets of data in response to specific web requests.  For APIs that are not accessible through the internet, use scientific software.</skos:scopeNote>
    <skos:altLabel xml:lang="en">APIs</skos:altLabel>
    <skos:broader rdf:resource="http://www.usgs.gov/science/USGSThesaurus/data%20services"/>
    <skos:inScheme rdf:resource="http://www.usgs.gov/science/USGSThesaurus"/>
  </rdf:Description>
  <rdf:Description about="http://www.usgs.gov/science/USGSThesaurus/map%20interfaces">
    <rdf:type rdf:resource="http://www.w3.org/2004/02/skos/core#Concept"/>
    <skos:prefLabel xml:lang="en">map interfaces</skos:prefLabel>
    <skos:scopeNote xml:lang="en">Online interfaces showing interactive maps and geospatial information</skos:scopeNote>
    <skos:altLabel xml:lang="en">map servers</skos:altLabel>
    <skos:broader rdf:resource="http://www.usgs.gov/science/USGSThesaurus/information%20services"/>
    <skos:narrower rdf:resource="http://www.usgs.gov/science/USGSThesaurus/web%20map%20services"/>
    <skos:inScheme rdf:resource="http://www.usgs.gov/science/USGSThesaurus"/>
  </rdf:Description>
  <rdf:Description about="http://www.usgs.gov/science/USGSThesaurus/web%20map%20services">
    <rdf:type rdf:resource="http://www.w3.org/2004/02/skos/core#Concept"/>
    <skos:prefLabel xml:lang="en">web map services</skos:prefLabel>
    <skos:scopeNote xml:lang="en">Internet services providing geospatial information that conform to formally defined specifications, for use in GIS and mapping software.</skos:scopeNote>
    <skos:altLabel xml:lang="en">OGC WMS</skos:altLabel>
    <skos:altLabel xml:lang="en">OGC WFS</skos:altLabel>
    <skos:altLabel xml:lang="en">OGC WCS</skos:altLabel>
    <skos:altLabel xml:lang="en">GIS services</skos:altLabel>
    <skos:broader rdf:resource="http://www.usgs.gov/science/USGSThesaurus/map%20interfaces"/>
    <skos:inScheme rdf:resource="http://www.usgs.gov/science/USGSThesaurus"/>
  </rdf:Description>
  <rdf:Description about="http://www.usgs.gov/science/USGSThesaurus/news%20services">
    <rdf:type rdf:resource="http://www.w3.org/2004/02/skos/core#Concept"/>
    <skos:prefLabel xml:lang="en">news services</skos:prefLabel>
    <skos:scopeNote xml:lang="en">Summaries of time-sensitive information of interest to the public, may include short audio or video presentations, may provide subscription services</skos:scopeNote>
    <skos:broader rdf:resource="http://www.usgs.gov/science/USGSThesaurus/information%20services"/>
    <skos:inScheme rdf:resource="http://www.usgs.gov/science/USGSThesaurus"/>
  </rdf:Description>
  <rdf:Description about="http://www.usgs.gov/science/USGSThesaurus/publishing">
    <rdf:type rdf:resource="http://www.w3.org/2004/02/skos/core#Concept"/>
    <skos:prefLabel xml:lang="en">publishing</skos:prefLabel>
    <skos:scopeNote xml:lang="en">Policies and procedures by which information is reviewed, approved, formatted for public distribution.</skos:scopeNote>
    <skos:broader rdf:resource="http://www.usgs.gov/science/USGSThesaurus/information%20services"/>
    <skos:inScheme rdf:resource="http://www.usgs.gov/science/USGSThesaurus"/>
  </rdf:Description>
  <rdf:Description about="http://www.usgs.gov/science/USGSThesaurus/reference%20services">
    <rdf:type rdf:resource="http://www.w3.org/2004/02/skos/core#Concept"/>
    <skos:prefLabel xml:lang="en">reference services</skos:prefLabel>
    <skos:scopeNote xml:lang="en"></skos:scopeNote>
    <skos:altLabel xml:lang="en">Earth Science Information Centers (ESICs)</skos:altLabel>
    <skos:broader rdf:resource="http://www.usgs.gov/science/USGSThesaurus/information%20services"/>
    <skos:inScheme rdf:resource="http://www.usgs.gov/science/USGSThesaurus"/>
  </rdf:Description>
  <rdf:Description about="http://www.usgs.gov/science/USGSThesaurus/sales%20and%20distribution%20services">
    <rdf:type rdf:resource="http://www.w3.org/2004/02/skos/core#Concept"/>
    <skos:prefLabel xml:lang="en">sales and distribution services</skos:prefLabel>
    <skos:scopeNote xml:lang="en">Online services by which products may be purchased</skos:scopeNote>
    <skos:altLabel xml:lang="en">maps on demand</skos:altLabel>
    <skos:broader rdf:resource="http://www.usgs.gov/science/USGSThesaurus/information%20services"/>
    <skos:inScheme rdf:resource="http://www.usgs.gov/science/USGSThesaurus"/>
  </rdf:Description>
  <rdf:Description about="http://www.usgs.gov/science/USGSThesaurus/search%20services">
    <rdf:type rdf:resource="http://www.w3.org/2004/02/skos/core#Concept"/>
    <skos:prefLabel xml:lang="en">search services</skos:prefLabel>
    <skos:scopeNote xml:lang="en">Automated information search systems</skos:scopeNote>
    <skos:altLabel xml:lang="en">search engines</skos:altLabel>
    <skos:broader rdf:resource="http://www.usgs.gov/science/USGSThesaurus/information%20services"/>
    <skos:inScheme rdf:resource="http://www.usgs.gov/science/USGSThesaurus"/>
  </rdf:Description>
  <rdf:Description about="http://www.usgs.gov/science/USGSThesaurus/media%20relations">
    <rdf:type rdf:resource="http://www.w3.org/2004/02/skos/core#Concept"/>
    <skos:prefLabel xml:lang="en">media relations</skos:prefLabel>
    <skos:scopeNote xml:lang="en"></skos:scopeNote>
    <skos:broader rdf:resource="http://www.usgs.gov/science/USGSThesaurus/user%20services"/>
    <skos:inScheme rdf:resource="http://www.usgs.gov/science/USGSThesaurus"/>
  </rdf:Description>
  <rdf:Description about="http://www.usgs.gov/science/USGSThesaurus/standards%20development">
    <rdf:type rdf:resource="http://www.w3.org/2004/02/skos/core#Concept"/>
    <skos:prefLabel xml:lang="en">standards development</skos:prefLabel>
    <skos:scopeNote xml:lang="en">Creation and maintenance of formal specifications by which research and monitoring are carried out</skos:scopeNote>
    <skos:broader rdf:resource="http://www.usgs.gov/science/USGSThesaurus/user%20services"/>
    <skos:related rdf:resource="http://www.usgs.gov/science/USGSThesaurus/standards"/>
    <skos:inScheme rdf:resource="http://www.usgs.gov/science/USGSThesaurus"/>
  </rdf:Description>
  <rdf:Description about="http://www.usgs.gov/science/USGSThesaurus/methods">
    <rdf:type rdf:resource="http://www.w3.org/2004/02/skos/core#Concept"/>
    <skos:prefLabel xml:lang="en">methods</skos:prefLabel>
    <skos:scopeNote xml:lang="en">Techniques, methods, procedures, or strategies for research, management, collection, or analysis of scientific information in USGS.</skos:scopeNote>
    <skos:broader rdf:resource="http://www.usgs.gov/science/USGSThesaurus/Categories"/>
    <skos:narrower rdf:resource="http://www.usgs.gov/science/USGSThesaurus/computational%20methods"/>
    <skos:narrower rdf:resource="http://www.usgs.gov/science/USGSThesaurus/field%20methods"/>
    <skos:narrower rdf:resource="http://www.usgs.gov/science/USGSThesaurus/laboratory%20methods"/>
    <skos:narrower rdf:resource="http://www.usgs.gov/science/USGSThesaurus/management%20methods"/>
    <skos:narrower rdf:resource="http://www.usgs.gov/science/USGSThesaurus/photography"/>
    <skos:narrower rdf:resource="http://www.usgs.gov/science/USGSThesaurus/remote%20sensing"/>
    <skos:narrower rdf:resource="http://www.usgs.gov/science/USGSThesaurus/scientific%20interpretation"/>
    <skos:narrower rdf:resource="http://www.usgs.gov/science/USGSThesaurus/videography"/>
    <skos:inScheme rdf:resource="http://www.usgs.gov/science/USGSThesaurus"/>
  </rdf:Description>
  <rdf:Description about="http://www.usgs.gov/science/USGSThesaurus/computational%20methods">
    <rdf:type rdf:resource="http://www.w3.org/2004/02/skos/core#Concept"/>
    <skos:prefLabel xml:lang="en">computational methods</skos:prefLabel>
    <skos:scopeNote xml:lang="en">Mathematical techniques used to analyze numerical data.</skos:scopeNote>
    <skos:altLabel xml:lang="en">mathematical methods</skos:altLabel>
    <skos:broader rdf:resource="http://www.usgs.gov/science/USGSThesaurus/methods"/>
    <skos:narrower rdf:resource="http://www.usgs.gov/science/USGSThesaurus/image%20analysis"/>
    <skos:narrower rdf:resource="http://www.usgs.gov/science/USGSThesaurus/mathematical%20modeling"/>
    <skos:narrower rdf:resource="http://www.usgs.gov/science/USGSThesaurus/relative%20abundance%20analysis"/>
    <skos:narrower rdf:resource="http://www.usgs.gov/science/USGSThesaurus/spatial%20analysis"/>
    <skos:narrower rdf:resource="http://www.usgs.gov/science/USGSThesaurus/statistical%20analysis"/>
    <skos:narrower rdf:resource="http://www.usgs.gov/science/USGSThesaurus/topological%20analysis"/>
    <skos:narrower rdf:resource="http://www.usgs.gov/science/USGSThesaurus/visualization%20methods"/>
    <skos:inScheme rdf:resource="http://www.usgs.gov/science/USGSThesaurus"/>
  </rdf:Description>
  <rdf:Description about="http://www.usgs.gov/science/USGSThesaurus/image%20analysis">
    <rdf:type rdf:resource="http://www.w3.org/2004/02/skos/core#Concept"/>
    <skos:prefLabel xml:lang="en">image analysis</skos:prefLabel>
    <skos:scopeNote xml:lang="en">Pattern analysis of the shapes and textures of images to identify features and derive information about them.</skos:scopeNote>
    <skos:broader rdf:resource="http://www.usgs.gov/science/USGSThesaurus/computational%20methods"/>
    <skos:related rdf:resource="http://www.usgs.gov/science/USGSThesaurus/geography"/>
    <skos:related rdf:resource="http://www.usgs.gov/science/USGSThesaurus/geospatial%20analysis"/>
    <skos:related rdf:resource="http://www.usgs.gov/science/USGSThesaurus/spatial%20analysis"/>
    <skos:inScheme rdf:resource="http://www.usgs.gov/science/USGSThesaurus"/>
  </rdf:Description>
  <rdf:Description about="http://www.usgs.gov/science/USGSThesaurus/mathematical%20modeling">
    <rdf:type rdf:resource="http://www.w3.org/2004/02/skos/core#Concept"/>
    <skos:prefLabel xml:lang="en">mathematical modeling</skos:prefLabel>
    <skos:scopeNote xml:lang="en">Creating mathematical expressions to represent a simplified view of real-world systems.</skos:scopeNote>
    <skos:altLabel xml:lang="en">fractal geometric methods</skos:altLabel>
    <skos:altLabel xml:lang="en">groundwater flow modeling</skos:altLabel>
    <skos:altLabel xml:lang="en">modeling (mathematical)</skos:altLabel>
    <skos:altLabel xml:lang="en">numerical methods</skos:altLabel>
    <!--FOR streamflow modeling USE mathematical modeling WITH streamflow-->
    <skos:altLabel xml:lang="en">streamflow modeling</skos:altLabel>
    <skos:broader rdf:resource="http://www.usgs.gov/science/USGSThesaurus/computational%20methods"/>
    <skos:narrower rdf:resource="http://www.usgs.gov/science/USGSThesaurus/mathematical%20simulation"/>
    <skos:related rdf:resource="http://www.usgs.gov/science/USGSThesaurus/spatial%20analysis"/>
    <skos:inScheme rdf:resource="http://www.usgs.gov/science/USGSThesaurus"/>
  </rdf:Description>
  <rdf:Description about="http://www.usgs.gov/science/USGSThesaurus/mathematical%20simulation">
    <rdf:type rdf:resource="http://www.w3.org/2004/02/skos/core#Concept"/>
    <skos:prefLabel xml:lang="en">mathematical simulation</skos:prefLabel>
    <skos:scopeNote xml:lang="en">A computer algorithm or model, which was created to represent a simplified version of a real world situation.</skos:scopeNote>
    <skos:broader rdf:resource="http://www.usgs.gov/science/USGSThesaurus/mathematical%20modeling"/>
    <skos:inScheme rdf:resource="http://www.usgs.gov/science/USGSThesaurus"/>
  </rdf:Description>
  <rdf:Description about="http://www.usgs.gov/science/USGSThesaurus/relative%20abundance%20analysis">
    <rdf:type rdf:resource="http://www.w3.org/2004/02/skos/core#Concept"/>
    <skos:prefLabel xml:lang="en">relative abundance analysis</skos:prefLabel>
    <skos:scopeNote xml:lang="en">Determination of the percentage of individuals of one group in comparison to the total of all individuals in a given area.</skos:scopeNote>
    <skos:broader rdf:resource="http://www.usgs.gov/science/USGSThesaurus/computational%20methods"/>
    <skos:related rdf:resource="http://www.usgs.gov/science/USGSThesaurus/ecosystem%20monitoring"/>
    <skos:related rdf:resource="http://www.usgs.gov/science/USGSThesaurus/population%20and%20community%20ecology"/>
    <skos:inScheme rdf:resource="http://www.usgs.gov/science/USGSThesaurus"/>
  </rdf:Description>
  <rdf:Description about="http://www.usgs.gov/science/USGSThesaurus/spatial%20analysis">
    <rdf:type rdf:resource="http://www.w3.org/2004/02/skos/core#Concept"/>
    <skos:prefLabel xml:lang="en">spatial analysis</skos:prefLabel>
    <skos:scopeNote xml:lang="en">Use of quantitative tools to study social, economic, and geographic data in relation to distributions and patterns in geographic space.</skos:scopeNote>
    <skos:broader rdf:resource="http://www.usgs.gov/science/USGSThesaurus/computational%20methods"/>
    <skos:narrower rdf:resource="http://www.usgs.gov/science/USGSThesaurus/geospatial%20analysis"/>
    <skos:related rdf:resource="http://www.usgs.gov/science/USGSThesaurus/geography"/>
    <skos:related rdf:resource="http://www.usgs.gov/science/USGSThesaurus/image%20analysis"/>
    <skos:related rdf:resource="http://www.usgs.gov/science/USGSThesaurus/mathematical%20modeling"/>
    <skos:related rdf:resource="http://www.usgs.gov/science/USGSThesaurus/topological%20analysis"/>
    <skos:inScheme rdf:resource="http://www.usgs.gov/science/USGSThesaurus"/>
  </rdf:Description>
  <rdf:Description about="http://www.usgs.gov/science/USGSThesaurus/geospatial%20analysis">
    <rdf:type rdf:resource="http://www.w3.org/2004/02/skos/core#Concept"/>
    <skos:prefLabel xml:lang="en">geospatial analysis</skos:prefLabel>
    <skos:scopeNote xml:lang="en">Detailed study of information such as measurements, counts, and computations as a function of geographical location.</skos:scopeNote>
    <skos:broader rdf:resource="http://www.usgs.gov/science/USGSThesaurus/spatial%20analysis"/>
    <skos:related rdf:resource="http://www.usgs.gov/science/USGSThesaurus/image%20analysis"/>
    <skos:related rdf:resource="http://www.usgs.gov/science/USGSThesaurus/topological%20analysis"/>
    <skos:inScheme rdf:resource="http://www.usgs.gov/science/USGSThesaurus"/>
  </rdf:Description>
  <rdf:Description about="http://www.usgs.gov/science/USGSThesaurus/statistical%20analysis">
    <rdf:type rdf:resource="http://www.w3.org/2004/02/skos/core#Concept"/>
    <skos:prefLabel xml:lang="en">statistical analysis</skos:prefLabel>
    <skos:scopeNote xml:lang="en">Branch of mathematics concerned with techniques to collect and interpret data.</skos:scopeNote>
    <skos:altLabel xml:lang="en">geostatistics</skos:altLabel>
    <skos:broader rdf:resource="http://www.usgs.gov/science/USGSThesaurus/computational%20methods"/>
    <skos:narrower rdf:resource="http://www.usgs.gov/science/USGSThesaurus/kriging"/>
    <skos:narrower rdf:resource="http://www.usgs.gov/science/USGSThesaurus/multivariate%20statistical%20analysis"/>
    <skos:narrower rdf:resource="http://www.usgs.gov/science/USGSThesaurus/regression%20analysis"/>
    <skos:narrower rdf:resource="http://www.usgs.gov/science/USGSThesaurus/time%20series%20analysis"/>
    <skos:inScheme rdf:resource="http://www.usgs.gov/science/USGSThesaurus"/>
  </rdf:Description>
  <rdf:Description about="http://www.usgs.gov/science/USGSThesaurus/kriging">
    <rdf:type rdf:resource="http://www.w3.org/2004/02/skos/core#Concept"/>
    <skos:prefLabel xml:lang="en">kriging</skos:prefLabel>
    <skos:scopeNote xml:lang="en">Statistical analysis technique which uses interpolation to best predict unknown data values from data observed at known locations.</skos:scopeNote>
    <skos:broader rdf:resource="http://www.usgs.gov/science/USGSThesaurus/statistical%20analysis"/>
    <skos:inScheme rdf:resource="http://www.usgs.gov/science/USGSThesaurus"/>
  </rdf:Description>
  <rdf:Description about="http://www.usgs.gov/science/USGSThesaurus/multivariate%20statistical%20analysis">
    <rdf:type rdf:resource="http://www.w3.org/2004/02/skos/core#Concept"/>
    <skos:prefLabel xml:lang="en">multivariate statistical analysis</skos:prefLabel>
    <skos:scopeNote xml:lang="en">Statistical study using a number of independent variables or measurements of the same attribute.</skos:scopeNote>
    <skos:broader rdf:resource="http://www.usgs.gov/science/USGSThesaurus/statistical%20analysis"/>
    <skos:inScheme rdf:resource="http://www.usgs.gov/science/USGSThesaurus"/>
  </rdf:Description>
  <rdf:Description about="http://www.usgs.gov/science/USGSThesaurus/regression%20analysis">
    <rdf:type rdf:resource="http://www.w3.org/2004/02/skos/core#Concept"/>
    <skos:prefLabel xml:lang="en">regression analysis</skos:prefLabel>
    <skos:scopeNote xml:lang="en">Statistical analysis based on the functional relationships of two or more related variables. Predicts the value of one variable when the other two are given.</skos:scopeNote>
    <skos:altLabel xml:lang="en">correlation</skos:altLabel>
    <skos:broader rdf:resource="http://www.usgs.gov/science/USGSThesaurus/statistical%20analysis"/>
    <skos:inScheme rdf:resource="http://www.usgs.gov/science/USGSThesaurus"/>
  </rdf:Description>
  <rdf:Description about="http://www.usgs.gov/science/USGSThesaurus/time%20series%20analysis">
    <rdf:type rdf:resource="http://www.w3.org/2004/02/skos/core#Concept"/>
    <skos:prefLabel xml:lang="en">time series analysis</skos:prefLabel>
    <skos:scopeNote xml:lang="en">Statistical analysis using frequency distribution in which time is an independent variable. A sequence of observations collected at regular time intervals is studied.</skos:scopeNote>
    <skos:broader rdf:resource="http://www.usgs.gov/science/USGSThesaurus/statistical%20analysis"/>
    <skos:related rdf:resource="http://www.usgs.gov/science/USGSThesaurus/time%20series%20datasets"/>
    <skos:inScheme rdf:resource="http://www.usgs.gov/science/USGSThesaurus"/>
  </rdf:Description>
  <rdf:Description about="http://www.usgs.gov/science/USGSThesaurus/topological%20analysis">
    <rdf:type rdf:resource="http://www.w3.org/2004/02/skos/core#Concept"/>
    <skos:prefLabel xml:lang="en">topological analysis</skos:prefLabel>
    <skos:scopeNote xml:lang="en">Branch of geometry concerned with the properties of objects that do not change even when deformed, twisted, stretched or otherwise changed in shape.</skos:scopeNote>
    <skos:broader rdf:resource="http://www.usgs.gov/science/USGSThesaurus/computational%20methods"/>
    <skos:related rdf:resource="http://www.usgs.gov/science/USGSThesaurus/geography"/>
    <skos:related rdf:resource="http://www.usgs.gov/science/USGSThesaurus/geospatial%20analysis"/>
    <skos:related rdf:resource="http://www.usgs.gov/science/USGSThesaurus/spatial%20analysis"/>
    <skos:inScheme rdf:resource="http://www.usgs.gov/science/USGSThesaurus"/>
  </rdf:Description>
  <rdf:Description about="http://www.usgs.gov/science/USGSThesaurus/visualization%20methods">
    <rdf:type rdf:resource="http://www.w3.org/2004/02/skos/core#Concept"/>
    <skos:prefLabel xml:lang="en">visualization methods</skos:prefLabel>
    <skos:scopeNote xml:lang="en">The application of two-dimensional or three-dimensional graphical techniques for the analysis and interpretation of complex numerical data.</skos:scopeNote>
    <skos:altLabel xml:lang="en">visualization</skos:altLabel>
    <skos:broader rdf:resource="http://www.usgs.gov/science/USGSThesaurus/computational%20methods"/>
    <skos:inScheme rdf:resource="http://www.usgs.gov/science/USGSThesaurus"/>
  </rdf:Description>
  <rdf:Description about="http://www.usgs.gov/science/USGSThesaurus/field%20methods">
    <rdf:type rdf:resource="http://www.w3.org/2004/02/skos/core#Concept"/>
    <skos:prefLabel xml:lang="en">field methods</skos:prefLabel>
    <skos:scopeNote xml:lang="en">Research procedures and instrumental means to measure, collect data and samples, and observe in the natural areas where the materials, phenomena, structures, or species being studied occur.</skos:scopeNote>
    <skos:broader rdf:resource="http://www.usgs.gov/science/USGSThesaurus/methods"/>
    <skos:narrower rdf:resource="http://www.usgs.gov/science/USGSThesaurus/field%20experiments"/>
    <skos:narrower rdf:resource="http://www.usgs.gov/science/USGSThesaurus/field%20inventory%20and%20monitoring"/>
    <skos:narrower rdf:resource="http://www.usgs.gov/science/USGSThesaurus/field%20sampling"/>
    <skos:narrower rdf:resource="http://www.usgs.gov/science/USGSThesaurus/geolocation%20measurement"/>
    <skos:narrower rdf:resource="http://www.usgs.gov/science/USGSThesaurus/real-time%20monitoring%20and%20reporting"/>
    <skos:inScheme rdf:resource="http://www.usgs.gov/science/USGSThesaurus"/>
  </rdf:Description>
  <rdf:Description about="http://www.usgs.gov/science/USGSThesaurus/field%20experiments">
    <rdf:type rdf:resource="http://www.w3.org/2004/02/skos/core#Concept"/>
    <skos:prefLabel xml:lang="en">field experiments</skos:prefLabel>
    <skos:scopeNote xml:lang="en">Deliberate arrangement of objects and events in the field to observe the behavioral response of natural systems or organisms.</skos:scopeNote>
    <skos:broader rdf:resource="http://www.usgs.gov/science/USGSThesaurus/field%20methods"/>
    <skos:narrower rdf:resource="http://www.usgs.gov/science/USGSThesaurus/tracer%20study"/>
    <skos:inScheme rdf:resource="http://www.usgs.gov/science/USGSThesaurus"/>
  </rdf:Description>
  <rdf:Description about="http://www.usgs.gov/science/USGSThesaurus/tracer%20study">
    <rdf:type rdf:resource="http://www.w3.org/2004/02/skos/core#Concept"/>
    <skos:prefLabel xml:lang="en">tracer study</skos:prefLabel>
    <skos:scopeNote xml:lang="en">Experiments in which stable, easily detected substances or radioisotopes are added to a material to follow the movement of the substance in the environment or to detect any physical or chemical changes with time.</skos:scopeNote>
    <skos:altLabel xml:lang="en">isotopic tracer study</skos:altLabel>
    <skos:altLabel xml:lang="en">radioisotope tracer study</skos:altLabel>
    <skos:broader rdf:resource="http://www.usgs.gov/science/USGSThesaurus/field%20experiments"/>
    <skos:inScheme rdf:resource="http://www.usgs.gov/science/USGSThesaurus"/>
  </rdf:Description>
  <rdf:Description about="http://www.usgs.gov/science/USGSThesaurus/field%20inventory%20and%20monitoring">
    <rdf:type rdf:resource="http://www.w3.org/2004/02/skos/core#Concept"/>
    <skos:prefLabel xml:lang="en">field inventory and monitoring</skos:prefLabel>
    <skos:scopeNote xml:lang="en">Repeated observation or sampling at a site, on a scheduled or event basis, for study and analysis.  In general, this category excludes sampling programs in which materials are obtained in the field and brought back to a laboratory for study and analysis.</skos:scopeNote>
    <skos:altLabel xml:lang="en">baseline characterization</skos:altLabel>
    <skos:altLabel xml:lang="en">field monitoring</skos:altLabel>
    <skos:altLabel xml:lang="en">field observation</skos:altLabel>
    <skos:altLabel xml:lang="en">inventory</skos:altLabel>
    <!--FOR ocean current measurement USE field inventory and monitoring WITH ocean currents-->
    <skos:altLabel xml:lang="en">ocean current measurement</skos:altLabel>
    <!--FOR ocean monitoring USE field inventory and monitoring WITH ocean characteristics-->
    <skos:altLabel xml:lang="en">ocean monitoring</skos:altLabel>
    <!--FOR ocean wave measurement USE field inventory and monitoring WITH ocean waves-->
    <skos:altLabel xml:lang="en">ocean wave measurement</skos:altLabel>
    <skos:altLabel xml:lang="en">reconnaissance</skos:altLabel>
    <skos:altLabel xml:lang="en">river discharge monitoring</skos:altLabel>
    <!--FOR volcano monitoring USE field inventory and monitoring WITH volcanic activity-->
    <skos:altLabel xml:lang="en">volcano monitoring</skos:altLabel>
    <!--FOR weather monitoring USE field inventory and monitoring WITH atmospheric and climatic processes-->
    <skos:altLabel xml:lang="en">weather monitoring</skos:altLabel>
    <!--FOR weather observations USE field inventory and monitoring WITH atmospheric and climatic processes-->
    <skos:altLabel xml:lang="en">weather observations</skos:altLabel>
    <!--FOR precipitation measurement USE field inventory and monitoring WITH precipitation (atmospheric)-->
    <skos:altLabel xml:lang="en">precipitation measurement</skos:altLabel>
    <!--FOR rainfall measurement USE field inventory and monitoring WITH precipitation (atmospheric)-->
    <skos:altLabel xml:lang="en">rainfall measurement</skos:altLabel>
    <!--FOR snowfall measurement USE field inventory and monitoring WITH precipitation (atmospheric)-->
    <skos:altLabel xml:lang="en">snowfall measurement</skos:altLabel>
    <skos:broader rdf:resource="http://www.usgs.gov/science/USGSThesaurus/field%20methods"/>
    <skos:narrower rdf:resource="http://www.usgs.gov/science/USGSThesaurus/CTD%20measurement"/>
    <skos:narrower rdf:resource="http://www.usgs.gov/science/USGSThesaurus/acoustic%20methods"/>
    <skos:narrower rdf:resource="http://www.usgs.gov/science/USGSThesaurus/animal%20and%20plant%20census"/>
    <skos:narrower rdf:resource="http://www.usgs.gov/science/USGSThesaurus/borehole%20logging"/>
    <skos:narrower rdf:resource="http://www.usgs.gov/science/USGSThesaurus/ecosystem%20monitoring"/>
    <skos:narrower rdf:resource="http://www.usgs.gov/science/USGSThesaurus/electromagnetic%20surveying"/>
    <skos:narrower rdf:resource="http://www.usgs.gov/science/USGSThesaurus/gravimeter%20measurement"/>
    <skos:narrower rdf:resource="http://www.usgs.gov/science/USGSThesaurus/handheld%20field%20spectroscopy"/>
    <skos:narrower rdf:resource="http://www.usgs.gov/science/USGSThesaurus/magnetometer%20measurement"/>
    <skos:narrower rdf:resource="http://www.usgs.gov/science/USGSThesaurus/optical%20methods"/>
    <skos:narrower rdf:resource="http://www.usgs.gov/science/USGSThesaurus/seismic%20methods"/>
    <skos:narrower rdf:resource="http://www.usgs.gov/science/USGSThesaurus/statistical%20surveying"/>
    <skos:narrower rdf:resource="http://www.usgs.gov/science/USGSThesaurus/stream-gage%20measurement"/>
    <skos:narrower rdf:resource="http://www.usgs.gov/science/USGSThesaurus/telemetry"/>
    <skos:narrower rdf:resource="http://www.usgs.gov/science/USGSThesaurus/tiltmeter%20measurement"/>
    <skos:narrower rdf:resource="http://www.usgs.gov/science/USGSThesaurus/tomography"/>
    <skos:narrower rdf:resource="http://www.usgs.gov/science/USGSThesaurus/video%20monitoring"/>
    <skos:narrower rdf:resource="http://www.usgs.gov/science/USGSThesaurus/vocalization%20methods"/>
    <skos:related rdf:resource="http://www.usgs.gov/science/USGSThesaurus/faunal%20and%20floral%20census%20%28microscopic%29"/>
    <skos:related rdf:resource="http://www.usgs.gov/science/USGSThesaurus/field%20monitoring%20stations"/>
    <skos:inScheme rdf:resource="http://www.usgs.gov/science/USGSThesaurus"/>
  </rdf:Description>
  <rdf:Description about="http://www.usgs.gov/science/USGSThesaurus/CTD%20measurement">
    <rdf:type rdf:resource="http://www.w3.org/2004/02/skos/core#Concept"/>
    <skos:prefLabel xml:lang="en">CTD measurement</skos:prefLabel>
    <skos:scopeNote xml:lang="en">Instrumental determination of conductivity, temperature, and pressure as a function of depth to determine the salinity of seawater.</skos:scopeNote>
    <skos:broader rdf:resource="http://www.usgs.gov/science/USGSThesaurus/field%20inventory%20and%20monitoring"/>
    <skos:related rdf:resource="http://www.usgs.gov/science/USGSThesaurus/limnology"/>
    <skos:related rdf:resource="http://www.usgs.gov/science/USGSThesaurus/marine%20chemistry"/>
    <skos:related rdf:resource="http://www.usgs.gov/science/USGSThesaurus/ocean%20sciences"/>
    <skos:inScheme rdf:resource="http://www.usgs.gov/science/USGSThesaurus"/>
  </rdf:Description>
  <rdf:Description about="http://www.usgs.gov/science/USGSThesaurus/acoustic%20methods">
    <rdf:type rdf:resource="http://www.w3.org/2004/02/skos/core#Concept"/>
    <skos:prefLabel xml:lang="en">acoustic methods</skos:prefLabel>
    <skos:scopeNote xml:lang="en">Study methods based on techniques of transmitting and receiving sound waves as well as measuring the properties of sound, such as pitch, absorption, frequency, intensity, or velocity.</skos:scopeNote>
    <skos:broader rdf:resource="http://www.usgs.gov/science/USGSThesaurus/field%20inventory%20and%20monitoring"/>
    <skos:narrower rdf:resource="http://www.usgs.gov/science/USGSThesaurus/acoustic%20doppler%20current%20profiling"/>
    <skos:narrower rdf:resource="http://www.usgs.gov/science/USGSThesaurus/sonar%20methods"/>
    <skos:inScheme rdf:resource="http://www.usgs.gov/science/USGSThesaurus"/>
  </rdf:Description>
  <rdf:Description about="http://www.usgs.gov/science/USGSThesaurus/acoustic%20doppler%20current%20profiling">
    <rdf:type rdf:resource="http://www.w3.org/2004/02/skos/core#Concept"/>
    <skos:prefLabel xml:lang="en">acoustic doppler current profiling</skos:prefLabel>
    <skos:scopeNote xml:lang="en">Field monitoring of water currents using the doppler effect with acoustic instruments.</skos:scopeNote>
    <skos:altLabel xml:lang="en">ADCP</skos:altLabel>
    <skos:altLabel xml:lang="en">hydroacoustics</skos:altLabel>
    <skos:altLabel xml:lang="en">acoustic doppler current profiler</skos:altLabel>
    <skos:broader rdf:resource="http://www.usgs.gov/science/USGSThesaurus/acoustic%20methods"/>
    <skos:related rdf:resource="http://www.usgs.gov/science/USGSThesaurus/stream-gage%20measurement"/>
    <skos:inScheme rdf:resource="http://www.usgs.gov/science/USGSThesaurus"/>
  </rdf:Description>
  <rdf:Description about="http://www.usgs.gov/science/USGSThesaurus/sonar%20methods">
    <rdf:type rdf:resource="http://www.w3.org/2004/02/skos/core#Concept"/>
    <skos:prefLabel xml:lang="en">sonar methods</skos:prefLabel>
    <skos:scopeNote xml:lang="en">SOund Navigation And Ranging techniques to detect submerged objects and to determine depths to the sea floor using reflections of sound waves.</skos:scopeNote>
    <skos:broader rdf:resource="http://www.usgs.gov/science/USGSThesaurus/acoustic%20methods"/>
    <skos:narrower rdf:resource="http://www.usgs.gov/science/USGSThesaurus/interferometric%20sonar"/>
    <skos:narrower rdf:resource="http://www.usgs.gov/science/USGSThesaurus/multibeam%20sonar"/>
    <skos:narrower rdf:resource="http://www.usgs.gov/science/USGSThesaurus/sidescan%20sonar"/>
    <skos:narrower rdf:resource="http://www.usgs.gov/science/USGSThesaurus/single-beam%20echo%20sounder"/>
    <skos:inScheme rdf:resource="http://www.usgs.gov/science/USGSThesaurus"/>
  </rdf:Description>
  <rdf:Description about="http://www.usgs.gov/science/USGSThesaurus/interferometric%20sonar">
    <rdf:type rdf:resource="http://www.w3.org/2004/02/skos/core#Concept"/>
    <skos:prefLabel xml:lang="en">interferometric sonar</skos:prefLabel>
    <skos:scopeNote xml:lang="en">Acoustic technique for determining depths or creating backscatter imagery in a wide swath of seafloor centered below the instrument platform.</skos:scopeNote>
    <skos:broader rdf:resource="http://www.usgs.gov/science/USGSThesaurus/sonar%20methods"/>
    <skos:related rdf:resource="http://www.usgs.gov/science/USGSThesaurus/sea-floor%20characteristics"/>
    <skos:related rdf:resource="http://www.usgs.gov/science/USGSThesaurus/bathymetry"/>
    <skos:related rdf:resource="http://www.usgs.gov/science/USGSThesaurus/sound%20velocity"/>
    <skos:related rdf:resource="http://www.usgs.gov/science/USGSThesaurus/sea-floor%20acoustic%20reflectivity"/>
    <skos:inScheme rdf:resource="http://www.usgs.gov/science/USGSThesaurus"/>
  </rdf:Description>
  <rdf:Description about="http://www.usgs.gov/science/USGSThesaurus/multibeam%20sonar">
    <rdf:type rdf:resource="http://www.w3.org/2004/02/skos/core#Concept"/>
    <skos:prefLabel xml:lang="en">multibeam sonar</skos:prefLabel>
    <skos:scopeNote xml:lang="en">Acoustic technique for determining depths or creating backscatter imagery in a wide swath of seafloor centered below the instrument platform.</skos:scopeNote>
    <skos:altLabel xml:lang="en">multibeam echo sounder</skos:altLabel>
    <skos:altLabel xml:lang="en">multibeam echosounder</skos:altLabel>
    <skos:altLabel xml:lang="en">multi-beam sonar</skos:altLabel>
    <skos:altLabel xml:lang="en">multi-beam echosounder</skos:altLabel>
    <skos:altLabel xml:lang="en">multi-beam echo sounder</skos:altLabel>
    <skos:broader rdf:resource="http://www.usgs.gov/science/USGSThesaurus/sonar%20methods"/>
    <skos:related rdf:resource="http://www.usgs.gov/science/USGSThesaurus/sea-floor%20characteristics"/>
    <skos:related rdf:resource="http://www.usgs.gov/science/USGSThesaurus/bathymetry"/>
    <skos:inScheme rdf:resource="http://www.usgs.gov/science/USGSThesaurus"/>
  </rdf:Description>
  <rdf:Description about="http://www.usgs.gov/science/USGSThesaurus/sidescan%20sonar">
    <rdf:type rdf:resource="http://www.w3.org/2004/02/skos/core#Concept"/>
    <skos:prefLabel xml:lang="en">sidescan sonar</skos:prefLabel>
    <skos:scopeNote xml:lang="en">Acoustic technique for creating oblique backscatter imagery of the seafloor.</skos:scopeNote>
    <skos:altLabel xml:lang="en">side-scan sonar</skos:altLabel>
    <!--FOR sidescan sonar mosaics USE sidescan sonar WITH image mosaics-->
    <skos:altLabel xml:lang="en">sidescan sonar mosaics</skos:altLabel>
    <skos:altLabel xml:lang="en">geological long-range inclined asdic</skos:altLabel>
    <skos:altLabel xml:lang="en">gloria</skos:altLabel>
    <skos:broader rdf:resource="http://www.usgs.gov/science/USGSThesaurus/sonar%20methods"/>
    <skos:related rdf:resource="http://www.usgs.gov/science/USGSThesaurus/sea-floor%20characteristics"/>
    <skos:related rdf:resource="http://www.usgs.gov/science/USGSThesaurus/sea-floor%20acoustic%20reflectivity"/>
    <skos:inScheme rdf:resource="http://www.usgs.gov/science/USGSThesaurus"/>
  </rdf:Description>
  <rdf:Description about="http://www.usgs.gov/science/USGSThesaurus/single-beam%20echo%20sounder">
    <rdf:type rdf:resource="http://www.w3.org/2004/02/skos/core#Concept"/>
    <skos:prefLabel xml:lang="en">single-beam echo sounder</skos:prefLabel>
    <skos:scopeNote xml:lang="en">Acoustic technique for determining seafloor depth directly below the instrument platform.</skos:scopeNote>
    <skos:altLabel xml:lang="en">fathometer</skos:altLabel>
    <skos:altLabel xml:lang="en">single-beam echosounder</skos:altLabel>
    <skos:altLabel xml:lang="en">single beam echo sounder</skos:altLabel>
    <skos:altLabel xml:lang="en">single beam echosounder</skos:altLabel>
    <skos:broader rdf:resource="http://www.usgs.gov/science/USGSThesaurus/sonar%20methods"/>
    <skos:related rdf:resource="http://www.usgs.gov/science/USGSThesaurus/bathymetry"/>
    <skos:inScheme rdf:resource="http://www.usgs.gov/science/USGSThesaurus"/>
  </rdf:Description>
  <rdf:Description about="http://www.usgs.gov/science/USGSThesaurus/animal%20and%20plant%20census">
    <rdf:type rdf:resource="http://www.w3.org/2004/02/skos/core#Concept"/>
    <skos:prefLabel xml:lang="en">animal and plant census</skos:prefLabel>
    <skos:scopeNote xml:lang="en">Inventory of macroscopic animals and plants by observation in the field. Used to estimate population and distribution.</skos:scopeNote>
    <skos:altLabel xml:lang="en">census</skos:altLabel>
    <skos:broader rdf:resource="http://www.usgs.gov/science/USGSThesaurus/field%20inventory%20and%20monitoring"/>
    <skos:inScheme rdf:resource="http://www.usgs.gov/science/USGSThesaurus"/>
  </rdf:Description>
  <rdf:Description about="http://www.usgs.gov/science/USGSThesaurus/borehole%20logging">
    <rdf:type rdf:resource="http://www.w3.org/2004/02/skos/core#Concept"/>
    <skos:prefLabel xml:lang="en">borehole logging</skos:prefLabel>
    <skos:scopeNote xml:lang="en">Method of recording the physical characteristics of the subsurface as a function of depth by observations during drilling of a well or borehole, studying the resulting core, or by lowering instruments into a drilled hole.</skos:scopeNote>
    <skos:altLabel xml:lang="en">well logging</skos:altLabel>
    <skos:broader rdf:resource="http://www.usgs.gov/science/USGSThesaurus/field%20inventory%20and%20monitoring"/>
    <skos:narrower rdf:resource="http://www.usgs.gov/science/USGSThesaurus/borehole%20temperature%20logging"/>
    <skos:narrower rdf:resource="http://www.usgs.gov/science/USGSThesaurus/electrical%20resistivity%20logging"/>
    <skos:narrower rdf:resource="http://www.usgs.gov/science/USGSThesaurus/gamma-ray%20logging"/>
    <skos:related rdf:resource="http://www.usgs.gov/science/USGSThesaurus/geophysics"/>
    <skos:related rdf:resource="http://www.usgs.gov/science/USGSThesaurus/stratigraphy"/>
    <skos:related rdf:resource="http://www.usgs.gov/science/USGSThesaurus/profiles"/>
    <skos:inScheme rdf:resource="http://www.usgs.gov/science/USGSThesaurus"/>
  </rdf:Description>
  <rdf:Description about="http://www.usgs.gov/science/USGSThesaurus/borehole%20temperature%20logging">
    <rdf:type rdf:resource="http://www.w3.org/2004/02/skos/core#Concept"/>
    <skos:prefLabel xml:lang="en">borehole temperature logging</skos:prefLabel>
    <skos:scopeNote xml:lang="en">Method of recording the measured temperature of the subsurface as a function of depth by lowering instruments into the hole.</skos:scopeNote>
    <skos:broader rdf:resource="http://www.usgs.gov/science/USGSThesaurus/borehole%20logging"/>
    <skos:related rdf:resource="http://www.usgs.gov/science/USGSThesaurus/geophysics"/>
    <skos:inScheme rdf:resource="http://www.usgs.gov/science/USGSThesaurus"/>
  </rdf:Description>
  <rdf:Description about="http://www.usgs.gov/science/USGSThesaurus/electrical%20resistivity%20logging">
    <rdf:type rdf:resource="http://www.w3.org/2004/02/skos/core#Concept"/>
    <skos:prefLabel xml:lang="en">electrical resistivity logging</skos:prefLabel>
    <skos:scopeNote xml:lang="en">Recordings made to identify the composition of subterranean materials at different depths in a borehole by measuring their ability to resist the flow of an electric current.</skos:scopeNote>
    <skos:altLabel xml:lang="en">resistivity sounding</skos:altLabel>
    <skos:broader rdf:resource="http://www.usgs.gov/science/USGSThesaurus/borehole%20logging"/>
    <skos:related rdf:resource="http://www.usgs.gov/science/USGSThesaurus/electromagnetic%20surveying"/>
    <skos:related rdf:resource="http://www.usgs.gov/science/USGSThesaurus/stratigraphy"/>
    <skos:inScheme rdf:resource="http://www.usgs.gov/science/USGSThesaurus"/>
  </rdf:Description>
  <rdf:Description about="http://www.usgs.gov/science/USGSThesaurus/gamma-ray%20logging">
    <rdf:type rdf:resource="http://www.w3.org/2004/02/skos/core#Concept"/>
    <skos:prefLabel xml:lang="en">gamma-ray logging</skos:prefLabel>
    <skos:scopeNote xml:lang="en">Recording of the measurements of natural gamma radiation emitted from the rocks in a borehole to study the subsurface structures.</skos:scopeNote>
    <skos:broader rdf:resource="http://www.usgs.gov/science/USGSThesaurus/borehole%20logging"/>
    <skos:related rdf:resource="http://www.usgs.gov/science/USGSThesaurus/stratigraphy"/>
    <skos:inScheme rdf:resource="http://www.usgs.gov/science/USGSThesaurus"/>
  </rdf:Description>
  <rdf:Description about="http://www.usgs.gov/science/USGSThesaurus/ecosystem%20monitoring">
    <rdf:type rdf:resource="http://www.w3.org/2004/02/skos/core#Concept"/>
    <skos:prefLabel xml:lang="en">ecosystem monitoring</skos:prefLabel>
    <skos:scopeNote xml:lang="en">Recording, evaluating, and actively intervening over time in the interaction of living and nonliving elements in a specific environment.</skos:scopeNote>
    <skos:altLabel xml:lang="en">indicator species observation</skos:altLabel>
    <!--FOR dendroecology USE ecosystem monitoring WITH vegetation-->
    <skos:altLabel xml:lang="en">dendroecology</skos:altLabel>
    <skos:broader rdf:resource="http://www.usgs.gov/science/USGSThesaurus/field%20inventory%20and%20monitoring"/>
    <skos:narrower rdf:resource="http://www.usgs.gov/science/USGSThesaurus/long-term%20ecological%20monitoring"/>
    <skos:related rdf:resource="http://www.usgs.gov/science/USGSThesaurus/biogeography"/>
    <skos:related rdf:resource="http://www.usgs.gov/science/USGSThesaurus/biological%20population%20management"/>
    <skos:related rdf:resource="http://www.usgs.gov/science/USGSThesaurus/bioremediation"/>
    <skos:related rdf:resource="http://www.usgs.gov/science/USGSThesaurus/ecology"/>
    <skos:related rdf:resource="http://www.usgs.gov/science/USGSThesaurus/ecosystem%20management"/>
    <skos:related rdf:resource="http://www.usgs.gov/science/USGSThesaurus/natural%20resource%20management"/>
    <skos:related rdf:resource="http://www.usgs.gov/science/USGSThesaurus/population%20and%20community%20ecology"/>
    <skos:related rdf:resource="http://www.usgs.gov/science/USGSThesaurus/relative%20abundance%20analysis"/>
    <skos:related rdf:resource="http://www.usgs.gov/science/USGSThesaurus/remediation"/>
    <skos:inScheme rdf:resource="http://www.usgs.gov/science/USGSThesaurus"/>
  </rdf:Description>
  <rdf:Description about="http://www.usgs.gov/science/USGSThesaurus/long-term%20ecological%20monitoring">
    <rdf:type rdf:resource="http://www.w3.org/2004/02/skos/core#Concept"/>
    <skos:prefLabel xml:lang="en">long-term ecological monitoring</skos:prefLabel>
    <skos:scopeNote xml:lang="en">Data collection over a period of years or decades to assess changes in selected biological communities and habitats.</skos:scopeNote>
    <skos:broader rdf:resource="http://www.usgs.gov/science/USGSThesaurus/ecosystem%20monitoring"/>
    <skos:related rdf:resource="http://www.usgs.gov/science/USGSThesaurus/ecology"/>
    <skos:inScheme rdf:resource="http://www.usgs.gov/science/USGSThesaurus"/>
  </rdf:Description>
  <rdf:Description about="http://www.usgs.gov/science/USGSThesaurus/electromagnetic%20surveying">
    <rdf:type rdf:resource="http://www.w3.org/2004/02/skos/core#Concept"/>
    <skos:prefLabel xml:lang="en">electromagnetic surveying</skos:prefLabel>
    <skos:scopeNote xml:lang="en">Method of determining the shape and constituency of near-surface earth structures by variations of responses of the materials to electrical and magnetic fields. Use for ground-based methods of imaging.</skos:scopeNote>
    <!--FOR magnetic surveying USE electromagnetic surveying WITH aeromagnetic surveying-->
    <skos:altLabel xml:lang="en">magnetic surveying</skos:altLabel>
    <skos:altLabel xml:lang="en">magnetotelluric sounding</skos:altLabel>
    <skos:broader rdf:resource="http://www.usgs.gov/science/USGSThesaurus/field%20inventory%20and%20monitoring"/>
    <skos:related rdf:resource="http://www.usgs.gov/science/USGSThesaurus/aeromagnetic%20surveying"/>
    <skos:related rdf:resource="http://www.usgs.gov/science/USGSThesaurus/electrical%20resistivity%20logging"/>
    <skos:inScheme rdf:resource="http://www.usgs.gov/science/USGSThesaurus"/>
  </rdf:Description>
  <rdf:Description about="http://www.usgs.gov/science/USGSThesaurus/gravimeter%20measurement">
    <rdf:type rdf:resource="http://www.w3.org/2004/02/skos/core#Concept"/>
    <skos:prefLabel xml:lang="en">gravimeter measurement</skos:prefLabel>
    <skos:scopeNote xml:lang="en">Use of a specialized instrument for measuring the earth's gravity at a given location.</skos:scopeNote>
    <skos:altLabel xml:lang="en">gravimetric methods</skos:altLabel>
    <skos:altLabel xml:lang="en">gravimetry</skos:altLabel>
    <skos:broader rdf:resource="http://www.usgs.gov/science/USGSThesaurus/field%20inventory%20and%20monitoring"/>
    <skos:inScheme rdf:resource="http://www.usgs.gov/science/USGSThesaurus"/>
  </rdf:Description>
  <rdf:Description about="http://www.usgs.gov/science/USGSThesaurus/handheld%20field%20spectroscopy">
    <rdf:type rdf:resource="http://www.w3.org/2004/02/skos/core#Concept"/>
    <skos:prefLabel xml:lang="en">handheld field spectroscopy</skos:prefLabel>
    <skos:scopeNote xml:lang="en">Use of portable equipment to measure spectral reflectance of materials in the field.</skos:scopeNote>
    <skos:altLabel xml:lang="en">hand-held field spectroscopy</skos:altLabel>
    <skos:broader rdf:resource="http://www.usgs.gov/science/USGSThesaurus/field%20inventory%20and%20monitoring"/>
    <skos:inScheme rdf:resource="http://www.usgs.gov/science/USGSThesaurus"/>
  </rdf:Description>
  <rdf:Description about="http://www.usgs.gov/science/USGSThesaurus/magnetometer%20measurement">
    <rdf:type rdf:resource="http://www.w3.org/2004/02/skos/core#Concept"/>
    <skos:prefLabel xml:lang="en">magnetometer measurement</skos:prefLabel>
    <skos:scopeNote xml:lang="en">Use of specialized instruments designed to measure the earth's magnetic field at a given location.</skos:scopeNote>
    <skos:altLabel xml:lang="en">magnetometry</skos:altLabel>
    <skos:broader rdf:resource="http://www.usgs.gov/science/USGSThesaurus/field%20inventory%20and%20monitoring"/>
    <skos:inScheme rdf:resource="http://www.usgs.gov/science/USGSThesaurus"/>
  </rdf:Description>
  <rdf:Description about="http://www.usgs.gov/science/USGSThesaurus/optical%20methods">
    <rdf:type rdf:resource="http://www.w3.org/2004/02/skos/core#Concept"/>
    <skos:prefLabel xml:lang="en">optical methods</skos:prefLabel>
    <skos:scopeNote xml:lang="en">Measurement of light transmission or reflectance in the field to estimate, for example, the density of suspended sediment in water bodies.</skos:scopeNote>
    <skos:altLabel xml:lang="en">optical backscatterance sensing</skos:altLabel>
    <skos:altLabel xml:lang="en">optical reflectance measurement</skos:altLabel>
    <skos:broader rdf:resource="http://www.usgs.gov/science/USGSThesaurus/field%20inventory%20and%20monitoring"/>
    <skos:inScheme rdf:resource="http://www.usgs.gov/science/USGSThesaurus"/>
  </rdf:Description>
  <rdf:Description about="http://www.usgs.gov/science/USGSThesaurus/seismic%20methods">
    <rdf:type rdf:resource="http://www.w3.org/2004/02/skos/core#Concept"/>
    <skos:prefLabel xml:lang="en">seismic methods</skos:prefLabel>
    <skos:scopeNote xml:lang="en">Procedures used to record and study earthquakes or earth vibrations including those that are artificially induced.</skos:scopeNote>
    <!--FOR seismic exploration USE seismic methods WITH natural resource exploration-->
    <skos:altLabel xml:lang="en">seismic exploration</skos:altLabel>
    <skos:altLabel xml:lang="en">seismic imaging</skos:altLabel>
    <skos:altLabel xml:lang="en">seismic profiles</skos:altLabel>
    <skos:altLabel xml:lang="en">seismograms</skos:altLabel>
    <skos:altLabel xml:lang="en">seismometry</skos:altLabel>
    <skos:broader rdf:resource="http://www.usgs.gov/science/USGSThesaurus/field%20inventory%20and%20monitoring"/>
    <skos:narrower rdf:resource="http://www.usgs.gov/science/USGSThesaurus/seismic%20networking"/>
    <skos:narrower rdf:resource="http://www.usgs.gov/science/USGSThesaurus/seismic%20reflection%20methods"/>
    <skos:narrower rdf:resource="http://www.usgs.gov/science/USGSThesaurus/seismic%20refraction%20methods"/>
    <skos:related rdf:resource="http://www.usgs.gov/science/USGSThesaurus/remote%20sensing"/>
    <skos:related rdf:resource="http://www.usgs.gov/science/USGSThesaurus/seismology"/>
    <skos:inScheme rdf:resource="http://www.usgs.gov/science/USGSThesaurus"/>
  </rdf:Description>
  <rdf:Description about="http://www.usgs.gov/science/USGSThesaurus/seismic%20networking">
    <rdf:type rdf:resource="http://www.w3.org/2004/02/skos/core#Concept"/>
    <skos:prefLabel xml:lang="en">seismic networking</skos:prefLabel>
    <skos:scopeNote xml:lang="en">Deploying, operating, and maintaining groups and arrays of instruments for detecting and describing local movements of the earth.</skos:scopeNote>
    <skos:altLabel xml:lang="en">earthquake monitoring</skos:altLabel>
    <skos:broader rdf:resource="http://www.usgs.gov/science/USGSThesaurus/seismic%20methods"/>
    <skos:related rdf:resource="http://www.usgs.gov/science/USGSThesaurus/seismology"/>
    <skos:inScheme rdf:resource="http://www.usgs.gov/science/USGSThesaurus"/>
  </rdf:Description>
  <rdf:Description about="http://www.usgs.gov/science/USGSThesaurus/seismic%20reflection%20methods">
    <rdf:type rdf:resource="http://www.w3.org/2004/02/skos/core#Concept"/>
    <skos:prefLabel xml:lang="en">seismic reflection methods</skos:prefLabel>
    <skos:scopeNote xml:lang="en">Geophysical technique to study the subsurface of the earth using sound waves induced by explosives, vibrating devices, or percussive equipment.  The reflections of the sound waves from the boundaries of different rocks are measured.</skos:scopeNote>
    <!--FOR seismic reflection survey maps USE seismic reflection methods WITH maps and atlases-->
    <skos:altLabel xml:lang="en">seismic reflection survey maps</skos:altLabel>
    <skos:broader rdf:resource="http://www.usgs.gov/science/USGSThesaurus/seismic%20methods"/>
    <skos:narrower rdf:resource="http://www.usgs.gov/science/USGSThesaurus/sub-bottom%20profiling"/>
    <skos:related rdf:resource="http://www.usgs.gov/science/USGSThesaurus/seismology"/>
    <skos:inScheme rdf:resource="http://www.usgs.gov/science/USGSThesaurus"/>
  </rdf:Description>
  <rdf:Description about="http://www.usgs.gov/science/USGSThesaurus/sub-bottom%20profiling">
    <rdf:type rdf:resource="http://www.w3.org/2004/02/skos/core#Concept"/>
    <skos:prefLabel xml:lang="en">sub-bottom profiling</skos:prefLabel>
    <skos:scopeNote xml:lang="en">Methods of imaging the structure of sediments below the sea floor using ship-borne or towed sensors with a variety of sound sources.</skos:scopeNote>
    <skos:altLabel xml:lang="en">chirp profiling</skos:altLabel>
    <skos:altLabel xml:lang="en">boomer profiling</skos:altLabel>
    <skos:altLabel xml:lang="en">sparker profiling</skos:altLabel>
    <skos:broader rdf:resource="http://www.usgs.gov/science/USGSThesaurus/seismic%20reflection%20methods"/>
    <skos:related rdf:resource="http://www.usgs.gov/science/USGSThesaurus/seismic%20refraction%20methods"/>
    <skos:related rdf:resource="http://www.usgs.gov/science/USGSThesaurus/profiles"/>
    <skos:inScheme rdf:resource="http://www.usgs.gov/science/USGSThesaurus"/>
  </rdf:Description>
  <rdf:Description about="http://www.usgs.gov/science/USGSThesaurus/seismic%20refraction%20methods">
    <rdf:type rdf:resource="http://www.w3.org/2004/02/skos/core#Concept"/>
    <skos:prefLabel xml:lang="en">seismic refraction methods</skos:prefLabel>
    <skos:scopeNote xml:lang="en">Geophysical technique to study the subsurface of the earth by generating compressional waves by means of hammering or explosive methods. The variations in velocity of the waves traveling through rocks or geological layers are measured.</skos:scopeNote>
    <skos:broader rdf:resource="http://www.usgs.gov/science/USGSThesaurus/seismic%20methods"/>
    <skos:related rdf:resource="http://www.usgs.gov/science/USGSThesaurus/seismology"/>
    <skos:related rdf:resource="http://www.usgs.gov/science/USGSThesaurus/sub-bottom%20profiling"/>
    <skos:inScheme rdf:resource="http://www.usgs.gov/science/USGSThesaurus"/>
  </rdf:Description>
  <rdf:Description about="http://www.usgs.gov/science/USGSThesaurus/statistical%20surveying">
    <rdf:type rdf:resource="http://www.w3.org/2004/02/skos/core#Concept"/>
    <skos:prefLabel xml:lang="en">statistical surveying</skos:prefLabel>
    <skos:scopeNote xml:lang="en">Information gathering by asking questions of selected people or organizations.</skos:scopeNote>
    <skos:altLabel xml:lang="en">canvassing</skos:altLabel>
    <skos:broader rdf:resource="http://www.usgs.gov/science/USGSThesaurus/field%20inventory%20and%20monitoring"/>
    <skos:inScheme rdf:resource="http://www.usgs.gov/science/USGSThesaurus"/>
  </rdf:Description>
  <rdf:Description about="http://www.usgs.gov/science/USGSThesaurus/stream-gage%20measurement">
    <rdf:type rdf:resource="http://www.w3.org/2004/02/skos/core#Concept"/>
    <skos:prefLabel xml:lang="en">stream-gage measurement</skos:prefLabel>
    <skos:scopeNote xml:lang="en">Use of specialized instruments designed for observing, checking, and recording the water discharge that occurs in a natural channel.</skos:scopeNote>
    <skos:altLabel xml:lang="en">gage-height monitoring</skos:altLabel>
    <skos:altLabel xml:lang="en">stream current monitoring</skos:altLabel>
    <skos:altLabel xml:lang="en">stream flow monitoring</skos:altLabel>
    <skos:altLabel xml:lang="en">stream gage monitoring</skos:altLabel>
    <skos:altLabel xml:lang="en">stream-flow monitoring</skos:altLabel>
    <skos:altLabel xml:lang="en">stream-gage monitoring</skos:altLabel>
    <skos:altLabel xml:lang="en">streamflow monitoring</skos:altLabel>
    <skos:broader rdf:resource="http://www.usgs.gov/science/USGSThesaurus/field%20inventory%20and%20monitoring"/>
    <skos:related rdf:resource="http://www.usgs.gov/science/USGSThesaurus/hydrology"/>
    <skos:related rdf:resource="http://www.usgs.gov/science/USGSThesaurus/streamflow"/>
    <skos:related rdf:resource="http://www.usgs.gov/science/USGSThesaurus/acoustic%20doppler%20current%20profiling"/>
    <skos:inScheme rdf:resource="http://www.usgs.gov/science/USGSThesaurus"/>
  </rdf:Description>
  <rdf:Description about="http://www.usgs.gov/science/USGSThesaurus/telemetry">
    <rdf:type rdf:resource="http://www.w3.org/2004/02/skos/core#Concept"/>
    <skos:prefLabel xml:lang="en">telemetry</skos:prefLabel>
    <skos:scopeNote xml:lang="en">Field technique using instruments which measure heat, radiation, speed, or other property and transmit the data to a distant receiver.</skos:scopeNote>
    <skos:altLabel xml:lang="en">biotelemetry</skos:altLabel>
    <skos:altLabel xml:lang="en">radio telemetry</skos:altLabel>
    <skos:broader rdf:resource="http://www.usgs.gov/science/USGSThesaurus/field%20inventory%20and%20monitoring"/>
    <skos:related rdf:resource="http://www.usgs.gov/science/USGSThesaurus/animal%20tracking"/>
    <skos:related rdf:resource="http://www.usgs.gov/science/USGSThesaurus/remote%20sensing"/>
    <skos:inScheme rdf:resource="http://www.usgs.gov/science/USGSThesaurus"/>
  </rdf:Description>
  <rdf:Description about="http://www.usgs.gov/science/USGSThesaurus/tiltmeter%20measurement">
    <rdf:type rdf:resource="http://www.w3.org/2004/02/skos/core#Concept"/>
    <skos:prefLabel xml:lang="en">tiltmeter measurement</skos:prefLabel>
    <skos:scopeNote xml:lang="en">Determination of tiny changes in the slope angle or tilt of the ground in order to monitor deformation caused by moving magma. Instruments detect variations in a liquid level or in the position of a pendulum.</skos:scopeNote>
    <skos:altLabel xml:lang="en">tiltmeter</skos:altLabel>
    <skos:broader rdf:resource="http://www.usgs.gov/science/USGSThesaurus/field%20inventory%20and%20monitoring"/>
    <skos:related rdf:resource="http://www.usgs.gov/science/USGSThesaurus/seismology"/>
    <skos:related rdf:resource="http://www.usgs.gov/science/USGSThesaurus/volcanology"/>
    <skos:inScheme rdf:resource="http://www.usgs.gov/science/USGSThesaurus"/>
  </rdf:Description>
  <rdf:Description about="http://www.usgs.gov/science/USGSThesaurus/tomography">
    <rdf:type rdf:resource="http://www.w3.org/2004/02/skos/core#Concept"/>
    <skos:prefLabel xml:lang="en">tomography</skos:prefLabel>
    <skos:scopeNote xml:lang="en">Observation of the internal structure of an object or, as is more typical in USGS research, a cross section of the earth's crust by changing the relative orientation of a signal generator, a sensor, or both.</skos:scopeNote>
    <skos:altLabel xml:lang="en">seismic tomography</skos:altLabel>
    <skos:altLabel xml:lang="en">radar tomography</skos:altLabel>
    <skos:broader rdf:resource="http://www.usgs.gov/science/USGSThesaurus/field%20inventory%20and%20monitoring"/>
    <skos:inScheme rdf:resource="http://www.usgs.gov/science/USGSThesaurus"/>
  </rdf:Description>
  <rdf:Description about="http://www.usgs.gov/science/USGSThesaurus/video%20monitoring">
    <rdf:type rdf:resource="http://www.w3.org/2004/02/skos/core#Concept"/>
    <skos:prefLabel xml:lang="en">video monitoring</skos:prefLabel>
    <skos:scopeNote xml:lang="en">Field study employing the use of filming or repeated photography with stationary optical or digital cameras to observe changes in a feature or organism.</skos:scopeNote>
    <skos:altLabel xml:lang="en">remote video monitoring</skos:altLabel>
    <skos:broader rdf:resource="http://www.usgs.gov/science/USGSThesaurus/field%20inventory%20and%20monitoring"/>
    <skos:related rdf:resource="http://www.usgs.gov/science/USGSThesaurus/videography"/>
    <skos:inScheme rdf:resource="http://www.usgs.gov/science/USGSThesaurus"/>
  </rdf:Description>
  <rdf:Description about="http://www.usgs.gov/science/USGSThesaurus/vocalization%20methods">
    <rdf:type rdf:resource="http://www.w3.org/2004/02/skos/core#Concept"/>
    <skos:prefLabel xml:lang="en">vocalization methods</skos:prefLabel>
    <skos:scopeNote xml:lang="en">Series of methods used to (a) record sonograms (sound spectrogram) of animal sounds which are analyzed to identify the presence of species in an area and to determine distinct sound patterns within a species, e.g., mating calls, danger alerts; (b) attract species to an area for inventory or monitoring by playing recorded animal sounds or mimicking them.</skos:scopeNote>
    <skos:broader rdf:resource="http://www.usgs.gov/science/USGSThesaurus/field%20inventory%20and%20monitoring"/>
    <skos:related rdf:resource="http://www.usgs.gov/science/USGSThesaurus/wildlife%20biology"/>
    <skos:inScheme rdf:resource="http://www.usgs.gov/science/USGSThesaurus"/>
  </rdf:Description>
  <rdf:Description about="http://www.usgs.gov/science/USGSThesaurus/field%20sampling">
    <rdf:type rdf:resource="http://www.w3.org/2004/02/skos/core#Concept"/>
    <skos:prefLabel xml:lang="en">field sampling</skos:prefLabel>
    <skos:scopeNote xml:lang="en">Collecting pieces or specimens or making measurements or observations at determined intervals or areas.  Results may be used as representative of the whole research area or population.</skos:scopeNote>
    <!--FOR fish inventories USE field sampling WITH fish-->
    <skos:altLabel xml:lang="en">fish inventories</skos:altLabel>
    <skos:broader rdf:resource="http://www.usgs.gov/science/USGSThesaurus/field%20methods"/>
    <skos:narrower rdf:resource="http://www.usgs.gov/science/USGSThesaurus/animal%20tracking"/>
    <skos:narrower rdf:resource="http://www.usgs.gov/science/USGSThesaurus/capturing%20%28animals%29"/>
    <skos:narrower rdf:resource="http://www.usgs.gov/science/USGSThesaurus/dredge%20sampling"/>
    <skos:narrower rdf:resource="http://www.usgs.gov/science/USGSThesaurus/drilling%20and%20coring"/>
    <skos:narrower rdf:resource="http://www.usgs.gov/science/USGSThesaurus/grab%20sampling"/>
    <skos:narrower rdf:resource="http://www.usgs.gov/science/USGSThesaurus/plant%20and%20animal%20tagging"/>
    <skos:narrower rdf:resource="http://www.usgs.gov/science/USGSThesaurus/plot%20sampling"/>
    <skos:narrower rdf:resource="http://www.usgs.gov/science/USGSThesaurus/sexing%20%28plants%20%26%20animals%29"/>
    <skos:narrower rdf:resource="http://www.usgs.gov/science/USGSThesaurus/specimen%20collecting"/>
    <skos:narrower rdf:resource="http://www.usgs.gov/science/USGSThesaurus/transect%20sampling"/>
    <skos:narrower rdf:resource="http://www.usgs.gov/science/USGSThesaurus/trenching"/>
    <skos:narrower rdf:resource="http://www.usgs.gov/science/USGSThesaurus/water%20sampling"/>
    <skos:inScheme rdf:resource="http://www.usgs.gov/science/USGSThesaurus"/>
  </rdf:Description>
  <rdf:Description about="http://www.usgs.gov/science/USGSThesaurus/animal%20tracking">
    <rdf:type rdf:resource="http://www.w3.org/2004/02/skos/core#Concept"/>
    <skos:prefLabel xml:lang="en">animal tracking</skos:prefLabel>
    <skos:scopeNote xml:lang="en">Method of studying animals by following spoor (footprints, droppings, scent, and other evidence) in an area to document the presence and movements of the animal and its interactions within the landscape.</skos:scopeNote>
    <skos:altLabel xml:lang="en">tracking</skos:altLabel>
    <skos:broader rdf:resource="http://www.usgs.gov/science/USGSThesaurus/field%20sampling"/>
    <skos:related rdf:resource="http://www.usgs.gov/science/USGSThesaurus/telemetry"/>
    <skos:related rdf:resource="http://www.usgs.gov/science/USGSThesaurus/wildlife%20biology"/>
    <skos:inScheme rdf:resource="http://www.usgs.gov/science/USGSThesaurus"/>
  </rdf:Description>
  <rdf:Description about="http://www.usgs.gov/science/USGSThesaurus/capturing%20%28animals%29">
    <rdf:type rdf:resource="http://www.w3.org/2004/02/skos/core#Concept"/>
    <skos:prefLabel xml:lang="en">capturing (animals)</skos:prefLabel>
    <skos:scopeNote xml:lang="en">Collecting individual animals in the field by various methods in order to obtain information about the species or population and its ecology. Capturing methods are adapted to the habits and habitats of the target species and include both live trapping and kill trapping methods.</skos:scopeNote>
    <skos:altLabel xml:lang="en">trapping (animals)</skos:altLabel>
    <skos:broader rdf:resource="http://www.usgs.gov/science/USGSThesaurus/field%20sampling"/>
    <skos:related rdf:resource="http://www.usgs.gov/science/USGSThesaurus/specimen%20collecting"/>
    <skos:related rdf:resource="http://www.usgs.gov/science/USGSThesaurus/zoology"/>
    <skos:inScheme rdf:resource="http://www.usgs.gov/science/USGSThesaurus"/>
  </rdf:Description>
  <rdf:Description about="http://www.usgs.gov/science/USGSThesaurus/dredge%20sampling">
    <rdf:type rdf:resource="http://www.w3.org/2004/02/skos/core#Concept"/>
    <skos:prefLabel xml:lang="en">dredge sampling</skos:prefLabel>
    <skos:scopeNote xml:lang="en">Collection of material from the bottom of a body of water by dragging an open container along the floor of the water body and returning the collected material to the investigators.</skos:scopeNote>
    <skos:broader rdf:resource="http://www.usgs.gov/science/USGSThesaurus/field%20sampling"/>
    <skos:inScheme rdf:resource="http://www.usgs.gov/science/USGSThesaurus"/>
  </rdf:Description>
  <rdf:Description about="http://www.usgs.gov/science/USGSThesaurus/drilling%20and%20coring">
    <rdf:type rdf:resource="http://www.w3.org/2004/02/skos/core#Concept"/>
    <skos:prefLabel xml:lang="en">drilling and coring</skos:prefLabel>
    <skos:scopeNote xml:lang="en">Cutting into the subsurface, for example into underground strata, ice, or a tree trunk, to remove material for examination. Intended for broad use wherever coring is done. The combination of this term with other terms will convey the context of the activity.</skos:scopeNote>
    <skos:altLabel xml:lang="en">core sampling</skos:altLabel>
    <skos:altLabel xml:lang="en">coring</skos:altLabel>
    <!--FOR ice core sampling USE drilling and coring WITH snow and ice cover-->
    <skos:altLabel xml:lang="en">ice core sampling</skos:altLabel>
    <skos:broader rdf:resource="http://www.usgs.gov/science/USGSThesaurus/field%20sampling"/>
    <skos:narrower rdf:resource="http://www.usgs.gov/science/USGSThesaurus/augering"/>
    <skos:narrower rdf:resource="http://www.usgs.gov/science/USGSThesaurus/box%20coring"/>
    <skos:narrower rdf:resource="http://www.usgs.gov/science/USGSThesaurus/gravity%20coring"/>
    <skos:narrower rdf:resource="http://www.usgs.gov/science/USGSThesaurus/piston%20coring"/>
    <skos:narrower rdf:resource="http://www.usgs.gov/science/USGSThesaurus/push%20coring"/>
    <skos:narrower rdf:resource="http://www.usgs.gov/science/USGSThesaurus/rotary%20drilling"/>
    <skos:narrower rdf:resource="http://www.usgs.gov/science/USGSThesaurus/vibracoring"/>
    <skos:related rdf:resource="http://www.usgs.gov/science/USGSThesaurus/botany"/>
    <skos:related rdf:resource="http://www.usgs.gov/science/USGSThesaurus/core%20analysis"/>
    <skos:related rdf:resource="http://www.usgs.gov/science/USGSThesaurus/geology"/>
    <skos:related rdf:resource="http://www.usgs.gov/science/USGSThesaurus/glaciology"/>
    <skos:related rdf:resource="http://www.usgs.gov/science/USGSThesaurus/well%20drilling"/>
    <skos:inScheme rdf:resource="http://www.usgs.gov/science/USGSThesaurus"/>
  </rdf:Description>
  <rdf:Description about="http://www.usgs.gov/science/USGSThesaurus/augering">
    <rdf:type rdf:resource="http://www.w3.org/2004/02/skos/core#Concept"/>
    <skos:prefLabel xml:lang="en">augering</skos:prefLabel>
    <skos:scopeNote xml:lang="en">Use of a device with rotating blades and possibly helical flanges to dig holes in unconsolidated material for subsurface sampling.</skos:scopeNote>
    <skos:broader rdf:resource="http://www.usgs.gov/science/USGSThesaurus/drilling%20and%20coring"/>
    <skos:inScheme rdf:resource="http://www.usgs.gov/science/USGSThesaurus"/>
  </rdf:Description>
  <rdf:Description about="http://www.usgs.gov/science/USGSThesaurus/box%20coring">
    <rdf:type rdf:resource="http://www.w3.org/2004/02/skos/core#Concept"/>
    <skos:prefLabel xml:lang="en">box coring</skos:prefLabel>
    <skos:scopeNote xml:lang="en">Use of a rectangular box pushed into soft sediment with a spade to facilitate lifting the sampled material, to isolate and extract relatively undisturbed underwater sediment.</skos:scopeNote>
    <skos:broader rdf:resource="http://www.usgs.gov/science/USGSThesaurus/drilling%20and%20coring"/>
    <skos:inScheme rdf:resource="http://www.usgs.gov/science/USGSThesaurus"/>
  </rdf:Description>
  <rdf:Description about="http://www.usgs.gov/science/USGSThesaurus/gravity%20coring">
    <rdf:type rdf:resource="http://www.w3.org/2004/02/skos/core#Concept"/>
    <skos:prefLabel xml:lang="en">gravity coring</skos:prefLabel>
    <skos:scopeNote xml:lang="en">Use of a simple tube pushed into underwater sediments by an overhanging weight, to extract relatively undisturbed material for study.</skos:scopeNote>
    <skos:broader rdf:resource="http://www.usgs.gov/science/USGSThesaurus/drilling%20and%20coring"/>
    <skos:inScheme rdf:resource="http://www.usgs.gov/science/USGSThesaurus"/>
  </rdf:Description>
  <rdf:Description about="http://www.usgs.gov/science/USGSThesaurus/piston%20coring">
    <rdf:type rdf:resource="http://www.w3.org/2004/02/skos/core#Concept"/>
    <skos:prefLabel xml:lang="en">piston coring</skos:prefLabel>
    <skos:scopeNote xml:lang="en">Use of a piston mechanism and a weight with a triggering mechanism to drive a coring tube deep into underwater sediments for extraction and study.</skos:scopeNote>
    <skos:broader rdf:resource="http://www.usgs.gov/science/USGSThesaurus/drilling%20and%20coring"/>
    <skos:inScheme rdf:resource="http://www.usgs.gov/science/USGSThesaurus"/>
  </rdf:Description>
  <rdf:Description about="http://www.usgs.gov/science/USGSThesaurus/push%20coring">
    <rdf:type rdf:resource="http://www.w3.org/2004/02/skos/core#Concept"/>
    <skos:prefLabel xml:lang="en">push coring</skos:prefLabel>
    <skos:scopeNote xml:lang="en">Use of a small, hand-held tube pressed into unconsolidated material for sampling.</skos:scopeNote>
    <skos:broader rdf:resource="http://www.usgs.gov/science/USGSThesaurus/drilling%20and%20coring"/>
    <skos:inScheme rdf:resource="http://www.usgs.gov/science/USGSThesaurus"/>
  </rdf:Description>
  <rdf:Description about="http://www.usgs.gov/science/USGSThesaurus/rotary%20drilling">
    <rdf:type rdf:resource="http://www.w3.org/2004/02/skos/core#Concept"/>
    <skos:prefLabel xml:lang="en">rotary drilling</skos:prefLabel>
    <skos:scopeNote xml:lang="en">Use of machinery to drive a rotating bit through earth materials in order to sample below the surface.</skos:scopeNote>
    <skos:broader rdf:resource="http://www.usgs.gov/science/USGSThesaurus/drilling%20and%20coring"/>
    <skos:inScheme rdf:resource="http://www.usgs.gov/science/USGSThesaurus"/>
  </rdf:Description>
  <rdf:Description about="http://www.usgs.gov/science/USGSThesaurus/vibracoring">
    <rdf:type rdf:resource="http://www.w3.org/2004/02/skos/core#Concept"/>
    <skos:prefLabel xml:lang="en">vibracoring</skos:prefLabel>
    <skos:scopeNote xml:lang="en">Application of vibration to a coring device in order to achieve greater penetration for sampling unconsolidated material.</skos:scopeNote>
    <skos:broader rdf:resource="http://www.usgs.gov/science/USGSThesaurus/drilling%20and%20coring"/>
    <skos:inScheme rdf:resource="http://www.usgs.gov/science/USGSThesaurus"/>
  </rdf:Description>
  <rdf:Description about="http://www.usgs.gov/science/USGSThesaurus/grab%20sampling">
    <rdf:type rdf:resource="http://www.w3.org/2004/02/skos/core#Concept"/>
    <skos:prefLabel xml:lang="en">grab sampling</skos:prefLabel>
    <skos:scopeNote xml:lang="en">Use of a mechanical device to seize a volume of unconsolidated surficial material for study.  This term applies when the device used is specifically crafted for grab sampling.</skos:scopeNote>
    <skos:broader rdf:resource="http://www.usgs.gov/science/USGSThesaurus/field%20sampling"/>
    <skos:inScheme rdf:resource="http://www.usgs.gov/science/USGSThesaurus"/>
  </rdf:Description>
  <rdf:Description about="http://www.usgs.gov/science/USGSThesaurus/plant%20and%20animal%20tagging">
    <rdf:type rdf:resource="http://www.w3.org/2004/02/skos/core#Concept"/>
    <skos:prefLabel xml:lang="en">plant and animal tagging</skos:prefLabel>
    <skos:scopeNote xml:lang="en">Methods of attaching a tag or marker to an organism as long-term identification for study purposes.</skos:scopeNote>
    <skos:altLabel xml:lang="en">animal tagging</skos:altLabel>
    <skos:altLabel xml:lang="en">banding</skos:altLabel>
    <skos:altLabel xml:lang="en">bird banding</skos:altLabel>
    <skos:altLabel xml:lang="en">radioisotope tagging</skos:altLabel>
    <skos:altLabel xml:lang="en">tagging</skos:altLabel>
    <skos:broader rdf:resource="http://www.usgs.gov/science/USGSThesaurus/field%20sampling"/>
    <skos:related rdf:resource="http://www.usgs.gov/science/USGSThesaurus/life%20sciences"/>
    <skos:inScheme rdf:resource="http://www.usgs.gov/science/USGSThesaurus"/>
  </rdf:Description>
  <rdf:Description about="http://www.usgs.gov/science/USGSThesaurus/plot%20sampling">
    <rdf:type rdf:resource="http://www.w3.org/2004/02/skos/core#Concept"/>
    <skos:prefLabel xml:lang="en">plot sampling</skos:prefLabel>
    <skos:scopeNote xml:lang="en">Outlining small areas of land within a larger area to use as samples to study biological populations or ecosystems.</skos:scopeNote>
    <skos:broader rdf:resource="http://www.usgs.gov/science/USGSThesaurus/field%20sampling"/>
    <skos:related rdf:resource="http://www.usgs.gov/science/USGSThesaurus/ecology"/>
    <skos:related rdf:resource="http://www.usgs.gov/science/USGSThesaurus/transect%20sampling"/>
    <skos:related rdf:resource="http://www.usgs.gov/science/USGSThesaurus/trenching"/>
    <skos:inScheme rdf:resource="http://www.usgs.gov/science/USGSThesaurus"/>
  </rdf:Description>
  <rdf:Description about="http://www.usgs.gov/science/USGSThesaurus/sexing%20%28plants%20%26%20animals%29">
    <rdf:type rdf:resource="http://www.w3.org/2004/02/skos/core#Concept"/>
    <skos:prefLabel xml:lang="en">sexing (plants &amp; animals)</skos:prefLabel>
    <skos:scopeNote xml:lang="en">Determination of the sex of an individual organism for study purposes, such as wildlife surveys.</skos:scopeNote>
    <skos:altLabel xml:lang="en">sexing (plants and animals)</skos:altLabel>
    <skos:broader rdf:resource="http://www.usgs.gov/science/USGSThesaurus/field%20sampling"/>
    <skos:related rdf:resource="http://www.usgs.gov/science/USGSThesaurus/life%20sciences"/>
    <skos:inScheme rdf:resource="http://www.usgs.gov/science/USGSThesaurus"/>
  </rdf:Description>
  <rdf:Description about="http://www.usgs.gov/science/USGSThesaurus/specimen%20collecting">
    <rdf:type rdf:resource="http://www.w3.org/2004/02/skos/core#Concept"/>
    <skos:prefLabel xml:lang="en">specimen collecting</skos:prefLabel>
    <skos:scopeNote xml:lang="en">Taking of samples from the environment for study.</skos:scopeNote>
    <skos:altLabel xml:lang="en">collection of specimens</skos:altLabel>
    <skos:broader rdf:resource="http://www.usgs.gov/science/USGSThesaurus/field%20sampling"/>
    <skos:related rdf:resource="http://www.usgs.gov/science/USGSThesaurus/capturing%20%28animals%29"/>
    <skos:inScheme rdf:resource="http://www.usgs.gov/science/USGSThesaurus"/>
  </rdf:Description>
  <rdf:Description about="http://www.usgs.gov/science/USGSThesaurus/transect%20sampling">
    <rdf:type rdf:resource="http://www.w3.org/2004/02/skos/core#Concept"/>
    <skos:prefLabel xml:lang="en">transect sampling</skos:prefLabel>
    <skos:scopeNote xml:lang="en">Systematic method of collecting field data by recording observations or collecting specimens along a vector or measured course across the environment.</skos:scopeNote>
    <skos:broader rdf:resource="http://www.usgs.gov/science/USGSThesaurus/field%20sampling"/>
    <skos:related rdf:resource="http://www.usgs.gov/science/USGSThesaurus/plot%20sampling"/>
    <skos:related rdf:resource="http://www.usgs.gov/science/USGSThesaurus/trenching"/>
    <skos:inScheme rdf:resource="http://www.usgs.gov/science/USGSThesaurus"/>
  </rdf:Description>
  <rdf:Description about="http://www.usgs.gov/science/USGSThesaurus/trenching">
    <rdf:type rdf:resource="http://www.w3.org/2004/02/skos/core#Concept"/>
    <skos:prefLabel xml:lang="en">trenching</skos:prefLabel>
    <skos:scopeNote xml:lang="en">Field method used by earth scientists to study the underground structure of an area. A long narrow ditch is dug to locate geologic features, such as a fault.</skos:scopeNote>
    <skos:broader rdf:resource="http://www.usgs.gov/science/USGSThesaurus/field%20sampling"/>
    <skos:related rdf:resource="http://www.usgs.gov/science/USGSThesaurus/plot%20sampling"/>
    <skos:related rdf:resource="http://www.usgs.gov/science/USGSThesaurus/sedimentology"/>
    <skos:related rdf:resource="http://www.usgs.gov/science/USGSThesaurus/soil%20sciences"/>
    <skos:related rdf:resource="http://www.usgs.gov/science/USGSThesaurus/transect%20sampling"/>
    <skos:inScheme rdf:resource="http://www.usgs.gov/science/USGSThesaurus"/>
  </rdf:Description>
  <rdf:Description about="http://www.usgs.gov/science/USGSThesaurus/water%20sampling">
    <rdf:type rdf:resource="http://www.w3.org/2004/02/skos/core#Concept"/>
    <skos:prefLabel xml:lang="en">water sampling</skos:prefLabel>
    <skos:scopeNote xml:lang="en">Methods of collecting a representative part of a body of water for testing in controlled conditions.</skos:scopeNote>
    <skos:broader rdf:resource="http://www.usgs.gov/science/USGSThesaurus/field%20sampling"/>
    <skos:related rdf:resource="http://www.usgs.gov/science/USGSThesaurus/hydrology"/>
    <skos:related rdf:resource="http://www.usgs.gov/science/USGSThesaurus/water%20chemistry"/>
    <skos:inScheme rdf:resource="http://www.usgs.gov/science/USGSThesaurus"/>
  </rdf:Description>
  <rdf:Description about="http://www.usgs.gov/science/USGSThesaurus/geolocation%20measurement">
    <rdf:type rdf:resource="http://www.w3.org/2004/02/skos/core#Concept"/>
    <skos:prefLabel xml:lang="en">geolocation measurement</skos:prefLabel>
    <skos:scopeNote xml:lang="en">Methods for establishing a geographic location on the surface of the earth.</skos:scopeNote>
    <skos:altLabel xml:lang="en">location measurement</skos:altLabel>
    <skos:altLabel xml:lang="en">navigating</skos:altLabel>
    <skos:altLabel xml:lang="en">orienteering</skos:altLabel>
    <skos:broader rdf:resource="http://www.usgs.gov/science/USGSThesaurus/field%20methods"/>
    <skos:narrower rdf:resource="http://www.usgs.gov/science/USGSThesaurus/GPS%20measurement"/>
    <skos:narrower rdf:resource="http://www.usgs.gov/science/USGSThesaurus/LORAN-C%20navigation"/>
    <skos:narrower rdf:resource="http://www.usgs.gov/science/USGSThesaurus/altimetry%20measurement"/>
    <skos:narrower rdf:resource="http://www.usgs.gov/science/USGSThesaurus/bathymetry%20measurement"/>
    <skos:narrower rdf:resource="http://www.usgs.gov/science/USGSThesaurus/land%20surveying"/>
    <skos:related rdf:resource="http://www.usgs.gov/science/USGSThesaurus/geographic%20information%20systems"/>
    <skos:related rdf:resource="http://www.usgs.gov/science/USGSThesaurus/geography"/>
    <skos:inScheme rdf:resource="http://www.usgs.gov/science/USGSThesaurus"/>
  </rdf:Description>
  <rdf:Description about="http://www.usgs.gov/science/USGSThesaurus/GPS%20measurement">
    <rdf:type rdf:resource="http://www.w3.org/2004/02/skos/core#Concept"/>
    <skos:prefLabel xml:lang="en">GPS measurement</skos:prefLabel>
    <skos:scopeNote xml:lang="en">Determination of distance and location using instruments receiving signals from the Global Positioning System, a system of satellites for identifying earth locations.</skos:scopeNote>
    <skos:altLabel xml:lang="en">global positioning measurement</skos:altLabel>
    <skos:altLabel xml:lang="en">differential GPS</skos:altLabel>
    <skos:altLabel xml:lang="en">DGPS</skos:altLabel>
    <skos:altLabel xml:lang="en">real-time kinematic navigation</skos:altLabel>
    <skos:broader rdf:resource="http://www.usgs.gov/science/USGSThesaurus/geolocation%20measurement"/>
    <skos:related rdf:resource="http://www.usgs.gov/science/USGSThesaurus/geographic%20information%20systems"/>
    <skos:related rdf:resource="http://www.usgs.gov/science/USGSThesaurus/geography"/>
    <skos:inScheme rdf:resource="http://www.usgs.gov/science/USGSThesaurus"/>
  </rdf:Description>
  <rdf:Description about="http://www.usgs.gov/science/USGSThesaurus/LORAN-C%20navigation">
    <rdf:type rdf:resource="http://www.w3.org/2004/02/skos/core#Concept"/>
    <skos:prefLabel xml:lang="en">LORAN-C navigation</skos:prefLabel>
    <skos:scopeNote xml:lang="en">Hyperbolic radio navigation system used for near-shore waters.</skos:scopeNote>
    <skos:broader rdf:resource="http://www.usgs.gov/science/USGSThesaurus/geolocation%20measurement"/>
    <skos:inScheme rdf:resource="http://www.usgs.gov/science/USGSThesaurus"/>
  </rdf:Description>
  <rdf:Description about="http://www.usgs.gov/science/USGSThesaurus/altimetry%20measurement">
    <rdf:type rdf:resource="http://www.w3.org/2004/02/skos/core#Concept"/>
    <skos:prefLabel xml:lang="en">altimetry measurement</skos:prefLabel>
    <skos:scopeNote xml:lang="en">The measurement of altitude, or height above mean sea level, using instruments such as aneroid barometers and radar altimeters.</skos:scopeNote>
    <!--FOR satellite altimetry USE altimetry measurement WITH remote sensing-->
    <skos:altLabel xml:lang="en">satellite altimetry</skos:altLabel>
    <skos:broader rdf:resource="http://www.usgs.gov/science/USGSThesaurus/geolocation%20measurement"/>
    <skos:related rdf:resource="http://www.usgs.gov/science/USGSThesaurus/geography"/>
    <skos:inScheme rdf:resource="http://www.usgs.gov/science/USGSThesaurus"/>
  </rdf:Description>
  <rdf:Description about="http://www.usgs.gov/science/USGSThesaurus/bathymetry%20measurement">
    <rdf:type rdf:resource="http://www.w3.org/2004/02/skos/core#Concept"/>
    <skos:prefLabel xml:lang="en">bathymetry measurement</skos:prefLabel>
    <skos:scopeNote xml:lang="en">Means of determining the depth to the floor of a body of water, especially the ocean.</skos:scopeNote>
    <skos:broader rdf:resource="http://www.usgs.gov/science/USGSThesaurus/geolocation%20measurement"/>
    <skos:related rdf:resource="http://www.usgs.gov/science/USGSThesaurus/geography"/>
    <skos:inScheme rdf:resource="http://www.usgs.gov/science/USGSThesaurus"/>
  </rdf:Description>
  <rdf:Description about="http://www.usgs.gov/science/USGSThesaurus/land%20surveying">
    <rdf:type rdf:resource="http://www.w3.org/2004/02/skos/core#Concept"/>
    <skos:prefLabel xml:lang="en">land surveying</skos:prefLabel>
    <skos:scopeNote xml:lang="en">Determining property boundaries, land area, elevations, and locations of features on the surface of the land by calculations based on the instrumental measurements of angles and distances or by use of global positional satellites.</skos:scopeNote>
    <skos:altLabel xml:lang="en">surveying</skos:altLabel>
    <skos:broader rdf:resource="http://www.usgs.gov/science/USGSThesaurus/geolocation%20measurement"/>
    <skos:related rdf:resource="http://www.usgs.gov/science/USGSThesaurus/geodesy"/>
    <skos:related rdf:resource="http://www.usgs.gov/science/USGSThesaurus/geography"/>
    <skos:inScheme rdf:resource="http://www.usgs.gov/science/USGSThesaurus"/>
  </rdf:Description>
  <rdf:Description about="http://www.usgs.gov/science/USGSThesaurus/real-time%20monitoring%20and%20reporting">
    <rdf:type rdf:resource="http://www.w3.org/2004/02/skos/core#Concept"/>
    <skos:prefLabel xml:lang="en">real-time monitoring and reporting</skos:prefLabel>
    <skos:scopeNote xml:lang="en">Gathering information through periodic or continuous measurement in the field to provide a view of current conditions. In some instances, observations may not be subject to rigorous review before release; this will be noted in the documentation accompanying the data.</skos:scopeNote>
    <skos:altLabel xml:lang="en">real-time data</skos:altLabel>
    <skos:broader rdf:resource="http://www.usgs.gov/science/USGSThesaurus/field%20methods"/>
    <skos:inScheme rdf:resource="http://www.usgs.gov/science/USGSThesaurus"/>
  </rdf:Description>
  <rdf:Description about="http://www.usgs.gov/science/USGSThesaurus/laboratory%20methods">
    <rdf:type rdf:resource="http://www.w3.org/2004/02/skos/core#Concept"/>
    <skos:prefLabel xml:lang="en">laboratory methods</skos:prefLabel>
    <skos:scopeNote xml:lang="en">Experimental techniques to analyze and test samples in a place equipped and designed for the work.</skos:scopeNote>
    <skos:broader rdf:resource="http://www.usgs.gov/science/USGSThesaurus/methods"/>
    <skos:narrower rdf:resource="http://www.usgs.gov/science/USGSThesaurus/age%20estimation%20methods"/>
    <skos:narrower rdf:resource="http://www.usgs.gov/science/USGSThesaurus/camera%20calibration"/>
    <skos:narrower rdf:resource="http://www.usgs.gov/science/USGSThesaurus/chemical%20analysis"/>
    <skos:narrower rdf:resource="http://www.usgs.gov/science/USGSThesaurus/core%20analysis"/>
    <skos:narrower rdf:resource="http://www.usgs.gov/science/USGSThesaurus/culturing%20%28specimens%29"/>
    <skos:narrower rdf:resource="http://www.usgs.gov/science/USGSThesaurus/faunal%20and%20floral%20census%20%28microscopic%29"/>
    <skos:narrower rdf:resource="http://www.usgs.gov/science/USGSThesaurus/grain-size%20analysis"/>
    <skos:narrower rdf:resource="http://www.usgs.gov/science/USGSThesaurus/isotopic%20analysis"/>
    <skos:narrower rdf:resource="http://www.usgs.gov/science/USGSThesaurus/meristics"/>
    <skos:narrower rdf:resource="http://www.usgs.gov/science/USGSThesaurus/microscopy"/>
    <skos:narrower rdf:resource="http://www.usgs.gov/science/USGSThesaurus/paleomagnetic%20analysis"/>
    <skos:narrower rdf:resource="http://www.usgs.gov/science/USGSThesaurus/petrography"/>
    <skos:narrower rdf:resource="http://www.usgs.gov/science/USGSThesaurus/plant%20and%20animal%20testing"/>
    <skos:narrower rdf:resource="http://www.usgs.gov/science/USGSThesaurus/subsampling"/>
    <skos:narrower rdf:resource="http://www.usgs.gov/science/USGSThesaurus/therapeutic%20methods"/>
    <skos:narrower rdf:resource="http://www.usgs.gov/science/USGSThesaurus/tree%20ring%20analysis"/>
    <skos:inScheme rdf:resource="http://www.usgs.gov/science/USGSThesaurus"/>
  </rdf:Description>
  <rdf:Description about="http://www.usgs.gov/science/USGSThesaurus/age%20estimation%20methods">
    <rdf:type rdf:resource="http://www.w3.org/2004/02/skos/core#Concept"/>
    <skos:prefLabel xml:lang="en">age estimation methods</skos:prefLabel>
    <skos:scopeNote xml:lang="en">Methods used to determine the age of earth materials, typically by laboratory analysis of properties of those materials. </skos:scopeNote>
    <skos:altLabel xml:lang="en">dating methods</skos:altLabel>
    <skos:broader rdf:resource="http://www.usgs.gov/science/USGSThesaurus/laboratory%20methods"/>
    <skos:narrower rdf:resource="http://www.usgs.gov/science/USGSThesaurus/fission-track%20dating"/>
    <skos:narrower rdf:resource="http://www.usgs.gov/science/USGSThesaurus/luminescence%20dating"/>
    <skos:narrower rdf:resource="http://www.usgs.gov/science/USGSThesaurus/sclerochronology"/>
    <skos:narrower rdf:resource="http://www.usgs.gov/science/USGSThesaurus/tephrochronology"/>
    <skos:related rdf:resource="http://www.usgs.gov/science/USGSThesaurus/radiometric%20dating"/>
    <skos:related rdf:resource="http://www.usgs.gov/science/USGSThesaurus/tree%20ring%20analysis"/>
    <skos:inScheme rdf:resource="http://www.usgs.gov/science/USGSThesaurus"/>
  </rdf:Description>
  <rdf:Description about="http://www.usgs.gov/science/USGSThesaurus/fission-track%20dating">
    <rdf:type rdf:resource="http://www.w3.org/2004/02/skos/core#Concept"/>
    <skos:prefLabel xml:lang="en">fission-track dating</skos:prefLabel>
    <skos:scopeNote xml:lang="en">Laboratory technique for determining the age of rocks and other geological materials by counts of spontaneous and induced fission tracks left by the radioactive isotope uranium-238.</skos:scopeNote>
    <skos:altLabel xml:lang="en">age dating (fission-track)</skos:altLabel>
    <skos:altLabel xml:lang="en">fission-track method</skos:altLabel>
    <skos:broader rdf:resource="http://www.usgs.gov/science/USGSThesaurus/age%20estimation%20methods"/>
    <skos:related rdf:resource="http://www.usgs.gov/science/USGSThesaurus/geochronology"/>
    <skos:related rdf:resource="http://www.usgs.gov/science/USGSThesaurus/radiometric%20dating"/>
    <skos:inScheme rdf:resource="http://www.usgs.gov/science/USGSThesaurus"/>
  </rdf:Description>
  <rdf:Description about="http://www.usgs.gov/science/USGSThesaurus/luminescence%20dating">
    <rdf:type rdf:resource="http://www.w3.org/2004/02/skos/core#Concept"/>
    <skos:prefLabel xml:lang="en">luminescence dating</skos:prefLabel>
    <skos:scopeNote xml:lang="en">Dating methods that involve the analysis of the optical properties of minerals exposed to environmental radiation.  Typically used to determine the age of subaerial exposure of surficial sediments.</skos:scopeNote>
    <skos:altLabel xml:lang="en">optically-stimulated luminescence dating</skos:altLabel>
    <skos:altLabel xml:lang="en">thermoluminescence dating</skos:altLabel>
    <skos:altLabel xml:lang="en">TL/OSL dating</skos:altLabel>
    <skos:broader rdf:resource="http://www.usgs.gov/science/USGSThesaurus/age%20estimation%20methods"/>
    <skos:inScheme rdf:resource="http://www.usgs.gov/science/USGSThesaurus"/>
  </rdf:Description>
  <rdf:Description about="http://www.usgs.gov/science/USGSThesaurus/sclerochronology">
    <rdf:type rdf:resource="http://www.w3.org/2004/02/skos/core#Concept"/>
    <skos:prefLabel xml:lang="en">sclerochronology</skos:prefLabel>
    <skos:scopeNote xml:lang="en">Description of the history of individual organisms by studying the variations in thickness of accretionary layers in their skeletons.</skos:scopeNote>
    <skos:broader rdf:resource="http://www.usgs.gov/science/USGSThesaurus/age%20estimation%20methods"/>
    <skos:inScheme rdf:resource="http://www.usgs.gov/science/USGSThesaurus"/>
  </rdf:Description>
  <rdf:Description about="http://www.usgs.gov/science/USGSThesaurus/tephrochronology">
    <rdf:type rdf:resource="http://www.w3.org/2004/02/skos/core#Concept"/>
    <skos:prefLabel xml:lang="en">tephrochronology</skos:prefLabel>
    <skos:scopeNote xml:lang="en">Age determination of rocks and deposits by correlation of volcanic ash layers (tephra) that bound the deposits below and above.</skos:scopeNote>
    <skos:broader rdf:resource="http://www.usgs.gov/science/USGSThesaurus/age%20estimation%20methods"/>
    <skos:related rdf:resource="http://www.usgs.gov/science/USGSThesaurus/lithostratigraphy"/>
    <skos:inScheme rdf:resource="http://www.usgs.gov/science/USGSThesaurus"/>
  </rdf:Description>
  <rdf:Description about="http://www.usgs.gov/science/USGSThesaurus/camera%20calibration">
    <rdf:type rdf:resource="http://www.w3.org/2004/02/skos/core#Concept"/>
    <skos:prefLabel xml:lang="en">camera calibration</skos:prefLabel>
    <skos:scopeNote xml:lang="en">Optical calibration of cameras that are typically used in airborne remote sensing.</skos:scopeNote>
    <skos:broader rdf:resource="http://www.usgs.gov/science/USGSThesaurus/laboratory%20methods"/>
    <skos:inScheme rdf:resource="http://www.usgs.gov/science/USGSThesaurus"/>
  </rdf:Description>
  <rdf:Description about="http://www.usgs.gov/science/USGSThesaurus/chemical%20analysis">
    <rdf:type rdf:resource="http://www.w3.org/2004/02/skos/core#Concept"/>
    <skos:prefLabel xml:lang="en">chemical analysis</skos:prefLabel>
    <skos:scopeNote xml:lang="en">Chemical techniques used to identify the composition of substances.</skos:scopeNote>
    <skos:altLabel xml:lang="en">detection (chemical)</skos:altLabel>
    <skos:altLabel xml:lang="en">geochemical surveys</skos:altLabel>
    <skos:altLabel xml:lang="en">leaching (analytical method)</skos:altLabel>
    <skos:altLabel xml:lang="en">mineralogical analysis</skos:altLabel>
    <skos:altLabel xml:lang="en">nuclear magnetic resonance spectroscopy</skos:altLabel>
    <!--FOR sediment geochemistry USE chemical analysis WITH unconsolidated deposits-->
    <skos:altLabel xml:lang="en">sediment geochemistry</skos:altLabel>
    <skos:broader rdf:resource="http://www.usgs.gov/science/USGSThesaurus/laboratory%20methods"/>
    <skos:narrower rdf:resource="http://www.usgs.gov/science/USGSThesaurus/DNA%20sequencing"/>
    <skos:narrower rdf:resource="http://www.usgs.gov/science/USGSThesaurus/atomic%20absorption%20analysis"/>
    <skos:narrower rdf:resource="http://www.usgs.gov/science/USGSThesaurus/atomic%20emission%20spectroscopy"/>
    <skos:narrower rdf:resource="http://www.usgs.gov/science/USGSThesaurus/chromatography"/>
    <skos:narrower rdf:resource="http://www.usgs.gov/science/USGSThesaurus/electrophoresis"/>
    <skos:narrower rdf:resource="http://www.usgs.gov/science/USGSThesaurus/flow%20cytometry"/>
    <skos:narrower rdf:resource="http://www.usgs.gov/science/USGSThesaurus/mass%20spectroscopy"/>
    <skos:narrower rdf:resource="http://www.usgs.gov/science/USGSThesaurus/neutron%20activation%20analysis"/>
    <skos:narrower rdf:resource="http://www.usgs.gov/science/USGSThesaurus/particle-beam%20spectroscopy"/>
    <skos:narrower rdf:resource="http://www.usgs.gov/science/USGSThesaurus/polymerase%20chain%20reaction"/>
    <skos:narrower rdf:resource="http://www.usgs.gov/science/USGSThesaurus/x-ray%20diffraction"/>
    <skos:narrower rdf:resource="http://www.usgs.gov/science/USGSThesaurus/x-ray%20fluorescence"/>
    <skos:related rdf:resource="http://www.usgs.gov/science/USGSThesaurus/biochemistry"/>
    <skos:related rdf:resource="http://www.usgs.gov/science/USGSThesaurus/geochemistry"/>
    <skos:inScheme rdf:resource="http://www.usgs.gov/science/USGSThesaurus"/>
  </rdf:Description>
  <rdf:Description about="http://www.usgs.gov/science/USGSThesaurus/DNA%20sequencing">
    <rdf:type rdf:resource="http://www.w3.org/2004/02/skos/core#Concept"/>
    <skos:prefLabel xml:lang="en">DNA sequencing</skos:prefLabel>
    <skos:scopeNote xml:lang="en">Biochemical procedure to determine the order of nucleotides in genes.</skos:scopeNote>
    <skos:altLabel xml:lang="en">gene sequencing</skos:altLabel>
    <skos:altLabel xml:lang="en">genome</skos:altLabel>
    <skos:broader rdf:resource="http://www.usgs.gov/science/USGSThesaurus/chemical%20analysis"/>
    <skos:related rdf:resource="http://www.usgs.gov/science/USGSThesaurus/biochemistry"/>
    <skos:related rdf:resource="http://www.usgs.gov/science/USGSThesaurus/genetics"/>
    <skos:inScheme rdf:resource="http://www.usgs.gov/science/USGSThesaurus"/>
  </rdf:Description>
  <rdf:Description about="http://www.usgs.gov/science/USGSThesaurus/atomic%20absorption%20analysis">
    <rdf:type rdf:resource="http://www.w3.org/2004/02/skos/core#Concept"/>
    <skos:prefLabel xml:lang="en">atomic absorption analysis</skos:prefLabel>
    <skos:scopeNote xml:lang="en">Technique used to identify chemicals based on the measurement of the spectra produced by atoms and molecules with absorption of electromagnetic radiation.</skos:scopeNote>
    <skos:broader rdf:resource="http://www.usgs.gov/science/USGSThesaurus/chemical%20analysis"/>
    <skos:related rdf:resource="http://www.usgs.gov/science/USGSThesaurus/biochemistry"/>
    <skos:related rdf:resource="http://www.usgs.gov/science/USGSThesaurus/geochemistry"/>
    <skos:inScheme rdf:resource="http://www.usgs.gov/science/USGSThesaurus"/>
  </rdf:Description>
  <rdf:Description about="http://www.usgs.gov/science/USGSThesaurus/atomic%20emission%20spectroscopy">
    <rdf:type rdf:resource="http://www.w3.org/2004/02/skos/core#Concept"/>
    <skos:prefLabel xml:lang="en">atomic emission spectroscopy</skos:prefLabel>
    <skos:scopeNote xml:lang="en">Chemical detection of element concentration by examining the intensity and wavelength of light emitted from the sample when gaseous sample is ionized and maintained in a plasma state.</skos:scopeNote>
    <skos:altLabel xml:lang="en">ICP-AES</skos:altLabel>
    <skos:altLabel xml:lang="en">inductively coupled plasma-atomic emission spectrometry</skos:altLabel>
    <skos:broader rdf:resource="http://www.usgs.gov/science/USGSThesaurus/chemical%20analysis"/>
    <skos:inScheme rdf:resource="http://www.usgs.gov/science/USGSThesaurus"/>
  </rdf:Description>
  <rdf:Description about="http://www.usgs.gov/science/USGSThesaurus/chromatography">
    <rdf:type rdf:resource="http://www.w3.org/2004/02/skos/core#Concept"/>
    <skos:prefLabel xml:lang="en">chromatography</skos:prefLabel>
    <skos:scopeNote xml:lang="en">Analytical techniques used to separate or partition the components of a gaseous or liquid mixture by differences in absorption rates during flow around or over surface absorbents such as columns of silica, filter papers, or gels.</skos:scopeNote>
    <skos:broader rdf:resource="http://www.usgs.gov/science/USGSThesaurus/chemical%20analysis"/>
    <skos:narrower rdf:resource="http://www.usgs.gov/science/USGSThesaurus/gas%20chromatography"/>
    <skos:narrower rdf:resource="http://www.usgs.gov/science/USGSThesaurus/liquid%20chromatography"/>
    <skos:related rdf:resource="http://www.usgs.gov/science/USGSThesaurus/biochemistry"/>
    <skos:related rdf:resource="http://www.usgs.gov/science/USGSThesaurus/geochemistry"/>
    <skos:inScheme rdf:resource="http://www.usgs.gov/science/USGSThesaurus"/>
  </rdf:Description>
  <rdf:Description about="http://www.usgs.gov/science/USGSThesaurus/gas%20chromatography">
    <rdf:type rdf:resource="http://www.w3.org/2004/02/skos/core#Concept"/>
    <skos:prefLabel xml:lang="en">gas chromatography</skos:prefLabel>
    <skos:scopeNote xml:lang="en">Chromatographic technique used to separate or partition the components of a mixture.  Solid and liquid samples are vaporized and passed through a column containing a liquid that differentially absorbs the  molecules.</skos:scopeNote>
    <skos:broader rdf:resource="http://www.usgs.gov/science/USGSThesaurus/chromatography"/>
    <skos:related rdf:resource="http://www.usgs.gov/science/USGSThesaurus/biochemistry"/>
    <skos:related rdf:resource="http://www.usgs.gov/science/USGSThesaurus/geochemistry"/>
    <skos:inScheme rdf:resource="http://www.usgs.gov/science/USGSThesaurus"/>
  </rdf:Description>
  <rdf:Description about="http://www.usgs.gov/science/USGSThesaurus/liquid%20chromatography">
    <rdf:type rdf:resource="http://www.w3.org/2004/02/skos/core#Concept"/>
    <skos:prefLabel xml:lang="en">liquid chromatography</skos:prefLabel>
    <skos:scopeNote xml:lang="en">Chromatographic technique to separate or partition the components of a mixture in which samples are liquid and passed through a column.</skos:scopeNote>
    <skos:altLabel xml:lang="en">HPLC</skos:altLabel>
    <skos:altLabel xml:lang="en">high-pressure liquid chromatography</skos:altLabel>
    <skos:broader rdf:resource="http://www.usgs.gov/science/USGSThesaurus/chromatography"/>
    <skos:related rdf:resource="http://www.usgs.gov/science/USGSThesaurus/biochemistry"/>
    <skos:related rdf:resource="http://www.usgs.gov/science/USGSThesaurus/geochemistry"/>
    <skos:inScheme rdf:resource="http://www.usgs.gov/science/USGSThesaurus"/>
  </rdf:Description>
  <rdf:Description about="http://www.usgs.gov/science/USGSThesaurus/electrophoresis">
    <rdf:type rdf:resource="http://www.w3.org/2004/02/skos/core#Concept"/>
    <skos:prefLabel xml:lang="en">electrophoresis</skos:prefLabel>
    <skos:scopeNote xml:lang="en">Analytical technique to separate and identify components in a mixture using the differential migration of molecules based on their net charge through a paper or gel medium.</skos:scopeNote>
    <skos:broader rdf:resource="http://www.usgs.gov/science/USGSThesaurus/chemical%20analysis"/>
    <skos:related rdf:resource="http://www.usgs.gov/science/USGSThesaurus/biochemistry"/>
    <skos:inScheme rdf:resource="http://www.usgs.gov/science/USGSThesaurus"/>
  </rdf:Description>
  <rdf:Description about="http://www.usgs.gov/science/USGSThesaurus/flow%20cytometry">
    <rdf:type rdf:resource="http://www.w3.org/2004/02/skos/core#Concept"/>
    <skos:prefLabel xml:lang="en">flow cytometry</skos:prefLabel>
    <skos:scopeNote xml:lang="en">Laboratory technique to determine the amount of DNA in cells tagged by fluorescent dye by measuring the intensity of fluorescence under a laser beam.</skos:scopeNote>
    <skos:broader rdf:resource="http://www.usgs.gov/science/USGSThesaurus/chemical%20analysis"/>
    <skos:related rdf:resource="http://www.usgs.gov/science/USGSThesaurus/biochemistry"/>
    <skos:related rdf:resource="http://www.usgs.gov/science/USGSThesaurus/cell%20biology"/>
    <skos:inScheme rdf:resource="http://www.usgs.gov/science/USGSThesaurus"/>
  </rdf:Description>
  <rdf:Description about="http://www.usgs.gov/science/USGSThesaurus/mass%20spectroscopy">
    <rdf:type rdf:resource="http://www.w3.org/2004/02/skos/core#Concept"/>
    <skos:prefLabel xml:lang="en">mass spectroscopy</skos:prefLabel>
    <skos:scopeNote xml:lang="en">Instrumental technique to separate and identify molecules.  Gaseous ions are formed, with or without fragmentation.  Their mass/charge ratios and relative electrical abundance are then measured or the spectra are recorded.</skos:scopeNote>
    <skos:altLabel xml:lang="en">mass spectrometry</skos:altLabel>
    <skos:broader rdf:resource="http://www.usgs.gov/science/USGSThesaurus/chemical%20analysis"/>
    <skos:related rdf:resource="http://www.usgs.gov/science/USGSThesaurus/biochemistry"/>
    <skos:related rdf:resource="http://www.usgs.gov/science/USGSThesaurus/geochemistry"/>
    <skos:inScheme rdf:resource="http://www.usgs.gov/science/USGSThesaurus"/>
  </rdf:Description>
  <rdf:Description about="http://www.usgs.gov/science/USGSThesaurus/neutron%20activation%20analysis">
    <rdf:type rdf:resource="http://www.w3.org/2004/02/skos/core#Concept"/>
    <skos:prefLabel xml:lang="en">neutron activation analysis</skos:prefLabel>
    <skos:scopeNote xml:lang="en">Sensitive laboratory technique for both qualitative and quantitative analysis of elements in samples.  Target nuclei are bombarded with neutron beams to start nuclear reactions which emit characteristic gamma ray radiations.</skos:scopeNote>
    <skos:broader rdf:resource="http://www.usgs.gov/science/USGSThesaurus/chemical%20analysis"/>
    <skos:related rdf:resource="http://www.usgs.gov/science/USGSThesaurus/biochemistry"/>
    <skos:related rdf:resource="http://www.usgs.gov/science/USGSThesaurus/geochemistry"/>
    <skos:inScheme rdf:resource="http://www.usgs.gov/science/USGSThesaurus"/>
  </rdf:Description>
  <rdf:Description about="http://www.usgs.gov/science/USGSThesaurus/particle-beam%20spectroscopy">
    <rdf:type rdf:resource="http://www.w3.org/2004/02/skos/core#Concept"/>
    <skos:prefLabel xml:lang="en">particle-beam spectroscopy</skos:prefLabel>
    <skos:scopeNote xml:lang="en">Analytical technique using a concentrated beam of charged subatomic particles.</skos:scopeNote>
    <skos:altLabel xml:lang="en">electron probe microanalysis</skos:altLabel>
    <skos:broader rdf:resource="http://www.usgs.gov/science/USGSThesaurus/chemical%20analysis"/>
    <skos:related rdf:resource="http://www.usgs.gov/science/USGSThesaurus/biochemistry"/>
    <skos:related rdf:resource="http://www.usgs.gov/science/USGSThesaurus/geochemistry"/>
    <skos:inScheme rdf:resource="http://www.usgs.gov/science/USGSThesaurus"/>
  </rdf:Description>
  <rdf:Description about="http://www.usgs.gov/science/USGSThesaurus/polymerase%20chain%20reaction">
    <rdf:type rdf:resource="http://www.w3.org/2004/02/skos/core#Concept"/>
    <skos:prefLabel xml:lang="en">polymerase chain reaction</skos:prefLabel>
    <skos:scopeNote xml:lang="en">Biochemical technique that uses enzymes to replicate new nucleotides of DNA from DNA triphosphates using DNA as a template.</skos:scopeNote>
    <skos:broader rdf:resource="http://www.usgs.gov/science/USGSThesaurus/chemical%20analysis"/>
    <skos:related rdf:resource="http://www.usgs.gov/science/USGSThesaurus/biochemistry"/>
    <skos:related rdf:resource="http://www.usgs.gov/science/USGSThesaurus/genetics"/>
    <skos:inScheme rdf:resource="http://www.usgs.gov/science/USGSThesaurus"/>
  </rdf:Description>
  <rdf:Description about="http://www.usgs.gov/science/USGSThesaurus/x-ray%20diffraction">
    <rdf:type rdf:resource="http://www.w3.org/2004/02/skos/core#Concept"/>
    <skos:prefLabel xml:lang="en">x-ray diffraction</skos:prefLabel>
    <skos:scopeNote xml:lang="en">Study of crystals which uses short wave electromagnetic radiations (x-rays). The xrays, scattered by the crystal atoms, show a characteristic interference pattern that is dependent upon the structure of the crystal.</skos:scopeNote>
    <skos:broader rdf:resource="http://www.usgs.gov/science/USGSThesaurus/chemical%20analysis"/>
    <skos:related rdf:resource="http://www.usgs.gov/science/USGSThesaurus/mineralogy"/>
    <skos:inScheme rdf:resource="http://www.usgs.gov/science/USGSThesaurus"/>
  </rdf:Description>
  <rdf:Description about="http://www.usgs.gov/science/USGSThesaurus/x-ray%20fluorescence">
    <rdf:type rdf:resource="http://www.w3.org/2004/02/skos/core#Concept"/>
    <skos:prefLabel xml:lang="en">x-ray fluorescence</skos:prefLabel>
    <skos:scopeNote xml:lang="en">Estimation of chemical element concentration by measuring the energy level of secondary X-rays generated when the sample is bombarded with high-energy X-rays or gamma rays.</skos:scopeNote>
    <skos:altLabel xml:lang="en">XRF</skos:altLabel>
    <skos:broader rdf:resource="http://www.usgs.gov/science/USGSThesaurus/chemical%20analysis"/>
    <skos:inScheme rdf:resource="http://www.usgs.gov/science/USGSThesaurus"/>
  </rdf:Description>
  <rdf:Description about="http://www.usgs.gov/science/USGSThesaurus/core%20analysis">
    <rdf:type rdf:resource="http://www.w3.org/2004/02/skos/core#Concept"/>
    <skos:prefLabel xml:lang="en">core analysis</skos:prefLabel>
    <skos:scopeNote xml:lang="en">Study of the composition and layers of cylindrical samples of rocks, trees, ice, and other materials extracted by drilling into a mass. Intended for broad use for the analysis of all types of core samples. The combination of this term with other terms will convey the context of the activity.</skos:scopeNote>
    <skos:broader rdf:resource="http://www.usgs.gov/science/USGSThesaurus/laboratory%20methods"/>
    <skos:related rdf:resource="http://www.usgs.gov/science/USGSThesaurus/drilling%20and%20coring"/>
    <skos:inScheme rdf:resource="http://www.usgs.gov/science/USGSThesaurus"/>
  </rdf:Description>
  <rdf:Description about="http://www.usgs.gov/science/USGSThesaurus/culturing%20%28specimens%29">
    <rdf:type rdf:resource="http://www.w3.org/2004/02/skos/core#Concept"/>
    <skos:prefLabel xml:lang="en">culturing (specimens)</skos:prefLabel>
    <skos:scopeNote xml:lang="en">Growing microorganisms, tissue cells, or other living matter in a specially prepared nutrient medium for diagnostic or scientific use.</skos:scopeNote>
    <skos:broader rdf:resource="http://www.usgs.gov/science/USGSThesaurus/laboratory%20methods"/>
    <skos:related rdf:resource="http://www.usgs.gov/science/USGSThesaurus/bacteriology"/>
    <skos:related rdf:resource="http://www.usgs.gov/science/USGSThesaurus/microbiology"/>
    <skos:inScheme rdf:resource="http://www.usgs.gov/science/USGSThesaurus"/>
  </rdf:Description>
  <rdf:Description about="http://www.usgs.gov/science/USGSThesaurus/faunal%20and%20floral%20census%20%28microscopic%29">
    <rdf:type rdf:resource="http://www.w3.org/2004/02/skos/core#Concept"/>
    <skos:prefLabel xml:lang="en">faunal and floral census (microscopic)</skos:prefLabel>
    <skos:scopeNote xml:lang="en">Records of counts of the different microscopic species in a core, soil, sediment, rock or water sample to determine geologic age or other characteristic of the sample.  Use for microscopic examinations.</skos:scopeNote>
    <skos:altLabel xml:lang="en">pollen analysis</skos:altLabel>
    <skos:broader rdf:resource="http://www.usgs.gov/science/USGSThesaurus/laboratory%20methods"/>
    <skos:related rdf:resource="http://www.usgs.gov/science/USGSThesaurus/field%20inventory%20and%20monitoring"/>
    <skos:related rdf:resource="http://www.usgs.gov/science/USGSThesaurus/microbiology"/>
    <skos:related rdf:resource="http://www.usgs.gov/science/USGSThesaurus/micropaleontology"/>
    <skos:related rdf:resource="http://www.usgs.gov/science/USGSThesaurus/microscopy"/>
    <skos:inScheme rdf:resource="http://www.usgs.gov/science/USGSThesaurus"/>
  </rdf:Description>
  <rdf:Description about="http://www.usgs.gov/science/USGSThesaurus/grain-size%20analysis">
    <rdf:type rdf:resource="http://www.w3.org/2004/02/skos/core#Concept"/>
    <skos:prefLabel xml:lang="en">grain-size analysis</skos:prefLabel>
    <skos:scopeNote xml:lang="en">Method of studying soils, sediments, sands, or rock by determining the size, distribution, and proportion of selected particles.</skos:scopeNote>
    <skos:altLabel xml:lang="en">grainsize analysis</skos:altLabel>
    <skos:altLabel xml:lang="en">granulometry</skos:altLabel>
    <skos:altLabel xml:lang="en">particle-size analysis</skos:altLabel>
    <skos:broader rdf:resource="http://www.usgs.gov/science/USGSThesaurus/laboratory%20methods"/>
    <skos:narrower rdf:resource="http://www.usgs.gov/science/USGSThesaurus/sieve-size%20analysis"/>
    <skos:related rdf:resource="http://www.usgs.gov/science/USGSThesaurus/sedimentology"/>
    <skos:inScheme rdf:resource="http://www.usgs.gov/science/USGSThesaurus"/>
  </rdf:Description>
  <rdf:Description about="http://www.usgs.gov/science/USGSThesaurus/sieve-size%20analysis">
    <rdf:type rdf:resource="http://www.w3.org/2004/02/skos/core#Concept"/>
    <skos:prefLabel xml:lang="en">sieve-size analysis</skos:prefLabel>
    <skos:scopeNote xml:lang="en">Analytic technique determining the distribution of the different sizes of particles in soil, sediment, or rock samples by measuring the percentage that will pass through mesh holes of known size.</skos:scopeNote>
    <skos:broader rdf:resource="http://www.usgs.gov/science/USGSThesaurus/grain-size%20analysis"/>
    <skos:related rdf:resource="http://www.usgs.gov/science/USGSThesaurus/sedimentology"/>
    <skos:inScheme rdf:resource="http://www.usgs.gov/science/USGSThesaurus"/>
  </rdf:Description>
  <rdf:Description about="http://www.usgs.gov/science/USGSThesaurus/isotopic%20analysis">
    <rdf:type rdf:resource="http://www.w3.org/2004/02/skos/core#Concept"/>
    <skos:prefLabel xml:lang="en">isotopic analysis</skos:prefLabel>
    <skos:scopeNote xml:lang="en">Experimental determination of the proportion of a given isotope (or isotopes) in a sample.</skos:scopeNote>
    <skos:broader rdf:resource="http://www.usgs.gov/science/USGSThesaurus/laboratory%20methods"/>
    <skos:narrower rdf:resource="http://www.usgs.gov/science/USGSThesaurus/light%20stable%20isotope%20analysis"/>
    <skos:narrower rdf:resource="http://www.usgs.gov/science/USGSThesaurus/radiometric%20dating"/>
    <skos:related rdf:resource="http://www.usgs.gov/science/USGSThesaurus/biochemistry"/>
    <skos:related rdf:resource="http://www.usgs.gov/science/USGSThesaurus/geochemistry"/>
    <skos:inScheme rdf:resource="http://www.usgs.gov/science/USGSThesaurus"/>
  </rdf:Description>
  <rdf:Description about="http://www.usgs.gov/science/USGSThesaurus/light%20stable%20isotope%20analysis">
    <rdf:type rdf:resource="http://www.w3.org/2004/02/skos/core#Concept"/>
    <skos:prefLabel xml:lang="en">light stable isotope analysis</skos:prefLabel>
    <skos:scopeNote xml:lang="en">Analytical technique using mass spectrometry to measure the different isotopic forms of low mass (light) elements such as oxygen, hydrogen, carbon, nitrogen and sulfur that occur in samples.</skos:scopeNote>
    <skos:altLabel xml:lang="en">light stable-isotope analysis</skos:altLabel>
    <skos:altLabel xml:lang="en">stable isotope analysis</skos:altLabel>
    <skos:broader rdf:resource="http://www.usgs.gov/science/USGSThesaurus/isotopic%20analysis"/>
    <skos:narrower rdf:resource="http://www.usgs.gov/science/USGSThesaurus/beryllium%20isotope%20analysis"/>
    <skos:narrower rdf:resource="http://www.usgs.gov/science/USGSThesaurus/carbon%20isotope%20analysis"/>
    <skos:narrower rdf:resource="http://www.usgs.gov/science/USGSThesaurus/oxygen%20isotope%20analysis"/>
    <skos:narrower rdf:resource="http://www.usgs.gov/science/USGSThesaurus/tritium%20analysis"/>
    <skos:related rdf:resource="http://www.usgs.gov/science/USGSThesaurus/biochemistry"/>
    <skos:related rdf:resource="http://www.usgs.gov/science/USGSThesaurus/geochemistry"/>
    <skos:inScheme rdf:resource="http://www.usgs.gov/science/USGSThesaurus"/>
  </rdf:Description>
  <rdf:Description about="http://www.usgs.gov/science/USGSThesaurus/beryllium%20isotope%20analysis">
    <rdf:type rdf:resource="http://www.w3.org/2004/02/skos/core#Concept"/>
    <skos:prefLabel xml:lang="en">beryllium isotope analysis</skos:prefLabel>
    <skos:scopeNote xml:lang="en">Method of age determination based on measurement of the activity of beryllium-10, used in dating deep-sea sediments, and in determining sedimentation rates.</skos:scopeNote>
    <skos:broader rdf:resource="http://www.usgs.gov/science/USGSThesaurus/light%20stable%20isotope%20analysis"/>
    <skos:inScheme rdf:resource="http://www.usgs.gov/science/USGSThesaurus"/>
  </rdf:Description>
  <rdf:Description about="http://www.usgs.gov/science/USGSThesaurus/carbon%20isotope%20analysis">
    <rdf:type rdf:resource="http://www.w3.org/2004/02/skos/core#Concept"/>
    <skos:prefLabel xml:lang="en">carbon isotope analysis</skos:prefLabel>
    <skos:scopeNote xml:lang="en">Experimental determination of the proportion of a given stable carbon isotope (C12 or C13) in a sample.</skos:scopeNote>
    <skos:broader rdf:resource="http://www.usgs.gov/science/USGSThesaurus/light%20stable%20isotope%20analysis"/>
    <skos:related rdf:resource="http://www.usgs.gov/science/USGSThesaurus/biochemistry"/>
    <skos:related rdf:resource="http://www.usgs.gov/science/USGSThesaurus/carbon-14%20analysis"/>
    <skos:related rdf:resource="http://www.usgs.gov/science/USGSThesaurus/geochemistry"/>
    <skos:inScheme rdf:resource="http://www.usgs.gov/science/USGSThesaurus"/>
  </rdf:Description>
  <rdf:Description about="http://www.usgs.gov/science/USGSThesaurus/oxygen%20isotope%20analysis">
    <rdf:type rdf:resource="http://www.w3.org/2004/02/skos/core#Concept"/>
    <skos:prefLabel xml:lang="en">oxygen isotope analysis</skos:prefLabel>
    <skos:scopeNote xml:lang="en">Experimental determination of the proportion of a given stable oxygen isotope in a sample.</skos:scopeNote>
    <skos:broader rdf:resource="http://www.usgs.gov/science/USGSThesaurus/light%20stable%20isotope%20analysis"/>
    <skos:related rdf:resource="http://www.usgs.gov/science/USGSThesaurus/biochemistry"/>
    <skos:related rdf:resource="http://www.usgs.gov/science/USGSThesaurus/geochemistry"/>
    <skos:inScheme rdf:resource="http://www.usgs.gov/science/USGSThesaurus"/>
  </rdf:Description>
  <rdf:Description about="http://www.usgs.gov/science/USGSThesaurus/tritium%20analysis">
    <rdf:type rdf:resource="http://www.w3.org/2004/02/skos/core#Concept"/>
    <skos:prefLabel xml:lang="en">tritium analysis</skos:prefLabel>
    <skos:scopeNote xml:lang="en">Mass spectrometric measurement of the decay of the radioactive isotope of hydrogen in water samples as a means of dating and investigating changes in water.</skos:scopeNote>
    <skos:altLabel xml:lang="en">tritium-helium dating</skos:altLabel>
    <skos:broader rdf:resource="http://www.usgs.gov/science/USGSThesaurus/light%20stable%20isotope%20analysis"/>
    <skos:related rdf:resource="http://www.usgs.gov/science/USGSThesaurus/biochemistry"/>
    <skos:related rdf:resource="http://www.usgs.gov/science/USGSThesaurus/geochemistry"/>
    <skos:inScheme rdf:resource="http://www.usgs.gov/science/USGSThesaurus"/>
  </rdf:Description>
  <rdf:Description about="http://www.usgs.gov/science/USGSThesaurus/radiometric%20dating">
    <rdf:type rdf:resource="http://www.w3.org/2004/02/skos/core#Concept"/>
    <skos:prefLabel xml:lang="en">radiometric dating</skos:prefLabel>
    <skos:scopeNote xml:lang="en">Methods for age determination of rocks and fossils by measuring the proportions of naturally occurring radioactive isotopes to their decay products.</skos:scopeNote>
    <skos:altLabel xml:lang="en">age dating (radiometric)</skos:altLabel>
    <skos:altLabel xml:lang="en">argon-argon dating</skos:altLabel>
    <skos:altLabel xml:lang="en">lead-210 dating</skos:altLabel>
    <skos:altLabel xml:lang="en">radiometric age determination</skos:altLabel>
    <skos:broader rdf:resource="http://www.usgs.gov/science/USGSThesaurus/isotopic%20analysis"/>
    <skos:narrower rdf:resource="http://www.usgs.gov/science/USGSThesaurus/carbon-14%20analysis"/>
    <skos:narrower rdf:resource="http://www.usgs.gov/science/USGSThesaurus/potassium-argon%20analysis"/>
    <skos:narrower rdf:resource="http://www.usgs.gov/science/USGSThesaurus/rubidium-strontium%20analysis"/>
    <skos:narrower rdf:resource="http://www.usgs.gov/science/USGSThesaurus/uranium-lead%20analysis"/>
    <skos:narrower rdf:resource="http://www.usgs.gov/science/USGSThesaurus/uranium-thorium%20analysis"/>
    <skos:related rdf:resource="http://www.usgs.gov/science/USGSThesaurus/fission-track%20dating"/>
    <skos:related rdf:resource="http://www.usgs.gov/science/USGSThesaurus/geochronology"/>
    <skos:related rdf:resource="http://www.usgs.gov/science/USGSThesaurus/age%20estimation%20methods"/>
    <skos:inScheme rdf:resource="http://www.usgs.gov/science/USGSThesaurus"/>
  </rdf:Description>
  <rdf:Description about="http://www.usgs.gov/science/USGSThesaurus/carbon-14%20analysis">
    <rdf:type rdf:resource="http://www.w3.org/2004/02/skos/core#Concept"/>
    <skos:prefLabel xml:lang="en">carbon-14 analysis</skos:prefLabel>
    <skos:scopeNote xml:lang="en">Method to determine the age of organic geologic and archaeological specimens, aged approximately 3,000 to 50,000 years, by determining the decay of the radioactive isotope carbon-14.</skos:scopeNote>
    <skos:altLabel xml:lang="en">carbon dating</skos:altLabel>
    <skos:altLabel xml:lang="en">radiocarbon dating</skos:altLabel>
    <skos:broader rdf:resource="http://www.usgs.gov/science/USGSThesaurus/radiometric%20dating"/>
    <skos:related rdf:resource="http://www.usgs.gov/science/USGSThesaurus/carbon%20isotope%20analysis"/>
    <skos:related rdf:resource="http://www.usgs.gov/science/USGSThesaurus/geochronology"/>
    <skos:inScheme rdf:resource="http://www.usgs.gov/science/USGSThesaurus"/>
  </rdf:Description>
  <rdf:Description about="http://www.usgs.gov/science/USGSThesaurus/potassium-argon%20analysis">
    <rdf:type rdf:resource="http://www.w3.org/2004/02/skos/core#Concept"/>
    <skos:prefLabel xml:lang="en">potassium-argon analysis</skos:prefLabel>
    <skos:scopeNote xml:lang="en">Radiometric age determination by comparison of the concentrations of radioactive potassium and argon daughter products.</skos:scopeNote>
    <skos:altLabel xml:lang="en">K-Ar dating</skos:altLabel>
    <skos:broader rdf:resource="http://www.usgs.gov/science/USGSThesaurus/radiometric%20dating"/>
    <skos:inScheme rdf:resource="http://www.usgs.gov/science/USGSThesaurus"/>
  </rdf:Description>
  <rdf:Description about="http://www.usgs.gov/science/USGSThesaurus/rubidium-strontium%20analysis">
    <rdf:type rdf:resource="http://www.w3.org/2004/02/skos/core#Concept"/>
    <skos:prefLabel xml:lang="en">rubidium-strontium analysis</skos:prefLabel>
    <skos:scopeNote xml:lang="en">Technique for dating ancient rocks based on measuring the ratio of the isotopes strontium-87 to ribidium-87 in samples. Uses the known half-life of radioactive isotopes of rubidium-87 that decay to isotopes of strontium-87 to determine rock ages.</skos:scopeNote>
    <skos:altLabel xml:lang="en">Rb-Sr age analysis</skos:altLabel>
    <skos:broader rdf:resource="http://www.usgs.gov/science/USGSThesaurus/radiometric%20dating"/>
    <skos:related rdf:resource="http://www.usgs.gov/science/USGSThesaurus/geochronology"/>
    <skos:inScheme rdf:resource="http://www.usgs.gov/science/USGSThesaurus"/>
  </rdf:Description>
  <rdf:Description about="http://www.usgs.gov/science/USGSThesaurus/uranium-lead%20analysis">
    <rdf:type rdf:resource="http://www.w3.org/2004/02/skos/core#Concept"/>
    <skos:prefLabel xml:lang="en">uranium-lead analysis</skos:prefLabel>
    <skos:scopeNote xml:lang="en">Radiometric dating technique to determine the age of earth materials from the ratio of the radioactive isotopes of uranium-235 or uranium-238 to the lead isotope decay products in the sample. The ratio is compared to the known half-life of the uranium isotopes.</skos:scopeNote>
    <skos:broader rdf:resource="http://www.usgs.gov/science/USGSThesaurus/radiometric%20dating"/>
    <skos:related rdf:resource="http://www.usgs.gov/science/USGSThesaurus/geochronology"/>
    <skos:inScheme rdf:resource="http://www.usgs.gov/science/USGSThesaurus"/>
  </rdf:Description>
  <rdf:Description about="http://www.usgs.gov/science/USGSThesaurus/uranium-thorium%20analysis">
    <rdf:type rdf:resource="http://www.w3.org/2004/02/skos/core#Concept"/>
    <skos:prefLabel xml:lang="en">uranium-thorium analysis</skos:prefLabel>
    <skos:scopeNote xml:lang="en">Radiometric dating technique used to determine the age of earth materials based on determining the ratio of uranium-238 to the decay product thorium-230. The ratio is compared to the known half-life of the uranium isotope.</skos:scopeNote>
    <skos:broader rdf:resource="http://www.usgs.gov/science/USGSThesaurus/radiometric%20dating"/>
    <skos:related rdf:resource="http://www.usgs.gov/science/USGSThesaurus/geochronology"/>
    <skos:inScheme rdf:resource="http://www.usgs.gov/science/USGSThesaurus"/>
  </rdf:Description>
  <rdf:Description about="http://www.usgs.gov/science/USGSThesaurus/meristics">
    <rdf:type rdf:resource="http://www.w3.org/2004/02/skos/core#Concept"/>
    <skos:prefLabel xml:lang="en">meristics</skos:prefLabel>
    <skos:scopeNote xml:lang="en">Branch of zoology concerned with classifying animals by counting and measuring body parts.</skos:scopeNote>
    <skos:altLabel xml:lang="en">morphometrics</skos:altLabel>
    <skos:broader rdf:resource="http://www.usgs.gov/science/USGSThesaurus/laboratory%20methods"/>
    <skos:related rdf:resource="http://www.usgs.gov/science/USGSThesaurus/morphology%20%28biological%29"/>
    <skos:related rdf:resource="http://www.usgs.gov/science/USGSThesaurus/systematics%20and%20taxonomy"/>
    <skos:inScheme rdf:resource="http://www.usgs.gov/science/USGSThesaurus"/>
  </rdf:Description>
  <rdf:Description about="http://www.usgs.gov/science/USGSThesaurus/microscopy">
    <rdf:type rdf:resource="http://www.w3.org/2004/02/skos/core#Concept"/>
    <skos:prefLabel xml:lang="en">microscopy</skos:prefLabel>
    <skos:scopeNote xml:lang="en">Laboratory methods using instruments that employ optical lenses or radiation to study objects too small to be seen by the naked eye.</skos:scopeNote>
    <skos:altLabel xml:lang="en">microscope methods</skos:altLabel>
    <skos:broader rdf:resource="http://www.usgs.gov/science/USGSThesaurus/laboratory%20methods"/>
    <skos:narrower rdf:resource="http://www.usgs.gov/science/USGSThesaurus/electron%20microscopy"/>
    <skos:narrower rdf:resource="http://www.usgs.gov/science/USGSThesaurus/optical%20microscopy"/>
    <skos:related rdf:resource="http://www.usgs.gov/science/USGSThesaurus/faunal%20and%20floral%20census%20%28microscopic%29"/>
    <skos:inScheme rdf:resource="http://www.usgs.gov/science/USGSThesaurus"/>
  </rdf:Description>
  <rdf:Description about="http://www.usgs.gov/science/USGSThesaurus/electron%20microscopy">
    <rdf:type rdf:resource="http://www.w3.org/2004/02/skos/core#Concept"/>
    <skos:prefLabel xml:lang="en">electron microscopy</skos:prefLabel>
    <skos:scopeNote xml:lang="en">Study of small particles of matter with a microscope that produces a magnified image by using a beam of electrons focused by magnetic lenses.</skos:scopeNote>
    <skos:broader rdf:resource="http://www.usgs.gov/science/USGSThesaurus/microscopy"/>
    <skos:narrower rdf:resource="http://www.usgs.gov/science/USGSThesaurus/scanning%20electron%20microscopy"/>
    <skos:inScheme rdf:resource="http://www.usgs.gov/science/USGSThesaurus"/>
  </rdf:Description>
  <rdf:Description about="http://www.usgs.gov/science/USGSThesaurus/scanning%20electron%20microscopy">
    <rdf:type rdf:resource="http://www.w3.org/2004/02/skos/core#Concept"/>
    <skos:prefLabel xml:lang="en">scanning electron microscopy</skos:prefLabel>
    <skos:scopeNote xml:lang="en">Microscope in which a finely focused beam of electrons is scanned across a specimen. The electronic intensity variations observed are used to construct an image of the specimen.</skos:scopeNote>
    <skos:broader rdf:resource="http://www.usgs.gov/science/USGSThesaurus/electron%20microscopy"/>
    <skos:inScheme rdf:resource="http://www.usgs.gov/science/USGSThesaurus"/>
  </rdf:Description>
  <rdf:Description about="http://www.usgs.gov/science/USGSThesaurus/optical%20microscopy">
    <rdf:type rdf:resource="http://www.w3.org/2004/02/skos/core#Concept"/>
    <skos:prefLabel xml:lang="en">optical microscopy</skos:prefLabel>
    <skos:scopeNote xml:lang="en">Scientific techniques using a microscope with one or more lenses illuminated with visible light to view small objects.</skos:scopeNote>
    <skos:broader rdf:resource="http://www.usgs.gov/science/USGSThesaurus/microscopy"/>
    <skos:narrower rdf:resource="http://www.usgs.gov/science/USGSThesaurus/microtomy"/>
    <skos:related rdf:resource="http://www.usgs.gov/science/USGSThesaurus/petrography"/>
    <skos:inScheme rdf:resource="http://www.usgs.gov/science/USGSThesaurus"/>
  </rdf:Description>
  <rdf:Description about="http://www.usgs.gov/science/USGSThesaurus/microtomy">
    <rdf:type rdf:resource="http://www.w3.org/2004/02/skos/core#Concept"/>
    <skos:prefLabel xml:lang="en">microtomy</skos:prefLabel>
    <skos:scopeNote xml:lang="en">Laboratory methods using special instruments, or microtomes, to cut very thin slices of specimens for microscopic studies.</skos:scopeNote>
    <skos:broader rdf:resource="http://www.usgs.gov/science/USGSThesaurus/optical%20microscopy"/>
    <skos:inScheme rdf:resource="http://www.usgs.gov/science/USGSThesaurus"/>
  </rdf:Description>
  <rdf:Description about="http://www.usgs.gov/science/USGSThesaurus/paleomagnetic%20analysis">
    <rdf:type rdf:resource="http://www.w3.org/2004/02/skos/core#Concept"/>
    <skos:prefLabel xml:lang="en">paleomagnetic analysis</skos:prefLabel>
    <skos:scopeNote xml:lang="en">Determination of the intensity and direction of residual magnetism in rocks to study changes in the earth's magnetic field during past geologic time.</skos:scopeNote>
    <skos:broader rdf:resource="http://www.usgs.gov/science/USGSThesaurus/laboratory%20methods"/>
    <skos:narrower rdf:resource="http://www.usgs.gov/science/USGSThesaurus/Curie%20temperature%20analysis"/>
    <skos:narrower rdf:resource="http://www.usgs.gov/science/USGSThesaurus/laboratory-induced%20magnetization%20analysis"/>
    <skos:narrower rdf:resource="http://www.usgs.gov/science/USGSThesaurus/magnetic%20hysteresis%20analysis"/>
    <skos:narrower rdf:resource="http://www.usgs.gov/science/USGSThesaurus/magnetic%20susceptibility%20analysis"/>
    <skos:narrower rdf:resource="http://www.usgs.gov/science/USGSThesaurus/natural%20remanent%20magnetization%20analysis"/>
    <skos:related rdf:resource="http://www.usgs.gov/science/USGSThesaurus/geophysics"/>
    <skos:inScheme rdf:resource="http://www.usgs.gov/science/USGSThesaurus"/>
  </rdf:Description>
  <rdf:Description about="http://www.usgs.gov/science/USGSThesaurus/Curie%20temperature%20analysis">
    <rdf:type rdf:resource="http://www.w3.org/2004/02/skos/core#Concept"/>
    <skos:prefLabel xml:lang="en">Curie temperature analysis</skos:prefLabel>
    <skos:scopeNote xml:lang="en">Analysis of rock specimens using the Curie temperature point above which ferromagnetic materials lose permanent magnetism.</skos:scopeNote>
    <skos:altLabel xml:lang="en">temperature analysis (Curie)</skos:altLabel>
    <skos:broader rdf:resource="http://www.usgs.gov/science/USGSThesaurus/paleomagnetic%20analysis"/>
    <skos:related rdf:resource="http://www.usgs.gov/science/USGSThesaurus/geophysics"/>
    <skos:inScheme rdf:resource="http://www.usgs.gov/science/USGSThesaurus"/>
  </rdf:Description>
  <rdf:Description about="http://www.usgs.gov/science/USGSThesaurus/laboratory-induced%20magnetization%20analysis">
    <rdf:type rdf:resource="http://www.w3.org/2004/02/skos/core#Concept"/>
    <skos:prefLabel xml:lang="en">laboratory-induced magnetization analysis</skos:prefLabel>
    <skos:scopeNote xml:lang="en">Laboratory method to study rocks using magnetometers to measure remanent magnetic fields induced in the samples.</skos:scopeNote>
    <skos:broader rdf:resource="http://www.usgs.gov/science/USGSThesaurus/paleomagnetic%20analysis"/>
    <skos:related rdf:resource="http://www.usgs.gov/science/USGSThesaurus/geophysics"/>
    <skos:inScheme rdf:resource="http://www.usgs.gov/science/USGSThesaurus"/>
  </rdf:Description>
  <rdf:Description about="http://www.usgs.gov/science/USGSThesaurus/magnetic%20hysteresis%20analysis">
    <rdf:type rdf:resource="http://www.w3.org/2004/02/skos/core#Concept"/>
    <skos:prefLabel xml:lang="en">magnetic hysteresis analysis</skos:prefLabel>
    <skos:scopeNote xml:lang="en">Nondestructive evaluation of ferromagnetic materials.  The evaluation is based on measurement of the variation of intensity of magnetization within an applied magnetic field due to changes in the magnetic domain structure of the materials under study.</skos:scopeNote>
    <skos:altLabel xml:lang="en">hysteresis</skos:altLabel>
    <skos:broader rdf:resource="http://www.usgs.gov/science/USGSThesaurus/paleomagnetic%20analysis"/>
    <skos:related rdf:resource="http://www.usgs.gov/science/USGSThesaurus/geophysics"/>
    <skos:inScheme rdf:resource="http://www.usgs.gov/science/USGSThesaurus"/>
  </rdf:Description>
  <rdf:Description about="http://www.usgs.gov/science/USGSThesaurus/magnetic%20susceptibility%20analysis">
    <rdf:type rdf:resource="http://www.w3.org/2004/02/skos/core#Concept"/>
    <skos:prefLabel xml:lang="en">magnetic susceptibility analysis</skos:prefLabel>
    <skos:scopeNote xml:lang="en">Nondestructive evaluation and location of magnetic materials in rock based on measuring the intensity of attraction of the materials to an induced magnetic field. Applications include geological and soil surveys, paleomagnetic studies, sedimentology, archaeological prospecting and core logging.</skos:scopeNote>
    <skos:broader rdf:resource="http://www.usgs.gov/science/USGSThesaurus/paleomagnetic%20analysis"/>
    <skos:related rdf:resource="http://www.usgs.gov/science/USGSThesaurus/geophysics"/>
    <skos:inScheme rdf:resource="http://www.usgs.gov/science/USGSThesaurus"/>
  </rdf:Description>
  <rdf:Description about="http://www.usgs.gov/science/USGSThesaurus/natural%20remanent%20magnetization%20analysis">
    <rdf:type rdf:resource="http://www.w3.org/2004/02/skos/core#Concept"/>
    <skos:prefLabel xml:lang="en">natural remanent magnetization analysis</skos:prefLabel>
    <skos:scopeNote xml:lang="en">Method which measures the intensity and direction of residual magnetism in rocks to determine their age and history.</skos:scopeNote>
    <skos:altLabel xml:lang="en">natural remnant magnetization analysis</skos:altLabel>
    <skos:broader rdf:resource="http://www.usgs.gov/science/USGSThesaurus/paleomagnetic%20analysis"/>
    <skos:related rdf:resource="http://www.usgs.gov/science/USGSThesaurus/geophysics"/>
    <skos:inScheme rdf:resource="http://www.usgs.gov/science/USGSThesaurus"/>
  </rdf:Description>
  <rdf:Description about="http://www.usgs.gov/science/USGSThesaurus/petrography">
    <rdf:type rdf:resource="http://www.w3.org/2004/02/skos/core#Concept"/>
    <skos:prefLabel xml:lang="en">petrography</skos:prefLabel>
    <skos:scopeNote xml:lang="en">Use of optical microscopy for the description and classification of rocks.</skos:scopeNote>
    <skos:altLabel xml:lang="en">thin section analysis</skos:altLabel>
    <skos:broader rdf:resource="http://www.usgs.gov/science/USGSThesaurus/laboratory%20methods"/>
    <skos:related rdf:resource="http://www.usgs.gov/science/USGSThesaurus/optical%20microscopy"/>
    <skos:related rdf:resource="http://www.usgs.gov/science/USGSThesaurus/petrology"/>
    <skos:related rdf:resource="http://www.usgs.gov/science/USGSThesaurus/rocks%20and%20deposits"/>
    <skos:inScheme rdf:resource="http://www.usgs.gov/science/USGSThesaurus"/>
  </rdf:Description>
  <rdf:Description about="http://www.usgs.gov/science/USGSThesaurus/plant%20and%20animal%20testing">
    <rdf:type rdf:resource="http://www.w3.org/2004/02/skos/core#Concept"/>
    <skos:prefLabel xml:lang="en">plant and animal testing</skos:prefLabel>
    <skos:scopeNote xml:lang="en">Use of live or dead organisms for scientific study.</skos:scopeNote>
    <skos:altLabel xml:lang="en">animal testing</skos:altLabel>
    <skos:broader rdf:resource="http://www.usgs.gov/science/USGSThesaurus/laboratory%20methods"/>
    <skos:related rdf:resource="http://www.usgs.gov/science/USGSThesaurus/anatomy%20and%20physiology"/>
    <skos:related rdf:resource="http://www.usgs.gov/science/USGSThesaurus/ecotoxicology"/>
    <skos:related rdf:resource="http://www.usgs.gov/science/USGSThesaurus/pathology"/>
    <skos:inScheme rdf:resource="http://www.usgs.gov/science/USGSThesaurus"/>
  </rdf:Description>
  <rdf:Description about="http://www.usgs.gov/science/USGSThesaurus/subsampling">
    <rdf:type rdf:resource="http://www.w3.org/2004/02/skos/core#Concept"/>
    <skos:prefLabel xml:lang="en">subsampling</skos:prefLabel>
    <skos:scopeNote xml:lang="en">Preparation of study materials by dividing or slicing cores, samples, or other collected materials.</skos:scopeNote>
    <skos:altLabel xml:lang="en">thin sectioning</skos:altLabel>
    <skos:broader rdf:resource="http://www.usgs.gov/science/USGSThesaurus/laboratory%20methods"/>
    <skos:inScheme rdf:resource="http://www.usgs.gov/science/USGSThesaurus"/>
  </rdf:Description>
  <rdf:Description about="http://www.usgs.gov/science/USGSThesaurus/therapeutic%20methods">
    <rdf:type rdf:resource="http://www.w3.org/2004/02/skos/core#Concept"/>
    <skos:prefLabel xml:lang="en">therapeutic methods</skos:prefLabel>
    <skos:scopeNote xml:lang="en">Methods of  restoring health with remedial agents or treatments.</skos:scopeNote>
    <skos:broader rdf:resource="http://www.usgs.gov/science/USGSThesaurus/laboratory%20methods"/>
    <skos:related rdf:resource="http://www.usgs.gov/science/USGSThesaurus/anatomy%20and%20physiology"/>
    <skos:related rdf:resource="http://www.usgs.gov/science/USGSThesaurus/ecotoxicology"/>
    <skos:related rdf:resource="http://www.usgs.gov/science/USGSThesaurus/pathology"/>
    <skos:inScheme rdf:resource="http://www.usgs.gov/science/USGSThesaurus"/>
  </rdf:Description>
  <rdf:Description about="http://www.usgs.gov/science/USGSThesaurus/tree%20ring%20analysis">
    <rdf:type rdf:resource="http://www.w3.org/2004/02/skos/core#Concept"/>
    <skos:prefLabel xml:lang="en">tree ring analysis</skos:prefLabel>
    <skos:scopeNote xml:lang="en">Study of the variations in width and number of tree rings to date historical events and to study periods of climatic and hydrologic changes.</skos:scopeNote>
    <skos:altLabel xml:lang="en">age dating (tree ring)</skos:altLabel>
    <skos:broader rdf:resource="http://www.usgs.gov/science/USGSThesaurus/laboratory%20methods"/>
    <skos:related rdf:resource="http://www.usgs.gov/science/USGSThesaurus/geochronology"/>
    <skos:related rdf:resource="http://www.usgs.gov/science/USGSThesaurus/age%20estimation%20methods"/>
    <skos:inScheme rdf:resource="http://www.usgs.gov/science/USGSThesaurus"/>
  </rdf:Description>
  <rdf:Description about="http://www.usgs.gov/science/USGSThesaurus/management%20methods">
    <rdf:type rdf:resource="http://www.w3.org/2004/02/skos/core#Concept"/>
    <skos:prefLabel xml:lang="en">management methods</skos:prefLabel>
    <skos:scopeNote xml:lang="en">Techniques of judiciously controlling or directing resources for a predetermined goal.</skos:scopeNote>
    <skos:broader rdf:resource="http://www.usgs.gov/science/USGSThesaurus/methods"/>
    <skos:narrower rdf:resource="http://www.usgs.gov/science/USGSThesaurus/decision%20support%20methods"/>
    <skos:narrower rdf:resource="http://www.usgs.gov/science/USGSThesaurus/environmental%20assessment"/>
    <skos:narrower rdf:resource="http://www.usgs.gov/science/USGSThesaurus/hazard%20preparedness"/>
    <skos:narrower rdf:resource="http://www.usgs.gov/science/USGSThesaurus/information%20technology%20methods"/>
    <skos:narrower rdf:resource="http://www.usgs.gov/science/USGSThesaurus/mitigation%20of%20coastal%20hazards"/>
    <skos:narrower rdf:resource="http://www.usgs.gov/science/USGSThesaurus/natural%20resource%20management"/>
    <skos:narrower rdf:resource="http://www.usgs.gov/science/USGSThesaurus/risk%20assessment"/>
    <skos:inScheme rdf:resource="http://www.usgs.gov/science/USGSThesaurus"/>
  </rdf:Description>
  <rdf:Description about="http://www.usgs.gov/science/USGSThesaurus/decision%20support%20methods">
    <rdf:type rdf:resource="http://www.w3.org/2004/02/skos/core#Concept"/>
    <skos:prefLabel xml:lang="en">decision support methods</skos:prefLabel>
    <skos:scopeNote xml:lang="en">Mathematical, analytical, and social procedures used to aid groups and individuals in the process of making decisions.  Includes protocols for discussion and mechanisms for facilitating communication among disparate groups as well as mechanical and technological aids to analysis and understanding.</skos:scopeNote>
    <skos:altLabel xml:lang="en">conflict resolution methods</skos:altLabel>
    <skos:broader rdf:resource="http://www.usgs.gov/science/USGSThesaurus/management%20methods"/>
    <skos:narrower rdf:resource="http://www.usgs.gov/science/USGSThesaurus/ecosystem%20services%20valuation"/>
    <skos:related rdf:resource="http://www.usgs.gov/science/USGSThesaurus/geographic%20information%20systems"/>
    <skos:inScheme rdf:resource="http://www.usgs.gov/science/USGSThesaurus"/>
  </rdf:Description>
  <rdf:Description about="http://www.usgs.gov/science/USGSThesaurus/ecosystem%20services%20valuation">
    <rdf:type rdf:resource="http://www.w3.org/2004/02/skos/core#Concept"/>
    <skos:prefLabel xml:lang="en">ecosystem services valuation</skos:prefLabel>
    <skos:scopeNote xml:lang="en">Assessment of the value of ecosystem functions in supporting, sustaining, or enriching life.</skos:scopeNote>
    <skos:broader rdf:resource="http://www.usgs.gov/science/USGSThesaurus/decision%20support%20methods"/>
    <skos:related rdf:resource="http://www.usgs.gov/science/USGSThesaurus/ecosystem%20functions"/>
    <skos:related rdf:resource="http://www.usgs.gov/science/USGSThesaurus/ecosystem%20management"/>
    <skos:related rdf:resource="http://www.usgs.gov/science/USGSThesaurus/ecosystems"/>
    <skos:inScheme rdf:resource="http://www.usgs.gov/science/USGSThesaurus"/>
  </rdf:Description>
  <rdf:Description about="http://www.usgs.gov/science/USGSThesaurus/environmental%20assessment">
    <rdf:type rdf:resource="http://www.w3.org/2004/02/skos/core#Concept"/>
    <skos:prefLabel xml:lang="en">environmental assessment</skos:prefLabel>
    <skos:scopeNote xml:lang="en">The evaluation of the status of a specific ecosystem or geographic area and how a proposed change in management or a proposed project will affect that status.</skos:scopeNote>
    <skos:altLabel xml:lang="en">environmental analysis</skos:altLabel>
    <skos:altLabel xml:lang="en">environmental impact assessment</skos:altLabel>
    <skos:broader rdf:resource="http://www.usgs.gov/science/USGSThesaurus/management%20methods"/>
    <skos:narrower rdf:resource="http://www.usgs.gov/science/USGSThesaurus/TMDL"/>
    <skos:inScheme rdf:resource="http://www.usgs.gov/science/USGSThesaurus"/>
  </rdf:Description>
  <rdf:Description about="http://www.usgs.gov/science/USGSThesaurus/TMDL">
    <rdf:type rdf:resource="http://www.w3.org/2004/02/skos/core#Concept"/>
    <skos:prefLabel xml:lang="en">TMDL</skos:prefLabel>
    <skos:scopeNote xml:lang="en">A calculation of the maximum amount of a pollutant that a waterbody can receive and still meet water-quality standards.</skos:scopeNote>
    <skos:altLabel xml:lang="en">total maximum daily load</skos:altLabel>
    <skos:broader rdf:resource="http://www.usgs.gov/science/USGSThesaurus/environmental%20assessment"/>
    <skos:inScheme rdf:resource="http://www.usgs.gov/science/USGSThesaurus"/>
  </rdf:Description>
  <rdf:Description about="http://www.usgs.gov/science/USGSThesaurus/hazard%20preparedness">
    <rdf:type rdf:resource="http://www.w3.org/2004/02/skos/core#Concept"/>
    <skos:prefLabel xml:lang="en">hazard preparedness</skos:prefLabel>
    <skos:scopeNote xml:lang="en">Awareness of the consequences of hazards and actions to be taken before, during, or after hazards occur or are encountered.</skos:scopeNote>
    <skos:altLabel xml:lang="en">early warning systems</skos:altLabel>
    <skos:altLabel xml:lang="en">emergency response planning</skos:altLabel>
    <!--FOR fire preparedness USE hazard preparedness WITH fires-->
    <skos:altLabel xml:lang="en">fire preparedness</skos:altLabel>
    <!--FOR flood preparedness USE hazard preparedness WITH floods-->
    <skos:altLabel xml:lang="en">flood preparedness</skos:altLabel>
    <!--FOR landslide preparedness USE hazard preparedness WITH landslides-->
    <skos:altLabel xml:lang="en">landslide preparedness</skos:altLabel>
    <!--FOR tsunami preparedness USE hazard preparedness WITH tsunamis-->
    <skos:altLabel xml:lang="en">tsunami preparedness</skos:altLabel>
    <skos:broader rdf:resource="http://www.usgs.gov/science/USGSThesaurus/management%20methods"/>
    <skos:narrower rdf:resource="http://www.usgs.gov/science/USGSThesaurus/aviation%20safety"/>
    <skos:narrower rdf:resource="http://www.usgs.gov/science/USGSThesaurus/earthquake%20preparedness"/>
    <skos:inScheme rdf:resource="http://www.usgs.gov/science/USGSThesaurus"/>
  </rdf:Description>
  <rdf:Description about="http://www.usgs.gov/science/USGSThesaurus/aviation%20safety">
    <rdf:type rdf:resource="http://www.w3.org/2004/02/skos/core#Concept"/>
    <skos:prefLabel xml:lang="en">aviation safety</skos:prefLabel>
    <skos:scopeNote xml:lang="en">Effects on air transportation of natural hazards such as volcanic activity (ash plumes and volcanic clouds).</skos:scopeNote>
    <skos:broader rdf:resource="http://www.usgs.gov/science/USGSThesaurus/hazard%20preparedness"/>
    <skos:related rdf:resource="http://www.usgs.gov/science/USGSThesaurus/volcanic%20activity"/>
    <skos:inScheme rdf:resource="http://www.usgs.gov/science/USGSThesaurus"/>
  </rdf:Description>
  <rdf:Description about="http://www.usgs.gov/science/USGSThesaurus/earthquake%20preparedness">
    <rdf:type rdf:resource="http://www.w3.org/2004/02/skos/core#Concept"/>
    <skos:prefLabel xml:lang="en">earthquake preparedness</skos:prefLabel>
    <skos:scopeNote xml:lang="en">Awareness of the consequences of earthquake events and actions to be taken before, during, or after events.</skos:scopeNote>
    <skos:broader rdf:resource="http://www.usgs.gov/science/USGSThesaurus/hazard%20preparedness"/>
    <skos:inScheme rdf:resource="http://www.usgs.gov/science/USGSThesaurus"/>
  </rdf:Description>
  <rdf:Description about="http://www.usgs.gov/science/USGSThesaurus/information%20technology%20methods">
    <rdf:type rdf:resource="http://www.w3.org/2004/02/skos/core#Concept"/>
    <skos:prefLabel xml:lang="en">information technology methods</skos:prefLabel>
    <skos:scopeNote xml:lang="en">Information-related concerns on which people focus their work in support of scientific investigations and research.</skos:scopeNote>
    <skos:altLabel xml:lang="en">informatics activities</skos:altLabel>
    <skos:broader rdf:resource="http://www.usgs.gov/science/USGSThesaurus/management%20methods"/>
    <skos:narrower rdf:resource="http://www.usgs.gov/science/USGSThesaurus/data%20communication"/>
    <skos:narrower rdf:resource="http://www.usgs.gov/science/USGSThesaurus/data%20integration"/>
    <skos:narrower rdf:resource="http://www.usgs.gov/science/USGSThesaurus/data%20management"/>
    <skos:narrower rdf:resource="http://www.usgs.gov/science/USGSThesaurus/information%20system%20administration"/>
    <skos:narrower rdf:resource="http://www.usgs.gov/science/USGSThesaurus/software%20development"/>
    <skos:inScheme rdf:resource="http://www.usgs.gov/science/USGSThesaurus"/>
  </rdf:Description>
  <rdf:Description about="http://www.usgs.gov/science/USGSThesaurus/data%20communication">
    <rdf:type rdf:resource="http://www.w3.org/2004/02/skos/core#Concept"/>
    <skos:prefLabel xml:lang="en">data communication</skos:prefLabel>
    <skos:scopeNote xml:lang="en">Design, development, and deployment of methods to convey scientific information to potential users.</skos:scopeNote>
    <skos:broader rdf:resource="http://www.usgs.gov/science/USGSThesaurus/information%20technology%20methods"/>
    <skos:narrower rdf:resource="http://www.usgs.gov/science/USGSThesaurus/markup%20and%20query%20language%20development"/>
    <skos:narrower rdf:resource="http://www.usgs.gov/science/USGSThesaurus/social%20network%20development"/>
    <skos:narrower rdf:resource="http://www.usgs.gov/science/USGSThesaurus/web%20interface%20development"/>
    <skos:narrower rdf:resource="http://www.usgs.gov/science/USGSThesaurus/web%20service%20development"/>
    <skos:inScheme rdf:resource="http://www.usgs.gov/science/USGSThesaurus"/>
  </rdf:Description>
  <rdf:Description about="http://www.usgs.gov/science/USGSThesaurus/markup%20and%20query%20language%20development">
    <rdf:type rdf:resource="http://www.w3.org/2004/02/skos/core#Concept"/>
    <skos:prefLabel xml:lang="en">markup and query language development</skos:prefLabel>
    <skos:scopeNote xml:lang="en">Design of the structure and format of digital queries and responses concerning scientific data resources.  Refers to exchanges in which the structure and content of the queries is interpreted by software both when generated and when received.</skos:scopeNote>
    <skos:broader rdf:resource="http://www.usgs.gov/science/USGSThesaurus/data%20communication"/>
    <skos:inScheme rdf:resource="http://www.usgs.gov/science/USGSThesaurus"/>
  </rdf:Description>
  <rdf:Description about="http://www.usgs.gov/science/USGSThesaurus/social%20network%20development">
    <rdf:type rdf:resource="http://www.w3.org/2004/02/skos/core#Concept"/>
    <skos:prefLabel xml:lang="en">social network development</skos:prefLabel>
    <skos:scopeNote xml:lang="en">Design and use of software and interfaces that facilitate interchange of information among people or organizations that produce scientific data and the potential users of those data.  Primarily refers to interactive web interfaces and services that enable discussion, collaboration, and comment on the data.</skos:scopeNote>
    <skos:broader rdf:resource="http://www.usgs.gov/science/USGSThesaurus/data%20communication"/>
    <skos:inScheme rdf:resource="http://www.usgs.gov/science/USGSThesaurus"/>
  </rdf:Description>
  <rdf:Description about="http://www.usgs.gov/science/USGSThesaurus/web%20interface%20development">
    <rdf:type rdf:resource="http://www.w3.org/2004/02/skos/core#Concept"/>
    <skos:prefLabel xml:lang="en">web interface development</skos:prefLabel>
    <skos:scopeNote xml:lang="en">Design of user interfaces for scientific information that are accessed using web browser software.</skos:scopeNote>
    <skos:broader rdf:resource="http://www.usgs.gov/science/USGSThesaurus/data%20communication"/>
    <skos:narrower rdf:resource="http://www.usgs.gov/science/USGSThesaurus/data%20packaging"/>
    <skos:inScheme rdf:resource="http://www.usgs.gov/science/USGSThesaurus"/>
  </rdf:Description>
  <rdf:Description about="http://www.usgs.gov/science/USGSThesaurus/data%20packaging">
    <rdf:type rdf:resource="http://www.w3.org/2004/02/skos/core#Concept"/>
    <skos:prefLabel xml:lang="en">data packaging</skos:prefLabel>
    <skos:scopeNote xml:lang="en">Design of the structure, format, and arrangement of scientific data in digital files in order to facilitate their transfer and effective use by people and organizations other than the originators.</skos:scopeNote>
    <skos:broader rdf:resource="http://www.usgs.gov/science/USGSThesaurus/web%20interface%20development"/>
    <skos:related rdf:resource="http://www.usgs.gov/science/USGSThesaurus/improvement%20of%20scientific%20data%20usability"/>
    <skos:inScheme rdf:resource="http://www.usgs.gov/science/USGSThesaurus"/>
  </rdf:Description>
  <rdf:Description about="http://www.usgs.gov/science/USGSThesaurus/web%20service%20development">
    <rdf:type rdf:resource="http://www.w3.org/2004/02/skos/core#Concept"/>
    <skos:prefLabel xml:lang="en">web service development</skos:prefLabel>
    <skos:scopeNote xml:lang="en">Design and deployment of data services accessed using the hypertext transfer protocol.</skos:scopeNote>
    <skos:broader rdf:resource="http://www.usgs.gov/science/USGSThesaurus/data%20communication"/>
    <skos:inScheme rdf:resource="http://www.usgs.gov/science/USGSThesaurus"/>
  </rdf:Description>
  <rdf:Description about="http://www.usgs.gov/science/USGSThesaurus/data%20integration">
    <rdf:type rdf:resource="http://www.w3.org/2004/02/skos/core#Concept"/>
    <skos:prefLabel xml:lang="en">data integration</skos:prefLabel>
    <skos:scopeNote xml:lang="en">Strategies which, when implemented, enable disparate data to be combined in a single analysis.  Includes combination of similar data from small components into larger, coherent assemblages as well as recognizing and exploiting relationships linking or connecting data that are maintained separately.  May include efforts to make scientific information more easily found and obtained.</skos:scopeNote>
    <skos:broader rdf:resource="http://www.usgs.gov/science/USGSThesaurus/information%20technology%20methods"/>
    <skos:narrower rdf:resource="http://www.usgs.gov/science/USGSThesaurus/information%20architecture"/>
    <skos:narrower rdf:resource="http://www.usgs.gov/science/USGSThesaurus/knowledge%20organization%20system%20development"/>
    <skos:inScheme rdf:resource="http://www.usgs.gov/science/USGSThesaurus"/>
  </rdf:Description>
  <rdf:Description about="http://www.usgs.gov/science/USGSThesaurus/information%20architecture">
    <rdf:type rdf:resource="http://www.w3.org/2004/02/skos/core#Concept"/>
    <skos:prefLabel xml:lang="en">information architecture</skos:prefLabel>
    <skos:scopeNote xml:lang="en">Design of conceptual, logical, and physical information system components (both data and software) to support effective maintenance, integration, or use of the data.</skos:scopeNote>
    <skos:broader rdf:resource="http://www.usgs.gov/science/USGSThesaurus/data%20integration"/>
    <skos:inScheme rdf:resource="http://www.usgs.gov/science/USGSThesaurus"/>
  </rdf:Description>
  <rdf:Description about="http://www.usgs.gov/science/USGSThesaurus/knowledge%20organization%20system%20development">
    <rdf:type rdf:resource="http://www.w3.org/2004/02/skos/core#Concept"/>
    <skos:prefLabel xml:lang="en">knowledge organization system development</skos:prefLabel>
    <skos:scopeNote xml:lang="en">Design and development of information systems that represent and relate concepts needed to identify, specify, organize, categorize, or characterize scientific information effectively.  Includes development of controlled vocabularies as well as hierarchical and networked concept schemes such as thesauri and ontologies.</skos:scopeNote>
    <skos:altLabel xml:lang="en">ontology development</skos:altLabel>
    <skos:broader rdf:resource="http://www.usgs.gov/science/USGSThesaurus/data%20integration"/>
    <skos:inScheme rdf:resource="http://www.usgs.gov/science/USGSThesaurus"/>
  </rdf:Description>
  <rdf:Description about="http://www.usgs.gov/science/USGSThesaurus/data%20management">
    <rdf:type rdf:resource="http://www.w3.org/2004/02/skos/core#Concept"/>
    <skos:prefLabel xml:lang="en">data management</skos:prefLabel>
    <skos:scopeNote xml:lang="en">Activities focused on the creation, documentation, and preservation of scientific data with the intent that the data continue to be usable in the future.</skos:scopeNote>
    <skos:altLabel xml:lang="en">information management</skos:altLabel>
    <skos:altLabel xml:lang="en">knowledge management</skos:altLabel>
    <skos:altLabel xml:lang="en">collection management</skos:altLabel>
    <skos:altLabel xml:lang="en">data curation</skos:altLabel>
    <skos:altLabel xml:lang="en">digital curation</skos:altLabel>
    <skos:broader rdf:resource="http://www.usgs.gov/science/USGSThesaurus/information%20technology%20methods"/>
    <skos:narrower rdf:resource="http://www.usgs.gov/science/USGSThesaurus/data%20preservation"/>
    <skos:narrower rdf:resource="http://www.usgs.gov/science/USGSThesaurus/digitization"/>
    <skos:narrower rdf:resource="http://www.usgs.gov/science/USGSThesaurus/improvement%20of%20scientific%20data%20usability"/>
    <skos:narrower rdf:resource="http://www.usgs.gov/science/USGSThesaurus/metadata%20management"/>
    <skos:inScheme rdf:resource="http://www.usgs.gov/science/USGSThesaurus"/>
  </rdf:Description>
  <rdf:Description about="http://www.usgs.gov/science/USGSThesaurus/data%20preservation">
    <rdf:type rdf:resource="http://www.w3.org/2004/02/skos/core#Concept"/>
    <skos:prefLabel xml:lang="en">data preservation</skos:prefLabel>
    <skos:scopeNote xml:lang="en">Design, development, and implementation of methods for ensuring that scientific information remain accessible and usable despite changes in technology and strategic directions in the originating organzation.</skos:scopeNote>
    <skos:altLabel xml:lang="en">data archiving</skos:altLabel>
    <skos:broader rdf:resource="http://www.usgs.gov/science/USGSThesaurus/data%20management"/>
    <skos:narrower rdf:resource="http://www.usgs.gov/science/USGSThesaurus/data%20rescue"/>
    <skos:inScheme rdf:resource="http://www.usgs.gov/science/USGSThesaurus"/>
  </rdf:Description>
  <rdf:Description about="http://www.usgs.gov/science/USGSThesaurus/data%20rescue">
    <rdf:type rdf:resource="http://www.w3.org/2004/02/skos/core#Concept"/>
    <skos:prefLabel xml:lang="en">data rescue</skos:prefLabel>
    <skos:scopeNote xml:lang="en">Reduction of the risk that scientific information will be lost or become unusable in the future.  Includes copying data from unstable to stable media, conversion of data files from unusable to usable formats, and creation of metadata allowing further changes to the data and other characteristics to be documented.</skos:scopeNote>
    <skos:broader rdf:resource="http://www.usgs.gov/science/USGSThesaurus/data%20preservation"/>
    <skos:inScheme rdf:resource="http://www.usgs.gov/science/USGSThesaurus"/>
  </rdf:Description>
  <rdf:Description about="http://www.usgs.gov/science/USGSThesaurus/digitization">
    <rdf:type rdf:resource="http://www.w3.org/2004/02/skos/core#Concept"/>
    <skos:prefLabel xml:lang="en">digitization</skos:prefLabel>
    <skos:scopeNote xml:lang="en">Compilation in digital form of data previously presented in analog forms such as contours on paper maps, plots, or other graphical materials, so that the digital data produced approximates the scientific measurements used to create the original printed materials.</skos:scopeNote>
    <skos:altLabel xml:lang="en">digitizing</skos:altLabel>
    <skos:broader rdf:resource="http://www.usgs.gov/science/USGSThesaurus/data%20management"/>
    <skos:inScheme rdf:resource="http://www.usgs.gov/science/USGSThesaurus"/>
  </rdf:Description>
  <rdf:Description about="http://www.usgs.gov/science/USGSThesaurus/improvement%20of%20scientific%20data%20usability">
    <rdf:type rdf:resource="http://www.w3.org/2004/02/skos/core#Concept"/>
    <skos:prefLabel xml:lang="en">improvement of scientific data usability</skos:prefLabel>
    <skos:scopeNote xml:lang="en">Retrospective modification of the structure, format, packaging, or documentation of an existing scientific data resource to improve the likelihood of effective use of the data by individuals or organizations who did not create the data.</skos:scopeNote>
    <skos:altLabel xml:lang="en">redatafication</skos:altLabel>
    <skos:broader rdf:resource="http://www.usgs.gov/science/USGSThesaurus/data%20management"/>
    <skos:related rdf:resource="http://www.usgs.gov/science/USGSThesaurus/data%20packaging"/>
    <skos:inScheme rdf:resource="http://www.usgs.gov/science/USGSThesaurus"/>
  </rdf:Description>
  <rdf:Description about="http://www.usgs.gov/science/USGSThesaurus/metadata%20management">
    <rdf:type rdf:resource="http://www.w3.org/2004/02/skos/core#Concept"/>
    <skos:prefLabel xml:lang="en">metadata management</skos:prefLabel>
    <skos:scopeNote xml:lang="en">Curation and maintenance of the documentation for scientific information resources.  Includes editing the metadata to improve consistency, completeness, and correctness, and modification of the structure of the documentation to improve its effectiveness in actual use.</skos:scopeNote>
    <skos:broader rdf:resource="http://www.usgs.gov/science/USGSThesaurus/data%20management"/>
    <skos:inScheme rdf:resource="http://www.usgs.gov/science/USGSThesaurus"/>
  </rdf:Description>
  <rdf:Description about="http://www.usgs.gov/science/USGSThesaurus/information%20system%20administration">
    <rdf:type rdf:resource="http://www.w3.org/2004/02/skos/core#Concept"/>
    <skos:prefLabel xml:lang="en">information system administration</skos:prefLabel>
    <skos:scopeNote xml:lang="en">Design, deployment, and maintenance of computing systems that support creation, maintenance, and use of scientific information.</skos:scopeNote>
    <skos:broader rdf:resource="http://www.usgs.gov/science/USGSThesaurus/information%20technology%20methods"/>
    <skos:narrower rdf:resource="http://www.usgs.gov/science/USGSThesaurus/database%20administration"/>
    <skos:narrower rdf:resource="http://www.usgs.gov/science/USGSThesaurus/information%20system%20security"/>
    <skos:narrower rdf:resource="http://www.usgs.gov/science/USGSThesaurus/network%20administration"/>
    <skos:related rdf:resource="http://www.usgs.gov/science/USGSThesaurus/information%20system%20design%20and%20development"/>
    <skos:inScheme rdf:resource="http://www.usgs.gov/science/USGSThesaurus"/>
  </rdf:Description>
  <rdf:Description about="http://www.usgs.gov/science/USGSThesaurus/database%20administration">
    <rdf:type rdf:resource="http://www.w3.org/2004/02/skos/core#Concept"/>
    <skos:prefLabel xml:lang="en">database administration</skos:prefLabel>
    <skos:scopeNote xml:lang="en">Design and implementation of strategies for arranging information within database management systems (including but not restricted to relational database management systems) so that the integrity and consistency of the information supports its intended uses.</skos:scopeNote>
    <skos:broader rdf:resource="http://www.usgs.gov/science/USGSThesaurus/information%20system%20administration"/>
    <skos:inScheme rdf:resource="http://www.usgs.gov/science/USGSThesaurus"/>
  </rdf:Description>
  <rdf:Description about="http://www.usgs.gov/science/USGSThesaurus/information%20system%20security">
    <rdf:type rdf:resource="http://www.w3.org/2004/02/skos/core#Concept"/>
    <skos:prefLabel xml:lang="en">information system security</skos:prefLabel>
    <skos:scopeNote xml:lang="en">Methods for ensuring that information systems are used for their intended purpose by those entitled to use them and that the information they contain retains its integrity and, where appropriate, confidentiality.</skos:scopeNote>
    <skos:broader rdf:resource="http://www.usgs.gov/science/USGSThesaurus/information%20system%20administration"/>
    <skos:inScheme rdf:resource="http://www.usgs.gov/science/USGSThesaurus"/>
  </rdf:Description>
  <rdf:Description about="http://www.usgs.gov/science/USGSThesaurus/network%20administration">
    <rdf:type rdf:resource="http://www.w3.org/2004/02/skos/core#Concept"/>
    <skos:prefLabel xml:lang="en">network administration</skos:prefLabel>
    <skos:scopeNote xml:lang="en">Methods for ensuring that computers communicate effectively with one another and follow established standards and guidelines for ensuring integrity in exchanging information and efficiency in operation.</skos:scopeNote>
    <skos:broader rdf:resource="http://www.usgs.gov/science/USGSThesaurus/information%20system%20administration"/>
    <skos:inScheme rdf:resource="http://www.usgs.gov/science/USGSThesaurus"/>
  </rdf:Description>
  <rdf:Description about="http://www.usgs.gov/science/USGSThesaurus/software%20development">
    <rdf:type rdf:resource="http://www.w3.org/2004/02/skos/core#Concept"/>
    <skos:prefLabel xml:lang="en">software development</skos:prefLabel>
    <skos:scopeNote xml:lang="en">Design and development of procedures and instructions by which  information is modified or presented.</skos:scopeNote>
    <skos:altLabel xml:lang="en">programming</skos:altLabel>
    <skos:altLabel xml:lang="en">computer programming</skos:altLabel>
    <skos:altLabel xml:lang="en">application development</skos:altLabel>
    <skos:broader rdf:resource="http://www.usgs.gov/science/USGSThesaurus/information%20technology%20methods"/>
    <skos:related rdf:resource="http://www.usgs.gov/science/USGSThesaurus/scientific%20software"/>
    <skos:inScheme rdf:resource="http://www.usgs.gov/science/USGSThesaurus"/>
  </rdf:Description>
  <rdf:Description about="http://www.usgs.gov/science/USGSThesaurus/mitigation%20of%20coastal%20hazards">
    <rdf:type rdf:resource="http://www.w3.org/2004/02/skos/core#Concept"/>
    <skos:prefLabel xml:lang="en">mitigation of coastal hazards</skos:prefLabel>
    <skos:scopeNote xml:lang="en">Actions taken to reduce risk of physical disruption in coastal environments.</skos:scopeNote>
    <skos:broader rdf:resource="http://www.usgs.gov/science/USGSThesaurus/management%20methods"/>
    <skos:narrower rdf:resource="http://www.usgs.gov/science/USGSThesaurus/coastal%20infrastructure%20relocation"/>
    <skos:narrower rdf:resource="http://www.usgs.gov/science/USGSThesaurus/hard%20shoreline%20stabilization"/>
    <skos:narrower rdf:resource="http://www.usgs.gov/science/USGSThesaurus/soft%20shoreline%20stabilization"/>
    <skos:related rdf:resource="http://www.usgs.gov/science/USGSThesaurus/engineering%20geology"/>
    <skos:related rdf:resource="http://www.usgs.gov/science/USGSThesaurus/coastal%20processes"/>
    <skos:inScheme rdf:resource="http://www.usgs.gov/science/USGSThesaurus"/>
  </rdf:Description>
  <rdf:Description about="http://www.usgs.gov/science/USGSThesaurus/coastal%20infrastructure%20relocation">
    <rdf:type rdf:resource="http://www.w3.org/2004/02/skos/core#Concept"/>
    <skos:prefLabel xml:lang="en">coastal infrastructure relocation</skos:prefLabel>
    <skos:scopeNote xml:lang="en">Landward relocation of infrastructure to reduce the risk from coastal hazards.</skos:scopeNote>
    <skos:broader rdf:resource="http://www.usgs.gov/science/USGSThesaurus/mitigation%20of%20coastal%20hazards"/>
    <skos:inScheme rdf:resource="http://www.usgs.gov/science/USGSThesaurus"/>
  </rdf:Description>
  <rdf:Description about="http://www.usgs.gov/science/USGSThesaurus/hard%20shoreline%20stabilization">
    <rdf:type rdf:resource="http://www.w3.org/2004/02/skos/core#Concept"/>
    <skos:prefLabel xml:lang="en">hard shoreline stabilization</skos:prefLabel>
    <skos:scopeNote xml:lang="en">Use of engineered structures to armor or otherwise protect the shoreline against erosional agents such as waves and currents.  Includes breakwaters, bulkheads, seawalls, groins, jetties, and revetments.</skos:scopeNote>
    <skos:broader rdf:resource="http://www.usgs.gov/science/USGSThesaurus/mitigation%20of%20coastal%20hazards"/>
    <skos:inScheme rdf:resource="http://www.usgs.gov/science/USGSThesaurus"/>
  </rdf:Description>
  <rdf:Description about="http://www.usgs.gov/science/USGSThesaurus/soft%20shoreline%20stabilization">
    <rdf:type rdf:resource="http://www.w3.org/2004/02/skos/core#Concept"/>
    <skos:prefLabel xml:lang="en">soft shoreline stabilization</skos:prefLabel>
    <skos:scopeNote xml:lang="en">Mitigating coastal erosion by managing the sediment budget (for example, beach nourishment or sand bypassing) or restoring dunes and wetlands (for example, by planting erosion-resistant vegetation).</skos:scopeNote>
    <skos:broader rdf:resource="http://www.usgs.gov/science/USGSThesaurus/mitigation%20of%20coastal%20hazards"/>
    <skos:inScheme rdf:resource="http://www.usgs.gov/science/USGSThesaurus"/>
  </rdf:Description>
  <rdf:Description about="http://www.usgs.gov/science/USGSThesaurus/natural%20resource%20management">
    <rdf:type rdf:resource="http://www.w3.org/2004/02/skos/core#Concept"/>
    <skos:prefLabel xml:lang="en">natural resource management</skos:prefLabel>
    <skos:scopeNote xml:lang="en">Using a combination of techniques to control or direct the use of resources and limit population size to reach a predetermined goal, such as sustainability.</skos:scopeNote>
    <skos:altLabel xml:lang="en">conservation</skos:altLabel>
    <skos:altLabel xml:lang="en">environmental management</skos:altLabel>
    <skos:altLabel xml:lang="en">environmental planning</skos:altLabel>
    <skos:altLabel xml:lang="en">resource conservation</skos:altLabel>
    <skos:altLabel xml:lang="en">resource restoration</skos:altLabel>
    <skos:broader rdf:resource="http://www.usgs.gov/science/USGSThesaurus/management%20methods"/>
    <skos:narrower rdf:resource="http://www.usgs.gov/science/USGSThesaurus/beach%20nourishment"/>
    <skos:narrower rdf:resource="http://www.usgs.gov/science/USGSThesaurus/biological%20population%20management"/>
    <skos:narrower rdf:resource="http://www.usgs.gov/science/USGSThesaurus/controlled%20flooding"/>
    <skos:narrower rdf:resource="http://www.usgs.gov/science/USGSThesaurus/ecosystem%20management"/>
    <skos:narrower rdf:resource="http://www.usgs.gov/science/USGSThesaurus/fire%20control"/>
    <skos:narrower rdf:resource="http://www.usgs.gov/science/USGSThesaurus/natural%20resource%20assessment"/>
    <skos:narrower rdf:resource="http://www.usgs.gov/science/USGSThesaurus/remediation"/>
    <skos:narrower rdf:resource="http://www.usgs.gov/science/USGSThesaurus/water%20resource%20management"/>
    <skos:narrower rdf:resource="http://www.usgs.gov/science/USGSThesaurus/watershed%20management"/>
    <skos:related rdf:resource="http://www.usgs.gov/science/USGSThesaurus/ecosystem%20monitoring"/>
    <skos:related rdf:resource="http://www.usgs.gov/science/USGSThesaurus/natural%20resources"/>
    <skos:related rdf:resource="http://www.usgs.gov/science/USGSThesaurus/population%20and%20community%20ecology"/>
    <skos:inScheme rdf:resource="http://www.usgs.gov/science/USGSThesaurus"/>
  </rdf:Description>
  <rdf:Description about="http://www.usgs.gov/science/USGSThesaurus/beach%20nourishment">
    <rdf:type rdf:resource="http://www.w3.org/2004/02/skos/core#Concept"/>
    <skos:prefLabel xml:lang="en">beach nourishment</skos:prefLabel>
    <skos:scopeNote xml:lang="en">Transfer of sand from offshore areas to resupply beach areas that have been eroded.</skos:scopeNote>
    <skos:altLabel xml:lang="en">beach replenishment</skos:altLabel>
    <skos:broader rdf:resource="http://www.usgs.gov/science/USGSThesaurus/natural%20resource%20management"/>
    <skos:related rdf:resource="http://www.usgs.gov/science/USGSThesaurus/natural%20resource%20extraction"/>
    <skos:related rdf:resource="http://www.usgs.gov/science/USGSThesaurus/dredging"/>
    <skos:inScheme rdf:resource="http://www.usgs.gov/science/USGSThesaurus"/>
  </rdf:Description>
  <rdf:Description about="http://www.usgs.gov/science/USGSThesaurus/biological%20population%20management">
    <rdf:type rdf:resource="http://www.w3.org/2004/02/skos/core#Concept"/>
    <skos:prefLabel xml:lang="en">biological population management</skos:prefLabel>
    <skos:scopeNote xml:lang="en">Judicious means of controlling or directing numbers and life conditions of organisms living in a specific locality to achieve a selected goal.</skos:scopeNote>
    <!--FOR conservation genetics USE biological population management WITH genetic diversity-->
    <skos:altLabel xml:lang="en">conservation genetics</skos:altLabel>
    <skos:broader rdf:resource="http://www.usgs.gov/science/USGSThesaurus/natural%20resource%20management"/>
    <skos:narrower rdf:resource="http://www.usgs.gov/science/USGSThesaurus/fishery%20management"/>
    <skos:narrower rdf:resource="http://www.usgs.gov/science/USGSThesaurus/pest%20control"/>
    <skos:narrower rdf:resource="http://www.usgs.gov/science/USGSThesaurus/reintroduction%20%28organisms%29"/>
    <skos:narrower rdf:resource="http://www.usgs.gov/science/USGSThesaurus/wildlife%20population%20management"/>
    <skos:related rdf:resource="http://www.usgs.gov/science/USGSThesaurus/ecosystem%20monitoring"/>
    <skos:related rdf:resource="http://www.usgs.gov/science/USGSThesaurus/population%20and%20community%20ecology"/>
    <skos:inScheme rdf:resource="http://www.usgs.gov/science/USGSThesaurus"/>
  </rdf:Description>
  <rdf:Description about="http://www.usgs.gov/science/USGSThesaurus/fishery%20management">
    <rdf:type rdf:resource="http://www.w3.org/2004/02/skos/core#Concept"/>
    <skos:prefLabel xml:lang="en">fishery management</skos:prefLabel>
    <skos:scopeNote xml:lang="en">Controlling or directing numbers and life conditions of fish living in a specific locality to achieve a selected goal.</skos:scopeNote>
    <skos:broader rdf:resource="http://www.usgs.gov/science/USGSThesaurus/biological%20population%20management"/>
    <skos:inScheme rdf:resource="http://www.usgs.gov/science/USGSThesaurus"/>
  </rdf:Description>
  <rdf:Description about="http://www.usgs.gov/science/USGSThesaurus/pest%20control">
    <rdf:type rdf:resource="http://www.w3.org/2004/02/skos/core#Concept"/>
    <skos:prefLabel xml:lang="en">pest control</skos:prefLabel>
    <skos:scopeNote xml:lang="en">Intentional reduction in the abundance of specific harmful organisms in a given area.</skos:scopeNote>
    <skos:broader rdf:resource="http://www.usgs.gov/science/USGSThesaurus/biological%20population%20management"/>
    <skos:inScheme rdf:resource="http://www.usgs.gov/science/USGSThesaurus"/>
  </rdf:Description>
  <rdf:Description about="http://www.usgs.gov/science/USGSThesaurus/reintroduction%20%28organisms%29">
    <rdf:type rdf:resource="http://www.w3.org/2004/02/skos/core#Concept"/>
    <skos:prefLabel xml:lang="en">reintroduction (organisms)</skos:prefLabel>
    <skos:scopeNote xml:lang="en">Return of a species to an area through the intervention of man.</skos:scopeNote>
    <skos:altLabel xml:lang="en">re-establishment (organisms)</skos:altLabel>
    <skos:altLabel xml:lang="en">recolonization (organisms)</skos:altLabel>
    <skos:broader rdf:resource="http://www.usgs.gov/science/USGSThesaurus/biological%20population%20management"/>
    <skos:inScheme rdf:resource="http://www.usgs.gov/science/USGSThesaurus"/>
  </rdf:Description>
  <rdf:Description about="http://www.usgs.gov/science/USGSThesaurus/wildlife%20population%20management">
    <rdf:type rdf:resource="http://www.w3.org/2004/02/skos/core#Concept"/>
    <skos:prefLabel xml:lang="en">wildlife population management</skos:prefLabel>
    <skos:scopeNote xml:lang="en">Monitoring and control of wildlife as a sustainable natural asset.</skos:scopeNote>
    <skos:broader rdf:resource="http://www.usgs.gov/science/USGSThesaurus/biological%20population%20management"/>
    <skos:narrower rdf:resource="http://www.usgs.gov/science/USGSThesaurus/game%20management"/>
    <skos:related rdf:resource="http://www.usgs.gov/science/USGSThesaurus/biogeography"/>
    <skos:related rdf:resource="http://www.usgs.gov/science/USGSThesaurus/wildlife%20biology"/>
    <skos:inScheme rdf:resource="http://www.usgs.gov/science/USGSThesaurus"/>
  </rdf:Description>
  <rdf:Description about="http://www.usgs.gov/science/USGSThesaurus/game%20management">
    <rdf:type rdf:resource="http://www.w3.org/2004/02/skos/core#Concept"/>
    <skos:prefLabel xml:lang="en">game management</skos:prefLabel>
    <skos:scopeNote xml:lang="en">Scientific monitoring and control of hunted wildlife.</skos:scopeNote>
    <skos:broader rdf:resource="http://www.usgs.gov/science/USGSThesaurus/wildlife%20population%20management"/>
    <skos:related rdf:resource="http://www.usgs.gov/science/USGSThesaurus/wildlife%20biology"/>
    <skos:inScheme rdf:resource="http://www.usgs.gov/science/USGSThesaurus"/>
  </rdf:Description>
  <rdf:Description about="http://www.usgs.gov/science/USGSThesaurus/controlled%20flooding">
    <rdf:type rdf:resource="http://www.w3.org/2004/02/skos/core#Concept"/>
    <skos:prefLabel xml:lang="en">controlled flooding</skos:prefLabel>
    <skos:scopeNote xml:lang="en">The deliberate inundation of land or wetland, or an increase in river flow below dams for restoration or research purposes. Do not confuse with flood control.</skos:scopeNote>
    <skos:altLabel xml:lang="en">flooding (controlled)</skos:altLabel>
    <skos:altLabel xml:lang="en">managed flooding</skos:altLabel>
    <skos:broader rdf:resource="http://www.usgs.gov/science/USGSThesaurus/natural%20resource%20management"/>
    <skos:related rdf:resource="http://www.usgs.gov/science/USGSThesaurus/floods"/>
    <skos:inScheme rdf:resource="http://www.usgs.gov/science/USGSThesaurus"/>
  </rdf:Description>
  <rdf:Description about="http://www.usgs.gov/science/USGSThesaurus/ecosystem%20management">
    <rdf:type rdf:resource="http://www.w3.org/2004/02/skos/core#Concept"/>
    <skos:prefLabel xml:lang="en">ecosystem management</skos:prefLabel>
    <skos:scopeNote xml:lang="en">Means of controlling or directing human practices, species populations, and physical environment within an ecosystem to achieve a selected state of sustainability.</skos:scopeNote>
    <skos:altLabel xml:lang="en">reintroduction (organisms)</skos:altLabel>
    <skos:altLabel xml:lang="en">ecosystem preservation</skos:altLabel>
    <skos:broader rdf:resource="http://www.usgs.gov/science/USGSThesaurus/natural%20resource%20management"/>
    <skos:related rdf:resource="http://www.usgs.gov/science/USGSThesaurus/ecosystem%20monitoring"/>
    <skos:related rdf:resource="http://www.usgs.gov/science/USGSThesaurus/ecosystem%20services%20valuation"/>
    <skos:inScheme rdf:resource="http://www.usgs.gov/science/USGSThesaurus"/>
  </rdf:Description>
  <rdf:Description about="http://www.usgs.gov/science/USGSThesaurus/fire%20control">
    <rdf:type rdf:resource="http://www.w3.org/2004/02/skos/core#Concept"/>
    <skos:prefLabel xml:lang="en">fire control</skos:prefLabel>
    <skos:scopeNote xml:lang="en">Human intervention to restrict or prevent fires in forests and grasslands.</skos:scopeNote>
    <skos:altLabel xml:lang="en">fire prevention</skos:altLabel>
    <skos:broader rdf:resource="http://www.usgs.gov/science/USGSThesaurus/natural%20resource%20management"/>
    <skos:narrower rdf:resource="http://www.usgs.gov/science/USGSThesaurus/controlled%20fires"/>
    <skos:related rdf:resource="http://www.usgs.gov/science/USGSThesaurus/controlled%20fires"/>
    <skos:inScheme rdf:resource="http://www.usgs.gov/science/USGSThesaurus"/>
  </rdf:Description>
  <rdf:Description about="http://www.usgs.gov/science/USGSThesaurus/controlled%20fires">
    <rdf:type rdf:resource="http://www.w3.org/2004/02/skos/core#Concept"/>
    <skos:prefLabel xml:lang="en">controlled fires</skos:prefLabel>
    <skos:scopeNote xml:lang="en">Prescribed burns used to burn trees, brush, and undergrowth that would fuel a large wildfire.  Do not confuse this term with 'fire control'.  It is one of the tools used in fire control.</skos:scopeNote>
    <skos:altLabel xml:lang="en">controlled burns</skos:altLabel>
    <skos:altLabel xml:lang="en">fires (controlled)</skos:altLabel>
    <skos:altLabel xml:lang="en">managed fires</skos:altLabel>
    <skos:broader rdf:resource="http://www.usgs.gov/science/USGSThesaurus/fire%20control"/>
    <skos:related rdf:resource="http://www.usgs.gov/science/USGSThesaurus/fires"/>
    <skos:related rdf:resource="http://www.usgs.gov/science/USGSThesaurus/fire%20control"/>
    <skos:inScheme rdf:resource="http://www.usgs.gov/science/USGSThesaurus"/>
  </rdf:Description>
  <rdf:Description about="http://www.usgs.gov/science/USGSThesaurus/natural%20resource%20assessment">
    <rdf:type rdf:resource="http://www.w3.org/2004/02/skos/core#Concept"/>
    <skos:prefLabel xml:lang="en">natural resource assessment</skos:prefLabel>
    <skos:scopeNote xml:lang="en">Estimation of the actual or potential value of natural materials and processes.</skos:scopeNote>
    <skos:altLabel xml:lang="en">resource assessment</skos:altLabel>
    <skos:broader rdf:resource="http://www.usgs.gov/science/USGSThesaurus/natural%20resource%20management"/>
    <skos:inScheme rdf:resource="http://www.usgs.gov/science/USGSThesaurus"/>
  </rdf:Description>
  <rdf:Description about="http://www.usgs.gov/science/USGSThesaurus/remediation">
    <rdf:type rdf:resource="http://www.w3.org/2004/02/skos/core#Concept"/>
    <skos:prefLabel xml:lang="en">remediation</skos:prefLabel>
    <skos:scopeNote xml:lang="en">Methods for decontaminating, reclaiming, and restoring natural resources or reducing the effects of hazards.</skos:scopeNote>
    <skos:altLabel xml:lang="en">reclamation</skos:altLabel>
    <skos:altLabel xml:lang="en">restoration</skos:altLabel>
    <skos:broader rdf:resource="http://www.usgs.gov/science/USGSThesaurus/natural%20resource%20management"/>
    <skos:narrower rdf:resource="http://www.usgs.gov/science/USGSThesaurus/bioremediation"/>
    <skos:related rdf:resource="http://www.usgs.gov/science/USGSThesaurus/ecology"/>
    <skos:related rdf:resource="http://www.usgs.gov/science/USGSThesaurus/ecosystem%20monitoring"/>
    <skos:related rdf:resource="http://www.usgs.gov/science/USGSThesaurus/engineering%20geology"/>
    <skos:inScheme rdf:resource="http://www.usgs.gov/science/USGSThesaurus"/>
  </rdf:Description>
  <rdf:Description about="http://www.usgs.gov/science/USGSThesaurus/bioremediation">
    <rdf:type rdf:resource="http://www.w3.org/2004/02/skos/core#Concept"/>
    <skos:prefLabel xml:lang="en">bioremediation</skos:prefLabel>
    <skos:scopeNote xml:lang="en">Use of biological methods, usually involving microorganisms, to break down or neutralize contaminants in soil, water, and wastes.</skos:scopeNote>
    <skos:altLabel xml:lang="en">biological remediation</skos:altLabel>
    <skos:altLabel xml:lang="en">revegetation</skos:altLabel>
    <skos:broader rdf:resource="http://www.usgs.gov/science/USGSThesaurus/remediation"/>
    <skos:related rdf:resource="http://www.usgs.gov/science/USGSThesaurus/ecology"/>
    <skos:related rdf:resource="http://www.usgs.gov/science/USGSThesaurus/ecosystem%20monitoring"/>
    <skos:inScheme rdf:resource="http://www.usgs.gov/science/USGSThesaurus"/>
  </rdf:Description>
  <rdf:Description about="http://www.usgs.gov/science/USGSThesaurus/water%20resource%20management">
    <rdf:type rdf:resource="http://www.w3.org/2004/02/skos/core#Concept"/>
    <skos:prefLabel xml:lang="en">water resource management</skos:prefLabel>
    <skos:scopeNote xml:lang="en">Methods of controlling or directing resources and activities related to water for a predetermined goal.</skos:scopeNote>
    <skos:altLabel xml:lang="en">artificial recharge</skos:altLabel>
    <skos:altLabel xml:lang="en">impoundment</skos:altLabel>
    <skos:altLabel xml:lang="en">reclaimed water</skos:altLabel>
    <skos:broader rdf:resource="http://www.usgs.gov/science/USGSThesaurus/natural%20resource%20management"/>
    <skos:related rdf:resource="http://www.usgs.gov/science/USGSThesaurus/hydraulic%20engineering"/>
    <skos:inScheme rdf:resource="http://www.usgs.gov/science/USGSThesaurus"/>
  </rdf:Description>
  <rdf:Description about="http://www.usgs.gov/science/USGSThesaurus/watershed%20management">
    <rdf:type rdf:resource="http://www.w3.org/2004/02/skos/core#Concept"/>
    <skos:prefLabel xml:lang="en">watershed management</skos:prefLabel>
    <skos:scopeNote xml:lang="en">Controlling and directing the resources and activities associated with the land and streams of a drainage basin to maintain the supply and quality of water and prevent floods, erosions, and other destructive conditions.</skos:scopeNote>
    <skos:broader rdf:resource="http://www.usgs.gov/science/USGSThesaurus/natural%20resource%20management"/>
    <skos:related rdf:resource="http://www.usgs.gov/science/USGSThesaurus/erosion"/>
    <skos:related rdf:resource="http://www.usgs.gov/science/USGSThesaurus/floods"/>
    <skos:related rdf:resource="http://www.usgs.gov/science/USGSThesaurus/streamflow"/>
    <skos:inScheme rdf:resource="http://www.usgs.gov/science/USGSThesaurus"/>
  </rdf:Description>
  <rdf:Description about="http://www.usgs.gov/science/USGSThesaurus/risk%20assessment">
    <rdf:type rdf:resource="http://www.w3.org/2004/02/skos/core#Concept"/>
    <skos:prefLabel xml:lang="en">risk assessment</skos:prefLabel>
    <skos:scopeNote xml:lang="en">The evaluation of the likelihood of adverse effects due to a given factor such as energy development or recurring hazardous events such as earthquakes.</skos:scopeNote>
    <skos:broader rdf:resource="http://www.usgs.gov/science/USGSThesaurus/management%20methods"/>
    <skos:narrower rdf:resource="http://www.usgs.gov/science/USGSThesaurus/earthquake%20probabilities"/>
    <skos:narrower rdf:resource="http://www.usgs.gov/science/USGSThesaurus/landslide%20susceptibility%20assessment"/>
    <skos:narrower rdf:resource="http://www.usgs.gov/science/USGSThesaurus/volcanic%20eruption%20prediction"/>
    <skos:inScheme rdf:resource="http://www.usgs.gov/science/USGSThesaurus"/>
  </rdf:Description>
  <rdf:Description about="http://www.usgs.gov/science/USGSThesaurus/earthquake%20probabilities">
    <rdf:type rdf:resource="http://www.w3.org/2004/02/skos/core#Concept"/>
    <skos:prefLabel xml:lang="en">earthquake probabilities</skos:prefLabel>
    <skos:scopeNote xml:lang="en">That aspect of seismology that deals with the physical conditions or indications that precede an earthquake, in order to predict its probability, size, time, and location.</skos:scopeNote>
    <skos:altLabel xml:lang="en">earthquake forecasting</skos:altLabel>
    <skos:altLabel xml:lang="en">earthquake prediction</skos:altLabel>
    <!--FOR seismicity maps USE earthquake probabilities WITH maps and atlases-->
    <skos:altLabel xml:lang="en">seismicity maps</skos:altLabel>
    <skos:broader rdf:resource="http://www.usgs.gov/science/USGSThesaurus/risk%20assessment"/>
    <skos:related rdf:resource="http://www.usgs.gov/science/USGSThesaurus/earthquakes"/>
    <skos:related rdf:resource="http://www.usgs.gov/science/USGSThesaurus/neotectonic%20processes"/>
    <skos:inScheme rdf:resource="http://www.usgs.gov/science/USGSThesaurus"/>
  </rdf:Description>
  <rdf:Description about="http://www.usgs.gov/science/USGSThesaurus/landslide%20susceptibility%20assessment">
    <rdf:type rdf:resource="http://www.w3.org/2004/02/skos/core#Concept"/>
    <skos:prefLabel xml:lang="en">landslide susceptibility assessment</skos:prefLabel>
    <skos:scopeNote xml:lang="en">Estimation of the probability of occurrence and likely severity of landslides in a given area.</skos:scopeNote>
    <!--FOR landslide susceptibility maps USE landslide susceptibility assessment WITH maps and atlases-->
    <skos:altLabel xml:lang="en">landslide susceptibility maps</skos:altLabel>
    <skos:altLabel xml:lang="en">slope stability</skos:altLabel>
    <!--FOR slope stability maps USE landslide susceptibility assessment WITH maps and atlases-->
    <skos:altLabel xml:lang="en">slope stability maps</skos:altLabel>
    <skos:broader rdf:resource="http://www.usgs.gov/science/USGSThesaurus/risk%20assessment"/>
    <skos:related rdf:resource="http://www.usgs.gov/science/USGSThesaurus/landslides"/>
    <skos:inScheme rdf:resource="http://www.usgs.gov/science/USGSThesaurus"/>
  </rdf:Description>
  <rdf:Description about="http://www.usgs.gov/science/USGSThesaurus/volcanic%20eruption%20prediction">
    <rdf:type rdf:resource="http://www.w3.org/2004/02/skos/core#Concept"/>
    <skos:prefLabel xml:lang="en">volcanic eruption prediction</skos:prefLabel>
    <skos:scopeNote xml:lang="en">Estimation of future volcanic activity using geological and geophysical observations.</skos:scopeNote>
    <skos:altLabel xml:lang="en">volcanic eruption forecasting</skos:altLabel>
    <skos:broader rdf:resource="http://www.usgs.gov/science/USGSThesaurus/risk%20assessment"/>
    <skos:related rdf:resource="http://www.usgs.gov/science/USGSThesaurus/volcanic%20activity"/>
    <skos:inScheme rdf:resource="http://www.usgs.gov/science/USGSThesaurus"/>
  </rdf:Description>
  <rdf:Description about="http://www.usgs.gov/science/USGSThesaurus/photography">
    <rdf:type rdf:resource="http://www.w3.org/2004/02/skos/core#Concept"/>
    <skos:prefLabel xml:lang="en">photography</skos:prefLabel>
    <skos:scopeNote xml:lang="en">Process of using digital or film cameras to collect images of objects.</skos:scopeNote>
    <!--FOR photographs USE photography WITH image collections-->
    <skos:altLabel xml:lang="en">photographs</skos:altLabel>
    <skos:broader rdf:resource="http://www.usgs.gov/science/USGSThesaurus/methods"/>
    <skos:narrower rdf:resource="http://www.usgs.gov/science/USGSThesaurus/underwater%20photography"/>
    <skos:related rdf:resource="http://www.usgs.gov/science/USGSThesaurus/videography"/>
    <skos:related rdf:resource="http://www.usgs.gov/science/USGSThesaurus/aerial%20photography"/>
    <skos:inScheme rdf:resource="http://www.usgs.gov/science/USGSThesaurus"/>
  </rdf:Description>
  <rdf:Description about="http://www.usgs.gov/science/USGSThesaurus/underwater%20photography">
    <rdf:type rdf:resource="http://www.w3.org/2004/02/skos/core#Concept"/>
    <skos:prefLabel xml:lang="en">underwater photography</skos:prefLabel>
    <skos:scopeNote xml:lang="en">Photographs taken below the water surface, usually in marine, lacustrine, and estuarine environments.  Subjects are typically benthic organisms and sedimentary structures on the sea floor.</skos:scopeNote>
    <skos:altLabel xml:lang="en">camera tows</skos:altLabel>
    <skos:broader rdf:resource="http://www.usgs.gov/science/USGSThesaurus/photography"/>
    <skos:related rdf:resource="http://www.usgs.gov/science/USGSThesaurus/ocean%20sciences"/>
    <skos:inScheme rdf:resource="http://www.usgs.gov/science/USGSThesaurus"/>
  </rdf:Description>
  <rdf:Description about="http://www.usgs.gov/science/USGSThesaurus/remote%20sensing">
    <rdf:type rdf:resource="http://www.w3.org/2004/02/skos/core#Concept"/>
    <skos:prefLabel xml:lang="en">remote sensing</skos:prefLabel>
    <skos:scopeNote xml:lang="en">Acquiring information about a natural feature or phenomenon, such as the Earth's surface, without actually being in contact with it. USGS remote sensing is usually carried out with airborne or spaceborne sensors or cameras.</skos:scopeNote>
    <!--FOR remote-sensing data USE remote sensing WITH image collections-->
    <skos:altLabel xml:lang="en">remote-sensing data</skos:altLabel>
    <!--FOR remote-sensing images USE remote sensing WITH image collections-->
    <skos:altLabel xml:lang="en">remote-sensing images</skos:altLabel>
    <skos:altLabel xml:lang="en">airborne imaging</skos:altLabel>
    <!--FOR composite burn index USE remote sensing WITH fire damage-->
    <skos:altLabel xml:lang="en">composite burn index</skos:altLabel>
    <!--FOR normalized burn ratio USE remote sensing WITH fire damage-->
    <skos:altLabel xml:lang="en">normalized burn ratio</skos:altLabel>
    <skos:altLabel xml:lang="en">photogrammetry</skos:altLabel>
    <!--FOR satellite altimetry USE remote sensing WITH altimetry measurement-->
    <skos:altLabel xml:lang="en">satellite altimetry</skos:altLabel>
    <skos:altLabel xml:lang="en">satellite imaging</skos:altLabel>
    <skos:altLabel xml:lang="en">space-borne sensing</skos:altLabel>
    <!--FOR satellite images USE remote sensing WITH image collections-->
    <skos:altLabel xml:lang="en">satellite images</skos:altLabel>
    <skos:broader rdf:resource="http://www.usgs.gov/science/USGSThesaurus/methods"/>
    <skos:narrower rdf:resource="http://www.usgs.gov/science/USGSThesaurus/IFSAR"/>
    <skos:narrower rdf:resource="http://www.usgs.gov/science/USGSThesaurus/LIDAR"/>
    <skos:narrower rdf:resource="http://www.usgs.gov/science/USGSThesaurus/aerial%20photography"/>
    <skos:narrower rdf:resource="http://www.usgs.gov/science/USGSThesaurus/aeromagnetic%20surveying"/>
    <skos:narrower rdf:resource="http://www.usgs.gov/science/USGSThesaurus/aeroradiometric%20surveying"/>
    <skos:narrower rdf:resource="http://www.usgs.gov/science/USGSThesaurus/hyperspectral%20imaging"/>
    <skos:narrower rdf:resource="http://www.usgs.gov/science/USGSThesaurus/infrared%20imaging"/>
    <skos:narrower rdf:resource="http://www.usgs.gov/science/USGSThesaurus/microwave%20imaging"/>
    <skos:narrower rdf:resource="http://www.usgs.gov/science/USGSThesaurus/multispectral%20imaging"/>
    <skos:narrower rdf:resource="http://www.usgs.gov/science/USGSThesaurus/panchromatic%20imaging"/>
    <skos:narrower rdf:resource="http://www.usgs.gov/science/USGSThesaurus/radar%20imaging"/>
    <skos:narrower rdf:resource="http://www.usgs.gov/science/USGSThesaurus/thermal%20imaging"/>
    <skos:narrower rdf:resource="http://www.usgs.gov/science/USGSThesaurus/visible%20light%20imaging"/>
    <skos:related rdf:resource="http://www.usgs.gov/science/USGSThesaurus/geography"/>
    <skos:related rdf:resource="http://www.usgs.gov/science/USGSThesaurus/seismic%20methods"/>
    <skos:related rdf:resource="http://www.usgs.gov/science/USGSThesaurus/telemetry"/>
    <skos:related rdf:resource="http://www.usgs.gov/science/USGSThesaurus/videography"/>
    <skos:inScheme rdf:resource="http://www.usgs.gov/science/USGSThesaurus"/>
  </rdf:Description>
  <rdf:Description about="http://www.usgs.gov/science/USGSThesaurus/IFSAR">
    <rdf:type rdf:resource="http://www.w3.org/2004/02/skos/core#Concept"/>
    <skos:prefLabel xml:lang="en">IFSAR</skos:prefLabel>
    <skos:scopeNote xml:lang="en">Interferometric comparison of radar reflectance imagery of the same area at different times to determine changes in the land surface, typically from a space-borne sensor.</skos:scopeNote>
    <skos:altLabel xml:lang="en">Interferometric Synthetic Aperture Radar (IFSAR)</skos:altLabel>
    <skos:altLabel xml:lang="en">SAR interferometry</skos:altLabel>
    <skos:altLabel xml:lang="en">InSAR</skos:altLabel>
    <skos:broader rdf:resource="http://www.usgs.gov/science/USGSThesaurus/remote%20sensing"/>
    <skos:related rdf:resource="http://www.usgs.gov/science/USGSThesaurus/geography"/>
    <skos:inScheme rdf:resource="http://www.usgs.gov/science/USGSThesaurus"/>
  </rdf:Description>
  <rdf:Description about="http://www.usgs.gov/science/USGSThesaurus/LIDAR">
    <rdf:type rdf:resource="http://www.w3.org/2004/02/skos/core#Concept"/>
    <skos:prefLabel xml:lang="en">LIDAR</skos:prefLabel>
    <skos:scopeNote xml:lang="en">LIDAR (LIght Detection and Ranging) is an airborne, spaceborne or ground-based laser-ranging technique commonly used for acquiring high-resolution topographic data.</skos:scopeNote>
    <!--FOR LIDAR images USE LIDAR WITH image collections-->
    <skos:altLabel xml:lang="en">LIDAR images</skos:altLabel>
    <skos:altLabel xml:lang="en">LIght Detection and Ranging</skos:altLabel>
    <skos:broader rdf:resource="http://www.usgs.gov/science/USGSThesaurus/remote%20sensing"/>
    <skos:related rdf:resource="http://www.usgs.gov/science/USGSThesaurus/geography"/>
    <skos:inScheme rdf:resource="http://www.usgs.gov/science/USGSThesaurus"/>
  </rdf:Description>
  <rdf:Description about="http://www.usgs.gov/science/USGSThesaurus/aerial%20photography">
    <rdf:type rdf:resource="http://www.w3.org/2004/02/skos/core#Concept"/>
    <skos:prefLabel xml:lang="en">aerial photography</skos:prefLabel>
    <skos:scopeNote xml:lang="en">The process of taking pictures with a camera from an aircraft. Use for both the process of photography from the air and the images produced by the process.</skos:scopeNote>
    <!--FOR aerial photographs USE aerial photography WITH image collections-->
    <skos:altLabel xml:lang="en">aerial photographs</skos:altLabel>
    <!--FOR aerial photos USE aerial photography WITH image collections-->
    <skos:altLabel xml:lang="en">aerial photos</skos:altLabel>
    <!--FOR air photos USE aerial photography WITH image collections-->
    <skos:altLabel xml:lang="en">air photos</skos:altLabel>
    <!--FOR orthoimagery USE aerial photography WITH image collections-->
    <skos:altLabel xml:lang="en">orthoimagery</skos:altLabel>
    <!--FOR orthophotographs USE aerial photography WITH image collections-->
    <skos:altLabel xml:lang="en">orthophotographs</skos:altLabel>
    <skos:broader rdf:resource="http://www.usgs.gov/science/USGSThesaurus/remote%20sensing"/>
    <skos:related rdf:resource="http://www.usgs.gov/science/USGSThesaurus/photography"/>
    <skos:inScheme rdf:resource="http://www.usgs.gov/science/USGSThesaurus"/>
  </rdf:Description>
  <rdf:Description about="http://www.usgs.gov/science/USGSThesaurus/aeromagnetic%20surveying">
    <rdf:type rdf:resource="http://www.w3.org/2004/02/skos/core#Concept"/>
    <skos:prefLabel xml:lang="en">aeromagnetic surveying</skos:prefLabel>
    <skos:scopeNote xml:lang="en">Mapping of the earth's magnetic field with the use of airborne electronic magnetometers.</skos:scopeNote>
    <!--FOR aeromagnetic maps USE aeromagnetic surveying WITH maps and atlases-->
    <skos:altLabel xml:lang="en">aeromagnetic maps</skos:altLabel>
    <!--FOR magnetic surveying USE aeromagnetic surveying WITH electromagnetic surveying-->
    <skos:altLabel xml:lang="en">magnetic surveying</skos:altLabel>
    <skos:broader rdf:resource="http://www.usgs.gov/science/USGSThesaurus/remote%20sensing"/>
    <skos:related rdf:resource="http://www.usgs.gov/science/USGSThesaurus/electromagnetic%20surveying"/>
    <skos:related rdf:resource="http://www.usgs.gov/science/USGSThesaurus/geography"/>
    <skos:inScheme rdf:resource="http://www.usgs.gov/science/USGSThesaurus"/>
  </rdf:Description>
  <rdf:Description about="http://www.usgs.gov/science/USGSThesaurus/aeroradiometric%20surveying">
    <rdf:type rdf:resource="http://www.w3.org/2004/02/skos/core#Concept"/>
    <skos:prefLabel xml:lang="en">aeroradiometric surveying</skos:prefLabel>
    <skos:scopeNote xml:lang="en">Mapping of gamma radiation from the earth's surface with airborne scintillation meters or gamma-ray spectrometers.</skos:scopeNote>
    <skos:altLabel xml:lang="en">gamma-ray spectrometric surveying</skos:altLabel>
    <skos:broader rdf:resource="http://www.usgs.gov/science/USGSThesaurus/remote%20sensing"/>
    <skos:related rdf:resource="http://www.usgs.gov/science/USGSThesaurus/geography"/>
    <skos:inScheme rdf:resource="http://www.usgs.gov/science/USGSThesaurus"/>
  </rdf:Description>
  <rdf:Description about="http://www.usgs.gov/science/USGSThesaurus/hyperspectral%20imaging">
    <rdf:type rdf:resource="http://www.w3.org/2004/02/skos/core#Concept"/>
    <skos:prefLabel xml:lang="en">hyperspectral imaging</skos:prefLabel>
    <skos:scopeNote xml:lang="en">Multispectral imaging technique that records many bands of imagery at very narrow bandwidths.</skos:scopeNote>
    <skos:broader rdf:resource="http://www.usgs.gov/science/USGSThesaurus/remote%20sensing"/>
    <skos:related rdf:resource="http://www.usgs.gov/science/USGSThesaurus/geography"/>
    <skos:inScheme rdf:resource="http://www.usgs.gov/science/USGSThesaurus"/>
  </rdf:Description>
  <rdf:Description about="http://www.usgs.gov/science/USGSThesaurus/infrared%20imaging">
    <rdf:type rdf:resource="http://www.w3.org/2004/02/skos/core#Concept"/>
    <skos:prefLabel xml:lang="en">infrared imaging</skos:prefLabel>
    <skos:scopeNote xml:lang="en">Method of remote sensing in which optical sensors produce visible representations of infrared rays or radiated heat from the observed objects and the temperature variations are represented by different colors in the image.</skos:scopeNote>
    <skos:broader rdf:resource="http://www.usgs.gov/science/USGSThesaurus/remote%20sensing"/>
    <skos:narrower rdf:resource="http://www.usgs.gov/science/USGSThesaurus/AVHRR"/>
    <skos:narrower rdf:resource="http://www.usgs.gov/science/USGSThesaurus/AVIRIS"/>
    <skos:related rdf:resource="http://www.usgs.gov/science/USGSThesaurus/geography"/>
    <skos:inScheme rdf:resource="http://www.usgs.gov/science/USGSThesaurus"/>
  </rdf:Description>
  <rdf:Description about="http://www.usgs.gov/science/USGSThesaurus/AVHRR">
    <rdf:type rdf:resource="http://www.w3.org/2004/02/skos/core#Concept"/>
    <skos:prefLabel xml:lang="en">AVHRR</skos:prefLabel>
    <skos:scopeNote xml:lang="en">Advanced Very High Resolution Radiometer or broad-band, four or five channel scanner, sensing in the visible, near-infrared, and thermal infrared portions of the electromagnetic spectrum. This information is used to estimate characteristics of the land and sea surface such as temperature and overall health of vegetation.</skos:scopeNote>
    <!--FOR AVHRR images USE AVHRR WITH image collections-->
    <skos:altLabel xml:lang="en">AVHRR images</skos:altLabel>
    <skos:altLabel xml:lang="en">Advanced Very High Resolution Radiometer (AVHRR)</skos:altLabel>
    <skos:broader rdf:resource="http://www.usgs.gov/science/USGSThesaurus/infrared%20imaging"/>
    <skos:related rdf:resource="http://www.usgs.gov/science/USGSThesaurus/geography"/>
    <skos:related rdf:resource="http://www.usgs.gov/science/USGSThesaurus/sea%20surface%20temperature"/>
    <skos:inScheme rdf:resource="http://www.usgs.gov/science/USGSThesaurus"/>
  </rdf:Description>
  <rdf:Description about="http://www.usgs.gov/science/USGSThesaurus/AVIRIS">
    <rdf:type rdf:resource="http://www.w3.org/2004/02/skos/core#Concept"/>
    <skos:prefLabel xml:lang="en">AVIRIS</skos:prefLabel>
    <skos:scopeNote xml:lang="en"></skos:scopeNote>
    <skos:altLabel xml:lang="en">airborne visible infrared imaging spectrometer</skos:altLabel>
    <skos:broader rdf:resource="http://www.usgs.gov/science/USGSThesaurus/infrared%20imaging"/>
    <skos:inScheme rdf:resource="http://www.usgs.gov/science/USGSThesaurus"/>
  </rdf:Description>
  <rdf:Description about="http://www.usgs.gov/science/USGSThesaurus/microwave%20imaging">
    <rdf:type rdf:resource="http://www.w3.org/2004/02/skos/core#Concept"/>
    <skos:prefLabel xml:lang="en">microwave imaging</skos:prefLabel>
    <skos:scopeNote xml:lang="en">Remote sensing method using short high frequency electromagnetic waves reflected or radiated from the ground.</skos:scopeNote>
    <skos:broader rdf:resource="http://www.usgs.gov/science/USGSThesaurus/remote%20sensing"/>
    <skos:narrower rdf:resource="http://www.usgs.gov/science/USGSThesaurus/SMMR"/>
    <skos:narrower rdf:resource="http://www.usgs.gov/science/USGSThesaurus/SSM%2FI"/>
    <skos:related rdf:resource="http://www.usgs.gov/science/USGSThesaurus/geography"/>
    <skos:related rdf:resource="http://www.usgs.gov/science/USGSThesaurus/radar%20imaging"/>
    <skos:inScheme rdf:resource="http://www.usgs.gov/science/USGSThesaurus"/>
  </rdf:Description>
  <rdf:Description about="http://www.usgs.gov/science/USGSThesaurus/SMMR">
    <rdf:type rdf:resource="http://www.w3.org/2004/02/skos/core#Concept"/>
    <skos:prefLabel xml:lang="en">SMMR</skos:prefLabel>
    <skos:scopeNote xml:lang="en">Scanning Multichannel Microwave Radiometer (SMMR), a technique which uses a multichannel microwave radiometer mounted on an airplane or satellite to measure polarized microwave radiances from the atmosphere, seas or land. Temperatures, wind speeds, sea ice coverage, and terrain parameters can be obtained.</skos:scopeNote>
    <skos:altLabel xml:lang="en">SMMR images</skos:altLabel>
    <skos:altLabel xml:lang="en">Scanning Multichannel Microwave Radiometer (SMMR)</skos:altLabel>
    <skos:broader rdf:resource="http://www.usgs.gov/science/USGSThesaurus/microwave%20imaging"/>
    <skos:related rdf:resource="http://www.usgs.gov/science/USGSThesaurus/geography"/>
    <skos:inScheme rdf:resource="http://www.usgs.gov/science/USGSThesaurus"/>
  </rdf:Description>
  <rdf:Description about="http://www.usgs.gov/science/USGSThesaurus/SSM%2FI">
    <rdf:type rdf:resource="http://www.w3.org/2004/02/skos/core#Concept"/>
    <skos:prefLabel xml:lang="en">SSM/I</skos:prefLabel>
    <skos:scopeNote xml:lang="en">Special Sensor Microwave/Imager (SSM/I), technique using passive microwave radiometers aboard satellites to measure the microwave reflectivity of the earth, oceans, and the atmosphere.</skos:scopeNote>
    <skos:altLabel xml:lang="en">SSM/I images</skos:altLabel>
    <skos:altLabel xml:lang="en">Special Sensor Microwave/Imager (SSM/I)</skos:altLabel>
    <skos:broader rdf:resource="http://www.usgs.gov/science/USGSThesaurus/microwave%20imaging"/>
    <skos:related rdf:resource="http://www.usgs.gov/science/USGSThesaurus/geography"/>
    <skos:related rdf:resource="http://www.usgs.gov/science/USGSThesaurus/snow%20and%20ice%20cover"/>
    <skos:inScheme rdf:resource="http://www.usgs.gov/science/USGSThesaurus"/>
  </rdf:Description>
  <rdf:Description about="http://www.usgs.gov/science/USGSThesaurus/multispectral%20imaging">
    <rdf:type rdf:resource="http://www.w3.org/2004/02/skos/core#Concept"/>
    <skos:prefLabel xml:lang="en">multispectral imaging</skos:prefLabel>
    <skos:scopeNote xml:lang="en">A method of remote sensing that obtains optical representations in two or more ranges of frequencies or wave lengths.</skos:scopeNote>
    <skos:altLabel xml:lang="en">advanced spaceborne thermal emission and reflection radiometer</skos:altLabel>
    <skos:altLabel xml:lang="en">ASTER</skos:altLabel>
    <!--FOR Landsat images USE multispectral imaging WITH image collections-->
    <skos:altLabel xml:lang="en">Landsat images</skos:altLabel>
    <skos:altLabel xml:lang="en">thematic mapper</skos:altLabel>
    <skos:altLabel xml:lang="en">MODIS</skos:altLabel>
    <skos:altLabel xml:lang="en">Moderate-resolution imaging spectroradiometer</skos:altLabel>
    <skos:broader rdf:resource="http://www.usgs.gov/science/USGSThesaurus/remote%20sensing"/>
    <skos:related rdf:resource="http://www.usgs.gov/science/USGSThesaurus/geography"/>
    <skos:inScheme rdf:resource="http://www.usgs.gov/science/USGSThesaurus"/>
  </rdf:Description>
  <rdf:Description about="http://www.usgs.gov/science/USGSThesaurus/panchromatic%20imaging">
    <rdf:type rdf:resource="http://www.w3.org/2004/02/skos/core#Concept"/>
    <skos:prefLabel xml:lang="en">panchromatic imaging</skos:prefLabel>
    <skos:scopeNote xml:lang="en">Photographic technique which uses emulsions, films, or plates sensitive to all colors in light to produce black-and-white photographs. Often used in aerial and satellite photography.</skos:scopeNote>
    <skos:broader rdf:resource="http://www.usgs.gov/science/USGSThesaurus/remote%20sensing"/>
    <skos:related rdf:resource="http://www.usgs.gov/science/USGSThesaurus/geography"/>
    <skos:inScheme rdf:resource="http://www.usgs.gov/science/USGSThesaurus"/>
  </rdf:Description>
  <rdf:Description about="http://www.usgs.gov/science/USGSThesaurus/radar%20imaging">
    <rdf:type rdf:resource="http://www.w3.org/2004/02/skos/core#Concept"/>
    <skos:prefLabel xml:lang="en">radar imaging</skos:prefLabel>
    <skos:scopeNote xml:lang="en">A remote sensing technique which uses the reflection of pulsed high frequency radio waves to determine the speed, direction, and distance of faraway objects.</skos:scopeNote>
    <skos:broader rdf:resource="http://www.usgs.gov/science/USGSThesaurus/remote%20sensing"/>
    <skos:narrower rdf:resource="http://www.usgs.gov/science/USGSThesaurus/SLAR"/>
    <skos:narrower rdf:resource="http://www.usgs.gov/science/USGSThesaurus/doppler%20radar%20imaging"/>
    <skos:related rdf:resource="http://www.usgs.gov/science/USGSThesaurus/geography"/>
    <skos:related rdf:resource="http://www.usgs.gov/science/USGSThesaurus/microwave%20imaging"/>
    <skos:inScheme rdf:resource="http://www.usgs.gov/science/USGSThesaurus"/>
  </rdf:Description>
  <rdf:Description about="http://www.usgs.gov/science/USGSThesaurus/SLAR">
    <rdf:type rdf:resource="http://www.w3.org/2004/02/skos/core#Concept"/>
    <skos:prefLabel xml:lang="en">SLAR</skos:prefLabel>
    <skos:scopeNote xml:lang="en">Side-looking Airborne Radar, an airborne radar imaging technique, uses an antenna mounted on an airplane or satellite to project radiation at right angles to the flight path and collect high resolution images.</skos:scopeNote>
    <skos:altLabel xml:lang="en">Side-Looking Airborne Radar (SLAR)</skos:altLabel>
    <skos:broader rdf:resource="http://www.usgs.gov/science/USGSThesaurus/radar%20imaging"/>
    <skos:related rdf:resource="http://www.usgs.gov/science/USGSThesaurus/geography"/>
    <skos:inScheme rdf:resource="http://www.usgs.gov/science/USGSThesaurus"/>
  </rdf:Description>
  <rdf:Description about="http://www.usgs.gov/science/USGSThesaurus/doppler%20radar%20imaging">
    <rdf:type rdf:resource="http://www.w3.org/2004/02/skos/core#Concept"/>
    <skos:prefLabel xml:lang="en">doppler radar imaging</skos:prefLabel>
    <skos:scopeNote xml:lang="en">Exploitation of the doppler effect in radar imaging to determine speed of airborne objects such as birds, butterflies, and clouds.</skos:scopeNote>
    <!--FOR radar ecology USE doppler radar imaging WITH population and community ecology-->
    <skos:altLabel xml:lang="en">radar ecology</skos:altLabel>
    <skos:broader rdf:resource="http://www.usgs.gov/science/USGSThesaurus/radar%20imaging"/>
    <skos:inScheme rdf:resource="http://www.usgs.gov/science/USGSThesaurus"/>
  </rdf:Description>
  <rdf:Description about="http://www.usgs.gov/science/USGSThesaurus/thermal%20imaging">
    <rdf:type rdf:resource="http://www.w3.org/2004/02/skos/core#Concept"/>
    <skos:prefLabel xml:lang="en">thermal imaging</skos:prefLabel>
    <skos:scopeNote xml:lang="en">Remote sensing techniques using instruments to measure emitted thermal radiation to form images of the earth's surface.</skos:scopeNote>
    <skos:broader rdf:resource="http://www.usgs.gov/science/USGSThesaurus/remote%20sensing"/>
    <skos:related rdf:resource="http://www.usgs.gov/science/USGSThesaurus/geography"/>
    <skos:inScheme rdf:resource="http://www.usgs.gov/science/USGSThesaurus"/>
  </rdf:Description>
  <rdf:Description about="http://www.usgs.gov/science/USGSThesaurus/visible%20light%20imaging">
    <rdf:type rdf:resource="http://www.w3.org/2004/02/skos/core#Concept"/>
    <skos:prefLabel xml:lang="en">visible light imaging</skos:prefLabel>
    <skos:scopeNote xml:lang="en">Remote sensing methods using electromagnetic radiation which is visible to the human eye to react with the coating on a photographic plate or film.</skos:scopeNote>
    <skos:altLabel xml:lang="en">satellite photography</skos:altLabel>
    <skos:broader rdf:resource="http://www.usgs.gov/science/USGSThesaurus/remote%20sensing"/>
    <skos:related rdf:resource="http://www.usgs.gov/science/USGSThesaurus/geography"/>
    <skos:inScheme rdf:resource="http://www.usgs.gov/science/USGSThesaurus"/>
  </rdf:Description>
  <rdf:Description about="http://www.usgs.gov/science/USGSThesaurus/scientific%20interpretation">
    <rdf:type rdf:resource="http://www.w3.org/2004/02/skos/core#Concept"/>
    <skos:prefLabel xml:lang="en">scientific interpretation</skos:prefLabel>
    <skos:scopeNote xml:lang="en">Application of scientific judgment as to the meaning of observations or models. Use for interpretations that are provided in formats similar to data, such as geospatial data.</skos:scopeNote>
    <skos:broader rdf:resource="http://www.usgs.gov/science/USGSThesaurus/methods"/>
    <skos:inScheme rdf:resource="http://www.usgs.gov/science/USGSThesaurus"/>
  </rdf:Description>
  <rdf:Description about="http://www.usgs.gov/science/USGSThesaurus/videography">
    <rdf:type rdf:resource="http://www.w3.org/2004/02/skos/core#Concept"/>
    <skos:prefLabel xml:lang="en">videography</skos:prefLabel>
    <skos:scopeNote xml:lang="en">The process of recording and editing analog or digital video.</skos:scopeNote>
    <skos:broader rdf:resource="http://www.usgs.gov/science/USGSThesaurus/methods"/>
    <skos:related rdf:resource="http://www.usgs.gov/science/USGSThesaurus/photography"/>
    <skos:related rdf:resource="http://www.usgs.gov/science/USGSThesaurus/remote%20sensing"/>
    <skos:related rdf:resource="http://www.usgs.gov/science/USGSThesaurus/video%20monitoring"/>
    <skos:inScheme rdf:resource="http://www.usgs.gov/science/USGSThesaurus"/>
  </rdf:Description>
  <rdf:Description about="http://www.usgs.gov/science/USGSThesaurus/product%20types">
    <rdf:type rdf:resource="http://www.w3.org/2004/02/skos/core#Concept"/>
    <skos:prefLabel xml:lang="en">product types</skos:prefLabel>
    <skos:scopeNote xml:lang="en">General representation of the information in a resource, such as a map or data set.</skos:scopeNote>
    <skos:broader rdf:resource="http://www.usgs.gov/science/USGSThesaurus/Categories"/>
    <skos:narrower rdf:resource="http://www.usgs.gov/science/USGSThesaurus/animations"/>
    <skos:narrower rdf:resource="http://www.usgs.gov/science/USGSThesaurus/catalogs%20and%20indexes"/>
    <skos:narrower rdf:resource="http://www.usgs.gov/science/USGSThesaurus/datasets"/>
    <skos:narrower rdf:resource="http://www.usgs.gov/science/USGSThesaurus/field%20activity%20logs"/>
    <skos:narrower rdf:resource="http://www.usgs.gov/science/USGSThesaurus/image%20collections"/>
    <skos:narrower rdf:resource="http://www.usgs.gov/science/USGSThesaurus/maps%20and%20atlases"/>
    <skos:narrower rdf:resource="http://www.usgs.gov/science/USGSThesaurus/materials%20standards"/>
    <skos:narrower rdf:resource="http://www.usgs.gov/science/USGSThesaurus/official%20communications"/>
    <skos:narrower rdf:resource="http://www.usgs.gov/science/USGSThesaurus/posters"/>
    <skos:narrower rdf:resource="http://www.usgs.gov/science/USGSThesaurus/presentation%20materials"/>
    <skos:narrower rdf:resource="http://www.usgs.gov/science/USGSThesaurus/reports"/>
    <skos:narrower rdf:resource="http://www.usgs.gov/science/USGSThesaurus/scientific%20software"/>
    <skos:narrower rdf:resource="http://www.usgs.gov/science/USGSThesaurus/sound%20recordings"/>
    <skos:narrower rdf:resource="http://www.usgs.gov/science/USGSThesaurus/terminologies%20and%20classifications"/>
    <skos:narrower rdf:resource="http://www.usgs.gov/science/USGSThesaurus/videos"/>
    <skos:inScheme rdf:resource="http://www.usgs.gov/science/USGSThesaurus"/>
  </rdf:Description>
  <rdf:Description about="http://www.usgs.gov/science/USGSThesaurus/animations">
    <rdf:type rdf:resource="http://www.w3.org/2004/02/skos/core#Concept"/>
    <skos:prefLabel xml:lang="en">animations</skos:prefLabel>
    <skos:scopeNote xml:lang="en">Graphical representation of scientific data presented as a timed sequence of visual images, normally without sound.</skos:scopeNote>
    <skos:broader rdf:resource="http://www.usgs.gov/science/USGSThesaurus/product%20types"/>
    <skos:inScheme rdf:resource="http://www.usgs.gov/science/USGSThesaurus"/>
  </rdf:Description>
  <rdf:Description about="http://www.usgs.gov/science/USGSThesaurus/catalogs%20and%20indexes">
    <rdf:type rdf:resource="http://www.w3.org/2004/02/skos/core#Concept"/>
    <skos:prefLabel xml:lang="en">catalogs and indexes</skos:prefLabel>
    <skos:scopeNote xml:lang="en">Detailed enumeration of related items listed in a given order, or alphabetical lists of topics used for information retrieval.</skos:scopeNote>
    <skos:altLabel xml:lang="en">indexes</skos:altLabel>
    <skos:altLabel xml:lang="en">lists of publications</skos:altLabel>
    <skos:altLabel xml:lang="en">metadata</skos:altLabel>
    <!--FOR clearinghouses USE catalogs and indexes WITH information services-->
    <skos:altLabel xml:lang="en">clearinghouses</skos:altLabel>
    <skos:broader rdf:resource="http://www.usgs.gov/science/USGSThesaurus/product%20types"/>
    <skos:narrower rdf:resource="http://www.usgs.gov/science/USGSThesaurus/bibliographies"/>
    <skos:narrower rdf:resource="http://www.usgs.gov/science/USGSThesaurus/directories"/>
    <skos:narrower rdf:resource="http://www.usgs.gov/science/USGSThesaurus/gazetteers"/>
    <skos:related rdf:resource="http://www.usgs.gov/science/USGSThesaurus/reports"/>
    <skos:inScheme rdf:resource="http://www.usgs.gov/science/USGSThesaurus"/>
  </rdf:Description>
  <rdf:Description about="http://www.usgs.gov/science/USGSThesaurus/bibliographies">
    <rdf:type rdf:resource="http://www.w3.org/2004/02/skos/core#Concept"/>
    <skos:prefLabel xml:lang="en">bibliographies</skos:prefLabel>
    <skos:scopeNote xml:lang="en">List of publications on a given topic, by an author or group, or published in a specific time period. Limited here to lists primarily of paper documents.</skos:scopeNote>
    <skos:broader rdf:resource="http://www.usgs.gov/science/USGSThesaurus/catalogs%20and%20indexes"/>
    <skos:related rdf:resource="http://www.usgs.gov/science/USGSThesaurus/reports"/>
    <skos:inScheme rdf:resource="http://www.usgs.gov/science/USGSThesaurus"/>
  </rdf:Description>
  <rdf:Description about="http://www.usgs.gov/science/USGSThesaurus/directories">
    <rdf:type rdf:resource="http://www.w3.org/2004/02/skos/core#Concept"/>
    <skos:prefLabel xml:lang="en">directories</skos:prefLabel>
    <skos:scopeNote xml:lang="en">Searchable lists of people, typically USGS staff.</skos:scopeNote>
    <skos:broader rdf:resource="http://www.usgs.gov/science/USGSThesaurus/catalogs%20and%20indexes"/>
    <skos:related rdf:resource="http://www.usgs.gov/science/USGSThesaurus/reports"/>
    <skos:inScheme rdf:resource="http://www.usgs.gov/science/USGSThesaurus"/>
  </rdf:Description>
  <rdf:Description about="http://www.usgs.gov/science/USGSThesaurus/gazetteers">
    <rdf:type rdf:resource="http://www.w3.org/2004/02/skos/core#Concept"/>
    <skos:prefLabel xml:lang="en">gazetteers</skos:prefLabel>
    <skos:scopeNote xml:lang="en">Indexed collections of geographic names.</skos:scopeNote>
    <skos:broader rdf:resource="http://www.usgs.gov/science/USGSThesaurus/catalogs%20and%20indexes"/>
    <skos:related rdf:resource="http://www.usgs.gov/science/USGSThesaurus/geographic%20names"/>
    <skos:inScheme rdf:resource="http://www.usgs.gov/science/USGSThesaurus"/>
  </rdf:Description>
  <rdf:Description about="http://www.usgs.gov/science/USGSThesaurus/datasets">
    <rdf:type rdf:resource="http://www.w3.org/2004/02/skos/core#Concept"/>
    <skos:prefLabel xml:lang="en">datasets</skos:prefLabel>
    <skos:scopeNote xml:lang="en">Digital information in a format suitable for direct input to software that can analyze its meaning in the scientific, engineering, or business context for which the data were collected.</skos:scopeNote>
    <skos:altLabel xml:lang="en">data</skos:altLabel>
    <skos:altLabel xml:lang="en">databases</skos:altLabel>
    <!--FOR streamflow data USE datasets WITH streamflow-->
    <skos:altLabel xml:lang="en">streamflow data</skos:altLabel>
    <!--FOR water-quality data USE datasets WITH water quality-->
    <skos:altLabel xml:lang="en">water-quality data</skos:altLabel>
    <skos:broader rdf:resource="http://www.usgs.gov/science/USGSThesaurus/product%20types"/>
    <skos:narrower rdf:resource="http://www.usgs.gov/science/USGSThesaurus/geospatial%20datasets"/>
    <skos:narrower rdf:resource="http://www.usgs.gov/science/USGSThesaurus/hydrographic%20datasets"/>
    <skos:narrower rdf:resource="http://www.usgs.gov/science/USGSThesaurus/profiles"/>
    <skos:narrower rdf:resource="http://www.usgs.gov/science/USGSThesaurus/time%20series%20datasets"/>
    <skos:inScheme rdf:resource="http://www.usgs.gov/science/USGSThesaurus"/>
  </rdf:Description>
  <rdf:Description about="http://www.usgs.gov/science/USGSThesaurus/geospatial%20datasets">
    <rdf:type rdf:resource="http://www.w3.org/2004/02/skos/core#Concept"/>
    <skos:prefLabel xml:lang="en">geospatial datasets</skos:prefLabel>
    <skos:scopeNote xml:lang="en">Collections of related digital information that are geographically referenced.</skos:scopeNote>
    <skos:altLabel xml:lang="en">DLG</skos:altLabel>
    <skos:altLabel xml:lang="en">GIS datasets</skos:altLabel>
    <skos:altLabel xml:lang="en">cartographic data (digital)</skos:altLabel>
    <skos:altLabel xml:lang="en">digital cartographic data</skos:altLabel>
    <skos:altLabel xml:lang="en">digital cartographic datasets</skos:altLabel>
    <skos:altLabel xml:lang="en">digital line graphs</skos:altLabel>
    <skos:altLabel xml:lang="en">geodata</skos:altLabel>
    <skos:altLabel xml:lang="en">geographic information system (GIS) datasets</skos:altLabel>
    <skos:altLabel xml:lang="en">geospatial data</skos:altLabel>
    <skos:broader rdf:resource="http://www.usgs.gov/science/USGSThesaurus/datasets"/>
    <skos:narrower rdf:resource="http://www.usgs.gov/science/USGSThesaurus/digital%20elevation%20models"/>
    <skos:narrower rdf:resource="http://www.usgs.gov/science/USGSThesaurus/navigational%20data"/>
    <skos:related rdf:resource="http://www.usgs.gov/science/USGSThesaurus/geographic%20information%20systems"/>
    <skos:related rdf:resource="http://www.usgs.gov/science/USGSThesaurus/hydrographic%20datasets"/>
    <skos:related rdf:resource="http://www.usgs.gov/science/USGSThesaurus/topography"/>
    <skos:inScheme rdf:resource="http://www.usgs.gov/science/USGSThesaurus"/>
  </rdf:Description>
  <rdf:Description about="http://www.usgs.gov/science/USGSThesaurus/digital%20elevation%20models">
    <rdf:type rdf:resource="http://www.w3.org/2004/02/skos/core#Concept"/>
    <skos:prefLabel xml:lang="en">digital elevation models</skos:prefLabel>
    <skos:scopeNote xml:lang="en">Gridded elevation, geographically referenced to the surface of the earth, as digital data</skos:scopeNote>
    <skos:altLabel xml:lang="en">digital terrain models</skos:altLabel>
    <skos:altLabel xml:lang="en">digital depth models</skos:altLabel>
    <skos:altLabel xml:lang="en">DEMs</skos:altLabel>
    <skos:altLabel xml:lang="en">DTMs</skos:altLabel>
    <skos:altLabel xml:lang="en">DDMs</skos:altLabel>
    <skos:broader rdf:resource="http://www.usgs.gov/science/USGSThesaurus/geospatial%20datasets"/>
    <skos:inScheme rdf:resource="http://www.usgs.gov/science/USGSThesaurus"/>
  </rdf:Description>
  <rdf:Description about="http://www.usgs.gov/science/USGSThesaurus/navigational%20data">
    <rdf:type rdf:resource="http://www.w3.org/2004/02/skos/core#Concept"/>
    <skos:prefLabel xml:lang="en">navigational data</skos:prefLabel>
    <skos:scopeNote xml:lang="en">Geospatial data indicating the locations of instruments, vessels, aircraft, or other vehicles used to collect scientific observations.  These data include horizontal coordinates in sequence, and may include time or vertical position.</skos:scopeNote>
    <skos:altLabel xml:lang="en">survey tracklines</skos:altLabel>
    <skos:altLabel xml:lang="en">survey ship tracklines</skos:altLabel>
    <skos:altLabel xml:lang="en">ship tracklines</skos:altLabel>
    <skos:altLabel xml:lang="en">survey tracks</skos:altLabel>
    <skos:altLabel xml:lang="en">ship tracks</skos:altLabel>
    <skos:altLabel xml:lang="en">survey flight lines</skos:altLabel>
    <skos:altLabel xml:lang="en">flight lines</skos:altLabel>
    <skos:broader rdf:resource="http://www.usgs.gov/science/USGSThesaurus/geospatial%20datasets"/>
    <skos:inScheme rdf:resource="http://www.usgs.gov/science/USGSThesaurus"/>
  </rdf:Description>
  <rdf:Description about="http://www.usgs.gov/science/USGSThesaurus/hydrographic%20datasets">
    <rdf:type rdf:resource="http://www.w3.org/2004/02/skos/core#Concept"/>
    <skos:prefLabel xml:lang="en">hydrographic datasets</skos:prefLabel>
    <skos:scopeNote xml:lang="en">Datasets for graphs showing variation of water elevation, velocity, streamflow, or other property of water with respect to time.</skos:scopeNote>
    <skos:broader rdf:resource="http://www.usgs.gov/science/USGSThesaurus/datasets"/>
    <skos:related rdf:resource="http://www.usgs.gov/science/USGSThesaurus/geospatial%20datasets"/>
    <skos:inScheme rdf:resource="http://www.usgs.gov/science/USGSThesaurus"/>
  </rdf:Description>
  <rdf:Description about="http://www.usgs.gov/science/USGSThesaurus/profiles">
    <rdf:type rdf:resource="http://www.w3.org/2004/02/skos/core#Concept"/>
    <skos:prefLabel xml:lang="en">profiles</skos:prefLabel>
    <skos:scopeNote xml:lang="en">Observations or calculations given for a series of depths, at or near the same horizontal position.</skos:scopeNote>
    <!--FOR sound velocity profiles USE profiles WITH sound velocity-->
    <skos:altLabel xml:lang="en">sound velocity profiles</skos:altLabel>
    <skos:broader rdf:resource="http://www.usgs.gov/science/USGSThesaurus/datasets"/>
    <skos:related rdf:resource="http://www.usgs.gov/science/USGSThesaurus/sub-bottom%20profiling"/>
    <skos:related rdf:resource="http://www.usgs.gov/science/USGSThesaurus/borehole%20logging"/>
    <skos:inScheme rdf:resource="http://www.usgs.gov/science/USGSThesaurus"/>
  </rdf:Description>
  <rdf:Description about="http://www.usgs.gov/science/USGSThesaurus/time%20series%20datasets">
    <rdf:type rdf:resource="http://www.w3.org/2004/02/skos/core#Concept"/>
    <skos:prefLabel xml:lang="en">time series datasets</skos:prefLabel>
    <skos:scopeNote xml:lang="en">Digital information describing observations taken at regular time intervals.  The time interval may vary; the type of observed phenomena and the location typically do not.</skos:scopeNote>
    <skos:broader rdf:resource="http://www.usgs.gov/science/USGSThesaurus/datasets"/>
    <skos:related rdf:resource="http://www.usgs.gov/science/USGSThesaurus/time%20series%20analysis"/>
    <skos:inScheme rdf:resource="http://www.usgs.gov/science/USGSThesaurus"/>
  </rdf:Description>
  <rdf:Description about="http://www.usgs.gov/science/USGSThesaurus/field%20activity%20logs">
    <rdf:type rdf:resource="http://www.w3.org/2004/02/skos/core#Concept"/>
    <skos:prefLabel xml:lang="en">field activity logs</skos:prefLabel>
    <skos:scopeNote xml:lang="en">Operational records for observation, inventory, sampling, or monitoring activities.</skos:scopeNote>
    <skos:altLabel xml:lang="en">field notebooks</skos:altLabel>
    <skos:altLabel xml:lang="en">operational logs</skos:altLabel>
    <skos:altLabel xml:lang="en">survey logs</skos:altLabel>
    <skos:altLabel xml:lang="en">logbooks</skos:altLabel>
    <skos:altLabel xml:lang="en">field notes</skos:altLabel>
    <skos:altLabel xml:lang="en">observation logs</skos:altLabel>
    <skos:altLabel xml:lang="en">log books</skos:altLabel>
    <skos:broader rdf:resource="http://www.usgs.gov/science/USGSThesaurus/product%20types"/>
    <skos:inScheme rdf:resource="http://www.usgs.gov/science/USGSThesaurus"/>
  </rdf:Description>
  <rdf:Description about="http://www.usgs.gov/science/USGSThesaurus/image%20collections">
    <rdf:type rdf:resource="http://www.w3.org/2004/02/skos/core#Concept"/>
    <skos:prefLabel xml:lang="en">image collections</skos:prefLabel>
    <skos:scopeNote xml:lang="en">Visible representations of objects or earth properties produced by cameras, spectral instruments, or as graphical representations of measurements.</skos:scopeNote>
    <!--FOR aerial photos USE image collections WITH aerial photography-->
    <skos:altLabel xml:lang="en">aerial photos</skos:altLabel>
    <!--FOR air photos USE image collections WITH aerial photography-->
    <skos:altLabel xml:lang="en">air photos</skos:altLabel>
    <!--FOR orthoimagery USE image collections WITH aerial photography-->
    <skos:altLabel xml:lang="en">orthoimagery</skos:altLabel>
    <!--FOR orthophotographs USE image collections WITH aerial photography-->
    <skos:altLabel xml:lang="en">orthophotographs</skos:altLabel>
    <!--FOR AVHRR images USE image collections WITH AVHRR-->
    <skos:altLabel xml:lang="en">AVHRR images</skos:altLabel>
    <!--FOR LIDAR images USE image collections WITH LIDAR-->
    <skos:altLabel xml:lang="en">LIDAR images</skos:altLabel>
    <!--FOR Landsat images USE image collections WITH multispectral imaging-->
    <skos:altLabel xml:lang="en">Landsat images</skos:altLabel>
    <!--FOR aerial photographs USE image collections WITH aerial photography-->
    <skos:altLabel xml:lang="en">aerial photographs</skos:altLabel>
    <!--FOR photographs USE image collections WITH photography-->
    <skos:altLabel xml:lang="en">photographs</skos:altLabel>
    <skos:altLabel xml:lang="en">pictures</skos:altLabel>
    <!--FOR scientists-at-work photographs USE image collections WITH scientific careers-->
    <skos:altLabel xml:lang="en">scientists-at-work photographs</skos:altLabel>
    <!--FOR remote-sensing data USE image collections WITH remote sensing-->
    <skos:altLabel xml:lang="en">remote-sensing data</skos:altLabel>
    <!--FOR remote-sensing images USE image collections WITH remote sensing-->
    <skos:altLabel xml:lang="en">remote-sensing images</skos:altLabel>
    <!--FOR satellite images USE image collections WITH remote sensing-->
    <skos:altLabel xml:lang="en">satellite images</skos:altLabel>
    <skos:broader rdf:resource="http://www.usgs.gov/science/USGSThesaurus/product%20types"/>
    <skos:narrower rdf:resource="http://www.usgs.gov/science/USGSThesaurus/image%20mosaics"/>
    <skos:inScheme rdf:resource="http://www.usgs.gov/science/USGSThesaurus"/>
  </rdf:Description>
  <rdf:Description about="http://www.usgs.gov/science/USGSThesaurus/image%20mosaics">
    <rdf:type rdf:resource="http://www.w3.org/2004/02/skos/core#Concept"/>
    <skos:prefLabel xml:lang="en">image mosaics</skos:prefLabel>
    <skos:scopeNote xml:lang="en">Composite images formed by overlapping existing images, typically arranged to achieve greater spatial coverage.</skos:scopeNote>
    <!--FOR sidescan sonar mosaics USE image mosaics WITH sidescan sonar-->
    <skos:altLabel xml:lang="en">sidescan sonar mosaics</skos:altLabel>
    <skos:broader rdf:resource="http://www.usgs.gov/science/USGSThesaurus/image%20collections"/>
    <skos:inScheme rdf:resource="http://www.usgs.gov/science/USGSThesaurus"/>
  </rdf:Description>
  <rdf:Description about="http://www.usgs.gov/science/USGSThesaurus/maps%20and%20atlases">
    <rdf:type rdf:resource="http://www.w3.org/2004/02/skos/core#Concept"/>
    <skos:prefLabel xml:lang="en">maps and atlases</skos:prefLabel>
    <skos:scopeNote xml:lang="en">Representation, usually on a flat surface, of a part or whole of the Earth or other parts of the universe.  Collections of maps linked digitally or bound together in a book are called atlases.</skos:scopeNote>
    <!--FOR cadastral maps USE maps and atlases WITH cadastral and legal land descriptions-->
    <skos:altLabel xml:lang="en">cadastral maps</skos:altLabel>
    <!--FOR earthquake activity maps USE maps and atlases WITH earthquake occurrences-->
    <skos:altLabel xml:lang="en">earthquake activity maps</skos:altLabel>
    <!--FOR ground motion maps USE maps and atlases WITH earthquake occurrences-->
    <skos:altLabel xml:lang="en">ground motion maps</skos:altLabel>
    <!--FOR seismic hazard maps USE maps and atlases WITH earthquake occurrences-->
    <skos:altLabel xml:lang="en">seismic hazard maps</skos:altLabel>
    <!--FOR shaking maps (seismic) USE maps and atlases WITH earthquake occurrences-->
    <skos:altLabel xml:lang="en">shaking maps (seismic)</skos:altLabel>
    <!--FOR earthquake epicenter maps USE maps and atlases WITH earthquake occurrences-->
    <skos:altLabel xml:lang="en">earthquake epicenter maps</skos:altLabel>
    <!--FOR engineering geology maps USE maps and atlases WITH engineering geology-->
    <skos:altLabel xml:lang="en">engineering geology maps</skos:altLabel>
    <!--FOR geotechnical properties maps USE maps and atlases WITH engineering geology-->
    <skos:altLabel xml:lang="en">geotechnical properties maps</skos:altLabel>
    <!--FOR rock mechanics maps USE maps and atlases WITH engineering geology-->
    <skos:altLabel xml:lang="en">rock mechanics maps</skos:altLabel>
    <!--FOR subsurface maps USE maps and atlases WITH geology-->
    <skos:altLabel xml:lang="en">subsurface maps</skos:altLabel>
    <!--FOR geophysical maps USE maps and atlases WITH geophysics-->
    <skos:altLabel xml:lang="en">geophysical maps</skos:altLabel>
    <!--FOR land subsidence maps USE maps and atlases WITH subsidence-->
    <skos:altLabel xml:lang="en">land subsidence maps</skos:altLabel>
    <!--FOR slope stability maps USE maps and atlases WITH landslide susceptibility assessment-->
    <skos:altLabel xml:lang="en">slope stability maps</skos:altLabel>
    <!--FOR aeromagnetic maps USE maps and atlases WITH aeromagnetic surveying-->
    <skos:altLabel xml:lang="en">aeromagnetic maps</skos:altLabel>
    <skos:altLabel xml:lang="en">atlases</skos:altLabel>
    <!--FOR basement maps USE maps and atlases WITH bedrock geologic units-->
    <skos:altLabel xml:lang="en">basement maps</skos:altLabel>
    <!--FOR depth-to maps USE maps and atlases WITH structure contours-->
    <skos:altLabel xml:lang="en">depth-to maps</skos:altLabel>
    <!--FOR earthquake occurrence maps USE maps and atlases WITH earthquake occurrences-->
    <skos:altLabel xml:lang="en">earthquake occurrence maps</skos:altLabel>
    <!--FOR geochemical anomaly maps USE maps and atlases WITH geochemistry-->
    <skos:altLabel xml:lang="en">geochemical anomaly maps</skos:altLabel>
    <!--FOR gravity anomaly maps USE maps and atlases WITH gravitational field (earth)-->
    <skos:altLabel xml:lang="en">gravity anomaly maps</skos:altLabel>
    <!--FOR hydrologic maps USE maps and atlases WITH hydrology-->
    <skos:altLabel xml:lang="en">hydrologic maps</skos:altLabel>
    <skos:altLabel xml:lang="en">land use maps</skos:altLabel>
    <!--FOR landslide maps USE maps and atlases WITH landslides-->
    <skos:altLabel xml:lang="en">landslide maps</skos:altLabel>
    <!--FOR landslide susceptibility maps USE maps and atlases WITH landslide susceptibility assessment-->
    <skos:altLabel xml:lang="en">landslide susceptibility maps</skos:altLabel>
    <!--FOR lithologic maps USE maps and atlases WITH rocks and deposits-->
    <skos:altLabel xml:lang="en">lithologic maps</skos:altLabel>
    <!--FOR magnetic anomaly maps USE maps and atlases WITH magnetic field (earth)-->
    <skos:altLabel xml:lang="en">magnetic anomaly maps</skos:altLabel>
    <skos:altLabel xml:lang="en">maps</skos:altLabel>
    <!--FOR paleotectonic maps USE maps and atlases WITH tectonic processes-->
    <skos:altLabel xml:lang="en">paleotectonic maps</skos:altLabel>
    <!--FOR seismic reflection survey maps USE maps and atlases WITH seismic reflection methods-->
    <skos:altLabel xml:lang="en">seismic reflection survey maps</skos:altLabel>
    <!--FOR species distribution maps USE maps and atlases WITH biogeography-->
    <skos:altLabel xml:lang="en">species distribution maps</skos:altLabel>
    <!--FOR surficial geologic maps USE maps and atlases WITH surficial geologic units-->
    <skos:altLabel xml:lang="en">surficial geologic maps</skos:altLabel>
    <!--FOR tectonic maps USE maps and atlases WITH tectonic processes-->
    <skos:altLabel xml:lang="en">tectonic maps</skos:altLabel>
    <!--FOR thickness maps USE maps and atlases WITH structure contours-->
    <skos:altLabel xml:lang="en">thickness maps</skos:altLabel>
    <skos:altLabel xml:lang="en">charts</skos:altLabel>
    <!--FOR seismicity maps USE maps and atlases WITH earthquake probabilities-->
    <skos:altLabel xml:lang="en">seismicity maps</skos:altLabel>
    <skos:broader rdf:resource="http://www.usgs.gov/science/USGSThesaurus/product%20types"/>
    <skos:narrower rdf:resource="http://www.usgs.gov/science/USGSThesaurus/geologic%20maps"/>
    <skos:narrower rdf:resource="http://www.usgs.gov/science/USGSThesaurus/topographic%20maps"/>
    <skos:related rdf:resource="http://www.usgs.gov/science/USGSThesaurus/cartography"/>
    <skos:inScheme rdf:resource="http://www.usgs.gov/science/USGSThesaurus"/>
  </rdf:Description>
  <rdf:Description about="http://www.usgs.gov/science/USGSThesaurus/geologic%20maps">
    <rdf:type rdf:resource="http://www.w3.org/2004/02/skos/core#Concept"/>
    <skos:prefLabel xml:lang="en">geologic maps</skos:prefLabel>
    <skos:scopeNote xml:lang="en">Maps depicting geological characteristics of the earth's surface, including lithology, geologic structure, age, and the results of crustal processes.</skos:scopeNote>
    <skos:altLabel xml:lang="en">geological maps</skos:altLabel>
    <skos:broader rdf:resource="http://www.usgs.gov/science/USGSThesaurus/maps%20and%20atlases"/>
    <skos:related rdf:resource="http://www.usgs.gov/science/USGSThesaurus/geologic%20structure"/>
    <skos:related rdf:resource="http://www.usgs.gov/science/USGSThesaurus/bedrock%20geologic%20units"/>
    <skos:related rdf:resource="http://www.usgs.gov/science/USGSThesaurus/surficial%20geologic%20units"/>
    <skos:related rdf:resource="http://www.usgs.gov/science/USGSThesaurus/geologic%20contacts"/>
    <skos:related rdf:resource="http://www.usgs.gov/science/USGSThesaurus/geology"/>
    <skos:inScheme rdf:resource="http://www.usgs.gov/science/USGSThesaurus"/>
  </rdf:Description>
  <rdf:Description about="http://www.usgs.gov/science/USGSThesaurus/topographic%20maps">
    <rdf:type rdf:resource="http://www.w3.org/2004/02/skos/core#Concept"/>
    <skos:prefLabel xml:lang="en">topographic maps</skos:prefLabel>
    <skos:scopeNote xml:lang="en">Maps depicting the elevation and relief of the land surface or depth of a water body (bathymetry) in an area, usually shown using contour lines.  Typically these maps include manmade features and administrative boundaries as well as vegetation and hydrographic features.</skos:scopeNote>
    <skos:altLabel xml:lang="en">elevation maps</skos:altLabel>
    <skos:altLabel xml:lang="en">topo maps</skos:altLabel>
    <skos:altLabel xml:lang="en">bathymetric maps</skos:altLabel>
    <skos:broader rdf:resource="http://www.usgs.gov/science/USGSThesaurus/maps%20and%20atlases"/>
    <skos:related rdf:resource="http://www.usgs.gov/science/USGSThesaurus/topography"/>
    <skos:inScheme rdf:resource="http://www.usgs.gov/science/USGSThesaurus"/>
  </rdf:Description>
  <rdf:Description about="http://www.usgs.gov/science/USGSThesaurus/materials%20standards">
    <rdf:type rdf:resource="http://www.w3.org/2004/02/skos/core#Concept"/>
    <skos:prefLabel xml:lang="en">materials standards</skos:prefLabel>
    <skos:scopeNote xml:lang="en">Physical materials such as chemicals, rocks, water, or biological materials that are used for reference when carrying out laboratory analysis.</skos:scopeNote>
    <skos:altLabel xml:lang="en">laboratory reference materials</skos:altLabel>
    <skos:altLabel xml:lang="en">standard reference samples</skos:altLabel>
    <skos:broader rdf:resource="http://www.usgs.gov/science/USGSThesaurus/product%20types"/>
    <skos:inScheme rdf:resource="http://www.usgs.gov/science/USGSThesaurus"/>
  </rdf:Description>
  <rdf:Description about="http://www.usgs.gov/science/USGSThesaurus/official%20communications">
    <rdf:type rdf:resource="http://www.w3.org/2004/02/skos/core#Concept"/>
    <skos:prefLabel xml:lang="en">official communications</skos:prefLabel>
    <skos:scopeNote xml:lang="en">Corporate releases of information by USGS not generally intended to document the details of scientific data or techniques for a scientific audience.</skos:scopeNote>
    <skos:broader rdf:resource="http://www.usgs.gov/science/USGSThesaurus/product%20types"/>
    <skos:narrower rdf:resource="http://www.usgs.gov/science/USGSThesaurus/news%20releases"/>
    <skos:narrower rdf:resource="http://www.usgs.gov/science/USGSThesaurus/policies%20and%20regulations"/>
    <skos:narrower rdf:resource="http://www.usgs.gov/science/USGSThesaurus/speeches%20and%20testimony"/>
    <skos:inScheme rdf:resource="http://www.usgs.gov/science/USGSThesaurus"/>
  </rdf:Description>
  <rdf:Description about="http://www.usgs.gov/science/USGSThesaurus/news%20releases">
    <rdf:type rdf:resource="http://www.w3.org/2004/02/skos/core#Concept"/>
    <skos:prefLabel xml:lang="en">news releases</skos:prefLabel>
    <skos:scopeNote xml:lang="en">Short information memoranda issued by organizations to highlight new activities, appointments, or discoveries for the news media.</skos:scopeNote>
    <skos:altLabel xml:lang="en">press releases</skos:altLabel>
    <skos:broader rdf:resource="http://www.usgs.gov/science/USGSThesaurus/official%20communications"/>
    <skos:inScheme rdf:resource="http://www.usgs.gov/science/USGSThesaurus"/>
  </rdf:Description>
  <rdf:Description about="http://www.usgs.gov/science/USGSThesaurus/policies%20and%20regulations">
    <rdf:type rdf:resource="http://www.w3.org/2004/02/skos/core#Concept"/>
    <skos:prefLabel xml:lang="en">policies and regulations</skos:prefLabel>
    <skos:scopeNote xml:lang="en">Rules, orders, and procedures issued by organizations or governments for administrative, controlling, and managing purposes.</skos:scopeNote>
    <skos:altLabel xml:lang="en">regulations</skos:altLabel>
    <skos:broader rdf:resource="http://www.usgs.gov/science/USGSThesaurus/official%20communications"/>
    <skos:related rdf:resource="http://www.usgs.gov/science/USGSThesaurus/reports"/>
    <skos:inScheme rdf:resource="http://www.usgs.gov/science/USGSThesaurus"/>
  </rdf:Description>
  <rdf:Description about="http://www.usgs.gov/science/USGSThesaurus/speeches%20and%20testimony">
    <rdf:type rdf:resource="http://www.w3.org/2004/02/skos/core#Concept"/>
    <skos:prefLabel xml:lang="en">speeches and testimony</skos:prefLabel>
    <skos:scopeNote xml:lang="en"></skos:scopeNote>
    <skos:altLabel xml:lang="en">oral presentations</skos:altLabel>
    <skos:altLabel xml:lang="en">talks</skos:altLabel>
    <skos:altLabel xml:lang="en">testimony</skos:altLabel>
    <skos:broader rdf:resource="http://www.usgs.gov/science/USGSThesaurus/official%20communications"/>
    <skos:inScheme rdf:resource="http://www.usgs.gov/science/USGSThesaurus"/>
  </rdf:Description>
  <rdf:Description about="http://www.usgs.gov/science/USGSThesaurus/posters">
    <rdf:type rdf:resource="http://www.w3.org/2004/02/skos/core#Concept"/>
    <skos:prefLabel xml:lang="en">posters</skos:prefLabel>
    <skos:scopeNote xml:lang="en">Large single sheets of paper or board imprinted with informative text and graphics. Intended for hanging or flat display.</skos:scopeNote>
    <skos:broader rdf:resource="http://www.usgs.gov/science/USGSThesaurus/product%20types"/>
    <skos:inScheme rdf:resource="http://www.usgs.gov/science/USGSThesaurus"/>
  </rdf:Description>
  <rdf:Description about="http://www.usgs.gov/science/USGSThesaurus/presentation%20materials">
    <rdf:type rdf:resource="http://www.w3.org/2004/02/skos/core#Concept"/>
    <skos:prefLabel xml:lang="en">presentation materials</skos:prefLabel>
    <skos:scopeNote xml:lang="en">Diagrams, photos, and text gathered together as part of a presentation given in a meeting or class.</skos:scopeNote>
    <skos:altLabel xml:lang="en">powerpoint</skos:altLabel>
    <skos:broader rdf:resource="http://www.usgs.gov/science/USGSThesaurus/product%20types"/>
    <skos:inScheme rdf:resource="http://www.usgs.gov/science/USGSThesaurus"/>
  </rdf:Description>
  <rdf:Description about="http://www.usgs.gov/science/USGSThesaurus/reports">
    <rdf:type rdf:resource="http://www.w3.org/2004/02/skos/core#Concept"/>
    <skos:prefLabel xml:lang="en">reports</skos:prefLabel>
    <skos:scopeNote xml:lang="en">Written items, especially those that are official, factual, or informative, often including graphics as well as text.</skos:scopeNote>
    <skos:altLabel xml:lang="en">abstracts</skos:altLabel>
    <skos:altLabel xml:lang="en">articles (publications)</skos:altLabel>
    <skos:altLabel xml:lang="en">biographies</skos:altLabel>
    <skos:altLabel xml:lang="en">books and book chapters</skos:altLabel>
    <skos:altLabel xml:lang="en">dissertations</skos:altLabel>
    <skos:altLabel xml:lang="en">documents</skos:altLabel>
    <skos:altLabel xml:lang="en">guidelines</skos:altLabel>
    <skos:altLabel xml:lang="en">journal articles</skos:altLabel>
    <skos:altLabel xml:lang="en">journals</skos:altLabel>
    <skos:altLabel xml:lang="en">memos</skos:altLabel>
    <skos:altLabel xml:lang="en">newsletters</skos:altLabel>
    <skos:altLabel xml:lang="en">pamphlets, brochures, and booklets</skos:altLabel>
    <skos:altLabel xml:lang="en">papers (publications)</skos:altLabel>
    <skos:altLabel xml:lang="en">planning reports</skos:altLabel>
    <skos:altLabel xml:lang="en">proceedings</skos:altLabel>
    <skos:altLabel xml:lang="en">published series</skos:altLabel>
    <skos:altLabel xml:lang="en">scientific reports</skos:altLabel>
    <skos:altLabel xml:lang="en">serial publications</skos:altLabel>
    <skos:altLabel xml:lang="en">technical reports</skos:altLabel>
    <skos:altLabel xml:lang="en">text documents</skos:altLabel>
    <skos:altLabel xml:lang="en">theses</skos:altLabel>
    <skos:altLabel xml:lang="en">transcripts</skos:altLabel>
    <skos:altLabel xml:lang="en">workshop reports</skos:altLabel>
    <skos:altLabel xml:lang="en">yearbooks</skos:altLabel>
    <skos:broader rdf:resource="http://www.usgs.gov/science/USGSThesaurus/product%20types"/>
    <skos:narrower rdf:resource="http://www.usgs.gov/science/USGSThesaurus/checklists"/>
    <skos:narrower rdf:resource="http://www.usgs.gov/science/USGSThesaurus/conference%20proceedings"/>
    <skos:narrower rdf:resource="http://www.usgs.gov/science/USGSThesaurus/guidebooks"/>
    <skos:narrower rdf:resource="http://www.usgs.gov/science/USGSThesaurus/manuals"/>
    <skos:narrower rdf:resource="http://www.usgs.gov/science/USGSThesaurus/standards"/>
    <skos:narrower rdf:resource="http://www.usgs.gov/science/USGSThesaurus/strategic%20plans"/>
    <skos:related rdf:resource="http://www.usgs.gov/science/USGSThesaurus/bibliographies"/>
    <skos:related rdf:resource="http://www.usgs.gov/science/USGSThesaurus/catalogs%20and%20indexes"/>
    <skos:related rdf:resource="http://www.usgs.gov/science/USGSThesaurus/directories"/>
    <skos:related rdf:resource="http://www.usgs.gov/science/USGSThesaurus/policies%20and%20regulations"/>
    <skos:inScheme rdf:resource="http://www.usgs.gov/science/USGSThesaurus"/>
  </rdf:Description>
  <rdf:Description about="http://www.usgs.gov/science/USGSThesaurus/checklists">
    <rdf:type rdf:resource="http://www.w3.org/2004/02/skos/core#Concept"/>
    <skos:prefLabel xml:lang="en">checklists</skos:prefLabel>
    <skos:scopeNote xml:lang="en">Inventories or lists of related items for checking off or reference.</skos:scopeNote>
    <skos:broader rdf:resource="http://www.usgs.gov/science/USGSThesaurus/reports"/>
    <skos:inScheme rdf:resource="http://www.usgs.gov/science/USGSThesaurus"/>
  </rdf:Description>
  <rdf:Description about="http://www.usgs.gov/science/USGSThesaurus/conference%20proceedings">
    <rdf:type rdf:resource="http://www.w3.org/2004/02/skos/core#Concept"/>
    <skos:prefLabel xml:lang="en">conference proceedings</skos:prefLabel>
    <skos:scopeNote xml:lang="en">Collections of abstracts or papers given during a specific meeting, conference, or workshop.</skos:scopeNote>
    <skos:broader rdf:resource="http://www.usgs.gov/science/USGSThesaurus/reports"/>
    <skos:inScheme rdf:resource="http://www.usgs.gov/science/USGSThesaurus"/>
  </rdf:Description>
  <rdf:Description about="http://www.usgs.gov/science/USGSThesaurus/guidebooks">
    <rdf:type rdf:resource="http://www.w3.org/2004/02/skos/core#Concept"/>
    <skos:prefLabel xml:lang="en">guidebooks</skos:prefLabel>
    <skos:scopeNote xml:lang="en">Books intended to direct and instruct travelers in a given area and often geared to special interests, such as observing local birds, understanding geological features, or locating endemic plants.</skos:scopeNote>
    <skos:altLabel xml:lang="en">field trip guidebooks</skos:altLabel>
    <skos:altLabel xml:lang="en">field guides</skos:altLabel>
    <skos:broader rdf:resource="http://www.usgs.gov/science/USGSThesaurus/reports"/>
    <skos:inScheme rdf:resource="http://www.usgs.gov/science/USGSThesaurus"/>
  </rdf:Description>
  <rdf:Description about="http://www.usgs.gov/science/USGSThesaurus/manuals">
    <rdf:type rdf:resource="http://www.w3.org/2004/02/skos/core#Concept"/>
    <skos:prefLabel xml:lang="en">manuals</skos:prefLabel>
    <skos:scopeNote xml:lang="en">Documents giving instructions on using specified equipment or accomplishing specified tasks.</skos:scopeNote>
    <skos:altLabel xml:lang="en">technical instructions</skos:altLabel>
    <skos:altLabel xml:lang="en">user guides</skos:altLabel>
    <skos:broader rdf:resource="http://www.usgs.gov/science/USGSThesaurus/reports"/>
    <skos:inScheme rdf:resource="http://www.usgs.gov/science/USGSThesaurus"/>
  </rdf:Description>
  <rdf:Description about="http://www.usgs.gov/science/USGSThesaurus/standards">
    <rdf:type rdf:resource="http://www.w3.org/2004/02/skos/core#Concept"/>
    <skos:prefLabel xml:lang="en">standards</skos:prefLabel>
    <skos:scopeNote xml:lang="en">An object or instrument of known properties used as a model, for comparison, or a set of rules used to assure quality.</skos:scopeNote>
    <skos:broader rdf:resource="http://www.usgs.gov/science/USGSThesaurus/reports"/>
    <skos:related rdf:resource="http://www.usgs.gov/science/USGSThesaurus/standards%20development"/>
    <skos:inScheme rdf:resource="http://www.usgs.gov/science/USGSThesaurus"/>
  </rdf:Description>
  <rdf:Description about="http://www.usgs.gov/science/USGSThesaurus/strategic%20plans">
    <rdf:type rdf:resource="http://www.w3.org/2004/02/skos/core#Concept"/>
    <skos:prefLabel xml:lang="en">strategic plans</skos:prefLabel>
    <skos:scopeNote xml:lang="en">Documents describing overall strategy, not presenting substantive scientific findings.</skos:scopeNote>
    <skos:altLabel xml:lang="en">science strategy</skos:altLabel>
    <skos:broader rdf:resource="http://www.usgs.gov/science/USGSThesaurus/reports"/>
    <skos:inScheme rdf:resource="http://www.usgs.gov/science/USGSThesaurus"/>
  </rdf:Description>
  <rdf:Description about="http://www.usgs.gov/science/USGSThesaurus/scientific%20software">
    <rdf:type rdf:resource="http://www.w3.org/2004/02/skos/core#Concept"/>
    <skos:prefLabel xml:lang="en">scientific software</skos:prefLabel>
    <skos:scopeNote xml:lang="en">Routines, programs, and procedures devised in order to direct computers to perform specific tasks.</skos:scopeNote>
    <skos:altLabel xml:lang="en">computer program</skos:altLabel>
    <skos:broader rdf:resource="http://www.usgs.gov/science/USGSThesaurus/product%20types"/>
    <skos:related rdf:resource="http://www.usgs.gov/science/USGSThesaurus/software%20development"/>
    <skos:inScheme rdf:resource="http://www.usgs.gov/science/USGSThesaurus"/>
  </rdf:Description>
  <rdf:Description about="http://www.usgs.gov/science/USGSThesaurus/sound%20recordings">
    <rdf:type rdf:resource="http://www.w3.org/2004/02/skos/core#Concept"/>
    <skos:prefLabel xml:lang="en">sound recordings</skos:prefLabel>
    <skos:scopeNote xml:lang="en">Information presented in a format for listening by the user.</skos:scopeNote>
    <skos:altLabel xml:lang="en">audio recordings</skos:altLabel>
    <skos:altLabel xml:lang="en">podcasts</skos:altLabel>
    <skos:broader rdf:resource="http://www.usgs.gov/science/USGSThesaurus/product%20types"/>
    <skos:inScheme rdf:resource="http://www.usgs.gov/science/USGSThesaurus"/>
  </rdf:Description>
  <rdf:Description about="http://www.usgs.gov/science/USGSThesaurus/terminologies%20and%20classifications">
    <rdf:type rdf:resource="http://www.w3.org/2004/02/skos/core#Concept"/>
    <skos:prefLabel xml:lang="en">terminologies and classifications</skos:prefLabel>
    <skos:scopeNote xml:lang="en">Collections of terms often including definitions or scope notes, with some stated relationships among terms</skos:scopeNote>
    <skos:altLabel xml:lang="en">glossaries</skos:altLabel>
    <skos:altLabel xml:lang="en">controlled vocabularies</skos:altLabel>
    <skos:broader rdf:resource="http://www.usgs.gov/science/USGSThesaurus/product%20types"/>
    <skos:narrower rdf:resource="http://www.usgs.gov/science/USGSThesaurus/geologic%20time%20scales"/>
    <skos:inScheme rdf:resource="http://www.usgs.gov/science/USGSThesaurus"/>
  </rdf:Description>
  <rdf:Description about="http://www.usgs.gov/science/USGSThesaurus/geologic%20time%20scales">
    <rdf:type rdf:resource="http://www.w3.org/2004/02/skos/core#Concept"/>
    <skos:prefLabel xml:lang="en">geologic time scales</skos:prefLabel>
    <skos:scopeNote xml:lang="en">Named divisions of geologic time used to specify relationships among geologic units and structural features</skos:scopeNote>
    <skos:broader rdf:resource="http://www.usgs.gov/science/USGSThesaurus/terminologies%20and%20classifications"/>
    <skos:inScheme rdf:resource="http://www.usgs.gov/science/USGSThesaurus"/>
  </rdf:Description>
  <rdf:Description about="http://www.usgs.gov/science/USGSThesaurus/videos">
    <rdf:type rdf:resource="http://www.w3.org/2004/02/skos/core#Concept"/>
    <skos:prefLabel xml:lang="en">videos</skos:prefLabel>
    <skos:scopeNote xml:lang="en">Animation or other motion pictures, including videotape and DVD products.</skos:scopeNote>
    <skos:broader rdf:resource="http://www.usgs.gov/science/USGSThesaurus/product%20types"/>
    <skos:inScheme rdf:resource="http://www.usgs.gov/science/USGSThesaurus"/>
  </rdf:Description>
  <rdf:Description about="http://www.usgs.gov/science/USGSThesaurus/sciences">
    <rdf:type rdf:resource="http://www.w3.org/2004/02/skos/core#Concept"/>
    <skos:prefLabel xml:lang="en">sciences</skos:prefLabel>
    <skos:scopeNote xml:lang="en">Major educational fields, fields of study, and professional groupings within USGS.</skos:scopeNote>
    <skos:broader rdf:resource="http://www.usgs.gov/science/USGSThesaurus/Categories"/>
    <skos:narrower rdf:resource="http://www.usgs.gov/science/USGSThesaurus/earth%20sciences"/>
    <skos:narrower rdf:resource="http://www.usgs.gov/science/USGSThesaurus/engineering%20sciences"/>
    <skos:narrower rdf:resource="http://www.usgs.gov/science/USGSThesaurus/information%20sciences"/>
    <skos:narrower rdf:resource="http://www.usgs.gov/science/USGSThesaurus/life%20sciences"/>
    <skos:narrower rdf:resource="http://www.usgs.gov/science/USGSThesaurus/planetary%20sciences"/>
    <skos:narrower rdf:resource="http://www.usgs.gov/science/USGSThesaurus/social%20sciences"/>
    <skos:inScheme rdf:resource="http://www.usgs.gov/science/USGSThesaurus"/>
  </rdf:Description>
  <rdf:Description about="http://www.usgs.gov/science/USGSThesaurus/earth%20sciences">
    <rdf:type rdf:resource="http://www.w3.org/2004/02/skos/core#Concept"/>
    <skos:prefLabel xml:lang="en">earth sciences</skos:prefLabel>
    <skos:scopeNote xml:lang="en">Broad term for all science related to the study of the earth.</skos:scopeNote>
    <skos:altLabel xml:lang="en">geosciences</skos:altLabel>
    <skos:broader rdf:resource="http://www.usgs.gov/science/USGSThesaurus/sciences"/>
    <skos:narrower rdf:resource="http://www.usgs.gov/science/USGSThesaurus/atmospheric%20sciences"/>
    <skos:narrower rdf:resource="http://www.usgs.gov/science/USGSThesaurus/geochemistry"/>
    <skos:narrower rdf:resource="http://www.usgs.gov/science/USGSThesaurus/geography"/>
    <skos:narrower rdf:resource="http://www.usgs.gov/science/USGSThesaurus/geology"/>
    <skos:narrower rdf:resource="http://www.usgs.gov/science/USGSThesaurus/geophysics"/>
    <skos:narrower rdf:resource="http://www.usgs.gov/science/USGSThesaurus/glaciology"/>
    <skos:narrower rdf:resource="http://www.usgs.gov/science/USGSThesaurus/hydrology"/>
    <skos:narrower rdf:resource="http://www.usgs.gov/science/USGSThesaurus/limnology"/>
    <skos:narrower rdf:resource="http://www.usgs.gov/science/USGSThesaurus/ocean%20sciences"/>
    <skos:narrower rdf:resource="http://www.usgs.gov/science/USGSThesaurus/paleontology"/>
    <skos:narrower rdf:resource="http://www.usgs.gov/science/USGSThesaurus/soil%20sciences"/>
    <skos:related rdf:resource="http://www.usgs.gov/science/USGSThesaurus/earth%20characteristics"/>
    <skos:related rdf:resource="http://www.usgs.gov/science/USGSThesaurus/natural%20resources"/>
    <skos:related rdf:resource="http://www.usgs.gov/science/USGSThesaurus/scientific%20careers"/>
    <skos:inScheme rdf:resource="http://www.usgs.gov/science/USGSThesaurus"/>
  </rdf:Description>
  <rdf:Description about="http://www.usgs.gov/science/USGSThesaurus/atmospheric%20sciences">
    <rdf:type rdf:resource="http://www.w3.org/2004/02/skos/core#Concept"/>
    <skos:prefLabel xml:lang="en">atmospheric sciences</skos:prefLabel>
    <skos:scopeNote xml:lang="en">Studies relating to composition, structure, physics, chemistry, and dynamics of the atmosphere.</skos:scopeNote>
    <skos:broader rdf:resource="http://www.usgs.gov/science/USGSThesaurus/earth%20sciences"/>
    <skos:narrower rdf:resource="http://www.usgs.gov/science/USGSThesaurus/climatology"/>
    <skos:narrower rdf:resource="http://www.usgs.gov/science/USGSThesaurus/meteorology"/>
    <skos:related rdf:resource="http://www.usgs.gov/science/USGSThesaurus/acid%20deposition"/>
    <skos:related rdf:resource="http://www.usgs.gov/science/USGSThesaurus/air%20temperature"/>
    <skos:related rdf:resource="http://www.usgs.gov/science/USGSThesaurus/atmospheric%20and%20climatic%20processes"/>
    <skos:related rdf:resource="http://www.usgs.gov/science/USGSThesaurus/atmospheric%20circulation"/>
    <skos:related rdf:resource="http://www.usgs.gov/science/USGSThesaurus/atmospheric%20composition"/>
    <skos:related rdf:resource="http://www.usgs.gov/science/USGSThesaurus/atmospheric%20deposition%20%28chemical%20%26%20particulate%29"/>
    <skos:related rdf:resource="http://www.usgs.gov/science/USGSThesaurus/atmospheric%20properties"/>
    <skos:related rdf:resource="http://www.usgs.gov/science/USGSThesaurus/droughts"/>
    <skos:related rdf:resource="http://www.usgs.gov/science/USGSThesaurus/fires"/>
    <skos:related rdf:resource="http://www.usgs.gov/science/USGSThesaurus/effects%20of%20climate%20change"/>
    <skos:related rdf:resource="http://www.usgs.gov/science/USGSThesaurus/greenhouse%20gases"/>
    <skos:related rdf:resource="http://www.usgs.gov/science/USGSThesaurus/ocean%20temperature"/>
    <skos:related rdf:resource="http://www.usgs.gov/science/USGSThesaurus/ocean-atmosphere%20interaction"/>
    <skos:related rdf:resource="http://www.usgs.gov/science/USGSThesaurus/ozone%20layer"/>
    <skos:related rdf:resource="http://www.usgs.gov/science/USGSThesaurus/precipitation%20%28atmospheric%29"/>
    <skos:inScheme rdf:resource="http://www.usgs.gov/science/USGSThesaurus"/>
  </rdf:Description>
  <rdf:Description about="http://www.usgs.gov/science/USGSThesaurus/climatology">
    <rdf:type rdf:resource="http://www.w3.org/2004/02/skos/core#Concept"/>
    <skos:prefLabel xml:lang="en">climatology</skos:prefLabel>
    <skos:scopeNote xml:lang="en">Scientific study of the characteristic weather conditions of geographic areas.</skos:scopeNote>
    <skos:broader rdf:resource="http://www.usgs.gov/science/USGSThesaurus/atmospheric%20sciences"/>
    <skos:related rdf:resource="http://www.usgs.gov/science/USGSThesaurus/climate%20change"/>
    <skos:related rdf:resource="http://www.usgs.gov/science/USGSThesaurus/desertification"/>
    <skos:related rdf:resource="http://www.usgs.gov/science/USGSThesaurus/meteorology"/>
    <skos:related rdf:resource="http://www.usgs.gov/science/USGSThesaurus/ocean%20circulation"/>
    <skos:related rdf:resource="http://www.usgs.gov/science/USGSThesaurus/sea-level%20change"/>
    <skos:inScheme rdf:resource="http://www.usgs.gov/science/USGSThesaurus"/>
  </rdf:Description>
  <rdf:Description about="http://www.usgs.gov/science/USGSThesaurus/meteorology">
    <rdf:type rdf:resource="http://www.w3.org/2004/02/skos/core#Concept"/>
    <skos:prefLabel xml:lang="en">meteorology</skos:prefLabel>
    <skos:scopeNote xml:lang="en">Branch of science dealing with the short-term variations of atmospheric conditions including wind, precipitation, temperature, humidity, cloud cover, and air pressure.</skos:scopeNote>
    <skos:broader rdf:resource="http://www.usgs.gov/science/USGSThesaurus/atmospheric%20sciences"/>
    <skos:related rdf:resource="http://www.usgs.gov/science/USGSThesaurus/atmospheric%20and%20climatic%20processes"/>
    <skos:related rdf:resource="http://www.usgs.gov/science/USGSThesaurus/climatology"/>
    <skos:related rdf:resource="http://www.usgs.gov/science/USGSThesaurus/hurricanes"/>
    <skos:related rdf:resource="http://www.usgs.gov/science/USGSThesaurus/hydrology"/>
    <skos:related rdf:resource="http://www.usgs.gov/science/USGSThesaurus/ocean%20currents"/>
    <skos:related rdf:resource="http://www.usgs.gov/science/USGSThesaurus/ocean%20sciences"/>
    <skos:related rdf:resource="http://www.usgs.gov/science/USGSThesaurus/planetary%20sciences"/>
    <skos:related rdf:resource="http://www.usgs.gov/science/USGSThesaurus/storms"/>
    <skos:related rdf:resource="http://www.usgs.gov/science/USGSThesaurus/tornadoes"/>
    <skos:inScheme rdf:resource="http://www.usgs.gov/science/USGSThesaurus"/>
  </rdf:Description>
  <rdf:Description about="http://www.usgs.gov/science/USGSThesaurus/geochemistry">
    <rdf:type rdf:resource="http://www.w3.org/2004/02/skos/core#Concept"/>
    <skos:prefLabel xml:lang="en">geochemistry</skos:prefLabel>
    <skos:scopeNote xml:lang="en">Study of the distribution of chemical elements and natural compounds on the earth and in the atmosphere and the chemical processes that affect the earth.</skos:scopeNote>
    <skos:altLabel xml:lang="en">chemistry (Earth sciences)</skos:altLabel>
    <!--FOR geochemical anomaly maps USE geochemistry WITH maps and atlases-->
    <skos:altLabel xml:lang="en">geochemical anomaly maps</skos:altLabel>
    <skos:broader rdf:resource="http://www.usgs.gov/science/USGSThesaurus/earth%20sciences"/>
    <skos:narrower rdf:resource="http://www.usgs.gov/science/USGSThesaurus/soil%20chemistry"/>
    <skos:narrower rdf:resource="http://www.usgs.gov/science/USGSThesaurus/water%20chemistry"/>
    <skos:related rdf:resource="http://www.usgs.gov/science/USGSThesaurus/atomic%20absorption%20analysis"/>
    <skos:related rdf:resource="http://www.usgs.gov/science/USGSThesaurus/biogeochemical%20cycling"/>
    <skos:related rdf:resource="http://www.usgs.gov/science/USGSThesaurus/carbon%20cycling"/>
    <skos:related rdf:resource="http://www.usgs.gov/science/USGSThesaurus/carbon%20isotope%20analysis"/>
    <skos:related rdf:resource="http://www.usgs.gov/science/USGSThesaurus/chemical%20analysis"/>
    <skos:related rdf:resource="http://www.usgs.gov/science/USGSThesaurus/chromatography"/>
    <skos:related rdf:resource="http://www.usgs.gov/science/USGSThesaurus/earth%20history"/>
    <skos:related rdf:resource="http://www.usgs.gov/science/USGSThesaurus/gas%20chromatography"/>
    <skos:related rdf:resource="http://www.usgs.gov/science/USGSThesaurus/geochemical%20processes"/>
    <skos:related rdf:resource="http://www.usgs.gov/science/USGSThesaurus/isotopic%20analysis"/>
    <skos:related rdf:resource="http://www.usgs.gov/science/USGSThesaurus/light%20stable%20isotope%20analysis"/>
    <skos:related rdf:resource="http://www.usgs.gov/science/USGSThesaurus/liquid%20chromatography"/>
    <skos:related rdf:resource="http://www.usgs.gov/science/USGSThesaurus/mass%20spectroscopy"/>
    <skos:related rdf:resource="http://www.usgs.gov/science/USGSThesaurus/metamorphism%20%28geological%29"/>
    <skos:related rdf:resource="http://www.usgs.gov/science/USGSThesaurus/neutron%20activation%20analysis"/>
    <skos:related rdf:resource="http://www.usgs.gov/science/USGSThesaurus/oxygen%20isotope%20analysis"/>
    <skos:related rdf:resource="http://www.usgs.gov/science/USGSThesaurus/particle-beam%20spectroscopy"/>
    <skos:related rdf:resource="http://www.usgs.gov/science/USGSThesaurus/tritium%20analysis"/>
    <skos:inScheme rdf:resource="http://www.usgs.gov/science/USGSThesaurus"/>
  </rdf:Description>
  <rdf:Description about="http://www.usgs.gov/science/USGSThesaurus/soil%20chemistry">
    <rdf:type rdf:resource="http://www.w3.org/2004/02/skos/core#Concept"/>
    <skos:prefLabel xml:lang="en">soil chemistry</skos:prefLabel>
    <skos:scopeNote xml:lang="en">Branch of chemistry concerned with the elements and compounds that make up soils. Includes chemical processes involving soils.</skos:scopeNote>
    <skos:broader rdf:resource="http://www.usgs.gov/science/USGSThesaurus/geochemistry"/>
    <skos:related rdf:resource="http://www.usgs.gov/science/USGSThesaurus/agriculture"/>
    <skos:related rdf:resource="http://www.usgs.gov/science/USGSThesaurus/soil%20resources"/>
    <skos:related rdf:resource="http://www.usgs.gov/science/USGSThesaurus/soil%20sciences"/>
    <skos:inScheme rdf:resource="http://www.usgs.gov/science/USGSThesaurus"/>
  </rdf:Description>
  <rdf:Description about="http://www.usgs.gov/science/USGSThesaurus/water%20chemistry">
    <rdf:type rdf:resource="http://www.w3.org/2004/02/skos/core#Concept"/>
    <skos:prefLabel xml:lang="en">water chemistry</skos:prefLabel>
    <skos:scopeNote xml:lang="en">Branch of chemistry that deals with the elements and compounds in water.</skos:scopeNote>
    <skos:broader rdf:resource="http://www.usgs.gov/science/USGSThesaurus/geochemistry"/>
    <skos:narrower rdf:resource="http://www.usgs.gov/science/USGSThesaurus/marine%20chemistry"/>
    <skos:related rdf:resource="http://www.usgs.gov/science/USGSThesaurus/groundwater%20quality"/>
    <skos:related rdf:resource="http://www.usgs.gov/science/USGSThesaurus/nutrient%20content%20%28water%29"/>
    <skos:related rdf:resource="http://www.usgs.gov/science/USGSThesaurus/oxygen%20content%20%28water%29"/>
    <skos:related rdf:resource="http://www.usgs.gov/science/USGSThesaurus/salinity"/>
    <skos:related rdf:resource="http://www.usgs.gov/science/USGSThesaurus/surface%20water%20quality"/>
    <skos:related rdf:resource="http://www.usgs.gov/science/USGSThesaurus/suspended%20material%20%28water%29"/>
    <skos:related rdf:resource="http://www.usgs.gov/science/USGSThesaurus/water%20hardness"/>
    <skos:related rdf:resource="http://www.usgs.gov/science/USGSThesaurus/water%20pH"/>
    <skos:related rdf:resource="http://www.usgs.gov/science/USGSThesaurus/water%20properties"/>
    <skos:related rdf:resource="http://www.usgs.gov/science/USGSThesaurus/water%20quality"/>
    <skos:related rdf:resource="http://www.usgs.gov/science/USGSThesaurus/water%20sampling"/>
    <skos:related rdf:resource="http://www.usgs.gov/science/USGSThesaurus/water%20temperature"/>
    <skos:inScheme rdf:resource="http://www.usgs.gov/science/USGSThesaurus"/>
  </rdf:Description>
  <rdf:Description about="http://www.usgs.gov/science/USGSThesaurus/marine%20chemistry">
    <rdf:type rdf:resource="http://www.w3.org/2004/02/skos/core#Concept"/>
    <skos:prefLabel xml:lang="en">marine chemistry</skos:prefLabel>
    <skos:scopeNote xml:lang="en">Branch of chemistry that deals with the properties, composition, structure, and interaction of substances in the seas and oceans.</skos:scopeNote>
    <skos:altLabel xml:lang="en">chemical oceanography</skos:altLabel>
    <skos:altLabel xml:lang="en">ocean chemistry</skos:altLabel>
    <skos:altLabel xml:lang="en">water properties (marine)</skos:altLabel>
    <skos:broader rdf:resource="http://www.usgs.gov/science/USGSThesaurus/water%20chemistry"/>
    <skos:related rdf:resource="http://www.usgs.gov/science/USGSThesaurus/CTD%20measurement"/>
    <skos:related rdf:resource="http://www.usgs.gov/science/USGSThesaurus/marine%20water%20quality"/>
    <skos:related rdf:resource="http://www.usgs.gov/science/USGSThesaurus/ocean%20characteristics"/>
    <skos:related rdf:resource="http://www.usgs.gov/science/USGSThesaurus/ocean%20salinity"/>
    <skos:related rdf:resource="http://www.usgs.gov/science/USGSThesaurus/ocean%20sciences"/>
    <skos:related rdf:resource="http://www.usgs.gov/science/USGSThesaurus/ocean%20acidification"/>
    <skos:inScheme rdf:resource="http://www.usgs.gov/science/USGSThesaurus"/>
  </rdf:Description>
  <rdf:Description about="http://www.usgs.gov/science/USGSThesaurus/geography">
    <rdf:type rdf:resource="http://www.w3.org/2004/02/skos/core#Concept"/>
    <skos:prefLabel xml:lang="en">geography</skos:prefLabel>
    <skos:scopeNote xml:lang="en">Study of the earth's landforms, topography, and climate, the distribution of flora and fauna, and the distribution, culture, and activities of human populations.</skos:scopeNote>
    <skos:altLabel xml:lang="en">geographic information sciences</skos:altLabel>
    <skos:broader rdf:resource="http://www.usgs.gov/science/USGSThesaurus/earth%20sciences"/>
    <skos:narrower rdf:resource="http://www.usgs.gov/science/USGSThesaurus/cartography"/>
    <skos:narrower rdf:resource="http://www.usgs.gov/science/USGSThesaurus/paleogeography"/>
    <skos:related rdf:resource="http://www.usgs.gov/science/USGSThesaurus/administrative%20and%20political%20boundaries"/>
    <skos:related rdf:resource="http://www.usgs.gov/science/USGSThesaurus/aeromagnetic%20surveying"/>
    <skos:related rdf:resource="http://www.usgs.gov/science/USGSThesaurus/aeroradiometric%20surveying"/>
    <skos:related rdf:resource="http://www.usgs.gov/science/USGSThesaurus/altimetry%20measurement"/>
    <skos:related rdf:resource="http://www.usgs.gov/science/USGSThesaurus/AVHRR"/>
    <skos:related rdf:resource="http://www.usgs.gov/science/USGSThesaurus/bathymetry%20measurement"/>
    <skos:related rdf:resource="http://www.usgs.gov/science/USGSThesaurus/cadastral%20and%20legal%20land%20descriptions"/>
    <skos:related rdf:resource="http://www.usgs.gov/science/USGSThesaurus/culture%20and%20demographics"/>
    <skos:related rdf:resource="http://www.usgs.gov/science/USGSThesaurus/geodesy"/>
    <skos:related rdf:resource="http://www.usgs.gov/science/USGSThesaurus/geographic%20information%20systems"/>
    <skos:related rdf:resource="http://www.usgs.gov/science/USGSThesaurus/geolocation%20measurement"/>
    <skos:related rdf:resource="http://www.usgs.gov/science/USGSThesaurus/GPS%20measurement"/>
    <skos:related rdf:resource="http://www.usgs.gov/science/USGSThesaurus/hyperspectral%20imaging"/>
    <skos:related rdf:resource="http://www.usgs.gov/science/USGSThesaurus/IFSAR"/>
    <skos:related rdf:resource="http://www.usgs.gov/science/USGSThesaurus/image%20analysis"/>
    <skos:related rdf:resource="http://www.usgs.gov/science/USGSThesaurus/infrared%20imaging"/>
    <skos:related rdf:resource="http://www.usgs.gov/science/USGSThesaurus/land%20surface%20characteristics"/>
    <skos:related rdf:resource="http://www.usgs.gov/science/USGSThesaurus/land%20surveying"/>
    <skos:related rdf:resource="http://www.usgs.gov/science/USGSThesaurus/land%20use%20change"/>
    <skos:related rdf:resource="http://www.usgs.gov/science/USGSThesaurus/LIDAR"/>
    <skos:related rdf:resource="http://www.usgs.gov/science/USGSThesaurus/map%20coordinate%20systems"/>
    <skos:related rdf:resource="http://www.usgs.gov/science/USGSThesaurus/microwave%20imaging"/>
    <skos:related rdf:resource="http://www.usgs.gov/science/USGSThesaurus/multispectral%20imaging"/>
    <skos:related rdf:resource="http://www.usgs.gov/science/USGSThesaurus/panchromatic%20imaging"/>
    <skos:related rdf:resource="http://www.usgs.gov/science/USGSThesaurus/radar%20imaging"/>
    <skos:related rdf:resource="http://www.usgs.gov/science/USGSThesaurus/remote%20sensing"/>
    <skos:related rdf:resource="http://www.usgs.gov/science/USGSThesaurus/SLAR"/>
    <skos:related rdf:resource="http://www.usgs.gov/science/USGSThesaurus/SMMR"/>
    <skos:related rdf:resource="http://www.usgs.gov/science/USGSThesaurus/spatial%20analysis"/>
    <skos:related rdf:resource="http://www.usgs.gov/science/USGSThesaurus/SSM%2FI"/>
    <skos:related rdf:resource="http://www.usgs.gov/science/USGSThesaurus/thermal%20imaging"/>
    <skos:related rdf:resource="http://www.usgs.gov/science/USGSThesaurus/topography"/>
    <skos:related rdf:resource="http://www.usgs.gov/science/USGSThesaurus/topological%20analysis"/>
    <skos:related rdf:resource="http://www.usgs.gov/science/USGSThesaurus/visible%20light%20imaging"/>
    <skos:inScheme rdf:resource="http://www.usgs.gov/science/USGSThesaurus"/>
  </rdf:Description>
  <rdf:Description about="http://www.usgs.gov/science/USGSThesaurus/cartography">
    <rdf:type rdf:resource="http://www.w3.org/2004/02/skos/core#Concept"/>
    <skos:prefLabel xml:lang="en">cartography</skos:prefLabel>
    <skos:scopeNote xml:lang="en">The science and art of making maps.</skos:scopeNote>
    <skos:altLabel xml:lang="en">digital cartography</skos:altLabel>
    <skos:altLabel xml:lang="en">map making</skos:altLabel>
    <skos:altLabel xml:lang="en">mapmaking</skos:altLabel>
    <skos:altLabel xml:lang="en">mapping</skos:altLabel>
    <skos:broader rdf:resource="http://www.usgs.gov/science/USGSThesaurus/geography"/>
    <skos:related rdf:resource="http://www.usgs.gov/science/USGSThesaurus/map%20coordinate%20systems"/>
    <skos:related rdf:resource="http://www.usgs.gov/science/USGSThesaurus/maps%20and%20atlases"/>
    <skos:inScheme rdf:resource="http://www.usgs.gov/science/USGSThesaurus"/>
  </rdf:Description>
  <rdf:Description about="http://www.usgs.gov/science/USGSThesaurus/paleogeography">
    <rdf:type rdf:resource="http://www.w3.org/2004/02/skos/core#Concept"/>
    <skos:prefLabel xml:lang="en">paleogeography</skos:prefLabel>
    <skos:scopeNote xml:lang="en">Study of the history of earth surface characteristics; geomorphology in the past.</skos:scopeNote>
    <skos:broader rdf:resource="http://www.usgs.gov/science/USGSThesaurus/geography"/>
    <skos:inScheme rdf:resource="http://www.usgs.gov/science/USGSThesaurus"/>
  </rdf:Description>
  <rdf:Description about="http://www.usgs.gov/science/USGSThesaurus/geology">
    <rdf:type rdf:resource="http://www.w3.org/2004/02/skos/core#Concept"/>
    <skos:prefLabel xml:lang="en">geology</skos:prefLabel>
    <skos:scopeNote xml:lang="en">Study of the planet earth, its composition, structure, physical and chemical processes, and history since its origin.</skos:scopeNote>
    <!--FOR subsurface maps USE geology WITH maps and atlases-->
    <skos:altLabel xml:lang="en">subsurface maps</skos:altLabel>
    <skos:broader rdf:resource="http://www.usgs.gov/science/USGSThesaurus/earth%20sciences"/>
    <skos:narrower rdf:resource="http://www.usgs.gov/science/USGSThesaurus/economic%20geology"/>
    <skos:narrower rdf:resource="http://www.usgs.gov/science/USGSThesaurus/geochronology"/>
    <skos:narrower rdf:resource="http://www.usgs.gov/science/USGSThesaurus/geomorphology"/>
    <skos:narrower rdf:resource="http://www.usgs.gov/science/USGSThesaurus/hydrogeology"/>
    <skos:narrower rdf:resource="http://www.usgs.gov/science/USGSThesaurus/marine%20geology"/>
    <skos:narrower rdf:resource="http://www.usgs.gov/science/USGSThesaurus/mineralogy"/>
    <skos:narrower rdf:resource="http://www.usgs.gov/science/USGSThesaurus/petrology"/>
    <skos:narrower rdf:resource="http://www.usgs.gov/science/USGSThesaurus/sedimentology"/>
    <skos:narrower rdf:resource="http://www.usgs.gov/science/USGSThesaurus/stratigraphy"/>
    <skos:narrower rdf:resource="http://www.usgs.gov/science/USGSThesaurus/structural%20geology"/>
    <skos:narrower rdf:resource="http://www.usgs.gov/science/USGSThesaurus/volcanology"/>
    <skos:related rdf:resource="http://www.usgs.gov/science/USGSThesaurus/drilling%20and%20coring"/>
    <skos:related rdf:resource="http://www.usgs.gov/science/USGSThesaurus/earth%20history"/>
    <skos:related rdf:resource="http://www.usgs.gov/science/USGSThesaurus/engineering%20geology"/>
    <skos:related rdf:resource="http://www.usgs.gov/science/USGSThesaurus/geologic%20processes"/>
    <skos:related rdf:resource="http://www.usgs.gov/science/USGSThesaurus/geologic%20history"/>
    <skos:related rdf:resource="http://www.usgs.gov/science/USGSThesaurus/metamorphism%20%28geological%29"/>
    <skos:related rdf:resource="http://www.usgs.gov/science/USGSThesaurus/geologic%20maps"/>
    <skos:inScheme rdf:resource="http://www.usgs.gov/science/USGSThesaurus"/>
  </rdf:Description>
  <rdf:Description about="http://www.usgs.gov/science/USGSThesaurus/economic%20geology">
    <rdf:type rdf:resource="http://www.w3.org/2004/02/skos/core#Concept"/>
    <skos:prefLabel xml:lang="en">economic geology</skos:prefLabel>
    <skos:scopeNote xml:lang="en">Scientific study of the formation, location, and use of marketable geologic materials including fuels, metals, minerals, and water.</skos:scopeNote>
    <skos:broader rdf:resource="http://www.usgs.gov/science/USGSThesaurus/geology"/>
    <skos:related rdf:resource="http://www.usgs.gov/science/USGSThesaurus/building%20stone%20resources"/>
    <skos:related rdf:resource="http://www.usgs.gov/science/USGSThesaurus/clay%20deposits"/>
    <skos:related rdf:resource="http://www.usgs.gov/science/USGSThesaurus/coal%20resources"/>
    <skos:related rdf:resource="http://www.usgs.gov/science/USGSThesaurus/coalbed%20methane%20resources"/>
    <skos:related rdf:resource="http://www.usgs.gov/science/USGSThesaurus/gas%20hydrate%20resources"/>
    <skos:related rdf:resource="http://www.usgs.gov/science/USGSThesaurus/gem%20resources"/>
    <skos:related rdf:resource="http://www.usgs.gov/science/USGSThesaurus/gravel%20deposits"/>
    <skos:related rdf:resource="http://www.usgs.gov/science/USGSThesaurus/metallic%20mineral%20resources"/>
    <skos:related rdf:resource="http://www.usgs.gov/science/USGSThesaurus/mineral%20resources"/>
    <skos:related rdf:resource="http://www.usgs.gov/science/USGSThesaurus/natural%20gas%20resources"/>
    <skos:related rdf:resource="http://www.usgs.gov/science/USGSThesaurus/nonmetallic%20mineral%20resources"/>
    <skos:related rdf:resource="http://www.usgs.gov/science/USGSThesaurus/energy%20resources"/>
    <skos:related rdf:resource="http://www.usgs.gov/science/USGSThesaurus/oil%20resources"/>
    <skos:related rdf:resource="http://www.usgs.gov/science/USGSThesaurus/oil%20sand%20resources"/>
    <skos:related rdf:resource="http://www.usgs.gov/science/USGSThesaurus/oil%20shale%20resources"/>
    <skos:related rdf:resource="http://www.usgs.gov/science/USGSThesaurus/sand%20deposits"/>
    <skos:related rdf:resource="http://www.usgs.gov/science/USGSThesaurus/soil%20resources"/>
    <skos:inScheme rdf:resource="http://www.usgs.gov/science/USGSThesaurus"/>
  </rdf:Description>
  <rdf:Description about="http://www.usgs.gov/science/USGSThesaurus/geochronology">
    <rdf:type rdf:resource="http://www.w3.org/2004/02/skos/core#Concept"/>
    <skos:prefLabel xml:lang="en">geochronology</skos:prefLabel>
    <skos:scopeNote xml:lang="en">Study of the age of the earth by dating geological formations, rocks, and fossils.</skos:scopeNote>
    <skos:broader rdf:resource="http://www.usgs.gov/science/USGSThesaurus/geology"/>
    <skos:related rdf:resource="http://www.usgs.gov/science/USGSThesaurus/carbon-14%20analysis"/>
    <skos:related rdf:resource="http://www.usgs.gov/science/USGSThesaurus/fission-track%20dating"/>
    <skos:related rdf:resource="http://www.usgs.gov/science/USGSThesaurus/radiometric%20dating"/>
    <skos:related rdf:resource="http://www.usgs.gov/science/USGSThesaurus/rubidium-strontium%20analysis"/>
    <skos:related rdf:resource="http://www.usgs.gov/science/USGSThesaurus/stratigraphy"/>
    <skos:related rdf:resource="http://www.usgs.gov/science/USGSThesaurus/tree%20ring%20analysis"/>
    <skos:related rdf:resource="http://www.usgs.gov/science/USGSThesaurus/uranium-lead%20analysis"/>
    <skos:related rdf:resource="http://www.usgs.gov/science/USGSThesaurus/uranium-thorium%20analysis"/>
    <skos:inScheme rdf:resource="http://www.usgs.gov/science/USGSThesaurus"/>
  </rdf:Description>
  <rdf:Description about="http://www.usgs.gov/science/USGSThesaurus/geomorphology">
    <rdf:type rdf:resource="http://www.w3.org/2004/02/skos/core#Concept"/>
    <skos:prefLabel xml:lang="en">geomorphology</skos:prefLabel>
    <skos:scopeNote xml:lang="en">Branch of geology dealing with surface land features and the processes that create and change them.</skos:scopeNote>
    <skos:altLabel xml:lang="en">speleology</skos:altLabel>
    <skos:broader rdf:resource="http://www.usgs.gov/science/USGSThesaurus/geology"/>
    <skos:related rdf:resource="http://www.usgs.gov/science/USGSThesaurus/bathymetry"/>
    <skos:related rdf:resource="http://www.usgs.gov/science/USGSThesaurus/erosion"/>
    <skos:related rdf:resource="http://www.usgs.gov/science/USGSThesaurus/subsidence"/>
    <skos:related rdf:resource="http://www.usgs.gov/science/USGSThesaurus/land%20surface%20characteristics"/>
    <skos:related rdf:resource="http://www.usgs.gov/science/USGSThesaurus/landslides"/>
    <skos:related rdf:resource="http://www.usgs.gov/science/USGSThesaurus/topography"/>
    <skos:inScheme rdf:resource="http://www.usgs.gov/science/USGSThesaurus"/>
  </rdf:Description>
  <rdf:Description about="http://www.usgs.gov/science/USGSThesaurus/hydrogeology">
    <rdf:type rdf:resource="http://www.w3.org/2004/02/skos/core#Concept"/>
    <skos:prefLabel xml:lang="en">hydrogeology</skos:prefLabel>
    <skos:scopeNote xml:lang="en">Study of subsurface waters and geologic aspects of surface waters.</skos:scopeNote>
    <skos:altLabel xml:lang="en">geohydrology</skos:altLabel>
    <skos:altLabel xml:lang="en">groundwater geology</skos:altLabel>
    <skos:altLabel xml:lang="en">hydrographic sections</skos:altLabel>
    <skos:broader rdf:resource="http://www.usgs.gov/science/USGSThesaurus/geology"/>
    <skos:related rdf:resource="http://www.usgs.gov/science/USGSThesaurus/geothermal%20resources"/>
    <skos:related rdf:resource="http://www.usgs.gov/science/USGSThesaurus/groundwater"/>
    <skos:related rdf:resource="http://www.usgs.gov/science/USGSThesaurus/groundwater%20flow"/>
    <skos:related rdf:resource="http://www.usgs.gov/science/USGSThesaurus/hydrothermal%20processes"/>
    <skos:related rdf:resource="http://www.usgs.gov/science/USGSThesaurus/water%20resources"/>
    <skos:related rdf:resource="http://www.usgs.gov/science/USGSThesaurus/hydrology"/>
    <skos:inScheme rdf:resource="http://www.usgs.gov/science/USGSThesaurus"/>
  </rdf:Description>
  <rdf:Description about="http://www.usgs.gov/science/USGSThesaurus/marine%20geology">
    <rdf:type rdf:resource="http://www.w3.org/2004/02/skos/core#Concept"/>
    <skos:prefLabel xml:lang="en">marine geology</skos:prefLabel>
    <skos:scopeNote xml:lang="en">Branch of geology concerned with the composition, geologic history, and earth processes of the ocean floor and the continental margin.</skos:scopeNote>
    <skos:altLabel xml:lang="en">geological oceanography</skos:altLabel>
    <skos:broader rdf:resource="http://www.usgs.gov/science/USGSThesaurus/geology"/>
    <skos:related rdf:resource="http://www.usgs.gov/science/USGSThesaurus/marine%20geophysics"/>
    <skos:related rdf:resource="http://www.usgs.gov/science/USGSThesaurus/ocean%20sciences"/>
    <skos:related rdf:resource="http://www.usgs.gov/science/USGSThesaurus/sea-floor%20characteristics"/>
    <skos:inScheme rdf:resource="http://www.usgs.gov/science/USGSThesaurus"/>
  </rdf:Description>
  <rdf:Description about="http://www.usgs.gov/science/USGSThesaurus/mineralogy">
    <rdf:type rdf:resource="http://www.w3.org/2004/02/skos/core#Concept"/>
    <skos:prefLabel xml:lang="en">mineralogy</skos:prefLabel>
    <skos:scopeNote xml:lang="en">Branch of earth sciences concerned with the study of naturally occurring inorganic elements or compounds.</skos:scopeNote>
    <skos:altLabel xml:lang="en">crystallography</skos:altLabel>
    <skos:altLabel xml:lang="en">gemology</skos:altLabel>
    <skos:broader rdf:resource="http://www.usgs.gov/science/USGSThesaurus/geology"/>
    <skos:related rdf:resource="http://www.usgs.gov/science/USGSThesaurus/gem%20resources"/>
    <skos:related rdf:resource="http://www.usgs.gov/science/USGSThesaurus/metallic%20mineral%20resources"/>
    <skos:related rdf:resource="http://www.usgs.gov/science/USGSThesaurus/mineral%20resources"/>
    <skos:related rdf:resource="http://www.usgs.gov/science/USGSThesaurus/x-ray%20diffraction"/>
    <skos:inScheme rdf:resource="http://www.usgs.gov/science/USGSThesaurus"/>
  </rdf:Description>
  <rdf:Description about="http://www.usgs.gov/science/USGSThesaurus/petrology">
    <rdf:type rdf:resource="http://www.w3.org/2004/02/skos/core#Concept"/>
    <skos:prefLabel xml:lang="en">petrology</skos:prefLabel>
    <skos:scopeNote xml:lang="en">Branch of earth sciences concerned with the origin, structure, alteration, and composition of rocks.</skos:scopeNote>
    <skos:broader rdf:resource="http://www.usgs.gov/science/USGSThesaurus/geology"/>
    <skos:related rdf:resource="http://www.usgs.gov/science/USGSThesaurus/diagenesis"/>
    <skos:related rdf:resource="http://www.usgs.gov/science/USGSThesaurus/igneous%20rocks"/>
    <skos:related rdf:resource="http://www.usgs.gov/science/USGSThesaurus/metamorphic%20rocks"/>
    <skos:related rdf:resource="http://www.usgs.gov/science/USGSThesaurus/petrography"/>
    <skos:related rdf:resource="http://www.usgs.gov/science/USGSThesaurus/rocks%20and%20deposits"/>
    <skos:related rdf:resource="http://www.usgs.gov/science/USGSThesaurus/sedimentary%20rocks"/>
    <skos:inScheme rdf:resource="http://www.usgs.gov/science/USGSThesaurus"/>
  </rdf:Description>
  <rdf:Description about="http://www.usgs.gov/science/USGSThesaurus/sedimentology">
    <rdf:type rdf:resource="http://www.w3.org/2004/02/skos/core#Concept"/>
    <skos:prefLabel xml:lang="en">sedimentology</skos:prefLabel>
    <skos:scopeNote xml:lang="en">Branch of earth sciences concerned with the study of the origin, composition, transport, and changes of materials deposited by water, wind, or ice.</skos:scopeNote>
    <skos:broader rdf:resource="http://www.usgs.gov/science/USGSThesaurus/geology"/>
    <skos:related rdf:resource="http://www.usgs.gov/science/USGSThesaurus/bedforms"/>
    <skos:related rdf:resource="http://www.usgs.gov/science/USGSThesaurus/building%20stone%20resources"/>
    <skos:related rdf:resource="http://www.usgs.gov/science/USGSThesaurus/clay%20deposits"/>
    <skos:related rdf:resource="http://www.usgs.gov/science/USGSThesaurus/diagenesis"/>
    <skos:related rdf:resource="http://www.usgs.gov/science/USGSThesaurus/erosion"/>
    <skos:related rdf:resource="http://www.usgs.gov/science/USGSThesaurus/grain-size%20analysis"/>
    <skos:related rdf:resource="http://www.usgs.gov/science/USGSThesaurus/gravel%20deposits"/>
    <skos:related rdf:resource="http://www.usgs.gov/science/USGSThesaurus/sand%20deposits"/>
    <skos:related rdf:resource="http://www.usgs.gov/science/USGSThesaurus/sediment%20transport"/>
    <skos:related rdf:resource="http://www.usgs.gov/science/USGSThesaurus/sedimentary%20rocks"/>
    <skos:related rdf:resource="http://www.usgs.gov/science/USGSThesaurus/sedimentation"/>
    <skos:related rdf:resource="http://www.usgs.gov/science/USGSThesaurus/sieve-size%20analysis"/>
    <skos:related rdf:resource="http://www.usgs.gov/science/USGSThesaurus/trenching"/>
    <skos:inScheme rdf:resource="http://www.usgs.gov/science/USGSThesaurus"/>
  </rdf:Description>
  <rdf:Description about="http://www.usgs.gov/science/USGSThesaurus/stratigraphy">
    <rdf:type rdf:resource="http://www.w3.org/2004/02/skos/core#Concept"/>
    <skos:prefLabel xml:lang="en">stratigraphy</skos:prefLabel>
    <skos:scopeNote xml:lang="en">Branch of geology concerned with the study of the formation, composition, ordering in time, and arrangement in space of stratified rocks.</skos:scopeNote>
    <skos:broader rdf:resource="http://www.usgs.gov/science/USGSThesaurus/geology"/>
    <skos:narrower rdf:resource="http://www.usgs.gov/science/USGSThesaurus/biostratigraphy"/>
    <skos:narrower rdf:resource="http://www.usgs.gov/science/USGSThesaurus/lithostratigraphy"/>
    <skos:related rdf:resource="http://www.usgs.gov/science/USGSThesaurus/bedrock%20geologic%20units"/>
    <skos:related rdf:resource="http://www.usgs.gov/science/USGSThesaurus/borehole%20logging"/>
    <skos:related rdf:resource="http://www.usgs.gov/science/USGSThesaurus/electrical%20resistivity%20logging"/>
    <skos:related rdf:resource="http://www.usgs.gov/science/USGSThesaurus/gamma-ray%20logging"/>
    <skos:related rdf:resource="http://www.usgs.gov/science/USGSThesaurus/geochronology"/>
    <skos:related rdf:resource="http://www.usgs.gov/science/USGSThesaurus/geologic%20contacts"/>
    <skos:related rdf:resource="http://www.usgs.gov/science/USGSThesaurus/geologic%20history"/>
    <skos:related rdf:resource="http://www.usgs.gov/science/USGSThesaurus/stratigraphic%20sections"/>
    <skos:related rdf:resource="http://www.usgs.gov/science/USGSThesaurus/surficial%20geologic%20units"/>
    <skos:related rdf:resource="http://www.usgs.gov/science/USGSThesaurus/unconformities"/>
    <skos:inScheme rdf:resource="http://www.usgs.gov/science/USGSThesaurus"/>
  </rdf:Description>
  <rdf:Description about="http://www.usgs.gov/science/USGSThesaurus/biostratigraphy">
    <rdf:type rdf:resource="http://www.w3.org/2004/02/skos/core#Concept"/>
    <skos:prefLabel xml:lang="en">biostratigraphy</skos:prefLabel>
    <skos:scopeNote xml:lang="en">Branch of geology concerned with the separation and differentiation of rock units based on the fossils they contain.</skos:scopeNote>
    <skos:broader rdf:resource="http://www.usgs.gov/science/USGSThesaurus/stratigraphy"/>
    <skos:related rdf:resource="http://www.usgs.gov/science/USGSThesaurus/geologic%20history"/>
    <skos:related rdf:resource="http://www.usgs.gov/science/USGSThesaurus/fossils"/>
    <skos:related rdf:resource="http://www.usgs.gov/science/USGSThesaurus/ichnofossils"/>
    <skos:related rdf:resource="http://www.usgs.gov/science/USGSThesaurus/paleontology"/>
    <skos:inScheme rdf:resource="http://www.usgs.gov/science/USGSThesaurus"/>
  </rdf:Description>
  <rdf:Description about="http://www.usgs.gov/science/USGSThesaurus/lithostratigraphy">
    <rdf:type rdf:resource="http://www.w3.org/2004/02/skos/core#Concept"/>
    <skos:prefLabel xml:lang="en">lithostratigraphy</skos:prefLabel>
    <skos:scopeNote xml:lang="en">Branch of stratigraphy dealing with the study of units of rock. Each unit is composed of a body of rock which is dominated by a certain lithology or similar color, mineralogic composition, and grain size.</skos:scopeNote>
    <skos:broader rdf:resource="http://www.usgs.gov/science/USGSThesaurus/stratigraphy"/>
    <skos:related rdf:resource="http://www.usgs.gov/science/USGSThesaurus/geologic%20history"/>
    <skos:related rdf:resource="http://www.usgs.gov/science/USGSThesaurus/tephrochronology"/>
    <skos:inScheme rdf:resource="http://www.usgs.gov/science/USGSThesaurus"/>
  </rdf:Description>
  <rdf:Description about="http://www.usgs.gov/science/USGSThesaurus/structural%20geology">
    <rdf:type rdf:resource="http://www.w3.org/2004/02/skos/core#Concept"/>
    <skos:prefLabel xml:lang="en">structural geology</skos:prefLabel>
    <skos:scopeNote xml:lang="en">Branch of geology concerned with the distribution, position, shape, and internal structure of rocks.</skos:scopeNote>
    <skos:broader rdf:resource="http://www.usgs.gov/science/USGSThesaurus/geology"/>
    <skos:related rdf:resource="http://www.usgs.gov/science/USGSThesaurus/earth%20structure"/>
    <skos:related rdf:resource="http://www.usgs.gov/science/USGSThesaurus/folding%20%28geologic%29"/>
    <skos:related rdf:resource="http://www.usgs.gov/science/USGSThesaurus/foliation%20%28geologic%29"/>
    <skos:related rdf:resource="http://www.usgs.gov/science/USGSThesaurus/fracture%20%28geologic%29"/>
    <skos:related rdf:resource="http://www.usgs.gov/science/USGSThesaurus/geologic%20structure"/>
    <skos:related rdf:resource="http://www.usgs.gov/science/USGSThesaurus/lineation%20%28geologic%29"/>
    <skos:related rdf:resource="http://www.usgs.gov/science/USGSThesaurus/neotectonic%20processes"/>
    <skos:related rdf:resource="http://www.usgs.gov/science/USGSThesaurus/structure%20contours"/>
    <skos:related rdf:resource="http://www.usgs.gov/science/USGSThesaurus/tectonic%20processes"/>
    <skos:related rdf:resource="http://www.usgs.gov/science/USGSThesaurus/tectonophysics"/>
    <skos:inScheme rdf:resource="http://www.usgs.gov/science/USGSThesaurus"/>
  </rdf:Description>
  <rdf:Description about="http://www.usgs.gov/science/USGSThesaurus/volcanology">
    <rdf:type rdf:resource="http://www.w3.org/2004/02/skos/core#Concept"/>
    <skos:prefLabel xml:lang="en">volcanology</skos:prefLabel>
    <skos:scopeNote xml:lang="en">The branch of geology that deals with volcanism and the processes involved in magma flow and eruption through a vent in the earth's surface.</skos:scopeNote>
    <skos:altLabel xml:lang="en">vulcanology</skos:altLabel>
    <skos:broader rdf:resource="http://www.usgs.gov/science/USGSThesaurus/geology"/>
    <skos:related rdf:resource="http://www.usgs.gov/science/USGSThesaurus/geothermal%20resources"/>
    <skos:related rdf:resource="http://www.usgs.gov/science/USGSThesaurus/seismology"/>
    <skos:related rdf:resource="http://www.usgs.gov/science/USGSThesaurus/tectonophysics"/>
    <skos:related rdf:resource="http://www.usgs.gov/science/USGSThesaurus/tiltmeter%20measurement"/>
    <skos:related rdf:resource="http://www.usgs.gov/science/USGSThesaurus/volcanic%20activity"/>
    <skos:inScheme rdf:resource="http://www.usgs.gov/science/USGSThesaurus"/>
  </rdf:Description>
  <rdf:Description about="http://www.usgs.gov/science/USGSThesaurus/geophysics">
    <rdf:type rdf:resource="http://www.w3.org/2004/02/skos/core#Concept"/>
    <skos:prefLabel xml:lang="en">geophysics</skos:prefLabel>
    <skos:scopeNote xml:lang="en">Branch of geology studying the physical characteristics and phenomena of the earth and its atmosphere.</skos:scopeNote>
    <!--FOR geophysical maps USE geophysics WITH maps and atlases-->
    <skos:altLabel xml:lang="en">geophysical maps</skos:altLabel>
    <skos:broader rdf:resource="http://www.usgs.gov/science/USGSThesaurus/earth%20sciences"/>
    <skos:narrower rdf:resource="http://www.usgs.gov/science/USGSThesaurus/geodesy"/>
    <skos:narrower rdf:resource="http://www.usgs.gov/science/USGSThesaurus/marine%20geophysics"/>
    <skos:narrower rdf:resource="http://www.usgs.gov/science/USGSThesaurus/seismology"/>
    <skos:narrower rdf:resource="http://www.usgs.gov/science/USGSThesaurus/tectonophysics"/>
    <skos:related rdf:resource="http://www.usgs.gov/science/USGSThesaurus/borehole%20logging"/>
    <skos:related rdf:resource="http://www.usgs.gov/science/USGSThesaurus/borehole%20temperature%20logging"/>
    <skos:related rdf:resource="http://www.usgs.gov/science/USGSThesaurus/core%20%28earth%29"/>
    <skos:related rdf:resource="http://www.usgs.gov/science/USGSThesaurus/Curie%20temperature%20analysis"/>
    <skos:related rdf:resource="http://www.usgs.gov/science/USGSThesaurus/gravitational%20field%20%28earth%29"/>
    <skos:related rdf:resource="http://www.usgs.gov/science/USGSThesaurus/heat%20flow%20%28earth%29"/>
    <skos:related rdf:resource="http://www.usgs.gov/science/USGSThesaurus/inner%20core%20%28earth%29"/>
    <skos:related rdf:resource="http://www.usgs.gov/science/USGSThesaurus/isostasy"/>
    <skos:related rdf:resource="http://www.usgs.gov/science/USGSThesaurus/laboratory-induced%20magnetization%20analysis"/>
    <skos:related rdf:resource="http://www.usgs.gov/science/USGSThesaurus/magnetic%20field%20%28earth%29"/>
    <skos:related rdf:resource="http://www.usgs.gov/science/USGSThesaurus/magnetic%20hysteresis%20analysis"/>
    <skos:related rdf:resource="http://www.usgs.gov/science/USGSThesaurus/magnetic%20susceptibility%20analysis"/>
    <skos:related rdf:resource="http://www.usgs.gov/science/USGSThesaurus/mantle%20%28earth%29"/>
    <skos:related rdf:resource="http://www.usgs.gov/science/USGSThesaurus/metamorphism%20%28geological%29"/>
    <skos:related rdf:resource="http://www.usgs.gov/science/USGSThesaurus/natural%20remanent%20magnetization%20analysis"/>
    <skos:related rdf:resource="http://www.usgs.gov/science/USGSThesaurus/outer%20core%20%28earth%29"/>
    <skos:related rdf:resource="http://www.usgs.gov/science/USGSThesaurus/paleomagnetic%20analysis"/>
    <skos:inScheme rdf:resource="http://www.usgs.gov/science/USGSThesaurus"/>
  </rdf:Description>
  <rdf:Description about="http://www.usgs.gov/science/USGSThesaurus/geodesy">
    <rdf:type rdf:resource="http://www.w3.org/2004/02/skos/core#Concept"/>
    <skos:prefLabel xml:lang="en">geodesy</skos:prefLabel>
    <skos:scopeNote xml:lang="en">Branch of science dealing with measuring the earth or large areas of the earth for making maps, determining the size and shape of the earth, and correlating gravitational, geological, and magnetic surveys of the earth.</skos:scopeNote>
    <skos:broader rdf:resource="http://www.usgs.gov/science/USGSThesaurus/geophysics"/>
    <skos:related rdf:resource="http://www.usgs.gov/science/USGSThesaurus/geography"/>
    <skos:related rdf:resource="http://www.usgs.gov/science/USGSThesaurus/land%20surveying"/>
    <skos:inScheme rdf:resource="http://www.usgs.gov/science/USGSThesaurus"/>
  </rdf:Description>
  <rdf:Description about="http://www.usgs.gov/science/USGSThesaurus/marine%20geophysics">
    <rdf:type rdf:resource="http://www.w3.org/2004/02/skos/core#Concept"/>
    <skos:prefLabel xml:lang="en">marine geophysics</skos:prefLabel>
    <skos:scopeNote xml:lang="en">Branch of earth sciences concerned with the physical processes of the oceans and continental margins.</skos:scopeNote>
    <skos:broader rdf:resource="http://www.usgs.gov/science/USGSThesaurus/geophysics"/>
    <skos:related rdf:resource="http://www.usgs.gov/science/USGSThesaurus/marine%20geology"/>
    <skos:related rdf:resource="http://www.usgs.gov/science/USGSThesaurus/ocean%20characteristics"/>
    <skos:related rdf:resource="http://www.usgs.gov/science/USGSThesaurus/ocean%20processes"/>
    <skos:related rdf:resource="http://www.usgs.gov/science/USGSThesaurus/ocean%20sciences"/>
    <skos:inScheme rdf:resource="http://www.usgs.gov/science/USGSThesaurus"/>
  </rdf:Description>
  <rdf:Description about="http://www.usgs.gov/science/USGSThesaurus/seismology">
    <rdf:type rdf:resource="http://www.w3.org/2004/02/skos/core#Concept"/>
    <skos:prefLabel xml:lang="en">seismology</skos:prefLabel>
    <skos:scopeNote xml:lang="en">Branch of earth sciences concerned with the study of earthquakes and man-induced seismic waves.</skos:scopeNote>
    <!--FOR earthquake seismology USE seismology WITH earthquake occurrences-->
    <skos:altLabel xml:lang="en">earthquake seismology</skos:altLabel>
    <!--FOR engineering seismology USE seismology WITH engineering sciences-->
    <skos:altLabel xml:lang="en">engineering seismology</skos:altLabel>
    <!--FOR exploration seismology USE seismology WITH natural resource exploration-->
    <skos:altLabel xml:lang="en">exploration seismology</skos:altLabel>
    <skos:broader rdf:resource="http://www.usgs.gov/science/USGSThesaurus/geophysics"/>
    <skos:narrower rdf:resource="http://www.usgs.gov/science/USGSThesaurus/paleoseismology"/>
    <skos:related rdf:resource="http://www.usgs.gov/science/USGSThesaurus/earthquake%20occurrences"/>
    <skos:related rdf:resource="http://www.usgs.gov/science/USGSThesaurus/earthquakes"/>
    <skos:related rdf:resource="http://www.usgs.gov/science/USGSThesaurus/seismic%20methods"/>
    <skos:related rdf:resource="http://www.usgs.gov/science/USGSThesaurus/seismic%20networking"/>
    <skos:related rdf:resource="http://www.usgs.gov/science/USGSThesaurus/seismic%20reflection%20methods"/>
    <skos:related rdf:resource="http://www.usgs.gov/science/USGSThesaurus/seismic%20refraction%20methods"/>
    <skos:related rdf:resource="http://www.usgs.gov/science/USGSThesaurus/tectonic%20processes"/>
    <skos:related rdf:resource="http://www.usgs.gov/science/USGSThesaurus/tiltmeter%20measurement"/>
    <skos:related rdf:resource="http://www.usgs.gov/science/USGSThesaurus/tsunamis"/>
    <skos:related rdf:resource="http://www.usgs.gov/science/USGSThesaurus/volcanology"/>
    <skos:inScheme rdf:resource="http://www.usgs.gov/science/USGSThesaurus"/>
  </rdf:Description>
  <rdf:Description about="http://www.usgs.gov/science/USGSThesaurus/paleoseismology">
    <rdf:type rdf:resource="http://www.w3.org/2004/02/skos/core#Concept"/>
    <skos:prefLabel xml:lang="en">paleoseismology</skos:prefLabel>
    <skos:scopeNote xml:lang="en">Branch of seismology concerned with ancient earthquakes.  Clues which indicate seismic activities in the geologic past are used  to date and determine the effects of those earthquakes.</skos:scopeNote>
    <skos:broader rdf:resource="http://www.usgs.gov/science/USGSThesaurus/seismology"/>
    <skos:related rdf:resource="http://www.usgs.gov/science/USGSThesaurus/geologic%20history"/>
    <skos:inScheme rdf:resource="http://www.usgs.gov/science/USGSThesaurus"/>
  </rdf:Description>
  <rdf:Description about="http://www.usgs.gov/science/USGSThesaurus/tectonophysics">
    <rdf:type rdf:resource="http://www.w3.org/2004/02/skos/core#Concept"/>
    <skos:prefLabel xml:lang="en">tectonophysics</skos:prefLabel>
    <skos:scopeNote xml:lang="en">Branch of geophysics concerned with the structural forces affecting the deformation, uplift, and movement of the earth's crust.</skos:scopeNote>
    <skos:broader rdf:resource="http://www.usgs.gov/science/USGSThesaurus/geophysics"/>
    <skos:related rdf:resource="http://www.usgs.gov/science/USGSThesaurus/asthenosphere"/>
    <skos:related rdf:resource="http://www.usgs.gov/science/USGSThesaurus/continental%20lithosphere"/>
    <skos:related rdf:resource="http://www.usgs.gov/science/USGSThesaurus/crust%20%28earth%29"/>
    <skos:related rdf:resource="http://www.usgs.gov/science/USGSThesaurus/earth%20history"/>
    <skos:related rdf:resource="http://www.usgs.gov/science/USGSThesaurus/earth%20structure"/>
    <skos:related rdf:resource="http://www.usgs.gov/science/USGSThesaurus/earthquakes"/>
    <skos:related rdf:resource="http://www.usgs.gov/science/USGSThesaurus/lithosphere"/>
    <skos:related rdf:resource="http://www.usgs.gov/science/USGSThesaurus/neotectonic%20processes"/>
    <skos:related rdf:resource="http://www.usgs.gov/science/USGSThesaurus/oceanic%20lithosphere"/>
    <skos:related rdf:resource="http://www.usgs.gov/science/USGSThesaurus/structural%20geology"/>
    <skos:related rdf:resource="http://www.usgs.gov/science/USGSThesaurus/tectonic%20processes"/>
    <skos:related rdf:resource="http://www.usgs.gov/science/USGSThesaurus/volcanology"/>
    <skos:inScheme rdf:resource="http://www.usgs.gov/science/USGSThesaurus"/>
  </rdf:Description>
  <rdf:Description about="http://www.usgs.gov/science/USGSThesaurus/glaciology">
    <rdf:type rdf:resource="http://www.w3.org/2004/02/skos/core#Concept"/>
    <skos:prefLabel xml:lang="en">glaciology</skos:prefLabel>
    <skos:scopeNote xml:lang="en">Science dealing with the features, origins, processes, and properties of snow, ice, glaciers, and ice sheets.</skos:scopeNote>
    <skos:altLabel xml:lang="en">cryology</skos:altLabel>
    <skos:altLabel xml:lang="en">glacial geology</skos:altLabel>
    <skos:broader rdf:resource="http://www.usgs.gov/science/USGSThesaurus/earth%20sciences"/>
    <skos:related rdf:resource="http://www.usgs.gov/science/USGSThesaurus/drilling%20and%20coring"/>
    <skos:related rdf:resource="http://www.usgs.gov/science/USGSThesaurus/erosion"/>
    <skos:related rdf:resource="http://www.usgs.gov/science/USGSThesaurus/glaciation"/>
    <skos:related rdf:resource="http://www.usgs.gov/science/USGSThesaurus/isostasy"/>
    <skos:related rdf:resource="http://www.usgs.gov/science/USGSThesaurus/snow%20and%20ice%20cover"/>
    <skos:inScheme rdf:resource="http://www.usgs.gov/science/USGSThesaurus"/>
  </rdf:Description>
  <rdf:Description about="http://www.usgs.gov/science/USGSThesaurus/hydrology">
    <rdf:type rdf:resource="http://www.w3.org/2004/02/skos/core#Concept"/>
    <skos:prefLabel xml:lang="en">hydrology</skos:prefLabel>
    <skos:scopeNote xml:lang="en">Branch of earth science that deals with water as it occurs in the atmosphere, on the surface of the ground, and underground.</skos:scopeNote>
    <!--FOR hydrologic maps USE hydrology WITH maps and atlases-->
    <skos:altLabel xml:lang="en">hydrologic maps</skos:altLabel>
    <skos:broader rdf:resource="http://www.usgs.gov/science/USGSThesaurus/earth%20sciences"/>
    <skos:narrower rdf:resource="http://www.usgs.gov/science/USGSThesaurus/hydrodynamics"/>
    <skos:related rdf:resource="http://www.usgs.gov/science/USGSThesaurus/domestic%20well%20water%20use"/>
    <skos:related rdf:resource="http://www.usgs.gov/science/USGSThesaurus/erosion"/>
    <skos:related rdf:resource="http://www.usgs.gov/science/USGSThesaurus/floods"/>
    <skos:related rdf:resource="http://www.usgs.gov/science/USGSThesaurus/geologic%20processes"/>
    <skos:related rdf:resource="http://www.usgs.gov/science/USGSThesaurus/groundwater%20quality"/>
    <skos:related rdf:resource="http://www.usgs.gov/science/USGSThesaurus/hydrothermal%20processes"/>
    <skos:related rdf:resource="http://www.usgs.gov/science/USGSThesaurus/industrial%20water%20use"/>
    <skos:related rdf:resource="http://www.usgs.gov/science/USGSThesaurus/irrigation"/>
    <skos:related rdf:resource="http://www.usgs.gov/science/USGSThesaurus/limnology"/>
    <skos:related rdf:resource="http://www.usgs.gov/science/USGSThesaurus/marine%20water%20quality"/>
    <skos:related rdf:resource="http://www.usgs.gov/science/USGSThesaurus/meteorology"/>
    <skos:related rdf:resource="http://www.usgs.gov/science/USGSThesaurus/mining%20water%20use"/>
    <skos:related rdf:resource="http://www.usgs.gov/science/USGSThesaurus/nutrient%20content%20%28water%29"/>
    <skos:related rdf:resource="http://www.usgs.gov/science/USGSThesaurus/ocean%20sciences"/>
    <skos:related rdf:resource="http://www.usgs.gov/science/USGSThesaurus/oxygen%20content%20%28water%29"/>
    <skos:related rdf:resource="http://www.usgs.gov/science/USGSThesaurus/power%20generation%20water%20use"/>
    <skos:related rdf:resource="http://www.usgs.gov/science/USGSThesaurus/precipitation%20%28atmospheric%29"/>
    <skos:related rdf:resource="http://www.usgs.gov/science/USGSThesaurus/stream%20discharge"/>
    <skos:related rdf:resource="http://www.usgs.gov/science/USGSThesaurus/river%20reaches"/>
    <skos:related rdf:resource="http://www.usgs.gov/science/USGSThesaurus/river%20systems"/>
    <skos:related rdf:resource="http://www.usgs.gov/science/USGSThesaurus/salinity"/>
    <skos:related rdf:resource="http://www.usgs.gov/science/USGSThesaurus/sediment%20transport"/>
    <skos:related rdf:resource="http://www.usgs.gov/science/USGSThesaurus/streamflow"/>
    <skos:related rdf:resource="http://www.usgs.gov/science/USGSThesaurus/stream-gage%20measurement"/>
    <skos:related rdf:resource="http://www.usgs.gov/science/USGSThesaurus/surface%20water%20%28non-marine%29"/>
    <skos:related rdf:resource="http://www.usgs.gov/science/USGSThesaurus/surface%20water%20quality"/>
    <skos:related rdf:resource="http://www.usgs.gov/science/USGSThesaurus/suspended%20material%20%28water%29"/>
    <skos:related rdf:resource="http://www.usgs.gov/science/USGSThesaurus/wastewater%20discharge"/>
    <skos:related rdf:resource="http://www.usgs.gov/science/USGSThesaurus/water%20circulation"/>
    <skos:related rdf:resource="http://www.usgs.gov/science/USGSThesaurus/water%20hardness"/>
    <skos:related rdf:resource="http://www.usgs.gov/science/USGSThesaurus/water%20pH"/>
    <skos:related rdf:resource="http://www.usgs.gov/science/USGSThesaurus/water%20properties"/>
    <skos:related rdf:resource="http://www.usgs.gov/science/USGSThesaurus/water%20quality"/>
    <skos:related rdf:resource="http://www.usgs.gov/science/USGSThesaurus/water%20resources"/>
    <skos:related rdf:resource="http://www.usgs.gov/science/USGSThesaurus/water%20sampling"/>
    <skos:related rdf:resource="http://www.usgs.gov/science/USGSThesaurus/water%20temperature"/>
    <skos:related rdf:resource="http://www.usgs.gov/science/USGSThesaurus/water%20use"/>
    <skos:related rdf:resource="http://www.usgs.gov/science/USGSThesaurus/wetland%20functions"/>
    <skos:related rdf:resource="http://www.usgs.gov/science/USGSThesaurus/hydrogeology"/>
    <skos:inScheme rdf:resource="http://www.usgs.gov/science/USGSThesaurus"/>
  </rdf:Description>
  <rdf:Description about="http://www.usgs.gov/science/USGSThesaurus/hydrodynamics">
    <rdf:type rdf:resource="http://www.w3.org/2004/02/skos/core#Concept"/>
    <skos:prefLabel xml:lang="en">hydrodynamics</skos:prefLabel>
    <skos:scopeNote xml:lang="en">Principles of fluid dynamics applied to water bodies.</skos:scopeNote>
    <skos:altLabel xml:lang="en">fluid dynamics</skos:altLabel>
    <skos:broader rdf:resource="http://www.usgs.gov/science/USGSThesaurus/hydrology"/>
    <skos:inScheme rdf:resource="http://www.usgs.gov/science/USGSThesaurus"/>
  </rdf:Description>
  <rdf:Description about="http://www.usgs.gov/science/USGSThesaurus/limnology">
    <rdf:type rdf:resource="http://www.w3.org/2004/02/skos/core#Concept"/>
    <skos:prefLabel xml:lang="en">limnology</skos:prefLabel>
    <skos:scopeNote xml:lang="en">Scientific study of the physical and biological characteristics of inland bodies of water such as lakes and ponds.</skos:scopeNote>
    <skos:broader rdf:resource="http://www.usgs.gov/science/USGSThesaurus/earth%20sciences"/>
    <skos:related rdf:resource="http://www.usgs.gov/science/USGSThesaurus/aquatic%20ecosystems"/>
    <skos:related rdf:resource="http://www.usgs.gov/science/USGSThesaurus/bathymetry"/>
    <skos:related rdf:resource="http://www.usgs.gov/science/USGSThesaurus/benthic%20ecosystems"/>
    <skos:related rdf:resource="http://www.usgs.gov/science/USGSThesaurus/CTD%20measurement"/>
    <skos:related rdf:resource="http://www.usgs.gov/science/USGSThesaurus/eutrophication"/>
    <skos:related rdf:resource="http://www.usgs.gov/science/USGSThesaurus/freshwater%20ecosystems"/>
    <skos:related rdf:resource="http://www.usgs.gov/science/USGSThesaurus/hydrology"/>
    <skos:related rdf:resource="http://www.usgs.gov/science/USGSThesaurus/surface%20water%20%28non-marine%29"/>
    <skos:related rdf:resource="http://www.usgs.gov/science/USGSThesaurus/surface%20water%20quality"/>
    <skos:related rdf:resource="http://www.usgs.gov/science/USGSThesaurus/water%20resources"/>
    <skos:inScheme rdf:resource="http://www.usgs.gov/science/USGSThesaurus"/>
  </rdf:Description>
  <rdf:Description about="http://www.usgs.gov/science/USGSThesaurus/ocean%20sciences">
    <rdf:type rdf:resource="http://www.w3.org/2004/02/skos/core#Concept"/>
    <skos:prefLabel xml:lang="en">ocean sciences</skos:prefLabel>
    <skos:scopeNote xml:lang="en">Sciences involved in the study of geological, biological, chemical, and physical characteristics and processes of the oceans.</skos:scopeNote>
    <skos:altLabel xml:lang="en">oceanography</skos:altLabel>
    <skos:altLabel xml:lang="en">physical oceanography</skos:altLabel>
    <skos:broader rdf:resource="http://www.usgs.gov/science/USGSThesaurus/earth%20sciences"/>
    <skos:narrower rdf:resource="http://www.usgs.gov/science/USGSThesaurus/paleoceanography"/>
    <skos:related rdf:resource="http://www.usgs.gov/science/USGSThesaurus/bathymetry"/>
    <skos:related rdf:resource="http://www.usgs.gov/science/USGSThesaurus/CTD%20measurement"/>
    <skos:related rdf:resource="http://www.usgs.gov/science/USGSThesaurus/effects%20of%20climate%20change"/>
    <skos:related rdf:resource="http://www.usgs.gov/science/USGSThesaurus/hydrology"/>
    <skos:related rdf:resource="http://www.usgs.gov/science/USGSThesaurus/marine%20biology"/>
    <skos:related rdf:resource="http://www.usgs.gov/science/USGSThesaurus/marine%20chemistry"/>
    <skos:related rdf:resource="http://www.usgs.gov/science/USGSThesaurus/marine%20geology"/>
    <skos:related rdf:resource="http://www.usgs.gov/science/USGSThesaurus/marine%20geophysics"/>
    <skos:related rdf:resource="http://www.usgs.gov/science/USGSThesaurus/marine%20water%20quality"/>
    <skos:related rdf:resource="http://www.usgs.gov/science/USGSThesaurus/meteorology"/>
    <skos:related rdf:resource="http://www.usgs.gov/science/USGSThesaurus/ocean%20characteristics"/>
    <skos:related rdf:resource="http://www.usgs.gov/science/USGSThesaurus/ocean%20circulation"/>
    <skos:related rdf:resource="http://www.usgs.gov/science/USGSThesaurus/ocean%20currents"/>
    <skos:related rdf:resource="http://www.usgs.gov/science/USGSThesaurus/ocean%20processes"/>
    <skos:related rdf:resource="http://www.usgs.gov/science/USGSThesaurus/ocean%20salinity"/>
    <skos:related rdf:resource="http://www.usgs.gov/science/USGSThesaurus/ocean%20temperature"/>
    <skos:related rdf:resource="http://www.usgs.gov/science/USGSThesaurus/ocean%20waves"/>
    <skos:related rdf:resource="http://www.usgs.gov/science/USGSThesaurus/ocean-atmosphere%20interaction"/>
    <skos:related rdf:resource="http://www.usgs.gov/science/USGSThesaurus/sea-floor%20characteristics"/>
    <skos:related rdf:resource="http://www.usgs.gov/science/USGSThesaurus/sea-level%20change"/>
    <skos:related rdf:resource="http://www.usgs.gov/science/USGSThesaurus/tides%20%28oceanic%29"/>
    <skos:related rdf:resource="http://www.usgs.gov/science/USGSThesaurus/tsunamis"/>
    <skos:related rdf:resource="http://www.usgs.gov/science/USGSThesaurus/underwater%20photography"/>
    <skos:inScheme rdf:resource="http://www.usgs.gov/science/USGSThesaurus"/>
  </rdf:Description>
  <rdf:Description about="http://www.usgs.gov/science/USGSThesaurus/paleoceanography">
    <rdf:type rdf:resource="http://www.w3.org/2004/02/skos/core#Concept"/>
    <skos:prefLabel xml:lang="en">paleoceanography</skos:prefLabel>
    <skos:scopeNote xml:lang="en">Study of the oceans in the geologic past, including their physical, chemical, biologic, and geologic history.</skos:scopeNote>
    <skos:broader rdf:resource="http://www.usgs.gov/science/USGSThesaurus/ocean%20sciences"/>
    <skos:related rdf:resource="http://www.usgs.gov/science/USGSThesaurus/paleontology"/>
    <skos:inScheme rdf:resource="http://www.usgs.gov/science/USGSThesaurus"/>
  </rdf:Description>
  <rdf:Description about="http://www.usgs.gov/science/USGSThesaurus/paleontology">
    <rdf:type rdf:resource="http://www.w3.org/2004/02/skos/core#Concept"/>
    <skos:prefLabel xml:lang="en">paleontology</skos:prefLabel>
    <skos:scopeNote xml:lang="en">Study of life in past geologic time based on fossil plants and animals.</skos:scopeNote>
    <skos:altLabel xml:lang="en">paleozoology</skos:altLabel>
    <skos:altLabel xml:lang="en">phylogeny</skos:altLabel>
    <skos:altLabel xml:lang="en">taphonomy</skos:altLabel>
    <skos:broader rdf:resource="http://www.usgs.gov/science/USGSThesaurus/earth%20sciences"/>
    <skos:narrower rdf:resource="http://www.usgs.gov/science/USGSThesaurus/invertebrate%20paleontology"/>
    <skos:narrower rdf:resource="http://www.usgs.gov/science/USGSThesaurus/micropaleontology"/>
    <skos:narrower rdf:resource="http://www.usgs.gov/science/USGSThesaurus/paleobotany"/>
    <skos:narrower rdf:resource="http://www.usgs.gov/science/USGSThesaurus/vertebrate%20paleontology"/>
    <skos:related rdf:resource="http://www.usgs.gov/science/USGSThesaurus/biostratigraphy"/>
    <skos:related rdf:resource="http://www.usgs.gov/science/USGSThesaurus/fossils"/>
    <skos:related rdf:resource="http://www.usgs.gov/science/USGSThesaurus/geologic%20history"/>
    <skos:related rdf:resource="http://www.usgs.gov/science/USGSThesaurus/ichnofossils"/>
    <skos:related rdf:resource="http://www.usgs.gov/science/USGSThesaurus/life%20sciences"/>
    <skos:related rdf:resource="http://www.usgs.gov/science/USGSThesaurus/paleoceanography"/>
    <skos:inScheme rdf:resource="http://www.usgs.gov/science/USGSThesaurus"/>
  </rdf:Description>
  <rdf:Description about="http://www.usgs.gov/science/USGSThesaurus/invertebrate%20paleontology">
    <rdf:type rdf:resource="http://www.w3.org/2004/02/skos/core#Concept"/>
    <skos:prefLabel xml:lang="en">invertebrate paleontology</skos:prefLabel>
    <skos:scopeNote xml:lang="en">Branch of paleontology which deals with fossil animals without backbones.</skos:scopeNote>
    <skos:broader rdf:resource="http://www.usgs.gov/science/USGSThesaurus/paleontology"/>
    <skos:related rdf:resource="http://www.usgs.gov/science/USGSThesaurus/bryozoans%20and%20brachiopods"/>
    <skos:related rdf:resource="http://www.usgs.gov/science/USGSThesaurus/conodonts"/>
    <skos:related rdf:resource="http://www.usgs.gov/science/USGSThesaurus/invertebrate%20zoology"/>
    <skos:related rdf:resource="http://www.usgs.gov/science/USGSThesaurus/invertebrates"/>
    <skos:related rdf:resource="http://www.usgs.gov/science/USGSThesaurus/trilobites"/>
    <skos:inScheme rdf:resource="http://www.usgs.gov/science/USGSThesaurus"/>
  </rdf:Description>
  <rdf:Description about="http://www.usgs.gov/science/USGSThesaurus/micropaleontology">
    <rdf:type rdf:resource="http://www.w3.org/2004/02/skos/core#Concept"/>
    <skos:prefLabel xml:lang="en">micropaleontology</skos:prefLabel>
    <skos:scopeNote xml:lang="en">Branch of paleontology dealing with fossils too small to be seen without a microscope.</skos:scopeNote>
    <skos:broader rdf:resource="http://www.usgs.gov/science/USGSThesaurus/paleontology"/>
    <skos:related rdf:resource="http://www.usgs.gov/science/USGSThesaurus/calcareous%20nannoplankton"/>
    <skos:related rdf:resource="http://www.usgs.gov/science/USGSThesaurus/conodonts"/>
    <skos:related rdf:resource="http://www.usgs.gov/science/USGSThesaurus/diatoms"/>
    <skos:related rdf:resource="http://www.usgs.gov/science/USGSThesaurus/dinoflagellates"/>
    <skos:related rdf:resource="http://www.usgs.gov/science/USGSThesaurus/faunal%20and%20floral%20census%20%28microscopic%29"/>
    <skos:related rdf:resource="http://www.usgs.gov/science/USGSThesaurus/fossils"/>
    <skos:related rdf:resource="http://www.usgs.gov/science/USGSThesaurus/protists"/>
    <skos:inScheme rdf:resource="http://www.usgs.gov/science/USGSThesaurus"/>
  </rdf:Description>
  <rdf:Description about="http://www.usgs.gov/science/USGSThesaurus/paleobotany">
    <rdf:type rdf:resource="http://www.w3.org/2004/02/skos/core#Concept"/>
    <skos:prefLabel xml:lang="en">paleobotany</skos:prefLabel>
    <skos:scopeNote xml:lang="en">Branch of paleontology concerned with the study of fossil plants and plant life in the geologic past.</skos:scopeNote>
    <skos:broader rdf:resource="http://www.usgs.gov/science/USGSThesaurus/paleontology"/>
    <skos:related rdf:resource="http://www.usgs.gov/science/USGSThesaurus/botany"/>
    <skos:related rdf:resource="http://www.usgs.gov/science/USGSThesaurus/palynology"/>
    <skos:inScheme rdf:resource="http://www.usgs.gov/science/USGSThesaurus"/>
  </rdf:Description>
  <rdf:Description about="http://www.usgs.gov/science/USGSThesaurus/vertebrate%20paleontology">
    <rdf:type rdf:resource="http://www.w3.org/2004/02/skos/core#Concept"/>
    <skos:prefLabel xml:lang="en">vertebrate paleontology</skos:prefLabel>
    <skos:scopeNote xml:lang="en">Branch of paleontology dealing with fossil animals that have spinal columns.</skos:scopeNote>
    <skos:broader rdf:resource="http://www.usgs.gov/science/USGSThesaurus/paleontology"/>
    <skos:related rdf:resource="http://www.usgs.gov/science/USGSThesaurus/dinosaurs"/>
    <skos:related rdf:resource="http://www.usgs.gov/science/USGSThesaurus/vertebrates"/>
    <skos:inScheme rdf:resource="http://www.usgs.gov/science/USGSThesaurus"/>
  </rdf:Description>
  <rdf:Description about="http://www.usgs.gov/science/USGSThesaurus/soil%20sciences">
    <rdf:type rdf:resource="http://www.w3.org/2004/02/skos/core#Concept"/>
    <skos:prefLabel xml:lang="en">soil sciences</skos:prefLabel>
    <skos:scopeNote xml:lang="en">Earth sciences dealing with the origin, classification, physical, chemical, and biological properties of soils.</skos:scopeNote>
    <skos:altLabel xml:lang="en">pedology (soils)</skos:altLabel>
    <skos:broader rdf:resource="http://www.usgs.gov/science/USGSThesaurus/earth%20sciences"/>
    <skos:related rdf:resource="http://www.usgs.gov/science/USGSThesaurus/soil%20chemistry"/>
    <skos:related rdf:resource="http://www.usgs.gov/science/USGSThesaurus/soil%20resources"/>
    <skos:related rdf:resource="http://www.usgs.gov/science/USGSThesaurus/trenching"/>
    <skos:related rdf:resource="http://www.usgs.gov/science/USGSThesaurus/soil%20horizons"/>
    <skos:inScheme rdf:resource="http://www.usgs.gov/science/USGSThesaurus"/>
  </rdf:Description>
  <rdf:Description about="http://www.usgs.gov/science/USGSThesaurus/engineering%20sciences">
    <rdf:type rdf:resource="http://www.w3.org/2004/02/skos/core#Concept"/>
    <skos:prefLabel xml:lang="en">engineering sciences</skos:prefLabel>
    <skos:scopeNote xml:lang="en">Sciences involved in the application of scientific and mathematical principles to construction, machinery, mechanical design, mining and manufacturing processes and other practical activities.</skos:scopeNote>
    <!--FOR engineering seismology USE engineering sciences WITH seismology-->
    <skos:altLabel xml:lang="en">engineering seismology</skos:altLabel>
    <skos:broader rdf:resource="http://www.usgs.gov/science/USGSThesaurus/sciences"/>
    <skos:narrower rdf:resource="http://www.usgs.gov/science/USGSThesaurus/engineering%20geology"/>
    <skos:narrower rdf:resource="http://www.usgs.gov/science/USGSThesaurus/hydraulic%20engineering"/>
    <skos:related rdf:resource="http://www.usgs.gov/science/USGSThesaurus/instrument%20design%20and%20development"/>
    <skos:related rdf:resource="http://www.usgs.gov/science/USGSThesaurus/mining%20hazards"/>
    <skos:related rdf:resource="http://www.usgs.gov/science/USGSThesaurus/scientific%20careers"/>
    <skos:inScheme rdf:resource="http://www.usgs.gov/science/USGSThesaurus"/>
  </rdf:Description>
  <rdf:Description about="http://www.usgs.gov/science/USGSThesaurus/engineering%20geology">
    <rdf:type rdf:resource="http://www.w3.org/2004/02/skos/core#Concept"/>
    <skos:prefLabel xml:lang="en">engineering geology</skos:prefLabel>
    <skos:scopeNote xml:lang="en">Branch of geology involved in the application of soil and rock mechanics, natural hazards, and other geological studies to the practice of engineering and construction.</skos:scopeNote>
    <!--FOR engineering geology maps USE engineering geology WITH maps and atlases-->
    <skos:altLabel xml:lang="en">engineering geology maps</skos:altLabel>
    <!--FOR geotechnical properties maps USE engineering geology WITH maps and atlases-->
    <skos:altLabel xml:lang="en">geotechnical properties maps</skos:altLabel>
    <!--FOR rock mechanics maps USE engineering geology WITH maps and atlases-->
    <skos:altLabel xml:lang="en">rock mechanics maps</skos:altLabel>
    <skos:broader rdf:resource="http://www.usgs.gov/science/USGSThesaurus/engineering%20sciences"/>
    <skos:related rdf:resource="http://www.usgs.gov/science/USGSThesaurus/geology"/>
    <skos:related rdf:resource="http://www.usgs.gov/science/USGSThesaurus/liquefaction"/>
    <skos:related rdf:resource="http://www.usgs.gov/science/USGSThesaurus/remediation"/>
    <skos:related rdf:resource="http://www.usgs.gov/science/USGSThesaurus/mitigation%20of%20coastal%20hazards"/>
    <skos:inScheme rdf:resource="http://www.usgs.gov/science/USGSThesaurus"/>
  </rdf:Description>
  <rdf:Description about="http://www.usgs.gov/science/USGSThesaurus/hydraulic%20engineering">
    <rdf:type rdf:resource="http://www.w3.org/2004/02/skos/core#Concept"/>
    <skos:prefLabel xml:lang="en">hydraulic engineering</skos:prefLabel>
    <skos:scopeNote xml:lang="en">Branch of engineering which applies the physical properties of fluids, such as flow and pressure, to the design and use of machinery, pumps, pipelines, etc.</skos:scopeNote>
    <skos:altLabel xml:lang="en">hydraulic models</skos:altLabel>
    <skos:altLabel xml:lang="en">hydraulics</skos:altLabel>
    <skos:broader rdf:resource="http://www.usgs.gov/science/USGSThesaurus/engineering%20sciences"/>
    <skos:related rdf:resource="http://www.usgs.gov/science/USGSThesaurus/domestic%20well%20water%20use"/>
    <skos:related rdf:resource="http://www.usgs.gov/science/USGSThesaurus/industrial%20water%20use"/>
    <skos:related rdf:resource="http://www.usgs.gov/science/USGSThesaurus/irrigation"/>
    <skos:related rdf:resource="http://www.usgs.gov/science/USGSThesaurus/mining%20water%20use"/>
    <skos:related rdf:resource="http://www.usgs.gov/science/USGSThesaurus/power%20generation%20water%20use"/>
    <skos:related rdf:resource="http://www.usgs.gov/science/USGSThesaurus/wastewater%20discharge"/>
    <skos:related rdf:resource="http://www.usgs.gov/science/USGSThesaurus/water%20use"/>
    <skos:related rdf:resource="http://www.usgs.gov/science/USGSThesaurus/water%20resource%20management"/>
    <skos:related rdf:resource="http://www.usgs.gov/science/USGSThesaurus/dredging"/>
    <skos:inScheme rdf:resource="http://www.usgs.gov/science/USGSThesaurus"/>
  </rdf:Description>
  <rdf:Description about="http://www.usgs.gov/science/USGSThesaurus/information%20sciences">
    <rdf:type rdf:resource="http://www.w3.org/2004/02/skos/core#Concept"/>
    <skos:prefLabel xml:lang="en">information sciences</skos:prefLabel>
    <skos:scopeNote xml:lang="en">Sciences dealing with the compilation, processing, classification, display, transmission, storage, and retrieval of recorded knowledge.</skos:scopeNote>
    <skos:broader rdf:resource="http://www.usgs.gov/science/USGSThesaurus/sciences"/>
    <skos:narrower rdf:resource="http://www.usgs.gov/science/USGSThesaurus/biological%20informatics"/>
    <skos:narrower rdf:resource="http://www.usgs.gov/science/USGSThesaurus/computer%20science"/>
    <skos:related rdf:resource="http://www.usgs.gov/science/USGSThesaurus/geographic%20information%20systems"/>
    <skos:related rdf:resource="http://www.usgs.gov/science/USGSThesaurus/information%20system%20design%20and%20development"/>
    <skos:related rdf:resource="http://www.usgs.gov/science/USGSThesaurus/metadata%20development"/>
    <skos:related rdf:resource="http://www.usgs.gov/science/USGSThesaurus/scientific%20careers"/>
    <skos:inScheme rdf:resource="http://www.usgs.gov/science/USGSThesaurus"/>
  </rdf:Description>
  <rdf:Description about="http://www.usgs.gov/science/USGSThesaurus/biological%20informatics">
    <rdf:type rdf:resource="http://www.w3.org/2004/02/skos/core#Concept"/>
    <skos:prefLabel xml:lang="en">biological informatics</skos:prefLabel>
    <skos:scopeNote xml:lang="en">Development and use of computer, statistical, and other tools in the collection, organization, dissemination, and use of information to solve problems in the life sciences. </skos:scopeNote>
    <skos:altLabel xml:lang="en">bioinformatics</skos:altLabel>
    <skos:broader rdf:resource="http://www.usgs.gov/science/USGSThesaurus/information%20sciences"/>
    <skos:related rdf:resource="http://www.usgs.gov/science/USGSThesaurus/life%20sciences"/>
    <skos:inScheme rdf:resource="http://www.usgs.gov/science/USGSThesaurus"/>
  </rdf:Description>
  <rdf:Description about="http://www.usgs.gov/science/USGSThesaurus/computer%20science">
    <rdf:type rdf:resource="http://www.w3.org/2004/02/skos/core#Concept"/>
    <skos:prefLabel xml:lang="en">computer science</skos:prefLabel>
    <skos:scopeNote xml:lang="en">Study of computers, including their design (architecture),  uses (computations, data processing), and systems control.</skos:scopeNote>
    <skos:broader rdf:resource="http://www.usgs.gov/science/USGSThesaurus/information%20sciences"/>
    <skos:inScheme rdf:resource="http://www.usgs.gov/science/USGSThesaurus"/>
  </rdf:Description>
  <rdf:Description about="http://www.usgs.gov/science/USGSThesaurus/life%20sciences">
    <rdf:type rdf:resource="http://www.w3.org/2004/02/skos/core#Concept"/>
    <skos:prefLabel xml:lang="en">life sciences</skos:prefLabel>
    <skos:scopeNote xml:lang="en">Branches of science that study living and fossil organisms.</skos:scopeNote>
    <skos:altLabel xml:lang="en">biological sciences</skos:altLabel>
    <skos:altLabel xml:lang="en">biology</skos:altLabel>
    <skos:broader rdf:resource="http://www.usgs.gov/science/USGSThesaurus/sciences"/>
    <skos:narrower rdf:resource="http://www.usgs.gov/science/USGSThesaurus/anatomy%20and%20physiology"/>
    <skos:narrower rdf:resource="http://www.usgs.gov/science/USGSThesaurus/aquatic%20biology"/>
    <skos:narrower rdf:resource="http://www.usgs.gov/science/USGSThesaurus/biochemistry"/>
    <skos:narrower rdf:resource="http://www.usgs.gov/science/USGSThesaurus/botany"/>
    <skos:narrower rdf:resource="http://www.usgs.gov/science/USGSThesaurus/cell%20biology"/>
    <skos:narrower rdf:resource="http://www.usgs.gov/science/USGSThesaurus/developmental%20biology"/>
    <skos:narrower rdf:resource="http://www.usgs.gov/science/USGSThesaurus/ecology"/>
    <skos:narrower rdf:resource="http://www.usgs.gov/science/USGSThesaurus/ecotoxicology"/>
    <skos:narrower rdf:resource="http://www.usgs.gov/science/USGSThesaurus/genetics"/>
    <skos:narrower rdf:resource="http://www.usgs.gov/science/USGSThesaurus/marine%20biology"/>
    <skos:narrower rdf:resource="http://www.usgs.gov/science/USGSThesaurus/microbiology"/>
    <skos:narrower rdf:resource="http://www.usgs.gov/science/USGSThesaurus/molecular%20biology"/>
    <skos:narrower rdf:resource="http://www.usgs.gov/science/USGSThesaurus/morphology%20%28biological%29"/>
    <skos:narrower rdf:resource="http://www.usgs.gov/science/USGSThesaurus/mycology"/>
    <skos:narrower rdf:resource="http://www.usgs.gov/science/USGSThesaurus/parasitology"/>
    <skos:narrower rdf:resource="http://www.usgs.gov/science/USGSThesaurus/pathology"/>
    <skos:narrower rdf:resource="http://www.usgs.gov/science/USGSThesaurus/systematics%20and%20taxonomy"/>
    <skos:narrower rdf:resource="http://www.usgs.gov/science/USGSThesaurus/zoology"/>
    <skos:related rdf:resource="http://www.usgs.gov/science/USGSThesaurus/biodiversity"/>
    <skos:related rdf:resource="http://www.usgs.gov/science/USGSThesaurus/biological%20informatics"/>
    <skos:related rdf:resource="http://www.usgs.gov/science/USGSThesaurus/biological%20productivity"/>
    <skos:related rdf:resource="http://www.usgs.gov/science/USGSThesaurus/biota"/>
    <skos:related rdf:resource="http://www.usgs.gov/science/USGSThesaurus/decomposers"/>
    <skos:related rdf:resource="http://www.usgs.gov/science/USGSThesaurus/disease%20vectors"/>
    <skos:related rdf:resource="http://www.usgs.gov/science/USGSThesaurus/dispersal%20%28organisms%29"/>
    <skos:related rdf:resource="http://www.usgs.gov/science/USGSThesaurus/endangered%20species"/>
    <skos:related rdf:resource="http://www.usgs.gov/science/USGSThesaurus/endemic%20species"/>
    <skos:related rdf:resource="http://www.usgs.gov/science/USGSThesaurus/extinction%20and%20extirpation"/>
    <skos:related rdf:resource="http://www.usgs.gov/science/USGSThesaurus/health%20and%20disease"/>
    <skos:related rdf:resource="http://www.usgs.gov/science/USGSThesaurus/invasive%20species"/>
    <skos:related rdf:resource="http://www.usgs.gov/science/USGSThesaurus/migration%20%28organisms%29"/>
    <skos:related rdf:resource="http://www.usgs.gov/science/USGSThesaurus/native%20species"/>
    <skos:related rdf:resource="http://www.usgs.gov/science/USGSThesaurus/natural%20resources"/>
    <skos:related rdf:resource="http://www.usgs.gov/science/USGSThesaurus/nonindigenous%20species"/>
    <skos:related rdf:resource="http://www.usgs.gov/science/USGSThesaurus/organism%20groupings%20%28non-taxonomic%29"/>
    <skos:related rdf:resource="http://www.usgs.gov/science/USGSThesaurus/organisms"/>
    <skos:related rdf:resource="http://www.usgs.gov/science/USGSThesaurus/paleontology"/>
    <skos:related rdf:resource="http://www.usgs.gov/science/USGSThesaurus/plant%20and%20animal%20tagging"/>
    <skos:related rdf:resource="http://www.usgs.gov/science/USGSThesaurus/scientific%20careers"/>
    <skos:related rdf:resource="http://www.usgs.gov/science/USGSThesaurus/sexing%20%28plants%20%26%20animals%29"/>
    <skos:inScheme rdf:resource="http://www.usgs.gov/science/USGSThesaurus"/>
  </rdf:Description>
  <rdf:Description about="http://www.usgs.gov/science/USGSThesaurus/anatomy%20and%20physiology">
    <rdf:type rdf:resource="http://www.w3.org/2004/02/skos/core#Concept"/>
    <skos:prefLabel xml:lang="en">anatomy and physiology</skos:prefLabel>
    <skos:scopeNote xml:lang="en">Study of the body structures (anatomy) and life functions and activities (physiology)of plants and animals.</skos:scopeNote>
    <skos:altLabel xml:lang="en">physiology</skos:altLabel>
    <skos:broader rdf:resource="http://www.usgs.gov/science/USGSThesaurus/life%20sciences"/>
    <skos:narrower rdf:resource="http://www.usgs.gov/science/USGSThesaurus/endocrinology"/>
    <skos:narrower rdf:resource="http://www.usgs.gov/science/USGSThesaurus/histology"/>
    <skos:narrower rdf:resource="http://www.usgs.gov/science/USGSThesaurus/immunology"/>
    <skos:related rdf:resource="http://www.usgs.gov/science/USGSThesaurus/plant%20and%20animal%20testing"/>
    <skos:related rdf:resource="http://www.usgs.gov/science/USGSThesaurus/therapeutic%20methods"/>
    <skos:inScheme rdf:resource="http://www.usgs.gov/science/USGSThesaurus"/>
  </rdf:Description>
  <rdf:Description about="http://www.usgs.gov/science/USGSThesaurus/endocrinology">
    <rdf:type rdf:resource="http://www.w3.org/2004/02/skos/core#Concept"/>
    <skos:prefLabel xml:lang="en">endocrinology</skos:prefLabel>
    <skos:scopeNote xml:lang="en">Study of the collection of ductless glands that secrete hormones which influence growth, gender, sexual maturity, and other attributes.</skos:scopeNote>
    <skos:broader rdf:resource="http://www.usgs.gov/science/USGSThesaurus/anatomy%20and%20physiology"/>
    <skos:related rdf:resource="http://www.usgs.gov/science/USGSThesaurus/health%20and%20disease"/>
    <skos:inScheme rdf:resource="http://www.usgs.gov/science/USGSThesaurus"/>
  </rdf:Description>
  <rdf:Description about="http://www.usgs.gov/science/USGSThesaurus/histology">
    <rdf:type rdf:resource="http://www.w3.org/2004/02/skos/core#Concept"/>
    <skos:prefLabel xml:lang="en">histology</skos:prefLabel>
    <skos:scopeNote xml:lang="en">Branch of anatomy concerned with the microscopic structure of plant and animal tissue.</skos:scopeNote>
    <skos:broader rdf:resource="http://www.usgs.gov/science/USGSThesaurus/anatomy%20and%20physiology"/>
    <skos:related rdf:resource="http://www.usgs.gov/science/USGSThesaurus/health%20and%20disease"/>
    <skos:inScheme rdf:resource="http://www.usgs.gov/science/USGSThesaurus"/>
  </rdf:Description>
  <rdf:Description about="http://www.usgs.gov/science/USGSThesaurus/immunology">
    <rdf:type rdf:resource="http://www.w3.org/2004/02/skos/core#Concept"/>
    <skos:prefLabel xml:lang="en">immunology</skos:prefLabel>
    <skos:scopeNote xml:lang="en">Branch of biology which studies the body's production of lymphocytes, antibodies, and macrophages in response to foreign substances or pathogenic organisms.</skos:scopeNote>
    <skos:broader rdf:resource="http://www.usgs.gov/science/USGSThesaurus/anatomy%20and%20physiology"/>
    <skos:related rdf:resource="http://www.usgs.gov/science/USGSThesaurus/health%20and%20disease"/>
    <skos:inScheme rdf:resource="http://www.usgs.gov/science/USGSThesaurus"/>
  </rdf:Description>
  <rdf:Description about="http://www.usgs.gov/science/USGSThesaurus/aquatic%20biology">
    <rdf:type rdf:resource="http://www.w3.org/2004/02/skos/core#Concept"/>
    <skos:prefLabel xml:lang="en">aquatic biology</skos:prefLabel>
    <skos:scopeNote xml:lang="en">The scientific study of organisms living in or near water.  This term is to be used for the science of 'aquatic biology' and for  biological studies in fresh and brackish water. For marine biological studies, use 'marine biology'.</skos:scopeNote>
    <skos:broader rdf:resource="http://www.usgs.gov/science/USGSThesaurus/life%20sciences"/>
    <skos:related rdf:resource="http://www.usgs.gov/science/USGSThesaurus/aquatic%20ecosystems"/>
    <skos:related rdf:resource="http://www.usgs.gov/science/USGSThesaurus/benthic%20ecosystems"/>
    <skos:related rdf:resource="http://www.usgs.gov/science/USGSThesaurus/commercial%20fishery%20resources"/>
    <skos:related rdf:resource="http://www.usgs.gov/science/USGSThesaurus/ecology"/>
    <skos:related rdf:resource="http://www.usgs.gov/science/USGSThesaurus/estuarine%20ecosystems"/>
    <skos:related rdf:resource="http://www.usgs.gov/science/USGSThesaurus/fishery%20resources"/>
    <skos:related rdf:resource="http://www.usgs.gov/science/USGSThesaurus/freshwater%20ecosystems"/>
    <skos:related rdf:resource="http://www.usgs.gov/science/USGSThesaurus/inland%20fishery%20resources"/>
    <skos:related rdf:resource="http://www.usgs.gov/science/USGSThesaurus/macroinvertebrates"/>
    <skos:related rdf:resource="http://www.usgs.gov/science/USGSThesaurus/marine%20biology"/>
    <skos:related rdf:resource="http://www.usgs.gov/science/USGSThesaurus/marine%20ecosystems"/>
    <skos:related rdf:resource="http://www.usgs.gov/science/USGSThesaurus/marine%20fishery%20resources"/>
    <skos:related rdf:resource="http://www.usgs.gov/science/USGSThesaurus/migratory%20species"/>
    <skos:related rdf:resource="http://www.usgs.gov/science/USGSThesaurus/plankton"/>
    <skos:related rdf:resource="http://www.usgs.gov/science/USGSThesaurus/recreational%20fishery%20resources"/>
    <skos:related rdf:resource="http://www.usgs.gov/science/USGSThesaurus/shellfish"/>
    <skos:related rdf:resource="http://www.usgs.gov/science/USGSThesaurus/water%20quality"/>
    <skos:related rdf:resource="http://www.usgs.gov/science/USGSThesaurus/wetland%20ecosystems"/>
    <skos:inScheme rdf:resource="http://www.usgs.gov/science/USGSThesaurus"/>
  </rdf:Description>
  <rdf:Description about="http://www.usgs.gov/science/USGSThesaurus/biochemistry">
    <rdf:type rdf:resource="http://www.w3.org/2004/02/skos/core#Concept"/>
    <skos:prefLabel xml:lang="en">biochemistry</skos:prefLabel>
    <skos:scopeNote xml:lang="en">Study of chemical processes that occur within or are mediated by living organisms.</skos:scopeNote>
    <skos:altLabel xml:lang="en">biogeochemistry</skos:altLabel>
    <skos:altLabel xml:lang="en">chemistry (life sciences)</skos:altLabel>
    <skos:altLabel xml:lang="en">environmental chemistry</skos:altLabel>
    <skos:broader rdf:resource="http://www.usgs.gov/science/USGSThesaurus/life%20sciences"/>
    <skos:related rdf:resource="http://www.usgs.gov/science/USGSThesaurus/atomic%20absorption%20analysis"/>
    <skos:related rdf:resource="http://www.usgs.gov/science/USGSThesaurus/biogeochemical%20cycling"/>
    <skos:related rdf:resource="http://www.usgs.gov/science/USGSThesaurus/carbon%20cycling"/>
    <skos:related rdf:resource="http://www.usgs.gov/science/USGSThesaurus/carbon%20isotope%20analysis"/>
    <skos:related rdf:resource="http://www.usgs.gov/science/USGSThesaurus/chemical%20analysis"/>
    <skos:related rdf:resource="http://www.usgs.gov/science/USGSThesaurus/chromatography"/>
    <skos:related rdf:resource="http://www.usgs.gov/science/USGSThesaurus/DNA%20sequencing"/>
    <skos:related rdf:resource="http://www.usgs.gov/science/USGSThesaurus/electrophoresis"/>
    <skos:related rdf:resource="http://www.usgs.gov/science/USGSThesaurus/flow%20cytometry"/>
    <skos:related rdf:resource="http://www.usgs.gov/science/USGSThesaurus/food%20web"/>
    <skos:related rdf:resource="http://www.usgs.gov/science/USGSThesaurus/gas%20chromatography"/>
    <skos:related rdf:resource="http://www.usgs.gov/science/USGSThesaurus/isotopic%20analysis"/>
    <skos:related rdf:resource="http://www.usgs.gov/science/USGSThesaurus/light%20stable%20isotope%20analysis"/>
    <skos:related rdf:resource="http://www.usgs.gov/science/USGSThesaurus/liquid%20chromatography"/>
    <skos:related rdf:resource="http://www.usgs.gov/science/USGSThesaurus/mass%20spectroscopy"/>
    <skos:related rdf:resource="http://www.usgs.gov/science/USGSThesaurus/mercury%20contamination"/>
    <skos:related rdf:resource="http://www.usgs.gov/science/USGSThesaurus/neutron%20activation%20analysis"/>
    <skos:related rdf:resource="http://www.usgs.gov/science/USGSThesaurus/nutrient%20cycling"/>
    <skos:related rdf:resource="http://www.usgs.gov/science/USGSThesaurus/oxygen%20isotope%20analysis"/>
    <skos:related rdf:resource="http://www.usgs.gov/science/USGSThesaurus/particle-beam%20spectroscopy"/>
    <skos:related rdf:resource="http://www.usgs.gov/science/USGSThesaurus/pesticide%20and%20herbicide%20contamination"/>
    <skos:related rdf:resource="http://www.usgs.gov/science/USGSThesaurus/polymerase%20chain%20reaction"/>
    <skos:related rdf:resource="http://www.usgs.gov/science/USGSThesaurus/tritium%20analysis"/>
    <skos:inScheme rdf:resource="http://www.usgs.gov/science/USGSThesaurus"/>
  </rdf:Description>
  <rdf:Description about="http://www.usgs.gov/science/USGSThesaurus/botany">
    <rdf:type rdf:resource="http://www.w3.org/2004/02/skos/core#Concept"/>
    <skos:prefLabel xml:lang="en">botany</skos:prefLabel>
    <skos:scopeNote xml:lang="en">The science of plants.</skos:scopeNote>
    <skos:broader rdf:resource="http://www.usgs.gov/science/USGSThesaurus/life%20sciences"/>
    <skos:narrower rdf:resource="http://www.usgs.gov/science/USGSThesaurus/palynology"/>
    <skos:narrower rdf:resource="http://www.usgs.gov/science/USGSThesaurus/phycology"/>
    <skos:related rdf:resource="http://www.usgs.gov/science/USGSThesaurus/drilling%20and%20coring"/>
    <skos:related rdf:resource="http://www.usgs.gov/science/USGSThesaurus/ferns%20and%20fern%20allies"/>
    <skos:related rdf:resource="http://www.usgs.gov/science/USGSThesaurus/flowering%20plants"/>
    <skos:related rdf:resource="http://www.usgs.gov/science/USGSThesaurus/forest%20resources"/>
    <skos:related rdf:resource="http://www.usgs.gov/science/USGSThesaurus/gymnosperms"/>
    <skos:related rdf:resource="http://www.usgs.gov/science/USGSThesaurus/liverworts%20and%20hornworts"/>
    <skos:related rdf:resource="http://www.usgs.gov/science/USGSThesaurus/mosses"/>
    <skos:related rdf:resource="http://www.usgs.gov/science/USGSThesaurus/mycology"/>
    <skos:related rdf:resource="http://www.usgs.gov/science/USGSThesaurus/nonvascular%20plants"/>
    <skos:related rdf:resource="http://www.usgs.gov/science/USGSThesaurus/paleobotany"/>
    <skos:related rdf:resource="http://www.usgs.gov/science/USGSThesaurus/plants%20%28organisms%29"/>
    <skos:related rdf:resource="http://www.usgs.gov/science/USGSThesaurus/producers%20%28organisms%29"/>
    <skos:related rdf:resource="http://www.usgs.gov/science/USGSThesaurus/vascular%20plants"/>
    <skos:related rdf:resource="http://www.usgs.gov/science/USGSThesaurus/vegetation"/>
    <skos:inScheme rdf:resource="http://www.usgs.gov/science/USGSThesaurus"/>
  </rdf:Description>
  <rdf:Description about="http://www.usgs.gov/science/USGSThesaurus/palynology">
    <rdf:type rdf:resource="http://www.w3.org/2004/02/skos/core#Concept"/>
    <skos:prefLabel xml:lang="en">palynology</skos:prefLabel>
    <skos:scopeNote xml:lang="en">Branch of botany concerned with the study of pollen and spores, especially fossil remains. These are used to study plant life and dispersal in geologic history and to date deposits.</skos:scopeNote>
    <skos:broader rdf:resource="http://www.usgs.gov/science/USGSThesaurus/botany"/>
    <skos:related rdf:resource="http://www.usgs.gov/science/USGSThesaurus/paleobotany"/>
    <skos:related rdf:resource="http://www.usgs.gov/science/USGSThesaurus/plants%20%28organisms%29"/>
    <skos:inScheme rdf:resource="http://www.usgs.gov/science/USGSThesaurus"/>
  </rdf:Description>
  <rdf:Description about="http://www.usgs.gov/science/USGSThesaurus/phycology">
    <rdf:type rdf:resource="http://www.w3.org/2004/02/skos/core#Concept"/>
    <skos:prefLabel xml:lang="en">phycology</skos:prefLabel>
    <skos:scopeNote xml:lang="en">Branch of biology concerned with the study of algae.</skos:scopeNote>
    <skos:altLabel xml:lang="en">algology</skos:altLabel>
    <skos:broader rdf:resource="http://www.usgs.gov/science/USGSThesaurus/botany"/>
    <skos:related rdf:resource="http://www.usgs.gov/science/USGSThesaurus/algae"/>
    <skos:related rdf:resource="http://www.usgs.gov/science/USGSThesaurus/algal%20blooms"/>
    <skos:related rdf:resource="http://www.usgs.gov/science/USGSThesaurus/calcareous%20nannoplankton"/>
    <skos:related rdf:resource="http://www.usgs.gov/science/USGSThesaurus/diatoms"/>
    <skos:related rdf:resource="http://www.usgs.gov/science/USGSThesaurus/dinoflagellates"/>
    <skos:related rdf:resource="http://www.usgs.gov/science/USGSThesaurus/lichens"/>
    <skos:related rdf:resource="http://www.usgs.gov/science/USGSThesaurus/plankton"/>
    <skos:inScheme rdf:resource="http://www.usgs.gov/science/USGSThesaurus"/>
  </rdf:Description>
  <rdf:Description about="http://www.usgs.gov/science/USGSThesaurus/cell%20biology">
    <rdf:type rdf:resource="http://www.w3.org/2004/02/skos/core#Concept"/>
    <skos:prefLabel xml:lang="en">cell biology</skos:prefLabel>
    <skos:scopeNote xml:lang="en">Branch of biology that deals with the study of the formation, structure, and physiology of cells.</skos:scopeNote>
    <skos:altLabel xml:lang="en">cellular biology</skos:altLabel>
    <skos:altLabel xml:lang="en">cytology</skos:altLabel>
    <skos:broader rdf:resource="http://www.usgs.gov/science/USGSThesaurus/life%20sciences"/>
    <skos:related rdf:resource="http://www.usgs.gov/science/USGSThesaurus/flow%20cytometry"/>
    <skos:related rdf:resource="http://www.usgs.gov/science/USGSThesaurus/molecular%20biology"/>
    <skos:inScheme rdf:resource="http://www.usgs.gov/science/USGSThesaurus"/>
  </rdf:Description>
  <rdf:Description about="http://www.usgs.gov/science/USGSThesaurus/developmental%20biology">
    <rdf:type rdf:resource="http://www.w3.org/2004/02/skos/core#Concept"/>
    <skos:prefLabel xml:lang="en">developmental biology</skos:prefLabel>
    <skos:scopeNote xml:lang="en">Scientific study of the processes related to the transformation of living organisms from single cells to complex multi-celled individuals.</skos:scopeNote>
    <skos:altLabel xml:lang="en">embryology</skos:altLabel>
    <skos:broader rdf:resource="http://www.usgs.gov/science/USGSThesaurus/life%20sciences"/>
    <skos:related rdf:resource="http://www.usgs.gov/science/USGSThesaurus/organism%20growth%20and%20development"/>
    <skos:inScheme rdf:resource="http://www.usgs.gov/science/USGSThesaurus"/>
  </rdf:Description>
  <rdf:Description about="http://www.usgs.gov/science/USGSThesaurus/ecology">
    <rdf:type rdf:resource="http://www.w3.org/2004/02/skos/core#Concept"/>
    <skos:prefLabel xml:lang="en">ecology</skos:prefLabel>
    <skos:scopeNote xml:lang="en">Study of the relations between living plants and animals and their environment.</skos:scopeNote>
    <skos:altLabel xml:lang="en">bionomics</skos:altLabel>
    <skos:broader rdf:resource="http://www.usgs.gov/science/USGSThesaurus/life%20sciences"/>
    <skos:related rdf:resource="http://www.usgs.gov/science/USGSThesaurus/animal%20behavior"/>
    <skos:related rdf:resource="http://www.usgs.gov/science/USGSThesaurus/aquatic%20biology"/>
    <skos:related rdf:resource="http://www.usgs.gov/science/USGSThesaurus/aquatic%20ecosystems"/>
    <skos:related rdf:resource="http://www.usgs.gov/science/USGSThesaurus/benthic%20ecosystems"/>
    <skos:related rdf:resource="http://www.usgs.gov/science/USGSThesaurus/bioaccumulation"/>
    <skos:related rdf:resource="http://www.usgs.gov/science/USGSThesaurus/biodiversity"/>
    <skos:related rdf:resource="http://www.usgs.gov/science/USGSThesaurus/biogeochemical%20cycling"/>
    <skos:related rdf:resource="http://www.usgs.gov/science/USGSThesaurus/biogeography"/>
    <skos:related rdf:resource="http://www.usgs.gov/science/USGSThesaurus/biological%20productivity"/>
    <skos:related rdf:resource="http://www.usgs.gov/science/USGSThesaurus/bioremediation"/>
    <skos:related rdf:resource="http://www.usgs.gov/science/USGSThesaurus/carbon%20cycling"/>
    <skos:related rdf:resource="http://www.usgs.gov/science/USGSThesaurus/carnivores"/>
    <skos:related rdf:resource="http://www.usgs.gov/science/USGSThesaurus/coastal%20ecosystems"/>
    <skos:related rdf:resource="http://www.usgs.gov/science/USGSThesaurus/community%20ecology"/>
    <skos:related rdf:resource="http://www.usgs.gov/science/USGSThesaurus/consumers%20%28organisms%29"/>
    <skos:related rdf:resource="http://www.usgs.gov/science/USGSThesaurus/decomposers"/>
    <skos:related rdf:resource="http://www.usgs.gov/science/USGSThesaurus/desert%20ecosystems"/>
    <skos:related rdf:resource="http://www.usgs.gov/science/USGSThesaurus/desertification"/>
    <skos:related rdf:resource="http://www.usgs.gov/science/USGSThesaurus/dispersal%20%28organisms%29"/>
    <skos:related rdf:resource="http://www.usgs.gov/science/USGSThesaurus/ecological%20competition"/>
    <skos:related rdf:resource="http://www.usgs.gov/science/USGSThesaurus/ecological%20processes"/>
    <skos:related rdf:resource="http://www.usgs.gov/science/USGSThesaurus/ecosystem%20functions"/>
    <skos:related rdf:resource="http://www.usgs.gov/science/USGSThesaurus/ecosystem%20monitoring"/>
    <skos:related rdf:resource="http://www.usgs.gov/science/USGSThesaurus/ecosystems"/>
    <skos:related rdf:resource="http://www.usgs.gov/science/USGSThesaurus/ecotoxicology"/>
    <skos:related rdf:resource="http://www.usgs.gov/science/USGSThesaurus/endangered%20species"/>
    <skos:related rdf:resource="http://www.usgs.gov/science/USGSThesaurus/endemic%20species"/>
    <skos:related rdf:resource="http://www.usgs.gov/science/USGSThesaurus/estuarine%20ecosystems"/>
    <skos:related rdf:resource="http://www.usgs.gov/science/USGSThesaurus/eutrophication"/>
    <skos:related rdf:resource="http://www.usgs.gov/science/USGSThesaurus/extinction%20and%20extirpation"/>
    <skos:related rdf:resource="http://www.usgs.gov/science/USGSThesaurus/fires"/>
    <skos:related rdf:resource="http://www.usgs.gov/science/USGSThesaurus/food%20web"/>
    <skos:related rdf:resource="http://www.usgs.gov/science/USGSThesaurus/forest%20ecosystems"/>
    <skos:related rdf:resource="http://www.usgs.gov/science/USGSThesaurus/forest%20resources"/>
    <skos:related rdf:resource="http://www.usgs.gov/science/USGSThesaurus/freshwater%20ecosystems"/>
    <skos:related rdf:resource="http://www.usgs.gov/science/USGSThesaurus/effects%20of%20climate%20change"/>
    <skos:related rdf:resource="http://www.usgs.gov/science/USGSThesaurus/grassland%20ecosystems"/>
    <skos:related rdf:resource="http://www.usgs.gov/science/USGSThesaurus/habitat%20alteration"/>
    <skos:related rdf:resource="http://www.usgs.gov/science/USGSThesaurus/herbivores"/>
    <skos:related rdf:resource="http://www.usgs.gov/science/USGSThesaurus/human%20impacts"/>
    <skos:related rdf:resource="http://www.usgs.gov/science/USGSThesaurus/invasive%20species"/>
    <skos:related rdf:resource="http://www.usgs.gov/science/USGSThesaurus/land%20use%20change"/>
    <skos:related rdf:resource="http://www.usgs.gov/science/USGSThesaurus/long-term%20ecological%20monitoring"/>
    <skos:related rdf:resource="http://www.usgs.gov/science/USGSThesaurus/marine%20ecosystems"/>
    <skos:related rdf:resource="http://www.usgs.gov/science/USGSThesaurus/mercury%20contamination"/>
    <skos:related rdf:resource="http://www.usgs.gov/science/USGSThesaurus/migration%20%28organisms%29"/>
    <skos:related rdf:resource="http://www.usgs.gov/science/USGSThesaurus/migratory%20species"/>
    <skos:related rdf:resource="http://www.usgs.gov/science/USGSThesaurus/native%20species"/>
    <skos:related rdf:resource="http://www.usgs.gov/science/USGSThesaurus/nonindigenous%20species"/>
    <skos:related rdf:resource="http://www.usgs.gov/science/USGSThesaurus/nutrient%20cycling"/>
    <skos:related rdf:resource="http://www.usgs.gov/science/USGSThesaurus/omnivores"/>
    <skos:related rdf:resource="http://www.usgs.gov/science/USGSThesaurus/pesticide%20and%20herbicide%20contamination"/>
    <skos:related rdf:resource="http://www.usgs.gov/science/USGSThesaurus/plot%20sampling"/>
    <skos:related rdf:resource="http://www.usgs.gov/science/USGSThesaurus/pollinators"/>
    <skos:related rdf:resource="http://www.usgs.gov/science/USGSThesaurus/population%20and%20community%20ecology"/>
    <skos:related rdf:resource="http://www.usgs.gov/science/USGSThesaurus/population%20dynamics"/>
    <skos:related rdf:resource="http://www.usgs.gov/science/USGSThesaurus/producers%20%28organisms%29"/>
    <skos:related rdf:resource="http://www.usgs.gov/science/USGSThesaurus/reef%20ecosystems"/>
    <skos:related rdf:resource="http://www.usgs.gov/science/USGSThesaurus/remediation"/>
    <skos:related rdf:resource="http://www.usgs.gov/science/USGSThesaurus/shrubland%20ecosystems"/>
    <skos:related rdf:resource="http://www.usgs.gov/science/USGSThesaurus/succession%20%28biological%29"/>
    <skos:related rdf:resource="http://www.usgs.gov/science/USGSThesaurus/terrestrial%20ecosystems"/>
    <skos:related rdf:resource="http://www.usgs.gov/science/USGSThesaurus/tundra%20ecosystems"/>
    <skos:related rdf:resource="http://www.usgs.gov/science/USGSThesaurus/vegetation"/>
    <skos:related rdf:resource="http://www.usgs.gov/science/USGSThesaurus/waste%20treatment%20and%20disposal"/>
    <skos:related rdf:resource="http://www.usgs.gov/science/USGSThesaurus/wetland%20ecosystems"/>
    <skos:related rdf:resource="http://www.usgs.gov/science/USGSThesaurus/wetland%20functions"/>
    <skos:inScheme rdf:resource="http://www.usgs.gov/science/USGSThesaurus"/>
  </rdf:Description>
  <rdf:Description about="http://www.usgs.gov/science/USGSThesaurus/ecotoxicology">
    <rdf:type rdf:resource="http://www.w3.org/2004/02/skos/core#Concept"/>
    <skos:prefLabel xml:lang="en">ecotoxicology</skos:prefLabel>
    <skos:scopeNote xml:lang="en">Scientific study of causes, dispersal, and effects of contaminants on the environment.</skos:scopeNote>
    <skos:altLabel xml:lang="en">environmental toxicology</skos:altLabel>
    <skos:altLabel xml:lang="en">toxicology</skos:altLabel>
    <skos:broader rdf:resource="http://www.usgs.gov/science/USGSThesaurus/life%20sciences"/>
    <skos:related rdf:resource="http://www.usgs.gov/science/USGSThesaurus/bioaccumulation"/>
    <skos:related rdf:resource="http://www.usgs.gov/science/USGSThesaurus/contaminant%20transport"/>
    <skos:related rdf:resource="http://www.usgs.gov/science/USGSThesaurus/ecology"/>
    <skos:related rdf:resource="http://www.usgs.gov/science/USGSThesaurus/hazards"/>
    <skos:related rdf:resource="http://www.usgs.gov/science/USGSThesaurus/human%20impacts"/>
    <skos:related rdf:resource="http://www.usgs.gov/science/USGSThesaurus/mercury%20contamination"/>
    <skos:related rdf:resource="http://www.usgs.gov/science/USGSThesaurus/contamination%20and%20pollution"/>
    <skos:related rdf:resource="http://www.usgs.gov/science/USGSThesaurus/pesticide%20and%20herbicide%20contamination"/>
    <skos:related rdf:resource="http://www.usgs.gov/science/USGSThesaurus/plant%20and%20animal%20testing"/>
    <skos:related rdf:resource="http://www.usgs.gov/science/USGSThesaurus/therapeutic%20methods"/>
    <skos:related rdf:resource="http://www.usgs.gov/science/USGSThesaurus/toxic%20radionuclide%20contamination"/>
    <skos:related rdf:resource="http://www.usgs.gov/science/USGSThesaurus/toxic%20trace%20element%20contamination"/>
    <skos:inScheme rdf:resource="http://www.usgs.gov/science/USGSThesaurus"/>
  </rdf:Description>
  <rdf:Description about="http://www.usgs.gov/science/USGSThesaurus/genetics">
    <rdf:type rdf:resource="http://www.w3.org/2004/02/skos/core#Concept"/>
    <skos:prefLabel xml:lang="en">genetics</skos:prefLabel>
    <skos:scopeNote xml:lang="en">Branch of biology that deals with heredity or the passing of traits in living organisms from one generation to the next.</skos:scopeNote>
    <skos:altLabel xml:lang="en">heredity</skos:altLabel>
    <skos:broader rdf:resource="http://www.usgs.gov/science/USGSThesaurus/life%20sciences"/>
    <skos:related rdf:resource="http://www.usgs.gov/science/USGSThesaurus/DNA%20sequencing"/>
    <skos:related rdf:resource="http://www.usgs.gov/science/USGSThesaurus/molecular%20biology"/>
    <skos:related rdf:resource="http://www.usgs.gov/science/USGSThesaurus/polymerase%20chain%20reaction"/>
    <skos:inScheme rdf:resource="http://www.usgs.gov/science/USGSThesaurus"/>
  </rdf:Description>
  <rdf:Description about="http://www.usgs.gov/science/USGSThesaurus/marine%20biology">
    <rdf:type rdf:resource="http://www.w3.org/2004/02/skos/core#Concept"/>
    <skos:prefLabel xml:lang="en">marine biology</skos:prefLabel>
    <skos:scopeNote xml:lang="en">Branch of biology concerned with the organisms and habitats of the seas and oceans.</skos:scopeNote>
    <skos:altLabel xml:lang="en">biological oceanography</skos:altLabel>
    <skos:broader rdf:resource="http://www.usgs.gov/science/USGSThesaurus/life%20sciences"/>
    <skos:related rdf:resource="http://www.usgs.gov/science/USGSThesaurus/aquatic%20biology"/>
    <skos:related rdf:resource="http://www.usgs.gov/science/USGSThesaurus/aquatic%20ecosystems"/>
    <skos:related rdf:resource="http://www.usgs.gov/science/USGSThesaurus/benthic%20ecosystems"/>
    <skos:related rdf:resource="http://www.usgs.gov/science/USGSThesaurus/commercial%20fishery%20resources"/>
    <skos:related rdf:resource="http://www.usgs.gov/science/USGSThesaurus/fishery%20resources"/>
    <skos:related rdf:resource="http://www.usgs.gov/science/USGSThesaurus/marine%20ecosystems"/>
    <skos:related rdf:resource="http://www.usgs.gov/science/USGSThesaurus/marine%20fishery%20resources"/>
    <skos:related rdf:resource="http://www.usgs.gov/science/USGSThesaurus/migratory%20species"/>
    <skos:related rdf:resource="http://www.usgs.gov/science/USGSThesaurus/ocean%20sciences"/>
    <skos:related rdf:resource="http://www.usgs.gov/science/USGSThesaurus/recreational%20fishery%20resources"/>
    <skos:related rdf:resource="http://www.usgs.gov/science/USGSThesaurus/reef%20ecosystems"/>
    <skos:related rdf:resource="http://www.usgs.gov/science/USGSThesaurus/whaling"/>
    <skos:inScheme rdf:resource="http://www.usgs.gov/science/USGSThesaurus"/>
  </rdf:Description>
  <rdf:Description about="http://www.usgs.gov/science/USGSThesaurus/microbiology">
    <rdf:type rdf:resource="http://www.w3.org/2004/02/skos/core#Concept"/>
    <skos:prefLabel xml:lang="en">microbiology</skos:prefLabel>
    <skos:scopeNote xml:lang="en">Branch of biology dealing with organisms too small to be seen without the use of a microscope.</skos:scopeNote>
    <skos:broader rdf:resource="http://www.usgs.gov/science/USGSThesaurus/life%20sciences"/>
    <skos:narrower rdf:resource="http://www.usgs.gov/science/USGSThesaurus/bacteriology"/>
    <skos:narrower rdf:resource="http://www.usgs.gov/science/USGSThesaurus/virology"/>
    <skos:related rdf:resource="http://www.usgs.gov/science/USGSThesaurus/archaea"/>
    <skos:related rdf:resource="http://www.usgs.gov/science/USGSThesaurus/bacteria"/>
    <skos:related rdf:resource="http://www.usgs.gov/science/USGSThesaurus/culturing%20%28specimens%29"/>
    <skos:related rdf:resource="http://www.usgs.gov/science/USGSThesaurus/faunal%20and%20floral%20census%20%28microscopic%29"/>
    <skos:related rdf:resource="http://www.usgs.gov/science/USGSThesaurus/plankton"/>
    <skos:related rdf:resource="http://www.usgs.gov/science/USGSThesaurus/producers%20%28organisms%29"/>
    <skos:related rdf:resource="http://www.usgs.gov/science/USGSThesaurus/protists"/>
    <skos:inScheme rdf:resource="http://www.usgs.gov/science/USGSThesaurus"/>
  </rdf:Description>
  <rdf:Description about="http://www.usgs.gov/science/USGSThesaurus/bacteriology">
    <rdf:type rdf:resource="http://www.w3.org/2004/02/skos/core#Concept"/>
    <skos:prefLabel xml:lang="en">bacteriology</skos:prefLabel>
    <skos:scopeNote xml:lang="en">Study of the single celled microorganisms known as bacteria.</skos:scopeNote>
    <skos:broader rdf:resource="http://www.usgs.gov/science/USGSThesaurus/microbiology"/>
    <skos:related rdf:resource="http://www.usgs.gov/science/USGSThesaurus/culturing%20%28specimens%29"/>
    <skos:related rdf:resource="http://www.usgs.gov/science/USGSThesaurus/health%20and%20disease"/>
    <skos:inScheme rdf:resource="http://www.usgs.gov/science/USGSThesaurus"/>
  </rdf:Description>
  <rdf:Description about="http://www.usgs.gov/science/USGSThesaurus/virology">
    <rdf:type rdf:resource="http://www.w3.org/2004/02/skos/core#Concept"/>
    <skos:prefLabel xml:lang="en">virology</skos:prefLabel>
    <skos:scopeNote xml:lang="en">Branch of biology dealing with viruses and viral diseases.</skos:scopeNote>
    <skos:broader rdf:resource="http://www.usgs.gov/science/USGSThesaurus/microbiology"/>
    <skos:related rdf:resource="http://www.usgs.gov/science/USGSThesaurus/environmental%20health%20%28human%29"/>
    <skos:related rdf:resource="http://www.usgs.gov/science/USGSThesaurus/viruses"/>
    <skos:inScheme rdf:resource="http://www.usgs.gov/science/USGSThesaurus"/>
  </rdf:Description>
  <rdf:Description about="http://www.usgs.gov/science/USGSThesaurus/molecular%20biology">
    <rdf:type rdf:resource="http://www.w3.org/2004/02/skos/core#Concept"/>
    <skos:prefLabel xml:lang="en">molecular biology</skos:prefLabel>
    <skos:scopeNote xml:lang="en">Branch of biology concerned with the study of physiology at the molecular level.</skos:scopeNote>
    <skos:broader rdf:resource="http://www.usgs.gov/science/USGSThesaurus/life%20sciences"/>
    <skos:related rdf:resource="http://www.usgs.gov/science/USGSThesaurus/cell%20biology"/>
    <skos:related rdf:resource="http://www.usgs.gov/science/USGSThesaurus/genetics"/>
    <skos:related rdf:resource="http://www.usgs.gov/science/USGSThesaurus/organism%20growth%20and%20development"/>
    <skos:inScheme rdf:resource="http://www.usgs.gov/science/USGSThesaurus"/>
  </rdf:Description>
  <rdf:Description about="http://www.usgs.gov/science/USGSThesaurus/morphology%20%28biological%29">
    <rdf:type rdf:resource="http://www.w3.org/2004/02/skos/core#Concept"/>
    <skos:prefLabel xml:lang="en">morphology (biological)</skos:prefLabel>
    <skos:scopeNote xml:lang="en">The scientific study of the form, shape, and structure of plants and animals and their fossil remains.</skos:scopeNote>
    <skos:broader rdf:resource="http://www.usgs.gov/science/USGSThesaurus/life%20sciences"/>
    <skos:related rdf:resource="http://www.usgs.gov/science/USGSThesaurus/meristics"/>
    <skos:inScheme rdf:resource="http://www.usgs.gov/science/USGSThesaurus"/>
  </rdf:Description>
  <rdf:Description about="http://www.usgs.gov/science/USGSThesaurus/mycology">
    <rdf:type rdf:resource="http://www.w3.org/2004/02/skos/core#Concept"/>
    <skos:prefLabel xml:lang="en">mycology</skos:prefLabel>
    <skos:scopeNote xml:lang="en">Branch of biology concerned with the study of fungi.</skos:scopeNote>
    <skos:broader rdf:resource="http://www.usgs.gov/science/USGSThesaurus/life%20sciences"/>
    <skos:related rdf:resource="http://www.usgs.gov/science/USGSThesaurus/botany"/>
    <skos:related rdf:resource="http://www.usgs.gov/science/USGSThesaurus/fungi"/>
    <skos:related rdf:resource="http://www.usgs.gov/science/USGSThesaurus/lichens"/>
    <skos:inScheme rdf:resource="http://www.usgs.gov/science/USGSThesaurus"/>
  </rdf:Description>
  <rdf:Description about="http://www.usgs.gov/science/USGSThesaurus/parasitology">
    <rdf:type rdf:resource="http://www.w3.org/2004/02/skos/core#Concept"/>
    <skos:prefLabel xml:lang="en">parasitology</skos:prefLabel>
    <skos:scopeNote xml:lang="en">Branch of biology concerned with the study of organisms that, living on or in another organism, take nutrition from the host and often harm it.</skos:scopeNote>
    <skos:broader rdf:resource="http://www.usgs.gov/science/USGSThesaurus/life%20sciences"/>
    <skos:related rdf:resource="http://www.usgs.gov/science/USGSThesaurus/health%20and%20disease"/>
    <skos:related rdf:resource="http://www.usgs.gov/science/USGSThesaurus/wildlife%20biology"/>
    <skos:inScheme rdf:resource="http://www.usgs.gov/science/USGSThesaurus"/>
  </rdf:Description>
  <rdf:Description about="http://www.usgs.gov/science/USGSThesaurus/pathology">
    <rdf:type rdf:resource="http://www.w3.org/2004/02/skos/core#Concept"/>
    <skos:prefLabel xml:lang="en">pathology</skos:prefLabel>
    <skos:scopeNote xml:lang="en">Branch of biology concerned with the study of the causes, progress, symptoms, diagnosis, and effects of diseases.</skos:scopeNote>
    <skos:altLabel xml:lang="en">pathobiology</skos:altLabel>
    <skos:broader rdf:resource="http://www.usgs.gov/science/USGSThesaurus/life%20sciences"/>
    <skos:related rdf:resource="http://www.usgs.gov/science/USGSThesaurus/health%20and%20disease"/>
    <skos:related rdf:resource="http://www.usgs.gov/science/USGSThesaurus/plant%20and%20animal%20testing"/>
    <skos:related rdf:resource="http://www.usgs.gov/science/USGSThesaurus/therapeutic%20methods"/>
    <skos:inScheme rdf:resource="http://www.usgs.gov/science/USGSThesaurus"/>
  </rdf:Description>
  <rdf:Description about="http://www.usgs.gov/science/USGSThesaurus/systematics%20and%20taxonomy">
    <rdf:type rdf:resource="http://www.w3.org/2004/02/skos/core#Concept"/>
    <skos:prefLabel xml:lang="en">systematics and taxonomy</skos:prefLabel>
    <skos:scopeNote xml:lang="en">Study of the identification, naming, and classification of organisms.</skos:scopeNote>
    <skos:altLabel xml:lang="en">taxonomy</skos:altLabel>
    <skos:broader rdf:resource="http://www.usgs.gov/science/USGSThesaurus/life%20sciences"/>
    <skos:related rdf:resource="http://www.usgs.gov/science/USGSThesaurus/meristics"/>
    <skos:inScheme rdf:resource="http://www.usgs.gov/science/USGSThesaurus"/>
  </rdf:Description>
  <rdf:Description about="http://www.usgs.gov/science/USGSThesaurus/zoology">
    <rdf:type rdf:resource="http://www.w3.org/2004/02/skos/core#Concept"/>
    <skos:prefLabel xml:lang="en">zoology</skos:prefLabel>
    <skos:scopeNote xml:lang="en">Branch of biology that deals with the reproduction, development and growth, anatomy, physiology, and behavior of animals.</skos:scopeNote>
    <skos:altLabel xml:lang="en">malacology</skos:altLabel>
    <skos:broader rdf:resource="http://www.usgs.gov/science/USGSThesaurus/life%20sciences"/>
    <skos:narrower rdf:resource="http://www.usgs.gov/science/USGSThesaurus/ethology"/>
    <skos:narrower rdf:resource="http://www.usgs.gov/science/USGSThesaurus/invertebrate%20zoology"/>
    <skos:narrower rdf:resource="http://www.usgs.gov/science/USGSThesaurus/vertebrate%20zoology"/>
    <skos:narrower rdf:resource="http://www.usgs.gov/science/USGSThesaurus/wildlife%20biology"/>
    <skos:related rdf:resource="http://www.usgs.gov/science/USGSThesaurus/animals"/>
    <skos:related rdf:resource="http://www.usgs.gov/science/USGSThesaurus/capturing%20%28animals%29"/>
    <skos:related rdf:resource="http://www.usgs.gov/science/USGSThesaurus/carnivores"/>
    <skos:related rdf:resource="http://www.usgs.gov/science/USGSThesaurus/consumers%20%28organisms%29"/>
    <skos:related rdf:resource="http://www.usgs.gov/science/USGSThesaurus/herbivores"/>
    <skos:related rdf:resource="http://www.usgs.gov/science/USGSThesaurus/migratory%20species"/>
    <skos:related rdf:resource="http://www.usgs.gov/science/USGSThesaurus/omnivores"/>
    <skos:related rdf:resource="http://www.usgs.gov/science/USGSThesaurus/pollinators"/>
    <skos:inScheme rdf:resource="http://www.usgs.gov/science/USGSThesaurus"/>
  </rdf:Description>
  <rdf:Description about="http://www.usgs.gov/science/USGSThesaurus/ethology">
    <rdf:type rdf:resource="http://www.w3.org/2004/02/skos/core#Concept"/>
    <skos:prefLabel xml:lang="en">ethology</skos:prefLabel>
    <skos:scopeNote xml:lang="en">Study of animal behavior under natural conditions</skos:scopeNote>
    <skos:broader rdf:resource="http://www.usgs.gov/science/USGSThesaurus/zoology"/>
    <skos:related rdf:resource="http://www.usgs.gov/science/USGSThesaurus/animal%20behavior"/>
    <skos:inScheme rdf:resource="http://www.usgs.gov/science/USGSThesaurus"/>
  </rdf:Description>
  <rdf:Description about="http://www.usgs.gov/science/USGSThesaurus/invertebrate%20zoology">
    <rdf:type rdf:resource="http://www.w3.org/2004/02/skos/core#Concept"/>
    <skos:prefLabel xml:lang="en">invertebrate zoology</skos:prefLabel>
    <skos:scopeNote xml:lang="en">Branch of biology dealing with animals having no backbones or spinal columns.</skos:scopeNote>
    <skos:broader rdf:resource="http://www.usgs.gov/science/USGSThesaurus/zoology"/>
    <skos:narrower rdf:resource="http://www.usgs.gov/science/USGSThesaurus/entomology"/>
    <skos:related rdf:resource="http://www.usgs.gov/science/USGSThesaurus/arachnids"/>
    <skos:related rdf:resource="http://www.usgs.gov/science/USGSThesaurus/arthropods"/>
    <skos:related rdf:resource="http://www.usgs.gov/science/USGSThesaurus/bryozoans%20and%20brachiopods"/>
    <skos:related rdf:resource="http://www.usgs.gov/science/USGSThesaurus/coelenterates"/>
    <skos:related rdf:resource="http://www.usgs.gov/science/USGSThesaurus/crustaceans"/>
    <skos:related rdf:resource="http://www.usgs.gov/science/USGSThesaurus/echinoderms"/>
    <skos:related rdf:resource="http://www.usgs.gov/science/USGSThesaurus/flatworms"/>
    <skos:related rdf:resource="http://www.usgs.gov/science/USGSThesaurus/horseshoe%20crabs"/>
    <skos:related rdf:resource="http://www.usgs.gov/science/USGSThesaurus/invertebrate%20paleontology"/>
    <skos:related rdf:resource="http://www.usgs.gov/science/USGSThesaurus/invertebrates"/>
    <skos:related rdf:resource="http://www.usgs.gov/science/USGSThesaurus/mollusks"/>
    <skos:related rdf:resource="http://www.usgs.gov/science/USGSThesaurus/ostracodes"/>
    <skos:related rdf:resource="http://www.usgs.gov/science/USGSThesaurus/roundworms"/>
    <skos:related rdf:resource="http://www.usgs.gov/science/USGSThesaurus/segmented%20worms"/>
    <skos:related rdf:resource="http://www.usgs.gov/science/USGSThesaurus/shellfish"/>
    <skos:related rdf:resource="http://www.usgs.gov/science/USGSThesaurus/sponges"/>
    <skos:related rdf:resource="http://www.usgs.gov/science/USGSThesaurus/worms"/>
    <skos:inScheme rdf:resource="http://www.usgs.gov/science/USGSThesaurus"/>
  </rdf:Description>
  <rdf:Description about="http://www.usgs.gov/science/USGSThesaurus/entomology">
    <rdf:type rdf:resource="http://www.w3.org/2004/02/skos/core#Concept"/>
    <skos:prefLabel xml:lang="en">entomology</skos:prefLabel>
    <skos:scopeNote xml:lang="en">Branch of zoology involved in studying insects.</skos:scopeNote>
    <skos:broader rdf:resource="http://www.usgs.gov/science/USGSThesaurus/invertebrate%20zoology"/>
    <skos:related rdf:resource="http://www.usgs.gov/science/USGSThesaurus/arachnids"/>
    <skos:related rdf:resource="http://www.usgs.gov/science/USGSThesaurus/butterflies%20and%20moths"/>
    <skos:related rdf:resource="http://www.usgs.gov/science/USGSThesaurus/insects"/>
    <skos:related rdf:resource="http://www.usgs.gov/science/USGSThesaurus/pollinators"/>
    <skos:inScheme rdf:resource="http://www.usgs.gov/science/USGSThesaurus"/>
  </rdf:Description>
  <rdf:Description about="http://www.usgs.gov/science/USGSThesaurus/vertebrate%20zoology">
    <rdf:type rdf:resource="http://www.w3.org/2004/02/skos/core#Concept"/>
    <skos:prefLabel xml:lang="en">vertebrate zoology</skos:prefLabel>
    <skos:scopeNote xml:lang="en">Branch of zoology that deals with animals that have spinal columns.</skos:scopeNote>
    <skos:broader rdf:resource="http://www.usgs.gov/science/USGSThesaurus/zoology"/>
    <skos:narrower rdf:resource="http://www.usgs.gov/science/USGSThesaurus/herpetology"/>
    <skos:narrower rdf:resource="http://www.usgs.gov/science/USGSThesaurus/ichthyology"/>
    <skos:narrower rdf:resource="http://www.usgs.gov/science/USGSThesaurus/mammalogy"/>
    <skos:narrower rdf:resource="http://www.usgs.gov/science/USGSThesaurus/ornithology"/>
    <skos:related rdf:resource="http://www.usgs.gov/science/USGSThesaurus/game%20species"/>
    <skos:related rdf:resource="http://www.usgs.gov/science/USGSThesaurus/vertebrates"/>
    <skos:inScheme rdf:resource="http://www.usgs.gov/science/USGSThesaurus"/>
  </rdf:Description>
  <rdf:Description about="http://www.usgs.gov/science/USGSThesaurus/herpetology">
    <rdf:type rdf:resource="http://www.w3.org/2004/02/skos/core#Concept"/>
    <skos:prefLabel xml:lang="en">herpetology</skos:prefLabel>
    <skos:scopeNote xml:lang="en">Branch of zoology concerned with the study of reptiles and amphibians.</skos:scopeNote>
    <skos:broader rdf:resource="http://www.usgs.gov/science/USGSThesaurus/vertebrate%20zoology"/>
    <skos:related rdf:resource="http://www.usgs.gov/science/USGSThesaurus/amphibians"/>
    <skos:related rdf:resource="http://www.usgs.gov/science/USGSThesaurus/reptiles"/>
    <skos:inScheme rdf:resource="http://www.usgs.gov/science/USGSThesaurus"/>
  </rdf:Description>
  <rdf:Description about="http://www.usgs.gov/science/USGSThesaurus/ichthyology">
    <rdf:type rdf:resource="http://www.w3.org/2004/02/skos/core#Concept"/>
    <skos:prefLabel xml:lang="en">ichthyology</skos:prefLabel>
    <skos:scopeNote xml:lang="en">Branch of zoology concerned with the study of fish.</skos:scopeNote>
    <skos:broader rdf:resource="http://www.usgs.gov/science/USGSThesaurus/vertebrate%20zoology"/>
    <skos:related rdf:resource="http://www.usgs.gov/science/USGSThesaurus/commercial%20fishery%20resources"/>
    <skos:related rdf:resource="http://www.usgs.gov/science/USGSThesaurus/fish"/>
    <skos:related rdf:resource="http://www.usgs.gov/science/USGSThesaurus/fishery%20resources"/>
    <skos:related rdf:resource="http://www.usgs.gov/science/USGSThesaurus/inland%20fishery%20resources"/>
    <skos:related rdf:resource="http://www.usgs.gov/science/USGSThesaurus/marine%20fishery%20resources"/>
    <skos:related rdf:resource="http://www.usgs.gov/science/USGSThesaurus/overfishing"/>
    <skos:related rdf:resource="http://www.usgs.gov/science/USGSThesaurus/recreational%20fishery%20resources"/>
    <skos:inScheme rdf:resource="http://www.usgs.gov/science/USGSThesaurus"/>
  </rdf:Description>
  <rdf:Description about="http://www.usgs.gov/science/USGSThesaurus/mammalogy">
    <rdf:type rdf:resource="http://www.w3.org/2004/02/skos/core#Concept"/>
    <skos:prefLabel xml:lang="en">mammalogy</skos:prefLabel>
    <skos:scopeNote xml:lang="en">Branch of zoology concerned with the study of mammals.</skos:scopeNote>
    <skos:broader rdf:resource="http://www.usgs.gov/science/USGSThesaurus/vertebrate%20zoology"/>
    <skos:related rdf:resource="http://www.usgs.gov/science/USGSThesaurus/mammals"/>
    <skos:inScheme rdf:resource="http://www.usgs.gov/science/USGSThesaurus"/>
  </rdf:Description>
  <rdf:Description about="http://www.usgs.gov/science/USGSThesaurus/ornithology">
    <rdf:type rdf:resource="http://www.w3.org/2004/02/skos/core#Concept"/>
    <skos:prefLabel xml:lang="en">ornithology</skos:prefLabel>
    <skos:scopeNote xml:lang="en">Branch of biology concerned with the study of birds.</skos:scopeNote>
    <skos:broader rdf:resource="http://www.usgs.gov/science/USGSThesaurus/vertebrate%20zoology"/>
    <skos:related rdf:resource="http://www.usgs.gov/science/USGSThesaurus/birds"/>
    <skos:related rdf:resource="http://www.usgs.gov/science/USGSThesaurus/pollinators"/>
    <skos:inScheme rdf:resource="http://www.usgs.gov/science/USGSThesaurus"/>
  </rdf:Description>
  <rdf:Description about="http://www.usgs.gov/science/USGSThesaurus/wildlife%20biology">
    <rdf:type rdf:resource="http://www.w3.org/2004/02/skos/core#Concept"/>
    <skos:prefLabel xml:lang="en">wildlife biology</skos:prefLabel>
    <skos:scopeNote xml:lang="en">Branch of biology dealing with living organisms, usually mammals, birds, or fishes, that are not domesticated or dependent on man.</skos:scopeNote>
    <skos:broader rdf:resource="http://www.usgs.gov/science/USGSThesaurus/zoology"/>
    <skos:related rdf:resource="http://www.usgs.gov/science/USGSThesaurus/animal%20tracking"/>
    <skos:related rdf:resource="http://www.usgs.gov/science/USGSThesaurus/game%20management"/>
    <skos:related rdf:resource="http://www.usgs.gov/science/USGSThesaurus/game%20species"/>
    <skos:related rdf:resource="http://www.usgs.gov/science/USGSThesaurus/overfishing"/>
    <skos:related rdf:resource="http://www.usgs.gov/science/USGSThesaurus/parasitology"/>
    <skos:related rdf:resource="http://www.usgs.gov/science/USGSThesaurus/vocalization%20methods"/>
    <skos:related rdf:resource="http://www.usgs.gov/science/USGSThesaurus/wildlife"/>
    <skos:related rdf:resource="http://www.usgs.gov/science/USGSThesaurus/wildlife%20population%20management"/>
    <skos:inScheme rdf:resource="http://www.usgs.gov/science/USGSThesaurus"/>
  </rdf:Description>
  <rdf:Description about="http://www.usgs.gov/science/USGSThesaurus/planetary%20sciences">
    <rdf:type rdf:resource="http://www.w3.org/2004/02/skos/core#Concept"/>
    <skos:prefLabel xml:lang="en">planetary sciences</skos:prefLabel>
    <skos:scopeNote xml:lang="en">Scientific study of the solid bodies of the solar system, including planets, moons, asteroids, meteorites, and interplanetary materials.</skos:scopeNote>
    <skos:altLabel xml:lang="en">astronomy</skos:altLabel>
    <skos:altLabel xml:lang="en">planetology</skos:altLabel>
    <skos:broader rdf:resource="http://www.usgs.gov/science/USGSThesaurus/sciences"/>
    <skos:related rdf:resource="http://www.usgs.gov/science/USGSThesaurus/meteorology"/>
    <skos:related rdf:resource="http://www.usgs.gov/science/USGSThesaurus/planetary%20bodies"/>
    <skos:related rdf:resource="http://www.usgs.gov/science/USGSThesaurus/scientific%20careers"/>
    <skos:inScheme rdf:resource="http://www.usgs.gov/science/USGSThesaurus"/>
  </rdf:Description>
  <rdf:Description about="http://www.usgs.gov/science/USGSThesaurus/social%20sciences">
    <rdf:type rdf:resource="http://www.w3.org/2004/02/skos/core#Concept"/>
    <skos:prefLabel xml:lang="en">social sciences</skos:prefLabel>
    <skos:scopeNote xml:lang="en">Sciences concerned with the structure and interrelationships of human societies, human institutions and organizations, and human culture over time.</skos:scopeNote>
    <skos:broader rdf:resource="http://www.usgs.gov/science/USGSThesaurus/sciences"/>
    <skos:narrower rdf:resource="http://www.usgs.gov/science/USGSThesaurus/archeology"/>
    <skos:related rdf:resource="http://www.usgs.gov/science/USGSThesaurus/business%20and%20economics"/>
    <skos:related rdf:resource="http://www.usgs.gov/science/USGSThesaurus/cadastral%20and%20legal%20land%20descriptions"/>
    <skos:related rdf:resource="http://www.usgs.gov/science/USGSThesaurus/culture%20and%20demographics"/>
    <skos:related rdf:resource="http://www.usgs.gov/science/USGSThesaurus/environmental%20health%20%28human%29"/>
    <skos:related rdf:resource="http://www.usgs.gov/science/USGSThesaurus/hazards"/>
    <skos:related rdf:resource="http://www.usgs.gov/science/USGSThesaurus/health%20and%20disease"/>
    <skos:related rdf:resource="http://www.usgs.gov/science/USGSThesaurus/human%20environmental%20safety"/>
    <skos:related rdf:resource="http://www.usgs.gov/science/USGSThesaurus/human%20impacts"/>
    <skos:related rdf:resource="http://www.usgs.gov/science/USGSThesaurus/land%20use%20change"/>
    <skos:related rdf:resource="http://www.usgs.gov/science/USGSThesaurus/mining%20hazards"/>
    <skos:related rdf:resource="http://www.usgs.gov/science/USGSThesaurus/overfishing"/>
    <skos:related rdf:resource="http://www.usgs.gov/science/USGSThesaurus/scientific%20careers"/>
    <skos:related rdf:resource="http://www.usgs.gov/science/USGSThesaurus/waste%20treatment%20and%20disposal"/>
    <skos:inScheme rdf:resource="http://www.usgs.gov/science/USGSThesaurus"/>
  </rdf:Description>
  <rdf:Description about="http://www.usgs.gov/science/USGSThesaurus/archeology">
    <rdf:type rdf:resource="http://www.w3.org/2004/02/skos/core#Concept"/>
    <skos:prefLabel xml:lang="en">archeology</skos:prefLabel>
    <skos:scopeNote xml:lang="en">Study of human cultures through the recovery and analysis of their material relics.</skos:scopeNote>
    <skos:altLabel xml:lang="en">archaeology</skos:altLabel>
    <skos:broader rdf:resource="http://www.usgs.gov/science/USGSThesaurus/social%20sciences"/>
    <skos:inScheme rdf:resource="http://www.usgs.gov/science/USGSThesaurus"/>
  </rdf:Description>
  <rdf:Description about="http://www.usgs.gov/science/USGSThesaurus/time%20periods">
    <rdf:type rdf:resource="http://www.w3.org/2004/02/skos/core#Concept"/>
    <skos:prefLabel xml:lang="en">time periods</skos:prefLabel>
    <skos:scopeNote xml:lang="en">Geologic time periods and seasons of the year</skos:scopeNote>
    <skos:broader rdf:resource="http://www.usgs.gov/science/USGSThesaurus/Categories"/>
    <skos:narrower rdf:resource="http://www.usgs.gov/science/USGSThesaurus/geologic%20time%20periods"/>
    <skos:narrower rdf:resource="http://www.usgs.gov/science/USGSThesaurus/seasons"/>
    <skos:inScheme rdf:resource="http://www.usgs.gov/science/USGSThesaurus"/>
  </rdf:Description>
  <rdf:Description about="http://www.usgs.gov/science/USGSThesaurus/geologic%20time%20periods">
    <rdf:type rdf:resource="http://www.w3.org/2004/02/skos/core#Concept"/>
    <skos:prefLabel xml:lang="en">geologic time periods</skos:prefLabel>
    <skos:scopeNote xml:lang="en"></skos:scopeNote>
    <skos:altLabel xml:lang="en">geologic age</skos:altLabel>
    <skos:altLabel xml:lang="en">geologic time</skos:altLabel>
    <skos:broader rdf:resource="http://www.usgs.gov/science/USGSThesaurus/time%20periods"/>
    <skos:narrower rdf:resource="http://www.usgs.gov/science/USGSThesaurus/Phanerozoic"/>
    <skos:narrower rdf:resource="http://www.usgs.gov/science/USGSThesaurus/Precambrian"/>
    <skos:inScheme rdf:resource="http://www.usgs.gov/science/USGSThesaurus"/>
  </rdf:Description>
  <rdf:Description about="http://www.usgs.gov/science/USGSThesaurus/Phanerozoic">
    <rdf:type rdf:resource="http://www.w3.org/2004/02/skos/core#Concept"/>
    <skos:prefLabel xml:lang="en">Phanerozoic</skos:prefLabel>
    <skos:scopeNote xml:lang="en"></skos:scopeNote>
    <skos:broader rdf:resource="http://www.usgs.gov/science/USGSThesaurus/geologic%20time%20periods"/>
    <skos:narrower rdf:resource="http://www.usgs.gov/science/USGSThesaurus/Cenozoic"/>
    <skos:narrower rdf:resource="http://www.usgs.gov/science/USGSThesaurus/Mesozoic"/>
    <skos:narrower rdf:resource="http://www.usgs.gov/science/USGSThesaurus/Paleozoic"/>
    <skos:inScheme rdf:resource="http://www.usgs.gov/science/USGSThesaurus"/>
  </rdf:Description>
  <rdf:Description about="http://www.usgs.gov/science/USGSThesaurus/Cenozoic">
    <rdf:type rdf:resource="http://www.w3.org/2004/02/skos/core#Concept"/>
    <skos:prefLabel xml:lang="en">Cenozoic</skos:prefLabel>
    <skos:scopeNote xml:lang="en"></skos:scopeNote>
    <skos:broader rdf:resource="http://www.usgs.gov/science/USGSThesaurus/Phanerozoic"/>
    <skos:narrower rdf:resource="http://www.usgs.gov/science/USGSThesaurus/Quaternary"/>
    <skos:narrower rdf:resource="http://www.usgs.gov/science/USGSThesaurus/Tertiary"/>
    <skos:inScheme rdf:resource="http://www.usgs.gov/science/USGSThesaurus"/>
  </rdf:Description>
  <rdf:Description about="http://www.usgs.gov/science/USGSThesaurus/Quaternary">
    <rdf:type rdf:resource="http://www.w3.org/2004/02/skos/core#Concept"/>
    <skos:prefLabel xml:lang="en">Quaternary</skos:prefLabel>
    <skos:scopeNote xml:lang="en"></skos:scopeNote>
    <skos:broader rdf:resource="http://www.usgs.gov/science/USGSThesaurus/Cenozoic"/>
    <skos:narrower rdf:resource="http://www.usgs.gov/science/USGSThesaurus/Holocene"/>
    <skos:narrower rdf:resource="http://www.usgs.gov/science/USGSThesaurus/Pleistocene"/>
    <skos:inScheme rdf:resource="http://www.usgs.gov/science/USGSThesaurus"/>
  </rdf:Description>
  <rdf:Description about="http://www.usgs.gov/science/USGSThesaurus/Holocene">
    <rdf:type rdf:resource="http://www.w3.org/2004/02/skos/core#Concept"/>
    <skos:prefLabel xml:lang="en">Holocene</skos:prefLabel>
    <skos:scopeNote xml:lang="en"></skos:scopeNote>
    <skos:broader rdf:resource="http://www.usgs.gov/science/USGSThesaurus/Quaternary"/>
    <skos:inScheme rdf:resource="http://www.usgs.gov/science/USGSThesaurus"/>
  </rdf:Description>
  <rdf:Description about="http://www.usgs.gov/science/USGSThesaurus/Pleistocene">
    <rdf:type rdf:resource="http://www.w3.org/2004/02/skos/core#Concept"/>
    <skos:prefLabel xml:lang="en">Pleistocene</skos:prefLabel>
    <skos:scopeNote xml:lang="en"></skos:scopeNote>
    <skos:altLabel xml:lang="en">ice age</skos:altLabel>
    <skos:broader rdf:resource="http://www.usgs.gov/science/USGSThesaurus/Quaternary"/>
    <skos:inScheme rdf:resource="http://www.usgs.gov/science/USGSThesaurus"/>
  </rdf:Description>
  <rdf:Description about="http://www.usgs.gov/science/USGSThesaurus/Tertiary">
    <rdf:type rdf:resource="http://www.w3.org/2004/02/skos/core#Concept"/>
    <skos:prefLabel xml:lang="en">Tertiary</skos:prefLabel>
    <skos:scopeNote xml:lang="en"></skos:scopeNote>
    <skos:broader rdf:resource="http://www.usgs.gov/science/USGSThesaurus/Cenozoic"/>
    <skos:narrower rdf:resource="http://www.usgs.gov/science/USGSThesaurus/Neogene"/>
    <skos:narrower rdf:resource="http://www.usgs.gov/science/USGSThesaurus/Paleogene"/>
    <skos:inScheme rdf:resource="http://www.usgs.gov/science/USGSThesaurus"/>
  </rdf:Description>
  <rdf:Description about="http://www.usgs.gov/science/USGSThesaurus/Neogene">
    <rdf:type rdf:resource="http://www.w3.org/2004/02/skos/core#Concept"/>
    <skos:prefLabel xml:lang="en">Neogene</skos:prefLabel>
    <skos:scopeNote xml:lang="en"></skos:scopeNote>
    <skos:broader rdf:resource="http://www.usgs.gov/science/USGSThesaurus/Tertiary"/>
    <skos:narrower rdf:resource="http://www.usgs.gov/science/USGSThesaurus/Miocene"/>
    <skos:narrower rdf:resource="http://www.usgs.gov/science/USGSThesaurus/Pliocene"/>
    <skos:inScheme rdf:resource="http://www.usgs.gov/science/USGSThesaurus"/>
  </rdf:Description>
  <rdf:Description about="http://www.usgs.gov/science/USGSThesaurus/Miocene">
    <rdf:type rdf:resource="http://www.w3.org/2004/02/skos/core#Concept"/>
    <skos:prefLabel xml:lang="en">Miocene</skos:prefLabel>
    <skos:scopeNote xml:lang="en"></skos:scopeNote>
    <skos:broader rdf:resource="http://www.usgs.gov/science/USGSThesaurus/Neogene"/>
    <skos:inScheme rdf:resource="http://www.usgs.gov/science/USGSThesaurus"/>
  </rdf:Description>
  <rdf:Description about="http://www.usgs.gov/science/USGSThesaurus/Pliocene">
    <rdf:type rdf:resource="http://www.w3.org/2004/02/skos/core#Concept"/>
    <skos:prefLabel xml:lang="en">Pliocene</skos:prefLabel>
    <skos:scopeNote xml:lang="en"></skos:scopeNote>
    <skos:broader rdf:resource="http://www.usgs.gov/science/USGSThesaurus/Neogene"/>
    <skos:inScheme rdf:resource="http://www.usgs.gov/science/USGSThesaurus"/>
  </rdf:Description>
  <rdf:Description about="http://www.usgs.gov/science/USGSThesaurus/Paleogene">
    <rdf:type rdf:resource="http://www.w3.org/2004/02/skos/core#Concept"/>
    <skos:prefLabel xml:lang="en">Paleogene</skos:prefLabel>
    <skos:scopeNote xml:lang="en"></skos:scopeNote>
    <skos:broader rdf:resource="http://www.usgs.gov/science/USGSThesaurus/Tertiary"/>
    <skos:narrower rdf:resource="http://www.usgs.gov/science/USGSThesaurus/Eocene"/>
    <skos:narrower rdf:resource="http://www.usgs.gov/science/USGSThesaurus/Oligocene"/>
    <skos:narrower rdf:resource="http://www.usgs.gov/science/USGSThesaurus/Paleocene"/>
    <skos:inScheme rdf:resource="http://www.usgs.gov/science/USGSThesaurus"/>
  </rdf:Description>
  <rdf:Description about="http://www.usgs.gov/science/USGSThesaurus/Eocene">
    <rdf:type rdf:resource="http://www.w3.org/2004/02/skos/core#Concept"/>
    <skos:prefLabel xml:lang="en">Eocene</skos:prefLabel>
    <skos:scopeNote xml:lang="en"></skos:scopeNote>
    <skos:broader rdf:resource="http://www.usgs.gov/science/USGSThesaurus/Paleogene"/>
    <skos:inScheme rdf:resource="http://www.usgs.gov/science/USGSThesaurus"/>
  </rdf:Description>
  <rdf:Description about="http://www.usgs.gov/science/USGSThesaurus/Oligocene">
    <rdf:type rdf:resource="http://www.w3.org/2004/02/skos/core#Concept"/>
    <skos:prefLabel xml:lang="en">Oligocene</skos:prefLabel>
    <skos:scopeNote xml:lang="en"></skos:scopeNote>
    <skos:broader rdf:resource="http://www.usgs.gov/science/USGSThesaurus/Paleogene"/>
    <skos:inScheme rdf:resource="http://www.usgs.gov/science/USGSThesaurus"/>
  </rdf:Description>
  <rdf:Description about="http://www.usgs.gov/science/USGSThesaurus/Paleocene">
    <rdf:type rdf:resource="http://www.w3.org/2004/02/skos/core#Concept"/>
    <skos:prefLabel xml:lang="en">Paleocene</skos:prefLabel>
    <skos:scopeNote xml:lang="en"></skos:scopeNote>
    <skos:broader rdf:resource="http://www.usgs.gov/science/USGSThesaurus/Paleogene"/>
    <skos:inScheme rdf:resource="http://www.usgs.gov/science/USGSThesaurus"/>
  </rdf:Description>
  <rdf:Description about="http://www.usgs.gov/science/USGSThesaurus/Mesozoic">
    <rdf:type rdf:resource="http://www.w3.org/2004/02/skos/core#Concept"/>
    <skos:prefLabel xml:lang="en">Mesozoic</skos:prefLabel>
    <skos:scopeNote xml:lang="en"></skos:scopeNote>
    <skos:broader rdf:resource="http://www.usgs.gov/science/USGSThesaurus/Phanerozoic"/>
    <skos:narrower rdf:resource="http://www.usgs.gov/science/USGSThesaurus/Cretaceous"/>
    <skos:narrower rdf:resource="http://www.usgs.gov/science/USGSThesaurus/Jurassic"/>
    <skos:narrower rdf:resource="http://www.usgs.gov/science/USGSThesaurus/Triassic"/>
    <skos:inScheme rdf:resource="http://www.usgs.gov/science/USGSThesaurus"/>
  </rdf:Description>
  <rdf:Description about="http://www.usgs.gov/science/USGSThesaurus/Cretaceous">
    <rdf:type rdf:resource="http://www.w3.org/2004/02/skos/core#Concept"/>
    <skos:prefLabel xml:lang="en">Cretaceous</skos:prefLabel>
    <skos:scopeNote xml:lang="en"></skos:scopeNote>
    <skos:broader rdf:resource="http://www.usgs.gov/science/USGSThesaurus/Mesozoic"/>
    <skos:inScheme rdf:resource="http://www.usgs.gov/science/USGSThesaurus"/>
  </rdf:Description>
  <rdf:Description about="http://www.usgs.gov/science/USGSThesaurus/Jurassic">
    <rdf:type rdf:resource="http://www.w3.org/2004/02/skos/core#Concept"/>
    <skos:prefLabel xml:lang="en">Jurassic</skos:prefLabel>
    <skos:scopeNote xml:lang="en"></skos:scopeNote>
    <skos:broader rdf:resource="http://www.usgs.gov/science/USGSThesaurus/Mesozoic"/>
    <skos:inScheme rdf:resource="http://www.usgs.gov/science/USGSThesaurus"/>
  </rdf:Description>
  <rdf:Description about="http://www.usgs.gov/science/USGSThesaurus/Triassic">
    <rdf:type rdf:resource="http://www.w3.org/2004/02/skos/core#Concept"/>
    <skos:prefLabel xml:lang="en">Triassic</skos:prefLabel>
    <skos:scopeNote xml:lang="en"></skos:scopeNote>
    <skos:broader rdf:resource="http://www.usgs.gov/science/USGSThesaurus/Mesozoic"/>
    <skos:inScheme rdf:resource="http://www.usgs.gov/science/USGSThesaurus"/>
  </rdf:Description>
  <rdf:Description about="http://www.usgs.gov/science/USGSThesaurus/Paleozoic">
    <rdf:type rdf:resource="http://www.w3.org/2004/02/skos/core#Concept"/>
    <skos:prefLabel xml:lang="en">Paleozoic</skos:prefLabel>
    <skos:scopeNote xml:lang="en"></skos:scopeNote>
    <skos:broader rdf:resource="http://www.usgs.gov/science/USGSThesaurus/Phanerozoic"/>
    <skos:narrower rdf:resource="http://www.usgs.gov/science/USGSThesaurus/Cambrian"/>
    <skos:narrower rdf:resource="http://www.usgs.gov/science/USGSThesaurus/Devonian"/>
    <skos:narrower rdf:resource="http://www.usgs.gov/science/USGSThesaurus/Mississippian"/>
    <skos:narrower rdf:resource="http://www.usgs.gov/science/USGSThesaurus/Ordovician"/>
    <skos:narrower rdf:resource="http://www.usgs.gov/science/USGSThesaurus/Pennsylvanian"/>
    <skos:narrower rdf:resource="http://www.usgs.gov/science/USGSThesaurus/Permian"/>
    <skos:narrower rdf:resource="http://www.usgs.gov/science/USGSThesaurus/Silurian"/>
    <skos:inScheme rdf:resource="http://www.usgs.gov/science/USGSThesaurus"/>
  </rdf:Description>
  <rdf:Description about="http://www.usgs.gov/science/USGSThesaurus/Cambrian">
    <rdf:type rdf:resource="http://www.w3.org/2004/02/skos/core#Concept"/>
    <skos:prefLabel xml:lang="en">Cambrian</skos:prefLabel>
    <skos:scopeNote xml:lang="en"></skos:scopeNote>
    <skos:broader rdf:resource="http://www.usgs.gov/science/USGSThesaurus/Paleozoic"/>
    <skos:inScheme rdf:resource="http://www.usgs.gov/science/USGSThesaurus"/>
  </rdf:Description>
  <rdf:Description about="http://www.usgs.gov/science/USGSThesaurus/Devonian">
    <rdf:type rdf:resource="http://www.w3.org/2004/02/skos/core#Concept"/>
    <skos:prefLabel xml:lang="en">Devonian</skos:prefLabel>
    <skos:scopeNote xml:lang="en"></skos:scopeNote>
    <skos:broader rdf:resource="http://www.usgs.gov/science/USGSThesaurus/Paleozoic"/>
    <skos:inScheme rdf:resource="http://www.usgs.gov/science/USGSThesaurus"/>
  </rdf:Description>
  <rdf:Description about="http://www.usgs.gov/science/USGSThesaurus/Mississippian">
    <rdf:type rdf:resource="http://www.w3.org/2004/02/skos/core#Concept"/>
    <skos:prefLabel xml:lang="en">Mississippian</skos:prefLabel>
    <skos:scopeNote xml:lang="en"></skos:scopeNote>
    <skos:altLabel xml:lang="en">lower carboniferous</skos:altLabel>
    <skos:broader rdf:resource="http://www.usgs.gov/science/USGSThesaurus/Paleozoic"/>
    <skos:inScheme rdf:resource="http://www.usgs.gov/science/USGSThesaurus"/>
  </rdf:Description>
  <rdf:Description about="http://www.usgs.gov/science/USGSThesaurus/Ordovician">
    <rdf:type rdf:resource="http://www.w3.org/2004/02/skos/core#Concept"/>
    <skos:prefLabel xml:lang="en">Ordovician</skos:prefLabel>
    <skos:scopeNote xml:lang="en"></skos:scopeNote>
    <skos:broader rdf:resource="http://www.usgs.gov/science/USGSThesaurus/Paleozoic"/>
    <skos:inScheme rdf:resource="http://www.usgs.gov/science/USGSThesaurus"/>
  </rdf:Description>
  <rdf:Description about="http://www.usgs.gov/science/USGSThesaurus/Pennsylvanian">
    <rdf:type rdf:resource="http://www.w3.org/2004/02/skos/core#Concept"/>
    <skos:prefLabel xml:lang="en">Pennsylvanian</skos:prefLabel>
    <skos:scopeNote xml:lang="en"></skos:scopeNote>
    <skos:altLabel xml:lang="en">upper carboniferous</skos:altLabel>
    <skos:broader rdf:resource="http://www.usgs.gov/science/USGSThesaurus/Paleozoic"/>
    <skos:inScheme rdf:resource="http://www.usgs.gov/science/USGSThesaurus"/>
  </rdf:Description>
  <rdf:Description about="http://www.usgs.gov/science/USGSThesaurus/Permian">
    <rdf:type rdf:resource="http://www.w3.org/2004/02/skos/core#Concept"/>
    <skos:prefLabel xml:lang="en">Permian</skos:prefLabel>
    <skos:scopeNote xml:lang="en"></skos:scopeNote>
    <skos:broader rdf:resource="http://www.usgs.gov/science/USGSThesaurus/Paleozoic"/>
    <skos:inScheme rdf:resource="http://www.usgs.gov/science/USGSThesaurus"/>
  </rdf:Description>
  <rdf:Description about="http://www.usgs.gov/science/USGSThesaurus/Silurian">
    <rdf:type rdf:resource="http://www.w3.org/2004/02/skos/core#Concept"/>
    <skos:prefLabel xml:lang="en">Silurian</skos:prefLabel>
    <skos:scopeNote xml:lang="en"></skos:scopeNote>
    <skos:broader rdf:resource="http://www.usgs.gov/science/USGSThesaurus/Paleozoic"/>
    <skos:inScheme rdf:resource="http://www.usgs.gov/science/USGSThesaurus"/>
  </rdf:Description>
  <rdf:Description about="http://www.usgs.gov/science/USGSThesaurus/Precambrian">
    <rdf:type rdf:resource="http://www.w3.org/2004/02/skos/core#Concept"/>
    <skos:prefLabel xml:lang="en">Precambrian</skos:prefLabel>
    <skos:scopeNote xml:lang="en"></skos:scopeNote>
    <skos:altLabel xml:lang="en">cryptozoic</skos:altLabel>
    <skos:broader rdf:resource="http://www.usgs.gov/science/USGSThesaurus/geologic%20time%20periods"/>
    <skos:narrower rdf:resource="http://www.usgs.gov/science/USGSThesaurus/Archaean"/>
    <skos:narrower rdf:resource="http://www.usgs.gov/science/USGSThesaurus/Hadean"/>
    <skos:narrower rdf:resource="http://www.usgs.gov/science/USGSThesaurus/Proterozoic"/>
    <skos:inScheme rdf:resource="http://www.usgs.gov/science/USGSThesaurus"/>
  </rdf:Description>
  <rdf:Description about="http://www.usgs.gov/science/USGSThesaurus/Archaean">
    <rdf:type rdf:resource="http://www.w3.org/2004/02/skos/core#Concept"/>
    <skos:prefLabel xml:lang="en">Archaean</skos:prefLabel>
    <skos:scopeNote xml:lang="en"></skos:scopeNote>
    <skos:broader rdf:resource="http://www.usgs.gov/science/USGSThesaurus/Precambrian"/>
    <skos:inScheme rdf:resource="http://www.usgs.gov/science/USGSThesaurus"/>
  </rdf:Description>
  <rdf:Description about="http://www.usgs.gov/science/USGSThesaurus/Hadean">
    <rdf:type rdf:resource="http://www.w3.org/2004/02/skos/core#Concept"/>
    <skos:prefLabel xml:lang="en">Hadean</skos:prefLabel>
    <skos:scopeNote xml:lang="en"></skos:scopeNote>
    <skos:broader rdf:resource="http://www.usgs.gov/science/USGSThesaurus/Precambrian"/>
    <skos:inScheme rdf:resource="http://www.usgs.gov/science/USGSThesaurus"/>
  </rdf:Description>
  <rdf:Description about="http://www.usgs.gov/science/USGSThesaurus/Proterozoic">
    <rdf:type rdf:resource="http://www.w3.org/2004/02/skos/core#Concept"/>
    <skos:prefLabel xml:lang="en">Proterozoic</skos:prefLabel>
    <skos:scopeNote xml:lang="en"></skos:scopeNote>
    <skos:broader rdf:resource="http://www.usgs.gov/science/USGSThesaurus/Precambrian"/>
    <skos:narrower rdf:resource="http://www.usgs.gov/science/USGSThesaurus/Neoproterozoic"/>
    <skos:inScheme rdf:resource="http://www.usgs.gov/science/USGSThesaurus"/>
  </rdf:Description>
  <rdf:Description about="http://www.usgs.gov/science/USGSThesaurus/Neoproterozoic">
    <rdf:type rdf:resource="http://www.w3.org/2004/02/skos/core#Concept"/>
    <skos:prefLabel xml:lang="en">Neoproterozoic</skos:prefLabel>
    <skos:scopeNote xml:lang="en">The latest geologic era of the Proterozoic Eon.</skos:scopeNote>
    <skos:broader rdf:resource="http://www.usgs.gov/science/USGSThesaurus/Proterozoic"/>
    <skos:narrower rdf:resource="http://www.usgs.gov/science/USGSThesaurus/Ediacaran"/>
    <skos:inScheme rdf:resource="http://www.usgs.gov/science/USGSThesaurus"/>
  </rdf:Description>
  <rdf:Description about="http://www.usgs.gov/science/USGSThesaurus/Ediacaran">
    <rdf:type rdf:resource="http://www.w3.org/2004/02/skos/core#Concept"/>
    <skos:prefLabel xml:lang="en">Ediacaran</skos:prefLabel>
    <skos:scopeNote xml:lang="en">The last geological period of the Neoproterozoic Era, just before the Cambrian Period of the Paleozoic Era.</skos:scopeNote>
    <skos:altLabel xml:lang="en">Vendian</skos:altLabel>
    <skos:broader rdf:resource="http://www.usgs.gov/science/USGSThesaurus/Neoproterozoic"/>
    <skos:inScheme rdf:resource="http://www.usgs.gov/science/USGSThesaurus"/>
  </rdf:Description>
  <rdf:Description about="http://www.usgs.gov/science/USGSThesaurus/seasons">
    <rdf:type rdf:resource="http://www.w3.org/2004/02/skos/core#Concept"/>
    <skos:prefLabel xml:lang="en">seasons</skos:prefLabel>
    <skos:scopeNote xml:lang="en"></skos:scopeNote>
    <skos:broader rdf:resource="http://www.usgs.gov/science/USGSThesaurus/time%20periods"/>
    <skos:narrower rdf:resource="http://www.usgs.gov/science/USGSThesaurus/autumn"/>
    <skos:narrower rdf:resource="http://www.usgs.gov/science/USGSThesaurus/spring%20%28season%29"/>
    <skos:narrower rdf:resource="http://www.usgs.gov/science/USGSThesaurus/summer"/>
    <skos:narrower rdf:resource="http://www.usgs.gov/science/USGSThesaurus/winter"/>
    <skos:inScheme rdf:resource="http://www.usgs.gov/science/USGSThesaurus"/>
  </rdf:Description>
  <rdf:Description about="http://www.usgs.gov/science/USGSThesaurus/autumn">
    <rdf:type rdf:resource="http://www.w3.org/2004/02/skos/core#Concept"/>
    <skos:prefLabel xml:lang="en">autumn</skos:prefLabel>
    <skos:scopeNote xml:lang="en"></skos:scopeNote>
    <skos:altLabel xml:lang="en">fall (season)</skos:altLabel>
    <skos:broader rdf:resource="http://www.usgs.gov/science/USGSThesaurus/seasons"/>
    <skos:inScheme rdf:resource="http://www.usgs.gov/science/USGSThesaurus"/>
  </rdf:Description>
  <rdf:Description about="http://www.usgs.gov/science/USGSThesaurus/spring%20%28season%29">
    <rdf:type rdf:resource="http://www.w3.org/2004/02/skos/core#Concept"/>
    <skos:prefLabel xml:lang="en">spring (season)</skos:prefLabel>
    <skos:scopeNote xml:lang="en"></skos:scopeNote>
    <skos:broader rdf:resource="http://www.usgs.gov/science/USGSThesaurus/seasons"/>
    <skos:inScheme rdf:resource="http://www.usgs.gov/science/USGSThesaurus"/>
  </rdf:Description>
  <rdf:Description about="http://www.usgs.gov/science/USGSThesaurus/summer">
    <rdf:type rdf:resource="http://www.w3.org/2004/02/skos/core#Concept"/>
    <skos:prefLabel xml:lang="en">summer</skos:prefLabel>
    <skos:scopeNote xml:lang="en"></skos:scopeNote>
    <skos:broader rdf:resource="http://www.usgs.gov/science/USGSThesaurus/seasons"/>
    <skos:inScheme rdf:resource="http://www.usgs.gov/science/USGSThesaurus"/>
  </rdf:Description>
  <rdf:Description about="http://www.usgs.gov/science/USGSThesaurus/winter">
    <rdf:type rdf:resource="http://www.w3.org/2004/02/skos/core#Concept"/>
    <skos:prefLabel xml:lang="en">winter</skos:prefLabel>
    <skos:scopeNote xml:lang="en"></skos:scopeNote>
    <skos:broader rdf:resource="http://www.usgs.gov/science/USGSThesaurus/seasons"/>
    <skos:inScheme rdf:resource="http://www.usgs.gov/science/USGSThesaurus"/>
  </rdf:Description>
  <rdf:Description about="http://www.usgs.gov/science/USGSThesaurus/topics">
    <rdf:type rdf:resource="http://www.w3.org/2004/02/skos/core#Concept"/>
    <skos:prefLabel xml:lang="en">topics</skos:prefLabel>
    <skos:scopeNote xml:lang="en">Themes, subjects, and concerns for which USGS information resources are relevant.</skos:scopeNote>
    <skos:broader rdf:resource="http://www.usgs.gov/science/USGSThesaurus/Categories"/>
    <skos:narrower rdf:resource="http://www.usgs.gov/science/USGSThesaurus/agriculture"/>
    <skos:narrower rdf:resource="http://www.usgs.gov/science/USGSThesaurus/biological%20and%20physical%20processes"/>
    <skos:narrower rdf:resource="http://www.usgs.gov/science/USGSThesaurus/contamination%20and%20pollution"/>
    <skos:narrower rdf:resource="http://www.usgs.gov/science/USGSThesaurus/culture%20and%20demographics"/>
    <skos:narrower rdf:resource="http://www.usgs.gov/science/USGSThesaurus/earth%20characteristics"/>
    <skos:narrower rdf:resource="http://www.usgs.gov/science/USGSThesaurus/effects%20of%20climate%20change"/>
    <skos:narrower rdf:resource="http://www.usgs.gov/science/USGSThesaurus/elements"/>
    <skos:narrower rdf:resource="http://www.usgs.gov/science/USGSThesaurus/field%20monitoring%20stations"/>
    <skos:narrower rdf:resource="http://www.usgs.gov/science/USGSThesaurus/hazards"/>
    <skos:narrower rdf:resource="http://www.usgs.gov/science/USGSThesaurus/health%20and%20disease"/>
    <skos:narrower rdf:resource="http://www.usgs.gov/science/USGSThesaurus/human%20impacts"/>
    <skos:narrower rdf:resource="http://www.usgs.gov/science/USGSThesaurus/information%20system%20design%20and%20development"/>
    <skos:narrower rdf:resource="http://www.usgs.gov/science/USGSThesaurus/instrument%20design%20and%20development"/>
    <skos:narrower rdf:resource="http://www.usgs.gov/science/USGSThesaurus/land%20use%20and%20land%20cover"/>
    <skos:narrower rdf:resource="http://www.usgs.gov/science/USGSThesaurus/map%20coordinate%20systems"/>
    <skos:narrower rdf:resource="http://www.usgs.gov/science/USGSThesaurus/natural%20resource%20exploration"/>
    <skos:narrower rdf:resource="http://www.usgs.gov/science/USGSThesaurus/natural%20resource%20extraction"/>
    <skos:narrower rdf:resource="http://www.usgs.gov/science/USGSThesaurus/natural%20resources"/>
    <skos:narrower rdf:resource="http://www.usgs.gov/science/USGSThesaurus/organism%20groupings%20%28non-taxonomic%29"/>
    <skos:narrower rdf:resource="http://www.usgs.gov/science/USGSThesaurus/organisms"/>
    <skos:narrower rdf:resource="http://www.usgs.gov/science/USGSThesaurus/planetary%20bodies"/>
    <skos:narrower rdf:resource="http://www.usgs.gov/science/USGSThesaurus/population%20and%20community%20ecology"/>
    <skos:narrower rdf:resource="http://www.usgs.gov/science/USGSThesaurus/recreation"/>
    <skos:narrower rdf:resource="http://www.usgs.gov/science/USGSThesaurus/scientific%20careers"/>
    <skos:narrower rdf:resource="http://www.usgs.gov/science/USGSThesaurus/water%20properties"/>
    <skos:narrower rdf:resource="http://www.usgs.gov/science/USGSThesaurus/water%20quality"/>
    <skos:narrower rdf:resource="http://www.usgs.gov/science/USGSThesaurus/water%20supply%20and%20demand"/>
    <skos:inScheme rdf:resource="http://www.usgs.gov/science/USGSThesaurus"/>
  </rdf:Description>
  <rdf:Description about="http://www.usgs.gov/science/USGSThesaurus/agriculture">
    <rdf:type rdf:resource="http://www.w3.org/2004/02/skos/core#Concept"/>
    <skos:prefLabel xml:lang="en">agriculture</skos:prefLabel>
    <skos:scopeNote xml:lang="en">The science and business of soil cultivation to raise crops and of animal husbandry to raise domesticated animals.</skos:scopeNote>
    <skos:altLabel xml:lang="en">farming</skos:altLabel>
    <skos:altLabel xml:lang="en">horticulture</skos:altLabel>
    <skos:altLabel xml:lang="en">livestock husbandry</skos:altLabel>
    <skos:broader rdf:resource="http://www.usgs.gov/science/USGSThesaurus/topics"/>
    <skos:narrower rdf:resource="http://www.usgs.gov/science/USGSThesaurus/aquaculture"/>
    <skos:related rdf:resource="http://www.usgs.gov/science/USGSThesaurus/soil%20chemistry"/>
    <skos:inScheme rdf:resource="http://www.usgs.gov/science/USGSThesaurus"/>
  </rdf:Description>
  <rdf:Description about="http://www.usgs.gov/science/USGSThesaurus/aquaculture">
    <rdf:type rdf:resource="http://www.w3.org/2004/02/skos/core#Concept"/>
    <skos:prefLabel xml:lang="en">aquaculture</skos:prefLabel>
    <skos:scopeNote xml:lang="en">The farming of organisms that live in water, such as fish, shellfish, and algae for human use.</skos:scopeNote>
    <skos:altLabel xml:lang="en">fish farming</skos:altLabel>
    <skos:broader rdf:resource="http://www.usgs.gov/science/USGSThesaurus/agriculture"/>
    <skos:related rdf:resource="http://www.usgs.gov/science/USGSThesaurus/commercial%20fishery%20resources"/>
    <skos:related rdf:resource="http://www.usgs.gov/science/USGSThesaurus/fishery%20resources"/>
    <skos:inScheme rdf:resource="http://www.usgs.gov/science/USGSThesaurus"/>
  </rdf:Description>
  <rdf:Description about="http://www.usgs.gov/science/USGSThesaurus/biological%20and%20physical%20processes">
    <rdf:type rdf:resource="http://www.w3.org/2004/02/skos/core#Concept"/>
    <skos:prefLabel xml:lang="en">biological and physical processes</skos:prefLabel>
    <skos:scopeNote xml:lang="en">All continuing activities, functions, and phenomena associated with organisms and non-living matter.</skos:scopeNote>
    <skos:altLabel xml:lang="en">bioenergetic processes</skos:altLabel>
    <skos:broader rdf:resource="http://www.usgs.gov/science/USGSThesaurus/topics"/>
    <skos:narrower rdf:resource="http://www.usgs.gov/science/USGSThesaurus/atmospheric%20and%20climatic%20processes"/>
    <skos:narrower rdf:resource="http://www.usgs.gov/science/USGSThesaurus/coastal%20processes"/>
    <skos:narrower rdf:resource="http://www.usgs.gov/science/USGSThesaurus/ecological%20processes"/>
    <skos:narrower rdf:resource="http://www.usgs.gov/science/USGSThesaurus/estuarine%20processes"/>
    <skos:narrower rdf:resource="http://www.usgs.gov/science/USGSThesaurus/evolution"/>
    <skos:narrower rdf:resource="http://www.usgs.gov/science/USGSThesaurus/fires"/>
    <skos:narrower rdf:resource="http://www.usgs.gov/science/USGSThesaurus/geochemical%20processes"/>
    <skos:narrower rdf:resource="http://www.usgs.gov/science/USGSThesaurus/geologic%20processes"/>
    <skos:narrower rdf:resource="http://www.usgs.gov/science/USGSThesaurus/hydrologic%20processes"/>
    <skos:narrower rdf:resource="http://www.usgs.gov/science/USGSThesaurus/impact%20cratering"/>
    <skos:narrower rdf:resource="http://www.usgs.gov/science/USGSThesaurus/ocean%20processes"/>
    <skos:narrower rdf:resource="http://www.usgs.gov/science/USGSThesaurus/physiological%20processes"/>
    <skos:inScheme rdf:resource="http://www.usgs.gov/science/USGSThesaurus"/>
  </rdf:Description>
  <rdf:Description about="http://www.usgs.gov/science/USGSThesaurus/atmospheric%20and%20climatic%20processes">
    <rdf:type rdf:resource="http://www.w3.org/2004/02/skos/core#Concept"/>
    <skos:prefLabel xml:lang="en">atmospheric and climatic processes</skos:prefLabel>
    <skos:scopeNote xml:lang="en">Phenomena affecting or occurring within the mass of gases that surrounds the earth, including its physics, chemistry, dynamics, and weather conditions.</skos:scopeNote>
    <skos:altLabel xml:lang="en">climate</skos:altLabel>
    <!--FOR weather monitoring USE atmospheric and climatic processes WITH field inventory and monitoring-->
    <skos:altLabel xml:lang="en">weather monitoring</skos:altLabel>
    <!--FOR weather observations USE atmospheric and climatic processes WITH field inventory and monitoring-->
    <skos:altLabel xml:lang="en">weather observations</skos:altLabel>
    <skos:altLabel xml:lang="en">weather</skos:altLabel>
    <skos:altLabel xml:lang="en">microclimate</skos:altLabel>
    <skos:broader rdf:resource="http://www.usgs.gov/science/USGSThesaurus/biological%20and%20physical%20processes"/>
    <skos:narrower rdf:resource="http://www.usgs.gov/science/USGSThesaurus/atmospheric%20circulation"/>
    <skos:narrower rdf:resource="http://www.usgs.gov/science/USGSThesaurus/atmospheric%20deposition%20%28chemical%20%26%20particulate%29"/>
    <skos:narrower rdf:resource="http://www.usgs.gov/science/USGSThesaurus/climate%20change"/>
    <skos:narrower rdf:resource="http://www.usgs.gov/science/USGSThesaurus/droughts"/>
    <skos:narrower rdf:resource="http://www.usgs.gov/science/USGSThesaurus/evaporation"/>
    <skos:narrower rdf:resource="http://www.usgs.gov/science/USGSThesaurus/greenhouse%20effect"/>
    <skos:narrower rdf:resource="http://www.usgs.gov/science/USGSThesaurus/ocean-atmosphere%20interaction"/>
    <skos:narrower rdf:resource="http://www.usgs.gov/science/USGSThesaurus/precipitation%20%28atmospheric%29"/>
    <skos:narrower rdf:resource="http://www.usgs.gov/science/USGSThesaurus/storms"/>
    <skos:narrower rdf:resource="http://www.usgs.gov/science/USGSThesaurus/wind"/>
    <skos:related rdf:resource="http://www.usgs.gov/science/USGSThesaurus/atmospheric%20properties"/>
    <skos:related rdf:resource="http://www.usgs.gov/science/USGSThesaurus/atmospheric%20sciences"/>
    <skos:related rdf:resource="http://www.usgs.gov/science/USGSThesaurus/meteorology"/>
    <skos:related rdf:resource="http://www.usgs.gov/science/USGSThesaurus/snow%20and%20ice%20cover"/>
    <skos:inScheme rdf:resource="http://www.usgs.gov/science/USGSThesaurus"/>
  </rdf:Description>
  <rdf:Description about="http://www.usgs.gov/science/USGSThesaurus/atmospheric%20circulation">
    <rdf:type rdf:resource="http://www.w3.org/2004/02/skos/core#Concept"/>
    <skos:prefLabel xml:lang="en">atmospheric circulation</skos:prefLabel>
    <skos:scopeNote xml:lang="en">Movement of atmospheric gases around the earth.</skos:scopeNote>
    <skos:broader rdf:resource="http://www.usgs.gov/science/USGSThesaurus/atmospheric%20and%20climatic%20processes"/>
    <skos:related rdf:resource="http://www.usgs.gov/science/USGSThesaurus/atmospheric%20sciences"/>
    <skos:related rdf:resource="http://www.usgs.gov/science/USGSThesaurus/water%20circulation"/>
    <skos:inScheme rdf:resource="http://www.usgs.gov/science/USGSThesaurus"/>
  </rdf:Description>
  <rdf:Description about="http://www.usgs.gov/science/USGSThesaurus/atmospheric%20deposition%20%28chemical%20%26%20particulate%29">
    <rdf:type rdf:resource="http://www.w3.org/2004/02/skos/core#Concept"/>
    <skos:prefLabel xml:lang="en">atmospheric deposition (chemical &amp; particulate)</skos:prefLabel>
    <skos:scopeNote xml:lang="en">The transfer of substances from the air to the surface of the earth, either in wet form (rain, fog, snow, dew, frost, hail) or in dry form (gases, aerosols, particles).</skos:scopeNote>
    <skos:altLabel xml:lang="en">atmospheric dust deposition</skos:altLabel>
    <skos:altLabel xml:lang="en">atmospheric deposition (chemical and particulate)</skos:altLabel>
    <skos:broader rdf:resource="http://www.usgs.gov/science/USGSThesaurus/atmospheric%20and%20climatic%20processes"/>
    <skos:narrower rdf:resource="http://www.usgs.gov/science/USGSThesaurus/acid%20deposition"/>
    <skos:related rdf:resource="http://www.usgs.gov/science/USGSThesaurus/atmospheric%20sciences"/>
    <skos:related rdf:resource="http://www.usgs.gov/science/USGSThesaurus/precipitation%20%28atmospheric%29"/>
    <skos:related rdf:resource="http://www.usgs.gov/science/USGSThesaurus/sedimentation"/>
    <skos:inScheme rdf:resource="http://www.usgs.gov/science/USGSThesaurus"/>
  </rdf:Description>
  <rdf:Description about="http://www.usgs.gov/science/USGSThesaurus/acid%20deposition">
    <rdf:type rdf:resource="http://www.w3.org/2004/02/skos/core#Concept"/>
    <skos:prefLabel xml:lang="en">acid deposition</skos:prefLabel>
    <skos:scopeNote xml:lang="en">The process by which emissions, chiefly sulfur and nitrogen compounds, either react with the atmosphere when deposited on earth by precipitation of snow, rain, or fog with a pH of 5.5 or below, or settle out as acidic particles or gases.</skos:scopeNote>
    <skos:altLabel xml:lang="en">acid precipitation</skos:altLabel>
    <skos:altLabel xml:lang="en">acid rain</skos:altLabel>
    <skos:altLabel xml:lang="en">acid snow</skos:altLabel>
    <skos:altLabel xml:lang="en">acidic deposition</skos:altLabel>
    <skos:broader rdf:resource="http://www.usgs.gov/science/USGSThesaurus/atmospheric%20deposition%20%28chemical%20%26%20particulate%29"/>
    <skos:related rdf:resource="http://www.usgs.gov/science/USGSThesaurus/atmospheric%20sciences"/>
    <skos:related rdf:resource="http://www.usgs.gov/science/USGSThesaurus/human%20impacts"/>
    <skos:inScheme rdf:resource="http://www.usgs.gov/science/USGSThesaurus"/>
  </rdf:Description>
  <rdf:Description about="http://www.usgs.gov/science/USGSThesaurus/climate%20change">
    <rdf:type rdf:resource="http://www.w3.org/2004/02/skos/core#Concept"/>
    <skos:prefLabel xml:lang="en">climate change</skos:prefLabel>
    <skos:scopeNote xml:lang="en">Long-term alteration in the characteristic weather conditions of a region, such as changes in precipitation and temperature.</skos:scopeNote>
    <skos:altLabel xml:lang="en">climatic change</skos:altLabel>
    <skos:altLabel xml:lang="en">global climate change</skos:altLabel>
    <skos:altLabel xml:lang="en">climate variability</skos:altLabel>
    <skos:altLabel xml:lang="en">paleoclimate</skos:altLabel>
    <skos:altLabel xml:lang="en">climate history</skos:altLabel>
    <skos:altLabel xml:lang="en">global warming</skos:altLabel>
    <skos:broader rdf:resource="http://www.usgs.gov/science/USGSThesaurus/atmospheric%20and%20climatic%20processes"/>
    <skos:narrower rdf:resource="http://www.usgs.gov/science/USGSThesaurus/desertification"/>
    <skos:related rdf:resource="http://www.usgs.gov/science/USGSThesaurus/climatology"/>
    <skos:related rdf:resource="http://www.usgs.gov/science/USGSThesaurus/effects%20of%20climate%20change"/>
    <skos:related rdf:resource="http://www.usgs.gov/science/USGSThesaurus/greenhouse%20gases"/>
    <skos:inScheme rdf:resource="http://www.usgs.gov/science/USGSThesaurus"/>
  </rdf:Description>
  <rdf:Description about="http://www.usgs.gov/science/USGSThesaurus/desertification">
    <rdf:type rdf:resource="http://www.w3.org/2004/02/skos/core#Concept"/>
    <skos:prefLabel xml:lang="en">desertification</skos:prefLabel>
    <skos:scopeNote xml:lang="en">The alteration of arable land to dry, barren land due to prolonged drought or the deleterious effects of human intervention including overgrazing, overpopulation, or destructive agricultural practices.</skos:scopeNote>
    <skos:broader rdf:resource="http://www.usgs.gov/science/USGSThesaurus/climate%20change"/>
    <skos:related rdf:resource="http://www.usgs.gov/science/USGSThesaurus/climatology"/>
    <skos:related rdf:resource="http://www.usgs.gov/science/USGSThesaurus/desert%20ecosystems"/>
    <skos:related rdf:resource="http://www.usgs.gov/science/USGSThesaurus/ecology"/>
    <skos:related rdf:resource="http://www.usgs.gov/science/USGSThesaurus/hazards"/>
    <skos:related rdf:resource="http://www.usgs.gov/science/USGSThesaurus/land%20use%20change"/>
    <skos:inScheme rdf:resource="http://www.usgs.gov/science/USGSThesaurus"/>
  </rdf:Description>
  <rdf:Description about="http://www.usgs.gov/science/USGSThesaurus/droughts">
    <rdf:type rdf:resource="http://www.w3.org/2004/02/skos/core#Concept"/>
    <skos:prefLabel xml:lang="en">droughts</skos:prefLabel>
    <skos:scopeNote xml:lang="en">Extended periods of moisture deficit over a sizeable area sufficient to have an adverse effect on vegetation, animals, or man.</skos:scopeNote>
    <skos:broader rdf:resource="http://www.usgs.gov/science/USGSThesaurus/atmospheric%20and%20climatic%20processes"/>
    <skos:related rdf:resource="http://www.usgs.gov/science/USGSThesaurus/atmospheric%20sciences"/>
    <skos:related rdf:resource="http://www.usgs.gov/science/USGSThesaurus/hazards"/>
    <skos:inScheme rdf:resource="http://www.usgs.gov/science/USGSThesaurus"/>
  </rdf:Description>
  <rdf:Description about="http://www.usgs.gov/science/USGSThesaurus/evaporation">
    <rdf:type rdf:resource="http://www.w3.org/2004/02/skos/core#Concept"/>
    <skos:prefLabel xml:lang="en">evaporation</skos:prefLabel>
    <skos:scopeNote xml:lang="en">Transfer of water from a surface into the atmosphere.</skos:scopeNote>
    <!--FOR evapotranspiration USE evaporation WITH transpiration-->
    <skos:altLabel xml:lang="en">evapotranspiration</skos:altLabel>
    <skos:broader rdf:resource="http://www.usgs.gov/science/USGSThesaurus/atmospheric%20and%20climatic%20processes"/>
    <skos:related rdf:resource="http://www.usgs.gov/science/USGSThesaurus/transpiration"/>
    <skos:related rdf:resource="http://www.usgs.gov/science/USGSThesaurus/water%20cycle"/>
    <skos:inScheme rdf:resource="http://www.usgs.gov/science/USGSThesaurus"/>
  </rdf:Description>
  <rdf:Description about="http://www.usgs.gov/science/USGSThesaurus/greenhouse%20effect">
    <rdf:type rdf:resource="http://www.w3.org/2004/02/skos/core#Concept"/>
    <skos:prefLabel xml:lang="en">greenhouse effect</skos:prefLabel>
    <skos:scopeNote xml:lang="en">Local, regional, or global warming in the atmosphere due to the higher heat capacity of certain gases such as carbon dioxide, methane, and ozone.</skos:scopeNote>
    <skos:broader rdf:resource="http://www.usgs.gov/science/USGSThesaurus/atmospheric%20and%20climatic%20processes"/>
    <skos:related rdf:resource="http://www.usgs.gov/science/USGSThesaurus/greenhouse%20gases"/>
    <skos:inScheme rdf:resource="http://www.usgs.gov/science/USGSThesaurus"/>
  </rdf:Description>
  <rdf:Description about="http://www.usgs.gov/science/USGSThesaurus/ocean-atmosphere%20interaction">
    <rdf:type rdf:resource="http://www.w3.org/2004/02/skos/core#Concept"/>
    <skos:prefLabel xml:lang="en">ocean-atmosphere interaction</skos:prefLabel>
    <skos:scopeNote xml:lang="en">Processes, including momentum, heat, gas and other exchanges, which result in profound effects on climate and interactions between the air in the lowest part of the atmosphere and the oceans.</skos:scopeNote>
    <skos:altLabel xml:lang="en">El Nino</skos:altLabel>
    <skos:altLabel xml:lang="en">La Nina</skos:altLabel>
    <skos:broader rdf:resource="http://www.usgs.gov/science/USGSThesaurus/atmospheric%20and%20climatic%20processes"/>
    <skos:narrower rdf:resource="http://www.usgs.gov/science/USGSThesaurus/El%20Nino-Southern%20Oscillation"/>
    <skos:related rdf:resource="http://www.usgs.gov/science/USGSThesaurus/atmospheric%20sciences"/>
    <skos:related rdf:resource="http://www.usgs.gov/science/USGSThesaurus/ocean%20processes"/>
    <skos:related rdf:resource="http://www.usgs.gov/science/USGSThesaurus/ocean%20sciences"/>
    <skos:inScheme rdf:resource="http://www.usgs.gov/science/USGSThesaurus"/>
  </rdf:Description>
  <rdf:Description about="http://www.usgs.gov/science/USGSThesaurus/El%20Nino-Southern%20Oscillation">
    <rdf:type rdf:resource="http://www.w3.org/2004/02/skos/core#Concept"/>
    <skos:prefLabel xml:lang="en">El Nino-Southern Oscillation</skos:prefLabel>
    <skos:scopeNote xml:lang="en">A roughly periodic variation in Pacific ocean sea-surface temperature causing changes in weather world-wide.</skos:scopeNote>
    <skos:altLabel xml:lang="en">ENSO</skos:altLabel>
    <skos:altLabel xml:lang="en">El Nino</skos:altLabel>
    <skos:altLabel xml:lang="en">La Nina</skos:altLabel>
    <skos:broader rdf:resource="http://www.usgs.gov/science/USGSThesaurus/ocean-atmosphere%20interaction"/>
    <skos:inScheme rdf:resource="http://www.usgs.gov/science/USGSThesaurus"/>
  </rdf:Description>
  <rdf:Description about="http://www.usgs.gov/science/USGSThesaurus/precipitation%20%28atmospheric%29">
    <rdf:type rdf:resource="http://www.w3.org/2004/02/skos/core#Concept"/>
    <skos:prefLabel xml:lang="en">precipitation (atmospheric)</skos:prefLabel>
    <skos:scopeNote xml:lang="en">Any or all forms of water particles that fall from the atmosphere, such as rain, snow, hail and sleet.</skos:scopeNote>
    <!--FOR rainfall measurement USE precipitation (atmospheric) WITH field inventory and monitoring-->
    <skos:altLabel xml:lang="en">rainfall measurement</skos:altLabel>
    <!--FOR snowfall measurement USE precipitation (atmospheric) WITH field inventory and monitoring-->
    <skos:altLabel xml:lang="en">snowfall measurement</skos:altLabel>
    <!--FOR precipitation measurement USE precipitation (atmospheric) WITH field inventory and monitoring-->
    <skos:altLabel xml:lang="en">precipitation measurement</skos:altLabel>
    <skos:altLabel xml:lang="en">rain</skos:altLabel>
    <skos:altLabel xml:lang="en">rainfall</skos:altLabel>
    <skos:altLabel xml:lang="en">snow</skos:altLabel>
    <skos:altLabel xml:lang="en">snowfall</skos:altLabel>
    <skos:broader rdf:resource="http://www.usgs.gov/science/USGSThesaurus/atmospheric%20and%20climatic%20processes"/>
    <skos:related rdf:resource="http://www.usgs.gov/science/USGSThesaurus/hydrologic%20processes"/>
    <skos:related rdf:resource="http://www.usgs.gov/science/USGSThesaurus/atmospheric%20deposition%20%28chemical%20%26%20particulate%29"/>
    <skos:related rdf:resource="http://www.usgs.gov/science/USGSThesaurus/atmospheric%20sciences"/>
    <skos:related rdf:resource="http://www.usgs.gov/science/USGSThesaurus/hydrology"/>
    <skos:related rdf:resource="http://www.usgs.gov/science/USGSThesaurus/storms"/>
    <skos:related rdf:resource="http://www.usgs.gov/science/USGSThesaurus/water%20cycle"/>
    <skos:inScheme rdf:resource="http://www.usgs.gov/science/USGSThesaurus"/>
  </rdf:Description>
  <rdf:Description about="http://www.usgs.gov/science/USGSThesaurus/storms">
    <rdf:type rdf:resource="http://www.w3.org/2004/02/skos/core#Concept"/>
    <skos:prefLabel xml:lang="en">storms</skos:prefLabel>
    <skos:scopeNote xml:lang="en">Atmospheric disturbances with winds of unusual force or direction. Accompanied by rain, snow, hail, or sleet, and often by thunder and lightning.</skos:scopeNote>
    <skos:broader rdf:resource="http://www.usgs.gov/science/USGSThesaurus/atmospheric%20and%20climatic%20processes"/>
    <skos:narrower rdf:resource="http://www.usgs.gov/science/USGSThesaurus/blizzards"/>
    <skos:narrower rdf:resource="http://www.usgs.gov/science/USGSThesaurus/dust%20storms"/>
    <skos:narrower rdf:resource="http://www.usgs.gov/science/USGSThesaurus/hurricanes"/>
    <skos:narrower rdf:resource="http://www.usgs.gov/science/USGSThesaurus/ice%20storms"/>
    <skos:narrower rdf:resource="http://www.usgs.gov/science/USGSThesaurus/tornadoes"/>
    <skos:related rdf:resource="http://www.usgs.gov/science/USGSThesaurus/hazards"/>
    <skos:related rdf:resource="http://www.usgs.gov/science/USGSThesaurus/meteorology"/>
    <skos:related rdf:resource="http://www.usgs.gov/science/USGSThesaurus/precipitation%20%28atmospheric%29"/>
    <skos:inScheme rdf:resource="http://www.usgs.gov/science/USGSThesaurus"/>
  </rdf:Description>
  <rdf:Description about="http://www.usgs.gov/science/USGSThesaurus/blizzards">
    <rdf:type rdf:resource="http://www.w3.org/2004/02/skos/core#Concept"/>
    <skos:prefLabel xml:lang="en">blizzards</skos:prefLabel>
    <skos:scopeNote xml:lang="en">Severe snowstorms with intense winds.</skos:scopeNote>
    <skos:broader rdf:resource="http://www.usgs.gov/science/USGSThesaurus/storms"/>
    <skos:inScheme rdf:resource="http://www.usgs.gov/science/USGSThesaurus"/>
  </rdf:Description>
  <rdf:Description about="http://www.usgs.gov/science/USGSThesaurus/dust%20storms">
    <rdf:type rdf:resource="http://www.w3.org/2004/02/skos/core#Concept"/>
    <skos:prefLabel xml:lang="en">dust storms</skos:prefLabel>
    <skos:scopeNote xml:lang="en">Atmospheric disturbances in which a significant amount of dust is transported.</skos:scopeNote>
    <skos:broader rdf:resource="http://www.usgs.gov/science/USGSThesaurus/storms"/>
    <skos:inScheme rdf:resource="http://www.usgs.gov/science/USGSThesaurus"/>
  </rdf:Description>
  <rdf:Description about="http://www.usgs.gov/science/USGSThesaurus/hurricanes">
    <rdf:type rdf:resource="http://www.w3.org/2004/02/skos/core#Concept"/>
    <skos:prefLabel xml:lang="en">hurricanes</skos:prefLabel>
    <skos:scopeNote xml:lang="en">Severe cyclones, or revolving storms, originating over the equatorial regions of the earth, accompanied by torrential rain, lightning, and winds with a speed greater than 74 miles per hour.</skos:scopeNote>
    <skos:altLabel xml:lang="en">typhoons</skos:altLabel>
    <skos:broader rdf:resource="http://www.usgs.gov/science/USGSThesaurus/storms"/>
    <skos:related rdf:resource="http://www.usgs.gov/science/USGSThesaurus/meteorology"/>
    <skos:inScheme rdf:resource="http://www.usgs.gov/science/USGSThesaurus"/>
  </rdf:Description>
  <rdf:Description about="http://www.usgs.gov/science/USGSThesaurus/ice%20storms">
    <rdf:type rdf:resource="http://www.w3.org/2004/02/skos/core#Concept"/>
    <skos:prefLabel xml:lang="en">ice storms</skos:prefLabel>
    <skos:scopeNote xml:lang="en">Storms in which falling snow or rain freezes on contact with surfaces on the ground.</skos:scopeNote>
    <skos:broader rdf:resource="http://www.usgs.gov/science/USGSThesaurus/storms"/>
    <skos:inScheme rdf:resource="http://www.usgs.gov/science/USGSThesaurus"/>
  </rdf:Description>
  <rdf:Description about="http://www.usgs.gov/science/USGSThesaurus/tornadoes">
    <rdf:type rdf:resource="http://www.w3.org/2004/02/skos/core#Concept"/>
    <skos:prefLabel xml:lang="en">tornadoes</skos:prefLabel>
    <skos:scopeNote xml:lang="en">Violent storms characterized by whirling funnels of wind moving at great speeds.</skos:scopeNote>
    <skos:broader rdf:resource="http://www.usgs.gov/science/USGSThesaurus/storms"/>
    <skos:related rdf:resource="http://www.usgs.gov/science/USGSThesaurus/meteorology"/>
    <skos:inScheme rdf:resource="http://www.usgs.gov/science/USGSThesaurus"/>
  </rdf:Description>
  <rdf:Description about="http://www.usgs.gov/science/USGSThesaurus/wind">
    <rdf:type rdf:resource="http://www.w3.org/2004/02/skos/core#Concept"/>
    <skos:prefLabel xml:lang="en">wind</skos:prefLabel>
    <skos:scopeNote xml:lang="en">Local air movements.</skos:scopeNote>
    <!--FOR wind erosion USE wind WITH erosion-->
    <skos:altLabel xml:lang="en">wind erosion</skos:altLabel>
    <skos:broader rdf:resource="http://www.usgs.gov/science/USGSThesaurus/atmospheric%20and%20climatic%20processes"/>
    <skos:inScheme rdf:resource="http://www.usgs.gov/science/USGSThesaurus"/>
  </rdf:Description>
  <rdf:Description about="http://www.usgs.gov/science/USGSThesaurus/coastal%20processes">
    <rdf:type rdf:resource="http://www.w3.org/2004/02/skos/core#Concept"/>
    <skos:prefLabel xml:lang="en">coastal processes</skos:prefLabel>
    <skos:scopeNote xml:lang="en">Processes unique to coastal areas including longshore transport, beach erosion, storm surge, shoreline change, delta formation, barrier island migration, beach stabilization by vegetation</skos:scopeNote>
    <!--FOR coastal erosion USE coastal processes WITH erosion-->
    <skos:altLabel xml:lang="en">coastal erosion</skos:altLabel>
    <!--FOR shoreline erosion USE coastal processes WITH erosion-->
    <skos:altLabel xml:lang="en">shoreline erosion</skos:altLabel>
    <!--FOR beach erosion USE coastal processes WITH erosion-->
    <skos:altLabel xml:lang="en">beach erosion</skos:altLabel>
    <!--FOR shoreline retreat USE coastal processes WITH erosion-->
    <skos:altLabel xml:lang="en">shoreline retreat</skos:altLabel>
    <skos:altLabel xml:lang="en">shoreline change</skos:altLabel>
    <!--FOR coastal hazards USE coastal processes WITH hazards-->
    <skos:altLabel xml:lang="en">coastal hazards</skos:altLabel>
    <skos:broader rdf:resource="http://www.usgs.gov/science/USGSThesaurus/biological%20and%20physical%20processes"/>
    <skos:narrower rdf:resource="http://www.usgs.gov/science/USGSThesaurus/barrier%20island%20migration"/>
    <skos:narrower rdf:resource="http://www.usgs.gov/science/USGSThesaurus/coastal%20emergence"/>
    <skos:narrower rdf:resource="http://www.usgs.gov/science/USGSThesaurus/coastal%20submergence"/>
    <skos:narrower rdf:resource="http://www.usgs.gov/science/USGSThesaurus/longshore%20currents"/>
    <skos:narrower rdf:resource="http://www.usgs.gov/science/USGSThesaurus/shoreline%20accretion"/>
    <skos:narrower rdf:resource="http://www.usgs.gov/science/USGSThesaurus/tidal%20currents"/>
    <skos:related rdf:resource="http://www.usgs.gov/science/USGSThesaurus/storm%20surge"/>
    <skos:related rdf:resource="http://www.usgs.gov/science/USGSThesaurus/mitigation%20of%20coastal%20hazards"/>
    <skos:inScheme rdf:resource="http://www.usgs.gov/science/USGSThesaurus"/>
  </rdf:Description>
  <rdf:Description about="http://www.usgs.gov/science/USGSThesaurus/barrier%20island%20migration">
    <rdf:type rdf:resource="http://www.w3.org/2004/02/skos/core#Concept"/>
    <skos:prefLabel xml:lang="en">barrier island migration</skos:prefLabel>
    <skos:scopeNote xml:lang="en">The slow, landward movement of barrier islands in response to sea level rise and repeated storm washover.</skos:scopeNote>
    <skos:broader rdf:resource="http://www.usgs.gov/science/USGSThesaurus/coastal%20processes"/>
    <skos:inScheme rdf:resource="http://www.usgs.gov/science/USGSThesaurus"/>
  </rdf:Description>
  <rdf:Description about="http://www.usgs.gov/science/USGSThesaurus/coastal%20emergence">
    <rdf:type rdf:resource="http://www.w3.org/2004/02/skos/core#Concept"/>
    <skos:prefLabel xml:lang="en">coastal emergence</skos:prefLabel>
    <skos:scopeNote xml:lang="en">Uplift of the coast accompanied by seaward displacement of the shoreline.</skos:scopeNote>
    <skos:broader rdf:resource="http://www.usgs.gov/science/USGSThesaurus/coastal%20processes"/>
    <skos:inScheme rdf:resource="http://www.usgs.gov/science/USGSThesaurus"/>
  </rdf:Description>
  <rdf:Description about="http://www.usgs.gov/science/USGSThesaurus/coastal%20submergence">
    <rdf:type rdf:resource="http://www.w3.org/2004/02/skos/core#Concept"/>
    <skos:prefLabel xml:lang="en">coastal submergence</skos:prefLabel>
    <skos:scopeNote xml:lang="en">Subsidence of the coast accompanied by landward displacement of the shoreline.</skos:scopeNote>
    <skos:broader rdf:resource="http://www.usgs.gov/science/USGSThesaurus/coastal%20processes"/>
    <skos:inScheme rdf:resource="http://www.usgs.gov/science/USGSThesaurus"/>
  </rdf:Description>
  <rdf:Description about="http://www.usgs.gov/science/USGSThesaurus/longshore%20currents">
    <rdf:type rdf:resource="http://www.w3.org/2004/02/skos/core#Concept"/>
    <skos:prefLabel xml:lang="en">longshore currents</skos:prefLabel>
    <skos:scopeNote xml:lang="en">Movement of water parallel to the coast due to waves striking the shoreline at an angle</skos:scopeNote>
    <!--FOR longshore drift USE longshore currents WITH sediment transport-->
    <skos:altLabel xml:lang="en">longshore drift</skos:altLabel>
    <!--FOR littoral drift USE longshore currents WITH sediment transport-->
    <skos:altLabel xml:lang="en">littoral drift</skos:altLabel>
    <skos:broader rdf:resource="http://www.usgs.gov/science/USGSThesaurus/coastal%20processes"/>
    <skos:inScheme rdf:resource="http://www.usgs.gov/science/USGSThesaurus"/>
  </rdf:Description>
  <rdf:Description about="http://www.usgs.gov/science/USGSThesaurus/shoreline%20accretion">
    <rdf:type rdf:resource="http://www.w3.org/2004/02/skos/core#Concept"/>
    <skos:prefLabel xml:lang="en">shoreline accretion</skos:prefLabel>
    <skos:scopeNote xml:lang="en">Seaward migration of the shoreline resulting from the addition of earth materials.</skos:scopeNote>
    <skos:broader rdf:resource="http://www.usgs.gov/science/USGSThesaurus/coastal%20processes"/>
    <skos:inScheme rdf:resource="http://www.usgs.gov/science/USGSThesaurus"/>
  </rdf:Description>
  <rdf:Description about="http://www.usgs.gov/science/USGSThesaurus/tidal%20currents">
    <rdf:type rdf:resource="http://www.w3.org/2004/02/skos/core#Concept"/>
    <skos:prefLabel xml:lang="en">tidal currents</skos:prefLabel>
    <skos:scopeNote xml:lang="en">Currents caused by tidal changes in water level from one body of water to another.</skos:scopeNote>
    <skos:broader rdf:resource="http://www.usgs.gov/science/USGSThesaurus/coastal%20processes"/>
    <skos:inScheme rdf:resource="http://www.usgs.gov/science/USGSThesaurus"/>
  </rdf:Description>
  <rdf:Description about="http://www.usgs.gov/science/USGSThesaurus/ecological%20processes">
    <rdf:type rdf:resource="http://www.w3.org/2004/02/skos/core#Concept"/>
    <skos:prefLabel xml:lang="en">ecological processes</skos:prefLabel>
    <skos:scopeNote xml:lang="en">Dynamic biogeochemical interactions that occur among and between biotic and abiotic components of the biosphere.</skos:scopeNote>
    <skos:altLabel xml:lang="en">ecological models</skos:altLabel>
    <skos:altLabel xml:lang="en">environmental processes</skos:altLabel>
    <skos:broader rdf:resource="http://www.usgs.gov/science/USGSThesaurus/biological%20and%20physical%20processes"/>
    <skos:narrower rdf:resource="http://www.usgs.gov/science/USGSThesaurus/algal%20blooms"/>
    <skos:narrower rdf:resource="http://www.usgs.gov/science/USGSThesaurus/bioaccumulation"/>
    <skos:narrower rdf:resource="http://www.usgs.gov/science/USGSThesaurus/biogeochemical%20cycling"/>
    <skos:narrower rdf:resource="http://www.usgs.gov/science/USGSThesaurus/biological%20productivity"/>
    <skos:narrower rdf:resource="http://www.usgs.gov/science/USGSThesaurus/contaminant%20transport"/>
    <skos:narrower rdf:resource="http://www.usgs.gov/science/USGSThesaurus/dispersal%20%28organisms%29"/>
    <skos:narrower rdf:resource="http://www.usgs.gov/science/USGSThesaurus/ecological%20competition"/>
    <skos:narrower rdf:resource="http://www.usgs.gov/science/USGSThesaurus/ecosystem%20functions"/>
    <skos:narrower rdf:resource="http://www.usgs.gov/science/USGSThesaurus/eutrophication"/>
    <skos:narrower rdf:resource="http://www.usgs.gov/science/USGSThesaurus/extinction%20and%20extirpation"/>
    <skos:narrower rdf:resource="http://www.usgs.gov/science/USGSThesaurus/habitat%20alteration"/>
    <skos:narrower rdf:resource="http://www.usgs.gov/science/USGSThesaurus/migration%20%28organisms%29"/>
    <skos:narrower rdf:resource="http://www.usgs.gov/science/USGSThesaurus/pollination"/>
    <skos:narrower rdf:resource="http://www.usgs.gov/science/USGSThesaurus/succession%20%28biological%29"/>
    <skos:narrower rdf:resource="http://www.usgs.gov/science/USGSThesaurus/transpiration"/>
    <skos:related rdf:resource="http://www.usgs.gov/science/USGSThesaurus/ecology"/>
    <skos:related rdf:resource="http://www.usgs.gov/science/USGSThesaurus/population%20and%20community%20ecology"/>
    <skos:related rdf:resource="http://www.usgs.gov/science/USGSThesaurus/soil%20formation"/>
    <skos:inScheme rdf:resource="http://www.usgs.gov/science/USGSThesaurus"/>
  </rdf:Description>
  <rdf:Description about="http://www.usgs.gov/science/USGSThesaurus/algal%20blooms">
    <rdf:type rdf:resource="http://www.w3.org/2004/02/skos/core#Concept"/>
    <skos:prefLabel xml:lang="en">algal blooms</skos:prefLabel>
    <skos:scopeNote xml:lang="en">Exceptional growth of algae and cyanobacteria in lakes, rivers or oceans due to excessive nutrients or climatic conditions.</skos:scopeNote>
    <skos:altLabel xml:lang="en">brown tides</skos:altLabel>
    <!--FOR harmful algal blooms USE algal blooms WITH hazards-->
    <skos:altLabel xml:lang="en">harmful algal blooms</skos:altLabel>
    <skos:altLabel xml:lang="en">red tides</skos:altLabel>
    <skos:broader rdf:resource="http://www.usgs.gov/science/USGSThesaurus/ecological%20processes"/>
    <skos:related rdf:resource="http://www.usgs.gov/science/USGSThesaurus/algae"/>
    <skos:related rdf:resource="http://www.usgs.gov/science/USGSThesaurus/hazards"/>
    <skos:related rdf:resource="http://www.usgs.gov/science/USGSThesaurus/phycology"/>
    <skos:related rdf:resource="http://www.usgs.gov/science/USGSThesaurus/population%20dynamics"/>
    <skos:inScheme rdf:resource="http://www.usgs.gov/science/USGSThesaurus"/>
  </rdf:Description>
  <rdf:Description about="http://www.usgs.gov/science/USGSThesaurus/bioaccumulation">
    <rdf:type rdf:resource="http://www.w3.org/2004/02/skos/core#Concept"/>
    <skos:prefLabel xml:lang="en">bioaccumulation</skos:prefLabel>
    <skos:scopeNote xml:lang="en">The biological sequestering of a substance at a higher concentration than that at which it occurs in the surrounding environment or medium.  Also, the process whereby a substance enters an organism through the gills, epithelial tissues, dietary, or other sources.</skos:scopeNote>
    <skos:altLabel xml:lang="en">bioconcentration</skos:altLabel>
    <skos:broader rdf:resource="http://www.usgs.gov/science/USGSThesaurus/ecological%20processes"/>
    <skos:related rdf:resource="http://www.usgs.gov/science/USGSThesaurus/ecology"/>
    <skos:related rdf:resource="http://www.usgs.gov/science/USGSThesaurus/ecotoxicology"/>
    <skos:inScheme rdf:resource="http://www.usgs.gov/science/USGSThesaurus"/>
  </rdf:Description>
  <rdf:Description about="http://www.usgs.gov/science/USGSThesaurus/biogeochemical%20cycling">
    <rdf:type rdf:resource="http://www.w3.org/2004/02/skos/core#Concept"/>
    <skos:prefLabel xml:lang="en">biogeochemical cycling</skos:prefLabel>
    <skos:scopeNote xml:lang="en">The cycling of chemical constituents through a biological system.</skos:scopeNote>
    <skos:altLabel xml:lang="en">biogeochemical functioning</skos:altLabel>
    <skos:altLabel xml:lang="en">biogeochemical processes</skos:altLabel>
    <skos:altLabel xml:lang="en">decomposition (organic)</skos:altLabel>
    <skos:altLabel xml:lang="en">organic decomposition</skos:altLabel>
    <skos:broader rdf:resource="http://www.usgs.gov/science/USGSThesaurus/ecological%20processes"/>
    <skos:narrower rdf:resource="http://www.usgs.gov/science/USGSThesaurus/carbon%20cycling"/>
    <skos:narrower rdf:resource="http://www.usgs.gov/science/USGSThesaurus/nutrient%20cycling"/>
    <skos:related rdf:resource="http://www.usgs.gov/science/USGSThesaurus/biochemistry"/>
    <skos:related rdf:resource="http://www.usgs.gov/science/USGSThesaurus/decomposers"/>
    <skos:related rdf:resource="http://www.usgs.gov/science/USGSThesaurus/ecology"/>
    <skos:related rdf:resource="http://www.usgs.gov/science/USGSThesaurus/geochemistry"/>
    <skos:related rdf:resource="http://www.usgs.gov/science/USGSThesaurus/geochemical%20processes"/>
    <skos:inScheme rdf:resource="http://www.usgs.gov/science/USGSThesaurus"/>
  </rdf:Description>
  <rdf:Description about="http://www.usgs.gov/science/USGSThesaurus/carbon%20cycling">
    <rdf:type rdf:resource="http://www.w3.org/2004/02/skos/core#Concept"/>
    <skos:prefLabel xml:lang="en">carbon cycling</skos:prefLabel>
    <skos:scopeNote xml:lang="en">The circulation of carbon in the biosphere, atmosphere, and hydrosphere through a series of processes that include photosynthesis, consumption, and respiration.</skos:scopeNote>
    <skos:broader rdf:resource="http://www.usgs.gov/science/USGSThesaurus/biogeochemical%20cycling"/>
    <skos:related rdf:resource="http://www.usgs.gov/science/USGSThesaurus/biochemistry"/>
    <skos:related rdf:resource="http://www.usgs.gov/science/USGSThesaurus/ecology"/>
    <skos:related rdf:resource="http://www.usgs.gov/science/USGSThesaurus/geochemistry"/>
    <skos:inScheme rdf:resource="http://www.usgs.gov/science/USGSThesaurus"/>
  </rdf:Description>
  <rdf:Description about="http://www.usgs.gov/science/USGSThesaurus/nutrient%20cycling">
    <rdf:type rdf:resource="http://www.w3.org/2004/02/skos/core#Concept"/>
    <skos:prefLabel xml:lang="en">nutrient cycling</skos:prefLabel>
    <skos:scopeNote xml:lang="en">The exchange of elements or compounds essential for the nourishment of organisms in an ecosystem.</skos:scopeNote>
    <skos:altLabel xml:lang="en">nutrient balance</skos:altLabel>
    <skos:broader rdf:resource="http://www.usgs.gov/science/USGSThesaurus/biogeochemical%20cycling"/>
    <skos:narrower rdf:resource="http://www.usgs.gov/science/USGSThesaurus/food%20web"/>
    <skos:related rdf:resource="http://www.usgs.gov/science/USGSThesaurus/biochemistry"/>
    <skos:related rdf:resource="http://www.usgs.gov/science/USGSThesaurus/ecology"/>
    <skos:related rdf:resource="http://www.usgs.gov/science/USGSThesaurus/nutrient%20content%20%28water%29"/>
    <skos:inScheme rdf:resource="http://www.usgs.gov/science/USGSThesaurus"/>
  </rdf:Description>
  <rdf:Description about="http://www.usgs.gov/science/USGSThesaurus/food%20web">
    <rdf:type rdf:resource="http://www.w3.org/2004/02/skos/core#Concept"/>
    <skos:prefLabel xml:lang="en">food web</skos:prefLabel>
    <skos:scopeNote xml:lang="en">The complex intertwining of the interrelated food chains in an ecosystem.</skos:scopeNote>
    <skos:altLabel xml:lang="en">food chain</skos:altLabel>
    <skos:altLabel xml:lang="en">food cycle</skos:altLabel>
    <skos:altLabel xml:lang="en">trophic level dynamics</skos:altLabel>
    <skos:altLabel xml:lang="en">trophic relationships</skos:altLabel>
    <skos:broader rdf:resource="http://www.usgs.gov/science/USGSThesaurus/nutrient%20cycling"/>
    <skos:related rdf:resource="http://www.usgs.gov/science/USGSThesaurus/biochemistry"/>
    <skos:related rdf:resource="http://www.usgs.gov/science/USGSThesaurus/ecology"/>
    <skos:inScheme rdf:resource="http://www.usgs.gov/science/USGSThesaurus"/>
  </rdf:Description>
  <rdf:Description about="http://www.usgs.gov/science/USGSThesaurus/biological%20productivity">
    <rdf:type rdf:resource="http://www.w3.org/2004/02/skos/core#Concept"/>
    <skos:prefLabel xml:lang="en">biological productivity</skos:prefLabel>
    <skos:scopeNote xml:lang="en">The rate at which primary producers in the ecosystem utilize solar energy to produce food for consumption by other organisms. Do not use this term for productivity of organisms related to studies of the reproduction rates of a species.</skos:scopeNote>
    <skos:broader rdf:resource="http://www.usgs.gov/science/USGSThesaurus/ecological%20processes"/>
    <skos:related rdf:resource="http://www.usgs.gov/science/USGSThesaurus/ecology"/>
    <skos:related rdf:resource="http://www.usgs.gov/science/USGSThesaurus/life%20sciences"/>
    <skos:inScheme rdf:resource="http://www.usgs.gov/science/USGSThesaurus"/>
  </rdf:Description>
  <rdf:Description about="http://www.usgs.gov/science/USGSThesaurus/contaminant%20transport">
    <rdf:type rdf:resource="http://www.w3.org/2004/02/skos/core#Concept"/>
    <skos:prefLabel xml:lang="en">contaminant transport</skos:prefLabel>
    <skos:scopeNote xml:lang="en">Processes involved in the movement of impurities through air, water, and soil.</skos:scopeNote>
    <skos:broader rdf:resource="http://www.usgs.gov/science/USGSThesaurus/ecological%20processes"/>
    <skos:related rdf:resource="http://www.usgs.gov/science/USGSThesaurus/ecotoxicology"/>
    <skos:inScheme rdf:resource="http://www.usgs.gov/science/USGSThesaurus"/>
  </rdf:Description>
  <rdf:Description about="http://www.usgs.gov/science/USGSThesaurus/dispersal%20%28organisms%29">
    <rdf:type rdf:resource="http://www.w3.org/2004/02/skos/core#Concept"/>
    <skos:prefLabel xml:lang="en">dispersal (organisms)</skos:prefLabel>
    <skos:scopeNote xml:lang="en">The dissemination or geographic spread of individuals of a plant or animal population.</skos:scopeNote>
    <skos:altLabel xml:lang="en">colonization (organisms)</skos:altLabel>
    <skos:broader rdf:resource="http://www.usgs.gov/science/USGSThesaurus/ecological%20processes"/>
    <skos:related rdf:resource="http://www.usgs.gov/science/USGSThesaurus/ecology"/>
    <skos:related rdf:resource="http://www.usgs.gov/science/USGSThesaurus/life%20sciences"/>
    <skos:related rdf:resource="http://www.usgs.gov/science/USGSThesaurus/migration%20%28organisms%29"/>
    <skos:inScheme rdf:resource="http://www.usgs.gov/science/USGSThesaurus"/>
  </rdf:Description>
  <rdf:Description about="http://www.usgs.gov/science/USGSThesaurus/ecological%20competition">
    <rdf:type rdf:resource="http://www.w3.org/2004/02/skos/core#Concept"/>
    <skos:prefLabel xml:lang="en">ecological competition</skos:prefLabel>
    <skos:scopeNote xml:lang="en">The struggle between members of two or more species for scarce environmental resources.</skos:scopeNote>
    <skos:broader rdf:resource="http://www.usgs.gov/science/USGSThesaurus/ecological%20processes"/>
    <skos:related rdf:resource="http://www.usgs.gov/science/USGSThesaurus/biodiversity"/>
    <skos:related rdf:resource="http://www.usgs.gov/science/USGSThesaurus/community%20ecology"/>
    <skos:related rdf:resource="http://www.usgs.gov/science/USGSThesaurus/ecology"/>
    <skos:related rdf:resource="http://www.usgs.gov/science/USGSThesaurus/endangered%20species"/>
    <skos:inScheme rdf:resource="http://www.usgs.gov/science/USGSThesaurus"/>
  </rdf:Description>
  <rdf:Description about="http://www.usgs.gov/science/USGSThesaurus/ecosystem%20functions">
    <rdf:type rdf:resource="http://www.w3.org/2004/02/skos/core#Concept"/>
    <skos:prefLabel xml:lang="en">ecosystem functions</skos:prefLabel>
    <skos:scopeNote xml:lang="en">The total life activities of organisms in habitats and the effects of those activities on the nonliving components of the environment.</skos:scopeNote>
    <!--FOR estuarine ecosystem functions USE ecosystem functions WITH estuarine ecosystems-->
    <skos:altLabel xml:lang="en">estuarine ecosystem functions</skos:altLabel>
    <skos:broader rdf:resource="http://www.usgs.gov/science/USGSThesaurus/ecological%20processes"/>
    <skos:narrower rdf:resource="http://www.usgs.gov/science/USGSThesaurus/wetland%20functions"/>
    <skos:related rdf:resource="http://www.usgs.gov/science/USGSThesaurus/ecology"/>
    <skos:related rdf:resource="http://www.usgs.gov/science/USGSThesaurus/ecosystem%20services%20valuation"/>
    <skos:related rdf:resource="http://www.usgs.gov/science/USGSThesaurus/ecosystems"/>
    <skos:inScheme rdf:resource="http://www.usgs.gov/science/USGSThesaurus"/>
  </rdf:Description>
  <rdf:Description about="http://www.usgs.gov/science/USGSThesaurus/wetland%20functions">
    <rdf:type rdf:resource="http://www.w3.org/2004/02/skos/core#Concept"/>
    <skos:prefLabel xml:lang="en">wetland functions</skos:prefLabel>
    <skos:scopeNote xml:lang="en">Processes related to wetlands such as support of ecosystems, evaporation effects on weather, nutrient cycles, etc.</skos:scopeNote>
    <skos:broader rdf:resource="http://www.usgs.gov/science/USGSThesaurus/ecosystem%20functions"/>
    <skos:related rdf:resource="http://www.usgs.gov/science/USGSThesaurus/wetland%20ecosystems"/>
    <skos:related rdf:resource="http://www.usgs.gov/science/USGSThesaurus/ecology"/>
    <skos:related rdf:resource="http://www.usgs.gov/science/USGSThesaurus/hydrology"/>
    <skos:inScheme rdf:resource="http://www.usgs.gov/science/USGSThesaurus"/>
  </rdf:Description>
  <rdf:Description about="http://www.usgs.gov/science/USGSThesaurus/eutrophication">
    <rdf:type rdf:resource="http://www.w3.org/2004/02/skos/core#Concept"/>
    <skos:prefLabel xml:lang="en">eutrophication</skos:prefLabel>
    <skos:scopeNote xml:lang="en">The process by which water becomes enriched with plant nutrients, most commonly phosphorus and nitrogen.</skos:scopeNote>
    <skos:broader rdf:resource="http://www.usgs.gov/science/USGSThesaurus/ecological%20processes"/>
    <skos:related rdf:resource="http://www.usgs.gov/science/USGSThesaurus/ecology"/>
    <skos:related rdf:resource="http://www.usgs.gov/science/USGSThesaurus/limnology"/>
    <skos:related rdf:resource="http://www.usgs.gov/science/USGSThesaurus/oxygen%20content%20%28water%29"/>
    <skos:inScheme rdf:resource="http://www.usgs.gov/science/USGSThesaurus"/>
  </rdf:Description>
  <rdf:Description about="http://www.usgs.gov/science/USGSThesaurus/extinction%20and%20extirpation">
    <rdf:type rdf:resource="http://www.w3.org/2004/02/skos/core#Concept"/>
    <skos:prefLabel xml:lang="en">extinction and extirpation</skos:prefLabel>
    <skos:scopeNote xml:lang="en">Extinction is the complete disappearance of a species from the earth.  Extirpation is the complete disappearance (elimination) of a species from a given region, island, or area.</skos:scopeNote>
    <skos:altLabel xml:lang="en">extirpation</skos:altLabel>
    <skos:broader rdf:resource="http://www.usgs.gov/science/USGSThesaurus/ecological%20processes"/>
    <skos:related rdf:resource="http://www.usgs.gov/science/USGSThesaurus/ecology"/>
    <skos:related rdf:resource="http://www.usgs.gov/science/USGSThesaurus/life%20sciences"/>
    <skos:inScheme rdf:resource="http://www.usgs.gov/science/USGSThesaurus"/>
  </rdf:Description>
  <rdf:Description about="http://www.usgs.gov/science/USGSThesaurus/habitat%20alteration">
    <rdf:type rdf:resource="http://www.w3.org/2004/02/skos/core#Concept"/>
    <skos:prefLabel xml:lang="en">habitat alteration</skos:prefLabel>
    <skos:scopeNote xml:lang="en">Natural or human-related changes in the environments where plants and animals live.</skos:scopeNote>
    <skos:altLabel xml:lang="en">habitat destruction</skos:altLabel>
    <skos:broader rdf:resource="http://www.usgs.gov/science/USGSThesaurus/ecological%20processes"/>
    <skos:narrower rdf:resource="http://www.usgs.gov/science/USGSThesaurus/fire%20damage"/>
    <skos:related rdf:resource="http://www.usgs.gov/science/USGSThesaurus/ecology"/>
    <skos:related rdf:resource="http://www.usgs.gov/science/USGSThesaurus/habitat%20fragmentation"/>
    <skos:inScheme rdf:resource="http://www.usgs.gov/science/USGSThesaurus"/>
  </rdf:Description>
  <rdf:Description about="http://www.usgs.gov/science/USGSThesaurus/fire%20damage">
    <rdf:type rdf:resource="http://www.w3.org/2004/02/skos/core#Concept"/>
    <skos:prefLabel xml:lang="en">fire damage</skos:prefLabel>
    <skos:scopeNote xml:lang="en">Destruction of surficial materials and vegetation by burning.</skos:scopeNote>
    <!--FOR composite burn index USE fire damage WITH remote sensing-->
    <skos:altLabel xml:lang="en">composite burn index</skos:altLabel>
    <!--FOR normalized burn ratio USE fire damage WITH remote sensing-->
    <skos:altLabel xml:lang="en">normalized burn ratio</skos:altLabel>
    <skos:broader rdf:resource="http://www.usgs.gov/science/USGSThesaurus/habitat%20alteration"/>
    <skos:inScheme rdf:resource="http://www.usgs.gov/science/USGSThesaurus"/>
  </rdf:Description>
  <rdf:Description about="http://www.usgs.gov/science/USGSThesaurus/migration%20%28organisms%29">
    <rdf:type rdf:resource="http://www.w3.org/2004/02/skos/core#Concept"/>
    <skos:prefLabel xml:lang="en">migration (organisms)</skos:prefLabel>
    <skos:scopeNote xml:lang="en">The movement of animals, often periodical, from one area to another due to seasonal changes, availability of food, or climatic conditions.</skos:scopeNote>
    <!--FOR biological invasions USE migration (organisms) WITH invasive species-->
    <skos:altLabel xml:lang="en">biological invasions</skos:altLabel>
    <!--FOR flyways USE migration (organisms) WITH biogeography-->
    <skos:altLabel xml:lang="en">flyways</skos:altLabel>
    <skos:altLabel xml:lang="en">seasonal migration</skos:altLabel>
    <skos:broader rdf:resource="http://www.usgs.gov/science/USGSThesaurus/ecological%20processes"/>
    <skos:related rdf:resource="http://www.usgs.gov/science/USGSThesaurus/animal%20behavior"/>
    <skos:related rdf:resource="http://www.usgs.gov/science/USGSThesaurus/biogeography"/>
    <skos:related rdf:resource="http://www.usgs.gov/science/USGSThesaurus/dispersal%20%28organisms%29"/>
    <skos:related rdf:resource="http://www.usgs.gov/science/USGSThesaurus/ecology"/>
    <skos:related rdf:resource="http://www.usgs.gov/science/USGSThesaurus/life%20sciences"/>
    <skos:related rdf:resource="http://www.usgs.gov/science/USGSThesaurus/migratory%20species"/>
    <skos:inScheme rdf:resource="http://www.usgs.gov/science/USGSThesaurus"/>
  </rdf:Description>
  <rdf:Description about="http://www.usgs.gov/science/USGSThesaurus/pollination">
    <rdf:type rdf:resource="http://www.w3.org/2004/02/skos/core#Concept"/>
    <skos:prefLabel xml:lang="en">pollination</skos:prefLabel>
    <skos:scopeNote xml:lang="en">Wind, bees, or other agents transfer plant pollen from flower anthers or cones to stigmas, thereby fertilizing plants for reproduction.</skos:scopeNote>
    <skos:broader rdf:resource="http://www.usgs.gov/science/USGSThesaurus/ecological%20processes"/>
    <skos:related rdf:resource="http://www.usgs.gov/science/USGSThesaurus/pollinators"/>
    <skos:inScheme rdf:resource="http://www.usgs.gov/science/USGSThesaurus"/>
  </rdf:Description>
  <rdf:Description about="http://www.usgs.gov/science/USGSThesaurus/succession%20%28biological%29">
    <rdf:type rdf:resource="http://www.w3.org/2004/02/skos/core#Concept"/>
    <skos:prefLabel xml:lang="en">succession (biological)</skos:prefLabel>
    <skos:scopeNote xml:lang="en">Gradual replacement of one species in an area by another.</skos:scopeNote>
    <skos:altLabel xml:lang="en">ecologic succession</skos:altLabel>
    <skos:broader rdf:resource="http://www.usgs.gov/science/USGSThesaurus/ecological%20processes"/>
    <skos:related rdf:resource="http://www.usgs.gov/science/USGSThesaurus/ecology"/>
    <skos:inScheme rdf:resource="http://www.usgs.gov/science/USGSThesaurus"/>
  </rdf:Description>
  <rdf:Description about="http://www.usgs.gov/science/USGSThesaurus/transpiration">
    <rdf:type rdf:resource="http://www.w3.org/2004/02/skos/core#Concept"/>
    <skos:prefLabel xml:lang="en">transpiration</skos:prefLabel>
    <skos:scopeNote xml:lang="en">Evaporation of water from plants.</skos:scopeNote>
    <!--FOR evapotranspiration USE transpiration WITH evaporation-->
    <skos:altLabel xml:lang="en">evapotranspiration</skos:altLabel>
    <skos:broader rdf:resource="http://www.usgs.gov/science/USGSThesaurus/ecological%20processes"/>
    <skos:related rdf:resource="http://www.usgs.gov/science/USGSThesaurus/evaporation"/>
    <skos:inScheme rdf:resource="http://www.usgs.gov/science/USGSThesaurus"/>
  </rdf:Description>
  <rdf:Description about="http://www.usgs.gov/science/USGSThesaurus/estuarine%20processes">
    <rdf:type rdf:resource="http://www.w3.org/2004/02/skos/core#Concept"/>
    <skos:prefLabel xml:lang="en">estuarine processes</skos:prefLabel>
    <skos:scopeNote xml:lang="en">Processes affecting estuaries including tides, waves, mixing of fluvial and marine waters</skos:scopeNote>
    <!--FOR estuarine sediment transport USE estuarine processes WITH sediment transport-->
    <skos:altLabel xml:lang="en">estuarine sediment transport</skos:altLabel>
    <skos:broader rdf:resource="http://www.usgs.gov/science/USGSThesaurus/biological%20and%20physical%20processes"/>
    <skos:narrower rdf:resource="http://www.usgs.gov/science/USGSThesaurus/estuarine%20currents"/>
    <skos:narrower rdf:resource="http://www.usgs.gov/science/USGSThesaurus/estuarine%20mixing"/>
    <skos:inScheme rdf:resource="http://www.usgs.gov/science/USGSThesaurus"/>
  </rdf:Description>
  <rdf:Description about="http://www.usgs.gov/science/USGSThesaurus/estuarine%20currents">
    <rdf:type rdf:resource="http://www.w3.org/2004/02/skos/core#Concept"/>
    <skos:prefLabel xml:lang="en">estuarine currents</skos:prefLabel>
    <skos:scopeNote xml:lang="en">Movement of water within estuaries due to the complex interaction of winds, tides, and variations in water density</skos:scopeNote>
    <skos:broader rdf:resource="http://www.usgs.gov/science/USGSThesaurus/estuarine%20processes"/>
    <skos:inScheme rdf:resource="http://www.usgs.gov/science/USGSThesaurus"/>
  </rdf:Description>
  <rdf:Description about="http://www.usgs.gov/science/USGSThesaurus/estuarine%20mixing">
    <rdf:type rdf:resource="http://www.w3.org/2004/02/skos/core#Concept"/>
    <skos:prefLabel xml:lang="en">estuarine mixing</skos:prefLabel>
    <skos:scopeNote xml:lang="en">Interaction of tidal forcing and river discharge in an estuary, leading to any of three vertical salinity profiles: salt wedge, stratified, or well mixed. We also include mixing due to extreme events such as storm surge.</skos:scopeNote>
    <skos:broader rdf:resource="http://www.usgs.gov/science/USGSThesaurus/estuarine%20processes"/>
    <skos:inScheme rdf:resource="http://www.usgs.gov/science/USGSThesaurus"/>
  </rdf:Description>
  <rdf:Description about="http://www.usgs.gov/science/USGSThesaurus/evolution">
    <rdf:type rdf:resource="http://www.w3.org/2004/02/skos/core#Concept"/>
    <skos:prefLabel xml:lang="en">evolution</skos:prefLabel>
    <skos:scopeNote xml:lang="en">Change in the genetic composition of populations of living organisms.</skos:scopeNote>
    <skos:altLabel xml:lang="en">gene flow</skos:altLabel>
    <skos:broader rdf:resource="http://www.usgs.gov/science/USGSThesaurus/biological%20and%20physical%20processes"/>
    <skos:inScheme rdf:resource="http://www.usgs.gov/science/USGSThesaurus"/>
  </rdf:Description>
  <rdf:Description about="http://www.usgs.gov/science/USGSThesaurus/fires">
    <rdf:type rdf:resource="http://www.w3.org/2004/02/skos/core#Concept"/>
    <skos:prefLabel xml:lang="en">fires</skos:prefLabel>
    <skos:scopeNote xml:lang="en">Combustion, marked by flames or intense heat, in natural settings, often ignited by lightning or human activities.  For fires set as part of natural resource management, use 'controlled fires'.   </skos:scopeNote>
    <!--FOR fire preparedness USE fires WITH hazard preparedness-->
    <skos:altLabel xml:lang="en">fire preparedness</skos:altLabel>
    <skos:altLabel xml:lang="en">fires (uncontrolled)</skos:altLabel>
    <skos:altLabel xml:lang="en">wildfires</skos:altLabel>
    <skos:broader rdf:resource="http://www.usgs.gov/science/USGSThesaurus/biological%20and%20physical%20processes"/>
    <skos:related rdf:resource="http://www.usgs.gov/science/USGSThesaurus/atmospheric%20sciences"/>
    <skos:related rdf:resource="http://www.usgs.gov/science/USGSThesaurus/controlled%20fires"/>
    <skos:related rdf:resource="http://www.usgs.gov/science/USGSThesaurus/ecology"/>
    <skos:related rdf:resource="http://www.usgs.gov/science/USGSThesaurus/hazards"/>
    <skos:related rdf:resource="http://www.usgs.gov/science/USGSThesaurus/human%20impacts"/>
    <skos:inScheme rdf:resource="http://www.usgs.gov/science/USGSThesaurus"/>
  </rdf:Description>
  <rdf:Description about="http://www.usgs.gov/science/USGSThesaurus/geochemical%20processes">
    <rdf:type rdf:resource="http://www.w3.org/2004/02/skos/core#Concept"/>
    <skos:prefLabel xml:lang="en">geochemical processes</skos:prefLabel>
    <skos:scopeNote xml:lang="en">Processes affecting the amount, distribution, or structure of chemical elements in air, water, soil, rocks, and minerals.</skos:scopeNote>
    <skos:broader rdf:resource="http://www.usgs.gov/science/USGSThesaurus/biological%20and%20physical%20processes"/>
    <skos:narrower rdf:resource="http://www.usgs.gov/science/USGSThesaurus/biodegradation"/>
    <skos:narrower rdf:resource="http://www.usgs.gov/science/USGSThesaurus/carbon%20sequestration"/>
    <skos:narrower rdf:resource="http://www.usgs.gov/science/USGSThesaurus/ocean%20acidification"/>
    <skos:narrower rdf:resource="http://www.usgs.gov/science/USGSThesaurus/ore%20formation"/>
    <skos:narrower rdf:resource="http://www.usgs.gov/science/USGSThesaurus/oxidation%20and%20reduction"/>
    <skos:narrower rdf:resource="http://www.usgs.gov/science/USGSThesaurus/reaction%20transport"/>
    <skos:narrower rdf:resource="http://www.usgs.gov/science/USGSThesaurus/sorption"/>
    <skos:related rdf:resource="http://www.usgs.gov/science/USGSThesaurus/geochemistry"/>
    <skos:related rdf:resource="http://www.usgs.gov/science/USGSThesaurus/soil%20formation"/>
    <skos:related rdf:resource="http://www.usgs.gov/science/USGSThesaurus/biogeochemical%20cycling"/>
    <skos:inScheme rdf:resource="http://www.usgs.gov/science/USGSThesaurus"/>
  </rdf:Description>
  <rdf:Description about="http://www.usgs.gov/science/USGSThesaurus/biodegradation">
    <rdf:type rdf:resource="http://www.w3.org/2004/02/skos/core#Concept"/>
    <skos:prefLabel xml:lang="en">biodegradation</skos:prefLabel>
    <skos:scopeNote xml:lang="en">Reduction in the concentration of harmful chemicals by the action of animals and plants.</skos:scopeNote>
    <skos:altLabel xml:lang="en">natural attenuation (harmful chemicals)</skos:altLabel>
    <skos:broader rdf:resource="http://www.usgs.gov/science/USGSThesaurus/geochemical%20processes"/>
    <skos:inScheme rdf:resource="http://www.usgs.gov/science/USGSThesaurus"/>
  </rdf:Description>
  <rdf:Description about="http://www.usgs.gov/science/USGSThesaurus/carbon%20sequestration">
    <rdf:type rdf:resource="http://www.w3.org/2004/02/skos/core#Concept"/>
    <skos:prefLabel xml:lang="en">carbon sequestration</skos:prefLabel>
    <skos:scopeNote xml:lang="en">Long-term storage of carbon in soils and terrestrial organic material, typically of importance in understanding the balance of CO2 in the global climate system.</skos:scopeNote>
    <skos:broader rdf:resource="http://www.usgs.gov/science/USGSThesaurus/geochemical%20processes"/>
    <skos:inScheme rdf:resource="http://www.usgs.gov/science/USGSThesaurus"/>
  </rdf:Description>
  <rdf:Description about="http://www.usgs.gov/science/USGSThesaurus/ocean%20acidification">
    <rdf:type rdf:resource="http://www.w3.org/2004/02/skos/core#Concept"/>
    <skos:prefLabel xml:lang="en">ocean acidification</skos:prefLabel>
    <skos:scopeNote xml:lang="en">Decrease in the pH of ocean waters as a result of the increase in atmospheric carbon dioxide concentration.</skos:scopeNote>
    <skos:broader rdf:resource="http://www.usgs.gov/science/USGSThesaurus/geochemical%20processes"/>
    <skos:related rdf:resource="http://www.usgs.gov/science/USGSThesaurus/marine%20chemistry"/>
    <skos:related rdf:resource="http://www.usgs.gov/science/USGSThesaurus/effects%20of%20climate%20change"/>
    <skos:related rdf:resource="http://www.usgs.gov/science/USGSThesaurus/ocean%20processes"/>
    <skos:inScheme rdf:resource="http://www.usgs.gov/science/USGSThesaurus"/>
  </rdf:Description>
  <rdf:Description about="http://www.usgs.gov/science/USGSThesaurus/ore%20formation">
    <rdf:type rdf:resource="http://www.w3.org/2004/02/skos/core#Concept"/>
    <skos:prefLabel xml:lang="en">ore formation</skos:prefLabel>
    <skos:scopeNote xml:lang="en">Geochemical processes resulting in concentration of useful chemical elements and compounds, in earth materials.  Typically refers to metal ores.</skos:scopeNote>
    <skos:altLabel xml:lang="en">metallogeny</skos:altLabel>
    <skos:broader rdf:resource="http://www.usgs.gov/science/USGSThesaurus/geochemical%20processes"/>
    <skos:inScheme rdf:resource="http://www.usgs.gov/science/USGSThesaurus"/>
  </rdf:Description>
  <rdf:Description about="http://www.usgs.gov/science/USGSThesaurus/oxidation%20and%20reduction">
    <rdf:type rdf:resource="http://www.w3.org/2004/02/skos/core#Concept"/>
    <skos:prefLabel xml:lang="en">oxidation and reduction</skos:prefLabel>
    <skos:scopeNote xml:lang="en">Addition or reduction of oxygen in a compound accompanied by exchange of electrons among atoms.</skos:scopeNote>
    <skos:altLabel xml:lang="en">fermentation</skos:altLabel>
    <skos:broader rdf:resource="http://www.usgs.gov/science/USGSThesaurus/geochemical%20processes"/>
    <skos:inScheme rdf:resource="http://www.usgs.gov/science/USGSThesaurus"/>
  </rdf:Description>
  <rdf:Description about="http://www.usgs.gov/science/USGSThesaurus/reaction%20transport">
    <rdf:type rdf:resource="http://www.w3.org/2004/02/skos/core#Concept"/>
    <skos:prefLabel xml:lang="en">reaction transport</skos:prefLabel>
    <skos:scopeNote xml:lang="en">Chemical reactions occurring during ground-water flow.</skos:scopeNote>
    <skos:broader rdf:resource="http://www.usgs.gov/science/USGSThesaurus/geochemical%20processes"/>
    <skos:related rdf:resource="http://www.usgs.gov/science/USGSThesaurus/groundwater%20flow"/>
    <skos:inScheme rdf:resource="http://www.usgs.gov/science/USGSThesaurus"/>
  </rdf:Description>
  <rdf:Description about="http://www.usgs.gov/science/USGSThesaurus/sorption">
    <rdf:type rdf:resource="http://www.w3.org/2004/02/skos/core#Concept"/>
    <skos:prefLabel xml:lang="en">sorption</skos:prefLabel>
    <skos:scopeNote xml:lang="en">Attachment of chemical substances to materials, either externally (by adsorption) or internally (by absorption).</skos:scopeNote>
    <skos:altLabel xml:lang="en">adsorption</skos:altLabel>
    <skos:altLabel xml:lang="en">absorption</skos:altLabel>
    <skos:broader rdf:resource="http://www.usgs.gov/science/USGSThesaurus/geochemical%20processes"/>
    <skos:inScheme rdf:resource="http://www.usgs.gov/science/USGSThesaurus"/>
  </rdf:Description>
  <rdf:Description about="http://www.usgs.gov/science/USGSThesaurus/geologic%20processes">
    <rdf:type rdf:resource="http://www.w3.org/2004/02/skos/core#Concept"/>
    <skos:prefLabel xml:lang="en">geologic processes</skos:prefLabel>
    <skos:scopeNote xml:lang="en">All types of processes involving geological structures.</skos:scopeNote>
    <skos:altLabel xml:lang="en">lithification</skos:altLabel>
    <skos:broader rdf:resource="http://www.usgs.gov/science/USGSThesaurus/biological%20and%20physical%20processes"/>
    <skos:narrower rdf:resource="http://www.usgs.gov/science/USGSThesaurus/deformation%20%28geologic%29"/>
    <skos:narrower rdf:resource="http://www.usgs.gov/science/USGSThesaurus/diagenesis"/>
    <skos:narrower rdf:resource="http://www.usgs.gov/science/USGSThesaurus/earth%20tides"/>
    <skos:narrower rdf:resource="http://www.usgs.gov/science/USGSThesaurus/earthquakes"/>
    <skos:narrower rdf:resource="http://www.usgs.gov/science/USGSThesaurus/erosion"/>
    <skos:narrower rdf:resource="http://www.usgs.gov/science/USGSThesaurus/glaciation"/>
    <skos:narrower rdf:resource="http://www.usgs.gov/science/USGSThesaurus/heat%20flow%20%28earth%29"/>
    <skos:narrower rdf:resource="http://www.usgs.gov/science/USGSThesaurus/hydrothermal%20processes"/>
    <skos:narrower rdf:resource="http://www.usgs.gov/science/USGSThesaurus/isostasy"/>
    <skos:narrower rdf:resource="http://www.usgs.gov/science/USGSThesaurus/liquefaction"/>
    <skos:narrower rdf:resource="http://www.usgs.gov/science/USGSThesaurus/magnetic%20storms"/>
    <skos:narrower rdf:resource="http://www.usgs.gov/science/USGSThesaurus/metamorphism%20%28geological%29"/>
    <skos:narrower rdf:resource="http://www.usgs.gov/science/USGSThesaurus/sediment%20transport"/>
    <skos:narrower rdf:resource="http://www.usgs.gov/science/USGSThesaurus/sedimentation"/>
    <skos:narrower rdf:resource="http://www.usgs.gov/science/USGSThesaurus/slope%20processes"/>
    <skos:narrower rdf:resource="http://www.usgs.gov/science/USGSThesaurus/soil%20formation"/>
    <skos:narrower rdf:resource="http://www.usgs.gov/science/USGSThesaurus/subsidence"/>
    <skos:narrower rdf:resource="http://www.usgs.gov/science/USGSThesaurus/tectonic%20processes"/>
    <skos:narrower rdf:resource="http://www.usgs.gov/science/USGSThesaurus/uplift"/>
    <skos:narrower rdf:resource="http://www.usgs.gov/science/USGSThesaurus/volcanic%20activity"/>
    <skos:related rdf:resource="http://www.usgs.gov/science/USGSThesaurus/geology"/>
    <skos:related rdf:resource="http://www.usgs.gov/science/USGSThesaurus/hydrology"/>
    <skos:related rdf:resource="http://www.usgs.gov/science/USGSThesaurus/tsunamis"/>
    <skos:inScheme rdf:resource="http://www.usgs.gov/science/USGSThesaurus"/>
  </rdf:Description>
  <rdf:Description about="http://www.usgs.gov/science/USGSThesaurus/deformation%20%28geologic%29">
    <rdf:type rdf:resource="http://www.w3.org/2004/02/skos/core#Concept"/>
    <skos:prefLabel xml:lang="en">deformation (geologic)</skos:prefLabel>
    <skos:scopeNote xml:lang="en">Change in form and structure of geologic materials in response to stress, typically heat and pressure.</skos:scopeNote>
    <skos:altLabel xml:lang="en">rheology</skos:altLabel>
    <skos:altLabel xml:lang="en">strain history</skos:altLabel>
    <skos:broader rdf:resource="http://www.usgs.gov/science/USGSThesaurus/geologic%20processes"/>
    <skos:narrower rdf:resource="http://www.usgs.gov/science/USGSThesaurus/folding%20%28geologic%29"/>
    <skos:narrower rdf:resource="http://www.usgs.gov/science/USGSThesaurus/fracture%20%28geologic%29"/>
    <skos:related rdf:resource="http://www.usgs.gov/science/USGSThesaurus/geologic%20structure"/>
    <skos:inScheme rdf:resource="http://www.usgs.gov/science/USGSThesaurus"/>
  </rdf:Description>
  <rdf:Description about="http://www.usgs.gov/science/USGSThesaurus/folding%20%28geologic%29">
    <rdf:type rdf:resource="http://www.w3.org/2004/02/skos/core#Concept"/>
    <skos:prefLabel xml:lang="en">folding (geologic)</skos:prefLabel>
    <skos:scopeNote xml:lang="en">A property of geologic structures to bend or curve from the planar layers.</skos:scopeNote>
    <skos:altLabel xml:lang="en">crenulation (geologic)</skos:altLabel>
    <skos:altLabel xml:lang="en">geologic folding</skos:altLabel>
    <skos:broader rdf:resource="http://www.usgs.gov/science/USGSThesaurus/deformation%20%28geologic%29"/>
    <skos:related rdf:resource="http://www.usgs.gov/science/USGSThesaurus/structural%20geology"/>
    <skos:related rdf:resource="http://www.usgs.gov/science/USGSThesaurus/tectonic%20processes"/>
    <skos:inScheme rdf:resource="http://www.usgs.gov/science/USGSThesaurus"/>
  </rdf:Description>
  <rdf:Description about="http://www.usgs.gov/science/USGSThesaurus/fracture%20%28geologic%29">
    <rdf:type rdf:resource="http://www.w3.org/2004/02/skos/core#Concept"/>
    <skos:prefLabel xml:lang="en">fracture (geologic)</skos:prefLabel>
    <skos:scopeNote xml:lang="en">Break in a geologic structure including cracks, joints, and faults.</skos:scopeNote>
    <skos:altLabel xml:lang="en">cleavage (rock)</skos:altLabel>
    <skos:altLabel xml:lang="en">jointing (geologic)</skos:altLabel>
    <skos:broader rdf:resource="http://www.usgs.gov/science/USGSThesaurus/deformation%20%28geologic%29"/>
    <skos:narrower rdf:resource="http://www.usgs.gov/science/USGSThesaurus/faulting%20%28geologic%29"/>
    <skos:related rdf:resource="http://www.usgs.gov/science/USGSThesaurus/structural%20geology"/>
    <skos:related rdf:resource="http://www.usgs.gov/science/USGSThesaurus/tectonic%20processes"/>
    <skos:inScheme rdf:resource="http://www.usgs.gov/science/USGSThesaurus"/>
  </rdf:Description>
  <rdf:Description about="http://www.usgs.gov/science/USGSThesaurus/faulting%20%28geologic%29">
    <rdf:type rdf:resource="http://www.w3.org/2004/02/skos/core#Concept"/>
    <skos:prefLabel xml:lang="en">faulting (geologic)</skos:prefLabel>
    <skos:scopeNote xml:lang="en">Movement of earth materials along fracture surfaces.</skos:scopeNote>
    <skos:altLabel xml:lang="en">geologic faulting</skos:altLabel>
    <skos:broader rdf:resource="http://www.usgs.gov/science/USGSThesaurus/fracture%20%28geologic%29"/>
    <skos:inScheme rdf:resource="http://www.usgs.gov/science/USGSThesaurus"/>
  </rdf:Description>
  <rdf:Description about="http://www.usgs.gov/science/USGSThesaurus/diagenesis">
    <rdf:type rdf:resource="http://www.w3.org/2004/02/skos/core#Concept"/>
    <skos:prefLabel xml:lang="en">diagenesis</skos:prefLabel>
    <skos:scopeNote xml:lang="en">Chemical, physical, and biological changes in sediment during and after its conversion to rock (lithification).</skos:scopeNote>
    <skos:broader rdf:resource="http://www.usgs.gov/science/USGSThesaurus/geologic%20processes"/>
    <skos:related rdf:resource="http://www.usgs.gov/science/USGSThesaurus/petrology"/>
    <skos:related rdf:resource="http://www.usgs.gov/science/USGSThesaurus/sedimentology"/>
    <skos:inScheme rdf:resource="http://www.usgs.gov/science/USGSThesaurus"/>
  </rdf:Description>
  <rdf:Description about="http://www.usgs.gov/science/USGSThesaurus/earth%20tides">
    <rdf:type rdf:resource="http://www.w3.org/2004/02/skos/core#Concept"/>
    <skos:prefLabel xml:lang="en">earth tides</skos:prefLabel>
    <skos:scopeNote xml:lang="en">Periodic changes in the earth surface topography caused by the gravitational attraction of the moon and sun, measured with tiltmeters.  Used in studies of volcanic activity.</skos:scopeNote>
    <skos:broader rdf:resource="http://www.usgs.gov/science/USGSThesaurus/geologic%20processes"/>
    <skos:inScheme rdf:resource="http://www.usgs.gov/science/USGSThesaurus"/>
  </rdf:Description>
  <rdf:Description about="http://www.usgs.gov/science/USGSThesaurus/earthquakes">
    <rdf:type rdf:resource="http://www.w3.org/2004/02/skos/core#Concept"/>
    <skos:prefLabel xml:lang="en">earthquakes</skos:prefLabel>
    <skos:scopeNote xml:lang="en">Ground shaking caused by the sudden release of accumulated strain by an abrupt shift of rock along a fracture in the earth or by volcanic or magmatic activity, or other sudden stress changes in the earth.</skos:scopeNote>
    <!--FOR earthquake hazards USE earthquakes WITH hazards-->
    <skos:altLabel xml:lang="en">earthquake hazards</skos:altLabel>
    <skos:broader rdf:resource="http://www.usgs.gov/science/USGSThesaurus/geologic%20processes"/>
    <skos:narrower rdf:resource="http://www.usgs.gov/science/USGSThesaurus/earthquake%20occurrences"/>
    <skos:related rdf:resource="http://www.usgs.gov/science/USGSThesaurus/tsunamis"/>
    <skos:related rdf:resource="http://www.usgs.gov/science/USGSThesaurus/earthquake%20probabilities"/>
    <skos:related rdf:resource="http://www.usgs.gov/science/USGSThesaurus/hazards"/>
    <skos:related rdf:resource="http://www.usgs.gov/science/USGSThesaurus/seismology"/>
    <skos:related rdf:resource="http://www.usgs.gov/science/USGSThesaurus/tectonic%20processes"/>
    <skos:related rdf:resource="http://www.usgs.gov/science/USGSThesaurus/tectonophysics"/>
    <skos:related rdf:resource="http://www.usgs.gov/science/USGSThesaurus/volcanic%20activity"/>
    <skos:inScheme rdf:resource="http://www.usgs.gov/science/USGSThesaurus"/>
  </rdf:Description>
  <rdf:Description about="http://www.usgs.gov/science/USGSThesaurus/earthquake%20occurrences">
    <rdf:type rdf:resource="http://www.w3.org/2004/02/skos/core#Concept"/>
    <skos:prefLabel xml:lang="en">earthquake occurrences</skos:prefLabel>
    <skos:scopeNote xml:lang="en">Time, location, severity, and mechanism of earthquake events, including the frequency and history of events in a given area.</skos:scopeNote>
    <!--FOR earthquake occurrence maps USE earthquake occurrences WITH maps and atlases-->
    <skos:altLabel xml:lang="en">earthquake occurrence maps</skos:altLabel>
    <!--FOR earthquake seismology USE earthquake occurrences WITH seismology-->
    <skos:altLabel xml:lang="en">earthquake seismology</skos:altLabel>
    <skos:altLabel xml:lang="en">seismic activity</skos:altLabel>
    <!--FOR earthquake activity maps USE earthquake occurrences WITH maps and atlases-->
    <skos:altLabel xml:lang="en">earthquake activity maps</skos:altLabel>
    <!--FOR earthquake epicenter maps USE earthquake occurrences WITH maps and atlases-->
    <skos:altLabel xml:lang="en">earthquake epicenter maps</skos:altLabel>
    <!--FOR ground motion maps USE earthquake occurrences WITH maps and atlases-->
    <skos:altLabel xml:lang="en">ground motion maps</skos:altLabel>
    <!--FOR seismic hazard maps USE earthquake occurrences WITH maps and atlases-->
    <skos:altLabel xml:lang="en">seismic hazard maps</skos:altLabel>
    <!--FOR shaking maps (seismic) USE earthquake occurrences WITH maps and atlases-->
    <skos:altLabel xml:lang="en">shaking maps (seismic)</skos:altLabel>
    <skos:altLabel xml:lang="en">seismicity</skos:altLabel>
    <skos:altLabel xml:lang="en">strong motion</skos:altLabel>
    <skos:altLabel xml:lang="en">ground motion</skos:altLabel>
    <skos:broader rdf:resource="http://www.usgs.gov/science/USGSThesaurus/earthquakes"/>
    <skos:related rdf:resource="http://www.usgs.gov/science/USGSThesaurus/seismology"/>
    <skos:inScheme rdf:resource="http://www.usgs.gov/science/USGSThesaurus"/>
  </rdf:Description>
  <rdf:Description about="http://www.usgs.gov/science/USGSThesaurus/erosion">
    <rdf:type rdf:resource="http://www.w3.org/2004/02/skos/core#Concept"/>
    <skos:prefLabel xml:lang="en">erosion</skos:prefLabel>
    <skos:scopeNote xml:lang="en">The process whereby materials of the earth's crust are loosened, dissolved, or worn away and simultaneously moved from one place to another.</skos:scopeNote>
    <!--FOR shoreline erosion USE erosion WITH coastal processes-->
    <skos:altLabel xml:lang="en">shoreline erosion</skos:altLabel>
    <!--FOR coastal erosion USE erosion WITH coastal processes-->
    <skos:altLabel xml:lang="en">coastal erosion</skos:altLabel>
    <!--FOR beach erosion USE erosion WITH coastal processes-->
    <skos:altLabel xml:lang="en">beach erosion</skos:altLabel>
    <!--FOR shoreline retreat USE erosion WITH coastal processes-->
    <skos:altLabel xml:lang="en">shoreline retreat</skos:altLabel>
    <!--FOR wind erosion USE erosion WITH wind-->
    <skos:altLabel xml:lang="en">wind erosion</skos:altLabel>
    <skos:altLabel xml:lang="en">dissolution</skos:altLabel>
    <skos:broader rdf:resource="http://www.usgs.gov/science/USGSThesaurus/geologic%20processes"/>
    <skos:narrower rdf:resource="http://www.usgs.gov/science/USGSThesaurus/sinkhole%20formation"/>
    <skos:related rdf:resource="http://www.usgs.gov/science/USGSThesaurus/geomorphology"/>
    <skos:related rdf:resource="http://www.usgs.gov/science/USGSThesaurus/glaciology"/>
    <skos:related rdf:resource="http://www.usgs.gov/science/USGSThesaurus/hydrology"/>
    <skos:related rdf:resource="http://www.usgs.gov/science/USGSThesaurus/sedimentology"/>
    <skos:related rdf:resource="http://www.usgs.gov/science/USGSThesaurus/watershed%20management"/>
    <skos:related rdf:resource="http://www.usgs.gov/science/USGSThesaurus/scour"/>
    <skos:inScheme rdf:resource="http://www.usgs.gov/science/USGSThesaurus"/>
  </rdf:Description>
  <rdf:Description about="http://www.usgs.gov/science/USGSThesaurus/sinkhole%20formation">
    <rdf:type rdf:resource="http://www.w3.org/2004/02/skos/core#Concept"/>
    <skos:prefLabel xml:lang="en">sinkhole formation</skos:prefLabel>
    <skos:scopeNote xml:lang="en">Localized collapse of the land surface usually due to erosion of the underlying materials.  Most commonly occurring in karst areas, but similar effects occur due to physical erosion in other terranes.</skos:scopeNote>
    <skos:broader rdf:resource="http://www.usgs.gov/science/USGSThesaurus/erosion"/>
    <skos:related rdf:resource="http://www.usgs.gov/science/USGSThesaurus/karst"/>
    <skos:inScheme rdf:resource="http://www.usgs.gov/science/USGSThesaurus"/>
  </rdf:Description>
  <rdf:Description about="http://www.usgs.gov/science/USGSThesaurus/glaciation">
    <rdf:type rdf:resource="http://www.w3.org/2004/02/skos/core#Concept"/>
    <skos:prefLabel xml:lang="en">glaciation</skos:prefLabel>
    <skos:scopeNote xml:lang="en">The geologic processes involved in the formation, movement, changes, and effects of large ice masses (glaciers).</skos:scopeNote>
    <skos:broader rdf:resource="http://www.usgs.gov/science/USGSThesaurus/geologic%20processes"/>
    <skos:related rdf:resource="http://www.usgs.gov/science/USGSThesaurus/foliation%20%28geologic%29"/>
    <skos:related rdf:resource="http://www.usgs.gov/science/USGSThesaurus/glaciology"/>
    <skos:related rdf:resource="http://www.usgs.gov/science/USGSThesaurus/snow%20and%20ice%20cover"/>
    <skos:inScheme rdf:resource="http://www.usgs.gov/science/USGSThesaurus"/>
  </rdf:Description>
  <rdf:Description about="http://www.usgs.gov/science/USGSThesaurus/heat%20flow%20%28earth%29">
    <rdf:type rdf:resource="http://www.w3.org/2004/02/skos/core#Concept"/>
    <skos:prefLabel xml:lang="en">heat flow (earth)</skos:prefLabel>
    <skos:scopeNote xml:lang="en">Energy transferred by a difference in temperature through the surface of the earth.</skos:scopeNote>
    <skos:altLabel xml:lang="en">geothermics</skos:altLabel>
    <skos:altLabel xml:lang="en">heatflow (earth)</skos:altLabel>
    <skos:broader rdf:resource="http://www.usgs.gov/science/USGSThesaurus/geologic%20processes"/>
    <skos:related rdf:resource="http://www.usgs.gov/science/USGSThesaurus/geophysics"/>
    <skos:inScheme rdf:resource="http://www.usgs.gov/science/USGSThesaurus"/>
  </rdf:Description>
  <rdf:Description about="http://www.usgs.gov/science/USGSThesaurus/hydrothermal%20processes">
    <rdf:type rdf:resource="http://www.w3.org/2004/02/skos/core#Concept"/>
    <skos:prefLabel xml:lang="en">hydrothermal processes</skos:prefLabel>
    <skos:scopeNote xml:lang="en">Natural phenomena relating to heated water generated by igneous activity.</skos:scopeNote>
    <skos:broader rdf:resource="http://www.usgs.gov/science/USGSThesaurus/geologic%20processes"/>
    <skos:related rdf:resource="http://www.usgs.gov/science/USGSThesaurus/hydrogeology"/>
    <skos:related rdf:resource="http://www.usgs.gov/science/USGSThesaurus/hydrology"/>
    <skos:inScheme rdf:resource="http://www.usgs.gov/science/USGSThesaurus"/>
  </rdf:Description>
  <rdf:Description about="http://www.usgs.gov/science/USGSThesaurus/isostasy">
    <rdf:type rdf:resource="http://www.w3.org/2004/02/skos/core#Concept"/>
    <skos:prefLabel xml:lang="en">isostasy</skos:prefLabel>
    <skos:scopeNote xml:lang="en">Condition of equilibrium or buoyancy of the earth's crust above the mantle.</skos:scopeNote>
    <skos:broader rdf:resource="http://www.usgs.gov/science/USGSThesaurus/geologic%20processes"/>
    <skos:related rdf:resource="http://www.usgs.gov/science/USGSThesaurus/geophysics"/>
    <skos:related rdf:resource="http://www.usgs.gov/science/USGSThesaurus/glaciology"/>
    <skos:inScheme rdf:resource="http://www.usgs.gov/science/USGSThesaurus"/>
  </rdf:Description>
  <rdf:Description about="http://www.usgs.gov/science/USGSThesaurus/liquefaction">
    <rdf:type rdf:resource="http://www.w3.org/2004/02/skos/core#Concept"/>
    <skos:prefLabel xml:lang="en">liquefaction</skos:prefLabel>
    <skos:scopeNote xml:lang="en">Physical process which can occur during an earthquake.  Clay-free soil deposits (primarily sands and silts)temporarily lose strength and behave as viscuous fluids, resulting in ground failure.</skos:scopeNote>
    <skos:broader rdf:resource="http://www.usgs.gov/science/USGSThesaurus/geologic%20processes"/>
    <skos:related rdf:resource="http://www.usgs.gov/science/USGSThesaurus/engineering%20geology"/>
    <skos:related rdf:resource="http://www.usgs.gov/science/USGSThesaurus/hazards"/>
    <skos:inScheme rdf:resource="http://www.usgs.gov/science/USGSThesaurus"/>
  </rdf:Description>
  <rdf:Description about="http://www.usgs.gov/science/USGSThesaurus/magnetic%20storms">
    <rdf:type rdf:resource="http://www.w3.org/2004/02/skos/core#Concept"/>
    <skos:prefLabel xml:lang="en">magnetic storms</skos:prefLabel>
    <skos:scopeNote xml:lang="en">A period of time during which the earth's magnetic field varies rapidly.  During magnetic storms, satellite electronics can be damaged through the build up and subsequent discharge of static electric charges and astronauts and high-altitude pilots can be subjected to increased levels of radiation.</skos:scopeNote>
    <skos:altLabel xml:lang="en">geomagnetic storms</skos:altLabel>
    <skos:broader rdf:resource="http://www.usgs.gov/science/USGSThesaurus/geologic%20processes"/>
    <skos:related rdf:resource="http://www.usgs.gov/science/USGSThesaurus/hazards"/>
    <skos:related rdf:resource="http://www.usgs.gov/science/USGSThesaurus/magnetic%20field%20%28earth%29"/>
    <skos:inScheme rdf:resource="http://www.usgs.gov/science/USGSThesaurus"/>
  </rdf:Description>
  <rdf:Description about="http://www.usgs.gov/science/USGSThesaurus/metamorphism%20%28geological%29">
    <rdf:type rdf:resource="http://www.w3.org/2004/02/skos/core#Concept"/>
    <skos:prefLabel xml:lang="en">metamorphism (geological)</skos:prefLabel>
    <skos:scopeNote xml:lang="en">Process by which rocks are altered in composition and texture by extreme heat, high pressure, or the action of chemicals.</skos:scopeNote>
    <skos:broader rdf:resource="http://www.usgs.gov/science/USGSThesaurus/geologic%20processes"/>
    <skos:narrower rdf:resource="http://www.usgs.gov/science/USGSThesaurus/alteration"/>
    <skos:related rdf:resource="http://www.usgs.gov/science/USGSThesaurus/geochemistry"/>
    <skos:related rdf:resource="http://www.usgs.gov/science/USGSThesaurus/geology"/>
    <skos:related rdf:resource="http://www.usgs.gov/science/USGSThesaurus/geophysics"/>
    <skos:related rdf:resource="http://www.usgs.gov/science/USGSThesaurus/metamorphic%20rocks"/>
    <skos:inScheme rdf:resource="http://www.usgs.gov/science/USGSThesaurus"/>
  </rdf:Description>
  <rdf:Description about="http://www.usgs.gov/science/USGSThesaurus/alteration">
    <rdf:type rdf:resource="http://www.w3.org/2004/02/skos/core#Concept"/>
    <skos:prefLabel xml:lang="en">alteration</skos:prefLabel>
    <skos:scopeNote xml:lang="en">Local changes in the mineralogy of a rock body due to low-grade metamorphism, weathering, or both.  May indicate underlying mineral deposits.</skos:scopeNote>
    <skos:broader rdf:resource="http://www.usgs.gov/science/USGSThesaurus/metamorphism%20%28geological%29"/>
    <skos:inScheme rdf:resource="http://www.usgs.gov/science/USGSThesaurus"/>
  </rdf:Description>
  <rdf:Description about="http://www.usgs.gov/science/USGSThesaurus/sediment%20transport">
    <rdf:type rdf:resource="http://www.w3.org/2004/02/skos/core#Concept"/>
    <skos:prefLabel xml:lang="en">sediment transport</skos:prefLabel>
    <skos:scopeNote xml:lang="en">Transport of solid particles of unconsolidated rock and mineral fragments, chemical precipitates, or biological materials.</skos:scopeNote>
    <skos:altLabel xml:lang="en">alluvial transport</skos:altLabel>
    <skos:altLabel xml:lang="en">bed load</skos:altLabel>
    <skos:altLabel xml:lang="en">bedload</skos:altLabel>
    <skos:altLabel xml:lang="en">density flow</skos:altLabel>
    <skos:altLabel xml:lang="en">dust transport</skos:altLabel>
    <skos:altLabel xml:lang="en">suspended load</skos:altLabel>
    <skos:altLabel xml:lang="en">turbidity flow</skos:altLabel>
    <!--FOR marine sediment transport USE sediment transport WITH ocean processes-->
    <skos:altLabel xml:lang="en">marine sediment transport</skos:altLabel>
    <!--FOR longshore drift USE sediment transport WITH longshore currents-->
    <skos:altLabel xml:lang="en">longshore drift</skos:altLabel>
    <!--FOR littoral drift USE sediment transport WITH longshore currents-->
    <skos:altLabel xml:lang="en">littoral drift</skos:altLabel>
    <!--FOR estuarine sediment transport USE sediment transport WITH estuarine processes-->
    <skos:altLabel xml:lang="en">estuarine sediment transport</skos:altLabel>
    <skos:broader rdf:resource="http://www.usgs.gov/science/USGSThesaurus/geologic%20processes"/>
    <skos:related rdf:resource="http://www.usgs.gov/science/USGSThesaurus/hydrology"/>
    <skos:related rdf:resource="http://www.usgs.gov/science/USGSThesaurus/sedimentology"/>
    <skos:inScheme rdf:resource="http://www.usgs.gov/science/USGSThesaurus"/>
  </rdf:Description>
  <rdf:Description about="http://www.usgs.gov/science/USGSThesaurus/sedimentation">
    <rdf:type rdf:resource="http://www.w3.org/2004/02/skos/core#Concept"/>
    <skos:prefLabel xml:lang="en">sedimentation</skos:prefLabel>
    <skos:scopeNote xml:lang="en">Process of deposition of sediments (loose, uncemented pieces of rock, mineral fragments, or biological materials).  The sediments settle out of water or air into layers on a surface.</skos:scopeNote>
    <skos:altLabel xml:lang="en">alluvial sedimentation</skos:altLabel>
    <skos:altLabel xml:lang="en">deposition (sediment)</skos:altLabel>
    <skos:altLabel xml:lang="en">dust deposition</skos:altLabel>
    <skos:broader rdf:resource="http://www.usgs.gov/science/USGSThesaurus/geologic%20processes"/>
    <skos:related rdf:resource="http://www.usgs.gov/science/USGSThesaurus/sedimentary%20rocks"/>
    <skos:related rdf:resource="http://www.usgs.gov/science/USGSThesaurus/sedimentology"/>
    <skos:related rdf:resource="http://www.usgs.gov/science/USGSThesaurus/atmospheric%20deposition%20%28chemical%20%26%20particulate%29"/>
    <skos:inScheme rdf:resource="http://www.usgs.gov/science/USGSThesaurus"/>
  </rdf:Description>
  <rdf:Description about="http://www.usgs.gov/science/USGSThesaurus/slope%20processes">
    <rdf:type rdf:resource="http://www.w3.org/2004/02/skos/core#Concept"/>
    <skos:prefLabel xml:lang="en">slope processes</skos:prefLabel>
    <skos:scopeNote xml:lang="en">The down slope movement of earth material under the influence of gravity.</skos:scopeNote>
    <skos:altLabel xml:lang="en">soil creep</skos:altLabel>
    <skos:altLabel xml:lang="en">mass wasting</skos:altLabel>
    <skos:broader rdf:resource="http://www.usgs.gov/science/USGSThesaurus/geologic%20processes"/>
    <skos:narrower rdf:resource="http://www.usgs.gov/science/USGSThesaurus/landslides"/>
    <skos:inScheme rdf:resource="http://www.usgs.gov/science/USGSThesaurus"/>
  </rdf:Description>
  <rdf:Description about="http://www.usgs.gov/science/USGSThesaurus/landslides">
    <rdf:type rdf:resource="http://www.w3.org/2004/02/skos/core#Concept"/>
    <skos:prefLabel xml:lang="en">landslides</skos:prefLabel>
    <skos:scopeNote xml:lang="en">Downslope movement of rock, soil, or artificial fill under the influences of gravity.</skos:scopeNote>
    <skos:altLabel xml:lang="en">avalanches</skos:altLabel>
    <skos:altLabel xml:lang="en">debris avalanches</skos:altLabel>
    <skos:altLabel xml:lang="en">debris flows</skos:altLabel>
    <!--FOR landslide maps USE landslides WITH maps and atlases-->
    <skos:altLabel xml:lang="en">landslide maps</skos:altLabel>
    <!--FOR landslide preparedness USE landslides WITH hazard preparedness-->
    <skos:altLabel xml:lang="en">landslide preparedness</skos:altLabel>
    <skos:altLabel xml:lang="en">rockfalls</skos:altLabel>
    <skos:altLabel xml:lang="en">slides (land)</skos:altLabel>
    <skos:altLabel xml:lang="en">slumps</skos:altLabel>
    <skos:altLabel xml:lang="en">earth flows</skos:altLabel>
    <skos:altLabel xml:lang="en">mudslides</skos:altLabel>
    <skos:broader rdf:resource="http://www.usgs.gov/science/USGSThesaurus/slope%20processes"/>
    <skos:narrower rdf:resource="http://www.usgs.gov/science/USGSThesaurus/lahars"/>
    <skos:related rdf:resource="http://www.usgs.gov/science/USGSThesaurus/geomorphology"/>
    <skos:related rdf:resource="http://www.usgs.gov/science/USGSThesaurus/hazards"/>
    <skos:related rdf:resource="http://www.usgs.gov/science/USGSThesaurus/landslide%20susceptibility%20assessment"/>
    <skos:inScheme rdf:resource="http://www.usgs.gov/science/USGSThesaurus"/>
  </rdf:Description>
  <rdf:Description about="http://www.usgs.gov/science/USGSThesaurus/lahars">
    <rdf:type rdf:resource="http://www.w3.org/2004/02/skos/core#Concept"/>
    <skos:prefLabel xml:lang="en">lahars</skos:prefLabel>
    <skos:scopeNote xml:lang="en">Downslope flow of ash and rock debris resulting from volcanic activity.</skos:scopeNote>
    <skos:broader rdf:resource="http://www.usgs.gov/science/USGSThesaurus/landslides"/>
    <skos:related rdf:resource="http://www.usgs.gov/science/USGSThesaurus/volcanic%20activity"/>
    <skos:inScheme rdf:resource="http://www.usgs.gov/science/USGSThesaurus"/>
  </rdf:Description>
  <rdf:Description about="http://www.usgs.gov/science/USGSThesaurus/soil%20formation">
    <rdf:type rdf:resource="http://www.w3.org/2004/02/skos/core#Concept"/>
    <skos:prefLabel xml:lang="en">soil formation</skos:prefLabel>
    <skos:scopeNote xml:lang="en">Geological, geochemical, and ecological processes that work together to produce soils.</skos:scopeNote>
    <skos:altLabel xml:lang="en">pedogenesis</skos:altLabel>
    <skos:broader rdf:resource="http://www.usgs.gov/science/USGSThesaurus/geologic%20processes"/>
    <skos:related rdf:resource="http://www.usgs.gov/science/USGSThesaurus/ecological%20processes"/>
    <skos:related rdf:resource="http://www.usgs.gov/science/USGSThesaurus/geochemical%20processes"/>
    <skos:related rdf:resource="http://www.usgs.gov/science/USGSThesaurus/soil%20horizons"/>
    <skos:inScheme rdf:resource="http://www.usgs.gov/science/USGSThesaurus"/>
  </rdf:Description>
  <rdf:Description about="http://www.usgs.gov/science/USGSThesaurus/subsidence">
    <rdf:type rdf:resource="http://www.w3.org/2004/02/skos/core#Concept"/>
    <skos:prefLabel xml:lang="en">subsidence</skos:prefLabel>
    <skos:scopeNote xml:lang="en">Settling, compaction, or caving in of land caused by subsurface mining, ground-water withdrawal, or pumping of oil and gas.</skos:scopeNote>
    <!--FOR land subsidence maps USE subsidence WITH maps and atlases-->
    <skos:altLabel xml:lang="en">land subsidence maps</skos:altLabel>
    <skos:altLabel xml:lang="en">land subsidence</skos:altLabel>
    <skos:broader rdf:resource="http://www.usgs.gov/science/USGSThesaurus/geologic%20processes"/>
    <skos:related rdf:resource="http://www.usgs.gov/science/USGSThesaurus/geomorphology"/>
    <skos:related rdf:resource="http://www.usgs.gov/science/USGSThesaurus/human%20impacts"/>
    <skos:inScheme rdf:resource="http://www.usgs.gov/science/USGSThesaurus"/>
  </rdf:Description>
  <rdf:Description about="http://www.usgs.gov/science/USGSThesaurus/tectonic%20processes">
    <rdf:type rdf:resource="http://www.w3.org/2004/02/skos/core#Concept"/>
    <skos:prefLabel xml:lang="en">tectonic processes</skos:prefLabel>
    <skos:scopeNote xml:lang="en">The structural forces affecting the deformation, uplift, and movement of the earth's crust.</skos:scopeNote>
    <skos:altLabel xml:lang="en">continental drift</skos:altLabel>
    <skos:altLabel xml:lang="en">dynamic geology</skos:altLabel>
    <!--FOR paleotectonic maps USE tectonic processes WITH maps and atlases-->
    <skos:altLabel xml:lang="en">paleotectonic maps</skos:altLabel>
    <skos:altLabel xml:lang="en">plate tectonics</skos:altLabel>
    <skos:altLabel xml:lang="en">subduction</skos:altLabel>
    <!--FOR tectonic maps USE tectonic processes WITH maps and atlases-->
    <skos:altLabel xml:lang="en">tectonic maps</skos:altLabel>
    <skos:altLabel xml:lang="en">tectonics</skos:altLabel>
    <skos:altLabel xml:lang="en">wilson cycle</skos:altLabel>
    <skos:broader rdf:resource="http://www.usgs.gov/science/USGSThesaurus/geologic%20processes"/>
    <skos:narrower rdf:resource="http://www.usgs.gov/science/USGSThesaurus/neotectonic%20processes"/>
    <skos:related rdf:resource="http://www.usgs.gov/science/USGSThesaurus/earth%20structure"/>
    <skos:related rdf:resource="http://www.usgs.gov/science/USGSThesaurus/earthquakes"/>
    <skos:related rdf:resource="http://www.usgs.gov/science/USGSThesaurus/folding%20%28geologic%29"/>
    <skos:related rdf:resource="http://www.usgs.gov/science/USGSThesaurus/foliation%20%28geologic%29"/>
    <skos:related rdf:resource="http://www.usgs.gov/science/USGSThesaurus/fracture%20%28geologic%29"/>
    <skos:related rdf:resource="http://www.usgs.gov/science/USGSThesaurus/lineation%20%28geologic%29"/>
    <skos:related rdf:resource="http://www.usgs.gov/science/USGSThesaurus/seismology"/>
    <skos:related rdf:resource="http://www.usgs.gov/science/USGSThesaurus/structural%20geology"/>
    <skos:related rdf:resource="http://www.usgs.gov/science/USGSThesaurus/tectonophysics"/>
    <skos:related rdf:resource="http://www.usgs.gov/science/USGSThesaurus/volcanic%20activity"/>
    <skos:inScheme rdf:resource="http://www.usgs.gov/science/USGSThesaurus"/>
  </rdf:Description>
  <rdf:Description about="http://www.usgs.gov/science/USGSThesaurus/neotectonic%20processes">
    <rdf:type rdf:resource="http://www.w3.org/2004/02/skos/core#Concept"/>
    <skos:prefLabel xml:lang="en">neotectonic processes</skos:prefLabel>
    <skos:scopeNote xml:lang="en">Changes which took place during geological time after the Miocene era and are associated with the structural forces that affect the deformation, uplift, and movement occurring in the earth's crust.</skos:scopeNote>
    <skos:altLabel xml:lang="en">neotectonics</skos:altLabel>
    <skos:broader rdf:resource="http://www.usgs.gov/science/USGSThesaurus/tectonic%20processes"/>
    <skos:related rdf:resource="http://www.usgs.gov/science/USGSThesaurus/earthquake%20probabilities"/>
    <skos:related rdf:resource="http://www.usgs.gov/science/USGSThesaurus/structural%20geology"/>
    <skos:related rdf:resource="http://www.usgs.gov/science/USGSThesaurus/tectonophysics"/>
    <skos:inScheme rdf:resource="http://www.usgs.gov/science/USGSThesaurus"/>
  </rdf:Description>
  <rdf:Description about="http://www.usgs.gov/science/USGSThesaurus/uplift">
    <rdf:type rdf:resource="http://www.w3.org/2004/02/skos/core#Concept"/>
    <skos:prefLabel xml:lang="en">uplift</skos:prefLabel>
    <skos:scopeNote xml:lang="en">Local or regional rise in the elevation of the land surface, usually due to tectonic or volcanic processes.</skos:scopeNote>
    <skos:broader rdf:resource="http://www.usgs.gov/science/USGSThesaurus/geologic%20processes"/>
    <skos:inScheme rdf:resource="http://www.usgs.gov/science/USGSThesaurus"/>
  </rdf:Description>
  <rdf:Description about="http://www.usgs.gov/science/USGSThesaurus/volcanic%20activity">
    <rdf:type rdf:resource="http://www.w3.org/2004/02/skos/core#Concept"/>
    <skos:prefLabel xml:lang="en">volcanic activity</skos:prefLabel>
    <skos:scopeNote xml:lang="en">Episodes during which gases, ash, and lava (molten rock) escape from vents in the earth's crust, accompanied by minor tremors.</skos:scopeNote>
    <skos:altLabel xml:lang="en">eruption</skos:altLabel>
    <skos:altLabel xml:lang="en">lava flows</skos:altLabel>
    <skos:altLabel xml:lang="en">pyroclastic flows</skos:altLabel>
    <skos:altLabel xml:lang="en">volcanism</skos:altLabel>
    <!--FOR volcano monitoring USE volcanic activity WITH field inventory and monitoring-->
    <skos:altLabel xml:lang="en">volcano monitoring</skos:altLabel>
    <skos:altLabel xml:lang="en">volcanic tremors</skos:altLabel>
    <skos:broader rdf:resource="http://www.usgs.gov/science/USGSThesaurus/geologic%20processes"/>
    <skos:narrower rdf:resource="http://www.usgs.gov/science/USGSThesaurus/volcanic%20gas%20emission"/>
    <skos:related rdf:resource="http://www.usgs.gov/science/USGSThesaurus/hazards"/>
    <skos:related rdf:resource="http://www.usgs.gov/science/USGSThesaurus/tectonic%20processes"/>
    <skos:related rdf:resource="http://www.usgs.gov/science/USGSThesaurus/volcanology"/>
    <skos:related rdf:resource="http://www.usgs.gov/science/USGSThesaurus/lahars"/>
    <skos:related rdf:resource="http://www.usgs.gov/science/USGSThesaurus/aviation%20safety"/>
    <skos:related rdf:resource="http://www.usgs.gov/science/USGSThesaurus/volcanic%20eruption%20prediction"/>
    <skos:related rdf:resource="http://www.usgs.gov/science/USGSThesaurus/earthquakes"/>
    <skos:inScheme rdf:resource="http://www.usgs.gov/science/USGSThesaurus"/>
  </rdf:Description>
  <rdf:Description about="http://www.usgs.gov/science/USGSThesaurus/volcanic%20gas%20emission">
    <rdf:type rdf:resource="http://www.w3.org/2004/02/skos/core#Concept"/>
    <skos:prefLabel xml:lang="en">volcanic gas emission</skos:prefLabel>
    <skos:scopeNote xml:lang="en">Emission of gases from fumaroles and volcanoes.</skos:scopeNote>
    <skos:altLabel xml:lang="en">fumarolic activity</skos:altLabel>
    <skos:broader rdf:resource="http://www.usgs.gov/science/USGSThesaurus/volcanic%20activity"/>
    <skos:inScheme rdf:resource="http://www.usgs.gov/science/USGSThesaurus"/>
  </rdf:Description>
  <rdf:Description about="http://www.usgs.gov/science/USGSThesaurus/hydrologic%20processes">
    <rdf:type rdf:resource="http://www.w3.org/2004/02/skos/core#Concept"/>
    <skos:prefLabel xml:lang="en">hydrologic processes</skos:prefLabel>
    <skos:scopeNote xml:lang="en"></skos:scopeNote>
    <skos:broader rdf:resource="http://www.usgs.gov/science/USGSThesaurus/biological%20and%20physical%20processes"/>
    <skos:narrower rdf:resource="http://www.usgs.gov/science/USGSThesaurus/floods"/>
    <skos:narrower rdf:resource="http://www.usgs.gov/science/USGSThesaurus/groundwater%20and%20surface-water%20interaction"/>
    <skos:narrower rdf:resource="http://www.usgs.gov/science/USGSThesaurus/groundwater%20flow"/>
    <skos:narrower rdf:resource="http://www.usgs.gov/science/USGSThesaurus/percolation"/>
    <skos:narrower rdf:resource="http://www.usgs.gov/science/USGSThesaurus/runoff"/>
    <skos:narrower rdf:resource="http://www.usgs.gov/science/USGSThesaurus/saltwater%20intrusion"/>
    <skos:narrower rdf:resource="http://www.usgs.gov/science/USGSThesaurus/scour"/>
    <skos:narrower rdf:resource="http://www.usgs.gov/science/USGSThesaurus/streamflow"/>
    <skos:narrower rdf:resource="http://www.usgs.gov/science/USGSThesaurus/water%20circulation"/>
    <skos:narrower rdf:resource="http://www.usgs.gov/science/USGSThesaurus/water%20cycle"/>
    <skos:related rdf:resource="http://www.usgs.gov/science/USGSThesaurus/precipitation%20%28atmospheric%29"/>
    <skos:inScheme rdf:resource="http://www.usgs.gov/science/USGSThesaurus"/>
  </rdf:Description>
  <rdf:Description about="http://www.usgs.gov/science/USGSThesaurus/floods">
    <rdf:type rdf:resource="http://www.w3.org/2004/02/skos/core#Concept"/>
    <skos:prefLabel xml:lang="en">floods</skos:prefLabel>
    <skos:scopeNote xml:lang="en">Relatively high water that overflows the natural or artificial banks of a stream or coastal area that submerges land not normally below water level.</skos:scopeNote>
    <skos:altLabel xml:lang="en">bankfull stage</skos:altLabel>
    <!--FOR flood preparedness USE floods WITH hazard preparedness-->
    <skos:altLabel xml:lang="en">flood preparedness</skos:altLabel>
    <skos:broader rdf:resource="http://www.usgs.gov/science/USGSThesaurus/hydrologic%20processes"/>
    <skos:narrower rdf:resource="http://www.usgs.gov/science/USGSThesaurus/storm%20surge"/>
    <skos:related rdf:resource="http://www.usgs.gov/science/USGSThesaurus/controlled%20flooding"/>
    <skos:related rdf:resource="http://www.usgs.gov/science/USGSThesaurus/hazards"/>
    <skos:related rdf:resource="http://www.usgs.gov/science/USGSThesaurus/hydrology"/>
    <skos:related rdf:resource="http://www.usgs.gov/science/USGSThesaurus/surface%20water%20%28non-marine%29"/>
    <skos:related rdf:resource="http://www.usgs.gov/science/USGSThesaurus/watershed%20management"/>
    <skos:inScheme rdf:resource="http://www.usgs.gov/science/USGSThesaurus"/>
  </rdf:Description>
  <rdf:Description about="http://www.usgs.gov/science/USGSThesaurus/storm%20surge">
    <rdf:type rdf:resource="http://www.w3.org/2004/02/skos/core#Concept"/>
    <skos:prefLabel xml:lang="en">storm surge</skos:prefLabel>
    <skos:scopeNote xml:lang="en">Coastal high water level caused by wind from storms.</skos:scopeNote>
    <skos:broader rdf:resource="http://www.usgs.gov/science/USGSThesaurus/floods"/>
    <skos:related rdf:resource="http://www.usgs.gov/science/USGSThesaurus/coastal%20processes"/>
    <skos:inScheme rdf:resource="http://www.usgs.gov/science/USGSThesaurus"/>
  </rdf:Description>
  <rdf:Description about="http://www.usgs.gov/science/USGSThesaurus/groundwater%20and%20surface-water%20interaction">
    <rdf:type rdf:resource="http://www.w3.org/2004/02/skos/core#Concept"/>
    <skos:prefLabel xml:lang="en">groundwater and surface-water interaction</skos:prefLabel>
    <skos:scopeNote xml:lang="en">Traditionally, management of water resources has focused on surface water or groundwater as if they were separate entities. As development of land and water resources increases, it is apparent that development of either of these resources affects the quantity and quality of the other. Nearly all surface-water features (streams, lakes, reservoirs, wetlands, and estuaries) interact with groundwater. These interactions take many forms. In many situations, surface-water bodies gain water and solutes from groundwater systems and in others the surface-water body is a source of groundwater recharge and causes changes in groundwater quality. As a result, withdrawal of water from streams can deplete groundwater or conversely, pumpage of groundwater can deplete water in streams, lakes, or wetlands. Pollution of surface water can cause degradation of groundwater quality and conversely pollution of groundwater can degrade surface water.</skos:scopeNote>
    <skos:altLabel xml:lang="en">aquifer-surface water interaction</skos:altLabel>
    <skos:altLabel xml:lang="en">ground-water/surface-water interaction</skos:altLabel>
    <skos:altLabel xml:lang="en">hyporheic zone processes</skos:altLabel>
    <skos:altLabel xml:lang="en">surface-water/ground-water interaction</skos:altLabel>
    <skos:altLabel xml:lang="en">groundwater/surface water interaction</skos:altLabel>
    <skos:altLabel xml:lang="en">surface water/groundwater interaction</skos:altLabel>
    <skos:broader rdf:resource="http://www.usgs.gov/science/USGSThesaurus/hydrologic%20processes"/>
    <skos:inScheme rdf:resource="http://www.usgs.gov/science/USGSThesaurus"/>
  </rdf:Description>
  <rdf:Description about="http://www.usgs.gov/science/USGSThesaurus/groundwater%20flow">
    <rdf:type rdf:resource="http://www.w3.org/2004/02/skos/core#Concept"/>
    <skos:prefLabel xml:lang="en">groundwater flow</skos:prefLabel>
    <skos:scopeNote xml:lang="en">Movement of subsurface water in the saturated zone from areas of recharge to areas of discharge.</skos:scopeNote>
    <skos:altLabel xml:lang="en">fluid migration</skos:altLabel>
    <skos:altLabel xml:lang="en">groundwater flow modeling</skos:altLabel>
    <skos:altLabel xml:lang="en">groundwater movement</skos:altLabel>
    <skos:altLabel xml:lang="en">ground-water flow</skos:altLabel>
    <skos:broader rdf:resource="http://www.usgs.gov/science/USGSThesaurus/hydrologic%20processes"/>
    <skos:related rdf:resource="http://www.usgs.gov/science/USGSThesaurus/groundwater"/>
    <skos:related rdf:resource="http://www.usgs.gov/science/USGSThesaurus/hydrogeology"/>
    <skos:related rdf:resource="http://www.usgs.gov/science/USGSThesaurus/water%20cycle"/>
    <skos:related rdf:resource="http://www.usgs.gov/science/USGSThesaurus/reaction%20transport"/>
    <skos:inScheme rdf:resource="http://www.usgs.gov/science/USGSThesaurus"/>
  </rdf:Description>
  <rdf:Description about="http://www.usgs.gov/science/USGSThesaurus/percolation">
    <rdf:type rdf:resource="http://www.w3.org/2004/02/skos/core#Concept"/>
    <skos:prefLabel xml:lang="en">percolation</skos:prefLabel>
    <skos:scopeNote xml:lang="en">The movement of water through fractures or interstices of a rock or soil.</skos:scopeNote>
    <skos:altLabel xml:lang="en">infiltration (water)</skos:altLabel>
    <skos:broader rdf:resource="http://www.usgs.gov/science/USGSThesaurus/hydrologic%20processes"/>
    <skos:related rdf:resource="http://www.usgs.gov/science/USGSThesaurus/permeability"/>
    <skos:inScheme rdf:resource="http://www.usgs.gov/science/USGSThesaurus"/>
  </rdf:Description>
  <rdf:Description about="http://www.usgs.gov/science/USGSThesaurus/runoff">
    <rdf:type rdf:resource="http://www.w3.org/2004/02/skos/core#Concept"/>
    <skos:prefLabel xml:lang="en">runoff</skos:prefLabel>
    <skos:scopeNote xml:lang="en">Flow of water over land surfaces (including paved surfaces), typically from precipitation.</skos:scopeNote>
    <skos:altLabel xml:lang="en">stormwater runoff</skos:altLabel>
    <skos:altLabel xml:lang="en">urban runoff</skos:altLabel>
    <skos:broader rdf:resource="http://www.usgs.gov/science/USGSThesaurus/hydrologic%20processes"/>
    <skos:inScheme rdf:resource="http://www.usgs.gov/science/USGSThesaurus"/>
  </rdf:Description>
  <rdf:Description about="http://www.usgs.gov/science/USGSThesaurus/saltwater%20intrusion">
    <rdf:type rdf:resource="http://www.w3.org/2004/02/skos/core#Concept"/>
    <skos:prefLabel xml:lang="en">saltwater intrusion</skos:prefLabel>
    <skos:scopeNote xml:lang="en">Infusion of saline waters in an aquifer or body of surface water.</skos:scopeNote>
    <skos:altLabel xml:lang="en">salt-water intrusion</skos:altLabel>
    <skos:broader rdf:resource="http://www.usgs.gov/science/USGSThesaurus/hydrologic%20processes"/>
    <skos:inScheme rdf:resource="http://www.usgs.gov/science/USGSThesaurus"/>
  </rdf:Description>
  <rdf:Description about="http://www.usgs.gov/science/USGSThesaurus/scour">
    <rdf:type rdf:resource="http://www.w3.org/2004/02/skos/core#Concept"/>
    <skos:prefLabel xml:lang="en">scour</skos:prefLabel>
    <skos:scopeNote xml:lang="en">Erosion of sediment in a stream bed, often occurring at manmade structures such as bridge supports.</skos:scopeNote>
    <skos:altLabel xml:lang="en">bridge scour</skos:altLabel>
    <skos:broader rdf:resource="http://www.usgs.gov/science/USGSThesaurus/hydrologic%20processes"/>
    <skos:related rdf:resource="http://www.usgs.gov/science/USGSThesaurus/hazards"/>
    <skos:related rdf:resource="http://www.usgs.gov/science/USGSThesaurus/erosion"/>
    <skos:inScheme rdf:resource="http://www.usgs.gov/science/USGSThesaurus"/>
  </rdf:Description>
  <rdf:Description about="http://www.usgs.gov/science/USGSThesaurus/streamflow">
    <rdf:type rdf:resource="http://www.w3.org/2004/02/skos/core#Concept"/>
    <skos:prefLabel xml:lang="en">streamflow</skos:prefLabel>
    <skos:scopeNote xml:lang="en">A type of channel flow, applied to a specific part of surface runoff in a stream, whether or not it is affected by diversion or regulation.</skos:scopeNote>
    <skos:altLabel xml:lang="en">flood stage</skos:altLabel>
    <skos:altLabel xml:lang="en">fluvial processes</skos:altLabel>
    <skos:altLabel xml:lang="en">gage height</skos:altLabel>
    <skos:altLabel xml:lang="en">stream current</skos:altLabel>
    <skos:altLabel xml:lang="en">stream flow</skos:altLabel>
    <skos:altLabel xml:lang="en">stream stage</skos:altLabel>
    <!--FOR streamflow data USE streamflow WITH datasets-->
    <skos:altLabel xml:lang="en">streamflow data</skos:altLabel>
    <!--FOR streamflow modeling USE streamflow WITH mathematical modeling-->
    <skos:altLabel xml:lang="en">streamflow modeling</skos:altLabel>
    <skos:broader rdf:resource="http://www.usgs.gov/science/USGSThesaurus/hydrologic%20processes"/>
    <skos:narrower rdf:resource="http://www.usgs.gov/science/USGSThesaurus/stream%20discharge"/>
    <skos:narrower rdf:resource="http://www.usgs.gov/science/USGSThesaurus/turbidity"/>
    <skos:related rdf:resource="http://www.usgs.gov/science/USGSThesaurus/hydrology"/>
    <skos:related rdf:resource="http://www.usgs.gov/science/USGSThesaurus/stream-gage%20measurement"/>
    <skos:related rdf:resource="http://www.usgs.gov/science/USGSThesaurus/surface%20water%20%28non-marine%29"/>
    <skos:related rdf:resource="http://www.usgs.gov/science/USGSThesaurus/water%20circulation"/>
    <skos:related rdf:resource="http://www.usgs.gov/science/USGSThesaurus/watershed%20management"/>
    <skos:related rdf:resource="http://www.usgs.gov/science/USGSThesaurus/surface-water%20level"/>
    <skos:inScheme rdf:resource="http://www.usgs.gov/science/USGSThesaurus"/>
  </rdf:Description>
  <rdf:Description about="http://www.usgs.gov/science/USGSThesaurus/stream%20discharge">
    <rdf:type rdf:resource="http://www.w3.org/2004/02/skos/core#Concept"/>
    <skos:prefLabel xml:lang="en">stream discharge</skos:prefLabel>
    <skos:scopeNote xml:lang="en">Volume of water in a stream passing a given point at a given moment in time, expressed as a measure of volume per unit of time, i.e. cubic feet per second, million gallons per day, or gallons per minute.</skos:scopeNote>
    <skos:altLabel xml:lang="en">river discharge</skos:altLabel>
    <skos:altLabel xml:lang="en">stream discharge monitoring</skos:altLabel>
    <skos:broader rdf:resource="http://www.usgs.gov/science/USGSThesaurus/streamflow"/>
    <skos:related rdf:resource="http://www.usgs.gov/science/USGSThesaurus/hydrology"/>
    <skos:related rdf:resource="http://www.usgs.gov/science/USGSThesaurus/river%20systems"/>
    <skos:related rdf:resource="http://www.usgs.gov/science/USGSThesaurus/surface%20water%20%28non-marine%29"/>
    <skos:inScheme rdf:resource="http://www.usgs.gov/science/USGSThesaurus"/>
  </rdf:Description>
  <rdf:Description about="http://www.usgs.gov/science/USGSThesaurus/turbidity">
    <rdf:type rdf:resource="http://www.w3.org/2004/02/skos/core#Concept"/>
    <skos:prefLabel xml:lang="en">turbidity</skos:prefLabel>
    <skos:scopeNote xml:lang="en">Cloudiness in the water column, caused by the presence of suspended and dissolved matter such as clay, silt, organic matter, or plankton.</skos:scopeNote>
    <skos:altLabel xml:lang="en">turbulence</skos:altLabel>
    <skos:broader rdf:resource="http://www.usgs.gov/science/USGSThesaurus/streamflow"/>
    <skos:inScheme rdf:resource="http://www.usgs.gov/science/USGSThesaurus"/>
  </rdf:Description>
  <rdf:Description about="http://www.usgs.gov/science/USGSThesaurus/water%20circulation">
    <rdf:type rdf:resource="http://www.w3.org/2004/02/skos/core#Concept"/>
    <skos:prefLabel xml:lang="en">water circulation</skos:prefLabel>
    <skos:scopeNote xml:lang="en">The flow of water in a body of water due to wind or other forces or variations in density or temperature. Use 'water circulation' for situations that are not specifically covered by narrower terms. Use 'ocean circulation' for water circulation in the oceans.</skos:scopeNote>
    <skos:altLabel xml:lang="en">circulation (water)</skos:altLabel>
    <skos:altLabel xml:lang="en">lake circulation</skos:altLabel>
    <skos:broader rdf:resource="http://www.usgs.gov/science/USGSThesaurus/hydrologic%20processes"/>
    <skos:related rdf:resource="http://www.usgs.gov/science/USGSThesaurus/atmospheric%20circulation"/>
    <skos:related rdf:resource="http://www.usgs.gov/science/USGSThesaurus/hydrology"/>
    <skos:related rdf:resource="http://www.usgs.gov/science/USGSThesaurus/ocean%20circulation"/>
    <skos:related rdf:resource="http://www.usgs.gov/science/USGSThesaurus/streamflow"/>
    <skos:inScheme rdf:resource="http://www.usgs.gov/science/USGSThesaurus"/>
  </rdf:Description>
  <rdf:Description about="http://www.usgs.gov/science/USGSThesaurus/water%20cycle">
    <rdf:type rdf:resource="http://www.w3.org/2004/02/skos/core#Concept"/>
    <skos:prefLabel xml:lang="en">water cycle</skos:prefLabel>
    <skos:scopeNote xml:lang="en">Interchange of water among land, oceans, and atmosphere.</skos:scopeNote>
    <skos:altLabel xml:lang="en">hydrologic cycle</skos:altLabel>
    <skos:altLabel xml:lang="en">recharge</skos:altLabel>
    <skos:broader rdf:resource="http://www.usgs.gov/science/USGSThesaurus/hydrologic%20processes"/>
    <skos:related rdf:resource="http://www.usgs.gov/science/USGSThesaurus/evaporation"/>
    <skos:related rdf:resource="http://www.usgs.gov/science/USGSThesaurus/precipitation%20%28atmospheric%29"/>
    <skos:related rdf:resource="http://www.usgs.gov/science/USGSThesaurus/groundwater%20flow"/>
    <skos:inScheme rdf:resource="http://www.usgs.gov/science/USGSThesaurus"/>
  </rdf:Description>
  <rdf:Description about="http://www.usgs.gov/science/USGSThesaurus/impact%20cratering">
    <rdf:type rdf:resource="http://www.w3.org/2004/02/skos/core#Concept"/>
    <skos:prefLabel xml:lang="en">impact cratering</skos:prefLabel>
    <skos:scopeNote xml:lang="en">Impact of extraterrestrial objects such as asteroids, comets, and meteorites on Earth.</skos:scopeNote>
    <skos:altLabel xml:lang="en">bolide impact</skos:altLabel>
    <skos:altLabel xml:lang="en">meteor impact</skos:altLabel>
    <skos:altLabel xml:lang="en">comet impact</skos:altLabel>
    <skos:altLabel xml:lang="en">asteroid impact</skos:altLabel>
    <skos:broader rdf:resource="http://www.usgs.gov/science/USGSThesaurus/biological%20and%20physical%20processes"/>
    <skos:related rdf:resource="http://www.usgs.gov/science/USGSThesaurus/hazards"/>
    <skos:related rdf:resource="http://www.usgs.gov/science/USGSThesaurus/planetary%20bodies"/>
    <skos:inScheme rdf:resource="http://www.usgs.gov/science/USGSThesaurus"/>
  </rdf:Description>
  <rdf:Description about="http://www.usgs.gov/science/USGSThesaurus/ocean%20processes">
    <rdf:type rdf:resource="http://www.w3.org/2004/02/skos/core#Concept"/>
    <skos:prefLabel xml:lang="en">ocean processes</skos:prefLabel>
    <skos:scopeNote xml:lang="en">Recurrent natural changes that are physical, biological, or chemical, actively affecting the seas and oceans.</skos:scopeNote>
    <!--FOR marine sediment transport USE ocean processes WITH sediment transport-->
    <skos:altLabel xml:lang="en">marine sediment transport</skos:altLabel>
    <!--FOR oceans USE ocean processes WITH ocean characteristics-->
    <skos:altLabel xml:lang="en">oceans</skos:altLabel>
    <!--FOR ocean hazards USE ocean processes WITH hazards-->
    <skos:altLabel xml:lang="en">ocean hazards</skos:altLabel>
    <skos:broader rdf:resource="http://www.usgs.gov/science/USGSThesaurus/biological%20and%20physical%20processes"/>
    <skos:narrower rdf:resource="http://www.usgs.gov/science/USGSThesaurus/ocean%20circulation"/>
    <skos:narrower rdf:resource="http://www.usgs.gov/science/USGSThesaurus/ocean%20currents"/>
    <skos:narrower rdf:resource="http://www.usgs.gov/science/USGSThesaurus/ocean%20waves"/>
    <skos:narrower rdf:resource="http://www.usgs.gov/science/USGSThesaurus/tides%20%28oceanic%29"/>
    <skos:related rdf:resource="http://www.usgs.gov/science/USGSThesaurus/marine%20geophysics"/>
    <skos:related rdf:resource="http://www.usgs.gov/science/USGSThesaurus/ocean%20characteristics"/>
    <skos:related rdf:resource="http://www.usgs.gov/science/USGSThesaurus/ocean%20sciences"/>
    <skos:related rdf:resource="http://www.usgs.gov/science/USGSThesaurus/ocean-atmosphere%20interaction"/>
    <skos:related rdf:resource="http://www.usgs.gov/science/USGSThesaurus/surface%20water%20%28non-marine%29"/>
    <skos:related rdf:resource="http://www.usgs.gov/science/USGSThesaurus/ocean%20acidification"/>
    <skos:inScheme rdf:resource="http://www.usgs.gov/science/USGSThesaurus"/>
  </rdf:Description>
  <rdf:Description about="http://www.usgs.gov/science/USGSThesaurus/ocean%20circulation">
    <rdf:type rdf:resource="http://www.w3.org/2004/02/skos/core#Concept"/>
    <skos:prefLabel xml:lang="en">ocean circulation</skos:prefLabel>
    <skos:scopeNote xml:lang="en">Movement of large masses of water within an ocean.</skos:scopeNote>
    <skos:altLabel xml:lang="en">circulation (ocean)</skos:altLabel>
    <skos:broader rdf:resource="http://www.usgs.gov/science/USGSThesaurus/ocean%20processes"/>
    <skos:related rdf:resource="http://www.usgs.gov/science/USGSThesaurus/climatology"/>
    <skos:related rdf:resource="http://www.usgs.gov/science/USGSThesaurus/ocean%20currents"/>
    <skos:related rdf:resource="http://www.usgs.gov/science/USGSThesaurus/ocean%20sciences"/>
    <skos:related rdf:resource="http://www.usgs.gov/science/USGSThesaurus/tides%20%28oceanic%29"/>
    <skos:related rdf:resource="http://www.usgs.gov/science/USGSThesaurus/water%20circulation"/>
    <skos:inScheme rdf:resource="http://www.usgs.gov/science/USGSThesaurus"/>
  </rdf:Description>
  <rdf:Description about="http://www.usgs.gov/science/USGSThesaurus/ocean%20currents">
    <rdf:type rdf:resource="http://www.w3.org/2004/02/skos/core#Concept"/>
    <skos:prefLabel xml:lang="en">ocean currents</skos:prefLabel>
    <skos:scopeNote xml:lang="en">Recurrent strong flows of seawater generated by wind or variations in water density along a given path.</skos:scopeNote>
    <!--FOR ocean current measurement USE ocean currents WITH field inventory and monitoring-->
    <skos:altLabel xml:lang="en">ocean current measurement</skos:altLabel>
    <skos:broader rdf:resource="http://www.usgs.gov/science/USGSThesaurus/ocean%20processes"/>
    <skos:related rdf:resource="http://www.usgs.gov/science/USGSThesaurus/meteorology"/>
    <skos:related rdf:resource="http://www.usgs.gov/science/USGSThesaurus/ocean%20circulation"/>
    <skos:related rdf:resource="http://www.usgs.gov/science/USGSThesaurus/ocean%20sciences"/>
    <skos:related rdf:resource="http://www.usgs.gov/science/USGSThesaurus/tides%20%28oceanic%29"/>
    <skos:inScheme rdf:resource="http://www.usgs.gov/science/USGSThesaurus"/>
  </rdf:Description>
  <rdf:Description about="http://www.usgs.gov/science/USGSThesaurus/ocean%20waves">
    <rdf:type rdf:resource="http://www.w3.org/2004/02/skos/core#Concept"/>
    <skos:prefLabel xml:lang="en">ocean waves</skos:prefLabel>
    <skos:scopeNote xml:lang="en">A periodic movement of seawater caused by wind, tide, and currents.</skos:scopeNote>
    <!--FOR ocean wave measurement USE ocean waves WITH field inventory and monitoring-->
    <skos:altLabel xml:lang="en">ocean wave measurement</skos:altLabel>
    <skos:altLabel xml:lang="en">water waves</skos:altLabel>
    <skos:broader rdf:resource="http://www.usgs.gov/science/USGSThesaurus/ocean%20processes"/>
    <skos:narrower rdf:resource="http://www.usgs.gov/science/USGSThesaurus/tsunamis"/>
    <skos:related rdf:resource="http://www.usgs.gov/science/USGSThesaurus/ocean%20sciences"/>
    <skos:inScheme rdf:resource="http://www.usgs.gov/science/USGSThesaurus"/>
  </rdf:Description>
  <rdf:Description about="http://www.usgs.gov/science/USGSThesaurus/tsunamis">
    <rdf:type rdf:resource="http://www.w3.org/2004/02/skos/core#Concept"/>
    <skos:prefLabel xml:lang="en">tsunamis</skos:prefLabel>
    <skos:scopeNote xml:lang="en">Sea waves generated by submarine earthquakes, volcanic eruptions, or landslides, which are generally imperceptible in deep water but may be very destructive when striking the shoreline.</skos:scopeNote>
    <skos:altLabel xml:lang="en">tidal waves</skos:altLabel>
    <!--FOR tsunami preparedness USE tsunamis WITH hazard preparedness-->
    <skos:altLabel xml:lang="en">tsunami preparedness</skos:altLabel>
    <skos:broader rdf:resource="http://www.usgs.gov/science/USGSThesaurus/ocean%20waves"/>
    <skos:related rdf:resource="http://www.usgs.gov/science/USGSThesaurus/earthquakes"/>
    <skos:related rdf:resource="http://www.usgs.gov/science/USGSThesaurus/geologic%20processes"/>
    <skos:related rdf:resource="http://www.usgs.gov/science/USGSThesaurus/hazards"/>
    <skos:related rdf:resource="http://www.usgs.gov/science/USGSThesaurus/ocean%20sciences"/>
    <skos:related rdf:resource="http://www.usgs.gov/science/USGSThesaurus/seismology"/>
    <skos:inScheme rdf:resource="http://www.usgs.gov/science/USGSThesaurus"/>
  </rdf:Description>
  <rdf:Description about="http://www.usgs.gov/science/USGSThesaurus/tides%20%28oceanic%29">
    <rdf:type rdf:resource="http://www.w3.org/2004/02/skos/core#Concept"/>
    <skos:prefLabel xml:lang="en">tides (oceanic)</skos:prefLabel>
    <skos:scopeNote xml:lang="en">The periodic rise and fall of the level of the sea due to the gravitational attraction of the moon and sun. Occurs twice each day.</skos:scopeNote>
    <skos:altLabel xml:lang="en">ocean tides</skos:altLabel>
    <skos:broader rdf:resource="http://www.usgs.gov/science/USGSThesaurus/ocean%20processes"/>
    <skos:related rdf:resource="http://www.usgs.gov/science/USGSThesaurus/ocean%20circulation"/>
    <skos:related rdf:resource="http://www.usgs.gov/science/USGSThesaurus/ocean%20currents"/>
    <skos:related rdf:resource="http://www.usgs.gov/science/USGSThesaurus/ocean%20sciences"/>
    <skos:inScheme rdf:resource="http://www.usgs.gov/science/USGSThesaurus"/>
  </rdf:Description>
  <rdf:Description about="http://www.usgs.gov/science/USGSThesaurus/physiological%20processes">
    <rdf:type rdf:resource="http://www.w3.org/2004/02/skos/core#Concept"/>
    <skos:prefLabel xml:lang="en">physiological processes</skos:prefLabel>
    <skos:scopeNote xml:lang="en">Characteristics and processes of individual organisms that are not the direct result of their interaction with other organisms or with the environment.</skos:scopeNote>
    <skos:broader rdf:resource="http://www.usgs.gov/science/USGSThesaurus/biological%20and%20physical%20processes"/>
    <skos:narrower rdf:resource="http://www.usgs.gov/science/USGSThesaurus/bioluminescence"/>
    <skos:narrower rdf:resource="http://www.usgs.gov/science/USGSThesaurus/organism%20growth%20and%20development"/>
    <skos:narrower rdf:resource="http://www.usgs.gov/science/USGSThesaurus/osmosis"/>
    <skos:narrower rdf:resource="http://www.usgs.gov/science/USGSThesaurus/photosynthesis"/>
    <skos:inScheme rdf:resource="http://www.usgs.gov/science/USGSThesaurus"/>
  </rdf:Description>
  <rdf:Description about="http://www.usgs.gov/science/USGSThesaurus/bioluminescence">
    <rdf:type rdf:resource="http://www.w3.org/2004/02/skos/core#Concept"/>
    <skos:prefLabel xml:lang="en">bioluminescence</skos:prefLabel>
    <skos:scopeNote xml:lang="en">Emission of light by organisms.</skos:scopeNote>
    <skos:broader rdf:resource="http://www.usgs.gov/science/USGSThesaurus/physiological%20processes"/>
    <skos:inScheme rdf:resource="http://www.usgs.gov/science/USGSThesaurus"/>
  </rdf:Description>
  <rdf:Description about="http://www.usgs.gov/science/USGSThesaurus/organism%20growth%20and%20development">
    <rdf:type rdf:resource="http://www.w3.org/2004/02/skos/core#Concept"/>
    <skos:prefLabel xml:lang="en">organism growth and development</skos:prefLabel>
    <skos:scopeNote xml:lang="en">Changes that living things undergo as they progress from inception as a single cell to adult forms.</skos:scopeNote>
    <skos:altLabel xml:lang="en">ontogeny</skos:altLabel>
    <skos:broader rdf:resource="http://www.usgs.gov/science/USGSThesaurus/physiological%20processes"/>
    <skos:narrower rdf:resource="http://www.usgs.gov/science/USGSThesaurus/anatomical%20deformities"/>
    <skos:narrower rdf:resource="http://www.usgs.gov/science/USGSThesaurus/metamorphosis"/>
    <skos:related rdf:resource="http://www.usgs.gov/science/USGSThesaurus/developmental%20biology"/>
    <skos:related rdf:resource="http://www.usgs.gov/science/USGSThesaurus/molecular%20biology"/>
    <skos:inScheme rdf:resource="http://www.usgs.gov/science/USGSThesaurus"/>
  </rdf:Description>
  <rdf:Description about="http://www.usgs.gov/science/USGSThesaurus/anatomical%20deformities">
    <rdf:type rdf:resource="http://www.w3.org/2004/02/skos/core#Concept"/>
    <skos:prefLabel xml:lang="en">anatomical deformities</skos:prefLabel>
    <skos:scopeNote xml:lang="en">Physical malformation of organisms typically resulting from exposure to contaminants, disease, or adverse environmental conditions.</skos:scopeNote>
    <skos:broader rdf:resource="http://www.usgs.gov/science/USGSThesaurus/organism%20growth%20and%20development"/>
    <skos:related rdf:resource="http://www.usgs.gov/science/USGSThesaurus/wildlife%20disease"/>
    <skos:inScheme rdf:resource="http://www.usgs.gov/science/USGSThesaurus"/>
  </rdf:Description>
  <rdf:Description about="http://www.usgs.gov/science/USGSThesaurus/metamorphosis">
    <rdf:type rdf:resource="http://www.w3.org/2004/02/skos/core#Concept"/>
    <skos:prefLabel xml:lang="en">metamorphosis</skos:prefLabel>
    <skos:scopeNote xml:lang="en">Transformation in animals, such as amphibians and insects, from one developmental stage to another.</skos:scopeNote>
    <skos:altLabel xml:lang="en">metamorphism (biological)</skos:altLabel>
    <skos:broader rdf:resource="http://www.usgs.gov/science/USGSThesaurus/organism%20growth%20and%20development"/>
    <skos:inScheme rdf:resource="http://www.usgs.gov/science/USGSThesaurus"/>
  </rdf:Description>
  <rdf:Description about="http://www.usgs.gov/science/USGSThesaurus/osmosis">
    <rdf:type rdf:resource="http://www.w3.org/2004/02/skos/core#Concept"/>
    <skos:prefLabel xml:lang="en">osmosis</skos:prefLabel>
    <skos:scopeNote xml:lang="en">Transfer of substances through biological membranes.</skos:scopeNote>
    <skos:broader rdf:resource="http://www.usgs.gov/science/USGSThesaurus/physiological%20processes"/>
    <skos:inScheme rdf:resource="http://www.usgs.gov/science/USGSThesaurus"/>
  </rdf:Description>
  <rdf:Description about="http://www.usgs.gov/science/USGSThesaurus/photosynthesis">
    <rdf:type rdf:resource="http://www.w3.org/2004/02/skos/core#Concept"/>
    <skos:prefLabel xml:lang="en">photosynthesis</skos:prefLabel>
    <skos:scopeNote xml:lang="en">Conversion of sunlight, water, and nutrients into energy by plants.</skos:scopeNote>
    <skos:broader rdf:resource="http://www.usgs.gov/science/USGSThesaurus/physiological%20processes"/>
    <skos:inScheme rdf:resource="http://www.usgs.gov/science/USGSThesaurus"/>
  </rdf:Description>
  <rdf:Description about="http://www.usgs.gov/science/USGSThesaurus/contamination%20and%20pollution">
    <rdf:type rdf:resource="http://www.w3.org/2004/02/skos/core#Concept"/>
    <skos:prefLabel xml:lang="en">contamination and pollution</skos:prefLabel>
    <skos:scopeNote xml:lang="en">Introduction of harmful substances into the environment by human action or natural processes.</skos:scopeNote>
    <!--FOR water pollution USE contamination and pollution WITH water resources-->
    <skos:altLabel xml:lang="en">water pollution</skos:altLabel>
    <!--FOR soil pollution USE contamination and pollution WITH soil resources-->
    <skos:altLabel xml:lang="en">soil pollution</skos:altLabel>
    <skos:altLabel xml:lang="en">natural contaminants</skos:altLabel>
    <skos:altLabel xml:lang="en">pollution</skos:altLabel>
    <!--FOR air pollution USE contamination and pollution WITH atmospheric composition-->
    <skos:altLabel xml:lang="en">air pollution</skos:altLabel>
    <skos:altLabel xml:lang="en">effluent</skos:altLabel>
    <skos:altLabel xml:lang="en">outfall</skos:altLabel>
    <skos:broader rdf:resource="http://www.usgs.gov/science/USGSThesaurus/topics"/>
    <skos:narrower rdf:resource="http://www.usgs.gov/science/USGSThesaurus/industrial%20pollution"/>
    <skos:narrower rdf:resource="http://www.usgs.gov/science/USGSThesaurus/nonpoint-source%20pollution"/>
    <skos:narrower rdf:resource="http://www.usgs.gov/science/USGSThesaurus/pesticide%20and%20herbicide%20contamination"/>
    <skos:narrower rdf:resource="http://www.usgs.gov/science/USGSThesaurus/pharmaceutical%20contamination"/>
    <skos:narrower rdf:resource="http://www.usgs.gov/science/USGSThesaurus/toxic%20radionuclide%20contamination"/>
    <skos:narrower rdf:resource="http://www.usgs.gov/science/USGSThesaurus/toxic%20trace%20element%20contamination"/>
    <skos:related rdf:resource="http://www.usgs.gov/science/USGSThesaurus/human%20impacts"/>
    <skos:related rdf:resource="http://www.usgs.gov/science/USGSThesaurus/waste%20treatment%20and%20disposal"/>
    <skos:related rdf:resource="http://www.usgs.gov/science/USGSThesaurus/ecotoxicology"/>
    <skos:related rdf:resource="http://www.usgs.gov/science/USGSThesaurus/hazards"/>
    <skos:related rdf:resource="http://www.usgs.gov/science/USGSThesaurus/water%20quality"/>
    <skos:inScheme rdf:resource="http://www.usgs.gov/science/USGSThesaurus"/>
  </rdf:Description>
  <rdf:Description about="http://www.usgs.gov/science/USGSThesaurus/industrial%20pollution">
    <rdf:type rdf:resource="http://www.w3.org/2004/02/skos/core#Concept"/>
    <skos:prefLabel xml:lang="en">industrial pollution</skos:prefLabel>
    <skos:scopeNote xml:lang="en">Introduction of harmful substances into the environment by manufacturing, power generation, mining, or material processing.</skos:scopeNote>
    <!--FOR oil spills USE industrial pollution WITH petroleum-->
    <skos:altLabel xml:lang="en">oil spills</skos:altLabel>
    <skos:altLabel xml:lang="en">polychlorinated biphenyls</skos:altLabel>
    <skos:altLabel xml:lang="en">PCBs</skos:altLabel>
    <skos:broader rdf:resource="http://www.usgs.gov/science/USGSThesaurus/contamination%20and%20pollution"/>
    <skos:narrower rdf:resource="http://www.usgs.gov/science/USGSThesaurus/mine%20drainage"/>
    <skos:related rdf:resource="http://www.usgs.gov/science/USGSThesaurus/abandoned%20mines%20and%20quarries"/>
    <skos:inScheme rdf:resource="http://www.usgs.gov/science/USGSThesaurus"/>
  </rdf:Description>
  <rdf:Description about="http://www.usgs.gov/science/USGSThesaurus/mine%20drainage">
    <rdf:type rdf:resource="http://www.w3.org/2004/02/skos/core#Concept"/>
    <skos:prefLabel xml:lang="en">mine drainage</skos:prefLabel>
    <skos:scopeNote xml:lang="en">Introduction of harmful substances into the environment from mines and tailings.</skos:scopeNote>
    <skos:broader rdf:resource="http://www.usgs.gov/science/USGSThesaurus/industrial%20pollution"/>
    <skos:related rdf:resource="http://www.usgs.gov/science/USGSThesaurus/mining%20hazards"/>
    <skos:inScheme rdf:resource="http://www.usgs.gov/science/USGSThesaurus"/>
  </rdf:Description>
  <rdf:Description about="http://www.usgs.gov/science/USGSThesaurus/nonpoint-source%20pollution">
    <rdf:type rdf:resource="http://www.w3.org/2004/02/skos/core#Concept"/>
    <skos:prefLabel xml:lang="en">nonpoint-source pollution</skos:prefLabel>
    <skos:scopeNote xml:lang="en">Contamination of the environment from sources spread widely across an area, not from a small number of identifiable locations.</skos:scopeNote>
    <skos:broader rdf:resource="http://www.usgs.gov/science/USGSThesaurus/contamination%20and%20pollution"/>
    <skos:inScheme rdf:resource="http://www.usgs.gov/science/USGSThesaurus"/>
  </rdf:Description>
  <rdf:Description about="http://www.usgs.gov/science/USGSThesaurus/pesticide%20and%20herbicide%20contamination">
    <rdf:type rdf:resource="http://www.w3.org/2004/02/skos/core#Concept"/>
    <skos:prefLabel xml:lang="en">pesticide and herbicide contamination</skos:prefLabel>
    <skos:scopeNote xml:lang="en">Pollution resulting from chemical agents applied to crops, rights of way, lawns, or residences to control weeds, insects, fungi, nematodes, rodents or other pests (pesticides) or kill undesirable plants (herbicides).</skos:scopeNote>
    <skos:altLabel xml:lang="en">biocide contamination</skos:altLabel>
    <skos:altLabel xml:lang="en">degradation products (chemical)</skos:altLabel>
    <skos:altLabel xml:lang="en">herbicide contamination</skos:altLabel>
    <skos:altLabel xml:lang="en">insecticide contamination</skos:altLabel>
    <skos:broader rdf:resource="http://www.usgs.gov/science/USGSThesaurus/contamination%20and%20pollution"/>
    <skos:related rdf:resource="http://www.usgs.gov/science/USGSThesaurus/biochemistry"/>
    <skos:related rdf:resource="http://www.usgs.gov/science/USGSThesaurus/ecology"/>
    <skos:related rdf:resource="http://www.usgs.gov/science/USGSThesaurus/ecotoxicology"/>
    <skos:inScheme rdf:resource="http://www.usgs.gov/science/USGSThesaurus"/>
  </rdf:Description>
  <rdf:Description about="http://www.usgs.gov/science/USGSThesaurus/pharmaceutical%20contamination">
    <rdf:type rdf:resource="http://www.w3.org/2004/02/skos/core#Concept"/>
    <skos:prefLabel xml:lang="en">pharmaceutical contamination</skos:prefLabel>
    <skos:scopeNote xml:lang="en">Unintentional release of pharmaceutical compounds into the environment; work focuses on the effects of these compounds on organisms and water resources.</skos:scopeNote>
    <skos:broader rdf:resource="http://www.usgs.gov/science/USGSThesaurus/contamination%20and%20pollution"/>
    <skos:inScheme rdf:resource="http://www.usgs.gov/science/USGSThesaurus"/>
  </rdf:Description>
  <rdf:Description about="http://www.usgs.gov/science/USGSThesaurus/toxic%20radionuclide%20contamination">
    <rdf:type rdf:resource="http://www.w3.org/2004/02/skos/core#Concept"/>
    <skos:prefLabel xml:lang="en">toxic radionuclide contamination</skos:prefLabel>
    <skos:scopeNote xml:lang="en">Introduction into the environment of unstable isotopes of elements that undergo radioactive decay, emitting radiation that is harmful to organisms.</skos:scopeNote>
    <skos:broader rdf:resource="http://www.usgs.gov/science/USGSThesaurus/contamination%20and%20pollution"/>
    <skos:related rdf:resource="http://www.usgs.gov/science/USGSThesaurus/ecotoxicology"/>
    <skos:related rdf:resource="http://www.usgs.gov/science/USGSThesaurus/environmental%20health%20%28human%29"/>
    <skos:related rdf:resource="http://www.usgs.gov/science/USGSThesaurus/radon"/>
    <skos:inScheme rdf:resource="http://www.usgs.gov/science/USGSThesaurus"/>
  </rdf:Description>
  <rdf:Description about="http://www.usgs.gov/science/USGSThesaurus/toxic%20trace%20element%20contamination">
    <rdf:type rdf:resource="http://www.w3.org/2004/02/skos/core#Concept"/>
    <skos:prefLabel xml:lang="en">toxic trace element contamination</skos:prefLabel>
    <skos:scopeNote xml:lang="en">Introduction into the environment of elements (such as arsenic, cadmium, lead, and mercury) which have a deleterious effect on living organisms when found naturally in only minor amounts (concentrations less than 1.0 milligram per liter) in water or sediment.</skos:scopeNote>
    <skos:broader rdf:resource="http://www.usgs.gov/science/USGSThesaurus/contamination%20and%20pollution"/>
    <skos:narrower rdf:resource="http://www.usgs.gov/science/USGSThesaurus/mercury%20contamination"/>
    <skos:related rdf:resource="http://www.usgs.gov/science/USGSThesaurus/ecotoxicology"/>
    <skos:related rdf:resource="http://www.usgs.gov/science/USGSThesaurus/environmental%20health%20%28human%29"/>
    <skos:inScheme rdf:resource="http://www.usgs.gov/science/USGSThesaurus"/>
  </rdf:Description>
  <rdf:Description about="http://www.usgs.gov/science/USGSThesaurus/mercury%20contamination">
    <rdf:type rdf:resource="http://www.w3.org/2004/02/skos/core#Concept"/>
    <skos:prefLabel xml:lang="en">mercury contamination</skos:prefLabel>
    <skos:scopeNote xml:lang="en">Biological disturbances caused by mercury compounds that have entered the environment.</skos:scopeNote>
    <skos:broader rdf:resource="http://www.usgs.gov/science/USGSThesaurus/toxic%20trace%20element%20contamination"/>
    <skos:related rdf:resource="http://www.usgs.gov/science/USGSThesaurus/biochemistry"/>
    <skos:related rdf:resource="http://www.usgs.gov/science/USGSThesaurus/ecology"/>
    <skos:related rdf:resource="http://www.usgs.gov/science/USGSThesaurus/ecotoxicology"/>
    <skos:inScheme rdf:resource="http://www.usgs.gov/science/USGSThesaurus"/>
  </rdf:Description>
  <rdf:Description about="http://www.usgs.gov/science/USGSThesaurus/culture%20and%20demographics">
    <rdf:type rdf:resource="http://www.w3.org/2004/02/skos/core#Concept"/>
    <skos:prefLabel xml:lang="en">culture and demographics</skos:prefLabel>
    <skos:scopeNote xml:lang="en">Information on human behavior, ways of living and thinking, and characteristics of human populations.</skos:scopeNote>
    <skos:altLabel xml:lang="en">demographics</skos:altLabel>
    <skos:altLabel xml:lang="en">socioeconomics</skos:altLabel>
    <skos:broader rdf:resource="http://www.usgs.gov/science/USGSThesaurus/topics"/>
    <skos:narrower rdf:resource="http://www.usgs.gov/science/USGSThesaurus/administrative%20and%20political%20boundaries"/>
    <skos:narrower rdf:resource="http://www.usgs.gov/science/USGSThesaurus/business%20and%20economics"/>
    <skos:narrower rdf:resource="http://www.usgs.gov/science/USGSThesaurus/cadastral%20and%20legal%20land%20descriptions"/>
    <skos:narrower rdf:resource="http://www.usgs.gov/science/USGSThesaurus/geographic%20names"/>
    <skos:narrower rdf:resource="http://www.usgs.gov/science/USGSThesaurus/laws%20and%20regulations"/>
    <skos:narrower rdf:resource="http://www.usgs.gov/science/USGSThesaurus/population%20%28human%29"/>
    <skos:narrower rdf:resource="http://www.usgs.gov/science/USGSThesaurus/transportation"/>
    <skos:related rdf:resource="http://www.usgs.gov/science/USGSThesaurus/geography"/>
    <skos:related rdf:resource="http://www.usgs.gov/science/USGSThesaurus/social%20sciences"/>
    <skos:inScheme rdf:resource="http://www.usgs.gov/science/USGSThesaurus"/>
  </rdf:Description>
  <rdf:Description about="http://www.usgs.gov/science/USGSThesaurus/administrative%20and%20political%20boundaries">
    <rdf:type rdf:resource="http://www.w3.org/2004/02/skos/core#Concept"/>
    <skos:prefLabel xml:lang="en">administrative and political boundaries</skos:prefLabel>
    <skos:scopeNote xml:lang="en">Lines drawn on maps or described in documents which encompass territory controlled by a government or organizational unit that may or may not align with geographic or cultural barriers. Use for datasets containing boundary representations for political/administrative units and related information.</skos:scopeNote>
    <skos:altLabel xml:lang="en">borders</skos:altLabel>
    <skos:altLabel xml:lang="en">geographic boundaries</skos:altLabel>
    <skos:altLabel xml:lang="en">governmental units</skos:altLabel>
    <skos:altLabel xml:lang="en">political boundaries</skos:altLabel>
    <skos:broader rdf:resource="http://www.usgs.gov/science/USGSThesaurus/culture%20and%20demographics"/>
    <skos:related rdf:resource="http://www.usgs.gov/science/USGSThesaurus/cadastral%20and%20legal%20land%20descriptions"/>
    <skos:related rdf:resource="http://www.usgs.gov/science/USGSThesaurus/geography"/>
    <skos:inScheme rdf:resource="http://www.usgs.gov/science/USGSThesaurus"/>
  </rdf:Description>
  <rdf:Description about="http://www.usgs.gov/science/USGSThesaurus/business%20and%20economics">
    <rdf:type rdf:resource="http://www.w3.org/2004/02/skos/core#Concept"/>
    <skos:prefLabel xml:lang="en">business and economics</skos:prefLabel>
    <skos:scopeNote xml:lang="en">The activities and processes associated with the production, distribution, and consumption of goods and services.</skos:scopeNote>
    <skos:altLabel xml:lang="en">commerce</skos:altLabel>
    <skos:altLabel xml:lang="en">economics</skos:altLabel>
    <skos:broader rdf:resource="http://www.usgs.gov/science/USGSThesaurus/culture%20and%20demographics"/>
    <skos:narrower rdf:resource="http://www.usgs.gov/science/USGSThesaurus/materials%20flow%20%28commodities%29"/>
    <skos:narrower rdf:resource="http://www.usgs.gov/science/USGSThesaurus/recycling"/>
    <skos:narrower rdf:resource="http://www.usgs.gov/science/USGSThesaurus/resource%20supply%20and%20demand"/>
    <skos:related rdf:resource="http://www.usgs.gov/science/USGSThesaurus/social%20sciences"/>
    <skos:inScheme rdf:resource="http://www.usgs.gov/science/USGSThesaurus"/>
  </rdf:Description>
  <rdf:Description about="http://www.usgs.gov/science/USGSThesaurus/materials%20flow%20%28commodities%29">
    <rdf:type rdf:resource="http://www.w3.org/2004/02/skos/core#Concept"/>
    <skos:prefLabel xml:lang="en">materials flow (commodities)</skos:prefLabel>
    <skos:scopeNote xml:lang="en">Industrial and commercial processes by which material resources are extracted, used or consumed, and disposed or recycled.</skos:scopeNote>
    <skos:broader rdf:resource="http://www.usgs.gov/science/USGSThesaurus/business%20and%20economics"/>
    <skos:inScheme rdf:resource="http://www.usgs.gov/science/USGSThesaurus"/>
  </rdf:Description>
  <rdf:Description about="http://www.usgs.gov/science/USGSThesaurus/recycling">
    <rdf:type rdf:resource="http://www.w3.org/2004/02/skos/core#Concept"/>
    <skos:prefLabel xml:lang="en">recycling</skos:prefLabel>
    <skos:scopeNote xml:lang="en">Physical processes by which previously-used materials are converted from scrap and waste to reusable forms.</skos:scopeNote>
    <skos:broader rdf:resource="http://www.usgs.gov/science/USGSThesaurus/business%20and%20economics"/>
    <skos:inScheme rdf:resource="http://www.usgs.gov/science/USGSThesaurus"/>
  </rdf:Description>
  <rdf:Description about="http://www.usgs.gov/science/USGSThesaurus/resource%20supply%20and%20demand">
    <rdf:type rdf:resource="http://www.w3.org/2004/02/skos/core#Concept"/>
    <skos:prefLabel xml:lang="en">resource supply and demand</skos:prefLabel>
    <skos:scopeNote xml:lang="en">Statistics indicating the commercial interests in material resources, typically mineral commodities, energy, or forest or fishery resources.</skos:scopeNote>
    <skos:broader rdf:resource="http://www.usgs.gov/science/USGSThesaurus/business%20and%20economics"/>
    <skos:inScheme rdf:resource="http://www.usgs.gov/science/USGSThesaurus"/>
  </rdf:Description>
  <rdf:Description about="http://www.usgs.gov/science/USGSThesaurus/cadastral%20and%20legal%20land%20descriptions">
    <rdf:type rdf:resource="http://www.w3.org/2004/02/skos/core#Concept"/>
    <skos:prefLabel xml:lang="en">cadastral and legal land descriptions</skos:prefLabel>
    <skos:scopeNote xml:lang="en">Records in official registers showing extent, boundaries, and ownerships of land for administration and taxation.</skos:scopeNote>
    <skos:altLabel xml:lang="en">land partitioning systems</skos:altLabel>
    <skos:altLabel xml:lang="en">legal land descriptions</skos:altLabel>
    <!--FOR cadastral maps USE cadastral and legal land descriptions WITH maps and atlases-->
    <skos:altLabel xml:lang="en">cadastral maps</skos:altLabel>
    <skos:broader rdf:resource="http://www.usgs.gov/science/USGSThesaurus/culture%20and%20demographics"/>
    <skos:related rdf:resource="http://www.usgs.gov/science/USGSThesaurus/administrative%20and%20political%20boundaries"/>
    <skos:related rdf:resource="http://www.usgs.gov/science/USGSThesaurus/geography"/>
    <skos:related rdf:resource="http://www.usgs.gov/science/USGSThesaurus/social%20sciences"/>
    <skos:inScheme rdf:resource="http://www.usgs.gov/science/USGSThesaurus"/>
  </rdf:Description>
  <rdf:Description about="http://www.usgs.gov/science/USGSThesaurus/geographic%20names">
    <rdf:type rdf:resource="http://www.w3.org/2004/02/skos/core#Concept"/>
    <skos:prefLabel xml:lang="en">geographic names</skos:prefLabel>
    <skos:scopeNote xml:lang="en">Names by which cultural and geographic features are known.  Generally to be used for collections of names stored in gazetteers.</skos:scopeNote>
    <skos:broader rdf:resource="http://www.usgs.gov/science/USGSThesaurus/culture%20and%20demographics"/>
    <skos:related rdf:resource="http://www.usgs.gov/science/USGSThesaurus/gazetteers"/>
    <skos:inScheme rdf:resource="http://www.usgs.gov/science/USGSThesaurus"/>
  </rdf:Description>
  <rdf:Description about="http://www.usgs.gov/science/USGSThesaurus/laws%20and%20regulations">
    <rdf:type rdf:resource="http://www.w3.org/2004/02/skos/core#Concept"/>
    <skos:prefLabel xml:lang="en">laws and regulations</skos:prefLabel>
    <skos:scopeNote xml:lang="en">Legal statements of the government regarding actions people or corporations might undertake.</skos:scopeNote>
    <skos:altLabel xml:lang="en">legal processes</skos:altLabel>
    <skos:altLabel xml:lang="en">legislation</skos:altLabel>
    <skos:altLabel xml:lang="en">statutes</skos:altLabel>
    <skos:broader rdf:resource="http://www.usgs.gov/science/USGSThesaurus/culture%20and%20demographics"/>
    <skos:inScheme rdf:resource="http://www.usgs.gov/science/USGSThesaurus"/>
  </rdf:Description>
  <rdf:Description about="http://www.usgs.gov/science/USGSThesaurus/population%20%28human%29">
    <rdf:type rdf:resource="http://www.w3.org/2004/02/skos/core#Concept"/>
    <skos:prefLabel xml:lang="en">population (human)</skos:prefLabel>
    <skos:scopeNote xml:lang="en">Geographic distribution and temporal trends of human habitation in specific areas</skos:scopeNote>
    <skos:broader rdf:resource="http://www.usgs.gov/science/USGSThesaurus/culture%20and%20demographics"/>
    <skos:inScheme rdf:resource="http://www.usgs.gov/science/USGSThesaurus"/>
  </rdf:Description>
  <rdf:Description about="http://www.usgs.gov/science/USGSThesaurus/transportation">
    <rdf:type rdf:resource="http://www.w3.org/2004/02/skos/core#Concept"/>
    <skos:prefLabel xml:lang="en">transportation</skos:prefLabel>
    <skos:scopeNote xml:lang="en">Movement of people or materials from one place to another for economic, political, or recreational purposes.</skos:scopeNote>
    <skos:altLabel xml:lang="en">air transportation</skos:altLabel>
    <skos:altLabel xml:lang="en">aviation</skos:altLabel>
    <skos:altLabel xml:lang="en">ground transportation</skos:altLabel>
    <skos:broader rdf:resource="http://www.usgs.gov/science/USGSThesaurus/culture%20and%20demographics"/>
    <skos:inScheme rdf:resource="http://www.usgs.gov/science/USGSThesaurus"/>
  </rdf:Description>
  <rdf:Description about="http://www.usgs.gov/science/USGSThesaurus/earth%20characteristics">
    <rdf:type rdf:resource="http://www.w3.org/2004/02/skos/core#Concept"/>
    <skos:prefLabel xml:lang="en">earth characteristics</skos:prefLabel>
    <skos:scopeNote xml:lang="en">The measurable, definable properties and features of the earth.</skos:scopeNote>
    <skos:broader rdf:resource="http://www.usgs.gov/science/USGSThesaurus/topics"/>
    <skos:narrower rdf:resource="http://www.usgs.gov/science/USGSThesaurus/atmospheric%20properties"/>
    <skos:narrower rdf:resource="http://www.usgs.gov/science/USGSThesaurus/earth%20material%20properties"/>
    <skos:narrower rdf:resource="http://www.usgs.gov/science/USGSThesaurus/earth%20structure"/>
    <skos:narrower rdf:resource="http://www.usgs.gov/science/USGSThesaurus/geologic%20history"/>
    <skos:narrower rdf:resource="http://www.usgs.gov/science/USGSThesaurus/geologic%20structure"/>
    <skos:narrower rdf:resource="http://www.usgs.gov/science/USGSThesaurus/gravitational%20field%20%28earth%29"/>
    <skos:narrower rdf:resource="http://www.usgs.gov/science/USGSThesaurus/land%20surface%20characteristics"/>
    <skos:narrower rdf:resource="http://www.usgs.gov/science/USGSThesaurus/magnetic%20field%20%28earth%29"/>
    <skos:narrower rdf:resource="http://www.usgs.gov/science/USGSThesaurus/ocean%20characteristics"/>
    <skos:narrower rdf:resource="http://www.usgs.gov/science/USGSThesaurus/rocks%20and%20deposits"/>
    <skos:narrower rdf:resource="http://www.usgs.gov/science/USGSThesaurus/snow%20and%20ice%20cover"/>
    <skos:narrower rdf:resource="http://www.usgs.gov/science/USGSThesaurus/stratigraphic%20sections"/>
    <skos:narrower rdf:resource="http://www.usgs.gov/science/USGSThesaurus/topography"/>
    <skos:related rdf:resource="http://www.usgs.gov/science/USGSThesaurus/earth%20sciences"/>
    <skos:inScheme rdf:resource="http://www.usgs.gov/science/USGSThesaurus"/>
  </rdf:Description>
  <rdf:Description about="http://www.usgs.gov/science/USGSThesaurus/atmospheric%20properties">
    <rdf:type rdf:resource="http://www.w3.org/2004/02/skos/core#Concept"/>
    <skos:prefLabel xml:lang="en">atmospheric properties</skos:prefLabel>
    <skos:scopeNote xml:lang="en">Characteristics of the mass of gases surrounding the earth  such as composition, temperature, pressure, and humidity.</skos:scopeNote>
    <skos:altLabel xml:lang="en">atmosphere properties</skos:altLabel>
    <skos:broader rdf:resource="http://www.usgs.gov/science/USGSThesaurus/earth%20characteristics"/>
    <skos:narrower rdf:resource="http://www.usgs.gov/science/USGSThesaurus/air%20temperature"/>
    <skos:narrower rdf:resource="http://www.usgs.gov/science/USGSThesaurus/atmospheric%20composition"/>
    <skos:related rdf:resource="http://www.usgs.gov/science/USGSThesaurus/atmospheric%20and%20climatic%20processes"/>
    <skos:related rdf:resource="http://www.usgs.gov/science/USGSThesaurus/atmospheric%20sciences"/>
    <skos:inScheme rdf:resource="http://www.usgs.gov/science/USGSThesaurus"/>
  </rdf:Description>
  <rdf:Description about="http://www.usgs.gov/science/USGSThesaurus/air%20temperature">
    <rdf:type rdf:resource="http://www.w3.org/2004/02/skos/core#Concept"/>
    <skos:prefLabel xml:lang="en">air temperature</skos:prefLabel>
    <skos:scopeNote xml:lang="en"></skos:scopeNote>
    <skos:altLabel xml:lang="en">temperature (air)</skos:altLabel>
    <skos:broader rdf:resource="http://www.usgs.gov/science/USGSThesaurus/atmospheric%20properties"/>
    <skos:related rdf:resource="http://www.usgs.gov/science/USGSThesaurus/atmospheric%20sciences"/>
    <skos:inScheme rdf:resource="http://www.usgs.gov/science/USGSThesaurus"/>
  </rdf:Description>
  <rdf:Description about="http://www.usgs.gov/science/USGSThesaurus/atmospheric%20composition">
    <rdf:type rdf:resource="http://www.w3.org/2004/02/skos/core#Concept"/>
    <skos:prefLabel xml:lang="en">atmospheric composition</skos:prefLabel>
    <skos:scopeNote xml:lang="en">Components of the mass of gases that surrounds a planet.  The earth's atmosphere consists of nitrogen, oxygen, and small portions of other gases.</skos:scopeNote>
    <!--FOR air pollution USE atmospheric composition WITH contamination and pollution-->
    <skos:altLabel xml:lang="en">air pollution</skos:altLabel>
    <skos:broader rdf:resource="http://www.usgs.gov/science/USGSThesaurus/atmospheric%20properties"/>
    <skos:narrower rdf:resource="http://www.usgs.gov/science/USGSThesaurus/greenhouse%20gases"/>
    <skos:narrower rdf:resource="http://www.usgs.gov/science/USGSThesaurus/ozone%20layer"/>
    <skos:related rdf:resource="http://www.usgs.gov/science/USGSThesaurus/atmospheric%20sciences"/>
    <skos:inScheme rdf:resource="http://www.usgs.gov/science/USGSThesaurus"/>
  </rdf:Description>
  <rdf:Description about="http://www.usgs.gov/science/USGSThesaurus/greenhouse%20gases">
    <rdf:type rdf:resource="http://www.w3.org/2004/02/skos/core#Concept"/>
    <skos:prefLabel xml:lang="en">greenhouse gases</skos:prefLabel>
    <skos:scopeNote xml:lang="en">Atmospheric gases, including carbon dioxide, fluorocarbons, methane, nitrous oxide, sulfur hexafluoride, ozone, and water vapor, that trap radiant (infrared) energy keeping the earth's surface warmer than it would otherwise be.</skos:scopeNote>
    <skos:broader rdf:resource="http://www.usgs.gov/science/USGSThesaurus/atmospheric%20composition"/>
    <skos:related rdf:resource="http://www.usgs.gov/science/USGSThesaurus/atmospheric%20sciences"/>
    <skos:related rdf:resource="http://www.usgs.gov/science/USGSThesaurus/climate%20change"/>
    <skos:related rdf:resource="http://www.usgs.gov/science/USGSThesaurus/ozone%20layer"/>
    <skos:related rdf:resource="http://www.usgs.gov/science/USGSThesaurus/greenhouse%20effect"/>
    <skos:inScheme rdf:resource="http://www.usgs.gov/science/USGSThesaurus"/>
  </rdf:Description>
  <rdf:Description about="http://www.usgs.gov/science/USGSThesaurus/ozone%20layer">
    <rdf:type rdf:resource="http://www.w3.org/2004/02/skos/core#Concept"/>
    <skos:prefLabel xml:lang="en">ozone layer</skos:prefLabel>
    <skos:scopeNote xml:lang="en">Upper atmosphere layer composed of ozone, a gas made up of molecules comprised of three oxygen atoms, which helps to shield the earth from ultraviolet rays.</skos:scopeNote>
    <skos:altLabel xml:lang="en">ozonesphere</skos:altLabel>
    <skos:broader rdf:resource="http://www.usgs.gov/science/USGSThesaurus/atmospheric%20composition"/>
    <skos:related rdf:resource="http://www.usgs.gov/science/USGSThesaurus/atmospheric%20sciences"/>
    <skos:related rdf:resource="http://www.usgs.gov/science/USGSThesaurus/greenhouse%20gases"/>
    <skos:inScheme rdf:resource="http://www.usgs.gov/science/USGSThesaurus"/>
  </rdf:Description>
  <rdf:Description about="http://www.usgs.gov/science/USGSThesaurus/earth%20material%20properties">
    <rdf:type rdf:resource="http://www.w3.org/2004/02/skos/core#Concept"/>
    <skos:prefLabel xml:lang="en">earth material properties</skos:prefLabel>
    <skos:scopeNote xml:lang="en">Physical characteristics of rocks and unconsolidated earth materials such as soils and sediments.</skos:scopeNote>
    <skos:broader rdf:resource="http://www.usgs.gov/science/USGSThesaurus/earth%20characteristics"/>
    <skos:narrower rdf:resource="http://www.usgs.gov/science/USGSThesaurus/bulk%20density"/>
    <skos:narrower rdf:resource="http://www.usgs.gov/science/USGSThesaurus/magnetism"/>
    <skos:narrower rdf:resource="http://www.usgs.gov/science/USGSThesaurus/permeability"/>
    <skos:narrower rdf:resource="http://www.usgs.gov/science/USGSThesaurus/porosity"/>
    <skos:narrower rdf:resource="http://www.usgs.gov/science/USGSThesaurus/radioactivity"/>
    <skos:narrower rdf:resource="http://www.usgs.gov/science/USGSThesaurus/resistivity"/>
    <skos:narrower rdf:resource="http://www.usgs.gov/science/USGSThesaurus/soil%20moisture"/>
    <skos:narrower rdf:resource="http://www.usgs.gov/science/USGSThesaurus/soil%20temperature"/>
    <skos:inScheme rdf:resource="http://www.usgs.gov/science/USGSThesaurus"/>
  </rdf:Description>
  <rdf:Description about="http://www.usgs.gov/science/USGSThesaurus/bulk%20density">
    <rdf:type rdf:resource="http://www.w3.org/2004/02/skos/core#Concept"/>
    <skos:prefLabel xml:lang="en">bulk density</skos:prefLabel>
    <skos:scopeNote xml:lang="en">Overall density of an unconsolidated earth material.</skos:scopeNote>
    <skos:broader rdf:resource="http://www.usgs.gov/science/USGSThesaurus/earth%20material%20properties"/>
    <skos:inScheme rdf:resource="http://www.usgs.gov/science/USGSThesaurus"/>
  </rdf:Description>
  <rdf:Description about="http://www.usgs.gov/science/USGSThesaurus/magnetism">
    <rdf:type rdf:resource="http://www.w3.org/2004/02/skos/core#Concept"/>
    <skos:prefLabel xml:lang="en">magnetism</skos:prefLabel>
    <skos:scopeNote xml:lang="en">Strength and orientation of the permanent magnetic field in a given sample of an earth material</skos:scopeNote>
    <skos:broader rdf:resource="http://www.usgs.gov/science/USGSThesaurus/earth%20material%20properties"/>
    <skos:narrower rdf:resource="http://www.usgs.gov/science/USGSThesaurus/magnetic%20susceptibility"/>
    <skos:narrower rdf:resource="http://www.usgs.gov/science/USGSThesaurus/remanent%20magnetism"/>
    <skos:inScheme rdf:resource="http://www.usgs.gov/science/USGSThesaurus"/>
  </rdf:Description>
  <rdf:Description about="http://www.usgs.gov/science/USGSThesaurus/magnetic%20susceptibility">
    <rdf:type rdf:resource="http://www.w3.org/2004/02/skos/core#Concept"/>
    <skos:prefLabel xml:lang="en">magnetic susceptibility</skos:prefLabel>
    <skos:scopeNote xml:lang="en">Degree to which a rock type or other earth material can acquire and retain the orientation and intensity of an applied magnetic field.</skos:scopeNote>
    <skos:broader rdf:resource="http://www.usgs.gov/science/USGSThesaurus/magnetism"/>
    <skos:inScheme rdf:resource="http://www.usgs.gov/science/USGSThesaurus"/>
  </rdf:Description>
  <rdf:Description about="http://www.usgs.gov/science/USGSThesaurus/remanent%20magnetism">
    <rdf:type rdf:resource="http://www.w3.org/2004/02/skos/core#Concept"/>
    <skos:prefLabel xml:lang="en">remanent magnetism</skos:prefLabel>
    <skos:scopeNote xml:lang="en">Magnetic characteristic of rocks and deposits reflective of the earth's magnetic field at the time of the deposit's formation.</skos:scopeNote>
    <skos:altLabel xml:lang="en">natural remanent magnetism</skos:altLabel>
    <skos:broader rdf:resource="http://www.usgs.gov/science/USGSThesaurus/magnetism"/>
    <skos:inScheme rdf:resource="http://www.usgs.gov/science/USGSThesaurus"/>
  </rdf:Description>
  <rdf:Description about="http://www.usgs.gov/science/USGSThesaurus/permeability">
    <rdf:type rdf:resource="http://www.w3.org/2004/02/skos/core#Concept"/>
    <skos:prefLabel xml:lang="en">permeability</skos:prefLabel>
    <skos:scopeNote xml:lang="en">The ability of fluids to pass through an earth material, typically depending on the connectedness of pore space in the material.</skos:scopeNote>
    <skos:altLabel xml:lang="en">soil permeability</skos:altLabel>
    <skos:broader rdf:resource="http://www.usgs.gov/science/USGSThesaurus/earth%20material%20properties"/>
    <skos:related rdf:resource="http://www.usgs.gov/science/USGSThesaurus/percolation"/>
    <skos:inScheme rdf:resource="http://www.usgs.gov/science/USGSThesaurus"/>
  </rdf:Description>
  <rdf:Description about="http://www.usgs.gov/science/USGSThesaurus/porosity">
    <rdf:type rdf:resource="http://www.w3.org/2004/02/skos/core#Concept"/>
    <skos:prefLabel xml:lang="en">porosity</skos:prefLabel>
    <skos:scopeNote xml:lang="en">The proportion of open space in a rock or unconsolidated material.</skos:scopeNote>
    <skos:altLabel xml:lang="en">interstices</skos:altLabel>
    <skos:altLabel xml:lang="en">soil porosity</skos:altLabel>
    <skos:broader rdf:resource="http://www.usgs.gov/science/USGSThesaurus/earth%20material%20properties"/>
    <skos:inScheme rdf:resource="http://www.usgs.gov/science/USGSThesaurus"/>
  </rdf:Description>
  <rdf:Description about="http://www.usgs.gov/science/USGSThesaurus/radioactivity">
    <rdf:type rdf:resource="http://www.w3.org/2004/02/skos/core#Concept"/>
    <skos:prefLabel xml:lang="en">radioactivity</skos:prefLabel>
    <skos:scopeNote xml:lang="en">Release of subatomic particles from earth materials.  Generally the energy of these particles is used to determine the chemical elements present.</skos:scopeNote>
    <skos:altLabel xml:lang="en">gamma ray emission</skos:altLabel>
    <skos:broader rdf:resource="http://www.usgs.gov/science/USGSThesaurus/earth%20material%20properties"/>
    <skos:inScheme rdf:resource="http://www.usgs.gov/science/USGSThesaurus"/>
  </rdf:Description>
  <rdf:Description about="http://www.usgs.gov/science/USGSThesaurus/resistivity">
    <rdf:type rdf:resource="http://www.w3.org/2004/02/skos/core#Concept"/>
    <skos:prefLabel xml:lang="en">resistivity</skos:prefLabel>
    <skos:scopeNote xml:lang="en">Electrical resistance of materials, often measured in boreholes.</skos:scopeNote>
    <skos:broader rdf:resource="http://www.usgs.gov/science/USGSThesaurus/earth%20material%20properties"/>
    <skos:inScheme rdf:resource="http://www.usgs.gov/science/USGSThesaurus"/>
  </rdf:Description>
  <rdf:Description about="http://www.usgs.gov/science/USGSThesaurus/soil%20moisture">
    <rdf:type rdf:resource="http://www.w3.org/2004/02/skos/core#Concept"/>
    <skos:prefLabel xml:lang="en">soil moisture</skos:prefLabel>
    <skos:scopeNote xml:lang="en">Water content of soil and other near-surface unconsolidated earth material</skos:scopeNote>
    <skos:broader rdf:resource="http://www.usgs.gov/science/USGSThesaurus/earth%20material%20properties"/>
    <skos:inScheme rdf:resource="http://www.usgs.gov/science/USGSThesaurus"/>
  </rdf:Description>
  <rdf:Description about="http://www.usgs.gov/science/USGSThesaurus/soil%20temperature">
    <rdf:type rdf:resource="http://www.w3.org/2004/02/skos/core#Concept"/>
    <skos:prefLabel xml:lang="en">soil temperature</skos:prefLabel>
    <skos:scopeNote xml:lang="en">Temperature and temperature gradients in soil and other near-surface unconsolidated earth materials</skos:scopeNote>
    <skos:broader rdf:resource="http://www.usgs.gov/science/USGSThesaurus/earth%20material%20properties"/>
    <skos:inScheme rdf:resource="http://www.usgs.gov/science/USGSThesaurus"/>
  </rdf:Description>
  <rdf:Description about="http://www.usgs.gov/science/USGSThesaurus/earth%20structure">
    <rdf:type rdf:resource="http://www.w3.org/2004/02/skos/core#Concept"/>
    <skos:prefLabel xml:lang="en">earth structure</skos:prefLabel>
    <skos:scopeNote xml:lang="en">Major interior structural features of the planet earth.</skos:scopeNote>
    <skos:broader rdf:resource="http://www.usgs.gov/science/USGSThesaurus/earth%20characteristics"/>
    <skos:narrower rdf:resource="http://www.usgs.gov/science/USGSThesaurus/core%20%28earth%29"/>
    <skos:narrower rdf:resource="http://www.usgs.gov/science/USGSThesaurus/crust%20%28earth%29"/>
    <skos:narrower rdf:resource="http://www.usgs.gov/science/USGSThesaurus/mantle%20%28earth%29"/>
    <skos:related rdf:resource="http://www.usgs.gov/science/USGSThesaurus/geologic%20structure"/>
    <skos:related rdf:resource="http://www.usgs.gov/science/USGSThesaurus/structural%20geology"/>
    <skos:related rdf:resource="http://www.usgs.gov/science/USGSThesaurus/tectonic%20processes"/>
    <skos:related rdf:resource="http://www.usgs.gov/science/USGSThesaurus/tectonophysics"/>
    <skos:inScheme rdf:resource="http://www.usgs.gov/science/USGSThesaurus"/>
  </rdf:Description>
  <rdf:Description about="http://www.usgs.gov/science/USGSThesaurus/core%20%28earth%29">
    <rdf:type rdf:resource="http://www.w3.org/2004/02/skos/core#Concept"/>
    <skos:prefLabel xml:lang="en">core (earth)</skos:prefLabel>
    <skos:scopeNote xml:lang="en">The superdense center of the earth composed of two layers: a liquid outer layer and a solid inner core of metallic iron-nickel alloy.</skos:scopeNote>
    <skos:broader rdf:resource="http://www.usgs.gov/science/USGSThesaurus/earth%20structure"/>
    <skos:narrower rdf:resource="http://www.usgs.gov/science/USGSThesaurus/inner%20core%20%28earth%29"/>
    <skos:narrower rdf:resource="http://www.usgs.gov/science/USGSThesaurus/outer%20core%20%28earth%29"/>
    <skos:related rdf:resource="http://www.usgs.gov/science/USGSThesaurus/geophysics"/>
    <skos:inScheme rdf:resource="http://www.usgs.gov/science/USGSThesaurus"/>
  </rdf:Description>
  <rdf:Description about="http://www.usgs.gov/science/USGSThesaurus/inner%20core%20%28earth%29">
    <rdf:type rdf:resource="http://www.w3.org/2004/02/skos/core#Concept"/>
    <skos:prefLabel xml:lang="en">inner core (earth)</skos:prefLabel>
    <skos:scopeNote xml:lang="en">The solid interior part of the earth's core, presumed to be composed principally of iron with an alloy of about 10 percent oxygen, sulfur, or nickel, or perhaps some combination of these three elements.  The inner core is about 1221 kilometers thick.</skos:scopeNote>
    <skos:broader rdf:resource="http://www.usgs.gov/science/USGSThesaurus/core%20%28earth%29"/>
    <skos:related rdf:resource="http://www.usgs.gov/science/USGSThesaurus/geophysics"/>
    <skos:inScheme rdf:resource="http://www.usgs.gov/science/USGSThesaurus"/>
  </rdf:Description>
  <rdf:Description about="http://www.usgs.gov/science/USGSThesaurus/outer%20core%20%28earth%29">
    <rdf:type rdf:resource="http://www.w3.org/2004/02/skos/core#Concept"/>
    <skos:prefLabel xml:lang="en">outer core (earth)</skos:prefLabel>
    <skos:scopeNote xml:lang="en">Outer zone of the earth's core between the mantle and the inner core.</skos:scopeNote>
    <skos:broader rdf:resource="http://www.usgs.gov/science/USGSThesaurus/core%20%28earth%29"/>
    <skos:related rdf:resource="http://www.usgs.gov/science/USGSThesaurus/geophysics"/>
    <skos:inScheme rdf:resource="http://www.usgs.gov/science/USGSThesaurus"/>
  </rdf:Description>
  <rdf:Description about="http://www.usgs.gov/science/USGSThesaurus/crust%20%28earth%29">
    <rdf:type rdf:resource="http://www.w3.org/2004/02/skos/core#Concept"/>
    <skos:prefLabel xml:lang="en">crust (earth)</skos:prefLabel>
    <skos:scopeNote xml:lang="en">The outermost layer of the earth which is relatively thin, of lower density than the core, and rocky.</skos:scopeNote>
    <skos:broader rdf:resource="http://www.usgs.gov/science/USGSThesaurus/earth%20structure"/>
    <skos:narrower rdf:resource="http://www.usgs.gov/science/USGSThesaurus/lithosphere"/>
    <skos:related rdf:resource="http://www.usgs.gov/science/USGSThesaurus/tectonophysics"/>
    <skos:inScheme rdf:resource="http://www.usgs.gov/science/USGSThesaurus"/>
  </rdf:Description>
  <rdf:Description about="http://www.usgs.gov/science/USGSThesaurus/lithosphere">
    <rdf:type rdf:resource="http://www.w3.org/2004/02/skos/core#Concept"/>
    <skos:prefLabel xml:lang="en">lithosphere</skos:prefLabel>
    <skos:scopeNote xml:lang="en">The solid outer zone of the earth comprising the crust and the upper layer of the mantle.</skos:scopeNote>
    <skos:broader rdf:resource="http://www.usgs.gov/science/USGSThesaurus/crust%20%28earth%29"/>
    <skos:narrower rdf:resource="http://www.usgs.gov/science/USGSThesaurus/continental%20lithosphere"/>
    <skos:narrower rdf:resource="http://www.usgs.gov/science/USGSThesaurus/oceanic%20lithosphere"/>
    <skos:related rdf:resource="http://www.usgs.gov/science/USGSThesaurus/mantle%20%28earth%29"/>
    <skos:related rdf:resource="http://www.usgs.gov/science/USGSThesaurus/rocks%20and%20deposits"/>
    <skos:related rdf:resource="http://www.usgs.gov/science/USGSThesaurus/tectonophysics"/>
    <skos:inScheme rdf:resource="http://www.usgs.gov/science/USGSThesaurus"/>
  </rdf:Description>
  <rdf:Description about="http://www.usgs.gov/science/USGSThesaurus/continental%20lithosphere">
    <rdf:type rdf:resource="http://www.w3.org/2004/02/skos/core#Concept"/>
    <skos:prefLabel xml:lang="en">continental lithosphere</skos:prefLabel>
    <skos:scopeNote xml:lang="en">The earth's hard, outermost shell comprised of the crust and the upper part of the mantle.</skos:scopeNote>
    <skos:altLabel xml:lang="en">craton</skos:altLabel>
    <skos:broader rdf:resource="http://www.usgs.gov/science/USGSThesaurus/lithosphere"/>
    <skos:related rdf:resource="http://www.usgs.gov/science/USGSThesaurus/tectonophysics"/>
    <skos:inScheme rdf:resource="http://www.usgs.gov/science/USGSThesaurus"/>
  </rdf:Description>
  <rdf:Description about="http://www.usgs.gov/science/USGSThesaurus/oceanic%20lithosphere">
    <rdf:type rdf:resource="http://www.w3.org/2004/02/skos/core#Concept"/>
    <skos:prefLabel xml:lang="en">oceanic lithosphere</skos:prefLabel>
    <skos:scopeNote xml:lang="en">The solid outer zone of the earth, covered by seawater, and comprised of the crust and the upper layer of the mantle.</skos:scopeNote>
    <skos:broader rdf:resource="http://www.usgs.gov/science/USGSThesaurus/lithosphere"/>
    <skos:related rdf:resource="http://www.usgs.gov/science/USGSThesaurus/ocean%20characteristics"/>
    <skos:related rdf:resource="http://www.usgs.gov/science/USGSThesaurus/sea-floor%20characteristics"/>
    <skos:related rdf:resource="http://www.usgs.gov/science/USGSThesaurus/tectonophysics"/>
    <skos:inScheme rdf:resource="http://www.usgs.gov/science/USGSThesaurus"/>
  </rdf:Description>
  <rdf:Description about="http://www.usgs.gov/science/USGSThesaurus/mantle%20%28earth%29">
    <rdf:type rdf:resource="http://www.w3.org/2004/02/skos/core#Concept"/>
    <skos:prefLabel xml:lang="en">mantle (earth)</skos:prefLabel>
    <skos:scopeNote xml:lang="en">Zone of earth's interior between the crust and the core.  It is 2,900 kilometers (1,740 miles) thick and consists of a dense upper layer (upper mantle) and a partially molten lower layer (lower mantle), separated by a transition zone.</skos:scopeNote>
    <skos:broader rdf:resource="http://www.usgs.gov/science/USGSThesaurus/earth%20structure"/>
    <skos:narrower rdf:resource="http://www.usgs.gov/science/USGSThesaurus/asthenosphere"/>
    <skos:related rdf:resource="http://www.usgs.gov/science/USGSThesaurus/geophysics"/>
    <skos:related rdf:resource="http://www.usgs.gov/science/USGSThesaurus/lithosphere"/>
    <skos:inScheme rdf:resource="http://www.usgs.gov/science/USGSThesaurus"/>
  </rdf:Description>
  <rdf:Description about="http://www.usgs.gov/science/USGSThesaurus/asthenosphere">
    <rdf:type rdf:resource="http://www.w3.org/2004/02/skos/core#Concept"/>
    <skos:prefLabel xml:lang="en">asthenosphere</skos:prefLabel>
    <skos:scopeNote xml:lang="en">A layer of the earth within the upper mantle and directly below the lithosphere. This layer has a semi-solid consistency that reaches to about 200 kilometers (124 miles) below the surface.</skos:scopeNote>
    <skos:broader rdf:resource="http://www.usgs.gov/science/USGSThesaurus/mantle%20%28earth%29"/>
    <skos:related rdf:resource="http://www.usgs.gov/science/USGSThesaurus/tectonophysics"/>
    <skos:inScheme rdf:resource="http://www.usgs.gov/science/USGSThesaurus"/>
  </rdf:Description>
  <rdf:Description about="http://www.usgs.gov/science/USGSThesaurus/geologic%20history">
    <rdf:type rdf:resource="http://www.w3.org/2004/02/skos/core#Concept"/>
    <skos:prefLabel xml:lang="en">geologic history</skos:prefLabel>
    <skos:scopeNote xml:lang="en">Record (and inferred reconstruction) of the origin and development of the earth since its formation.</skos:scopeNote>
    <skos:altLabel xml:lang="en">chronostratigraphy</skos:altLabel>
    <skos:altLabel xml:lang="en">geohistory</skos:altLabel>
    <skos:broader rdf:resource="http://www.usgs.gov/science/USGSThesaurus/earth%20characteristics"/>
    <skos:narrower rdf:resource="http://www.usgs.gov/science/USGSThesaurus/earth%20history"/>
    <skos:related rdf:resource="http://www.usgs.gov/science/USGSThesaurus/geology"/>
    <skos:related rdf:resource="http://www.usgs.gov/science/USGSThesaurus/paleontology"/>
    <skos:related rdf:resource="http://www.usgs.gov/science/USGSThesaurus/paleoseismology"/>
    <skos:related rdf:resource="http://www.usgs.gov/science/USGSThesaurus/stratigraphy"/>
    <skos:related rdf:resource="http://www.usgs.gov/science/USGSThesaurus/biostratigraphy"/>
    <skos:related rdf:resource="http://www.usgs.gov/science/USGSThesaurus/lithostratigraphy"/>
    <skos:inScheme rdf:resource="http://www.usgs.gov/science/USGSThesaurus"/>
  </rdf:Description>
  <rdf:Description about="http://www.usgs.gov/science/USGSThesaurus/earth%20history">
    <rdf:type rdf:resource="http://www.w3.org/2004/02/skos/core#Concept"/>
    <skos:prefLabel xml:lang="en">earth history</skos:prefLabel>
    <skos:scopeNote xml:lang="en">The structural and compositional changes that the earth has undergone from its formation. Use for discussions of the whole earth (or large sections of it) instead of regional studies.</skos:scopeNote>
    <skos:broader rdf:resource="http://www.usgs.gov/science/USGSThesaurus/geologic%20history"/>
    <skos:related rdf:resource="http://www.usgs.gov/science/USGSThesaurus/geochemistry"/>
    <skos:related rdf:resource="http://www.usgs.gov/science/USGSThesaurus/geology"/>
    <skos:related rdf:resource="http://www.usgs.gov/science/USGSThesaurus/tectonophysics"/>
    <skos:inScheme rdf:resource="http://www.usgs.gov/science/USGSThesaurus"/>
  </rdf:Description>
  <rdf:Description about="http://www.usgs.gov/science/USGSThesaurus/geologic%20structure">
    <rdf:type rdf:resource="http://www.w3.org/2004/02/skos/core#Concept"/>
    <skos:prefLabel xml:lang="en">geologic structure</skos:prefLabel>
    <skos:scopeNote xml:lang="en">General position of rocks in an area, and geometrical relationships among rocks.</skos:scopeNote>
    <skos:broader rdf:resource="http://www.usgs.gov/science/USGSThesaurus/earth%20characteristics"/>
    <skos:narrower rdf:resource="http://www.usgs.gov/science/USGSThesaurus/foliation%20%28geologic%29"/>
    <skos:narrower rdf:resource="http://www.usgs.gov/science/USGSThesaurus/lineation%20%28geologic%29"/>
    <skos:narrower rdf:resource="http://www.usgs.gov/science/USGSThesaurus/structure%20contours"/>
    <skos:related rdf:resource="http://www.usgs.gov/science/USGSThesaurus/earth%20structure"/>
    <skos:related rdf:resource="http://www.usgs.gov/science/USGSThesaurus/stratigraphic%20sections"/>
    <skos:related rdf:resource="http://www.usgs.gov/science/USGSThesaurus/structural%20geology"/>
    <skos:related rdf:resource="http://www.usgs.gov/science/USGSThesaurus/deformation%20%28geologic%29"/>
    <skos:related rdf:resource="http://www.usgs.gov/science/USGSThesaurus/geologic%20maps"/>
    <skos:inScheme rdf:resource="http://www.usgs.gov/science/USGSThesaurus"/>
  </rdf:Description>
  <rdf:Description about="http://www.usgs.gov/science/USGSThesaurus/foliation%20%28geologic%29">
    <rdf:type rdf:resource="http://www.w3.org/2004/02/skos/core#Concept"/>
    <skos:prefLabel xml:lang="en">foliation (geologic)</skos:prefLabel>
    <skos:scopeNote xml:lang="en">The property of rocks or glaciers splitting into thin layers or plates due to the orientation of crystals and dynamic movement.</skos:scopeNote>
    <skos:broader rdf:resource="http://www.usgs.gov/science/USGSThesaurus/geologic%20structure"/>
    <skos:related rdf:resource="http://www.usgs.gov/science/USGSThesaurus/glaciation"/>
    <skos:related rdf:resource="http://www.usgs.gov/science/USGSThesaurus/structural%20geology"/>
    <skos:related rdf:resource="http://www.usgs.gov/science/USGSThesaurus/tectonic%20processes"/>
    <skos:inScheme rdf:resource="http://www.usgs.gov/science/USGSThesaurus"/>
  </rdf:Description>
  <rdf:Description about="http://www.usgs.gov/science/USGSThesaurus/lineation%20%28geologic%29">
    <rdf:type rdf:resource="http://www.w3.org/2004/02/skos/core#Concept"/>
    <skos:prefLabel xml:lang="en">lineation (geologic)</skos:prefLabel>
    <skos:scopeNote xml:lang="en">Linear topographic feature on the earth's surface or in rocks.</skos:scopeNote>
    <skos:altLabel xml:lang="en">lineaments</skos:altLabel>
    <skos:broader rdf:resource="http://www.usgs.gov/science/USGSThesaurus/geologic%20structure"/>
    <skos:related rdf:resource="http://www.usgs.gov/science/USGSThesaurus/structural%20geology"/>
    <skos:related rdf:resource="http://www.usgs.gov/science/USGSThesaurus/tectonic%20processes"/>
    <skos:inScheme rdf:resource="http://www.usgs.gov/science/USGSThesaurus"/>
  </rdf:Description>
  <rdf:Description about="http://www.usgs.gov/science/USGSThesaurus/structure%20contours">
    <rdf:type rdf:resource="http://www.w3.org/2004/02/skos/core#Concept"/>
    <skos:prefLabel xml:lang="en">structure contours</skos:prefLabel>
    <skos:scopeNote xml:lang="en">Gridding and contouring lines drawn on geologic maps to depict boundaries of structural features.</skos:scopeNote>
    <!--FOR depth-to maps USE structure contours WITH maps and atlases-->
    <skos:altLabel xml:lang="en">depth-to maps</skos:altLabel>
    <!--FOR thickness maps USE structure contours WITH maps and atlases-->
    <skos:altLabel xml:lang="en">thickness maps</skos:altLabel>
    <skos:broader rdf:resource="http://www.usgs.gov/science/USGSThesaurus/geologic%20structure"/>
    <skos:related rdf:resource="http://www.usgs.gov/science/USGSThesaurus/structural%20geology"/>
    <skos:inScheme rdf:resource="http://www.usgs.gov/science/USGSThesaurus"/>
  </rdf:Description>
  <rdf:Description about="http://www.usgs.gov/science/USGSThesaurus/gravitational%20field%20%28earth%29">
    <rdf:type rdf:resource="http://www.w3.org/2004/02/skos/core#Concept"/>
    <skos:prefLabel xml:lang="en">gravitational field (earth)</skos:prefLabel>
    <skos:scopeNote xml:lang="en">Region or space around earth's mass which exerts a force that mutually attracts other masses in proportion to the product of the two masses and the distance between them.</skos:scopeNote>
    <!--FOR gravity anomaly maps USE gravitational field (earth) WITH maps and atlases-->
    <skos:altLabel xml:lang="en">gravity anomaly maps</skos:altLabel>
    <skos:altLabel xml:lang="en">gravity field</skos:altLabel>
    <skos:altLabel xml:lang="en">gravity</skos:altLabel>
    <skos:broader rdf:resource="http://www.usgs.gov/science/USGSThesaurus/earth%20characteristics"/>
    <skos:narrower rdf:resource="http://www.usgs.gov/science/USGSThesaurus/bouguer%20anomaly"/>
    <skos:narrower rdf:resource="http://www.usgs.gov/science/USGSThesaurus/free-air%20anomaly"/>
    <skos:narrower rdf:resource="http://www.usgs.gov/science/USGSThesaurus/isostatic%20anomaly"/>
    <skos:related rdf:resource="http://www.usgs.gov/science/USGSThesaurus/geophysics"/>
    <skos:inScheme rdf:resource="http://www.usgs.gov/science/USGSThesaurus"/>
  </rdf:Description>
  <rdf:Description about="http://www.usgs.gov/science/USGSThesaurus/bouguer%20anomaly">
    <rdf:type rdf:resource="http://www.w3.org/2004/02/skos/core#Concept"/>
    <skos:prefLabel xml:lang="en">bouguer anomaly</skos:prefLabel>
    <skos:scopeNote xml:lang="en">Gravity anomaly corrected to remove the effects of topography using knowledge of the terrain in the area surrounding the measurement station.</skos:scopeNote>
    <skos:broader rdf:resource="http://www.usgs.gov/science/USGSThesaurus/gravitational%20field%20%28earth%29"/>
    <skos:inScheme rdf:resource="http://www.usgs.gov/science/USGSThesaurus"/>
  </rdf:Description>
  <rdf:Description about="http://www.usgs.gov/science/USGSThesaurus/free-air%20anomaly">
    <rdf:type rdf:resource="http://www.w3.org/2004/02/skos/core#Concept"/>
    <skos:prefLabel xml:lang="en">free-air anomaly</skos:prefLabel>
    <skos:scopeNote xml:lang="en">Gravity anomaly corrected for elevation of the location at which the measurements were made.</skos:scopeNote>
    <skos:broader rdf:resource="http://www.usgs.gov/science/USGSThesaurus/gravitational%20field%20%28earth%29"/>
    <skos:inScheme rdf:resource="http://www.usgs.gov/science/USGSThesaurus"/>
  </rdf:Description>
  <rdf:Description about="http://www.usgs.gov/science/USGSThesaurus/isostatic%20anomaly">
    <rdf:type rdf:resource="http://www.w3.org/2004/02/skos/core#Concept"/>
    <skos:prefLabel xml:lang="en">isostatic anomaly</skos:prefLabel>
    <skos:scopeNote xml:lang="en">Gravity anomaly corrected for the effects of low-density rocks underlying mountains.</skos:scopeNote>
    <skos:broader rdf:resource="http://www.usgs.gov/science/USGSThesaurus/gravitational%20field%20%28earth%29"/>
    <skos:inScheme rdf:resource="http://www.usgs.gov/science/USGSThesaurus"/>
  </rdf:Description>
  <rdf:Description about="http://www.usgs.gov/science/USGSThesaurus/land%20surface%20characteristics">
    <rdf:type rdf:resource="http://www.w3.org/2004/02/skos/core#Concept"/>
    <skos:prefLabel xml:lang="en">land surface characteristics</skos:prefLabel>
    <skos:scopeNote xml:lang="en">Features and attributes of earth's land surface.</skos:scopeNote>
    <skos:altLabel xml:lang="en">landscape</skos:altLabel>
    <skos:altLabel xml:lang="en">physiography</skos:altLabel>
    <skos:broader rdf:resource="http://www.usgs.gov/science/USGSThesaurus/earth%20characteristics"/>
    <skos:narrower rdf:resource="http://www.usgs.gov/science/USGSThesaurus/karst"/>
    <skos:related rdf:resource="http://www.usgs.gov/science/USGSThesaurus/geography"/>
    <skos:related rdf:resource="http://www.usgs.gov/science/USGSThesaurus/geomorphology"/>
    <skos:related rdf:resource="http://www.usgs.gov/science/USGSThesaurus/sea-floor%20characteristics"/>
    <skos:inScheme rdf:resource="http://www.usgs.gov/science/USGSThesaurus"/>
  </rdf:Description>
  <rdf:Description about="http://www.usgs.gov/science/USGSThesaurus/karst">
    <rdf:type rdf:resource="http://www.w3.org/2004/02/skos/core#Concept"/>
    <skos:prefLabel xml:lang="en">karst</skos:prefLabel>
    <skos:scopeNote xml:lang="en">Landscape characterized by dissolution features in carbonate or evaporite terranes, often containing caves and sinkholes.</skos:scopeNote>
    <skos:altLabel xml:lang="en">karst topography</skos:altLabel>
    <skos:altLabel xml:lang="en">karstic</skos:altLabel>
    <skos:broader rdf:resource="http://www.usgs.gov/science/USGSThesaurus/land%20surface%20characteristics"/>
    <skos:related rdf:resource="http://www.usgs.gov/science/USGSThesaurus/sinkhole%20formation"/>
    <skos:inScheme rdf:resource="http://www.usgs.gov/science/USGSThesaurus"/>
  </rdf:Description>
  <rdf:Description about="http://www.usgs.gov/science/USGSThesaurus/magnetic%20field%20%28earth%29">
    <rdf:type rdf:resource="http://www.w3.org/2004/02/skos/core#Concept"/>
    <skos:prefLabel xml:lang="en">magnetic field (earth)</skos:prefLabel>
    <skos:scopeNote xml:lang="en">The magnetic region surrounding earth.  It is generated by the dipolar characteristic of earth's core whereby earth itself acts as a great spherical magnet with poles near, but not exactly at, the North and South poles.</skos:scopeNote>
    <skos:altLabel xml:lang="en">geomagnetic field</skos:altLabel>
    <skos:altLabel xml:lang="en">geomagnetics</skos:altLabel>
    <skos:altLabel xml:lang="en">geomagnetism</skos:altLabel>
    <!--FOR magnetic anomaly maps USE magnetic field (earth) WITH maps and atlases-->
    <skos:altLabel xml:lang="en">magnetic anomaly maps</skos:altLabel>
    <skos:altLabel xml:lang="en">magnetic field</skos:altLabel>
    <skos:altLabel xml:lang="en">magnetosphere</skos:altLabel>
    <skos:broader rdf:resource="http://www.usgs.gov/science/USGSThesaurus/earth%20characteristics"/>
    <skos:related rdf:resource="http://www.usgs.gov/science/USGSThesaurus/geophysics"/>
    <skos:related rdf:resource="http://www.usgs.gov/science/USGSThesaurus/magnetic%20storms"/>
    <skos:inScheme rdf:resource="http://www.usgs.gov/science/USGSThesaurus"/>
  </rdf:Description>
  <rdf:Description about="http://www.usgs.gov/science/USGSThesaurus/ocean%20characteristics">
    <rdf:type rdf:resource="http://www.w3.org/2004/02/skos/core#Concept"/>
    <skos:prefLabel xml:lang="en">ocean characteristics</skos:prefLabel>
    <skos:scopeNote xml:lang="en">The attributes and process of seas and oceans.</skos:scopeNote>
    <!--FOR ocean monitoring USE ocean characteristics WITH field inventory and monitoring-->
    <skos:altLabel xml:lang="en">ocean monitoring</skos:altLabel>
    <!--FOR oceans USE ocean characteristics WITH ocean processes-->
    <skos:altLabel xml:lang="en">oceans</skos:altLabel>
    <skos:broader rdf:resource="http://www.usgs.gov/science/USGSThesaurus/earth%20characteristics"/>
    <skos:narrower rdf:resource="http://www.usgs.gov/science/USGSThesaurus/ocean%20salinity"/>
    <skos:narrower rdf:resource="http://www.usgs.gov/science/USGSThesaurus/ocean%20temperature"/>
    <skos:narrower rdf:resource="http://www.usgs.gov/science/USGSThesaurus/sea-floor%20characteristics"/>
    <skos:narrower rdf:resource="http://www.usgs.gov/science/USGSThesaurus/sea-level%20change"/>
    <skos:related rdf:resource="http://www.usgs.gov/science/USGSThesaurus/marine%20chemistry"/>
    <skos:related rdf:resource="http://www.usgs.gov/science/USGSThesaurus/marine%20geophysics"/>
    <skos:related rdf:resource="http://www.usgs.gov/science/USGSThesaurus/ocean%20processes"/>
    <skos:related rdf:resource="http://www.usgs.gov/science/USGSThesaurus/ocean%20sciences"/>
    <skos:related rdf:resource="http://www.usgs.gov/science/USGSThesaurus/oceanic%20lithosphere"/>
    <skos:related rdf:resource="http://www.usgs.gov/science/USGSThesaurus/surface%20water%20%28non-marine%29"/>
    <skos:related rdf:resource="http://www.usgs.gov/science/USGSThesaurus/water%20resources"/>
    <skos:related rdf:resource="http://www.usgs.gov/science/USGSThesaurus/sea%20ice%20concentration"/>
    <skos:inScheme rdf:resource="http://www.usgs.gov/science/USGSThesaurus"/>
  </rdf:Description>
  <rdf:Description about="http://www.usgs.gov/science/USGSThesaurus/ocean%20salinity">
    <rdf:type rdf:resource="http://www.w3.org/2004/02/skos/core#Concept"/>
    <skos:prefLabel xml:lang="en">ocean salinity</skos:prefLabel>
    <skos:scopeNote xml:lang="en">Measure of the percentage of dissolved salts in seawater.</skos:scopeNote>
    <skos:broader rdf:resource="http://www.usgs.gov/science/USGSThesaurus/ocean%20characteristics"/>
    <skos:related rdf:resource="http://www.usgs.gov/science/USGSThesaurus/marine%20chemistry"/>
    <skos:related rdf:resource="http://www.usgs.gov/science/USGSThesaurus/ocean%20sciences"/>
    <skos:related rdf:resource="http://www.usgs.gov/science/USGSThesaurus/salinity"/>
    <skos:inScheme rdf:resource="http://www.usgs.gov/science/USGSThesaurus"/>
  </rdf:Description>
  <rdf:Description about="http://www.usgs.gov/science/USGSThesaurus/ocean%20temperature">
    <rdf:type rdf:resource="http://www.w3.org/2004/02/skos/core#Concept"/>
    <skos:prefLabel xml:lang="en">ocean temperature</skos:prefLabel>
    <skos:scopeNote xml:lang="en">Distribution of heat in the oceans, including surface water, thermocline and mode waters, and deep waters.  Includes discussion and measures of both in-situ and potential temperature.</skos:scopeNote>
    <skos:altLabel xml:lang="en">temperature (ocean)</skos:altLabel>
    <skos:broader rdf:resource="http://www.usgs.gov/science/USGSThesaurus/ocean%20characteristics"/>
    <skos:narrower rdf:resource="http://www.usgs.gov/science/USGSThesaurus/sea%20surface%20temperature"/>
    <skos:related rdf:resource="http://www.usgs.gov/science/USGSThesaurus/atmospheric%20sciences"/>
    <skos:related rdf:resource="http://www.usgs.gov/science/USGSThesaurus/ocean%20sciences"/>
    <skos:inScheme rdf:resource="http://www.usgs.gov/science/USGSThesaurus"/>
  </rdf:Description>
  <rdf:Description about="http://www.usgs.gov/science/USGSThesaurus/sea%20surface%20temperature">
    <rdf:type rdf:resource="http://www.w3.org/2004/02/skos/core#Concept"/>
    <skos:prefLabel xml:lang="en">sea surface temperature</skos:prefLabel>
    <skos:scopeNote xml:lang="en">Observed temperature of surface ocean waters, typically encompassing the entire mixed layer. Some observational methods, however, may measure a much smaller depth range.  Includes temperature data obtained in-situ or by remote sensing methods.</skos:scopeNote>
    <skos:altLabel xml:lang="en">sst</skos:altLabel>
    <skos:altLabel xml:lang="en">temperature (sea surface)</skos:altLabel>
    <skos:altLabel xml:lang="en">sea-surface temperature</skos:altLabel>
    <skos:broader rdf:resource="http://www.usgs.gov/science/USGSThesaurus/ocean%20temperature"/>
    <skos:related rdf:resource="http://www.usgs.gov/science/USGSThesaurus/AVHRR"/>
    <skos:inScheme rdf:resource="http://www.usgs.gov/science/USGSThesaurus"/>
  </rdf:Description>
  <rdf:Description about="http://www.usgs.gov/science/USGSThesaurus/sea-floor%20characteristics">
    <rdf:type rdf:resource="http://www.w3.org/2004/02/skos/core#Concept"/>
    <skos:prefLabel xml:lang="en">sea-floor characteristics</skos:prefLabel>
    <skos:scopeNote xml:lang="en">Geomorphic features and geographic, compositional, and textural variation in the materials composing the ocean floor. Includes both large-scale structures (such as seamounts and rises) and fine-scale variations in rocks and deposits on the sea floor.</skos:scopeNote>
    <skos:altLabel xml:lang="en">ocean bottom characteristics</skos:altLabel>
    <skos:altLabel xml:lang="en">sea floor characteristics</skos:altLabel>
    <skos:altLabel xml:lang="en">seafloor characteristics</skos:altLabel>
    <skos:broader rdf:resource="http://www.usgs.gov/science/USGSThesaurus/ocean%20characteristics"/>
    <skos:narrower rdf:resource="http://www.usgs.gov/science/USGSThesaurus/sea-floor%20acoustic%20reflectivity"/>
    <skos:related rdf:resource="http://www.usgs.gov/science/USGSThesaurus/bathymetry"/>
    <skos:related rdf:resource="http://www.usgs.gov/science/USGSThesaurus/land%20surface%20characteristics"/>
    <skos:related rdf:resource="http://www.usgs.gov/science/USGSThesaurus/marine%20geology"/>
    <skos:related rdf:resource="http://www.usgs.gov/science/USGSThesaurus/ocean%20sciences"/>
    <skos:related rdf:resource="http://www.usgs.gov/science/USGSThesaurus/oceanic%20lithosphere"/>
    <skos:related rdf:resource="http://www.usgs.gov/science/USGSThesaurus/sidescan%20sonar"/>
    <skos:related rdf:resource="http://www.usgs.gov/science/USGSThesaurus/multibeam%20sonar"/>
    <skos:related rdf:resource="http://www.usgs.gov/science/USGSThesaurus/interferometric%20sonar"/>
    <skos:inScheme rdf:resource="http://www.usgs.gov/science/USGSThesaurus"/>
  </rdf:Description>
  <rdf:Description about="http://www.usgs.gov/science/USGSThesaurus/sea-floor%20acoustic%20reflectivity">
    <rdf:type rdf:resource="http://www.w3.org/2004/02/skos/core#Concept"/>
    <skos:prefLabel xml:lang="en">sea-floor acoustic reflectivity</skos:prefLabel>
    <skos:scopeNote xml:lang="en">Acoustic energy received by a sidescan sonar system, providing a measure of the roughness of the sea floor.</skos:scopeNote>
    <skos:altLabel xml:lang="en">sea-floor acoustic backscatter</skos:altLabel>
    <skos:altLabel xml:lang="en">backscatter (sea floor)</skos:altLabel>
    <skos:broader rdf:resource="http://www.usgs.gov/science/USGSThesaurus/sea-floor%20characteristics"/>
    <skos:related rdf:resource="http://www.usgs.gov/science/USGSThesaurus/sidescan%20sonar"/>
    <skos:related rdf:resource="http://www.usgs.gov/science/USGSThesaurus/interferometric%20sonar"/>
    <skos:inScheme rdf:resource="http://www.usgs.gov/science/USGSThesaurus"/>
  </rdf:Description>
  <rdf:Description about="http://www.usgs.gov/science/USGSThesaurus/sea-level%20change">
    <rdf:type rdf:resource="http://www.w3.org/2004/02/skos/core#Concept"/>
    <skos:prefLabel xml:lang="en">sea-level change</skos:prefLabel>
    <skos:scopeNote xml:lang="en">Variation in the relative vertical position of land and ocean waters. Caused globally by changes in the distribution of ice masses and the shape of the oceans, and locally by the rate of uplift or subsidence of the land surface.  Includes both global (eustatic) and local (relative) sea-level variations.</skos:scopeNote>
    <skos:altLabel xml:lang="en">sea-level rise</skos:altLabel>
    <skos:broader rdf:resource="http://www.usgs.gov/science/USGSThesaurus/ocean%20characteristics"/>
    <skos:related rdf:resource="http://www.usgs.gov/science/USGSThesaurus/climatology"/>
    <skos:related rdf:resource="http://www.usgs.gov/science/USGSThesaurus/effects%20of%20climate%20change"/>
    <skos:related rdf:resource="http://www.usgs.gov/science/USGSThesaurus/ocean%20sciences"/>
    <skos:inScheme rdf:resource="http://www.usgs.gov/science/USGSThesaurus"/>
  </rdf:Description>
  <rdf:Description about="http://www.usgs.gov/science/USGSThesaurus/rocks%20and%20deposits">
    <rdf:type rdf:resource="http://www.w3.org/2004/02/skos/core#Concept"/>
    <skos:prefLabel xml:lang="en">rocks and deposits</skos:prefLabel>
    <skos:scopeNote xml:lang="en">Solid masses that make up the earth's crust as well as accumulations of materials. Use for major rock types and unconsolidated deposits. For deposits of economic value, see related terms.</skos:scopeNote>
    <skos:altLabel xml:lang="en">crystals</skos:altLabel>
    <!--FOR lithologic maps USE rocks and deposits WITH maps and atlases-->
    <skos:altLabel xml:lang="en">lithologic maps</skos:altLabel>
    <skos:altLabel xml:lang="en">lithology</skos:altLabel>
    <skos:altLabel xml:lang="en">rock composition</skos:altLabel>
    <skos:broader rdf:resource="http://www.usgs.gov/science/USGSThesaurus/earth%20characteristics"/>
    <skos:narrower rdf:resource="http://www.usgs.gov/science/USGSThesaurus/fossils"/>
    <skos:narrower rdf:resource="http://www.usgs.gov/science/USGSThesaurus/igneous%20rocks"/>
    <skos:narrower rdf:resource="http://www.usgs.gov/science/USGSThesaurus/metamorphic%20rocks"/>
    <skos:narrower rdf:resource="http://www.usgs.gov/science/USGSThesaurus/mineral%20deposits"/>
    <skos:narrower rdf:resource="http://www.usgs.gov/science/USGSThesaurus/permafrost"/>
    <skos:narrower rdf:resource="http://www.usgs.gov/science/USGSThesaurus/petroleum"/>
    <skos:narrower rdf:resource="http://www.usgs.gov/science/USGSThesaurus/sedimentary%20rocks"/>
    <skos:narrower rdf:resource="http://www.usgs.gov/science/USGSThesaurus/unconsolidated%20deposits"/>
    <skos:related rdf:resource="http://www.usgs.gov/science/USGSThesaurus/building%20stone%20resources"/>
    <skos:related rdf:resource="http://www.usgs.gov/science/USGSThesaurus/lithosphere"/>
    <skos:related rdf:resource="http://www.usgs.gov/science/USGSThesaurus/petrography"/>
    <skos:related rdf:resource="http://www.usgs.gov/science/USGSThesaurus/petrology"/>
    <skos:related rdf:resource="http://www.usgs.gov/science/USGSThesaurus/meteorites"/>
    <skos:inScheme rdf:resource="http://www.usgs.gov/science/USGSThesaurus"/>
  </rdf:Description>
  <rdf:Description about="http://www.usgs.gov/science/USGSThesaurus/fossils">
    <rdf:type rdf:resource="http://www.w3.org/2004/02/skos/core#Concept"/>
    <skos:prefLabel xml:lang="en">fossils</skos:prefLabel>
    <skos:scopeNote xml:lang="en">Recognizable remains such as bones, shells, leaves, burrows, impressions, or tracks of past life on the earth.</skos:scopeNote>
    <skos:altLabel xml:lang="en">index fossils</skos:altLabel>
    <skos:altLabel xml:lang="en">microfossils</skos:altLabel>
    <skos:broader rdf:resource="http://www.usgs.gov/science/USGSThesaurus/rocks%20and%20deposits"/>
    <skos:narrower rdf:resource="http://www.usgs.gov/science/USGSThesaurus/ichnofossils"/>
    <skos:related rdf:resource="http://www.usgs.gov/science/USGSThesaurus/biostratigraphy"/>
    <skos:related rdf:resource="http://www.usgs.gov/science/USGSThesaurus/micropaleontology"/>
    <skos:related rdf:resource="http://www.usgs.gov/science/USGSThesaurus/paleontology"/>
    <skos:related rdf:resource="http://www.usgs.gov/science/USGSThesaurus/trilobites"/>
    <skos:inScheme rdf:resource="http://www.usgs.gov/science/USGSThesaurus"/>
  </rdf:Description>
  <rdf:Description about="http://www.usgs.gov/science/USGSThesaurus/ichnofossils">
    <rdf:type rdf:resource="http://www.w3.org/2004/02/skos/core#Concept"/>
    <skos:prefLabel xml:lang="en">ichnofossils</skos:prefLabel>
    <skos:scopeNote xml:lang="en">Fossilized remains of the traces of animal activity from different geologic time periods including burrows, tracks, trails, borings, and other features found in sedimentary structures.</skos:scopeNote>
    <skos:altLabel xml:lang="en">trace fossils</skos:altLabel>
    <skos:broader rdf:resource="http://www.usgs.gov/science/USGSThesaurus/fossils"/>
    <skos:related rdf:resource="http://www.usgs.gov/science/USGSThesaurus/biostratigraphy"/>
    <skos:related rdf:resource="http://www.usgs.gov/science/USGSThesaurus/paleontology"/>
    <skos:inScheme rdf:resource="http://www.usgs.gov/science/USGSThesaurus"/>
  </rdf:Description>
  <rdf:Description about="http://www.usgs.gov/science/USGSThesaurus/igneous%20rocks">
    <rdf:type rdf:resource="http://www.w3.org/2004/02/skos/core#Concept"/>
    <skos:prefLabel xml:lang="en">igneous rocks</skos:prefLabel>
    <skos:scopeNote xml:lang="en">Rocks formed from melted rock that has cooled and solidified.</skos:scopeNote>
    <skos:broader rdf:resource="http://www.usgs.gov/science/USGSThesaurus/rocks%20and%20deposits"/>
    <skos:narrower rdf:resource="http://www.usgs.gov/science/USGSThesaurus/plutonic%20rocks"/>
    <skos:narrower rdf:resource="http://www.usgs.gov/science/USGSThesaurus/volcanic%20rocks"/>
    <skos:related rdf:resource="http://www.usgs.gov/science/USGSThesaurus/petrology"/>
    <skos:inScheme rdf:resource="http://www.usgs.gov/science/USGSThesaurus"/>
  </rdf:Description>
  <rdf:Description about="http://www.usgs.gov/science/USGSThesaurus/plutonic%20rocks">
    <rdf:type rdf:resource="http://www.w3.org/2004/02/skos/core#Concept"/>
    <skos:prefLabel xml:lang="en">plutonic rocks</skos:prefLabel>
    <skos:scopeNote xml:lang="en">Rocks formed at considerable depth by crystallization of magma and/or by chemical alteration. They are characteristically medium- to coarse-grained, of granitoid texture.</skos:scopeNote>
    <skos:altLabel xml:lang="en">intrusive rocks</skos:altLabel>
    <skos:altLabel xml:lang="en">magma</skos:altLabel>
    <skos:broader rdf:resource="http://www.usgs.gov/science/USGSThesaurus/igneous%20rocks"/>
    <skos:inScheme rdf:resource="http://www.usgs.gov/science/USGSThesaurus"/>
  </rdf:Description>
  <rdf:Description about="http://www.usgs.gov/science/USGSThesaurus/volcanic%20rocks">
    <rdf:type rdf:resource="http://www.w3.org/2004/02/skos/core#Concept"/>
    <skos:prefLabel xml:lang="en">volcanic rocks</skos:prefLabel>
    <skos:scopeNote xml:lang="en">A generally finely crystalline or glassy igneous rock resulting from volcanic action at or near the earth's surface, either ejected explosively or extruded as lava. The term includes near-surface intrusions that form a part of the volcanic structure.</skos:scopeNote>
    <skos:altLabel xml:lang="en">lava</skos:altLabel>
    <skos:altLabel xml:lang="en">pyroclastic</skos:altLabel>
    <skos:altLabel xml:lang="en">tuff</skos:altLabel>
    <skos:altLabel xml:lang="en">volcanic ash</skos:altLabel>
    <skos:broader rdf:resource="http://www.usgs.gov/science/USGSThesaurus/igneous%20rocks"/>
    <skos:inScheme rdf:resource="http://www.usgs.gov/science/USGSThesaurus"/>
  </rdf:Description>
  <rdf:Description about="http://www.usgs.gov/science/USGSThesaurus/metamorphic%20rocks">
    <rdf:type rdf:resource="http://www.w3.org/2004/02/skos/core#Concept"/>
    <skos:prefLabel xml:lang="en">metamorphic rocks</skos:prefLabel>
    <skos:scopeNote xml:lang="en">Sedimentary or igneous rocks which have undergone such intense changes in temperature, pressure, structural stress, or chemical environment that they are transformed into denser rocks.</skos:scopeNote>
    <skos:broader rdf:resource="http://www.usgs.gov/science/USGSThesaurus/rocks%20and%20deposits"/>
    <skos:related rdf:resource="http://www.usgs.gov/science/USGSThesaurus/metamorphism%20%28geological%29"/>
    <skos:related rdf:resource="http://www.usgs.gov/science/USGSThesaurus/petrology"/>
    <skos:inScheme rdf:resource="http://www.usgs.gov/science/USGSThesaurus"/>
  </rdf:Description>
  <rdf:Description about="http://www.usgs.gov/science/USGSThesaurus/mineral%20deposits">
    <rdf:type rdf:resource="http://www.w3.org/2004/02/skos/core#Concept"/>
    <skos:prefLabel xml:lang="en">mineral deposits</skos:prefLabel>
    <skos:scopeNote xml:lang="en">Deposits in which particular minerals are concentrated, typically noticed and studied if the minerals have economic value.</skos:scopeNote>
    <skos:altLabel xml:lang="en">ore deposits</skos:altLabel>
    <skos:broader rdf:resource="http://www.usgs.gov/science/USGSThesaurus/rocks%20and%20deposits"/>
    <skos:related rdf:resource="http://www.usgs.gov/science/USGSThesaurus/mineral%20resources"/>
    <skos:related rdf:resource="http://www.usgs.gov/science/USGSThesaurus/coal%20resources"/>
    <skos:inScheme rdf:resource="http://www.usgs.gov/science/USGSThesaurus"/>
  </rdf:Description>
  <rdf:Description about="http://www.usgs.gov/science/USGSThesaurus/permafrost">
    <rdf:type rdf:resource="http://www.w3.org/2004/02/skos/core#Concept"/>
    <skos:prefLabel xml:lang="en">permafrost</skos:prefLabel>
    <skos:scopeNote xml:lang="en">Rocks and deposits in which the interstitial waters remain perennially frozen.</skos:scopeNote>
    <skos:broader rdf:resource="http://www.usgs.gov/science/USGSThesaurus/rocks%20and%20deposits"/>
    <skos:inScheme rdf:resource="http://www.usgs.gov/science/USGSThesaurus"/>
  </rdf:Description>
  <rdf:Description about="http://www.usgs.gov/science/USGSThesaurus/petroleum">
    <rdf:type rdf:resource="http://www.w3.org/2004/02/skos/core#Concept"/>
    <skos:prefLabel xml:lang="en">petroleum</skos:prefLabel>
    <skos:scopeNote xml:lang="en">Naturally occurring hydrocarbons, typically fluid or gas, often of economic use.  Includes oil, natural gas, and asphaltic compounds found in tar sands and oil shales.</skos:scopeNote>
    <!--FOR oil spills USE petroleum WITH industrial pollution-->
    <skos:altLabel xml:lang="en">oil spills</skos:altLabel>
    <skos:broader rdf:resource="http://www.usgs.gov/science/USGSThesaurus/rocks%20and%20deposits"/>
    <skos:related rdf:resource="http://www.usgs.gov/science/USGSThesaurus/oil%20resources"/>
    <skos:related rdf:resource="http://www.usgs.gov/science/USGSThesaurus/natural%20gas%20resources"/>
    <skos:inScheme rdf:resource="http://www.usgs.gov/science/USGSThesaurus"/>
  </rdf:Description>
  <rdf:Description about="http://www.usgs.gov/science/USGSThesaurus/sedimentary%20rocks">
    <rdf:type rdf:resource="http://www.w3.org/2004/02/skos/core#Concept"/>
    <skos:prefLabel xml:lang="en">sedimentary rocks</skos:prefLabel>
    <skos:scopeNote xml:lang="en">Rocks formed by the consolidation of loose, uncemented pieces of sediments.</skos:scopeNote>
    <skos:broader rdf:resource="http://www.usgs.gov/science/USGSThesaurus/rocks%20and%20deposits"/>
    <skos:narrower rdf:resource="http://www.usgs.gov/science/USGSThesaurus/bedforms"/>
    <skos:related rdf:resource="http://www.usgs.gov/science/USGSThesaurus/petrology"/>
    <skos:related rdf:resource="http://www.usgs.gov/science/USGSThesaurus/sedimentation"/>
    <skos:related rdf:resource="http://www.usgs.gov/science/USGSThesaurus/sedimentology"/>
    <skos:inScheme rdf:resource="http://www.usgs.gov/science/USGSThesaurus"/>
  </rdf:Description>
  <rdf:Description about="http://www.usgs.gov/science/USGSThesaurus/bedforms">
    <rdf:type rdf:resource="http://www.w3.org/2004/02/skos/core#Concept"/>
    <skos:prefLabel xml:lang="en">bedforms</skos:prefLabel>
    <skos:scopeNote xml:lang="en">Fluctuations from horizontal layers in sediments or sedimentary rocks made by flow on the beds of alluvial channels.</skos:scopeNote>
    <skos:altLabel xml:lang="en">bed forms</skos:altLabel>
    <skos:broader rdf:resource="http://www.usgs.gov/science/USGSThesaurus/sedimentary%20rocks"/>
    <skos:related rdf:resource="http://www.usgs.gov/science/USGSThesaurus/sedimentology"/>
    <skos:inScheme rdf:resource="http://www.usgs.gov/science/USGSThesaurus"/>
  </rdf:Description>
  <rdf:Description about="http://www.usgs.gov/science/USGSThesaurus/unconsolidated%20deposits">
    <rdf:type rdf:resource="http://www.w3.org/2004/02/skos/core#Concept"/>
    <skos:prefLabel xml:lang="en">unconsolidated deposits</skos:prefLabel>
    <skos:scopeNote xml:lang="en">Loosely bound sediments such as sand, gravel, and silt which tend to accumulate in low areas or valleys.</skos:scopeNote>
    <skos:altLabel xml:lang="en">alluvium</skos:altLabel>
    <skos:altLabel xml:lang="en">eolian sediments</skos:altLabel>
    <skos:altLabel xml:lang="en">loess</skos:altLabel>
    <skos:altLabel xml:lang="en">sediments</skos:altLabel>
    <skos:altLabel xml:lang="en">surficial deposits</skos:altLabel>
    <!--FOR sediment geochemistry USE unconsolidated deposits WITH chemical analysis-->
    <skos:altLabel xml:lang="en">sediment geochemistry</skos:altLabel>
    <skos:broader rdf:resource="http://www.usgs.gov/science/USGSThesaurus/rocks%20and%20deposits"/>
    <skos:narrower rdf:resource="http://www.usgs.gov/science/USGSThesaurus/clay%20deposits"/>
    <skos:narrower rdf:resource="http://www.usgs.gov/science/USGSThesaurus/gravel%20deposits"/>
    <skos:narrower rdf:resource="http://www.usgs.gov/science/USGSThesaurus/mine%20waste"/>
    <skos:narrower rdf:resource="http://www.usgs.gov/science/USGSThesaurus/sand%20deposits"/>
    <skos:narrower rdf:resource="http://www.usgs.gov/science/USGSThesaurus/soil%20horizons"/>
    <skos:inScheme rdf:resource="http://www.usgs.gov/science/USGSThesaurus"/>
  </rdf:Description>
  <rdf:Description about="http://www.usgs.gov/science/USGSThesaurus/clay%20deposits">
    <rdf:type rdf:resource="http://www.w3.org/2004/02/skos/core#Concept"/>
    <skos:prefLabel xml:lang="en">clay deposits</skos:prefLabel>
    <skos:scopeNote xml:lang="en">Fine-grained sedimentary soil deposits, containing hydrated silicas of aluminum, that are plastic and sticky when wet and harden when heated.</skos:scopeNote>
    <skos:broader rdf:resource="http://www.usgs.gov/science/USGSThesaurus/unconsolidated%20deposits"/>
    <skos:related rdf:resource="http://www.usgs.gov/science/USGSThesaurus/economic%20geology"/>
    <skos:related rdf:resource="http://www.usgs.gov/science/USGSThesaurus/nonmetallic%20mineral%20resources"/>
    <skos:related rdf:resource="http://www.usgs.gov/science/USGSThesaurus/sedimentology"/>
    <skos:inScheme rdf:resource="http://www.usgs.gov/science/USGSThesaurus"/>
  </rdf:Description>
  <rdf:Description about="http://www.usgs.gov/science/USGSThesaurus/gravel%20deposits">
    <rdf:type rdf:resource="http://www.w3.org/2004/02/skos/core#Concept"/>
    <skos:prefLabel xml:lang="en">gravel deposits</skos:prefLabel>
    <skos:scopeNote xml:lang="en">Alluvial accumulations of small unconsolidated rock fragments, such as pebbles and cobbles, used in construction as fill, ground cover, or aggregate for concrete.</skos:scopeNote>
    <skos:broader rdf:resource="http://www.usgs.gov/science/USGSThesaurus/unconsolidated%20deposits"/>
    <skos:related rdf:resource="http://www.usgs.gov/science/USGSThesaurus/economic%20geology"/>
    <skos:related rdf:resource="http://www.usgs.gov/science/USGSThesaurus/nonmetallic%20mineral%20resources"/>
    <skos:related rdf:resource="http://www.usgs.gov/science/USGSThesaurus/sedimentology"/>
    <skos:inScheme rdf:resource="http://www.usgs.gov/science/USGSThesaurus"/>
  </rdf:Description>
  <rdf:Description about="http://www.usgs.gov/science/USGSThesaurus/mine%20waste">
    <rdf:type rdf:resource="http://www.w3.org/2004/02/skos/core#Concept"/>
    <skos:prefLabel xml:lang="en">mine waste</skos:prefLabel>
    <skos:scopeNote xml:lang="en">Earth materials removed during mining and concentrated in piles or beds, typically near the site of extraction.  Tailings are mine waste that has been processed to remove valuable components; unprocessed mine waste includes overburden removed to reach commodity materials such as ore or coal.</skos:scopeNote>
    <skos:altLabel xml:lang="en">tailing piles</skos:altLabel>
    <skos:altLabel xml:lang="en">mine tailings</skos:altLabel>
    <skos:altLabel xml:lang="en">mine spoil</skos:altLabel>
    <skos:broader rdf:resource="http://www.usgs.gov/science/USGSThesaurus/unconsolidated%20deposits"/>
    <skos:inScheme rdf:resource="http://www.usgs.gov/science/USGSThesaurus"/>
  </rdf:Description>
  <rdf:Description about="http://www.usgs.gov/science/USGSThesaurus/sand%20deposits">
    <rdf:type rdf:resource="http://www.w3.org/2004/02/skos/core#Concept"/>
    <skos:prefLabel xml:lang="en">sand deposits</skos:prefLabel>
    <skos:scopeNote xml:lang="en">Deposits of loose particles of rock or mineral (sediment) that range in size from 0.0625-2.0 millimeters in diameter.</skos:scopeNote>
    <skos:broader rdf:resource="http://www.usgs.gov/science/USGSThesaurus/unconsolidated%20deposits"/>
    <skos:related rdf:resource="http://www.usgs.gov/science/USGSThesaurus/economic%20geology"/>
    <skos:related rdf:resource="http://www.usgs.gov/science/USGSThesaurus/nonmetallic%20mineral%20resources"/>
    <skos:related rdf:resource="http://www.usgs.gov/science/USGSThesaurus/sedimentology"/>
    <skos:inScheme rdf:resource="http://www.usgs.gov/science/USGSThesaurus"/>
  </rdf:Description>
  <rdf:Description about="http://www.usgs.gov/science/USGSThesaurus/soil%20horizons">
    <rdf:type rdf:resource="http://www.w3.org/2004/02/skos/core#Concept"/>
    <skos:prefLabel xml:lang="en">soil horizons</skos:prefLabel>
    <skos:scopeNote xml:lang="en">Layers in soil defined by physical, chemical, biological, or mineralogical properties which vary with depth.</skos:scopeNote>
    <skos:altLabel xml:lang="en">A horizon</skos:altLabel>
    <skos:altLabel xml:lang="en">B horizon</skos:altLabel>
    <skos:altLabel xml:lang="en">C horizon</skos:altLabel>
    <skos:broader rdf:resource="http://www.usgs.gov/science/USGSThesaurus/unconsolidated%20deposits"/>
    <skos:related rdf:resource="http://www.usgs.gov/science/USGSThesaurus/soil%20formation"/>
    <skos:related rdf:resource="http://www.usgs.gov/science/USGSThesaurus/soil%20sciences"/>
    <skos:inScheme rdf:resource="http://www.usgs.gov/science/USGSThesaurus"/>
  </rdf:Description>
  <rdf:Description about="http://www.usgs.gov/science/USGSThesaurus/snow%20and%20ice%20cover">
    <rdf:type rdf:resource="http://www.w3.org/2004/02/skos/core#Concept"/>
    <skos:prefLabel xml:lang="en">snow and ice cover</skos:prefLabel>
    <skos:scopeNote xml:lang="en">Accumulation of snow or ice blanketing land surfaces.</skos:scopeNote>
    <skos:altLabel xml:lang="en">cryosphere</skos:altLabel>
    <skos:altLabel xml:lang="en">glaciers</skos:altLabel>
    <!--FOR ice core sampling USE snow and ice cover WITH drilling and coring-->
    <skos:altLabel xml:lang="en">ice core sampling</skos:altLabel>
    <skos:altLabel xml:lang="en">ice</skos:altLabel>
    <skos:altLabel xml:lang="en">snowpack</skos:altLabel>
    <skos:broader rdf:resource="http://www.usgs.gov/science/USGSThesaurus/earth%20characteristics"/>
    <skos:narrower rdf:resource="http://www.usgs.gov/science/USGSThesaurus/sea%20ice%20concentration"/>
    <skos:related rdf:resource="http://www.usgs.gov/science/USGSThesaurus/atmospheric%20and%20climatic%20processes"/>
    <skos:related rdf:resource="http://www.usgs.gov/science/USGSThesaurus/glaciation"/>
    <skos:related rdf:resource="http://www.usgs.gov/science/USGSThesaurus/glaciology"/>
    <skos:related rdf:resource="http://www.usgs.gov/science/USGSThesaurus/SSM%2FI"/>
    <skos:related rdf:resource="http://www.usgs.gov/science/USGSThesaurus/surface%20water%20%28non-marine%29"/>
    <skos:inScheme rdf:resource="http://www.usgs.gov/science/USGSThesaurus"/>
  </rdf:Description>
  <rdf:Description about="http://www.usgs.gov/science/USGSThesaurus/sea%20ice%20concentration">
    <rdf:type rdf:resource="http://www.w3.org/2004/02/skos/core#Concept"/>
    <skos:prefLabel xml:lang="en">sea ice concentration</skos:prefLabel>
    <skos:scopeNote xml:lang="en">Proportion of ocean area in a given region that contains or is covered by floating ice.</skos:scopeNote>
    <skos:altLabel xml:lang="en">sea-ice concentration</skos:altLabel>
    <skos:altLabel xml:lang="en">sea ice cover</skos:altLabel>
    <skos:broader rdf:resource="http://www.usgs.gov/science/USGSThesaurus/snow%20and%20ice%20cover"/>
    <skos:related rdf:resource="http://www.usgs.gov/science/USGSThesaurus/ocean%20characteristics"/>
    <skos:inScheme rdf:resource="http://www.usgs.gov/science/USGSThesaurus"/>
  </rdf:Description>
  <rdf:Description about="http://www.usgs.gov/science/USGSThesaurus/stratigraphic%20sections">
    <rdf:type rdf:resource="http://www.w3.org/2004/02/skos/core#Concept"/>
    <skos:prefLabel xml:lang="en">stratigraphic sections</skos:prefLabel>
    <skos:scopeNote xml:lang="en">Vertical arrangement in layers of rock units whose sequence is used to study the geological history of the strata.</skos:scopeNote>
    <skos:altLabel xml:lang="en">geologic sections</skos:altLabel>
    <skos:altLabel xml:lang="en">geologic units</skos:altLabel>
    <skos:altLabel xml:lang="en">sections (geologic)</skos:altLabel>
    <skos:altLabel xml:lang="en">sections (stratigraphic)</skos:altLabel>
    <skos:broader rdf:resource="http://www.usgs.gov/science/USGSThesaurus/earth%20characteristics"/>
    <skos:narrower rdf:resource="http://www.usgs.gov/science/USGSThesaurus/bedrock%20geologic%20units"/>
    <skos:narrower rdf:resource="http://www.usgs.gov/science/USGSThesaurus/geologic%20contacts"/>
    <skos:narrower rdf:resource="http://www.usgs.gov/science/USGSThesaurus/surficial%20geologic%20units"/>
    <skos:related rdf:resource="http://www.usgs.gov/science/USGSThesaurus/geologic%20structure"/>
    <skos:related rdf:resource="http://www.usgs.gov/science/USGSThesaurus/stratigraphy"/>
    <skos:inScheme rdf:resource="http://www.usgs.gov/science/USGSThesaurus"/>
  </rdf:Description>
  <rdf:Description about="http://www.usgs.gov/science/USGSThesaurus/bedrock%20geologic%20units">
    <rdf:type rdf:resource="http://www.w3.org/2004/02/skos/core#Concept"/>
    <skos:prefLabel xml:lang="en">bedrock geologic units</skos:prefLabel>
    <skos:scopeNote xml:lang="en">Units of consolidated (solid) rock that underlie soils or other unconsolidated materials.</skos:scopeNote>
    <!--FOR basement maps USE bedrock geologic units WITH maps and atlases-->
    <skos:altLabel xml:lang="en">basement maps</skos:altLabel>
    <skos:altLabel xml:lang="en">geologic formations</skos:altLabel>
    <skos:broader rdf:resource="http://www.usgs.gov/science/USGSThesaurus/stratigraphic%20sections"/>
    <skos:related rdf:resource="http://www.usgs.gov/science/USGSThesaurus/stratigraphy"/>
    <skos:related rdf:resource="http://www.usgs.gov/science/USGSThesaurus/geologic%20maps"/>
    <skos:inScheme rdf:resource="http://www.usgs.gov/science/USGSThesaurus"/>
  </rdf:Description>
  <rdf:Description about="http://www.usgs.gov/science/USGSThesaurus/geologic%20contacts">
    <rdf:type rdf:resource="http://www.w3.org/2004/02/skos/core#Concept"/>
    <skos:prefLabel xml:lang="en">geologic contacts</skos:prefLabel>
    <skos:scopeNote xml:lang="en">Junctions of two different rock formations varying by type or age of rock, including faults, unconformities, and bedding planes.</skos:scopeNote>
    <skos:altLabel xml:lang="en">contacts (geologic)</skos:altLabel>
    <skos:broader rdf:resource="http://www.usgs.gov/science/USGSThesaurus/stratigraphic%20sections"/>
    <skos:narrower rdf:resource="http://www.usgs.gov/science/USGSThesaurus/unconformities"/>
    <skos:related rdf:resource="http://www.usgs.gov/science/USGSThesaurus/stratigraphy"/>
    <skos:related rdf:resource="http://www.usgs.gov/science/USGSThesaurus/geologic%20maps"/>
    <skos:inScheme rdf:resource="http://www.usgs.gov/science/USGSThesaurus"/>
  </rdf:Description>
  <rdf:Description about="http://www.usgs.gov/science/USGSThesaurus/unconformities">
    <rdf:type rdf:resource="http://www.w3.org/2004/02/skos/core#Concept"/>
    <skos:prefLabel xml:lang="en">unconformities</skos:prefLabel>
    <skos:scopeNote xml:lang="en">The contact between older rocks and younger sedimentary rocks where erosion had removed some of the older rocks before the younger rocks were deposited.</skos:scopeNote>
    <skos:broader rdf:resource="http://www.usgs.gov/science/USGSThesaurus/geologic%20contacts"/>
    <skos:related rdf:resource="http://www.usgs.gov/science/USGSThesaurus/stratigraphy"/>
    <skos:inScheme rdf:resource="http://www.usgs.gov/science/USGSThesaurus"/>
  </rdf:Description>
  <rdf:Description about="http://www.usgs.gov/science/USGSThesaurus/surficial%20geologic%20units">
    <rdf:type rdf:resource="http://www.w3.org/2004/02/skos/core#Concept"/>
    <skos:prefLabel xml:lang="en">surficial geologic units</skos:prefLabel>
    <skos:scopeNote xml:lang="en">Rock units on the earth's surface.</skos:scopeNote>
    <!--FOR surficial geologic maps USE surficial geologic units WITH maps and atlases-->
    <skos:altLabel xml:lang="en">surficial geologic maps</skos:altLabel>
    <skos:broader rdf:resource="http://www.usgs.gov/science/USGSThesaurus/stratigraphic%20sections"/>
    <skos:related rdf:resource="http://www.usgs.gov/science/USGSThesaurus/stratigraphy"/>
    <skos:related rdf:resource="http://www.usgs.gov/science/USGSThesaurus/geologic%20maps"/>
    <skos:inScheme rdf:resource="http://www.usgs.gov/science/USGSThesaurus"/>
  </rdf:Description>
  <rdf:Description about="http://www.usgs.gov/science/USGSThesaurus/topography">
    <rdf:type rdf:resource="http://www.w3.org/2004/02/skos/core#Concept"/>
    <skos:prefLabel xml:lang="en">topography</skos:prefLabel>
    <skos:scopeNote xml:lang="en">Configuration of the land surface and sea floor.</skos:scopeNote>
    <skos:altLabel xml:lang="en">elevation and relief</skos:altLabel>
    <skos:broader rdf:resource="http://www.usgs.gov/science/USGSThesaurus/earth%20characteristics"/>
    <skos:narrower rdf:resource="http://www.usgs.gov/science/USGSThesaurus/bathymetry"/>
    <skos:related rdf:resource="http://www.usgs.gov/science/USGSThesaurus/geography"/>
    <skos:related rdf:resource="http://www.usgs.gov/science/USGSThesaurus/geomorphology"/>
    <skos:related rdf:resource="http://www.usgs.gov/science/USGSThesaurus/geospatial%20datasets"/>
    <skos:related rdf:resource="http://www.usgs.gov/science/USGSThesaurus/topographic%20maps"/>
    <skos:inScheme rdf:resource="http://www.usgs.gov/science/USGSThesaurus"/>
  </rdf:Description>
  <rdf:Description about="http://www.usgs.gov/science/USGSThesaurus/bathymetry">
    <rdf:type rdf:resource="http://www.w3.org/2004/02/skos/core#Concept"/>
    <skos:prefLabel xml:lang="en">bathymetry</skos:prefLabel>
    <skos:scopeNote xml:lang="en">The elevation of the earth's surface beneath a body of water, especially the ocean, typically determined by measurements of depth from the water surface.</skos:scopeNote>
    <skos:altLabel xml:lang="en">bathymetry data</skos:altLabel>
    <skos:altLabel xml:lang="en">sea floor topography</skos:altLabel>
    <skos:altLabel xml:lang="en">underwater contours</skos:altLabel>
    <skos:broader rdf:resource="http://www.usgs.gov/science/USGSThesaurus/topography"/>
    <skos:related rdf:resource="http://www.usgs.gov/science/USGSThesaurus/geomorphology"/>
    <skos:related rdf:resource="http://www.usgs.gov/science/USGSThesaurus/limnology"/>
    <skos:related rdf:resource="http://www.usgs.gov/science/USGSThesaurus/ocean%20sciences"/>
    <skos:related rdf:resource="http://www.usgs.gov/science/USGSThesaurus/sea-floor%20characteristics"/>
    <skos:related rdf:resource="http://www.usgs.gov/science/USGSThesaurus/single-beam%20echo%20sounder"/>
    <skos:related rdf:resource="http://www.usgs.gov/science/USGSThesaurus/multibeam%20sonar"/>
    <skos:related rdf:resource="http://www.usgs.gov/science/USGSThesaurus/interferometric%20sonar"/>
    <skos:inScheme rdf:resource="http://www.usgs.gov/science/USGSThesaurus"/>
  </rdf:Description>
  <rdf:Description about="http://www.usgs.gov/science/USGSThesaurus/effects%20of%20climate%20change">
    <rdf:type rdf:resource="http://www.w3.org/2004/02/skos/core#Concept"/>
    <skos:prefLabel xml:lang="en">effects of climate change</skos:prefLabel>
    <skos:scopeNote xml:lang="en">Characteristics and behaviors of organisms and earth systems that are modified as a result of changes in global, regional, or local climate.</skos:scopeNote>
    <skos:altLabel xml:lang="en">global change</skos:altLabel>
    <skos:altLabel xml:lang="en">climate effects</skos:altLabel>
    <skos:altLabel xml:lang="en">climate change effects</skos:altLabel>
    <skos:broader rdf:resource="http://www.usgs.gov/science/USGSThesaurus/topics"/>
    <skos:related rdf:resource="http://www.usgs.gov/science/USGSThesaurus/atmospheric%20sciences"/>
    <skos:related rdf:resource="http://www.usgs.gov/science/USGSThesaurus/climate%20change"/>
    <skos:related rdf:resource="http://www.usgs.gov/science/USGSThesaurus/ecology"/>
    <skos:related rdf:resource="http://www.usgs.gov/science/USGSThesaurus/ocean%20sciences"/>
    <skos:related rdf:resource="http://www.usgs.gov/science/USGSThesaurus/sea-level%20change"/>
    <skos:related rdf:resource="http://www.usgs.gov/science/USGSThesaurus/ocean%20acidification"/>
    <skos:inScheme rdf:resource="http://www.usgs.gov/science/USGSThesaurus"/>
  </rdf:Description>
  <rdf:Description about="http://www.usgs.gov/science/USGSThesaurus/elements">
    <rdf:type rdf:resource="http://www.w3.org/2004/02/skos/core#Concept"/>
    <skos:prefLabel xml:lang="en">elements</skos:prefLabel>
    <skos:scopeNote xml:lang="en">Chemical elements and element groups</skos:scopeNote>
    <skos:broader rdf:resource="http://www.usgs.gov/science/USGSThesaurus/topics"/>
    <skos:narrower rdf:resource="http://www.usgs.gov/science/USGSThesaurus/chemical%20element%20groups"/>
    <skos:narrower rdf:resource="http://www.usgs.gov/science/USGSThesaurus/chemical%20elements"/>
    <skos:inScheme rdf:resource="http://www.usgs.gov/science/USGSThesaurus"/>
  </rdf:Description>
  <rdf:Description about="http://www.usgs.gov/science/USGSThesaurus/chemical%20element%20groups">
    <rdf:type rdf:resource="http://www.w3.org/2004/02/skos/core#Concept"/>
    <skos:prefLabel xml:lang="en">chemical element groups</skos:prefLabel>
    <skos:scopeNote xml:lang="en">Groups shown at &lt;http://periodic.lanl.gov/&gt;</skos:scopeNote>
    <skos:broader rdf:resource="http://www.usgs.gov/science/USGSThesaurus/elements"/>
    <skos:narrower rdf:resource="http://www.usgs.gov/science/USGSThesaurus/actinide%20series%20elements"/>
    <skos:narrower rdf:resource="http://www.usgs.gov/science/USGSThesaurus/alkali%20metal%20elements"/>
    <skos:narrower rdf:resource="http://www.usgs.gov/science/USGSThesaurus/alkaline%20earth%20elements"/>
    <skos:narrower rdf:resource="http://www.usgs.gov/science/USGSThesaurus/halogen%20elements"/>
    <skos:narrower rdf:resource="http://www.usgs.gov/science/USGSThesaurus/lanthanide%20series%20elements"/>
    <skos:narrower rdf:resource="http://www.usgs.gov/science/USGSThesaurus/metal%20elements"/>
    <skos:narrower rdf:resource="http://www.usgs.gov/science/USGSThesaurus/noble%20gas%20elements"/>
    <skos:narrower rdf:resource="http://www.usgs.gov/science/USGSThesaurus/nonmetal%20elements"/>
    <skos:narrower rdf:resource="http://www.usgs.gov/science/USGSThesaurus/rare%20earth%20elements"/>
    <skos:inScheme rdf:resource="http://www.usgs.gov/science/USGSThesaurus"/>
  </rdf:Description>
  <rdf:Description about="http://www.usgs.gov/science/USGSThesaurus/actinide%20series%20elements">
    <rdf:type rdf:resource="http://www.w3.org/2004/02/skos/core#Concept"/>
    <skos:prefLabel xml:lang="en">actinide series elements</skos:prefLabel>
    <skos:scopeNote xml:lang="en"></skos:scopeNote>
    <skos:broader rdf:resource="http://www.usgs.gov/science/USGSThesaurus/chemical%20element%20groups"/>
    <skos:related rdf:resource="http://www.usgs.gov/science/USGSThesaurus/actinium"/>
    <skos:related rdf:resource="http://www.usgs.gov/science/USGSThesaurus/thorium"/>
    <skos:related rdf:resource="http://www.usgs.gov/science/USGSThesaurus/protactinium"/>
    <skos:related rdf:resource="http://www.usgs.gov/science/USGSThesaurus/uranium"/>
    <skos:related rdf:resource="http://www.usgs.gov/science/USGSThesaurus/neptunium"/>
    <skos:related rdf:resource="http://www.usgs.gov/science/USGSThesaurus/plutonium"/>
    <skos:related rdf:resource="http://www.usgs.gov/science/USGSThesaurus/americium"/>
    <skos:related rdf:resource="http://www.usgs.gov/science/USGSThesaurus/curium"/>
    <skos:related rdf:resource="http://www.usgs.gov/science/USGSThesaurus/berkelium"/>
    <skos:related rdf:resource="http://www.usgs.gov/science/USGSThesaurus/californium"/>
    <skos:related rdf:resource="http://www.usgs.gov/science/USGSThesaurus/einsteinium"/>
    <skos:related rdf:resource="http://www.usgs.gov/science/USGSThesaurus/fermium"/>
    <skos:related rdf:resource="http://www.usgs.gov/science/USGSThesaurus/mendelevium"/>
    <skos:related rdf:resource="http://www.usgs.gov/science/USGSThesaurus/nobelium"/>
    <skos:related rdf:resource="http://www.usgs.gov/science/USGSThesaurus/lawrencium"/>
    <skos:inScheme rdf:resource="http://www.usgs.gov/science/USGSThesaurus"/>
  </rdf:Description>
  <rdf:Description about="http://www.usgs.gov/science/USGSThesaurus/alkali%20metal%20elements">
    <rdf:type rdf:resource="http://www.w3.org/2004/02/skos/core#Concept"/>
    <skos:prefLabel xml:lang="en">alkali metal elements</skos:prefLabel>
    <skos:scopeNote xml:lang="en"></skos:scopeNote>
    <skos:broader rdf:resource="http://www.usgs.gov/science/USGSThesaurus/chemical%20element%20groups"/>
    <skos:related rdf:resource="http://www.usgs.gov/science/USGSThesaurus/hydrogen"/>
    <skos:related rdf:resource="http://www.usgs.gov/science/USGSThesaurus/lithium"/>
    <skos:related rdf:resource="http://www.usgs.gov/science/USGSThesaurus/sodium"/>
    <skos:related rdf:resource="http://www.usgs.gov/science/USGSThesaurus/potassium"/>
    <skos:related rdf:resource="http://www.usgs.gov/science/USGSThesaurus/rubidium"/>
    <skos:related rdf:resource="http://www.usgs.gov/science/USGSThesaurus/cesium"/>
    <skos:related rdf:resource="http://www.usgs.gov/science/USGSThesaurus/francium"/>
    <skos:inScheme rdf:resource="http://www.usgs.gov/science/USGSThesaurus"/>
  </rdf:Description>
  <rdf:Description about="http://www.usgs.gov/science/USGSThesaurus/alkaline%20earth%20elements">
    <rdf:type rdf:resource="http://www.w3.org/2004/02/skos/core#Concept"/>
    <skos:prefLabel xml:lang="en">alkaline earth elements</skos:prefLabel>
    <skos:scopeNote xml:lang="en"></skos:scopeNote>
    <skos:broader rdf:resource="http://www.usgs.gov/science/USGSThesaurus/chemical%20element%20groups"/>
    <skos:related rdf:resource="http://www.usgs.gov/science/USGSThesaurus/beryllium"/>
    <skos:related rdf:resource="http://www.usgs.gov/science/USGSThesaurus/magnesium"/>
    <skos:related rdf:resource="http://www.usgs.gov/science/USGSThesaurus/calcium"/>
    <skos:related rdf:resource="http://www.usgs.gov/science/USGSThesaurus/strontium"/>
    <skos:related rdf:resource="http://www.usgs.gov/science/USGSThesaurus/barium"/>
    <skos:related rdf:resource="http://www.usgs.gov/science/USGSThesaurus/radium"/>
    <skos:inScheme rdf:resource="http://www.usgs.gov/science/USGSThesaurus"/>
  </rdf:Description>
  <rdf:Description about="http://www.usgs.gov/science/USGSThesaurus/halogen%20elements">
    <rdf:type rdf:resource="http://www.w3.org/2004/02/skos/core#Concept"/>
    <skos:prefLabel xml:lang="en">halogen elements</skos:prefLabel>
    <skos:scopeNote xml:lang="en"></skos:scopeNote>
    <skos:broader rdf:resource="http://www.usgs.gov/science/USGSThesaurus/chemical%20element%20groups"/>
    <skos:related rdf:resource="http://www.usgs.gov/science/USGSThesaurus/fluorine"/>
    <skos:related rdf:resource="http://www.usgs.gov/science/USGSThesaurus/chlorine"/>
    <skos:related rdf:resource="http://www.usgs.gov/science/USGSThesaurus/bromine"/>
    <skos:related rdf:resource="http://www.usgs.gov/science/USGSThesaurus/iodine"/>
    <skos:related rdf:resource="http://www.usgs.gov/science/USGSThesaurus/astatine"/>
    <skos:inScheme rdf:resource="http://www.usgs.gov/science/USGSThesaurus"/>
  </rdf:Description>
  <rdf:Description about="http://www.usgs.gov/science/USGSThesaurus/lanthanide%20series%20elements">
    <rdf:type rdf:resource="http://www.w3.org/2004/02/skos/core#Concept"/>
    <skos:prefLabel xml:lang="en">lanthanide series elements</skos:prefLabel>
    <skos:scopeNote xml:lang="en"></skos:scopeNote>
    <skos:broader rdf:resource="http://www.usgs.gov/science/USGSThesaurus/chemical%20element%20groups"/>
    <skos:related rdf:resource="http://www.usgs.gov/science/USGSThesaurus/rare%20earth%20elements"/>
    <skos:related rdf:resource="http://www.usgs.gov/science/USGSThesaurus/lanthanum"/>
    <skos:related rdf:resource="http://www.usgs.gov/science/USGSThesaurus/cerium"/>
    <skos:related rdf:resource="http://www.usgs.gov/science/USGSThesaurus/praseodymium"/>
    <skos:related rdf:resource="http://www.usgs.gov/science/USGSThesaurus/neodymium"/>
    <skos:related rdf:resource="http://www.usgs.gov/science/USGSThesaurus/promethium"/>
    <skos:related rdf:resource="http://www.usgs.gov/science/USGSThesaurus/samarium"/>
    <skos:related rdf:resource="http://www.usgs.gov/science/USGSThesaurus/europium"/>
    <skos:related rdf:resource="http://www.usgs.gov/science/USGSThesaurus/gadolinium"/>
    <skos:related rdf:resource="http://www.usgs.gov/science/USGSThesaurus/terbium"/>
    <skos:related rdf:resource="http://www.usgs.gov/science/USGSThesaurus/dysprosium"/>
    <skos:related rdf:resource="http://www.usgs.gov/science/USGSThesaurus/holmium"/>
    <skos:related rdf:resource="http://www.usgs.gov/science/USGSThesaurus/erbium"/>
    <skos:related rdf:resource="http://www.usgs.gov/science/USGSThesaurus/thulium"/>
    <skos:related rdf:resource="http://www.usgs.gov/science/USGSThesaurus/ytterbium"/>
    <skos:related rdf:resource="http://www.usgs.gov/science/USGSThesaurus/lutetium"/>
    <skos:inScheme rdf:resource="http://www.usgs.gov/science/USGSThesaurus"/>
  </rdf:Description>
  <rdf:Description about="http://www.usgs.gov/science/USGSThesaurus/metal%20elements">
    <rdf:type rdf:resource="http://www.w3.org/2004/02/skos/core#Concept"/>
    <skos:prefLabel xml:lang="en">metal elements</skos:prefLabel>
    <skos:scopeNote xml:lang="en"></skos:scopeNote>
    <skos:broader rdf:resource="http://www.usgs.gov/science/USGSThesaurus/chemical%20element%20groups"/>
    <skos:related rdf:resource="http://www.usgs.gov/science/USGSThesaurus/scandium"/>
    <skos:related rdf:resource="http://www.usgs.gov/science/USGSThesaurus/titanium"/>
    <skos:related rdf:resource="http://www.usgs.gov/science/USGSThesaurus/vanadium"/>
    <skos:related rdf:resource="http://www.usgs.gov/science/USGSThesaurus/chromium"/>
    <skos:related rdf:resource="http://www.usgs.gov/science/USGSThesaurus/manganese"/>
    <skos:related rdf:resource="http://www.usgs.gov/science/USGSThesaurus/iron"/>
    <skos:related rdf:resource="http://www.usgs.gov/science/USGSThesaurus/cobalt"/>
    <skos:related rdf:resource="http://www.usgs.gov/science/USGSThesaurus/nickel"/>
    <skos:related rdf:resource="http://www.usgs.gov/science/USGSThesaurus/copper"/>
    <skos:related rdf:resource="http://www.usgs.gov/science/USGSThesaurus/zinc"/>
    <skos:related rdf:resource="http://www.usgs.gov/science/USGSThesaurus/yttrium"/>
    <skos:related rdf:resource="http://www.usgs.gov/science/USGSThesaurus/zirconium"/>
    <skos:related rdf:resource="http://www.usgs.gov/science/USGSThesaurus/niobium"/>
    <skos:related rdf:resource="http://www.usgs.gov/science/USGSThesaurus/molybdenum"/>
    <skos:related rdf:resource="http://www.usgs.gov/science/USGSThesaurus/technetium"/>
    <skos:related rdf:resource="http://www.usgs.gov/science/USGSThesaurus/ruthenium"/>
    <skos:related rdf:resource="http://www.usgs.gov/science/USGSThesaurus/rhodium"/>
    <skos:related rdf:resource="http://www.usgs.gov/science/USGSThesaurus/palladium"/>
    <skos:related rdf:resource="http://www.usgs.gov/science/USGSThesaurus/silver"/>
    <skos:related rdf:resource="http://www.usgs.gov/science/USGSThesaurus/cadmium"/>
    <skos:related rdf:resource="http://www.usgs.gov/science/USGSThesaurus/hafnium"/>
    <skos:related rdf:resource="http://www.usgs.gov/science/USGSThesaurus/tantalum"/>
    <skos:related rdf:resource="http://www.usgs.gov/science/USGSThesaurus/tungsten"/>
    <skos:related rdf:resource="http://www.usgs.gov/science/USGSThesaurus/rhenium"/>
    <skos:related rdf:resource="http://www.usgs.gov/science/USGSThesaurus/osmium"/>
    <skos:related rdf:resource="http://www.usgs.gov/science/USGSThesaurus/iridium"/>
    <skos:related rdf:resource="http://www.usgs.gov/science/USGSThesaurus/platinum"/>
    <skos:related rdf:resource="http://www.usgs.gov/science/USGSThesaurus/gold"/>
    <skos:related rdf:resource="http://www.usgs.gov/science/USGSThesaurus/mercury"/>
    <skos:related rdf:resource="http://www.usgs.gov/science/USGSThesaurus/rutherfordium"/>
    <skos:related rdf:resource="http://www.usgs.gov/science/USGSThesaurus/dubnium"/>
    <skos:related rdf:resource="http://www.usgs.gov/science/USGSThesaurus/seaborgium"/>
    <skos:related rdf:resource="http://www.usgs.gov/science/USGSThesaurus/bohrium"/>
    <skos:related rdf:resource="http://www.usgs.gov/science/USGSThesaurus/hassium"/>
    <skos:related rdf:resource="http://www.usgs.gov/science/USGSThesaurus/meitnerium"/>
    <skos:related rdf:resource="http://www.usgs.gov/science/USGSThesaurus/darmstadtium"/>
    <skos:related rdf:resource="http://www.usgs.gov/science/USGSThesaurus/ununnilium"/>
    <skos:related rdf:resource="http://www.usgs.gov/science/USGSThesaurus/ununnunium"/>
    <skos:related rdf:resource="http://www.usgs.gov/science/USGSThesaurus/ununnubium"/>
    <skos:related rdf:resource="http://www.usgs.gov/science/USGSThesaurus/aluminum"/>
    <skos:related rdf:resource="http://www.usgs.gov/science/USGSThesaurus/gallium"/>
    <skos:related rdf:resource="http://www.usgs.gov/science/USGSThesaurus/germanium"/>
    <skos:related rdf:resource="http://www.usgs.gov/science/USGSThesaurus/indium"/>
    <skos:related rdf:resource="http://www.usgs.gov/science/USGSThesaurus/tin"/>
    <skos:related rdf:resource="http://www.usgs.gov/science/USGSThesaurus/antimony"/>
    <skos:related rdf:resource="http://www.usgs.gov/science/USGSThesaurus/thallium"/>
    <skos:related rdf:resource="http://www.usgs.gov/science/USGSThesaurus/lead"/>
    <skos:related rdf:resource="http://www.usgs.gov/science/USGSThesaurus/bismuth"/>
    <skos:related rdf:resource="http://www.usgs.gov/science/USGSThesaurus/polonium"/>
    <skos:inScheme rdf:resource="http://www.usgs.gov/science/USGSThesaurus"/>
  </rdf:Description>
  <rdf:Description about="http://www.usgs.gov/science/USGSThesaurus/noble%20gas%20elements">
    <rdf:type rdf:resource="http://www.w3.org/2004/02/skos/core#Concept"/>
    <skos:prefLabel xml:lang="en">noble gas elements</skos:prefLabel>
    <skos:scopeNote xml:lang="en"></skos:scopeNote>
    <skos:altLabel xml:lang="en">inert gases</skos:altLabel>
    <skos:broader rdf:resource="http://www.usgs.gov/science/USGSThesaurus/chemical%20element%20groups"/>
    <skos:related rdf:resource="http://www.usgs.gov/science/USGSThesaurus/helium"/>
    <skos:related rdf:resource="http://www.usgs.gov/science/USGSThesaurus/neon"/>
    <skos:related rdf:resource="http://www.usgs.gov/science/USGSThesaurus/argon"/>
    <skos:related rdf:resource="http://www.usgs.gov/science/USGSThesaurus/krypton"/>
    <skos:related rdf:resource="http://www.usgs.gov/science/USGSThesaurus/xenon"/>
    <skos:related rdf:resource="http://www.usgs.gov/science/USGSThesaurus/radon"/>
    <skos:inScheme rdf:resource="http://www.usgs.gov/science/USGSThesaurus"/>
  </rdf:Description>
  <rdf:Description about="http://www.usgs.gov/science/USGSThesaurus/nonmetal%20elements">
    <rdf:type rdf:resource="http://www.w3.org/2004/02/skos/core#Concept"/>
    <skos:prefLabel xml:lang="en">nonmetal elements</skos:prefLabel>
    <skos:scopeNote xml:lang="en"></skos:scopeNote>
    <skos:broader rdf:resource="http://www.usgs.gov/science/USGSThesaurus/chemical%20element%20groups"/>
    <skos:related rdf:resource="http://www.usgs.gov/science/USGSThesaurus/boron"/>
    <skos:related rdf:resource="http://www.usgs.gov/science/USGSThesaurus/carbon"/>
    <skos:related rdf:resource="http://www.usgs.gov/science/USGSThesaurus/nitrogen"/>
    <skos:related rdf:resource="http://www.usgs.gov/science/USGSThesaurus/oxygen"/>
    <skos:related rdf:resource="http://www.usgs.gov/science/USGSThesaurus/silicon"/>
    <skos:related rdf:resource="http://www.usgs.gov/science/USGSThesaurus/phosphorus"/>
    <skos:related rdf:resource="http://www.usgs.gov/science/USGSThesaurus/sulfur"/>
    <skos:related rdf:resource="http://www.usgs.gov/science/USGSThesaurus/arsenic"/>
    <skos:related rdf:resource="http://www.usgs.gov/science/USGSThesaurus/selenium"/>
    <skos:related rdf:resource="http://www.usgs.gov/science/USGSThesaurus/tellurium"/>
    <skos:inScheme rdf:resource="http://www.usgs.gov/science/USGSThesaurus"/>
  </rdf:Description>
  <rdf:Description about="http://www.usgs.gov/science/USGSThesaurus/rare%20earth%20elements">
    <rdf:type rdf:resource="http://www.w3.org/2004/02/skos/core#Concept"/>
    <skos:prefLabel xml:lang="en">rare earth elements</skos:prefLabel>
    <skos:scopeNote xml:lang="en"></skos:scopeNote>
    <skos:broader rdf:resource="http://www.usgs.gov/science/USGSThesaurus/chemical%20element%20groups"/>
    <skos:related rdf:resource="http://www.usgs.gov/science/USGSThesaurus/scandium"/>
    <skos:related rdf:resource="http://www.usgs.gov/science/USGSThesaurus/yttrium"/>
    <skos:related rdf:resource="http://www.usgs.gov/science/USGSThesaurus/lanthanide%20series%20elements"/>
    <skos:inScheme rdf:resource="http://www.usgs.gov/science/USGSThesaurus"/>
  </rdf:Description>
  <rdf:Description about="http://www.usgs.gov/science/USGSThesaurus/chemical%20elements">
    <rdf:type rdf:resource="http://www.w3.org/2004/02/skos/core#Concept"/>
    <skos:prefLabel xml:lang="en">chemical elements</skos:prefLabel>
    <skos:scopeNote xml:lang="en">Chemical substances distinguished by atomic number. http://periodic.lanl.gov/</skos:scopeNote>
    <skos:broader rdf:resource="http://www.usgs.gov/science/USGSThesaurus/elements"/>
    <skos:narrower rdf:resource="http://www.usgs.gov/science/USGSThesaurus/actinium"/>
    <skos:narrower rdf:resource="http://www.usgs.gov/science/USGSThesaurus/aluminum"/>
    <skos:narrower rdf:resource="http://www.usgs.gov/science/USGSThesaurus/americium"/>
    <skos:narrower rdf:resource="http://www.usgs.gov/science/USGSThesaurus/antimony"/>
    <skos:narrower rdf:resource="http://www.usgs.gov/science/USGSThesaurus/argon"/>
    <skos:narrower rdf:resource="http://www.usgs.gov/science/USGSThesaurus/arsenic"/>
    <skos:narrower rdf:resource="http://www.usgs.gov/science/USGSThesaurus/astatine"/>
    <skos:narrower rdf:resource="http://www.usgs.gov/science/USGSThesaurus/barium"/>
    <skos:narrower rdf:resource="http://www.usgs.gov/science/USGSThesaurus/berkelium"/>
    <skos:narrower rdf:resource="http://www.usgs.gov/science/USGSThesaurus/beryllium"/>
    <skos:narrower rdf:resource="http://www.usgs.gov/science/USGSThesaurus/bismuth"/>
    <skos:narrower rdf:resource="http://www.usgs.gov/science/USGSThesaurus/bohrium"/>
    <skos:narrower rdf:resource="http://www.usgs.gov/science/USGSThesaurus/boron"/>
    <skos:narrower rdf:resource="http://www.usgs.gov/science/USGSThesaurus/bromine"/>
    <skos:narrower rdf:resource="http://www.usgs.gov/science/USGSThesaurus/cadmium"/>
    <skos:narrower rdf:resource="http://www.usgs.gov/science/USGSThesaurus/calcium"/>
    <skos:narrower rdf:resource="http://www.usgs.gov/science/USGSThesaurus/californium"/>
    <skos:narrower rdf:resource="http://www.usgs.gov/science/USGSThesaurus/carbon"/>
    <skos:narrower rdf:resource="http://www.usgs.gov/science/USGSThesaurus/cerium"/>
    <skos:narrower rdf:resource="http://www.usgs.gov/science/USGSThesaurus/cesium"/>
    <skos:narrower rdf:resource="http://www.usgs.gov/science/USGSThesaurus/chlorine"/>
    <skos:narrower rdf:resource="http://www.usgs.gov/science/USGSThesaurus/chromium"/>
    <skos:narrower rdf:resource="http://www.usgs.gov/science/USGSThesaurus/cobalt"/>
    <skos:narrower rdf:resource="http://www.usgs.gov/science/USGSThesaurus/copper"/>
    <skos:narrower rdf:resource="http://www.usgs.gov/science/USGSThesaurus/curium"/>
    <skos:narrower rdf:resource="http://www.usgs.gov/science/USGSThesaurus/darmstadtium"/>
    <skos:narrower rdf:resource="http://www.usgs.gov/science/USGSThesaurus/dubnium"/>
    <skos:narrower rdf:resource="http://www.usgs.gov/science/USGSThesaurus/dysprosium"/>
    <skos:narrower rdf:resource="http://www.usgs.gov/science/USGSThesaurus/einsteinium"/>
    <skos:narrower rdf:resource="http://www.usgs.gov/science/USGSThesaurus/erbium"/>
    <skos:narrower rdf:resource="http://www.usgs.gov/science/USGSThesaurus/europium"/>
    <skos:narrower rdf:resource="http://www.usgs.gov/science/USGSThesaurus/fermium"/>
    <skos:narrower rdf:resource="http://www.usgs.gov/science/USGSThesaurus/fluorine"/>
    <skos:narrower rdf:resource="http://www.usgs.gov/science/USGSThesaurus/francium"/>
    <skos:narrower rdf:resource="http://www.usgs.gov/science/USGSThesaurus/gadolinium"/>
    <skos:narrower rdf:resource="http://www.usgs.gov/science/USGSThesaurus/gallium"/>
    <skos:narrower rdf:resource="http://www.usgs.gov/science/USGSThesaurus/germanium"/>
    <skos:narrower rdf:resource="http://www.usgs.gov/science/USGSThesaurus/gold"/>
    <skos:narrower rdf:resource="http://www.usgs.gov/science/USGSThesaurus/hafnium"/>
    <skos:narrower rdf:resource="http://www.usgs.gov/science/USGSThesaurus/hassium"/>
    <skos:narrower rdf:resource="http://www.usgs.gov/science/USGSThesaurus/helium"/>
    <skos:narrower rdf:resource="http://www.usgs.gov/science/USGSThesaurus/holmium"/>
    <skos:narrower rdf:resource="http://www.usgs.gov/science/USGSThesaurus/hydrogen"/>
    <skos:narrower rdf:resource="http://www.usgs.gov/science/USGSThesaurus/indium"/>
    <skos:narrower rdf:resource="http://www.usgs.gov/science/USGSThesaurus/iodine"/>
    <skos:narrower rdf:resource="http://www.usgs.gov/science/USGSThesaurus/iridium"/>
    <skos:narrower rdf:resource="http://www.usgs.gov/science/USGSThesaurus/iron"/>
    <skos:narrower rdf:resource="http://www.usgs.gov/science/USGSThesaurus/krypton"/>
    <skos:narrower rdf:resource="http://www.usgs.gov/science/USGSThesaurus/lanthanum"/>
    <skos:narrower rdf:resource="http://www.usgs.gov/science/USGSThesaurus/lawrencium"/>
    <skos:narrower rdf:resource="http://www.usgs.gov/science/USGSThesaurus/lead"/>
    <skos:narrower rdf:resource="http://www.usgs.gov/science/USGSThesaurus/lithium"/>
    <skos:narrower rdf:resource="http://www.usgs.gov/science/USGSThesaurus/lutetium"/>
    <skos:narrower rdf:resource="http://www.usgs.gov/science/USGSThesaurus/magnesium"/>
    <skos:narrower rdf:resource="http://www.usgs.gov/science/USGSThesaurus/manganese"/>
    <skos:narrower rdf:resource="http://www.usgs.gov/science/USGSThesaurus/meitnerium"/>
    <skos:narrower rdf:resource="http://www.usgs.gov/science/USGSThesaurus/mendelevium"/>
    <skos:narrower rdf:resource="http://www.usgs.gov/science/USGSThesaurus/mercury"/>
    <skos:narrower rdf:resource="http://www.usgs.gov/science/USGSThesaurus/molybdenum"/>
    <skos:narrower rdf:resource="http://www.usgs.gov/science/USGSThesaurus/neodymium"/>
    <skos:narrower rdf:resource="http://www.usgs.gov/science/USGSThesaurus/neon"/>
    <skos:narrower rdf:resource="http://www.usgs.gov/science/USGSThesaurus/neptunium"/>
    <skos:narrower rdf:resource="http://www.usgs.gov/science/USGSThesaurus/nickel"/>
    <skos:narrower rdf:resource="http://www.usgs.gov/science/USGSThesaurus/niobium"/>
    <skos:narrower rdf:resource="http://www.usgs.gov/science/USGSThesaurus/nitrogen"/>
    <skos:narrower rdf:resource="http://www.usgs.gov/science/USGSThesaurus/nobelium"/>
    <skos:narrower rdf:resource="http://www.usgs.gov/science/USGSThesaurus/osmium"/>
    <skos:narrower rdf:resource="http://www.usgs.gov/science/USGSThesaurus/oxygen"/>
    <skos:narrower rdf:resource="http://www.usgs.gov/science/USGSThesaurus/palladium"/>
    <skos:narrower rdf:resource="http://www.usgs.gov/science/USGSThesaurus/phosphorus"/>
    <skos:narrower rdf:resource="http://www.usgs.gov/science/USGSThesaurus/platinum"/>
    <skos:narrower rdf:resource="http://www.usgs.gov/science/USGSThesaurus/plutonium"/>
    <skos:narrower rdf:resource="http://www.usgs.gov/science/USGSThesaurus/polonium"/>
    <skos:narrower rdf:resource="http://www.usgs.gov/science/USGSThesaurus/potassium"/>
    <skos:narrower rdf:resource="http://www.usgs.gov/science/USGSThesaurus/praseodymium"/>
    <skos:narrower rdf:resource="http://www.usgs.gov/science/USGSThesaurus/promethium"/>
    <skos:narrower rdf:resource="http://www.usgs.gov/science/USGSThesaurus/protactinium"/>
    <skos:narrower rdf:resource="http://www.usgs.gov/science/USGSThesaurus/radium"/>
    <skos:narrower rdf:resource="http://www.usgs.gov/science/USGSThesaurus/radon"/>
    <skos:narrower rdf:resource="http://www.usgs.gov/science/USGSThesaurus/rhenium"/>
    <skos:narrower rdf:resource="http://www.usgs.gov/science/USGSThesaurus/rhodium"/>
    <skos:narrower rdf:resource="http://www.usgs.gov/science/USGSThesaurus/rubidium"/>
    <skos:narrower rdf:resource="http://www.usgs.gov/science/USGSThesaurus/ruthenium"/>
    <skos:narrower rdf:resource="http://www.usgs.gov/science/USGSThesaurus/rutherfordium"/>
    <skos:narrower rdf:resource="http://www.usgs.gov/science/USGSThesaurus/samarium"/>
    <skos:narrower rdf:resource="http://www.usgs.gov/science/USGSThesaurus/scandium"/>
    <skos:narrower rdf:resource="http://www.usgs.gov/science/USGSThesaurus/seaborgium"/>
    <skos:narrower rdf:resource="http://www.usgs.gov/science/USGSThesaurus/selenium"/>
    <skos:narrower rdf:resource="http://www.usgs.gov/science/USGSThesaurus/silicon"/>
    <skos:narrower rdf:resource="http://www.usgs.gov/science/USGSThesaurus/silver"/>
    <skos:narrower rdf:resource="http://www.usgs.gov/science/USGSThesaurus/sodium"/>
    <skos:narrower rdf:resource="http://www.usgs.gov/science/USGSThesaurus/strontium"/>
    <skos:narrower rdf:resource="http://www.usgs.gov/science/USGSThesaurus/sulfur"/>
    <skos:narrower rdf:resource="http://www.usgs.gov/science/USGSThesaurus/tantalum"/>
    <skos:narrower rdf:resource="http://www.usgs.gov/science/USGSThesaurus/technetium"/>
    <skos:narrower rdf:resource="http://www.usgs.gov/science/USGSThesaurus/tellurium"/>
    <skos:narrower rdf:resource="http://www.usgs.gov/science/USGSThesaurus/terbium"/>
    <skos:narrower rdf:resource="http://www.usgs.gov/science/USGSThesaurus/thallium"/>
    <skos:narrower rdf:resource="http://www.usgs.gov/science/USGSThesaurus/thorium"/>
    <skos:narrower rdf:resource="http://www.usgs.gov/science/USGSThesaurus/thulium"/>
    <skos:narrower rdf:resource="http://www.usgs.gov/science/USGSThesaurus/tin"/>
    <skos:narrower rdf:resource="http://www.usgs.gov/science/USGSThesaurus/titanium"/>
    <skos:narrower rdf:resource="http://www.usgs.gov/science/USGSThesaurus/tungsten"/>
    <skos:narrower rdf:resource="http://www.usgs.gov/science/USGSThesaurus/ununnilium"/>
    <skos:narrower rdf:resource="http://www.usgs.gov/science/USGSThesaurus/ununnubium"/>
    <skos:narrower rdf:resource="http://www.usgs.gov/science/USGSThesaurus/ununnunium"/>
    <skos:narrower rdf:resource="http://www.usgs.gov/science/USGSThesaurus/uranium"/>
    <skos:narrower rdf:resource="http://www.usgs.gov/science/USGSThesaurus/vanadium"/>
    <skos:narrower rdf:resource="http://www.usgs.gov/science/USGSThesaurus/xenon"/>
    <skos:narrower rdf:resource="http://www.usgs.gov/science/USGSThesaurus/ytterbium"/>
    <skos:narrower rdf:resource="http://www.usgs.gov/science/USGSThesaurus/yttrium"/>
    <skos:narrower rdf:resource="http://www.usgs.gov/science/USGSThesaurus/zinc"/>
    <skos:narrower rdf:resource="http://www.usgs.gov/science/USGSThesaurus/zirconium"/>
    <skos:inScheme rdf:resource="http://www.usgs.gov/science/USGSThesaurus"/>
  </rdf:Description>
  <rdf:Description about="http://www.usgs.gov/science/USGSThesaurus/actinium">
    <rdf:type rdf:resource="http://www.w3.org/2004/02/skos/core#Concept"/>
    <skos:prefLabel xml:lang="en">actinium</skos:prefLabel>
    <skos:scopeNote xml:lang="en">Rare earth (actinide series) element with symbol Ac and atomic number 89 &lt;http://periodic.lanl.gov/89.shtml&gt;</skos:scopeNote>
    <skos:altLabel xml:lang="en">Ac</skos:altLabel>
    <skos:broader rdf:resource="http://www.usgs.gov/science/USGSThesaurus/chemical%20elements"/>
    <skos:related rdf:resource="http://www.usgs.gov/science/USGSThesaurus/actinide%20series%20elements"/>
    <skos:inScheme rdf:resource="http://www.usgs.gov/science/USGSThesaurus"/>
  </rdf:Description>
  <rdf:Description about="http://www.usgs.gov/science/USGSThesaurus/aluminum">
    <rdf:type rdf:resource="http://www.w3.org/2004/02/skos/core#Concept"/>
    <skos:prefLabel xml:lang="en">aluminum</skos:prefLabel>
    <skos:scopeNote xml:lang="en">Metalloid element with symbol Al and atomic number 13 &lt;http://periodic.lanl.gov/13.shtml&gt;</skos:scopeNote>
    <skos:altLabel xml:lang="en">Al</skos:altLabel>
    <skos:broader rdf:resource="http://www.usgs.gov/science/USGSThesaurus/chemical%20elements"/>
    <skos:related rdf:resource="http://www.usgs.gov/science/USGSThesaurus/metal%20elements"/>
    <skos:inScheme rdf:resource="http://www.usgs.gov/science/USGSThesaurus"/>
  </rdf:Description>
  <rdf:Description about="http://www.usgs.gov/science/USGSThesaurus/americium">
    <rdf:type rdf:resource="http://www.w3.org/2004/02/skos/core#Concept"/>
    <skos:prefLabel xml:lang="en">americium</skos:prefLabel>
    <skos:scopeNote xml:lang="en">Rare earth (actinide series) element with symbol Am and atomic number 95 &lt;http://periodic.lanl.gov/95.shtml&gt;</skos:scopeNote>
    <skos:altLabel xml:lang="en">Am</skos:altLabel>
    <skos:broader rdf:resource="http://www.usgs.gov/science/USGSThesaurus/chemical%20elements"/>
    <skos:related rdf:resource="http://www.usgs.gov/science/USGSThesaurus/actinide%20series%20elements"/>
    <skos:inScheme rdf:resource="http://www.usgs.gov/science/USGSThesaurus"/>
  </rdf:Description>
  <rdf:Description about="http://www.usgs.gov/science/USGSThesaurus/antimony">
    <rdf:type rdf:resource="http://www.w3.org/2004/02/skos/core#Concept"/>
    <skos:prefLabel xml:lang="en">antimony</skos:prefLabel>
    <skos:scopeNote xml:lang="en">Metalloid element with symbol Sb and atomic number 51 &lt;http://periodic.lanl.gov/51.shtml&gt;</skos:scopeNote>
    <skos:altLabel xml:lang="en">Sb</skos:altLabel>
    <skos:broader rdf:resource="http://www.usgs.gov/science/USGSThesaurus/chemical%20elements"/>
    <skos:related rdf:resource="http://www.usgs.gov/science/USGSThesaurus/metal%20elements"/>
    <skos:inScheme rdf:resource="http://www.usgs.gov/science/USGSThesaurus"/>
  </rdf:Description>
  <rdf:Description about="http://www.usgs.gov/science/USGSThesaurus/argon">
    <rdf:type rdf:resource="http://www.w3.org/2004/02/skos/core#Concept"/>
    <skos:prefLabel xml:lang="en">argon</skos:prefLabel>
    <skos:scopeNote xml:lang="en">Noble gas element with symbol Ar and atomic number 18 &lt;http://periodic.lanl.gov/18.shtml&gt;</skos:scopeNote>
    <skos:altLabel xml:lang="en">Ar</skos:altLabel>
    <skos:broader rdf:resource="http://www.usgs.gov/science/USGSThesaurus/chemical%20elements"/>
    <skos:related rdf:resource="http://www.usgs.gov/science/USGSThesaurus/noble%20gas%20elements"/>
    <skos:inScheme rdf:resource="http://www.usgs.gov/science/USGSThesaurus"/>
  </rdf:Description>
  <rdf:Description about="http://www.usgs.gov/science/USGSThesaurus/arsenic">
    <rdf:type rdf:resource="http://www.w3.org/2004/02/skos/core#Concept"/>
    <skos:prefLabel xml:lang="en">arsenic</skos:prefLabel>
    <skos:scopeNote xml:lang="en">Nonmetal element with symbol As and atomic number 33 &lt;http://periodic.lanl.gov/33.shtml&gt;</skos:scopeNote>
    <skos:altLabel xml:lang="en">As</skos:altLabel>
    <skos:broader rdf:resource="http://www.usgs.gov/science/USGSThesaurus/chemical%20elements"/>
    <skos:related rdf:resource="http://www.usgs.gov/science/USGSThesaurus/nonmetal%20elements"/>
    <skos:inScheme rdf:resource="http://www.usgs.gov/science/USGSThesaurus"/>
  </rdf:Description>
  <rdf:Description about="http://www.usgs.gov/science/USGSThesaurus/astatine">
    <rdf:type rdf:resource="http://www.w3.org/2004/02/skos/core#Concept"/>
    <skos:prefLabel xml:lang="en">astatine</skos:prefLabel>
    <skos:scopeNote xml:lang="en">Halogen element with symbol At and atomic number 85 &lt;http://periodic.lanl.gov/85.shtml&gt;</skos:scopeNote>
    <skos:altLabel xml:lang="en">At</skos:altLabel>
    <skos:broader rdf:resource="http://www.usgs.gov/science/USGSThesaurus/chemical%20elements"/>
    <skos:related rdf:resource="http://www.usgs.gov/science/USGSThesaurus/halogen%20elements"/>
    <skos:inScheme rdf:resource="http://www.usgs.gov/science/USGSThesaurus"/>
  </rdf:Description>
  <rdf:Description about="http://www.usgs.gov/science/USGSThesaurus/barium">
    <rdf:type rdf:resource="http://www.w3.org/2004/02/skos/core#Concept"/>
    <skos:prefLabel xml:lang="en">barium</skos:prefLabel>
    <skos:scopeNote xml:lang="en">Alkaline earth element with symbol Ba and atomic number 56 &lt;http://periodic.lanl.gov/56.shtml&gt;</skos:scopeNote>
    <skos:altLabel xml:lang="en">Ba</skos:altLabel>
    <skos:broader rdf:resource="http://www.usgs.gov/science/USGSThesaurus/chemical%20elements"/>
    <skos:related rdf:resource="http://www.usgs.gov/science/USGSThesaurus/alkaline%20earth%20elements"/>
    <skos:inScheme rdf:resource="http://www.usgs.gov/science/USGSThesaurus"/>
  </rdf:Description>
  <rdf:Description about="http://www.usgs.gov/science/USGSThesaurus/berkelium">
    <rdf:type rdf:resource="http://www.w3.org/2004/02/skos/core#Concept"/>
    <skos:prefLabel xml:lang="en">berkelium</skos:prefLabel>
    <skos:scopeNote xml:lang="en">Rare earth (actinide series) element with symbol Bk and atomic number 97 &lt;http://periodic.lanl.gov/97.shtml&gt;</skos:scopeNote>
    <skos:altLabel xml:lang="en">Bk</skos:altLabel>
    <skos:broader rdf:resource="http://www.usgs.gov/science/USGSThesaurus/chemical%20elements"/>
    <skos:related rdf:resource="http://www.usgs.gov/science/USGSThesaurus/actinide%20series%20elements"/>
    <skos:inScheme rdf:resource="http://www.usgs.gov/science/USGSThesaurus"/>
  </rdf:Description>
  <rdf:Description about="http://www.usgs.gov/science/USGSThesaurus/beryllium">
    <rdf:type rdf:resource="http://www.w3.org/2004/02/skos/core#Concept"/>
    <skos:prefLabel xml:lang="en">beryllium</skos:prefLabel>
    <skos:scopeNote xml:lang="en">Alkaline earth element with symbol Be and atomic number 4 &lt;http://periodic.lanl.gov/4.shtml&gt;</skos:scopeNote>
    <skos:altLabel xml:lang="en">Be</skos:altLabel>
    <skos:broader rdf:resource="http://www.usgs.gov/science/USGSThesaurus/chemical%20elements"/>
    <skos:related rdf:resource="http://www.usgs.gov/science/USGSThesaurus/alkaline%20earth%20elements"/>
    <skos:inScheme rdf:resource="http://www.usgs.gov/science/USGSThesaurus"/>
  </rdf:Description>
  <rdf:Description about="http://www.usgs.gov/science/USGSThesaurus/bismuth">
    <rdf:type rdf:resource="http://www.w3.org/2004/02/skos/core#Concept"/>
    <skos:prefLabel xml:lang="en">bismuth</skos:prefLabel>
    <skos:scopeNote xml:lang="en">Metalloid element with symbol Bi and atomic number 83 &lt;http://periodic.lanl.gov/83.shtml&gt;</skos:scopeNote>
    <skos:altLabel xml:lang="en">Bi</skos:altLabel>
    <skos:broader rdf:resource="http://www.usgs.gov/science/USGSThesaurus/chemical%20elements"/>
    <skos:related rdf:resource="http://www.usgs.gov/science/USGSThesaurus/metal%20elements"/>
    <skos:inScheme rdf:resource="http://www.usgs.gov/science/USGSThesaurus"/>
  </rdf:Description>
  <rdf:Description about="http://www.usgs.gov/science/USGSThesaurus/bohrium">
    <rdf:type rdf:resource="http://www.w3.org/2004/02/skos/core#Concept"/>
    <skos:prefLabel xml:lang="en">bohrium</skos:prefLabel>
    <skos:scopeNote xml:lang="en">Metal element with symbol Bh and atomic number 107 &lt;http://periodic.lanl.gov/107.shtml&gt;</skos:scopeNote>
    <skos:altLabel xml:lang="en">Bh</skos:altLabel>
    <skos:broader rdf:resource="http://www.usgs.gov/science/USGSThesaurus/chemical%20elements"/>
    <skos:related rdf:resource="http://www.usgs.gov/science/USGSThesaurus/metal%20elements"/>
    <skos:inScheme rdf:resource="http://www.usgs.gov/science/USGSThesaurus"/>
  </rdf:Description>
  <rdf:Description about="http://www.usgs.gov/science/USGSThesaurus/boron">
    <rdf:type rdf:resource="http://www.w3.org/2004/02/skos/core#Concept"/>
    <skos:prefLabel xml:lang="en">boron</skos:prefLabel>
    <skos:scopeNote xml:lang="en">Nonmetal element with symbol B and atomic number 5 &lt;http://periodic.lanl.gov/5.shtml&gt;</skos:scopeNote>
    <skos:altLabel xml:lang="en">B</skos:altLabel>
    <skos:broader rdf:resource="http://www.usgs.gov/science/USGSThesaurus/chemical%20elements"/>
    <skos:related rdf:resource="http://www.usgs.gov/science/USGSThesaurus/nonmetal%20elements"/>
    <skos:inScheme rdf:resource="http://www.usgs.gov/science/USGSThesaurus"/>
  </rdf:Description>
  <rdf:Description about="http://www.usgs.gov/science/USGSThesaurus/bromine">
    <rdf:type rdf:resource="http://www.w3.org/2004/02/skos/core#Concept"/>
    <skos:prefLabel xml:lang="en">bromine</skos:prefLabel>
    <skos:scopeNote xml:lang="en">Halogen element with symbol Br and atomic number 35 &lt;http://periodic.lanl.gov/35.shtml&gt;</skos:scopeNote>
    <skos:altLabel xml:lang="en">Br</skos:altLabel>
    <skos:broader rdf:resource="http://www.usgs.gov/science/USGSThesaurus/chemical%20elements"/>
    <skos:related rdf:resource="http://www.usgs.gov/science/USGSThesaurus/halogen%20elements"/>
    <skos:inScheme rdf:resource="http://www.usgs.gov/science/USGSThesaurus"/>
  </rdf:Description>
  <rdf:Description about="http://www.usgs.gov/science/USGSThesaurus/cadmium">
    <rdf:type rdf:resource="http://www.w3.org/2004/02/skos/core#Concept"/>
    <skos:prefLabel xml:lang="en">cadmium</skos:prefLabel>
    <skos:scopeNote xml:lang="en">Metal element with symbol Cd and atomic number 48 &lt;http://periodic.lanl.gov/48.shtml&gt;</skos:scopeNote>
    <skos:altLabel xml:lang="en">Cd</skos:altLabel>
    <skos:broader rdf:resource="http://www.usgs.gov/science/USGSThesaurus/chemical%20elements"/>
    <skos:related rdf:resource="http://www.usgs.gov/science/USGSThesaurus/metal%20elements"/>
    <skos:inScheme rdf:resource="http://www.usgs.gov/science/USGSThesaurus"/>
  </rdf:Description>
  <rdf:Description about="http://www.usgs.gov/science/USGSThesaurus/calcium">
    <rdf:type rdf:resource="http://www.w3.org/2004/02/skos/core#Concept"/>
    <skos:prefLabel xml:lang="en">calcium</skos:prefLabel>
    <skos:scopeNote xml:lang="en">Alkaline earth element with symbol Ca and atomic number 20 &lt;http://periodic.lanl.gov/20.shtml&gt;</skos:scopeNote>
    <skos:altLabel xml:lang="en">Ca</skos:altLabel>
    <skos:broader rdf:resource="http://www.usgs.gov/science/USGSThesaurus/chemical%20elements"/>
    <skos:related rdf:resource="http://www.usgs.gov/science/USGSThesaurus/alkaline%20earth%20elements"/>
    <skos:inScheme rdf:resource="http://www.usgs.gov/science/USGSThesaurus"/>
  </rdf:Description>
  <rdf:Description about="http://www.usgs.gov/science/USGSThesaurus/californium">
    <rdf:type rdf:resource="http://www.w3.org/2004/02/skos/core#Concept"/>
    <skos:prefLabel xml:lang="en">californium</skos:prefLabel>
    <skos:scopeNote xml:lang="en">Rare earth (actinide series) element with symbol Cf and atomic number 98 &lt;http://periodic.lanl.gov/98.shtml&gt;</skos:scopeNote>
    <skos:altLabel xml:lang="en">Cf</skos:altLabel>
    <skos:broader rdf:resource="http://www.usgs.gov/science/USGSThesaurus/chemical%20elements"/>
    <skos:related rdf:resource="http://www.usgs.gov/science/USGSThesaurus/actinide%20series%20elements"/>
    <skos:inScheme rdf:resource="http://www.usgs.gov/science/USGSThesaurus"/>
  </rdf:Description>
  <rdf:Description about="http://www.usgs.gov/science/USGSThesaurus/carbon">
    <rdf:type rdf:resource="http://www.w3.org/2004/02/skos/core#Concept"/>
    <skos:prefLabel xml:lang="en">carbon</skos:prefLabel>
    <skos:scopeNote xml:lang="en">Nonmetal element with symbol C and atomic number 6 &lt;http://periodic.lanl.gov/6.shtml&gt;</skos:scopeNote>
    <skos:altLabel xml:lang="en">C</skos:altLabel>
    <skos:broader rdf:resource="http://www.usgs.gov/science/USGSThesaurus/chemical%20elements"/>
    <skos:related rdf:resource="http://www.usgs.gov/science/USGSThesaurus/nonmetal%20elements"/>
    <skos:inScheme rdf:resource="http://www.usgs.gov/science/USGSThesaurus"/>
  </rdf:Description>
  <rdf:Description about="http://www.usgs.gov/science/USGSThesaurus/cerium">
    <rdf:type rdf:resource="http://www.w3.org/2004/02/skos/core#Concept"/>
    <skos:prefLabel xml:lang="en">cerium</skos:prefLabel>
    <skos:scopeNote xml:lang="en">Rare earth (lanthanide series) element with symbol Ce and atomic number 58 &lt;http://periodic.lanl.gov/58.shtml&gt;</skos:scopeNote>
    <skos:altLabel xml:lang="en">Ce</skos:altLabel>
    <skos:broader rdf:resource="http://www.usgs.gov/science/USGSThesaurus/chemical%20elements"/>
    <skos:related rdf:resource="http://www.usgs.gov/science/USGSThesaurus/lanthanide%20series%20elements"/>
    <skos:inScheme rdf:resource="http://www.usgs.gov/science/USGSThesaurus"/>
  </rdf:Description>
  <rdf:Description about="http://www.usgs.gov/science/USGSThesaurus/cesium">
    <rdf:type rdf:resource="http://www.w3.org/2004/02/skos/core#Concept"/>
    <skos:prefLabel xml:lang="en">cesium</skos:prefLabel>
    <skos:scopeNote xml:lang="en">Alkali metal element with symbol Cs and atomic number 55 &lt;http://periodic.lanl.gov/55.shtml&gt;</skos:scopeNote>
    <skos:altLabel xml:lang="en">Cs</skos:altLabel>
    <skos:broader rdf:resource="http://www.usgs.gov/science/USGSThesaurus/chemical%20elements"/>
    <skos:related rdf:resource="http://www.usgs.gov/science/USGSThesaurus/alkali%20metal%20elements"/>
    <skos:inScheme rdf:resource="http://www.usgs.gov/science/USGSThesaurus"/>
  </rdf:Description>
  <rdf:Description about="http://www.usgs.gov/science/USGSThesaurus/chlorine">
    <rdf:type rdf:resource="http://www.w3.org/2004/02/skos/core#Concept"/>
    <skos:prefLabel xml:lang="en">chlorine</skos:prefLabel>
    <skos:scopeNote xml:lang="en">Halogen element with symbol Cl and atomic number 17 &lt;http://periodic.lanl.gov/17.shtml&gt;</skos:scopeNote>
    <skos:altLabel xml:lang="en">Cl</skos:altLabel>
    <skos:broader rdf:resource="http://www.usgs.gov/science/USGSThesaurus/chemical%20elements"/>
    <skos:related rdf:resource="http://www.usgs.gov/science/USGSThesaurus/halogen%20elements"/>
    <skos:inScheme rdf:resource="http://www.usgs.gov/science/USGSThesaurus"/>
  </rdf:Description>
  <rdf:Description about="http://www.usgs.gov/science/USGSThesaurus/chromium">
    <rdf:type rdf:resource="http://www.w3.org/2004/02/skos/core#Concept"/>
    <skos:prefLabel xml:lang="en">chromium</skos:prefLabel>
    <skos:scopeNote xml:lang="en">Metal element with symbol Cr and atomic number 24 &lt;http://periodic.lanl.gov/24.shtml&gt;</skos:scopeNote>
    <skos:altLabel xml:lang="en">Cr</skos:altLabel>
    <skos:broader rdf:resource="http://www.usgs.gov/science/USGSThesaurus/chemical%20elements"/>
    <skos:related rdf:resource="http://www.usgs.gov/science/USGSThesaurus/metal%20elements"/>
    <skos:inScheme rdf:resource="http://www.usgs.gov/science/USGSThesaurus"/>
  </rdf:Description>
  <rdf:Description about="http://www.usgs.gov/science/USGSThesaurus/cobalt">
    <rdf:type rdf:resource="http://www.w3.org/2004/02/skos/core#Concept"/>
    <skos:prefLabel xml:lang="en">cobalt</skos:prefLabel>
    <skos:scopeNote xml:lang="en">Metal element with symbol Co and atomic number 27 &lt;http://periodic.lanl.gov/27.shtml&gt;</skos:scopeNote>
    <skos:altLabel xml:lang="en">Co</skos:altLabel>
    <skos:broader rdf:resource="http://www.usgs.gov/science/USGSThesaurus/chemical%20elements"/>
    <skos:related rdf:resource="http://www.usgs.gov/science/USGSThesaurus/metal%20elements"/>
    <skos:inScheme rdf:resource="http://www.usgs.gov/science/USGSThesaurus"/>
  </rdf:Description>
  <rdf:Description about="http://www.usgs.gov/science/USGSThesaurus/copper">
    <rdf:type rdf:resource="http://www.w3.org/2004/02/skos/core#Concept"/>
    <skos:prefLabel xml:lang="en">copper</skos:prefLabel>
    <skos:scopeNote xml:lang="en">Metal element with symbol Cu and atomic number 29 &lt;http://periodic.lanl.gov/29.shtml&gt;</skos:scopeNote>
    <skos:altLabel xml:lang="en">Cu</skos:altLabel>
    <skos:broader rdf:resource="http://www.usgs.gov/science/USGSThesaurus/chemical%20elements"/>
    <skos:related rdf:resource="http://www.usgs.gov/science/USGSThesaurus/metal%20elements"/>
    <skos:inScheme rdf:resource="http://www.usgs.gov/science/USGSThesaurus"/>
  </rdf:Description>
  <rdf:Description about="http://www.usgs.gov/science/USGSThesaurus/curium">
    <rdf:type rdf:resource="http://www.w3.org/2004/02/skos/core#Concept"/>
    <skos:prefLabel xml:lang="en">curium</skos:prefLabel>
    <skos:scopeNote xml:lang="en">Rare earth (actinide series) element with symbol Cm and atomic number 96 &lt;http://periodic.lanl.gov/96.shtml&gt;</skos:scopeNote>
    <skos:altLabel xml:lang="en">Cm</skos:altLabel>
    <skos:broader rdf:resource="http://www.usgs.gov/science/USGSThesaurus/chemical%20elements"/>
    <skos:related rdf:resource="http://www.usgs.gov/science/USGSThesaurus/actinide%20series%20elements"/>
    <skos:inScheme rdf:resource="http://www.usgs.gov/science/USGSThesaurus"/>
  </rdf:Description>
  <rdf:Description about="http://www.usgs.gov/science/USGSThesaurus/darmstadtium">
    <rdf:type rdf:resource="http://www.w3.org/2004/02/skos/core#Concept"/>
    <skos:prefLabel xml:lang="en">darmstadtium</skos:prefLabel>
    <skos:scopeNote xml:lang="en">Metal element with symbol Ds and atomic number 110 &lt;http://periodic.lanl.gov/110.shtml&gt;</skos:scopeNote>
    <skos:altLabel xml:lang="en">Ds</skos:altLabel>
    <skos:broader rdf:resource="http://www.usgs.gov/science/USGSThesaurus/chemical%20elements"/>
    <skos:related rdf:resource="http://www.usgs.gov/science/USGSThesaurus/metal%20elements"/>
    <skos:inScheme rdf:resource="http://www.usgs.gov/science/USGSThesaurus"/>
  </rdf:Description>
  <rdf:Description about="http://www.usgs.gov/science/USGSThesaurus/dubnium">
    <rdf:type rdf:resource="http://www.w3.org/2004/02/skos/core#Concept"/>
    <skos:prefLabel xml:lang="en">dubnium</skos:prefLabel>
    <skos:scopeNote xml:lang="en">Metal element with symbol Db and atomic number 105 &lt;http://periodic.lanl.gov/105.shtml&gt;</skos:scopeNote>
    <skos:altLabel xml:lang="en">Db</skos:altLabel>
    <skos:broader rdf:resource="http://www.usgs.gov/science/USGSThesaurus/chemical%20elements"/>
    <skos:related rdf:resource="http://www.usgs.gov/science/USGSThesaurus/metal%20elements"/>
    <skos:inScheme rdf:resource="http://www.usgs.gov/science/USGSThesaurus"/>
  </rdf:Description>
  <rdf:Description about="http://www.usgs.gov/science/USGSThesaurus/dysprosium">
    <rdf:type rdf:resource="http://www.w3.org/2004/02/skos/core#Concept"/>
    <skos:prefLabel xml:lang="en">dysprosium</skos:prefLabel>
    <skos:scopeNote xml:lang="en">Rare earth (lanthanide series) element with symbol Dy and atomic number 66 &lt;http://periodic.lanl.gov/66.shtml&gt;</skos:scopeNote>
    <skos:altLabel xml:lang="en">Dy</skos:altLabel>
    <skos:broader rdf:resource="http://www.usgs.gov/science/USGSThesaurus/chemical%20elements"/>
    <skos:related rdf:resource="http://www.usgs.gov/science/USGSThesaurus/lanthanide%20series%20elements"/>
    <skos:inScheme rdf:resource="http://www.usgs.gov/science/USGSThesaurus"/>
  </rdf:Description>
  <rdf:Description about="http://www.usgs.gov/science/USGSThesaurus/einsteinium">
    <rdf:type rdf:resource="http://www.w3.org/2004/02/skos/core#Concept"/>
    <skos:prefLabel xml:lang="en">einsteinium</skos:prefLabel>
    <skos:scopeNote xml:lang="en">Rare earth (actinide series) element with symbol Es and atomic number 99 &lt;http://periodic.lanl.gov/99.shtml&gt;</skos:scopeNote>
    <skos:altLabel xml:lang="en">Es</skos:altLabel>
    <skos:broader rdf:resource="http://www.usgs.gov/science/USGSThesaurus/chemical%20elements"/>
    <skos:related rdf:resource="http://www.usgs.gov/science/USGSThesaurus/actinide%20series%20elements"/>
    <skos:inScheme rdf:resource="http://www.usgs.gov/science/USGSThesaurus"/>
  </rdf:Description>
  <rdf:Description about="http://www.usgs.gov/science/USGSThesaurus/erbium">
    <rdf:type rdf:resource="http://www.w3.org/2004/02/skos/core#Concept"/>
    <skos:prefLabel xml:lang="en">erbium</skos:prefLabel>
    <skos:scopeNote xml:lang="en">Rare earth (lanthanide series) element with symbol Er and atomic number 68 &lt;http://periodic.lanl.gov/68.shtml&gt;</skos:scopeNote>
    <skos:altLabel xml:lang="en">Er</skos:altLabel>
    <skos:broader rdf:resource="http://www.usgs.gov/science/USGSThesaurus/chemical%20elements"/>
    <skos:related rdf:resource="http://www.usgs.gov/science/USGSThesaurus/lanthanide%20series%20elements"/>
    <skos:inScheme rdf:resource="http://www.usgs.gov/science/USGSThesaurus"/>
  </rdf:Description>
  <rdf:Description about="http://www.usgs.gov/science/USGSThesaurus/europium">
    <rdf:type rdf:resource="http://www.w3.org/2004/02/skos/core#Concept"/>
    <skos:prefLabel xml:lang="en">europium</skos:prefLabel>
    <skos:scopeNote xml:lang="en">Rare earth (lanthanide series) element with symbol Eu and atomic number 63 &lt;http://periodic.lanl.gov/63.shtml&gt;</skos:scopeNote>
    <skos:altLabel xml:lang="en">Eu</skos:altLabel>
    <skos:broader rdf:resource="http://www.usgs.gov/science/USGSThesaurus/chemical%20elements"/>
    <skos:related rdf:resource="http://www.usgs.gov/science/USGSThesaurus/lanthanide%20series%20elements"/>
    <skos:inScheme rdf:resource="http://www.usgs.gov/science/USGSThesaurus"/>
  </rdf:Description>
  <rdf:Description about="http://www.usgs.gov/science/USGSThesaurus/fermium">
    <rdf:type rdf:resource="http://www.w3.org/2004/02/skos/core#Concept"/>
    <skos:prefLabel xml:lang="en">fermium</skos:prefLabel>
    <skos:scopeNote xml:lang="en">Rare earth (actinide series) element with symbol Fm and atomic number 100 &lt;http://periodic.lanl.gov/100.shtml&gt;</skos:scopeNote>
    <skos:altLabel xml:lang="en">Fm</skos:altLabel>
    <skos:broader rdf:resource="http://www.usgs.gov/science/USGSThesaurus/chemical%20elements"/>
    <skos:related rdf:resource="http://www.usgs.gov/science/USGSThesaurus/actinide%20series%20elements"/>
    <skos:inScheme rdf:resource="http://www.usgs.gov/science/USGSThesaurus"/>
  </rdf:Description>
  <rdf:Description about="http://www.usgs.gov/science/USGSThesaurus/fluorine">
    <rdf:type rdf:resource="http://www.w3.org/2004/02/skos/core#Concept"/>
    <skos:prefLabel xml:lang="en">fluorine</skos:prefLabel>
    <skos:scopeNote xml:lang="en">Halogen element with symbol F and atomic number 9 &lt;http://periodic.lanl.gov/9.shtml&gt;</skos:scopeNote>
    <skos:altLabel xml:lang="en">F</skos:altLabel>
    <skos:broader rdf:resource="http://www.usgs.gov/science/USGSThesaurus/chemical%20elements"/>
    <skos:related rdf:resource="http://www.usgs.gov/science/USGSThesaurus/halogen%20elements"/>
    <skos:inScheme rdf:resource="http://www.usgs.gov/science/USGSThesaurus"/>
  </rdf:Description>
  <rdf:Description about="http://www.usgs.gov/science/USGSThesaurus/francium">
    <rdf:type rdf:resource="http://www.w3.org/2004/02/skos/core#Concept"/>
    <skos:prefLabel xml:lang="en">francium</skos:prefLabel>
    <skos:scopeNote xml:lang="en">Alkali metal element with symbol Fr and atomic number 87 &lt;http://periodic.lanl.gov/87.shtml&gt;</skos:scopeNote>
    <skos:altLabel xml:lang="en">Fr</skos:altLabel>
    <skos:broader rdf:resource="http://www.usgs.gov/science/USGSThesaurus/chemical%20elements"/>
    <skos:related rdf:resource="http://www.usgs.gov/science/USGSThesaurus/alkali%20metal%20elements"/>
    <skos:inScheme rdf:resource="http://www.usgs.gov/science/USGSThesaurus"/>
  </rdf:Description>
  <rdf:Description about="http://www.usgs.gov/science/USGSThesaurus/gadolinium">
    <rdf:type rdf:resource="http://www.w3.org/2004/02/skos/core#Concept"/>
    <skos:prefLabel xml:lang="en">gadolinium</skos:prefLabel>
    <skos:scopeNote xml:lang="en">Rare earth (lanthanide series) element with symbol Gd and atomic number 64 &lt;http://periodic.lanl.gov/64.shtml&gt;</skos:scopeNote>
    <skos:altLabel xml:lang="en">Gd</skos:altLabel>
    <skos:broader rdf:resource="http://www.usgs.gov/science/USGSThesaurus/chemical%20elements"/>
    <skos:related rdf:resource="http://www.usgs.gov/science/USGSThesaurus/lanthanide%20series%20elements"/>
    <skos:inScheme rdf:resource="http://www.usgs.gov/science/USGSThesaurus"/>
  </rdf:Description>
  <rdf:Description about="http://www.usgs.gov/science/USGSThesaurus/gallium">
    <rdf:type rdf:resource="http://www.w3.org/2004/02/skos/core#Concept"/>
    <skos:prefLabel xml:lang="en">gallium</skos:prefLabel>
    <skos:scopeNote xml:lang="en">Metalloid element with symbol Ga and atomic number 31 &lt;http://periodic.lanl.gov/31.shtml&gt;</skos:scopeNote>
    <skos:altLabel xml:lang="en">Ga</skos:altLabel>
    <skos:broader rdf:resource="http://www.usgs.gov/science/USGSThesaurus/chemical%20elements"/>
    <skos:related rdf:resource="http://www.usgs.gov/science/USGSThesaurus/metal%20elements"/>
    <skos:inScheme rdf:resource="http://www.usgs.gov/science/USGSThesaurus"/>
  </rdf:Description>
  <rdf:Description about="http://www.usgs.gov/science/USGSThesaurus/germanium">
    <rdf:type rdf:resource="http://www.w3.org/2004/02/skos/core#Concept"/>
    <skos:prefLabel xml:lang="en">germanium</skos:prefLabel>
    <skos:scopeNote xml:lang="en">Metalloid element with symbol Ge and atomic number 32 &lt;http://periodic.lanl.gov/32.shtml&gt;</skos:scopeNote>
    <skos:altLabel xml:lang="en">Ge</skos:altLabel>
    <skos:broader rdf:resource="http://www.usgs.gov/science/USGSThesaurus/chemical%20elements"/>
    <skos:related rdf:resource="http://www.usgs.gov/science/USGSThesaurus/metal%20elements"/>
    <skos:inScheme rdf:resource="http://www.usgs.gov/science/USGSThesaurus"/>
  </rdf:Description>
  <rdf:Description about="http://www.usgs.gov/science/USGSThesaurus/gold">
    <rdf:type rdf:resource="http://www.w3.org/2004/02/skos/core#Concept"/>
    <skos:prefLabel xml:lang="en">gold</skos:prefLabel>
    <skos:scopeNote xml:lang="en">Metal element with symbol Au and atomic number 79 &lt;http://periodic.lanl.gov/79.shtml&gt;</skos:scopeNote>
    <skos:altLabel xml:lang="en">Au</skos:altLabel>
    <skos:broader rdf:resource="http://www.usgs.gov/science/USGSThesaurus/chemical%20elements"/>
    <skos:related rdf:resource="http://www.usgs.gov/science/USGSThesaurus/metal%20elements"/>
    <skos:inScheme rdf:resource="http://www.usgs.gov/science/USGSThesaurus"/>
  </rdf:Description>
  <rdf:Description about="http://www.usgs.gov/science/USGSThesaurus/hafnium">
    <rdf:type rdf:resource="http://www.w3.org/2004/02/skos/core#Concept"/>
    <skos:prefLabel xml:lang="en">hafnium</skos:prefLabel>
    <skos:scopeNote xml:lang="en">Metal element with symbol Hf and atomic number 72 &lt;http://periodic.lanl.gov/72.shtml&gt;</skos:scopeNote>
    <skos:altLabel xml:lang="en">Hf</skos:altLabel>
    <skos:broader rdf:resource="http://www.usgs.gov/science/USGSThesaurus/chemical%20elements"/>
    <skos:related rdf:resource="http://www.usgs.gov/science/USGSThesaurus/metal%20elements"/>
    <skos:inScheme rdf:resource="http://www.usgs.gov/science/USGSThesaurus"/>
  </rdf:Description>
  <rdf:Description about="http://www.usgs.gov/science/USGSThesaurus/hassium">
    <rdf:type rdf:resource="http://www.w3.org/2004/02/skos/core#Concept"/>
    <skos:prefLabel xml:lang="en">hassium</skos:prefLabel>
    <skos:scopeNote xml:lang="en">Metal element with symbol Hs and atomic number 108 &lt;http://periodic.lanl.gov/108.shtml&gt;</skos:scopeNote>
    <skos:altLabel xml:lang="en">Hs</skos:altLabel>
    <skos:broader rdf:resource="http://www.usgs.gov/science/USGSThesaurus/chemical%20elements"/>
    <skos:related rdf:resource="http://www.usgs.gov/science/USGSThesaurus/metal%20elements"/>
    <skos:inScheme rdf:resource="http://www.usgs.gov/science/USGSThesaurus"/>
  </rdf:Description>
  <rdf:Description about="http://www.usgs.gov/science/USGSThesaurus/helium">
    <rdf:type rdf:resource="http://www.w3.org/2004/02/skos/core#Concept"/>
    <skos:prefLabel xml:lang="en">helium</skos:prefLabel>
    <skos:scopeNote xml:lang="en">Noble gas element with symbol He and atomic number 2 &lt;http://periodic.lanl.gov/2.shtml&gt;</skos:scopeNote>
    <skos:altLabel xml:lang="en">He</skos:altLabel>
    <skos:broader rdf:resource="http://www.usgs.gov/science/USGSThesaurus/chemical%20elements"/>
    <skos:related rdf:resource="http://www.usgs.gov/science/USGSThesaurus/noble%20gas%20elements"/>
    <skos:inScheme rdf:resource="http://www.usgs.gov/science/USGSThesaurus"/>
  </rdf:Description>
  <rdf:Description about="http://www.usgs.gov/science/USGSThesaurus/holmium">
    <rdf:type rdf:resource="http://www.w3.org/2004/02/skos/core#Concept"/>
    <skos:prefLabel xml:lang="en">holmium</skos:prefLabel>
    <skos:scopeNote xml:lang="en">Rare earth (lanthanide series) element with symbol Ho and atomic number 67 &lt;http://periodic.lanl.gov/67.shtml&gt;</skos:scopeNote>
    <skos:altLabel xml:lang="en">Ho</skos:altLabel>
    <skos:broader rdf:resource="http://www.usgs.gov/science/USGSThesaurus/chemical%20elements"/>
    <skos:related rdf:resource="http://www.usgs.gov/science/USGSThesaurus/lanthanide%20series%20elements"/>
    <skos:inScheme rdf:resource="http://www.usgs.gov/science/USGSThesaurus"/>
  </rdf:Description>
  <rdf:Description about="http://www.usgs.gov/science/USGSThesaurus/hydrogen">
    <rdf:type rdf:resource="http://www.w3.org/2004/02/skos/core#Concept"/>
    <skos:prefLabel xml:lang="en">hydrogen</skos:prefLabel>
    <skos:scopeNote xml:lang="en">Alkali metal element with symbol H and atomic number 1 &lt;http://periodic.lanl.gov/1.shtml&gt;</skos:scopeNote>
    <skos:altLabel xml:lang="en">H</skos:altLabel>
    <skos:broader rdf:resource="http://www.usgs.gov/science/USGSThesaurus/chemical%20elements"/>
    <skos:related rdf:resource="http://www.usgs.gov/science/USGSThesaurus/alkali%20metal%20elements"/>
    <skos:inScheme rdf:resource="http://www.usgs.gov/science/USGSThesaurus"/>
  </rdf:Description>
  <rdf:Description about="http://www.usgs.gov/science/USGSThesaurus/indium">
    <rdf:type rdf:resource="http://www.w3.org/2004/02/skos/core#Concept"/>
    <skos:prefLabel xml:lang="en">indium</skos:prefLabel>
    <skos:scopeNote xml:lang="en">Metalloid element with symbol In and atomic number 49 &lt;http://periodic.lanl.gov/49.shtml&gt;</skos:scopeNote>
    <skos:altLabel xml:lang="en">In</skos:altLabel>
    <skos:broader rdf:resource="http://www.usgs.gov/science/USGSThesaurus/chemical%20elements"/>
    <skos:related rdf:resource="http://www.usgs.gov/science/USGSThesaurus/metal%20elements"/>
    <skos:inScheme rdf:resource="http://www.usgs.gov/science/USGSThesaurus"/>
  </rdf:Description>
  <rdf:Description about="http://www.usgs.gov/science/USGSThesaurus/iodine">
    <rdf:type rdf:resource="http://www.w3.org/2004/02/skos/core#Concept"/>
    <skos:prefLabel xml:lang="en">iodine</skos:prefLabel>
    <skos:scopeNote xml:lang="en">Halogen element with symbol I and atomic number 53 &lt;http://periodic.lanl.gov/53.shtml&gt;</skos:scopeNote>
    <skos:altLabel xml:lang="en">I</skos:altLabel>
    <skos:broader rdf:resource="http://www.usgs.gov/science/USGSThesaurus/chemical%20elements"/>
    <skos:related rdf:resource="http://www.usgs.gov/science/USGSThesaurus/halogen%20elements"/>
    <skos:inScheme rdf:resource="http://www.usgs.gov/science/USGSThesaurus"/>
  </rdf:Description>
  <rdf:Description about="http://www.usgs.gov/science/USGSThesaurus/iridium">
    <rdf:type rdf:resource="http://www.w3.org/2004/02/skos/core#Concept"/>
    <skos:prefLabel xml:lang="en">iridium</skos:prefLabel>
    <skos:scopeNote xml:lang="en">Metal element with symbol Ir and atomic number 77 &lt;http://periodic.lanl.gov/77.shtml&gt;</skos:scopeNote>
    <skos:altLabel xml:lang="en">Ir</skos:altLabel>
    <skos:altLabel xml:lang="en">irridium</skos:altLabel>
    <skos:broader rdf:resource="http://www.usgs.gov/science/USGSThesaurus/chemical%20elements"/>
    <skos:related rdf:resource="http://www.usgs.gov/science/USGSThesaurus/metal%20elements"/>
    <skos:inScheme rdf:resource="http://www.usgs.gov/science/USGSThesaurus"/>
  </rdf:Description>
  <rdf:Description about="http://www.usgs.gov/science/USGSThesaurus/iron">
    <rdf:type rdf:resource="http://www.w3.org/2004/02/skos/core#Concept"/>
    <skos:prefLabel xml:lang="en">iron</skos:prefLabel>
    <skos:scopeNote xml:lang="en">Metal element with symbol Fe and atomic number 26 &lt;http://periodic.lanl.gov/26.shtml&gt;</skos:scopeNote>
    <skos:altLabel xml:lang="en">Fe</skos:altLabel>
    <skos:broader rdf:resource="http://www.usgs.gov/science/USGSThesaurus/chemical%20elements"/>
    <skos:related rdf:resource="http://www.usgs.gov/science/USGSThesaurus/metal%20elements"/>
    <skos:inScheme rdf:resource="http://www.usgs.gov/science/USGSThesaurus"/>
  </rdf:Description>
  <rdf:Description about="http://www.usgs.gov/science/USGSThesaurus/krypton">
    <rdf:type rdf:resource="http://www.w3.org/2004/02/skos/core#Concept"/>
    <skos:prefLabel xml:lang="en">krypton</skos:prefLabel>
    <skos:scopeNote xml:lang="en">Noble gas element with symbol Kr and atomic number 36 &lt;http://periodic.lanl.gov/36.shtml&gt;</skos:scopeNote>
    <skos:altLabel xml:lang="en">Kr</skos:altLabel>
    <skos:broader rdf:resource="http://www.usgs.gov/science/USGSThesaurus/chemical%20elements"/>
    <skos:related rdf:resource="http://www.usgs.gov/science/USGSThesaurus/noble%20gas%20elements"/>
    <skos:inScheme rdf:resource="http://www.usgs.gov/science/USGSThesaurus"/>
  </rdf:Description>
  <rdf:Description about="http://www.usgs.gov/science/USGSThesaurus/lanthanum">
    <rdf:type rdf:resource="http://www.w3.org/2004/02/skos/core#Concept"/>
    <skos:prefLabel xml:lang="en">lanthanum</skos:prefLabel>
    <skos:scopeNote xml:lang="en">Rare earth (lanthanide series) element with symbol La and atomic number 57 &lt;http://periodic.lanl.gov/57.shtml&gt;</skos:scopeNote>
    <skos:altLabel xml:lang="en">La</skos:altLabel>
    <skos:broader rdf:resource="http://www.usgs.gov/science/USGSThesaurus/chemical%20elements"/>
    <skos:related rdf:resource="http://www.usgs.gov/science/USGSThesaurus/lanthanide%20series%20elements"/>
    <skos:inScheme rdf:resource="http://www.usgs.gov/science/USGSThesaurus"/>
  </rdf:Description>
  <rdf:Description about="http://www.usgs.gov/science/USGSThesaurus/lawrencium">
    <rdf:type rdf:resource="http://www.w3.org/2004/02/skos/core#Concept"/>
    <skos:prefLabel xml:lang="en">lawrencium</skos:prefLabel>
    <skos:scopeNote xml:lang="en">Rare earth (actinide series) element with symbol Lr and atomic number 103 &lt;http://periodic.lanl.gov/103.shtml&gt;</skos:scopeNote>
    <skos:altLabel xml:lang="en">Lr</skos:altLabel>
    <skos:broader rdf:resource="http://www.usgs.gov/science/USGSThesaurus/chemical%20elements"/>
    <skos:related rdf:resource="http://www.usgs.gov/science/USGSThesaurus/actinide%20series%20elements"/>
    <skos:inScheme rdf:resource="http://www.usgs.gov/science/USGSThesaurus"/>
  </rdf:Description>
  <rdf:Description about="http://www.usgs.gov/science/USGSThesaurus/lead">
    <rdf:type rdf:resource="http://www.w3.org/2004/02/skos/core#Concept"/>
    <skos:prefLabel xml:lang="en">lead</skos:prefLabel>
    <skos:scopeNote xml:lang="en">Metalloid element with symbol Pb and atomic number 82 &lt;http://periodic.lanl.gov/82.shtml&gt;</skos:scopeNote>
    <skos:altLabel xml:lang="en">Pb</skos:altLabel>
    <skos:broader rdf:resource="http://www.usgs.gov/science/USGSThesaurus/chemical%20elements"/>
    <skos:related rdf:resource="http://www.usgs.gov/science/USGSThesaurus/metal%20elements"/>
    <skos:inScheme rdf:resource="http://www.usgs.gov/science/USGSThesaurus"/>
  </rdf:Description>
  <rdf:Description about="http://www.usgs.gov/science/USGSThesaurus/lithium">
    <rdf:type rdf:resource="http://www.w3.org/2004/02/skos/core#Concept"/>
    <skos:prefLabel xml:lang="en">lithium</skos:prefLabel>
    <skos:scopeNote xml:lang="en">Alkali metal element with symbol Li and atomic number 3 &lt;http://periodic.lanl.gov/3.shtml&gt;</skos:scopeNote>
    <skos:altLabel xml:lang="en">Li</skos:altLabel>
    <skos:broader rdf:resource="http://www.usgs.gov/science/USGSThesaurus/chemical%20elements"/>
    <skos:related rdf:resource="http://www.usgs.gov/science/USGSThesaurus/alkali%20metal%20elements"/>
    <skos:inScheme rdf:resource="http://www.usgs.gov/science/USGSThesaurus"/>
  </rdf:Description>
  <rdf:Description about="http://www.usgs.gov/science/USGSThesaurus/lutetium">
    <rdf:type rdf:resource="http://www.w3.org/2004/02/skos/core#Concept"/>
    <skos:prefLabel xml:lang="en">lutetium</skos:prefLabel>
    <skos:scopeNote xml:lang="en">Rare earth (lanthanide series) element with symbol Lu and atomic number 71 &lt;http://periodic.lanl.gov/71.shtml&gt;</skos:scopeNote>
    <skos:altLabel xml:lang="en">Lu</skos:altLabel>
    <skos:broader rdf:resource="http://www.usgs.gov/science/USGSThesaurus/chemical%20elements"/>
    <skos:related rdf:resource="http://www.usgs.gov/science/USGSThesaurus/lanthanide%20series%20elements"/>
    <skos:inScheme rdf:resource="http://www.usgs.gov/science/USGSThesaurus"/>
  </rdf:Description>
  <rdf:Description about="http://www.usgs.gov/science/USGSThesaurus/magnesium">
    <rdf:type rdf:resource="http://www.w3.org/2004/02/skos/core#Concept"/>
    <skos:prefLabel xml:lang="en">magnesium</skos:prefLabel>
    <skos:scopeNote xml:lang="en">Alkaline earth element with symbol Mg and atomic number 12 &lt;http://periodic.lanl.gov/12.shtml&gt;</skos:scopeNote>
    <skos:altLabel xml:lang="en">Mg</skos:altLabel>
    <skos:broader rdf:resource="http://www.usgs.gov/science/USGSThesaurus/chemical%20elements"/>
    <skos:related rdf:resource="http://www.usgs.gov/science/USGSThesaurus/alkaline%20earth%20elements"/>
    <skos:inScheme rdf:resource="http://www.usgs.gov/science/USGSThesaurus"/>
  </rdf:Description>
  <rdf:Description about="http://www.usgs.gov/science/USGSThesaurus/manganese">
    <rdf:type rdf:resource="http://www.w3.org/2004/02/skos/core#Concept"/>
    <skos:prefLabel xml:lang="en">manganese</skos:prefLabel>
    <skos:scopeNote xml:lang="en">Metal element with symbol Mn and atomic number 25 &lt;http://periodic.lanl.gov/25.shtml&gt;</skos:scopeNote>
    <skos:altLabel xml:lang="en">Mn</skos:altLabel>
    <skos:broader rdf:resource="http://www.usgs.gov/science/USGSThesaurus/chemical%20elements"/>
    <skos:related rdf:resource="http://www.usgs.gov/science/USGSThesaurus/metal%20elements"/>
    <skos:inScheme rdf:resource="http://www.usgs.gov/science/USGSThesaurus"/>
  </rdf:Description>
  <rdf:Description about="http://www.usgs.gov/science/USGSThesaurus/meitnerium">
    <rdf:type rdf:resource="http://www.w3.org/2004/02/skos/core#Concept"/>
    <skos:prefLabel xml:lang="en">meitnerium</skos:prefLabel>
    <skos:scopeNote xml:lang="en">Metal element with symbol Mt and atomic number 109 &lt;http://periodic.lanl.gov/109.shtml&gt;</skos:scopeNote>
    <skos:altLabel xml:lang="en">Mt</skos:altLabel>
    <skos:broader rdf:resource="http://www.usgs.gov/science/USGSThesaurus/chemical%20elements"/>
    <skos:related rdf:resource="http://www.usgs.gov/science/USGSThesaurus/metal%20elements"/>
    <skos:inScheme rdf:resource="http://www.usgs.gov/science/USGSThesaurus"/>
  </rdf:Description>
  <rdf:Description about="http://www.usgs.gov/science/USGSThesaurus/mendelevium">
    <rdf:type rdf:resource="http://www.w3.org/2004/02/skos/core#Concept"/>
    <skos:prefLabel xml:lang="en">mendelevium</skos:prefLabel>
    <skos:scopeNote xml:lang="en">Rare earth (actinide series) element with symbol Md and atomic number 101 &lt;http://periodic.lanl.gov/101.shtml&gt;</skos:scopeNote>
    <skos:altLabel xml:lang="en">Md</skos:altLabel>
    <skos:broader rdf:resource="http://www.usgs.gov/science/USGSThesaurus/chemical%20elements"/>
    <skos:related rdf:resource="http://www.usgs.gov/science/USGSThesaurus/actinide%20series%20elements"/>
    <skos:inScheme rdf:resource="http://www.usgs.gov/science/USGSThesaurus"/>
  </rdf:Description>
  <rdf:Description about="http://www.usgs.gov/science/USGSThesaurus/mercury">
    <rdf:type rdf:resource="http://www.w3.org/2004/02/skos/core#Concept"/>
    <skos:prefLabel xml:lang="en">mercury</skos:prefLabel>
    <skos:scopeNote xml:lang="en">Metal element with symbol Hg and atomic number 80 &lt;http://periodic.lanl.gov/80.shtml&gt;</skos:scopeNote>
    <skos:altLabel xml:lang="en">Hg</skos:altLabel>
    <skos:broader rdf:resource="http://www.usgs.gov/science/USGSThesaurus/chemical%20elements"/>
    <skos:related rdf:resource="http://www.usgs.gov/science/USGSThesaurus/metal%20elements"/>
    <skos:inScheme rdf:resource="http://www.usgs.gov/science/USGSThesaurus"/>
  </rdf:Description>
  <rdf:Description about="http://www.usgs.gov/science/USGSThesaurus/molybdenum">
    <rdf:type rdf:resource="http://www.w3.org/2004/02/skos/core#Concept"/>
    <skos:prefLabel xml:lang="en">molybdenum</skos:prefLabel>
    <skos:scopeNote xml:lang="en">Metal element with symbol Mo and atomic number 42 &lt;http://periodic.lanl.gov/42.shtml&gt;</skos:scopeNote>
    <skos:altLabel xml:lang="en">Mo</skos:altLabel>
    <skos:broader rdf:resource="http://www.usgs.gov/science/USGSThesaurus/chemical%20elements"/>
    <skos:related rdf:resource="http://www.usgs.gov/science/USGSThesaurus/metal%20elements"/>
    <skos:inScheme rdf:resource="http://www.usgs.gov/science/USGSThesaurus"/>
  </rdf:Description>
  <rdf:Description about="http://www.usgs.gov/science/USGSThesaurus/neodymium">
    <rdf:type rdf:resource="http://www.w3.org/2004/02/skos/core#Concept"/>
    <skos:prefLabel xml:lang="en">neodymium</skos:prefLabel>
    <skos:scopeNote xml:lang="en">Rare earth (lanthanide series) element with symbol Nd and atomic number 60 &lt;http://periodic.lanl.gov/60.shtml&gt;</skos:scopeNote>
    <skos:altLabel xml:lang="en">Nd</skos:altLabel>
    <skos:broader rdf:resource="http://www.usgs.gov/science/USGSThesaurus/chemical%20elements"/>
    <skos:related rdf:resource="http://www.usgs.gov/science/USGSThesaurus/lanthanide%20series%20elements"/>
    <skos:inScheme rdf:resource="http://www.usgs.gov/science/USGSThesaurus"/>
  </rdf:Description>
  <rdf:Description about="http://www.usgs.gov/science/USGSThesaurus/neon">
    <rdf:type rdf:resource="http://www.w3.org/2004/02/skos/core#Concept"/>
    <skos:prefLabel xml:lang="en">neon</skos:prefLabel>
    <skos:scopeNote xml:lang="en">Noble gas element with symbol Ne and atomic number 10 &lt;http://periodic.lanl.gov/10.shtml&gt;</skos:scopeNote>
    <skos:altLabel xml:lang="en">Ne</skos:altLabel>
    <skos:broader rdf:resource="http://www.usgs.gov/science/USGSThesaurus/chemical%20elements"/>
    <skos:related rdf:resource="http://www.usgs.gov/science/USGSThesaurus/noble%20gas%20elements"/>
    <skos:inScheme rdf:resource="http://www.usgs.gov/science/USGSThesaurus"/>
  </rdf:Description>
  <rdf:Description about="http://www.usgs.gov/science/USGSThesaurus/neptunium">
    <rdf:type rdf:resource="http://www.w3.org/2004/02/skos/core#Concept"/>
    <skos:prefLabel xml:lang="en">neptunium</skos:prefLabel>
    <skos:scopeNote xml:lang="en">Rare earth (actinide series) element with symbol Np and atomic number 93 &lt;http://periodic.lanl.gov/93.shtml&gt;</skos:scopeNote>
    <skos:altLabel xml:lang="en">Np</skos:altLabel>
    <skos:broader rdf:resource="http://www.usgs.gov/science/USGSThesaurus/chemical%20elements"/>
    <skos:related rdf:resource="http://www.usgs.gov/science/USGSThesaurus/actinide%20series%20elements"/>
    <skos:inScheme rdf:resource="http://www.usgs.gov/science/USGSThesaurus"/>
  </rdf:Description>
  <rdf:Description about="http://www.usgs.gov/science/USGSThesaurus/nickel">
    <rdf:type rdf:resource="http://www.w3.org/2004/02/skos/core#Concept"/>
    <skos:prefLabel xml:lang="en">nickel</skos:prefLabel>
    <skos:scopeNote xml:lang="en">Metal element with symbol Ni and atomic number 28 &lt;http://periodic.lanl.gov/28.shtml&gt;</skos:scopeNote>
    <skos:altLabel xml:lang="en">Ni</skos:altLabel>
    <skos:broader rdf:resource="http://www.usgs.gov/science/USGSThesaurus/chemical%20elements"/>
    <skos:related rdf:resource="http://www.usgs.gov/science/USGSThesaurus/metal%20elements"/>
    <skos:inScheme rdf:resource="http://www.usgs.gov/science/USGSThesaurus"/>
  </rdf:Description>
  <rdf:Description about="http://www.usgs.gov/science/USGSThesaurus/niobium">
    <rdf:type rdf:resource="http://www.w3.org/2004/02/skos/core#Concept"/>
    <skos:prefLabel xml:lang="en">niobium</skos:prefLabel>
    <skos:scopeNote xml:lang="en">Metal element with symbol Nb and atomic number 41 &lt;http://periodic.lanl.gov/41.shtml&gt;</skos:scopeNote>
    <skos:altLabel xml:lang="en">Nb</skos:altLabel>
    <skos:altLabel xml:lang="en">columbium</skos:altLabel>
    <skos:broader rdf:resource="http://www.usgs.gov/science/USGSThesaurus/chemical%20elements"/>
    <skos:related rdf:resource="http://www.usgs.gov/science/USGSThesaurus/metal%20elements"/>
    <skos:inScheme rdf:resource="http://www.usgs.gov/science/USGSThesaurus"/>
  </rdf:Description>
  <rdf:Description about="http://www.usgs.gov/science/USGSThesaurus/nitrogen">
    <rdf:type rdf:resource="http://www.w3.org/2004/02/skos/core#Concept"/>
    <skos:prefLabel xml:lang="en">nitrogen</skos:prefLabel>
    <skos:scopeNote xml:lang="en">Nonmetal element with symbol N and atomic number 7 &lt;http://periodic.lanl.gov/7.shtml&gt;</skos:scopeNote>
    <skos:altLabel xml:lang="en">N</skos:altLabel>
    <skos:broader rdf:resource="http://www.usgs.gov/science/USGSThesaurus/chemical%20elements"/>
    <skos:related rdf:resource="http://www.usgs.gov/science/USGSThesaurus/nonmetal%20elements"/>
    <skos:inScheme rdf:resource="http://www.usgs.gov/science/USGSThesaurus"/>
  </rdf:Description>
  <rdf:Description about="http://www.usgs.gov/science/USGSThesaurus/nobelium">
    <rdf:type rdf:resource="http://www.w3.org/2004/02/skos/core#Concept"/>
    <skos:prefLabel xml:lang="en">nobelium</skos:prefLabel>
    <skos:scopeNote xml:lang="en">Rare earth (actinide series) element with symbol No and atomic number 102 &lt;http://periodic.lanl.gov/102.shtml&gt;</skos:scopeNote>
    <skos:altLabel xml:lang="en">No</skos:altLabel>
    <skos:broader rdf:resource="http://www.usgs.gov/science/USGSThesaurus/chemical%20elements"/>
    <skos:related rdf:resource="http://www.usgs.gov/science/USGSThesaurus/actinide%20series%20elements"/>
    <skos:inScheme rdf:resource="http://www.usgs.gov/science/USGSThesaurus"/>
  </rdf:Description>
  <rdf:Description about="http://www.usgs.gov/science/USGSThesaurus/osmium">
    <rdf:type rdf:resource="http://www.w3.org/2004/02/skos/core#Concept"/>
    <skos:prefLabel xml:lang="en">osmium</skos:prefLabel>
    <skos:scopeNote xml:lang="en">Metal element with symbol Os and atomic number 76 &lt;http://periodic.lanl.gov/76.shtml&gt;</skos:scopeNote>
    <skos:altLabel xml:lang="en">Os</skos:altLabel>
    <skos:broader rdf:resource="http://www.usgs.gov/science/USGSThesaurus/chemical%20elements"/>
    <skos:related rdf:resource="http://www.usgs.gov/science/USGSThesaurus/metal%20elements"/>
    <skos:inScheme rdf:resource="http://www.usgs.gov/science/USGSThesaurus"/>
  </rdf:Description>
  <rdf:Description about="http://www.usgs.gov/science/USGSThesaurus/oxygen">
    <rdf:type rdf:resource="http://www.w3.org/2004/02/skos/core#Concept"/>
    <skos:prefLabel xml:lang="en">oxygen</skos:prefLabel>
    <skos:scopeNote xml:lang="en">Nonmetal element with symbol O and atomic number 8 &lt;http://periodic.lanl.gov/8.shtml&gt;</skos:scopeNote>
    <skos:altLabel xml:lang="en">O</skos:altLabel>
    <skos:broader rdf:resource="http://www.usgs.gov/science/USGSThesaurus/chemical%20elements"/>
    <skos:related rdf:resource="http://www.usgs.gov/science/USGSThesaurus/nonmetal%20elements"/>
    <skos:inScheme rdf:resource="http://www.usgs.gov/science/USGSThesaurus"/>
  </rdf:Description>
  <rdf:Description about="http://www.usgs.gov/science/USGSThesaurus/palladium">
    <rdf:type rdf:resource="http://www.w3.org/2004/02/skos/core#Concept"/>
    <skos:prefLabel xml:lang="en">palladium</skos:prefLabel>
    <skos:scopeNote xml:lang="en">Metal element with symbol Pd and atomic number 46 &lt;http://periodic.lanl.gov/46.shtml&gt;</skos:scopeNote>
    <skos:altLabel xml:lang="en">Pd</skos:altLabel>
    <skos:broader rdf:resource="http://www.usgs.gov/science/USGSThesaurus/chemical%20elements"/>
    <skos:related rdf:resource="http://www.usgs.gov/science/USGSThesaurus/metal%20elements"/>
    <skos:inScheme rdf:resource="http://www.usgs.gov/science/USGSThesaurus"/>
  </rdf:Description>
  <rdf:Description about="http://www.usgs.gov/science/USGSThesaurus/phosphorus">
    <rdf:type rdf:resource="http://www.w3.org/2004/02/skos/core#Concept"/>
    <skos:prefLabel xml:lang="en">phosphorus</skos:prefLabel>
    <skos:scopeNote xml:lang="en">Nonmetal element with symbol P and atomic number 15 &lt;http://periodic.lanl.gov/15.shtml&gt;</skos:scopeNote>
    <skos:altLabel xml:lang="en">P</skos:altLabel>
    <skos:broader rdf:resource="http://www.usgs.gov/science/USGSThesaurus/chemical%20elements"/>
    <skos:related rdf:resource="http://www.usgs.gov/science/USGSThesaurus/nonmetal%20elements"/>
    <skos:inScheme rdf:resource="http://www.usgs.gov/science/USGSThesaurus"/>
  </rdf:Description>
  <rdf:Description about="http://www.usgs.gov/science/USGSThesaurus/platinum">
    <rdf:type rdf:resource="http://www.w3.org/2004/02/skos/core#Concept"/>
    <skos:prefLabel xml:lang="en">platinum</skos:prefLabel>
    <skos:scopeNote xml:lang="en">Metal element with symbol Pt and atomic number 78 &lt;http://periodic.lanl.gov/78.shtml&gt;</skos:scopeNote>
    <skos:altLabel xml:lang="en">Pt</skos:altLabel>
    <skos:broader rdf:resource="http://www.usgs.gov/science/USGSThesaurus/chemical%20elements"/>
    <skos:related rdf:resource="http://www.usgs.gov/science/USGSThesaurus/metal%20elements"/>
    <skos:inScheme rdf:resource="http://www.usgs.gov/science/USGSThesaurus"/>
  </rdf:Description>
  <rdf:Description about="http://www.usgs.gov/science/USGSThesaurus/plutonium">
    <rdf:type rdf:resource="http://www.w3.org/2004/02/skos/core#Concept"/>
    <skos:prefLabel xml:lang="en">plutonium</skos:prefLabel>
    <skos:scopeNote xml:lang="en">Rare earth (actinide series) element with symbol Pu and atomic number 94 &lt;http://periodic.lanl.gov/94.shtml&gt;</skos:scopeNote>
    <skos:altLabel xml:lang="en">Pu</skos:altLabel>
    <skos:broader rdf:resource="http://www.usgs.gov/science/USGSThesaurus/chemical%20elements"/>
    <skos:related rdf:resource="http://www.usgs.gov/science/USGSThesaurus/actinide%20series%20elements"/>
    <skos:inScheme rdf:resource="http://www.usgs.gov/science/USGSThesaurus"/>
  </rdf:Description>
  <rdf:Description about="http://www.usgs.gov/science/USGSThesaurus/polonium">
    <rdf:type rdf:resource="http://www.w3.org/2004/02/skos/core#Concept"/>
    <skos:prefLabel xml:lang="en">polonium</skos:prefLabel>
    <skos:scopeNote xml:lang="en">Metalloid element with symbol Po and atomic number 84 &lt;http://periodic.lanl.gov/84.shtml&gt;</skos:scopeNote>
    <skos:altLabel xml:lang="en">Po</skos:altLabel>
    <skos:broader rdf:resource="http://www.usgs.gov/science/USGSThesaurus/chemical%20elements"/>
    <skos:related rdf:resource="http://www.usgs.gov/science/USGSThesaurus/metal%20elements"/>
    <skos:inScheme rdf:resource="http://www.usgs.gov/science/USGSThesaurus"/>
  </rdf:Description>
  <rdf:Description about="http://www.usgs.gov/science/USGSThesaurus/potassium">
    <rdf:type rdf:resource="http://www.w3.org/2004/02/skos/core#Concept"/>
    <skos:prefLabel xml:lang="en">potassium</skos:prefLabel>
    <skos:scopeNote xml:lang="en">Alkali metal element with symbol K and atomic number 19 &lt;http://periodic.lanl.gov/19.shtml&gt;</skos:scopeNote>
    <skos:altLabel xml:lang="en">K</skos:altLabel>
    <skos:broader rdf:resource="http://www.usgs.gov/science/USGSThesaurus/chemical%20elements"/>
    <skos:related rdf:resource="http://www.usgs.gov/science/USGSThesaurus/alkali%20metal%20elements"/>
    <skos:inScheme rdf:resource="http://www.usgs.gov/science/USGSThesaurus"/>
  </rdf:Description>
  <rdf:Description about="http://www.usgs.gov/science/USGSThesaurus/praseodymium">
    <rdf:type rdf:resource="http://www.w3.org/2004/02/skos/core#Concept"/>
    <skos:prefLabel xml:lang="en">praseodymium</skos:prefLabel>
    <skos:scopeNote xml:lang="en">Rare earth (lanthanide series) element with symbol Pr and atomic number 59 &lt;http://periodic.lanl.gov/59.shtml&gt;</skos:scopeNote>
    <skos:altLabel xml:lang="en">Pr</skos:altLabel>
    <skos:broader rdf:resource="http://www.usgs.gov/science/USGSThesaurus/chemical%20elements"/>
    <skos:related rdf:resource="http://www.usgs.gov/science/USGSThesaurus/lanthanide%20series%20elements"/>
    <skos:inScheme rdf:resource="http://www.usgs.gov/science/USGSThesaurus"/>
  </rdf:Description>
  <rdf:Description about="http://www.usgs.gov/science/USGSThesaurus/promethium">
    <rdf:type rdf:resource="http://www.w3.org/2004/02/skos/core#Concept"/>
    <skos:prefLabel xml:lang="en">promethium</skos:prefLabel>
    <skos:scopeNote xml:lang="en">Rare earth (lanthanide series) element with symbol Pm and atomic number 61 &lt;http://periodic.lanl.gov/61.shtml&gt;</skos:scopeNote>
    <skos:altLabel xml:lang="en">Pm</skos:altLabel>
    <skos:broader rdf:resource="http://www.usgs.gov/science/USGSThesaurus/chemical%20elements"/>
    <skos:related rdf:resource="http://www.usgs.gov/science/USGSThesaurus/lanthanide%20series%20elements"/>
    <skos:inScheme rdf:resource="http://www.usgs.gov/science/USGSThesaurus"/>
  </rdf:Description>
  <rdf:Description about="http://www.usgs.gov/science/USGSThesaurus/protactinium">
    <rdf:type rdf:resource="http://www.w3.org/2004/02/skos/core#Concept"/>
    <skos:prefLabel xml:lang="en">protactinium</skos:prefLabel>
    <skos:scopeNote xml:lang="en">Rare earth (actinide series) element with symbol Pa and atomic number 91 &lt;http://periodic.lanl.gov/91.shtml&gt;</skos:scopeNote>
    <skos:altLabel xml:lang="en">Pa</skos:altLabel>
    <skos:broader rdf:resource="http://www.usgs.gov/science/USGSThesaurus/chemical%20elements"/>
    <skos:related rdf:resource="http://www.usgs.gov/science/USGSThesaurus/actinide%20series%20elements"/>
    <skos:inScheme rdf:resource="http://www.usgs.gov/science/USGSThesaurus"/>
  </rdf:Description>
  <rdf:Description about="http://www.usgs.gov/science/USGSThesaurus/radium">
    <rdf:type rdf:resource="http://www.w3.org/2004/02/skos/core#Concept"/>
    <skos:prefLabel xml:lang="en">radium</skos:prefLabel>
    <skos:scopeNote xml:lang="en">Alkaline earth element with symbol Ra and atomic number 88 &lt;http://periodic.lanl.gov/88.shtml&gt;</skos:scopeNote>
    <skos:altLabel xml:lang="en">Ra</skos:altLabel>
    <skos:broader rdf:resource="http://www.usgs.gov/science/USGSThesaurus/chemical%20elements"/>
    <skos:related rdf:resource="http://www.usgs.gov/science/USGSThesaurus/alkaline%20earth%20elements"/>
    <skos:inScheme rdf:resource="http://www.usgs.gov/science/USGSThesaurus"/>
  </rdf:Description>
  <rdf:Description about="http://www.usgs.gov/science/USGSThesaurus/radon">
    <rdf:type rdf:resource="http://www.w3.org/2004/02/skos/core#Concept"/>
    <skos:prefLabel xml:lang="en">radon</skos:prefLabel>
    <skos:scopeNote xml:lang="en">Noble gas element with symbol Rn and atomic number 86 &lt;http://periodic.lanl.gov/86.shtml&gt;</skos:scopeNote>
    <skos:altLabel xml:lang="en">Rn</skos:altLabel>
    <skos:broader rdf:resource="http://www.usgs.gov/science/USGSThesaurus/chemical%20elements"/>
    <skos:related rdf:resource="http://www.usgs.gov/science/USGSThesaurus/toxic%20radionuclide%20contamination"/>
    <skos:related rdf:resource="http://www.usgs.gov/science/USGSThesaurus/noble%20gas%20elements"/>
    <skos:inScheme rdf:resource="http://www.usgs.gov/science/USGSThesaurus"/>
  </rdf:Description>
  <rdf:Description about="http://www.usgs.gov/science/USGSThesaurus/rhenium">
    <rdf:type rdf:resource="http://www.w3.org/2004/02/skos/core#Concept"/>
    <skos:prefLabel xml:lang="en">rhenium</skos:prefLabel>
    <skos:scopeNote xml:lang="en">Metal element with symbol Re and atomic number 75 &lt;http://periodic.lanl.gov/75.shtml&gt;</skos:scopeNote>
    <skos:altLabel xml:lang="en">Re</skos:altLabel>
    <skos:broader rdf:resource="http://www.usgs.gov/science/USGSThesaurus/chemical%20elements"/>
    <skos:related rdf:resource="http://www.usgs.gov/science/USGSThesaurus/metal%20elements"/>
    <skos:inScheme rdf:resource="http://www.usgs.gov/science/USGSThesaurus"/>
  </rdf:Description>
  <rdf:Description about="http://www.usgs.gov/science/USGSThesaurus/rhodium">
    <rdf:type rdf:resource="http://www.w3.org/2004/02/skos/core#Concept"/>
    <skos:prefLabel xml:lang="en">rhodium</skos:prefLabel>
    <skos:scopeNote xml:lang="en">Metal element with symbol Rh and atomic number 45 &lt;http://periodic.lanl.gov/45.shtml&gt;</skos:scopeNote>
    <skos:altLabel xml:lang="en">Rh</skos:altLabel>
    <skos:broader rdf:resource="http://www.usgs.gov/science/USGSThesaurus/chemical%20elements"/>
    <skos:related rdf:resource="http://www.usgs.gov/science/USGSThesaurus/metal%20elements"/>
    <skos:inScheme rdf:resource="http://www.usgs.gov/science/USGSThesaurus"/>
  </rdf:Description>
  <rdf:Description about="http://www.usgs.gov/science/USGSThesaurus/rubidium">
    <rdf:type rdf:resource="http://www.w3.org/2004/02/skos/core#Concept"/>
    <skos:prefLabel xml:lang="en">rubidium</skos:prefLabel>
    <skos:scopeNote xml:lang="en">Alkali metal element with symbol Rb and atomic number 37 &lt;http://periodic.lanl.gov/37.shtml&gt;</skos:scopeNote>
    <skos:altLabel xml:lang="en">Rb</skos:altLabel>
    <skos:broader rdf:resource="http://www.usgs.gov/science/USGSThesaurus/chemical%20elements"/>
    <skos:related rdf:resource="http://www.usgs.gov/science/USGSThesaurus/alkali%20metal%20elements"/>
    <skos:inScheme rdf:resource="http://www.usgs.gov/science/USGSThesaurus"/>
  </rdf:Description>
  <rdf:Description about="http://www.usgs.gov/science/USGSThesaurus/ruthenium">
    <rdf:type rdf:resource="http://www.w3.org/2004/02/skos/core#Concept"/>
    <skos:prefLabel xml:lang="en">ruthenium</skos:prefLabel>
    <skos:scopeNote xml:lang="en">Metal element with symbol Ru and atomic number 44 &lt;http://periodic.lanl.gov/44.shtml&gt;</skos:scopeNote>
    <skos:altLabel xml:lang="en">Ru</skos:altLabel>
    <skos:broader rdf:resource="http://www.usgs.gov/science/USGSThesaurus/chemical%20elements"/>
    <skos:related rdf:resource="http://www.usgs.gov/science/USGSThesaurus/metal%20elements"/>
    <skos:inScheme rdf:resource="http://www.usgs.gov/science/USGSThesaurus"/>
  </rdf:Description>
  <rdf:Description about="http://www.usgs.gov/science/USGSThesaurus/rutherfordium">
    <rdf:type rdf:resource="http://www.w3.org/2004/02/skos/core#Concept"/>
    <skos:prefLabel xml:lang="en">rutherfordium</skos:prefLabel>
    <skos:scopeNote xml:lang="en">Metal element with symbol Rf and atomic number 104 &lt;http://periodic.lanl.gov/104.shtml&gt;</skos:scopeNote>
    <skos:altLabel xml:lang="en">Rf</skos:altLabel>
    <skos:broader rdf:resource="http://www.usgs.gov/science/USGSThesaurus/chemical%20elements"/>
    <skos:related rdf:resource="http://www.usgs.gov/science/USGSThesaurus/metal%20elements"/>
    <skos:inScheme rdf:resource="http://www.usgs.gov/science/USGSThesaurus"/>
  </rdf:Description>
  <rdf:Description about="http://www.usgs.gov/science/USGSThesaurus/samarium">
    <rdf:type rdf:resource="http://www.w3.org/2004/02/skos/core#Concept"/>
    <skos:prefLabel xml:lang="en">samarium</skos:prefLabel>
    <skos:scopeNote xml:lang="en">Rare earth (lanthanide series) element with symbol Sm and atomic number 62 &lt;http://periodic.lanl.gov/62.shtml&gt;</skos:scopeNote>
    <skos:altLabel xml:lang="en">Sm</skos:altLabel>
    <skos:broader rdf:resource="http://www.usgs.gov/science/USGSThesaurus/chemical%20elements"/>
    <skos:related rdf:resource="http://www.usgs.gov/science/USGSThesaurus/lanthanide%20series%20elements"/>
    <skos:inScheme rdf:resource="http://www.usgs.gov/science/USGSThesaurus"/>
  </rdf:Description>
  <rdf:Description about="http://www.usgs.gov/science/USGSThesaurus/scandium">
    <rdf:type rdf:resource="http://www.w3.org/2004/02/skos/core#Concept"/>
    <skos:prefLabel xml:lang="en">scandium</skos:prefLabel>
    <skos:scopeNote xml:lang="en">Metal element with symbol Sc and atomic number 21 &lt;http://periodic.lanl.gov/21.shtml&gt;</skos:scopeNote>
    <skos:altLabel xml:lang="en">Sc</skos:altLabel>
    <skos:broader rdf:resource="http://www.usgs.gov/science/USGSThesaurus/chemical%20elements"/>
    <skos:related rdf:resource="http://www.usgs.gov/science/USGSThesaurus/rare%20earth%20elements"/>
    <skos:related rdf:resource="http://www.usgs.gov/science/USGSThesaurus/metal%20elements"/>
    <skos:inScheme rdf:resource="http://www.usgs.gov/science/USGSThesaurus"/>
  </rdf:Description>
  <rdf:Description about="http://www.usgs.gov/science/USGSThesaurus/seaborgium">
    <rdf:type rdf:resource="http://www.w3.org/2004/02/skos/core#Concept"/>
    <skos:prefLabel xml:lang="en">seaborgium</skos:prefLabel>
    <skos:scopeNote xml:lang="en">Metal element with symbol Sg and atomic number 106 &lt;http://periodic.lanl.gov/106.shtml&gt;</skos:scopeNote>
    <skos:altLabel xml:lang="en">Sg</skos:altLabel>
    <skos:broader rdf:resource="http://www.usgs.gov/science/USGSThesaurus/chemical%20elements"/>
    <skos:related rdf:resource="http://www.usgs.gov/science/USGSThesaurus/metal%20elements"/>
    <skos:inScheme rdf:resource="http://www.usgs.gov/science/USGSThesaurus"/>
  </rdf:Description>
  <rdf:Description about="http://www.usgs.gov/science/USGSThesaurus/selenium">
    <rdf:type rdf:resource="http://www.w3.org/2004/02/skos/core#Concept"/>
    <skos:prefLabel xml:lang="en">selenium</skos:prefLabel>
    <skos:scopeNote xml:lang="en">Nonmetal element with symbol Se and atomic number 34 &lt;http://periodic.lanl.gov/34.shtml&gt;</skos:scopeNote>
    <skos:altLabel xml:lang="en">Se</skos:altLabel>
    <skos:broader rdf:resource="http://www.usgs.gov/science/USGSThesaurus/chemical%20elements"/>
    <skos:related rdf:resource="http://www.usgs.gov/science/USGSThesaurus/nonmetal%20elements"/>
    <skos:inScheme rdf:resource="http://www.usgs.gov/science/USGSThesaurus"/>
  </rdf:Description>
  <rdf:Description about="http://www.usgs.gov/science/USGSThesaurus/silicon">
    <rdf:type rdf:resource="http://www.w3.org/2004/02/skos/core#Concept"/>
    <skos:prefLabel xml:lang="en">silicon</skos:prefLabel>
    <skos:scopeNote xml:lang="en">Nonmetal element with symbol si and atomic number 14 &lt;http://periodic.lanl.gov/14.shtml&gt;</skos:scopeNote>
    <skos:broader rdf:resource="http://www.usgs.gov/science/USGSThesaurus/chemical%20elements"/>
    <skos:related rdf:resource="http://www.usgs.gov/science/USGSThesaurus/nonmetal%20elements"/>
    <skos:inScheme rdf:resource="http://www.usgs.gov/science/USGSThesaurus"/>
  </rdf:Description>
  <rdf:Description about="http://www.usgs.gov/science/USGSThesaurus/silver">
    <rdf:type rdf:resource="http://www.w3.org/2004/02/skos/core#Concept"/>
    <skos:prefLabel xml:lang="en">silver</skos:prefLabel>
    <skos:scopeNote xml:lang="en">Metal element with symbol Ag and atomic number 47 &lt;http://periodic.lanl.gov/47.shtml&gt;</skos:scopeNote>
    <skos:altLabel xml:lang="en">Ag</skos:altLabel>
    <skos:broader rdf:resource="http://www.usgs.gov/science/USGSThesaurus/chemical%20elements"/>
    <skos:related rdf:resource="http://www.usgs.gov/science/USGSThesaurus/metal%20elements"/>
    <skos:inScheme rdf:resource="http://www.usgs.gov/science/USGSThesaurus"/>
  </rdf:Description>
  <rdf:Description about="http://www.usgs.gov/science/USGSThesaurus/sodium">
    <rdf:type rdf:resource="http://www.w3.org/2004/02/skos/core#Concept"/>
    <skos:prefLabel xml:lang="en">sodium</skos:prefLabel>
    <skos:scopeNote xml:lang="en">Alkali metal element with symbol Na and atomic number 11 &lt;http://periodic.lanl.gov/11.shtml&gt;</skos:scopeNote>
    <skos:altLabel xml:lang="en">Na</skos:altLabel>
    <skos:broader rdf:resource="http://www.usgs.gov/science/USGSThesaurus/chemical%20elements"/>
    <skos:related rdf:resource="http://www.usgs.gov/science/USGSThesaurus/alkali%20metal%20elements"/>
    <skos:inScheme rdf:resource="http://www.usgs.gov/science/USGSThesaurus"/>
  </rdf:Description>
  <rdf:Description about="http://www.usgs.gov/science/USGSThesaurus/strontium">
    <rdf:type rdf:resource="http://www.w3.org/2004/02/skos/core#Concept"/>
    <skos:prefLabel xml:lang="en">strontium</skos:prefLabel>
    <skos:scopeNote xml:lang="en">Alkaline earth element with symbol Sr and atomic number 38 &lt;http://periodic.lanl.gov/38.shtml&gt;</skos:scopeNote>
    <skos:altLabel xml:lang="en">Sr</skos:altLabel>
    <skos:broader rdf:resource="http://www.usgs.gov/science/USGSThesaurus/chemical%20elements"/>
    <skos:related rdf:resource="http://www.usgs.gov/science/USGSThesaurus/alkaline%20earth%20elements"/>
    <skos:inScheme rdf:resource="http://www.usgs.gov/science/USGSThesaurus"/>
  </rdf:Description>
  <rdf:Description about="http://www.usgs.gov/science/USGSThesaurus/sulfur">
    <rdf:type rdf:resource="http://www.w3.org/2004/02/skos/core#Concept"/>
    <skos:prefLabel xml:lang="en">sulfur</skos:prefLabel>
    <skos:scopeNote xml:lang="en">Nonmetal element with symbol S and atomic number 16 &lt;http://periodic.lanl.gov/16.shtml&gt;</skos:scopeNote>
    <skos:altLabel xml:lang="en">S</skos:altLabel>
    <skos:broader rdf:resource="http://www.usgs.gov/science/USGSThesaurus/chemical%20elements"/>
    <skos:related rdf:resource="http://www.usgs.gov/science/USGSThesaurus/nonmetal%20elements"/>
    <skos:inScheme rdf:resource="http://www.usgs.gov/science/USGSThesaurus"/>
  </rdf:Description>
  <rdf:Description about="http://www.usgs.gov/science/USGSThesaurus/tantalum">
    <rdf:type rdf:resource="http://www.w3.org/2004/02/skos/core#Concept"/>
    <skos:prefLabel xml:lang="en">tantalum</skos:prefLabel>
    <skos:scopeNote xml:lang="en">Metal element with symbol Ta and atomic number 73 &lt;http://periodic.lanl.gov/73.shtml&gt;</skos:scopeNote>
    <skos:altLabel xml:lang="en">Ta</skos:altLabel>
    <skos:broader rdf:resource="http://www.usgs.gov/science/USGSThesaurus/chemical%20elements"/>
    <skos:related rdf:resource="http://www.usgs.gov/science/USGSThesaurus/metal%20elements"/>
    <skos:inScheme rdf:resource="http://www.usgs.gov/science/USGSThesaurus"/>
  </rdf:Description>
  <rdf:Description about="http://www.usgs.gov/science/USGSThesaurus/technetium">
    <rdf:type rdf:resource="http://www.w3.org/2004/02/skos/core#Concept"/>
    <skos:prefLabel xml:lang="en">technetium</skos:prefLabel>
    <skos:scopeNote xml:lang="en">Metal element with symbol Tc and atomic number 43 &lt;http://periodic.lanl.gov/43.shtml&gt;</skos:scopeNote>
    <skos:altLabel xml:lang="en">Tc</skos:altLabel>
    <skos:broader rdf:resource="http://www.usgs.gov/science/USGSThesaurus/chemical%20elements"/>
    <skos:related rdf:resource="http://www.usgs.gov/science/USGSThesaurus/metal%20elements"/>
    <skos:inScheme rdf:resource="http://www.usgs.gov/science/USGSThesaurus"/>
  </rdf:Description>
  <rdf:Description about="http://www.usgs.gov/science/USGSThesaurus/tellurium">
    <rdf:type rdf:resource="http://www.w3.org/2004/02/skos/core#Concept"/>
    <skos:prefLabel xml:lang="en">tellurium</skos:prefLabel>
    <skos:scopeNote xml:lang="en">Nonmetal element with symbol Te and atomic number 52 &lt;http://periodic.lanl.gov/52.shtml&gt;</skos:scopeNote>
    <skos:altLabel xml:lang="en">Te</skos:altLabel>
    <skos:broader rdf:resource="http://www.usgs.gov/science/USGSThesaurus/chemical%20elements"/>
    <skos:related rdf:resource="http://www.usgs.gov/science/USGSThesaurus/nonmetal%20elements"/>
    <skos:inScheme rdf:resource="http://www.usgs.gov/science/USGSThesaurus"/>
  </rdf:Description>
  <rdf:Description about="http://www.usgs.gov/science/USGSThesaurus/terbium">
    <rdf:type rdf:resource="http://www.w3.org/2004/02/skos/core#Concept"/>
    <skos:prefLabel xml:lang="en">terbium</skos:prefLabel>
    <skos:scopeNote xml:lang="en">Rare earth (lanthanide series) element with symbol Tb and atomic number 65 &lt;http://periodic.lanl.gov/65.shtml&gt;</skos:scopeNote>
    <skos:altLabel xml:lang="en">Tb</skos:altLabel>
    <skos:broader rdf:resource="http://www.usgs.gov/science/USGSThesaurus/chemical%20elements"/>
    <skos:related rdf:resource="http://www.usgs.gov/science/USGSThesaurus/lanthanide%20series%20elements"/>
    <skos:inScheme rdf:resource="http://www.usgs.gov/science/USGSThesaurus"/>
  </rdf:Description>
  <rdf:Description about="http://www.usgs.gov/science/USGSThesaurus/thallium">
    <rdf:type rdf:resource="http://www.w3.org/2004/02/skos/core#Concept"/>
    <skos:prefLabel xml:lang="en">thallium</skos:prefLabel>
    <skos:scopeNote xml:lang="en">Metalloid element with symbol Tl and atomic number 81 &lt;http://periodic.lanl.gov/81.shtml&gt;</skos:scopeNote>
    <skos:altLabel xml:lang="en">Tl</skos:altLabel>
    <skos:broader rdf:resource="http://www.usgs.gov/science/USGSThesaurus/chemical%20elements"/>
    <skos:related rdf:resource="http://www.usgs.gov/science/USGSThesaurus/metal%20elements"/>
    <skos:inScheme rdf:resource="http://www.usgs.gov/science/USGSThesaurus"/>
  </rdf:Description>
  <rdf:Description about="http://www.usgs.gov/science/USGSThesaurus/thorium">
    <rdf:type rdf:resource="http://www.w3.org/2004/02/skos/core#Concept"/>
    <skos:prefLabel xml:lang="en">thorium</skos:prefLabel>
    <skos:scopeNote xml:lang="en">Rare earth (actinide series) element with symbol Th and atomic number 90 &lt;http://periodic.lanl.gov/90.shtml&gt;</skos:scopeNote>
    <skos:altLabel xml:lang="en">Th</skos:altLabel>
    <skos:broader rdf:resource="http://www.usgs.gov/science/USGSThesaurus/chemical%20elements"/>
    <skos:related rdf:resource="http://www.usgs.gov/science/USGSThesaurus/actinide%20series%20elements"/>
    <skos:inScheme rdf:resource="http://www.usgs.gov/science/USGSThesaurus"/>
  </rdf:Description>
  <rdf:Description about="http://www.usgs.gov/science/USGSThesaurus/thulium">
    <rdf:type rdf:resource="http://www.w3.org/2004/02/skos/core#Concept"/>
    <skos:prefLabel xml:lang="en">thulium</skos:prefLabel>
    <skos:scopeNote xml:lang="en">Rare earth (lanthanide series) element with symbol Tm and atomic number 69 &lt;http://periodic.lanl.gov/69.shtml&gt;</skos:scopeNote>
    <skos:altLabel xml:lang="en">Tm</skos:altLabel>
    <skos:broader rdf:resource="http://www.usgs.gov/science/USGSThesaurus/chemical%20elements"/>
    <skos:related rdf:resource="http://www.usgs.gov/science/USGSThesaurus/lanthanide%20series%20elements"/>
    <skos:inScheme rdf:resource="http://www.usgs.gov/science/USGSThesaurus"/>
  </rdf:Description>
  <rdf:Description about="http://www.usgs.gov/science/USGSThesaurus/tin">
    <rdf:type rdf:resource="http://www.w3.org/2004/02/skos/core#Concept"/>
    <skos:prefLabel xml:lang="en">tin</skos:prefLabel>
    <skos:scopeNote xml:lang="en">Metalloid element with symbol Sn and atomic number 50 &lt;http://periodic.lanl.gov/50.shtml&gt;</skos:scopeNote>
    <skos:altLabel xml:lang="en">Sn</skos:altLabel>
    <skos:broader rdf:resource="http://www.usgs.gov/science/USGSThesaurus/chemical%20elements"/>
    <skos:related rdf:resource="http://www.usgs.gov/science/USGSThesaurus/metal%20elements"/>
    <skos:inScheme rdf:resource="http://www.usgs.gov/science/USGSThesaurus"/>
  </rdf:Description>
  <rdf:Description about="http://www.usgs.gov/science/USGSThesaurus/titanium">
    <rdf:type rdf:resource="http://www.w3.org/2004/02/skos/core#Concept"/>
    <skos:prefLabel xml:lang="en">titanium</skos:prefLabel>
    <skos:scopeNote xml:lang="en">Metal element with symbol Ti and atomic number 22 &lt;http://periodic.lanl.gov/22.shtml&gt;</skos:scopeNote>
    <skos:altLabel xml:lang="en">Ti</skos:altLabel>
    <skos:broader rdf:resource="http://www.usgs.gov/science/USGSThesaurus/chemical%20elements"/>
    <skos:related rdf:resource="http://www.usgs.gov/science/USGSThesaurus/metal%20elements"/>
    <skos:inScheme rdf:resource="http://www.usgs.gov/science/USGSThesaurus"/>
  </rdf:Description>
  <rdf:Description about="http://www.usgs.gov/science/USGSThesaurus/tungsten">
    <rdf:type rdf:resource="http://www.w3.org/2004/02/skos/core#Concept"/>
    <skos:prefLabel xml:lang="en">tungsten</skos:prefLabel>
    <skos:scopeNote xml:lang="en">Metal element with symbol W and atomic number 74 &lt;http://periodic.lanl.gov/74.shtml&gt;</skos:scopeNote>
    <skos:altLabel xml:lang="en">W</skos:altLabel>
    <skos:broader rdf:resource="http://www.usgs.gov/science/USGSThesaurus/chemical%20elements"/>
    <skos:related rdf:resource="http://www.usgs.gov/science/USGSThesaurus/metal%20elements"/>
    <skos:inScheme rdf:resource="http://www.usgs.gov/science/USGSThesaurus"/>
  </rdf:Description>
  <rdf:Description about="http://www.usgs.gov/science/USGSThesaurus/ununnilium">
    <rdf:type rdf:resource="http://www.w3.org/2004/02/skos/core#Concept"/>
    <skos:prefLabel xml:lang="en">ununnilium</skos:prefLabel>
    <skos:scopeNote xml:lang="en">Metal element with symbol Uuu and atomic number 111 &lt;http://periodic.lanl.gov/111.shtml&gt;</skos:scopeNote>
    <skos:altLabel xml:lang="en">Uuu</skos:altLabel>
    <skos:broader rdf:resource="http://www.usgs.gov/science/USGSThesaurus/chemical%20elements"/>
    <skos:related rdf:resource="http://www.usgs.gov/science/USGSThesaurus/metal%20elements"/>
    <skos:inScheme rdf:resource="http://www.usgs.gov/science/USGSThesaurus"/>
  </rdf:Description>
  <rdf:Description about="http://www.usgs.gov/science/USGSThesaurus/ununnubium">
    <rdf:type rdf:resource="http://www.w3.org/2004/02/skos/core#Concept"/>
    <skos:prefLabel xml:lang="en">ununnubium</skos:prefLabel>
    <skos:scopeNote xml:lang="en">Metal element with symbol Uub and atomic number 113 &lt;http://periodic.lanl.gov/113.shtml&gt;</skos:scopeNote>
    <skos:altLabel xml:lang="en">Uub</skos:altLabel>
    <skos:broader rdf:resource="http://www.usgs.gov/science/USGSThesaurus/chemical%20elements"/>
    <skos:related rdf:resource="http://www.usgs.gov/science/USGSThesaurus/metal%20elements"/>
    <skos:inScheme rdf:resource="http://www.usgs.gov/science/USGSThesaurus"/>
  </rdf:Description>
  <rdf:Description about="http://www.usgs.gov/science/USGSThesaurus/ununnunium">
    <rdf:type rdf:resource="http://www.w3.org/2004/02/skos/core#Concept"/>
    <skos:prefLabel xml:lang="en">ununnunium</skos:prefLabel>
    <skos:scopeNote xml:lang="en">Metal element with symbol Uun and atomic number 112 &lt;http://periodic.lanl.gov/112.shtml&gt;</skos:scopeNote>
    <skos:altLabel xml:lang="en">Uun</skos:altLabel>
    <skos:broader rdf:resource="http://www.usgs.gov/science/USGSThesaurus/chemical%20elements"/>
    <skos:related rdf:resource="http://www.usgs.gov/science/USGSThesaurus/metal%20elements"/>
    <skos:inScheme rdf:resource="http://www.usgs.gov/science/USGSThesaurus"/>
  </rdf:Description>
  <rdf:Description about="http://www.usgs.gov/science/USGSThesaurus/uranium">
    <rdf:type rdf:resource="http://www.w3.org/2004/02/skos/core#Concept"/>
    <skos:prefLabel xml:lang="en">uranium</skos:prefLabel>
    <skos:scopeNote xml:lang="en">Rare earth (actinide series) element with symbol U and atomic number 92 &lt;http://periodic.lanl.gov/92.shtml&gt;</skos:scopeNote>
    <skos:altLabel xml:lang="en">U</skos:altLabel>
    <skos:broader rdf:resource="http://www.usgs.gov/science/USGSThesaurus/chemical%20elements"/>
    <skos:related rdf:resource="http://www.usgs.gov/science/USGSThesaurus/actinide%20series%20elements"/>
    <skos:inScheme rdf:resource="http://www.usgs.gov/science/USGSThesaurus"/>
  </rdf:Description>
  <rdf:Description about="http://www.usgs.gov/science/USGSThesaurus/vanadium">
    <rdf:type rdf:resource="http://www.w3.org/2004/02/skos/core#Concept"/>
    <skos:prefLabel xml:lang="en">vanadium</skos:prefLabel>
    <skos:scopeNote xml:lang="en">Metal element with symbol V and atomic number 23 &lt;http://periodic.lanl.gov/23.shtml&gt;</skos:scopeNote>
    <skos:altLabel xml:lang="en">V</skos:altLabel>
    <skos:broader rdf:resource="http://www.usgs.gov/science/USGSThesaurus/chemical%20elements"/>
    <skos:related rdf:resource="http://www.usgs.gov/science/USGSThesaurus/metal%20elements"/>
    <skos:inScheme rdf:resource="http://www.usgs.gov/science/USGSThesaurus"/>
  </rdf:Description>
  <rdf:Description about="http://www.usgs.gov/science/USGSThesaurus/xenon">
    <rdf:type rdf:resource="http://www.w3.org/2004/02/skos/core#Concept"/>
    <skos:prefLabel xml:lang="en">xenon</skos:prefLabel>
    <skos:scopeNote xml:lang="en">Noble gas element with symbol Xe and atomic number 54 &lt;http://periodic.lanl.gov/54.shtml&gt;</skos:scopeNote>
    <skos:altLabel xml:lang="en">Xe</skos:altLabel>
    <skos:broader rdf:resource="http://www.usgs.gov/science/USGSThesaurus/chemical%20elements"/>
    <skos:related rdf:resource="http://www.usgs.gov/science/USGSThesaurus/noble%20gas%20elements"/>
    <skos:inScheme rdf:resource="http://www.usgs.gov/science/USGSThesaurus"/>
  </rdf:Description>
  <rdf:Description about="http://www.usgs.gov/science/USGSThesaurus/ytterbium">
    <rdf:type rdf:resource="http://www.w3.org/2004/02/skos/core#Concept"/>
    <skos:prefLabel xml:lang="en">ytterbium</skos:prefLabel>
    <skos:scopeNote xml:lang="en">Rare earth (lanthanide series) element with symbol Yb and atomic number 70 &lt;http://periodic.lanl.gov/70.shtml&gt;</skos:scopeNote>
    <skos:altLabel xml:lang="en">Yb</skos:altLabel>
    <skos:broader rdf:resource="http://www.usgs.gov/science/USGSThesaurus/chemical%20elements"/>
    <skos:related rdf:resource="http://www.usgs.gov/science/USGSThesaurus/lanthanide%20series%20elements"/>
    <skos:inScheme rdf:resource="http://www.usgs.gov/science/USGSThesaurus"/>
  </rdf:Description>
  <rdf:Description about="http://www.usgs.gov/science/USGSThesaurus/yttrium">
    <rdf:type rdf:resource="http://www.w3.org/2004/02/skos/core#Concept"/>
    <skos:prefLabel xml:lang="en">yttrium</skos:prefLabel>
    <skos:scopeNote xml:lang="en">Metal element with symbol Y and atomic number 39 &lt;http://periodic.lanl.gov/39.shtml&gt;</skos:scopeNote>
    <skos:altLabel xml:lang="en">Y</skos:altLabel>
    <skos:broader rdf:resource="http://www.usgs.gov/science/USGSThesaurus/chemical%20elements"/>
    <skos:related rdf:resource="http://www.usgs.gov/science/USGSThesaurus/rare%20earth%20elements"/>
    <skos:related rdf:resource="http://www.usgs.gov/science/USGSThesaurus/metal%20elements"/>
    <skos:inScheme rdf:resource="http://www.usgs.gov/science/USGSThesaurus"/>
  </rdf:Description>
  <rdf:Description about="http://www.usgs.gov/science/USGSThesaurus/zinc">
    <rdf:type rdf:resource="http://www.w3.org/2004/02/skos/core#Concept"/>
    <skos:prefLabel xml:lang="en">zinc</skos:prefLabel>
    <skos:scopeNote xml:lang="en">Metal element with symbol Zn and atomic number 30 &lt;http://periodic.lanl.gov/30.shtml&gt;</skos:scopeNote>
    <skos:altLabel xml:lang="en">Zn</skos:altLabel>
    <skos:broader rdf:resource="http://www.usgs.gov/science/USGSThesaurus/chemical%20elements"/>
    <skos:related rdf:resource="http://www.usgs.gov/science/USGSThesaurus/metal%20elements"/>
    <skos:inScheme rdf:resource="http://www.usgs.gov/science/USGSThesaurus"/>
  </rdf:Description>
  <rdf:Description about="http://www.usgs.gov/science/USGSThesaurus/zirconium">
    <rdf:type rdf:resource="http://www.w3.org/2004/02/skos/core#Concept"/>
    <skos:prefLabel xml:lang="en">zirconium</skos:prefLabel>
    <skos:scopeNote xml:lang="en">Metal element with symbol Zr and atomic number 40 &lt;http://periodic.lanl.gov/40.shtml&gt;</skos:scopeNote>
    <skos:altLabel xml:lang="en">Zr</skos:altLabel>
    <skos:broader rdf:resource="http://www.usgs.gov/science/USGSThesaurus/chemical%20elements"/>
    <skos:related rdf:resource="http://www.usgs.gov/science/USGSThesaurus/metal%20elements"/>
    <skos:inScheme rdf:resource="http://www.usgs.gov/science/USGSThesaurus"/>
  </rdf:Description>
  <rdf:Description about="http://www.usgs.gov/science/USGSThesaurus/field%20monitoring%20stations">
    <rdf:type rdf:resource="http://www.w3.org/2004/02/skos/core#Concept"/>
    <skos:prefLabel xml:lang="en">field monitoring stations</skos:prefLabel>
    <skos:scopeNote xml:lang="en">Locations where USGS scientists or their collaborators make measurements of natural phenomena.</skos:scopeNote>
    <skos:altLabel xml:lang="en">benchmarks</skos:altLabel>
    <skos:altLabel xml:lang="en">field stations</skos:altLabel>
    <skos:altLabel xml:lang="en">seismic monitoring stations</skos:altLabel>
    <skos:altLabel xml:lang="en">stream gaging stations</skos:altLabel>
    <skos:broader rdf:resource="http://www.usgs.gov/science/USGSThesaurus/topics"/>
    <skos:related rdf:resource="http://www.usgs.gov/science/USGSThesaurus/field%20inventory%20and%20monitoring"/>
    <skos:inScheme rdf:resource="http://www.usgs.gov/science/USGSThesaurus"/>
  </rdf:Description>
  <rdf:Description about="http://www.usgs.gov/science/USGSThesaurus/hazards">
    <rdf:type rdf:resource="http://www.w3.org/2004/02/skos/core#Concept"/>
    <skos:prefLabel xml:lang="en">hazards</skos:prefLabel>
    <skos:scopeNote xml:lang="en">Potential dangers from both natural processes (e.g., earthquakes, floods, and climate change) and human impacts on the environment.</skos:scopeNote>
    <skos:altLabel xml:lang="en">catastrophes</skos:altLabel>
    <skos:altLabel xml:lang="en">disasters</skos:altLabel>
    <!--FOR earthquake hazards USE hazards WITH earthquakes-->
    <skos:altLabel xml:lang="en">earthquake hazards</skos:altLabel>
    <skos:altLabel xml:lang="en">emergency management resources</skos:altLabel>
    <skos:altLabel xml:lang="en">environmental hazards</skos:altLabel>
    <skos:altLabel xml:lang="en">geologic hazards</skos:altLabel>
    <!--FOR harmful algal blooms USE hazards WITH algal blooms-->
    <skos:altLabel xml:lang="en">harmful algal blooms</skos:altLabel>
    <!--FOR coastal hazards USE hazards WITH coastal processes-->
    <skos:altLabel xml:lang="en">coastal hazards</skos:altLabel>
    <!--FOR ocean hazards USE hazards WITH ocean processes-->
    <skos:altLabel xml:lang="en">ocean hazards</skos:altLabel>
    <skos:broader rdf:resource="http://www.usgs.gov/science/USGSThesaurus/topics"/>
    <skos:related rdf:resource="http://www.usgs.gov/science/USGSThesaurus/scour"/>
    <skos:related rdf:resource="http://www.usgs.gov/science/USGSThesaurus/algal%20blooms"/>
    <skos:related rdf:resource="http://www.usgs.gov/science/USGSThesaurus/desertification"/>
    <skos:related rdf:resource="http://www.usgs.gov/science/USGSThesaurus/droughts"/>
    <skos:related rdf:resource="http://www.usgs.gov/science/USGSThesaurus/earthquakes"/>
    <skos:related rdf:resource="http://www.usgs.gov/science/USGSThesaurus/ecotoxicology"/>
    <skos:related rdf:resource="http://www.usgs.gov/science/USGSThesaurus/fires"/>
    <skos:related rdf:resource="http://www.usgs.gov/science/USGSThesaurus/floods"/>
    <skos:related rdf:resource="http://www.usgs.gov/science/USGSThesaurus/human%20impacts"/>
    <skos:related rdf:resource="http://www.usgs.gov/science/USGSThesaurus/landslides"/>
    <skos:related rdf:resource="http://www.usgs.gov/science/USGSThesaurus/liquefaction"/>
    <skos:related rdf:resource="http://www.usgs.gov/science/USGSThesaurus/mining%20hazards"/>
    <skos:related rdf:resource="http://www.usgs.gov/science/USGSThesaurus/contamination%20and%20pollution"/>
    <skos:related rdf:resource="http://www.usgs.gov/science/USGSThesaurus/social%20sciences"/>
    <skos:related rdf:resource="http://www.usgs.gov/science/USGSThesaurus/storms"/>
    <skos:related rdf:resource="http://www.usgs.gov/science/USGSThesaurus/tsunamis"/>
    <skos:related rdf:resource="http://www.usgs.gov/science/USGSThesaurus/volcanic%20activity"/>
    <skos:related rdf:resource="http://www.usgs.gov/science/USGSThesaurus/impact%20cratering"/>
    <skos:related rdf:resource="http://www.usgs.gov/science/USGSThesaurus/magnetic%20storms"/>
    <skos:inScheme rdf:resource="http://www.usgs.gov/science/USGSThesaurus"/>
  </rdf:Description>
  <rdf:Description about="http://www.usgs.gov/science/USGSThesaurus/health%20and%20disease">
    <rdf:type rdf:resource="http://www.w3.org/2004/02/skos/core#Concept"/>
    <skos:prefLabel xml:lang="en">health and disease</skos:prefLabel>
    <skos:scopeNote xml:lang="en">Normal and abnormal conditions of plant and animal bodies.  Covers both human and non-human health and disease topics. For human health and disease, use the narrower term 'environmental health (human)'.</skos:scopeNote>
    <skos:altLabel xml:lang="en">disease</skos:altLabel>
    <skos:altLabel xml:lang="en">nutrition</skos:altLabel>
    <skos:broader rdf:resource="http://www.usgs.gov/science/USGSThesaurus/topics"/>
    <skos:narrower rdf:resource="http://www.usgs.gov/science/USGSThesaurus/disease%20vectors"/>
    <skos:narrower rdf:resource="http://www.usgs.gov/science/USGSThesaurus/environmental%20health%20%28human%29"/>
    <skos:narrower rdf:resource="http://www.usgs.gov/science/USGSThesaurus/wildlife%20disease"/>
    <skos:narrower rdf:resource="http://www.usgs.gov/science/USGSThesaurus/zoonotic%20diseases"/>
    <skos:related rdf:resource="http://www.usgs.gov/science/USGSThesaurus/bacteriology"/>
    <skos:related rdf:resource="http://www.usgs.gov/science/USGSThesaurus/endocrinology"/>
    <skos:related rdf:resource="http://www.usgs.gov/science/USGSThesaurus/histology"/>
    <skos:related rdf:resource="http://www.usgs.gov/science/USGSThesaurus/immunology"/>
    <skos:related rdf:resource="http://www.usgs.gov/science/USGSThesaurus/life%20sciences"/>
    <skos:related rdf:resource="http://www.usgs.gov/science/USGSThesaurus/parasitology"/>
    <skos:related rdf:resource="http://www.usgs.gov/science/USGSThesaurus/pathology"/>
    <skos:related rdf:resource="http://www.usgs.gov/science/USGSThesaurus/social%20sciences"/>
    <skos:inScheme rdf:resource="http://www.usgs.gov/science/USGSThesaurus"/>
  </rdf:Description>
  <rdf:Description about="http://www.usgs.gov/science/USGSThesaurus/disease%20vectors">
    <rdf:type rdf:resource="http://www.w3.org/2004/02/skos/core#Concept"/>
    <skos:prefLabel xml:lang="en">disease vectors</skos:prefLabel>
    <skos:scopeNote xml:lang="en">Organisms, such as insects, that transmit pathogens from one host to another.</skos:scopeNote>
    <skos:broader rdf:resource="http://www.usgs.gov/science/USGSThesaurus/health%20and%20disease"/>
    <skos:related rdf:resource="http://www.usgs.gov/science/USGSThesaurus/life%20sciences"/>
    <skos:inScheme rdf:resource="http://www.usgs.gov/science/USGSThesaurus"/>
  </rdf:Description>
  <rdf:Description about="http://www.usgs.gov/science/USGSThesaurus/environmental%20health%20%28human%29">
    <rdf:type rdf:resource="http://www.w3.org/2004/02/skos/core#Concept"/>
    <skos:prefLabel xml:lang="en">environmental health (human)</skos:prefLabel>
    <skos:scopeNote xml:lang="en">Effects of the environment on human health.</skos:scopeNote>
    <skos:altLabel xml:lang="en">disease (human)</skos:altLabel>
    <skos:altLabel xml:lang="en">health (human)</skos:altLabel>
    <skos:altLabel xml:lang="en">human disease</skos:altLabel>
    <skos:altLabel xml:lang="en">human health</skos:altLabel>
    <skos:broader rdf:resource="http://www.usgs.gov/science/USGSThesaurus/health%20and%20disease"/>
    <skos:narrower rdf:resource="http://www.usgs.gov/science/USGSThesaurus/human%20environmental%20safety"/>
    <skos:related rdf:resource="http://www.usgs.gov/science/USGSThesaurus/human%20impacts"/>
    <skos:related rdf:resource="http://www.usgs.gov/science/USGSThesaurus/social%20sciences"/>
    <skos:related rdf:resource="http://www.usgs.gov/science/USGSThesaurus/toxic%20radionuclide%20contamination"/>
    <skos:related rdf:resource="http://www.usgs.gov/science/USGSThesaurus/toxic%20trace%20element%20contamination"/>
    <skos:related rdf:resource="http://www.usgs.gov/science/USGSThesaurus/virology"/>
    <skos:inScheme rdf:resource="http://www.usgs.gov/science/USGSThesaurus"/>
  </rdf:Description>
  <rdf:Description about="http://www.usgs.gov/science/USGSThesaurus/human%20environmental%20safety">
    <rdf:type rdf:resource="http://www.w3.org/2004/02/skos/core#Concept"/>
    <skos:prefLabel xml:lang="en">human environmental safety</skos:prefLabel>
    <skos:scopeNote xml:lang="en">Monitoring and managing potentially harmful factors in the environment for human safety.</skos:scopeNote>
    <skos:altLabel xml:lang="en">safety issues (human)</skos:altLabel>
    <skos:broader rdf:resource="http://www.usgs.gov/science/USGSThesaurus/environmental%20health%20%28human%29"/>
    <skos:related rdf:resource="http://www.usgs.gov/science/USGSThesaurus/social%20sciences"/>
    <skos:inScheme rdf:resource="http://www.usgs.gov/science/USGSThesaurus"/>
  </rdf:Description>
  <rdf:Description about="http://www.usgs.gov/science/USGSThesaurus/wildlife%20disease">
    <rdf:type rdf:resource="http://www.w3.org/2004/02/skos/core#Concept"/>
    <skos:prefLabel xml:lang="en">wildlife disease</skos:prefLabel>
    <skos:scopeNote xml:lang="en">Includes viral, bacterial, and fungal infections as well as exposure of organisms to dangerous chemicals or toxic substances.</skos:scopeNote>
    <skos:broader rdf:resource="http://www.usgs.gov/science/USGSThesaurus/health%20and%20disease"/>
    <skos:narrower rdf:resource="http://www.usgs.gov/science/USGSThesaurus/avian%20influenza"/>
    <skos:narrower rdf:resource="http://www.usgs.gov/science/USGSThesaurus/chronic%20wasting%20disease"/>
    <skos:narrower rdf:resource="http://www.usgs.gov/science/USGSThesaurus/white-nose%20syndrome"/>
    <skos:related rdf:resource="http://www.usgs.gov/science/USGSThesaurus/anatomical%20deformities"/>
    <skos:inScheme rdf:resource="http://www.usgs.gov/science/USGSThesaurus"/>
  </rdf:Description>
  <rdf:Description about="http://www.usgs.gov/science/USGSThesaurus/avian%20influenza">
    <rdf:type rdf:resource="http://www.w3.org/2004/02/skos/core#Concept"/>
    <skos:prefLabel xml:lang="en">avian influenza</skos:prefLabel>
    <skos:scopeNote xml:lang="en">A virulent disease of poultry and wild birds that has spread throughout a large geographic area in Asia and Eastern Europe since it was first documented in 1997 in Asia.</skos:scopeNote>
    <skos:altLabel xml:lang="en">avian flu</skos:altLabel>
    <skos:altLabel xml:lang="en">bird flu</skos:altLabel>
    <skos:altLabel xml:lang="en">HPAI</skos:altLabel>
    <skos:altLabel xml:lang="en">H5N1</skos:altLabel>
    <skos:broader rdf:resource="http://www.usgs.gov/science/USGSThesaurus/wildlife%20disease"/>
    <skos:inScheme rdf:resource="http://www.usgs.gov/science/USGSThesaurus"/>
  </rdf:Description>
  <rdf:Description about="http://www.usgs.gov/science/USGSThesaurus/chronic%20wasting%20disease">
    <rdf:type rdf:resource="http://www.w3.org/2004/02/skos/core#Concept"/>
    <skos:prefLabel xml:lang="en">chronic wasting disease</skos:prefLabel>
    <skos:scopeNote xml:lang="en">Transmissible neurological disease of deer and elk that produces small lesions in the brains of infected animals; may be transmitted to humans who consume the meat of infected animals.</skos:scopeNote>
    <skos:altLabel xml:lang="en">CWD</skos:altLabel>
    <skos:broader rdf:resource="http://www.usgs.gov/science/USGSThesaurus/wildlife%20disease"/>
    <skos:inScheme rdf:resource="http://www.usgs.gov/science/USGSThesaurus"/>
  </rdf:Description>
  <rdf:Description about="http://www.usgs.gov/science/USGSThesaurus/white-nose%20syndrome">
    <rdf:type rdf:resource="http://www.w3.org/2004/02/skos/core#Concept"/>
    <skos:prefLabel xml:lang="en">white-nose syndrome</skos:prefLabel>
    <skos:scopeNote xml:lang="en">Disease affecting hibernating bats caused by a white fungus infecting the skin of the muzzle, ears, and wings</skos:scopeNote>
    <skos:altLabel xml:lang="en">WNS</skos:altLabel>
    <skos:broader rdf:resource="http://www.usgs.gov/science/USGSThesaurus/wildlife%20disease"/>
    <skos:inScheme rdf:resource="http://www.usgs.gov/science/USGSThesaurus"/>
  </rdf:Description>
  <rdf:Description about="http://www.usgs.gov/science/USGSThesaurus/zoonotic%20diseases">
    <rdf:type rdf:resource="http://www.w3.org/2004/02/skos/core#Concept"/>
    <skos:prefLabel xml:lang="en">zoonotic diseases</skos:prefLabel>
    <skos:scopeNote xml:lang="en">Diseases of animals that can be communicated to humans</skos:scopeNote>
    <skos:altLabel xml:lang="en">zoonosis</skos:altLabel>
    <skos:altLabel xml:lang="en">zoonoses</skos:altLabel>
    <skos:broader rdf:resource="http://www.usgs.gov/science/USGSThesaurus/health%20and%20disease"/>
    <skos:inScheme rdf:resource="http://www.usgs.gov/science/USGSThesaurus"/>
  </rdf:Description>
  <rdf:Description about="http://www.usgs.gov/science/USGSThesaurus/human%20impacts">
    <rdf:type rdf:resource="http://www.w3.org/2004/02/skos/core#Concept"/>
    <skos:prefLabel xml:lang="en">human impacts</skos:prefLabel>
    <skos:scopeNote xml:lang="en">The effects, intentional or unintentional, beneficial or harmful, direct or indirect, which human activities have upon the environment and living things.</skos:scopeNote>
    <skos:broader rdf:resource="http://www.usgs.gov/science/USGSThesaurus/topics"/>
    <skos:narrower rdf:resource="http://www.usgs.gov/science/USGSThesaurus/abandoned%20mines%20and%20quarries"/>
    <skos:narrower rdf:resource="http://www.usgs.gov/science/USGSThesaurus/deforestation"/>
    <skos:narrower rdf:resource="http://www.usgs.gov/science/USGSThesaurus/dredging"/>
    <skos:narrower rdf:resource="http://www.usgs.gov/science/USGSThesaurus/land%20use%20change"/>
    <skos:narrower rdf:resource="http://www.usgs.gov/science/USGSThesaurus/mining%20hazards"/>
    <skos:narrower rdf:resource="http://www.usgs.gov/science/USGSThesaurus/overfishing"/>
    <skos:narrower rdf:resource="http://www.usgs.gov/science/USGSThesaurus/overgrazing"/>
    <skos:narrower rdf:resource="http://www.usgs.gov/science/USGSThesaurus/waste%20treatment%20and%20disposal"/>
    <skos:related rdf:resource="http://www.usgs.gov/science/USGSThesaurus/acid%20deposition"/>
    <skos:related rdf:resource="http://www.usgs.gov/science/USGSThesaurus/ecology"/>
    <skos:related rdf:resource="http://www.usgs.gov/science/USGSThesaurus/ecotoxicology"/>
    <skos:related rdf:resource="http://www.usgs.gov/science/USGSThesaurus/environmental%20health%20%28human%29"/>
    <skos:related rdf:resource="http://www.usgs.gov/science/USGSThesaurus/fires"/>
    <skos:related rdf:resource="http://www.usgs.gov/science/USGSThesaurus/hazards"/>
    <skos:related rdf:resource="http://www.usgs.gov/science/USGSThesaurus/invasive%20species"/>
    <skos:related rdf:resource="http://www.usgs.gov/science/USGSThesaurus/subsidence"/>
    <skos:related rdf:resource="http://www.usgs.gov/science/USGSThesaurus/social%20sciences"/>
    <skos:related rdf:resource="http://www.usgs.gov/science/USGSThesaurus/contamination%20and%20pollution"/>
    <skos:inScheme rdf:resource="http://www.usgs.gov/science/USGSThesaurus"/>
  </rdf:Description>
  <rdf:Description about="http://www.usgs.gov/science/USGSThesaurus/abandoned%20mines%20and%20quarries">
    <rdf:type rdf:resource="http://www.w3.org/2004/02/skos/core#Concept"/>
    <skos:prefLabel xml:lang="en">abandoned mines and quarries</skos:prefLabel>
    <skos:scopeNote xml:lang="en">Mines and quarries that have been abandoned and may expose harmful chemicals to the environment.</skos:scopeNote>
    <skos:broader rdf:resource="http://www.usgs.gov/science/USGSThesaurus/human%20impacts"/>
    <skos:related rdf:resource="http://www.usgs.gov/science/USGSThesaurus/industrial%20pollution"/>
    <skos:inScheme rdf:resource="http://www.usgs.gov/science/USGSThesaurus"/>
  </rdf:Description>
  <rdf:Description about="http://www.usgs.gov/science/USGSThesaurus/deforestation">
    <rdf:type rdf:resource="http://www.w3.org/2004/02/skos/core#Concept"/>
    <skos:prefLabel xml:lang="en">deforestation</skos:prefLabel>
    <skos:scopeNote xml:lang="en">Reduction in the density of forest cover or tree canopy, typically by harvesting trees for human use or clearing land for other purposes such as agriculture.</skos:scopeNote>
    <skos:broader rdf:resource="http://www.usgs.gov/science/USGSThesaurus/human%20impacts"/>
    <skos:inScheme rdf:resource="http://www.usgs.gov/science/USGSThesaurus"/>
  </rdf:Description>
  <rdf:Description about="http://www.usgs.gov/science/USGSThesaurus/dredging">
    <rdf:type rdf:resource="http://www.w3.org/2004/02/skos/core#Concept"/>
    <skos:prefLabel xml:lang="en">dredging</skos:prefLabel>
    <skos:scopeNote xml:lang="en">Removal of sediments from water bodies to aid navigation or to transfer material to another location.</skos:scopeNote>
    <skos:broader rdf:resource="http://www.usgs.gov/science/USGSThesaurus/human%20impacts"/>
    <skos:related rdf:resource="http://www.usgs.gov/science/USGSThesaurus/hydraulic%20engineering"/>
    <skos:related rdf:resource="http://www.usgs.gov/science/USGSThesaurus/beach%20nourishment"/>
    <skos:inScheme rdf:resource="http://www.usgs.gov/science/USGSThesaurus"/>
  </rdf:Description>
  <rdf:Description about="http://www.usgs.gov/science/USGSThesaurus/land%20use%20change">
    <rdf:type rdf:resource="http://www.w3.org/2004/02/skos/core#Concept"/>
    <skos:prefLabel xml:lang="en">land use change</skos:prefLabel>
    <skos:scopeNote xml:lang="en">Effect of changing land use patterns on ecological systems.</skos:scopeNote>
    <skos:altLabel xml:lang="en">urbanization</skos:altLabel>
    <skos:broader rdf:resource="http://www.usgs.gov/science/USGSThesaurus/human%20impacts"/>
    <skos:narrower rdf:resource="http://www.usgs.gov/science/USGSThesaurus/habitat%20fragmentation"/>
    <skos:related rdf:resource="http://www.usgs.gov/science/USGSThesaurus/desertification"/>
    <skos:related rdf:resource="http://www.usgs.gov/science/USGSThesaurus/ecology"/>
    <skos:related rdf:resource="http://www.usgs.gov/science/USGSThesaurus/geography"/>
    <skos:related rdf:resource="http://www.usgs.gov/science/USGSThesaurus/social%20sciences"/>
    <skos:related rdf:resource="http://www.usgs.gov/science/USGSThesaurus/land%20use%20and%20land%20cover"/>
    <skos:inScheme rdf:resource="http://www.usgs.gov/science/USGSThesaurus"/>
  </rdf:Description>
  <rdf:Description about="http://www.usgs.gov/science/USGSThesaurus/habitat%20fragmentation">
    <rdf:type rdf:resource="http://www.w3.org/2004/02/skos/core#Concept"/>
    <skos:prefLabel xml:lang="en">habitat fragmentation</skos:prefLabel>
    <skos:scopeNote xml:lang="en">Disruption of once-continuous natural habitats by human activities such as agriculture, urbanization, resource extraction, and the construction of roads, railways, fences, and pipelines.</skos:scopeNote>
    <skos:broader rdf:resource="http://www.usgs.gov/science/USGSThesaurus/land%20use%20change"/>
    <skos:related rdf:resource="http://www.usgs.gov/science/USGSThesaurus/habitat%20alteration"/>
    <skos:inScheme rdf:resource="http://www.usgs.gov/science/USGSThesaurus"/>
  </rdf:Description>
  <rdf:Description about="http://www.usgs.gov/science/USGSThesaurus/mining%20hazards">
    <rdf:type rdf:resource="http://www.w3.org/2004/02/skos/core#Concept"/>
    <skos:prefLabel xml:lang="en">mining hazards</skos:prefLabel>
    <skos:scopeNote xml:lang="en">Dangerous conditions which result from the extraction of naturally occurring mineral deposits.  Includes tunnel collapses, fires, and explosions.</skos:scopeNote>
    <skos:broader rdf:resource="http://www.usgs.gov/science/USGSThesaurus/human%20impacts"/>
    <skos:related rdf:resource="http://www.usgs.gov/science/USGSThesaurus/engineering%20sciences"/>
    <skos:related rdf:resource="http://www.usgs.gov/science/USGSThesaurus/hazards"/>
    <skos:related rdf:resource="http://www.usgs.gov/science/USGSThesaurus/social%20sciences"/>
    <skos:related rdf:resource="http://www.usgs.gov/science/USGSThesaurus/waste%20treatment%20and%20disposal"/>
    <skos:related rdf:resource="http://www.usgs.gov/science/USGSThesaurus/mine%20drainage"/>
    <skos:inScheme rdf:resource="http://www.usgs.gov/science/USGSThesaurus"/>
  </rdf:Description>
  <rdf:Description about="http://www.usgs.gov/science/USGSThesaurus/overfishing">
    <rdf:type rdf:resource="http://www.w3.org/2004/02/skos/core#Concept"/>
    <skos:prefLabel xml:lang="en">overfishing</skos:prefLabel>
    <skos:scopeNote xml:lang="en">Taking too many fish from an area beyond the capacity for the population to replenish its numbers. The balance of the ecosystem is upset, leading to long-term depletion of fish stock.</skos:scopeNote>
    <skos:altLabel xml:lang="en">over-fishing</skos:altLabel>
    <skos:broader rdf:resource="http://www.usgs.gov/science/USGSThesaurus/human%20impacts"/>
    <skos:related rdf:resource="http://www.usgs.gov/science/USGSThesaurus/fishery%20resources"/>
    <skos:related rdf:resource="http://www.usgs.gov/science/USGSThesaurus/ichthyology"/>
    <skos:related rdf:resource="http://www.usgs.gov/science/USGSThesaurus/social%20sciences"/>
    <skos:related rdf:resource="http://www.usgs.gov/science/USGSThesaurus/wildlife%20biology"/>
    <skos:inScheme rdf:resource="http://www.usgs.gov/science/USGSThesaurus"/>
  </rdf:Description>
  <rdf:Description about="http://www.usgs.gov/science/USGSThesaurus/overgrazing">
    <rdf:type rdf:resource="http://www.w3.org/2004/02/skos/core#Concept"/>
    <skos:prefLabel xml:lang="en">overgrazing</skos:prefLabel>
    <skos:scopeNote xml:lang="en">The practice of allowing animals to eat vegetation, especially ground cover, beyond the capacity of the plant population to replenish itself. Leads to erosion and other harm to the ecosystem.</skos:scopeNote>
    <skos:altLabel xml:lang="en">over-grazing</skos:altLabel>
    <skos:broader rdf:resource="http://www.usgs.gov/science/USGSThesaurus/human%20impacts"/>
    <skos:inScheme rdf:resource="http://www.usgs.gov/science/USGSThesaurus"/>
  </rdf:Description>
  <rdf:Description about="http://www.usgs.gov/science/USGSThesaurus/waste%20treatment%20and%20disposal">
    <rdf:type rdf:resource="http://www.w3.org/2004/02/skos/core#Concept"/>
    <skos:prefLabel xml:lang="en">waste treatment and disposal</skos:prefLabel>
    <skos:scopeNote xml:lang="en">The chemical and physical methods to recycle or dispose of materials which, without treatment, are deemed to have no further value or are too contaminated to be used.</skos:scopeNote>
    <skos:altLabel xml:lang="en">nuclear waste repositories</skos:altLabel>
    <skos:altLabel xml:lang="en">radioactive waste repositories</skos:altLabel>
    <skos:altLabel xml:lang="en">sewage disposal</skos:altLabel>
    <skos:altLabel xml:lang="en">waste repositories</skos:altLabel>
    <skos:altLabel xml:lang="en">waste treatment</skos:altLabel>
    <skos:altLabel xml:lang="en">wastewater treatment</skos:altLabel>
    <skos:broader rdf:resource="http://www.usgs.gov/science/USGSThesaurus/human%20impacts"/>
    <skos:related rdf:resource="http://www.usgs.gov/science/USGSThesaurus/ecology"/>
    <skos:related rdf:resource="http://www.usgs.gov/science/USGSThesaurus/mining%20hazards"/>
    <skos:related rdf:resource="http://www.usgs.gov/science/USGSThesaurus/contamination%20and%20pollution"/>
    <skos:related rdf:resource="http://www.usgs.gov/science/USGSThesaurus/social%20sciences"/>
    <skos:related rdf:resource="http://www.usgs.gov/science/USGSThesaurus/wastewater%20discharge"/>
    <skos:inScheme rdf:resource="http://www.usgs.gov/science/USGSThesaurus"/>
  </rdf:Description>
  <rdf:Description about="http://www.usgs.gov/science/USGSThesaurus/information%20system%20design%20and%20development">
    <rdf:type rdf:resource="http://www.w3.org/2004/02/skos/core#Concept"/>
    <skos:prefLabel xml:lang="en">information system design and development</skos:prefLabel>
    <skos:scopeNote xml:lang="en">Use for the design and development of information systems.  Do not use for general cases in which information systems are part of the activity.</skos:scopeNote>
    <skos:broader rdf:resource="http://www.usgs.gov/science/USGSThesaurus/topics"/>
    <skos:narrower rdf:resource="http://www.usgs.gov/science/USGSThesaurus/geographic%20information%20systems"/>
    <skos:narrower rdf:resource="http://www.usgs.gov/science/USGSThesaurus/metadata%20development"/>
    <skos:related rdf:resource="http://www.usgs.gov/science/USGSThesaurus/information%20system%20administration"/>
    <skos:related rdf:resource="http://www.usgs.gov/science/USGSThesaurus/information%20sciences"/>
    <skos:inScheme rdf:resource="http://www.usgs.gov/science/USGSThesaurus"/>
  </rdf:Description>
  <rdf:Description about="http://www.usgs.gov/science/USGSThesaurus/geographic%20information%20systems">
    <rdf:type rdf:resource="http://www.w3.org/2004/02/skos/core#Concept"/>
    <skos:prefLabel xml:lang="en">geographic information systems</skos:prefLabel>
    <skos:scopeNote xml:lang="en">Computer software that allows geospatially referenced data to be linked to geographic features. Use this term only for information that is about GIS and not for the use of GIS in applications and projects.</skos:scopeNote>
    <skos:altLabel xml:lang="en">GIS</skos:altLabel>
    <skos:altLabel xml:lang="en">geographic information systems (GIS)</skos:altLabel>
    <skos:broader rdf:resource="http://www.usgs.gov/science/USGSThesaurus/information%20system%20design%20and%20development"/>
    <skos:related rdf:resource="http://www.usgs.gov/science/USGSThesaurus/decision%20support%20methods"/>
    <skos:related rdf:resource="http://www.usgs.gov/science/USGSThesaurus/geography"/>
    <skos:related rdf:resource="http://www.usgs.gov/science/USGSThesaurus/geolocation%20measurement"/>
    <skos:related rdf:resource="http://www.usgs.gov/science/USGSThesaurus/geospatial%20datasets"/>
    <skos:related rdf:resource="http://www.usgs.gov/science/USGSThesaurus/GPS%20measurement"/>
    <skos:related rdf:resource="http://www.usgs.gov/science/USGSThesaurus/information%20sciences"/>
    <skos:related rdf:resource="http://www.usgs.gov/science/USGSThesaurus/map%20coordinate%20systems"/>
    <skos:inScheme rdf:resource="http://www.usgs.gov/science/USGSThesaurus"/>
  </rdf:Description>
  <rdf:Description about="http://www.usgs.gov/science/USGSThesaurus/metadata%20development">
    <rdf:type rdf:resource="http://www.w3.org/2004/02/skos/core#Concept"/>
    <skos:prefLabel xml:lang="en">metadata development</skos:prefLabel>
    <skos:scopeNote xml:lang="en">Use for the development of metadata schemes and applications.  Do not use for general cases where metadata are part of the activities.</skos:scopeNote>
    <skos:broader rdf:resource="http://www.usgs.gov/science/USGSThesaurus/information%20system%20design%20and%20development"/>
    <skos:related rdf:resource="http://www.usgs.gov/science/USGSThesaurus/information%20sciences"/>
    <skos:inScheme rdf:resource="http://www.usgs.gov/science/USGSThesaurus"/>
  </rdf:Description>
  <rdf:Description about="http://www.usgs.gov/science/USGSThesaurus/instrument%20design%20and%20development">
    <rdf:type rdf:resource="http://www.w3.org/2004/02/skos/core#Concept"/>
    <skos:prefLabel xml:lang="en">instrument design and development</skos:prefLabel>
    <skos:scopeNote xml:lang="en">Includes the design and development of software for a particular instrument.</skos:scopeNote>
    <skos:altLabel xml:lang="en">tool development</skos:altLabel>
    <skos:broader rdf:resource="http://www.usgs.gov/science/USGSThesaurus/topics"/>
    <skos:related rdf:resource="http://www.usgs.gov/science/USGSThesaurus/engineering%20sciences"/>
    <skos:inScheme rdf:resource="http://www.usgs.gov/science/USGSThesaurus"/>
  </rdf:Description>
  <rdf:Description about="http://www.usgs.gov/science/USGSThesaurus/land%20use%20and%20land%20cover">
    <rdf:type rdf:resource="http://www.w3.org/2004/02/skos/core#Concept"/>
    <skos:prefLabel xml:lang="en">land use and land cover</skos:prefLabel>
    <skos:scopeNote xml:lang="en">The vegetation, water, natural surface, and cultural features on the land surface.</skos:scopeNote>
    <skos:broader rdf:resource="http://www.usgs.gov/science/USGSThesaurus/topics"/>
    <skos:related rdf:resource="http://www.usgs.gov/science/USGSThesaurus/land%20use%20change"/>
    <skos:inScheme rdf:resource="http://www.usgs.gov/science/USGSThesaurus"/>
  </rdf:Description>
  <rdf:Description about="http://www.usgs.gov/science/USGSThesaurus/map%20coordinate%20systems">
    <rdf:type rdf:resource="http://www.w3.org/2004/02/skos/core#Concept"/>
    <skos:prefLabel xml:lang="en">map coordinate systems</skos:prefLabel>
    <skos:scopeNote xml:lang="en">Systems using sets of numbers combined with geometric nets or grids to specific positions on a map or globe.</skos:scopeNote>
    <skos:altLabel xml:lang="en">coordinate systems</skos:altLabel>
    <skos:altLabel xml:lang="en">geographic coordinate systems</skos:altLabel>
    <skos:altLabel xml:lang="en">grid coordinate systems</skos:altLabel>
    <skos:altLabel xml:lang="en">horizontal datums</skos:altLabel>
    <skos:altLabel xml:lang="en">map projections</skos:altLabel>
    <skos:altLabel xml:lang="en">vertical datums</skos:altLabel>
    <skos:broader rdf:resource="http://www.usgs.gov/science/USGSThesaurus/topics"/>
    <skos:related rdf:resource="http://www.usgs.gov/science/USGSThesaurus/cartography"/>
    <skos:related rdf:resource="http://www.usgs.gov/science/USGSThesaurus/geographic%20information%20systems"/>
    <skos:related rdf:resource="http://www.usgs.gov/science/USGSThesaurus/geography"/>
    <skos:inScheme rdf:resource="http://www.usgs.gov/science/USGSThesaurus"/>
  </rdf:Description>
  <rdf:Description about="http://www.usgs.gov/science/USGSThesaurus/natural%20resource%20exploration">
    <rdf:type rdf:resource="http://www.w3.org/2004/02/skos/core#Concept"/>
    <skos:prefLabel xml:lang="en">natural resource exploration</skos:prefLabel>
    <skos:scopeNote xml:lang="en">Techniques for locating deposits or stocks of useful minerals, water, and other resources using reconnaissance or instrumental methods.</skos:scopeNote>
    <skos:altLabel xml:lang="en">dowsing</skos:altLabel>
    <!--FOR exploration seismology USE natural resource exploration WITH seismology-->
    <skos:altLabel xml:lang="en">exploration seismology</skos:altLabel>
    <skos:altLabel xml:lang="en">exploration</skos:altLabel>
    <skos:altLabel xml:lang="en">prospecting</skos:altLabel>
    <!--FOR seismic exploration USE natural resource exploration WITH seismic methods-->
    <skos:altLabel xml:lang="en">seismic exploration</skos:altLabel>
    <skos:broader rdf:resource="http://www.usgs.gov/science/USGSThesaurus/topics"/>
    <skos:inScheme rdf:resource="http://www.usgs.gov/science/USGSThesaurus"/>
  </rdf:Description>
  <rdf:Description about="http://www.usgs.gov/science/USGSThesaurus/natural%20resource%20extraction">
    <rdf:type rdf:resource="http://www.w3.org/2004/02/skos/core#Concept"/>
    <skos:prefLabel xml:lang="en">natural resource extraction</skos:prefLabel>
    <skos:scopeNote xml:lang="en">Removal of natural materials or properties (such as heat) for use.</skos:scopeNote>
    <skos:altLabel xml:lang="en">resource extraction</skos:altLabel>
    <skos:broader rdf:resource="http://www.usgs.gov/science/USGSThesaurus/topics"/>
    <skos:narrower rdf:resource="http://www.usgs.gov/science/USGSThesaurus/enhanced%20oil%20recovery"/>
    <skos:narrower rdf:resource="http://www.usgs.gov/science/USGSThesaurus/hydraulic%20fracturing"/>
    <skos:narrower rdf:resource="http://www.usgs.gov/science/USGSThesaurus/mining%20and%20quarrying"/>
    <skos:narrower rdf:resource="http://www.usgs.gov/science/USGSThesaurus/placer%20deposit%20mining"/>
    <skos:narrower rdf:resource="http://www.usgs.gov/science/USGSThesaurus/well%20drilling"/>
    <skos:related rdf:resource="http://www.usgs.gov/science/USGSThesaurus/beach%20nourishment"/>
    <skos:inScheme rdf:resource="http://www.usgs.gov/science/USGSThesaurus"/>
  </rdf:Description>
  <rdf:Description about="http://www.usgs.gov/science/USGSThesaurus/enhanced%20oil%20recovery">
    <rdf:type rdf:resource="http://www.w3.org/2004/02/skos/core#Concept"/>
    <skos:prefLabel xml:lang="en">enhanced oil recovery</skos:prefLabel>
    <skos:scopeNote xml:lang="en">Injection of steam, gas, or other chemical compounds into hydrocarbon reservoirs to stimulate the production of usable oil beyond what is possible through natural pressure, water injection, and pumping at the wellhead.</skos:scopeNote>
    <skos:altLabel xml:lang="en">EOR</skos:altLabel>
    <skos:altLabel xml:lang="en">tertiary oil recovery</skos:altLabel>
    <skos:broader rdf:resource="http://www.usgs.gov/science/USGSThesaurus/natural%20resource%20extraction"/>
    <skos:inScheme rdf:resource="http://www.usgs.gov/science/USGSThesaurus"/>
  </rdf:Description>
  <rdf:Description about="http://www.usgs.gov/science/USGSThesaurus/hydraulic%20fracturing">
    <rdf:type rdf:resource="http://www.w3.org/2004/02/skos/core#Concept"/>
    <skos:prefLabel xml:lang="en">hydraulic fracturing</skos:prefLabel>
    <skos:scopeNote xml:lang="en">Injection of water and other fluids through a well into geologic formations in order to increase the permeability of the rock units and thus permit natural gas or oil to be produced from them.</skos:scopeNote>
    <skos:altLabel xml:lang="en">hydrofracking</skos:altLabel>
    <skos:altLabel xml:lang="en">fracking</skos:altLabel>
    <skos:broader rdf:resource="http://www.usgs.gov/science/USGSThesaurus/natural%20resource%20extraction"/>
    <skos:inScheme rdf:resource="http://www.usgs.gov/science/USGSThesaurus"/>
  </rdf:Description>
  <rdf:Description about="http://www.usgs.gov/science/USGSThesaurus/mining%20and%20quarrying">
    <rdf:type rdf:resource="http://www.w3.org/2004/02/skos/core#Concept"/>
    <skos:prefLabel xml:lang="en">mining and quarrying</skos:prefLabel>
    <skos:scopeNote xml:lang="en">Extracting mineral deposits from a pit, tunnel, or excavation.</skos:scopeNote>
    <skos:altLabel xml:lang="en">quarrying</skos:altLabel>
    <skos:broader rdf:resource="http://www.usgs.gov/science/USGSThesaurus/natural%20resource%20extraction"/>
    <skos:inScheme rdf:resource="http://www.usgs.gov/science/USGSThesaurus"/>
  </rdf:Description>
  <rdf:Description about="http://www.usgs.gov/science/USGSThesaurus/placer%20deposit%20mining">
    <rdf:type rdf:resource="http://www.w3.org/2004/02/skos/core#Concept"/>
    <skos:prefLabel xml:lang="en">placer deposit mining</skos:prefLabel>
    <skos:scopeNote xml:lang="en">Extraction of minerals, typically metal ores, from unconsolidated surficial materials such as stream sediments.</skos:scopeNote>
    <skos:broader rdf:resource="http://www.usgs.gov/science/USGSThesaurus/natural%20resource%20extraction"/>
    <skos:inScheme rdf:resource="http://www.usgs.gov/science/USGSThesaurus"/>
  </rdf:Description>
  <rdf:Description about="http://www.usgs.gov/science/USGSThesaurus/well%20drilling">
    <rdf:type rdf:resource="http://www.w3.org/2004/02/skos/core#Concept"/>
    <skos:prefLabel xml:lang="en">well drilling</skos:prefLabel>
    <skos:scopeNote xml:lang="en">The process of artificial excavation for the purpose of withdrawing water, oil, or gas from underground.</skos:scopeNote>
    <skos:broader rdf:resource="http://www.usgs.gov/science/USGSThesaurus/natural%20resource%20extraction"/>
    <skos:related rdf:resource="http://www.usgs.gov/science/USGSThesaurus/drilling%20and%20coring"/>
    <skos:inScheme rdf:resource="http://www.usgs.gov/science/USGSThesaurus"/>
  </rdf:Description>
  <rdf:Description about="http://www.usgs.gov/science/USGSThesaurus/natural%20resources">
    <rdf:type rdf:resource="http://www.w3.org/2004/02/skos/core#Concept"/>
    <skos:prefLabel xml:lang="en">natural resources</skos:prefLabel>
    <skos:scopeNote xml:lang="en">Stocks of anything naturally occurring that have a beneficial use for man including economic, nutritional, recreational, aesthetic, and other benefits.</skos:scopeNote>
    <skos:broader rdf:resource="http://www.usgs.gov/science/USGSThesaurus/topics"/>
    <skos:narrower rdf:resource="http://www.usgs.gov/science/USGSThesaurus/energy%20resources"/>
    <skos:narrower rdf:resource="http://www.usgs.gov/science/USGSThesaurus/fishery%20resources"/>
    <skos:narrower rdf:resource="http://www.usgs.gov/science/USGSThesaurus/forest%20resources"/>
    <skos:narrower rdf:resource="http://www.usgs.gov/science/USGSThesaurus/mineral%20resources"/>
    <skos:narrower rdf:resource="http://www.usgs.gov/science/USGSThesaurus/soil%20resources"/>
    <skos:narrower rdf:resource="http://www.usgs.gov/science/USGSThesaurus/water%20resources"/>
    <skos:related rdf:resource="http://www.usgs.gov/science/USGSThesaurus/earth%20sciences"/>
    <skos:related rdf:resource="http://www.usgs.gov/science/USGSThesaurus/life%20sciences"/>
    <skos:related rdf:resource="http://www.usgs.gov/science/USGSThesaurus/natural%20resource%20management"/>
    <skos:inScheme rdf:resource="http://www.usgs.gov/science/USGSThesaurus"/>
  </rdf:Description>
  <rdf:Description about="http://www.usgs.gov/science/USGSThesaurus/energy%20resources">
    <rdf:type rdf:resource="http://www.w3.org/2004/02/skos/core#Concept"/>
    <skos:prefLabel xml:lang="en">energy resources</skos:prefLabel>
    <skos:scopeNote xml:lang="en">Natural resources that are used for heat and power generation, including oil, natural gas, coal, and geothermal energy.</skos:scopeNote>
    <skos:altLabel xml:lang="en">energy sources</skos:altLabel>
    <skos:altLabel xml:lang="en">fossil fuels</skos:altLabel>
    <skos:broader rdf:resource="http://www.usgs.gov/science/USGSThesaurus/natural%20resources"/>
    <skos:narrower rdf:resource="http://www.usgs.gov/science/USGSThesaurus/coal%20resources"/>
    <skos:narrower rdf:resource="http://www.usgs.gov/science/USGSThesaurus/geothermal%20resources"/>
    <skos:narrower rdf:resource="http://www.usgs.gov/science/USGSThesaurus/natural%20gas%20resources"/>
    <skos:narrower rdf:resource="http://www.usgs.gov/science/USGSThesaurus/oil%20resources"/>
    <skos:narrower rdf:resource="http://www.usgs.gov/science/USGSThesaurus/wind%20energy"/>
    <skos:related rdf:resource="http://www.usgs.gov/science/USGSThesaurus/economic%20geology"/>
    <skos:inScheme rdf:resource="http://www.usgs.gov/science/USGSThesaurus"/>
  </rdf:Description>
  <rdf:Description about="http://www.usgs.gov/science/USGSThesaurus/coal%20resources">
    <rdf:type rdf:resource="http://www.w3.org/2004/02/skos/core#Concept"/>
    <skos:prefLabel xml:lang="en">coal resources</skos:prefLabel>
    <skos:scopeNote xml:lang="en">Fuel resources such as anthracite, lignite, bituminous coal, or coke, consisting largely of carbonaceous material and formed from fossilized plants.</skos:scopeNote>
    <skos:altLabel xml:lang="en">anthracite resources</skos:altLabel>
    <skos:altLabel xml:lang="en">bituminous coal resources</skos:altLabel>
    <skos:altLabel xml:lang="en">lignite resources</skos:altLabel>
    <skos:altLabel xml:lang="en">subbituminous coal resources</skos:altLabel>
    <skos:broader rdf:resource="http://www.usgs.gov/science/USGSThesaurus/energy%20resources"/>
    <skos:related rdf:resource="http://www.usgs.gov/science/USGSThesaurus/coalbed%20methane%20resources"/>
    <skos:related rdf:resource="http://www.usgs.gov/science/USGSThesaurus/economic%20geology"/>
    <skos:related rdf:resource="http://www.usgs.gov/science/USGSThesaurus/mineral%20deposits"/>
    <skos:inScheme rdf:resource="http://www.usgs.gov/science/USGSThesaurus"/>
  </rdf:Description>
  <rdf:Description about="http://www.usgs.gov/science/USGSThesaurus/geothermal%20resources">
    <rdf:type rdf:resource="http://www.w3.org/2004/02/skos/core#Concept"/>
    <skos:prefLabel xml:lang="en">geothermal resources</skos:prefLabel>
    <skos:scopeNote xml:lang="en">Energy resources related to the earth's internal heat, commonly applied to springs or vents discharging hot water or steam.</skos:scopeNote>
    <skos:broader rdf:resource="http://www.usgs.gov/science/USGSThesaurus/energy%20resources"/>
    <skos:related rdf:resource="http://www.usgs.gov/science/USGSThesaurus/hydrogeology"/>
    <skos:related rdf:resource="http://www.usgs.gov/science/USGSThesaurus/volcanology"/>
    <skos:inScheme rdf:resource="http://www.usgs.gov/science/USGSThesaurus"/>
  </rdf:Description>
  <rdf:Description about="http://www.usgs.gov/science/USGSThesaurus/natural%20gas%20resources">
    <rdf:type rdf:resource="http://www.w3.org/2004/02/skos/core#Concept"/>
    <skos:prefLabel xml:lang="en">natural gas resources</skos:prefLabel>
    <skos:scopeNote xml:lang="en">Stocks of naturally formed hydrocarbon gases which are usually associated with petroleum fields.  Useful for heating, they are principally methane, but can be ethane, butane, or propane.</skos:scopeNote>
    <skos:altLabel xml:lang="en">petroleum resources (gas)</skos:altLabel>
    <skos:broader rdf:resource="http://www.usgs.gov/science/USGSThesaurus/energy%20resources"/>
    <skos:narrower rdf:resource="http://www.usgs.gov/science/USGSThesaurus/coalbed%20methane%20resources"/>
    <skos:narrower rdf:resource="http://www.usgs.gov/science/USGSThesaurus/gas%20hydrate%20resources"/>
    <skos:related rdf:resource="http://www.usgs.gov/science/USGSThesaurus/petroleum"/>
    <skos:related rdf:resource="http://www.usgs.gov/science/USGSThesaurus/economic%20geology"/>
    <skos:inScheme rdf:resource="http://www.usgs.gov/science/USGSThesaurus"/>
  </rdf:Description>
  <rdf:Description about="http://www.usgs.gov/science/USGSThesaurus/coalbed%20methane%20resources">
    <rdf:type rdf:resource="http://www.w3.org/2004/02/skos/core#Concept"/>
    <skos:prefLabel xml:lang="en">coalbed methane resources</skos:prefLabel>
    <skos:scopeNote xml:lang="en">Resources of methane-rich gas generated and stored in coalbeds.</skos:scopeNote>
    <skos:altLabel xml:lang="en">coal bed methane resources</skos:altLabel>
    <skos:altLabel xml:lang="en">methane resources (coalbed)</skos:altLabel>
    <skos:broader rdf:resource="http://www.usgs.gov/science/USGSThesaurus/natural%20gas%20resources"/>
    <skos:related rdf:resource="http://www.usgs.gov/science/USGSThesaurus/coal%20resources"/>
    <skos:related rdf:resource="http://www.usgs.gov/science/USGSThesaurus/economic%20geology"/>
    <skos:inScheme rdf:resource="http://www.usgs.gov/science/USGSThesaurus"/>
  </rdf:Description>
  <rdf:Description about="http://www.usgs.gov/science/USGSThesaurus/gas%20hydrate%20resources">
    <rdf:type rdf:resource="http://www.w3.org/2004/02/skos/core#Concept"/>
    <skos:prefLabel xml:lang="en">gas hydrate resources</skos:prefLabel>
    <skos:scopeNote xml:lang="en">Deposits of a crystalline solid in which water molecules trap gas molecules, usually methane, in a cagelike structure known as a clathrate occurring in sediments overlain by cold deep water.</skos:scopeNote>
    <skos:altLabel xml:lang="en">methane hydrate resources</skos:altLabel>
    <skos:broader rdf:resource="http://www.usgs.gov/science/USGSThesaurus/natural%20gas%20resources"/>
    <skos:related rdf:resource="http://www.usgs.gov/science/USGSThesaurus/economic%20geology"/>
    <skos:inScheme rdf:resource="http://www.usgs.gov/science/USGSThesaurus"/>
  </rdf:Description>
  <rdf:Description about="http://www.usgs.gov/science/USGSThesaurus/oil%20resources">
    <rdf:type rdf:resource="http://www.w3.org/2004/02/skos/core#Concept"/>
    <skos:prefLabel xml:lang="en">oil resources</skos:prefLabel>
    <skos:scopeNote xml:lang="en">Deposits (pools) of highly valuable liquid hydrocarbons or fossil fuels.</skos:scopeNote>
    <skos:altLabel xml:lang="en">petroleum resources (oil)</skos:altLabel>
    <skos:broader rdf:resource="http://www.usgs.gov/science/USGSThesaurus/energy%20resources"/>
    <skos:narrower rdf:resource="http://www.usgs.gov/science/USGSThesaurus/oil%20sand%20resources"/>
    <skos:narrower rdf:resource="http://www.usgs.gov/science/USGSThesaurus/oil%20shale%20resources"/>
    <skos:related rdf:resource="http://www.usgs.gov/science/USGSThesaurus/petroleum"/>
    <skos:related rdf:resource="http://www.usgs.gov/science/USGSThesaurus/economic%20geology"/>
    <skos:inScheme rdf:resource="http://www.usgs.gov/science/USGSThesaurus"/>
  </rdf:Description>
  <rdf:Description about="http://www.usgs.gov/science/USGSThesaurus/oil%20sand%20resources">
    <rdf:type rdf:resource="http://www.w3.org/2004/02/skos/core#Concept"/>
    <skos:prefLabel xml:lang="en">oil sand resources</skos:prefLabel>
    <skos:scopeNote xml:lang="en">Deposits of sandstone or unconsolidated sand containing bitumen that can be extracted as an oil resource.</skos:scopeNote>
    <skos:altLabel xml:lang="en">tar sand resources</skos:altLabel>
    <skos:broader rdf:resource="http://www.usgs.gov/science/USGSThesaurus/oil%20resources"/>
    <skos:related rdf:resource="http://www.usgs.gov/science/USGSThesaurus/economic%20geology"/>
    <skos:inScheme rdf:resource="http://www.usgs.gov/science/USGSThesaurus"/>
  </rdf:Description>
  <rdf:Description about="http://www.usgs.gov/science/USGSThesaurus/oil%20shale%20resources">
    <rdf:type rdf:resource="http://www.w3.org/2004/02/skos/core#Concept"/>
    <skos:prefLabel xml:lang="en">oil shale resources</skos:prefLabel>
    <skos:scopeNote xml:lang="en">Deposits of finely grained sedimentary rock containing kerogen that can be distilled to produce liquid or gaseous hydrocarbons.</skos:scopeNote>
    <skos:broader rdf:resource="http://www.usgs.gov/science/USGSThesaurus/oil%20resources"/>
    <skos:related rdf:resource="http://www.usgs.gov/science/USGSThesaurus/economic%20geology"/>
    <skos:inScheme rdf:resource="http://www.usgs.gov/science/USGSThesaurus"/>
  </rdf:Description>
  <rdf:Description about="http://www.usgs.gov/science/USGSThesaurus/wind%20energy">
    <rdf:type rdf:resource="http://www.w3.org/2004/02/skos/core#Concept"/>
    <skos:prefLabel xml:lang="en">wind energy</skos:prefLabel>
    <skos:scopeNote xml:lang="en">Use of prevailing wind as a source of energy to drive turbines or other machinery.</skos:scopeNote>
    <skos:broader rdf:resource="http://www.usgs.gov/science/USGSThesaurus/energy%20resources"/>
    <skos:inScheme rdf:resource="http://www.usgs.gov/science/USGSThesaurus"/>
  </rdf:Description>
  <rdf:Description about="http://www.usgs.gov/science/USGSThesaurus/fishery%20resources">
    <rdf:type rdf:resource="http://www.w3.org/2004/02/skos/core#Concept"/>
    <skos:prefLabel xml:lang="en">fishery resources</skos:prefLabel>
    <skos:scopeNote xml:lang="en">The stock of anadromous, marine, and freshwater fish in fishing areas of commercial, subsistence, and recreational value.</skos:scopeNote>
    <skos:broader rdf:resource="http://www.usgs.gov/science/USGSThesaurus/natural%20resources"/>
    <skos:narrower rdf:resource="http://www.usgs.gov/science/USGSThesaurus/commercial%20fishery%20resources"/>
    <skos:narrower rdf:resource="http://www.usgs.gov/science/USGSThesaurus/inland%20fishery%20resources"/>
    <skos:narrower rdf:resource="http://www.usgs.gov/science/USGSThesaurus/marine%20fishery%20resources"/>
    <skos:narrower rdf:resource="http://www.usgs.gov/science/USGSThesaurus/recreational%20fishery%20resources"/>
    <skos:narrower rdf:resource="http://www.usgs.gov/science/USGSThesaurus/subsistence%20fishery%20resources"/>
    <skos:related rdf:resource="http://www.usgs.gov/science/USGSThesaurus/aquaculture"/>
    <skos:related rdf:resource="http://www.usgs.gov/science/USGSThesaurus/aquatic%20biology"/>
    <skos:related rdf:resource="http://www.usgs.gov/science/USGSThesaurus/ichthyology"/>
    <skos:related rdf:resource="http://www.usgs.gov/science/USGSThesaurus/marine%20biology"/>
    <skos:related rdf:resource="http://www.usgs.gov/science/USGSThesaurus/overfishing"/>
    <skos:inScheme rdf:resource="http://www.usgs.gov/science/USGSThesaurus"/>
  </rdf:Description>
  <rdf:Description about="http://www.usgs.gov/science/USGSThesaurus/commercial%20fishery%20resources">
    <rdf:type rdf:resource="http://www.w3.org/2004/02/skos/core#Concept"/>
    <skos:prefLabel xml:lang="en">commercial fishery resources</skos:prefLabel>
    <skos:scopeNote xml:lang="en">Stocks of fish and other seafood used for marketing purposes.</skos:scopeNote>
    <skos:broader rdf:resource="http://www.usgs.gov/science/USGSThesaurus/fishery%20resources"/>
    <skos:related rdf:resource="http://www.usgs.gov/science/USGSThesaurus/aquaculture"/>
    <skos:related rdf:resource="http://www.usgs.gov/science/USGSThesaurus/aquatic%20biology"/>
    <skos:related rdf:resource="http://www.usgs.gov/science/USGSThesaurus/ichthyology"/>
    <skos:related rdf:resource="http://www.usgs.gov/science/USGSThesaurus/marine%20biology"/>
    <skos:related rdf:resource="http://www.usgs.gov/science/USGSThesaurus/marine%20fishery%20resources"/>
    <skos:inScheme rdf:resource="http://www.usgs.gov/science/USGSThesaurus"/>
  </rdf:Description>
  <rdf:Description about="http://www.usgs.gov/science/USGSThesaurus/inland%20fishery%20resources">
    <rdf:type rdf:resource="http://www.w3.org/2004/02/skos/core#Concept"/>
    <skos:prefLabel xml:lang="en">inland fishery resources</skos:prefLabel>
    <skos:scopeNote xml:lang="en">Stocks of fish available to be taken in lakes, streams, ponds, rivers, and other inland bodies of water.</skos:scopeNote>
    <skos:broader rdf:resource="http://www.usgs.gov/science/USGSThesaurus/fishery%20resources"/>
    <skos:related rdf:resource="http://www.usgs.gov/science/USGSThesaurus/aquatic%20biology"/>
    <skos:related rdf:resource="http://www.usgs.gov/science/USGSThesaurus/ichthyology"/>
    <skos:inScheme rdf:resource="http://www.usgs.gov/science/USGSThesaurus"/>
  </rdf:Description>
  <rdf:Description about="http://www.usgs.gov/science/USGSThesaurus/marine%20fishery%20resources">
    <rdf:type rdf:resource="http://www.w3.org/2004/02/skos/core#Concept"/>
    <skos:prefLabel xml:lang="en">marine fishery resources</skos:prefLabel>
    <skos:scopeNote xml:lang="en">The stock of fisheries located in seas and oceans.</skos:scopeNote>
    <skos:altLabel xml:lang="en">coastal fisheries</skos:altLabel>
    <skos:altLabel xml:lang="en">coastal fishing</skos:altLabel>
    <skos:altLabel xml:lang="en">deep sea fisheries</skos:altLabel>
    <skos:altLabel xml:lang="en">deep sea fishing</skos:altLabel>
    <skos:altLabel xml:lang="en">reef fisheries</skos:altLabel>
    <skos:altLabel xml:lang="en">reef fishing</skos:altLabel>
    <skos:broader rdf:resource="http://www.usgs.gov/science/USGSThesaurus/fishery%20resources"/>
    <skos:narrower rdf:resource="http://www.usgs.gov/science/USGSThesaurus/whaling"/>
    <skos:related rdf:resource="http://www.usgs.gov/science/USGSThesaurus/aquatic%20biology"/>
    <skos:related rdf:resource="http://www.usgs.gov/science/USGSThesaurus/commercial%20fishery%20resources"/>
    <skos:related rdf:resource="http://www.usgs.gov/science/USGSThesaurus/ichthyology"/>
    <skos:related rdf:resource="http://www.usgs.gov/science/USGSThesaurus/marine%20biology"/>
    <skos:related rdf:resource="http://www.usgs.gov/science/USGSThesaurus/reef%20ecosystems"/>
    <skos:inScheme rdf:resource="http://www.usgs.gov/science/USGSThesaurus"/>
  </rdf:Description>
  <rdf:Description about="http://www.usgs.gov/science/USGSThesaurus/whaling">
    <rdf:type rdf:resource="http://www.w3.org/2004/02/skos/core#Concept"/>
    <skos:prefLabel xml:lang="en">whaling</skos:prefLabel>
    <skos:scopeNote xml:lang="en">Taking whales from the ocean for marketing or subsistence purposes.</skos:scopeNote>
    <skos:broader rdf:resource="http://www.usgs.gov/science/USGSThesaurus/marine%20fishery%20resources"/>
    <skos:related rdf:resource="http://www.usgs.gov/science/USGSThesaurus/marine%20biology"/>
    <skos:inScheme rdf:resource="http://www.usgs.gov/science/USGSThesaurus"/>
  </rdf:Description>
  <rdf:Description about="http://www.usgs.gov/science/USGSThesaurus/recreational%20fishery%20resources">
    <rdf:type rdf:resource="http://www.w3.org/2004/02/skos/core#Concept"/>
    <skos:prefLabel xml:lang="en">recreational fishery resources</skos:prefLabel>
    <skos:scopeNote xml:lang="en">The stock of fish and other seafood resources in areas used for recreational fishing.</skos:scopeNote>
    <skos:altLabel xml:lang="en">recreational fishing</skos:altLabel>
    <skos:altLabel xml:lang="en">sport fishing</skos:altLabel>
    <skos:broader rdf:resource="http://www.usgs.gov/science/USGSThesaurus/fishery%20resources"/>
    <skos:related rdf:resource="http://www.usgs.gov/science/USGSThesaurus/aquatic%20biology"/>
    <skos:related rdf:resource="http://www.usgs.gov/science/USGSThesaurus/ichthyology"/>
    <skos:related rdf:resource="http://www.usgs.gov/science/USGSThesaurus/marine%20biology"/>
    <skos:inScheme rdf:resource="http://www.usgs.gov/science/USGSThesaurus"/>
  </rdf:Description>
  <rdf:Description about="http://www.usgs.gov/science/USGSThesaurus/subsistence%20fishery%20resources">
    <rdf:type rdf:resource="http://www.w3.org/2004/02/skos/core#Concept"/>
    <skos:prefLabel xml:lang="en">subsistence fishery resources</skos:prefLabel>
    <skos:scopeNote xml:lang="en">The stock of fish taken and eaten by local populations rather than marketed.</skos:scopeNote>
    <skos:broader rdf:resource="http://www.usgs.gov/science/USGSThesaurus/fishery%20resources"/>
    <skos:inScheme rdf:resource="http://www.usgs.gov/science/USGSThesaurus"/>
  </rdf:Description>
  <rdf:Description about="http://www.usgs.gov/science/USGSThesaurus/forest%20resources">
    <rdf:type rdf:resource="http://www.w3.org/2004/02/skos/core#Concept"/>
    <skos:prefLabel xml:lang="en">forest resources</skos:prefLabel>
    <skos:scopeNote xml:lang="en">Trees and associated vegetation available for human use.  Use for timber and other forest resources with economic value.</skos:scopeNote>
    <skos:altLabel xml:lang="en">forestry</skos:altLabel>
    <skos:broader rdf:resource="http://www.usgs.gov/science/USGSThesaurus/natural%20resources"/>
    <skos:related rdf:resource="http://www.usgs.gov/science/USGSThesaurus/botany"/>
    <skos:related rdf:resource="http://www.usgs.gov/science/USGSThesaurus/ecology"/>
    <skos:related rdf:resource="http://www.usgs.gov/science/USGSThesaurus/forest%20ecosystems"/>
    <skos:inScheme rdf:resource="http://www.usgs.gov/science/USGSThesaurus"/>
  </rdf:Description>
  <rdf:Description about="http://www.usgs.gov/science/USGSThesaurus/mineral%20resources">
    <rdf:type rdf:resource="http://www.w3.org/2004/02/skos/core#Concept"/>
    <skos:prefLabel xml:lang="en">mineral resources</skos:prefLabel>
    <skos:scopeNote xml:lang="en">Natural occurrences of useful inorganic elements or compounds.</skos:scopeNote>
    <skos:broader rdf:resource="http://www.usgs.gov/science/USGSThesaurus/natural%20resources"/>
    <skos:narrower rdf:resource="http://www.usgs.gov/science/USGSThesaurus/metallic%20mineral%20resources"/>
    <skos:narrower rdf:resource="http://www.usgs.gov/science/USGSThesaurus/nonmetallic%20mineral%20resources"/>
    <skos:related rdf:resource="http://www.usgs.gov/science/USGSThesaurus/economic%20geology"/>
    <skos:related rdf:resource="http://www.usgs.gov/science/USGSThesaurus/mineralogy"/>
    <skos:related rdf:resource="http://www.usgs.gov/science/USGSThesaurus/mineral%20deposits"/>
    <skos:inScheme rdf:resource="http://www.usgs.gov/science/USGSThesaurus"/>
  </rdf:Description>
  <rdf:Description about="http://www.usgs.gov/science/USGSThesaurus/metallic%20mineral%20resources">
    <rdf:type rdf:resource="http://www.w3.org/2004/02/skos/core#Concept"/>
    <skos:prefLabel xml:lang="en">metallic mineral resources</skos:prefLabel>
    <skos:scopeNote xml:lang="en">Resources from which ductile, malleable, opaque,and reflective metals that are also good heat and electricity conductors can be extracted.</skos:scopeNote>
    <skos:altLabel xml:lang="en">ore deposits (metallic)</skos:altLabel>
    <skos:altLabel xml:lang="en">metallic ores</skos:altLabel>
    <skos:broader rdf:resource="http://www.usgs.gov/science/USGSThesaurus/mineral%20resources"/>
    <skos:related rdf:resource="http://www.usgs.gov/science/USGSThesaurus/economic%20geology"/>
    <skos:related rdf:resource="http://www.usgs.gov/science/USGSThesaurus/mineralogy"/>
    <skos:related rdf:resource="http://www.usgs.gov/science/USGSThesaurus/nonmetallic%20mineral%20resources"/>
    <skos:inScheme rdf:resource="http://www.usgs.gov/science/USGSThesaurus"/>
  </rdf:Description>
  <rdf:Description about="http://www.usgs.gov/science/USGSThesaurus/nonmetallic%20mineral%20resources">
    <rdf:type rdf:resource="http://www.w3.org/2004/02/skos/core#Concept"/>
    <skos:prefLabel xml:lang="en">nonmetallic mineral resources</skos:prefLabel>
    <skos:scopeNote xml:lang="en">Useful mineral deposits that are not metals.  Includes materials used for construction, decoration, fuel, and industrial purposes.</skos:scopeNote>
    <skos:altLabel xml:lang="en">industrial mineral resources</skos:altLabel>
    <skos:altLabel xml:lang="en">industrial minerals</skos:altLabel>
    <skos:broader rdf:resource="http://www.usgs.gov/science/USGSThesaurus/mineral%20resources"/>
    <skos:narrower rdf:resource="http://www.usgs.gov/science/USGSThesaurus/building%20stone%20resources"/>
    <skos:narrower rdf:resource="http://www.usgs.gov/science/USGSThesaurus/gem%20resources"/>
    <skos:related rdf:resource="http://www.usgs.gov/science/USGSThesaurus/clay%20deposits"/>
    <skos:related rdf:resource="http://www.usgs.gov/science/USGSThesaurus/economic%20geology"/>
    <skos:related rdf:resource="http://www.usgs.gov/science/USGSThesaurus/gravel%20deposits"/>
    <skos:related rdf:resource="http://www.usgs.gov/science/USGSThesaurus/metallic%20mineral%20resources"/>
    <skos:related rdf:resource="http://www.usgs.gov/science/USGSThesaurus/sand%20deposits"/>
    <skos:inScheme rdf:resource="http://www.usgs.gov/science/USGSThesaurus"/>
  </rdf:Description>
  <rdf:Description about="http://www.usgs.gov/science/USGSThesaurus/building%20stone%20resources">
    <rdf:type rdf:resource="http://www.w3.org/2004/02/skos/core#Concept"/>
    <skos:prefLabel xml:lang="en">building stone resources</skos:prefLabel>
    <skos:scopeNote xml:lang="en">Deposits of rocks used in construction, including crushed stone and dimension stone. Dimension stone includes limestone and granite, quarried in large blocks, and shaped in cubes, panels and other forms.</skos:scopeNote>
    <skos:altLabel xml:lang="en">crushed stone</skos:altLabel>
    <skos:altLabel xml:lang="en">dimension stone</skos:altLabel>
    <skos:broader rdf:resource="http://www.usgs.gov/science/USGSThesaurus/nonmetallic%20mineral%20resources"/>
    <skos:related rdf:resource="http://www.usgs.gov/science/USGSThesaurus/economic%20geology"/>
    <skos:related rdf:resource="http://www.usgs.gov/science/USGSThesaurus/rocks%20and%20deposits"/>
    <skos:related rdf:resource="http://www.usgs.gov/science/USGSThesaurus/sedimentology"/>
    <skos:inScheme rdf:resource="http://www.usgs.gov/science/USGSThesaurus"/>
  </rdf:Description>
  <rdf:Description about="http://www.usgs.gov/science/USGSThesaurus/gem%20resources">
    <rdf:type rdf:resource="http://www.w3.org/2004/02/skos/core#Concept"/>
    <skos:prefLabel xml:lang="en">gem resources</skos:prefLabel>
    <skos:scopeNote xml:lang="en">Deposits of rare minerals prized for their color, durability, sparkle, and clarity when cut and polished and used as ornaments or jewelry.</skos:scopeNote>
    <skos:broader rdf:resource="http://www.usgs.gov/science/USGSThesaurus/nonmetallic%20mineral%20resources"/>
    <skos:related rdf:resource="http://www.usgs.gov/science/USGSThesaurus/economic%20geology"/>
    <skos:related rdf:resource="http://www.usgs.gov/science/USGSThesaurus/mineralogy"/>
    <skos:inScheme rdf:resource="http://www.usgs.gov/science/USGSThesaurus"/>
  </rdf:Description>
  <rdf:Description about="http://www.usgs.gov/science/USGSThesaurus/soil%20resources">
    <rdf:type rdf:resource="http://www.w3.org/2004/02/skos/core#Concept"/>
    <skos:prefLabel xml:lang="en">soil resources</skos:prefLabel>
    <skos:scopeNote xml:lang="en">Natural resources of unconsolidated fragmented rock, humus, and mineral matter that cover the surface of the earth.</skos:scopeNote>
    <!--FOR soil pollution USE soil resources WITH contamination and pollution-->
    <skos:altLabel xml:lang="en">soil pollution</skos:altLabel>
    <skos:broader rdf:resource="http://www.usgs.gov/science/USGSThesaurus/natural%20resources"/>
    <skos:related rdf:resource="http://www.usgs.gov/science/USGSThesaurus/economic%20geology"/>
    <skos:related rdf:resource="http://www.usgs.gov/science/USGSThesaurus/soil%20chemistry"/>
    <skos:related rdf:resource="http://www.usgs.gov/science/USGSThesaurus/soil%20sciences"/>
    <skos:inScheme rdf:resource="http://www.usgs.gov/science/USGSThesaurus"/>
  </rdf:Description>
  <rdf:Description about="http://www.usgs.gov/science/USGSThesaurus/water%20resources">
    <rdf:type rdf:resource="http://www.w3.org/2004/02/skos/core#Concept"/>
    <skos:prefLabel xml:lang="en">water resources</skos:prefLabel>
    <skos:scopeNote xml:lang="en">Stocks of water, the liquid derived from precipitation. A constituent of living matter and necessity for all life, it covers a large proportion of the earth's surface.</skos:scopeNote>
    <skos:altLabel xml:lang="en">hydrosphere</skos:altLabel>
    <!--FOR water pollution USE water resources WITH contamination and pollution-->
    <skos:altLabel xml:lang="en">water pollution</skos:altLabel>
    <skos:broader rdf:resource="http://www.usgs.gov/science/USGSThesaurus/natural%20resources"/>
    <skos:narrower rdf:resource="http://www.usgs.gov/science/USGSThesaurus/groundwater"/>
    <skos:narrower rdf:resource="http://www.usgs.gov/science/USGSThesaurus/surface%20water%20%28non-marine%29"/>
    <skos:related rdf:resource="http://www.usgs.gov/science/USGSThesaurus/hydrogeology"/>
    <skos:related rdf:resource="http://www.usgs.gov/science/USGSThesaurus/hydrology"/>
    <skos:related rdf:resource="http://www.usgs.gov/science/USGSThesaurus/limnology"/>
    <skos:related rdf:resource="http://www.usgs.gov/science/USGSThesaurus/ocean%20characteristics"/>
    <skos:inScheme rdf:resource="http://www.usgs.gov/science/USGSThesaurus"/>
  </rdf:Description>
  <rdf:Description about="http://www.usgs.gov/science/USGSThesaurus/groundwater">
    <rdf:type rdf:resource="http://www.w3.org/2004/02/skos/core#Concept"/>
    <skos:prefLabel xml:lang="en">groundwater</skos:prefLabel>
    <skos:scopeNote xml:lang="en">All water that exists beneath the land surface, but more commonly applied to water in fully saturated soils and geologic formations.</skos:scopeNote>
    <skos:altLabel xml:lang="en">freshwater (ground)</skos:altLabel>
    <skos:altLabel xml:lang="en">ground-water</skos:altLabel>
    <skos:altLabel xml:lang="en">water subsurface</skos:altLabel>
    <skos:altLabel xml:lang="en">ground water</skos:altLabel>
    <skos:broader rdf:resource="http://www.usgs.gov/science/USGSThesaurus/water%20resources"/>
    <skos:narrower rdf:resource="http://www.usgs.gov/science/USGSThesaurus/groundwater%20level"/>
    <skos:related rdf:resource="http://www.usgs.gov/science/USGSThesaurus/freshwater%20ecosystems"/>
    <skos:related rdf:resource="http://www.usgs.gov/science/USGSThesaurus/groundwater%20flow"/>
    <skos:related rdf:resource="http://www.usgs.gov/science/USGSThesaurus/groundwater%20quality"/>
    <skos:related rdf:resource="http://www.usgs.gov/science/USGSThesaurus/hydrogeology"/>
    <skos:inScheme rdf:resource="http://www.usgs.gov/science/USGSThesaurus"/>
  </rdf:Description>
  <rdf:Description about="http://www.usgs.gov/science/USGSThesaurus/groundwater%20level">
    <rdf:type rdf:resource="http://www.w3.org/2004/02/skos/core#Concept"/>
    <skos:prefLabel xml:lang="en">groundwater level</skos:prefLabel>
    <skos:scopeNote xml:lang="en">Depth in a well or aquifer at which groundwater occurs.</skos:scopeNote>
    <skos:altLabel xml:lang="en">aquifer level</skos:altLabel>
    <skos:altLabel xml:lang="en">potentiometric surface</skos:altLabel>
    <skos:altLabel xml:lang="en">water table</skos:altLabel>
    <skos:altLabel xml:lang="en">ground-water level</skos:altLabel>
    <skos:broader rdf:resource="http://www.usgs.gov/science/USGSThesaurus/groundwater"/>
    <skos:narrower rdf:resource="http://www.usgs.gov/science/USGSThesaurus/unsaturated%20zone"/>
    <skos:related rdf:resource="http://www.usgs.gov/science/USGSThesaurus/surface-water%20level"/>
    <skos:inScheme rdf:resource="http://www.usgs.gov/science/USGSThesaurus"/>
  </rdf:Description>
  <rdf:Description about="http://www.usgs.gov/science/USGSThesaurus/unsaturated%20zone">
    <rdf:type rdf:resource="http://www.w3.org/2004/02/skos/core#Concept"/>
    <skos:prefLabel xml:lang="en">unsaturated zone</skos:prefLabel>
    <skos:scopeNote xml:lang="en">The portion of the subsurface above the ground water table.</skos:scopeNote>
    <skos:altLabel xml:lang="en">vadose zone</skos:altLabel>
    <skos:broader rdf:resource="http://www.usgs.gov/science/USGSThesaurus/groundwater%20level"/>
    <skos:inScheme rdf:resource="http://www.usgs.gov/science/USGSThesaurus"/>
  </rdf:Description>
  <rdf:Description about="http://www.usgs.gov/science/USGSThesaurus/surface%20water%20%28non-marine%29">
    <rdf:type rdf:resource="http://www.w3.org/2004/02/skos/core#Concept"/>
    <skos:prefLabel xml:lang="en">surface water (non-marine)</skos:prefLabel>
    <skos:scopeNote xml:lang="en">Open bodies of water, such as lakes, rivers, or streams.  All non-marine waters on the  surface of the earth, including fresh, brackish, and salt water.</skos:scopeNote>
    <skos:altLabel xml:lang="en">freshwater (surface)</skos:altLabel>
    <skos:broader rdf:resource="http://www.usgs.gov/science/USGSThesaurus/water%20resources"/>
    <skos:narrower rdf:resource="http://www.usgs.gov/science/USGSThesaurus/river%20systems"/>
    <skos:narrower rdf:resource="http://www.usgs.gov/science/USGSThesaurus/surface-water%20level"/>
    <skos:related rdf:resource="http://www.usgs.gov/science/USGSThesaurus/floods"/>
    <skos:related rdf:resource="http://www.usgs.gov/science/USGSThesaurus/freshwater%20ecosystems"/>
    <skos:related rdf:resource="http://www.usgs.gov/science/USGSThesaurus/hydrology"/>
    <skos:related rdf:resource="http://www.usgs.gov/science/USGSThesaurus/limnology"/>
    <skos:related rdf:resource="http://www.usgs.gov/science/USGSThesaurus/ocean%20characteristics"/>
    <skos:related rdf:resource="http://www.usgs.gov/science/USGSThesaurus/ocean%20processes"/>
    <skos:related rdf:resource="http://www.usgs.gov/science/USGSThesaurus/stream%20discharge"/>
    <skos:related rdf:resource="http://www.usgs.gov/science/USGSThesaurus/snow%20and%20ice%20cover"/>
    <skos:related rdf:resource="http://www.usgs.gov/science/USGSThesaurus/streamflow"/>
    <skos:related rdf:resource="http://www.usgs.gov/science/USGSThesaurus/surface%20water%20quality"/>
    <skos:inScheme rdf:resource="http://www.usgs.gov/science/USGSThesaurus"/>
  </rdf:Description>
  <rdf:Description about="http://www.usgs.gov/science/USGSThesaurus/river%20systems">
    <rdf:type rdf:resource="http://www.w3.org/2004/02/skos/core#Concept"/>
    <skos:prefLabel xml:lang="en">river systems</skos:prefLabel>
    <skos:scopeNote xml:lang="en">Long water courses including main streams and tributaries.</skos:scopeNote>
    <!--FOR river ecosystems USE river systems WITH freshwater ecosystems-->
    <skos:altLabel xml:lang="en">river ecosystems</skos:altLabel>
    <skos:broader rdf:resource="http://www.usgs.gov/science/USGSThesaurus/surface%20water%20%28non-marine%29"/>
    <skos:narrower rdf:resource="http://www.usgs.gov/science/USGSThesaurus/river%20reaches"/>
    <skos:related rdf:resource="http://www.usgs.gov/science/USGSThesaurus/hydrology"/>
    <skos:related rdf:resource="http://www.usgs.gov/science/USGSThesaurus/stream%20discharge"/>
    <skos:inScheme rdf:resource="http://www.usgs.gov/science/USGSThesaurus"/>
  </rdf:Description>
  <rdf:Description about="http://www.usgs.gov/science/USGSThesaurus/river%20reaches">
    <rdf:type rdf:resource="http://www.w3.org/2004/02/skos/core#Concept"/>
    <skos:prefLabel xml:lang="en">river reaches</skos:prefLabel>
    <skos:scopeNote xml:lang="en">Continuous parts of streams between two specified points.</skos:scopeNote>
    <skos:altLabel xml:lang="en">reaches (hydraulic)</skos:altLabel>
    <skos:altLabel xml:lang="en">reaches (streams)</skos:altLabel>
    <skos:broader rdf:resource="http://www.usgs.gov/science/USGSThesaurus/river%20systems"/>
    <skos:related rdf:resource="http://www.usgs.gov/science/USGSThesaurus/hydrology"/>
    <skos:inScheme rdf:resource="http://www.usgs.gov/science/USGSThesaurus"/>
  </rdf:Description>
  <rdf:Description about="http://www.usgs.gov/science/USGSThesaurus/surface-water%20level">
    <rdf:type rdf:resource="http://www.w3.org/2004/02/skos/core#Concept"/>
    <skos:prefLabel xml:lang="en">surface-water level</skos:prefLabel>
    <skos:scopeNote xml:lang="en">Height of the water surface in a lake or reservoir. For water levels in flowing streams, refer to streamflow.</skos:scopeNote>
    <skos:broader rdf:resource="http://www.usgs.gov/science/USGSThesaurus/surface%20water%20%28non-marine%29"/>
    <skos:related rdf:resource="http://www.usgs.gov/science/USGSThesaurus/groundwater%20level"/>
    <skos:related rdf:resource="http://www.usgs.gov/science/USGSThesaurus/streamflow"/>
    <skos:inScheme rdf:resource="http://www.usgs.gov/science/USGSThesaurus"/>
  </rdf:Description>
  <rdf:Description about="http://www.usgs.gov/science/USGSThesaurus/organism%20groupings%20%28non-taxonomic%29">
    <rdf:type rdf:resource="http://www.w3.org/2004/02/skos/core#Concept"/>
    <skos:prefLabel xml:lang="en">organism groupings (non-taxonomic)</skos:prefLabel>
    <skos:scopeNote xml:lang="en">Used for categories of living organisms that are not taxonomic and that include species from more than one taxonomic group.</skos:scopeNote>
    <skos:broader rdf:resource="http://www.usgs.gov/science/USGSThesaurus/topics"/>
    <skos:narrower rdf:resource="http://www.usgs.gov/science/USGSThesaurus/benthos"/>
    <skos:narrower rdf:resource="http://www.usgs.gov/science/USGSThesaurus/biota"/>
    <skos:narrower rdf:resource="http://www.usgs.gov/science/USGSThesaurus/consumers%20%28organisms%29"/>
    <skos:narrower rdf:resource="http://www.usgs.gov/science/USGSThesaurus/decomposers"/>
    <skos:narrower rdf:resource="http://www.usgs.gov/science/USGSThesaurus/endangered%20species"/>
    <skos:narrower rdf:resource="http://www.usgs.gov/science/USGSThesaurus/game%20species"/>
    <skos:narrower rdf:resource="http://www.usgs.gov/science/USGSThesaurus/genetically%20engineered%20organisms"/>
    <skos:narrower rdf:resource="http://www.usgs.gov/science/USGSThesaurus/keystone%20species"/>
    <skos:narrower rdf:resource="http://www.usgs.gov/science/USGSThesaurus/macroinvertebrates"/>
    <skos:narrower rdf:resource="http://www.usgs.gov/science/USGSThesaurus/microbes"/>
    <skos:narrower rdf:resource="http://www.usgs.gov/science/USGSThesaurus/migratory%20species"/>
    <skos:narrower rdf:resource="http://www.usgs.gov/science/USGSThesaurus/native%20species"/>
    <skos:narrower rdf:resource="http://www.usgs.gov/science/USGSThesaurus/nekton"/>
    <skos:narrower rdf:resource="http://www.usgs.gov/science/USGSThesaurus/nonindigenous%20species"/>
    <skos:narrower rdf:resource="http://www.usgs.gov/science/USGSThesaurus/nuisance%20species"/>
    <skos:narrower rdf:resource="http://www.usgs.gov/science/USGSThesaurus/parasites"/>
    <skos:narrower rdf:resource="http://www.usgs.gov/science/USGSThesaurus/plankton"/>
    <skos:narrower rdf:resource="http://www.usgs.gov/science/USGSThesaurus/pollinators"/>
    <skos:narrower rdf:resource="http://www.usgs.gov/science/USGSThesaurus/producers%20%28organisms%29"/>
    <skos:narrower rdf:resource="http://www.usgs.gov/science/USGSThesaurus/shellfish"/>
    <skos:narrower rdf:resource="http://www.usgs.gov/science/USGSThesaurus/vegetation"/>
    <skos:narrower rdf:resource="http://www.usgs.gov/science/USGSThesaurus/wildlife"/>
    <skos:related rdf:resource="http://www.usgs.gov/science/USGSThesaurus/life%20sciences"/>
    <skos:related rdf:resource="http://www.usgs.gov/science/USGSThesaurus/organisms"/>
    <skos:inScheme rdf:resource="http://www.usgs.gov/science/USGSThesaurus"/>
  </rdf:Description>
  <rdf:Description about="http://www.usgs.gov/science/USGSThesaurus/benthos">
    <rdf:type rdf:resource="http://www.w3.org/2004/02/skos/core#Concept"/>
    <skos:prefLabel xml:lang="en">benthos</skos:prefLabel>
    <skos:scopeNote xml:lang="en">Animals that live on the bottom of water bodies.</skos:scopeNote>
    <skos:broader rdf:resource="http://www.usgs.gov/science/USGSThesaurus/organism%20groupings%20%28non-taxonomic%29"/>
    <skos:inScheme rdf:resource="http://www.usgs.gov/science/USGSThesaurus"/>
  </rdf:Description>
  <rdf:Description about="http://www.usgs.gov/science/USGSThesaurus/biota">
    <rdf:type rdf:resource="http://www.w3.org/2004/02/skos/core#Concept"/>
    <skos:prefLabel xml:lang="en">biota</skos:prefLabel>
    <skos:scopeNote xml:lang="en">All living organisms in an area.</skos:scopeNote>
    <skos:broader rdf:resource="http://www.usgs.gov/science/USGSThesaurus/organism%20groupings%20%28non-taxonomic%29"/>
    <skos:related rdf:resource="http://www.usgs.gov/science/USGSThesaurus/life%20sciences"/>
    <skos:inScheme rdf:resource="http://www.usgs.gov/science/USGSThesaurus"/>
  </rdf:Description>
  <rdf:Description about="http://www.usgs.gov/science/USGSThesaurus/consumers%20%28organisms%29">
    <rdf:type rdf:resource="http://www.w3.org/2004/02/skos/core#Concept"/>
    <skos:prefLabel xml:lang="en">consumers (organisms)</skos:prefLabel>
    <skos:scopeNote xml:lang="en">Organisms unable to produce food from nonliving matter and dependent on ingesting other animals, plants, or particulate organic matter.</skos:scopeNote>
    <skos:broader rdf:resource="http://www.usgs.gov/science/USGSThesaurus/organism%20groupings%20%28non-taxonomic%29"/>
    <skos:narrower rdf:resource="http://www.usgs.gov/science/USGSThesaurus/carnivores"/>
    <skos:narrower rdf:resource="http://www.usgs.gov/science/USGSThesaurus/herbivores"/>
    <skos:narrower rdf:resource="http://www.usgs.gov/science/USGSThesaurus/omnivores"/>
    <skos:related rdf:resource="http://www.usgs.gov/science/USGSThesaurus/ecology"/>
    <skos:related rdf:resource="http://www.usgs.gov/science/USGSThesaurus/zoology"/>
    <skos:inScheme rdf:resource="http://www.usgs.gov/science/USGSThesaurus"/>
  </rdf:Description>
  <rdf:Description about="http://www.usgs.gov/science/USGSThesaurus/carnivores">
    <rdf:type rdf:resource="http://www.w3.org/2004/02/skos/core#Concept"/>
    <skos:prefLabel xml:lang="en">carnivores</skos:prefLabel>
    <skos:scopeNote xml:lang="en">Flesh-eating animals.</skos:scopeNote>
    <skos:altLabel xml:lang="en">predators</skos:altLabel>
    <skos:broader rdf:resource="http://www.usgs.gov/science/USGSThesaurus/consumers%20%28organisms%29"/>
    <skos:related rdf:resource="http://www.usgs.gov/science/USGSThesaurus/ecology"/>
    <skos:related rdf:resource="http://www.usgs.gov/science/USGSThesaurus/zoology"/>
    <skos:inScheme rdf:resource="http://www.usgs.gov/science/USGSThesaurus"/>
  </rdf:Description>
  <rdf:Description about="http://www.usgs.gov/science/USGSThesaurus/herbivores">
    <rdf:type rdf:resource="http://www.w3.org/2004/02/skos/core#Concept"/>
    <skos:prefLabel xml:lang="en">herbivores</skos:prefLabel>
    <skos:scopeNote xml:lang="en">Animals that eat chiefly plants or their products, such as seeds, nectar, and fruit.</skos:scopeNote>
    <skos:broader rdf:resource="http://www.usgs.gov/science/USGSThesaurus/consumers%20%28organisms%29"/>
    <skos:related rdf:resource="http://www.usgs.gov/science/USGSThesaurus/ecology"/>
    <skos:related rdf:resource="http://www.usgs.gov/science/USGSThesaurus/zoology"/>
    <skos:inScheme rdf:resource="http://www.usgs.gov/science/USGSThesaurus"/>
  </rdf:Description>
  <rdf:Description about="http://www.usgs.gov/science/USGSThesaurus/omnivores">
    <rdf:type rdf:resource="http://www.w3.org/2004/02/skos/core#Concept"/>
    <skos:prefLabel xml:lang="en">omnivores</skos:prefLabel>
    <skos:scopeNote xml:lang="en">Animals that eat both plant and animal materials.</skos:scopeNote>
    <skos:broader rdf:resource="http://www.usgs.gov/science/USGSThesaurus/consumers%20%28organisms%29"/>
    <skos:related rdf:resource="http://www.usgs.gov/science/USGSThesaurus/ecology"/>
    <skos:related rdf:resource="http://www.usgs.gov/science/USGSThesaurus/zoology"/>
    <skos:inScheme rdf:resource="http://www.usgs.gov/science/USGSThesaurus"/>
  </rdf:Description>
  <rdf:Description about="http://www.usgs.gov/science/USGSThesaurus/decomposers">
    <rdf:type rdf:resource="http://www.w3.org/2004/02/skos/core#Concept"/>
    <skos:prefLabel xml:lang="en">decomposers</skos:prefLabel>
    <skos:scopeNote xml:lang="en">Organisms, chiefly microorganisms and invertebrates, that feed on dead plant or animal matter breaking it down and recycling the resulting elements and compounds in the environment.</skos:scopeNote>
    <skos:broader rdf:resource="http://www.usgs.gov/science/USGSThesaurus/organism%20groupings%20%28non-taxonomic%29"/>
    <skos:related rdf:resource="http://www.usgs.gov/science/USGSThesaurus/biogeochemical%20cycling"/>
    <skos:related rdf:resource="http://www.usgs.gov/science/USGSThesaurus/ecology"/>
    <skos:related rdf:resource="http://www.usgs.gov/science/USGSThesaurus/life%20sciences"/>
    <skos:inScheme rdf:resource="http://www.usgs.gov/science/USGSThesaurus"/>
  </rdf:Description>
  <rdf:Description about="http://www.usgs.gov/science/USGSThesaurus/endangered%20species">
    <rdf:type rdf:resource="http://www.w3.org/2004/02/skos/core#Concept"/>
    <skos:prefLabel xml:lang="en">endangered species</skos:prefLabel>
    <skos:scopeNote xml:lang="en">Plant or animal species reduced to such low numbers of individuals that they are at risk of becoming extinct.</skos:scopeNote>
    <skos:broader rdf:resource="http://www.usgs.gov/science/USGSThesaurus/organism%20groupings%20%28non-taxonomic%29"/>
    <skos:related rdf:resource="http://www.usgs.gov/science/USGSThesaurus/biodiversity"/>
    <skos:related rdf:resource="http://www.usgs.gov/science/USGSThesaurus/ecological%20competition"/>
    <skos:related rdf:resource="http://www.usgs.gov/science/USGSThesaurus/ecology"/>
    <skos:related rdf:resource="http://www.usgs.gov/science/USGSThesaurus/life%20sciences"/>
    <skos:inScheme rdf:resource="http://www.usgs.gov/science/USGSThesaurus"/>
  </rdf:Description>
  <rdf:Description about="http://www.usgs.gov/science/USGSThesaurus/game%20species">
    <rdf:type rdf:resource="http://www.w3.org/2004/02/skos/core#Concept"/>
    <skos:prefLabel xml:lang="en">game species</skos:prefLabel>
    <skos:scopeNote xml:lang="en">Species of wild animals that are hunted for food or sport.</skos:scopeNote>
    <skos:broader rdf:resource="http://www.usgs.gov/science/USGSThesaurus/organism%20groupings%20%28non-taxonomic%29"/>
    <skos:related rdf:resource="http://www.usgs.gov/science/USGSThesaurus/vertebrate%20zoology"/>
    <skos:related rdf:resource="http://www.usgs.gov/science/USGSThesaurus/wildlife%20biology"/>
    <skos:inScheme rdf:resource="http://www.usgs.gov/science/USGSThesaurus"/>
  </rdf:Description>
  <rdf:Description about="http://www.usgs.gov/science/USGSThesaurus/genetically%20engineered%20organisms">
    <rdf:type rdf:resource="http://www.w3.org/2004/02/skos/core#Concept"/>
    <skos:prefLabel xml:lang="en">genetically engineered organisms</skos:prefLabel>
    <skos:scopeNote xml:lang="en">Organisms whose DNA has been modified through the insertion or deletion of DNA fragments from the same or another species, in order to produce or enhance desirable traits such as increased yield, resistance to pests, adaptation to drastically changed environments, or formation of entirely new compounds.</skos:scopeNote>
    <skos:altLabel xml:lang="en">genetically modified organisms</skos:altLabel>
    <skos:broader rdf:resource="http://www.usgs.gov/science/USGSThesaurus/organism%20groupings%20%28non-taxonomic%29"/>
    <skos:inScheme rdf:resource="http://www.usgs.gov/science/USGSThesaurus"/>
  </rdf:Description>
  <rdf:Description about="http://www.usgs.gov/science/USGSThesaurus/keystone%20species">
    <rdf:type rdf:resource="http://www.w3.org/2004/02/skos/core#Concept"/>
    <skos:prefLabel xml:lang="en">keystone species</skos:prefLabel>
    <skos:scopeNote xml:lang="en">Species whose abundance and ecological role has a dramatic effect on the other species in an ecosystem.</skos:scopeNote>
    <skos:broader rdf:resource="http://www.usgs.gov/science/USGSThesaurus/organism%20groupings%20%28non-taxonomic%29"/>
    <skos:inScheme rdf:resource="http://www.usgs.gov/science/USGSThesaurus"/>
  </rdf:Description>
  <rdf:Description about="http://www.usgs.gov/science/USGSThesaurus/macroinvertebrates">
    <rdf:type rdf:resource="http://www.w3.org/2004/02/skos/core#Concept"/>
    <skos:prefLabel xml:lang="en">macroinvertebrates</skos:prefLabel>
    <skos:scopeNote xml:lang="en">Invertebrate animals large enough to be studied without a microscope.</skos:scopeNote>
    <skos:broader rdf:resource="http://www.usgs.gov/science/USGSThesaurus/organism%20groupings%20%28non-taxonomic%29"/>
    <skos:related rdf:resource="http://www.usgs.gov/science/USGSThesaurus/aquatic%20biology"/>
    <skos:inScheme rdf:resource="http://www.usgs.gov/science/USGSThesaurus"/>
  </rdf:Description>
  <rdf:Description about="http://www.usgs.gov/science/USGSThesaurus/microbes">
    <rdf:type rdf:resource="http://www.w3.org/2004/02/skos/core#Concept"/>
    <skos:prefLabel xml:lang="en">microbes</skos:prefLabel>
    <skos:scopeNote xml:lang="en">Microscopic, typically one-celled organisms.</skos:scopeNote>
    <skos:altLabel xml:lang="en">microorganisms</skos:altLabel>
    <skos:broader rdf:resource="http://www.usgs.gov/science/USGSThesaurus/organism%20groupings%20%28non-taxonomic%29"/>
    <skos:inScheme rdf:resource="http://www.usgs.gov/science/USGSThesaurus"/>
  </rdf:Description>
  <rdf:Description about="http://www.usgs.gov/science/USGSThesaurus/migratory%20species">
    <rdf:type rdf:resource="http://www.w3.org/2004/02/skos/core#Concept"/>
    <skos:prefLabel xml:lang="en">migratory species</skos:prefLabel>
    <skos:scopeNote xml:lang="en">Species that have a pattern of moving from one geographical area to another, primarily according to the seasons, and usually traveling long distances along established routes.</skos:scopeNote>
    <!--FOR anadromous fish USE migratory species WITH fish-->
    <skos:altLabel xml:lang="en">anadromous fish</skos:altLabel>
    <!--FOR diadromous fish USE migratory species WITH fish-->
    <skos:altLabel xml:lang="en">diadromous fish</skos:altLabel>
    <skos:broader rdf:resource="http://www.usgs.gov/science/USGSThesaurus/organism%20groupings%20%28non-taxonomic%29"/>
    <skos:related rdf:resource="http://www.usgs.gov/science/USGSThesaurus/animal%20behavior"/>
    <skos:related rdf:resource="http://www.usgs.gov/science/USGSThesaurus/aquatic%20biology"/>
    <skos:related rdf:resource="http://www.usgs.gov/science/USGSThesaurus/biogeography"/>
    <skos:related rdf:resource="http://www.usgs.gov/science/USGSThesaurus/ecology"/>
    <skos:related rdf:resource="http://www.usgs.gov/science/USGSThesaurus/marine%20biology"/>
    <skos:related rdf:resource="http://www.usgs.gov/science/USGSThesaurus/migration%20%28organisms%29"/>
    <skos:related rdf:resource="http://www.usgs.gov/science/USGSThesaurus/zoology"/>
    <skos:inScheme rdf:resource="http://www.usgs.gov/science/USGSThesaurus"/>
  </rdf:Description>
  <rdf:Description about="http://www.usgs.gov/science/USGSThesaurus/native%20species">
    <rdf:type rdf:resource="http://www.w3.org/2004/02/skos/core#Concept"/>
    <skos:prefLabel xml:lang="en">native species</skos:prefLabel>
    <skos:scopeNote xml:lang="en">Organisms originating in the area where they live.</skos:scopeNote>
    <skos:altLabel xml:lang="en">indigenous species</skos:altLabel>
    <skos:broader rdf:resource="http://www.usgs.gov/science/USGSThesaurus/organism%20groupings%20%28non-taxonomic%29"/>
    <skos:narrower rdf:resource="http://www.usgs.gov/science/USGSThesaurus/endemic%20species"/>
    <skos:related rdf:resource="http://www.usgs.gov/science/USGSThesaurus/biodiversity"/>
    <skos:related rdf:resource="http://www.usgs.gov/science/USGSThesaurus/ecology"/>
    <skos:related rdf:resource="http://www.usgs.gov/science/USGSThesaurus/life%20sciences"/>
    <skos:related rdf:resource="http://www.usgs.gov/science/USGSThesaurus/nonindigenous%20species"/>
    <skos:inScheme rdf:resource="http://www.usgs.gov/science/USGSThesaurus"/>
  </rdf:Description>
  <rdf:Description about="http://www.usgs.gov/science/USGSThesaurus/endemic%20species">
    <rdf:type rdf:resource="http://www.w3.org/2004/02/skos/core#Concept"/>
    <skos:prefLabel xml:lang="en">endemic species</skos:prefLabel>
    <skos:scopeNote xml:lang="en">Plant and animals species native to and confined to specific geographic areas.</skos:scopeNote>
    <skos:broader rdf:resource="http://www.usgs.gov/science/USGSThesaurus/native%20species"/>
    <skos:related rdf:resource="http://www.usgs.gov/science/USGSThesaurus/biodiversity"/>
    <skos:related rdf:resource="http://www.usgs.gov/science/USGSThesaurus/ecology"/>
    <skos:related rdf:resource="http://www.usgs.gov/science/USGSThesaurus/life%20sciences"/>
    <skos:inScheme rdf:resource="http://www.usgs.gov/science/USGSThesaurus"/>
  </rdf:Description>
  <rdf:Description about="http://www.usgs.gov/science/USGSThesaurus/nekton">
    <rdf:type rdf:resource="http://www.w3.org/2004/02/skos/core#Concept"/>
    <skos:prefLabel xml:lang="en">nekton</skos:prefLabel>
    <skos:scopeNote xml:lang="en">Free-swimming aquatic organisms able to move without depending on waves, currents, and tides.</skos:scopeNote>
    <skos:broader rdf:resource="http://www.usgs.gov/science/USGSThesaurus/organism%20groupings%20%28non-taxonomic%29"/>
    <skos:inScheme rdf:resource="http://www.usgs.gov/science/USGSThesaurus"/>
  </rdf:Description>
  <rdf:Description about="http://www.usgs.gov/science/USGSThesaurus/nonindigenous%20species">
    <rdf:type rdf:resource="http://www.w3.org/2004/02/skos/core#Concept"/>
    <skos:prefLabel xml:lang="en">nonindigenous species</skos:prefLabel>
    <skos:scopeNote xml:lang="en">Organisms accidentally or intentionally introduced into areas where they did not previously originate or live.</skos:scopeNote>
    <skos:altLabel xml:lang="en">alien species</skos:altLabel>
    <skos:altLabel xml:lang="en">exotic species</skos:altLabel>
    <skos:altLabel xml:lang="en">foreign species</skos:altLabel>
    <skos:altLabel xml:lang="en">introduced species</skos:altLabel>
    <skos:altLabel xml:lang="en">non-indigenous species</skos:altLabel>
    <skos:altLabel xml:lang="en">non-native species</skos:altLabel>
    <skos:broader rdf:resource="http://www.usgs.gov/science/USGSThesaurus/organism%20groupings%20%28non-taxonomic%29"/>
    <skos:narrower rdf:resource="http://www.usgs.gov/science/USGSThesaurus/invasive%20species"/>
    <skos:related rdf:resource="http://www.usgs.gov/science/USGSThesaurus/biodiversity"/>
    <skos:related rdf:resource="http://www.usgs.gov/science/USGSThesaurus/ecology"/>
    <skos:related rdf:resource="http://www.usgs.gov/science/USGSThesaurus/life%20sciences"/>
    <skos:related rdf:resource="http://www.usgs.gov/science/USGSThesaurus/native%20species"/>
    <skos:inScheme rdf:resource="http://www.usgs.gov/science/USGSThesaurus"/>
  </rdf:Description>
  <rdf:Description about="http://www.usgs.gov/science/USGSThesaurus/invasive%20species">
    <rdf:type rdf:resource="http://www.w3.org/2004/02/skos/core#Concept"/>
    <skos:prefLabel xml:lang="en">invasive species</skos:prefLabel>
    <skos:scopeNote xml:lang="en">Plant, animal, or microbe species that is non-native (or alien) to the ecosystem under consideration and whose introduction causes or is likely to cause economic or environmental harm, or harm to human health.</skos:scopeNote>
    <!--FOR biological invasions USE invasive species WITH migration (organisms)-->
    <skos:altLabel xml:lang="en">biological invasions</skos:altLabel>
    <skos:altLabel xml:lang="en">invader species</skos:altLabel>
    <skos:broader rdf:resource="http://www.usgs.gov/science/USGSThesaurus/nonindigenous%20species"/>
    <skos:related rdf:resource="http://www.usgs.gov/science/USGSThesaurus/biodiversity"/>
    <skos:related rdf:resource="http://www.usgs.gov/science/USGSThesaurus/ecology"/>
    <skos:related rdf:resource="http://www.usgs.gov/science/USGSThesaurus/human%20impacts"/>
    <skos:related rdf:resource="http://www.usgs.gov/science/USGSThesaurus/life%20sciences"/>
    <skos:inScheme rdf:resource="http://www.usgs.gov/science/USGSThesaurus"/>
  </rdf:Description>
  <rdf:Description about="http://www.usgs.gov/science/USGSThesaurus/nuisance%20species">
    <rdf:type rdf:resource="http://www.w3.org/2004/02/skos/core#Concept"/>
    <skos:prefLabel xml:lang="en">nuisance species</skos:prefLabel>
    <skos:scopeNote xml:lang="en">Organisms whose presence or behavior has undesirable effects on human activities.</skos:scopeNote>
    <skos:broader rdf:resource="http://www.usgs.gov/science/USGSThesaurus/organism%20groupings%20%28non-taxonomic%29"/>
    <skos:inScheme rdf:resource="http://www.usgs.gov/science/USGSThesaurus"/>
  </rdf:Description>
  <rdf:Description about="http://www.usgs.gov/science/USGSThesaurus/parasites">
    <rdf:type rdf:resource="http://www.w3.org/2004/02/skos/core#Concept"/>
    <skos:prefLabel xml:lang="en">parasites</skos:prefLabel>
    <skos:scopeNote xml:lang="en">Symbiotic organisms that are detrimental to the host.</skos:scopeNote>
    <skos:broader rdf:resource="http://www.usgs.gov/science/USGSThesaurus/organism%20groupings%20%28non-taxonomic%29"/>
    <skos:inScheme rdf:resource="http://www.usgs.gov/science/USGSThesaurus"/>
  </rdf:Description>
  <rdf:Description about="http://www.usgs.gov/science/USGSThesaurus/plankton">
    <rdf:type rdf:resource="http://www.w3.org/2004/02/skos/core#Concept"/>
    <skos:prefLabel xml:lang="en">plankton</skos:prefLabel>
    <skos:scopeNote xml:lang="en">Floating aquatic plants (phytoplankton) and animals (zooplankton) which are often microscopic and drift with the current in lakes, rivers, and oceans.</skos:scopeNote>
    <!--FOR planktonic ecosystems USE plankton WITH aquatic ecosystems-->
    <skos:altLabel xml:lang="en">planktonic ecosystems</skos:altLabel>
    <skos:altLabel xml:lang="en">zooplankton</skos:altLabel>
    <skos:broader rdf:resource="http://www.usgs.gov/science/USGSThesaurus/organism%20groupings%20%28non-taxonomic%29"/>
    <skos:narrower rdf:resource="http://www.usgs.gov/science/USGSThesaurus/phytoplankton"/>
    <skos:related rdf:resource="http://www.usgs.gov/science/USGSThesaurus/aquatic%20biology"/>
    <skos:related rdf:resource="http://www.usgs.gov/science/USGSThesaurus/calcareous%20nannoplankton"/>
    <skos:related rdf:resource="http://www.usgs.gov/science/USGSThesaurus/microbiology"/>
    <skos:related rdf:resource="http://www.usgs.gov/science/USGSThesaurus/phycology"/>
    <skos:inScheme rdf:resource="http://www.usgs.gov/science/USGSThesaurus"/>
  </rdf:Description>
  <rdf:Description about="http://www.usgs.gov/science/USGSThesaurus/phytoplankton">
    <rdf:type rdf:resource="http://www.w3.org/2004/02/skos/core#Concept"/>
    <skos:prefLabel xml:lang="en">phytoplankton</skos:prefLabel>
    <skos:scopeNote xml:lang="en">Small, mostly microscopic aquatic plants such as algae and bacteria suspended in water.</skos:scopeNote>
    <skos:broader rdf:resource="http://www.usgs.gov/science/USGSThesaurus/plankton"/>
    <skos:related rdf:resource="http://www.usgs.gov/science/USGSThesaurus/calcareous%20nannoplankton"/>
    <skos:inScheme rdf:resource="http://www.usgs.gov/science/USGSThesaurus"/>
  </rdf:Description>
  <rdf:Description about="http://www.usgs.gov/science/USGSThesaurus/pollinators">
    <rdf:type rdf:resource="http://www.w3.org/2004/02/skos/core#Concept"/>
    <skos:prefLabel xml:lang="en">pollinators</skos:prefLabel>
    <skos:scopeNote xml:lang="en">Organisms that aid in the growth and distribution of plants by transferring pollen as a byproduct of their feeding activities.</skos:scopeNote>
    <skos:broader rdf:resource="http://www.usgs.gov/science/USGSThesaurus/organism%20groupings%20%28non-taxonomic%29"/>
    <skos:related rdf:resource="http://www.usgs.gov/science/USGSThesaurus/ecology"/>
    <skos:related rdf:resource="http://www.usgs.gov/science/USGSThesaurus/entomology"/>
    <skos:related rdf:resource="http://www.usgs.gov/science/USGSThesaurus/ornithology"/>
    <skos:related rdf:resource="http://www.usgs.gov/science/USGSThesaurus/pollination"/>
    <skos:related rdf:resource="http://www.usgs.gov/science/USGSThesaurus/zoology"/>
    <skos:inScheme rdf:resource="http://www.usgs.gov/science/USGSThesaurus"/>
  </rdf:Description>
  <rdf:Description about="http://www.usgs.gov/science/USGSThesaurus/producers%20%28organisms%29">
    <rdf:type rdf:resource="http://www.w3.org/2004/02/skos/core#Concept"/>
    <skos:prefLabel xml:lang="en">producers (organisms)</skos:prefLabel>
    <skos:scopeNote xml:lang="en">Organisms, chiefly green plants, which use inorganic elements, compounds, and light to produce their food (photosynthesis). They are a source of food for animals.</skos:scopeNote>
    <skos:broader rdf:resource="http://www.usgs.gov/science/USGSThesaurus/organism%20groupings%20%28non-taxonomic%29"/>
    <skos:related rdf:resource="http://www.usgs.gov/science/USGSThesaurus/botany"/>
    <skos:related rdf:resource="http://www.usgs.gov/science/USGSThesaurus/ecology"/>
    <skos:related rdf:resource="http://www.usgs.gov/science/USGSThesaurus/microbiology"/>
    <skos:inScheme rdf:resource="http://www.usgs.gov/science/USGSThesaurus"/>
  </rdf:Description>
  <rdf:Description about="http://www.usgs.gov/science/USGSThesaurus/shellfish">
    <rdf:type rdf:resource="http://www.w3.org/2004/02/skos/core#Concept"/>
    <skos:prefLabel xml:lang="en">shellfish</skos:prefLabel>
    <skos:scopeNote xml:lang="en">Aquatic invertebrates with shells, usually mollusks and crustaceans. Includes clams, lobsters, and oysters.</skos:scopeNote>
    <skos:broader rdf:resource="http://www.usgs.gov/science/USGSThesaurus/organism%20groupings%20%28non-taxonomic%29"/>
    <skos:related rdf:resource="http://www.usgs.gov/science/USGSThesaurus/aquatic%20biology"/>
    <skos:related rdf:resource="http://www.usgs.gov/science/USGSThesaurus/crustaceans"/>
    <skos:related rdf:resource="http://www.usgs.gov/science/USGSThesaurus/invertebrate%20zoology"/>
    <skos:related rdf:resource="http://www.usgs.gov/science/USGSThesaurus/mollusks"/>
    <skos:inScheme rdf:resource="http://www.usgs.gov/science/USGSThesaurus"/>
  </rdf:Description>
  <rdf:Description about="http://www.usgs.gov/science/USGSThesaurus/vegetation">
    <rdf:type rdf:resource="http://www.w3.org/2004/02/skos/core#Concept"/>
    <skos:prefLabel xml:lang="en">vegetation</skos:prefLabel>
    <skos:scopeNote xml:lang="en">Plant life or general plant cover in an area.</skos:scopeNote>
    <skos:altLabel xml:lang="en">grasses</skos:altLabel>
    <skos:altLabel xml:lang="en">trees</skos:altLabel>
    <!--FOR dendroecology USE vegetation WITH ecosystem monitoring-->
    <skos:altLabel xml:lang="en">dendroecology</skos:altLabel>
    <skos:broader rdf:resource="http://www.usgs.gov/science/USGSThesaurus/organism%20groupings%20%28non-taxonomic%29"/>
    <skos:narrower rdf:resource="http://www.usgs.gov/science/USGSThesaurus/aquatic%20vegetation"/>
    <skos:narrower rdf:resource="http://www.usgs.gov/science/USGSThesaurus/periphyton"/>
    <skos:narrower rdf:resource="http://www.usgs.gov/science/USGSThesaurus/weeds"/>
    <skos:related rdf:resource="http://www.usgs.gov/science/USGSThesaurus/botany"/>
    <skos:related rdf:resource="http://www.usgs.gov/science/USGSThesaurus/ecology"/>
    <skos:related rdf:resource="http://www.usgs.gov/science/USGSThesaurus/plants%20%28organisms%29"/>
    <skos:inScheme rdf:resource="http://www.usgs.gov/science/USGSThesaurus"/>
  </rdf:Description>
  <rdf:Description about="http://www.usgs.gov/science/USGSThesaurus/aquatic%20vegetation">
    <rdf:type rdf:resource="http://www.w3.org/2004/02/skos/core#Concept"/>
    <skos:prefLabel xml:lang="en">aquatic vegetation</skos:prefLabel>
    <skos:scopeNote xml:lang="en">Plants living primarily in or under water.</skos:scopeNote>
    <skos:altLabel xml:lang="en">hydrophytes</skos:altLabel>
    <skos:altLabel xml:lang="en">mangroves</skos:altLabel>
    <skos:altLabel xml:lang="en">seagrass</skos:altLabel>
    <skos:altLabel xml:lang="en">seaweeds</skos:altLabel>
    <skos:broader rdf:resource="http://www.usgs.gov/science/USGSThesaurus/vegetation"/>
    <skos:inScheme rdf:resource="http://www.usgs.gov/science/USGSThesaurus"/>
  </rdf:Description>
  <rdf:Description about="http://www.usgs.gov/science/USGSThesaurus/periphyton">
    <rdf:type rdf:resource="http://www.w3.org/2004/02/skos/core#Concept"/>
    <skos:prefLabel xml:lang="en">periphyton</skos:prefLabel>
    <skos:scopeNote xml:lang="en">A plant assemblage including microbial communities of algae and cyanobacteria living attached to submerged aquatic vegetation.</skos:scopeNote>
    <skos:broader rdf:resource="http://www.usgs.gov/science/USGSThesaurus/vegetation"/>
    <skos:related rdf:resource="http://www.usgs.gov/science/USGSThesaurus/algae"/>
    <skos:inScheme rdf:resource="http://www.usgs.gov/science/USGSThesaurus"/>
  </rdf:Description>
  <rdf:Description about="http://www.usgs.gov/science/USGSThesaurus/weeds">
    <rdf:type rdf:resource="http://www.w3.org/2004/02/skos/core#Concept"/>
    <skos:prefLabel xml:lang="en">weeds</skos:prefLabel>
    <skos:scopeNote xml:lang="en">Plants whose presence in an area is undesirable.</skos:scopeNote>
    <skos:broader rdf:resource="http://www.usgs.gov/science/USGSThesaurus/vegetation"/>
    <skos:inScheme rdf:resource="http://www.usgs.gov/science/USGSThesaurus"/>
  </rdf:Description>
  <rdf:Description about="http://www.usgs.gov/science/USGSThesaurus/wildlife">
    <rdf:type rdf:resource="http://www.w3.org/2004/02/skos/core#Concept"/>
    <skos:prefLabel xml:lang="en">wildlife</skos:prefLabel>
    <skos:scopeNote xml:lang="en">Undomesticated organisms living in natural settings without dependence on man.</skos:scopeNote>
    <skos:broader rdf:resource="http://www.usgs.gov/science/USGSThesaurus/organism%20groupings%20%28non-taxonomic%29"/>
    <skos:related rdf:resource="http://www.usgs.gov/science/USGSThesaurus/animals"/>
    <skos:related rdf:resource="http://www.usgs.gov/science/USGSThesaurus/wildlife%20biology"/>
    <skos:inScheme rdf:resource="http://www.usgs.gov/science/USGSThesaurus"/>
  </rdf:Description>
  <rdf:Description about="http://www.usgs.gov/science/USGSThesaurus/organisms">
    <rdf:type rdf:resource="http://www.w3.org/2004/02/skos/core#Concept"/>
    <skos:prefLabel xml:lang="en">organisms</skos:prefLabel>
    <skos:scopeNote xml:lang="en">Living individuals that grow, reproduce, and die.</skos:scopeNote>
    <skos:altLabel xml:lang="en">biological organisms</skos:altLabel>
    <skos:broader rdf:resource="http://www.usgs.gov/science/USGSThesaurus/topics"/>
    <skos:narrower rdf:resource="http://www.usgs.gov/science/USGSThesaurus/algae"/>
    <skos:narrower rdf:resource="http://www.usgs.gov/science/USGSThesaurus/animals"/>
    <skos:narrower rdf:resource="http://www.usgs.gov/science/USGSThesaurus/archaea"/>
    <skos:narrower rdf:resource="http://www.usgs.gov/science/USGSThesaurus/bacteria"/>
    <skos:narrower rdf:resource="http://www.usgs.gov/science/USGSThesaurus/fungi"/>
    <skos:narrower rdf:resource="http://www.usgs.gov/science/USGSThesaurus/lichens"/>
    <skos:narrower rdf:resource="http://www.usgs.gov/science/USGSThesaurus/plants%20%28organisms%29"/>
    <skos:narrower rdf:resource="http://www.usgs.gov/science/USGSThesaurus/protists"/>
    <skos:narrower rdf:resource="http://www.usgs.gov/science/USGSThesaurus/viruses"/>
    <skos:related rdf:resource="http://www.usgs.gov/science/USGSThesaurus/life%20sciences"/>
    <skos:related rdf:resource="http://www.usgs.gov/science/USGSThesaurus/organism%20groupings%20%28non-taxonomic%29"/>
    <skos:inScheme rdf:resource="http://www.usgs.gov/science/USGSThesaurus"/>
  </rdf:Description>
  <rdf:Description about="http://www.usgs.gov/science/USGSThesaurus/algae">
    <rdf:type rdf:resource="http://www.w3.org/2004/02/skos/core#Concept"/>
    <skos:prefLabel xml:lang="en">algae</skos:prefLabel>
    <skos:scopeNote xml:lang="en">Chlorophyll-bearing primarily aquatic nonvascular species that have no true roots, stems, or leaves; most algae are microscopic, but some species can be as large as vascular plants.</skos:scopeNote>
    <skos:broader rdf:resource="http://www.usgs.gov/science/USGSThesaurus/organisms"/>
    <skos:narrower rdf:resource="http://www.usgs.gov/science/USGSThesaurus/calcareous%20nannoplankton"/>
    <skos:narrower rdf:resource="http://www.usgs.gov/science/USGSThesaurus/diatoms"/>
    <skos:narrower rdf:resource="http://www.usgs.gov/science/USGSThesaurus/dinoflagellates"/>
    <skos:related rdf:resource="http://www.usgs.gov/science/USGSThesaurus/algal%20blooms"/>
    <skos:related rdf:resource="http://www.usgs.gov/science/USGSThesaurus/bacteria"/>
    <skos:related rdf:resource="http://www.usgs.gov/science/USGSThesaurus/phycology"/>
    <skos:related rdf:resource="http://www.usgs.gov/science/USGSThesaurus/protists"/>
    <skos:related rdf:resource="http://www.usgs.gov/science/USGSThesaurus/periphyton"/>
    <skos:inScheme rdf:resource="http://www.usgs.gov/science/USGSThesaurus"/>
  </rdf:Description>
  <rdf:Description about="http://www.usgs.gov/science/USGSThesaurus/calcareous%20nannoplankton">
    <rdf:type rdf:resource="http://www.w3.org/2004/02/skos/core#Concept"/>
    <skos:prefLabel xml:lang="en">calcareous nannoplankton</skos:prefLabel>
    <skos:scopeNote xml:lang="en">Organisms of the kingdom Protista that normally produce coccoliths, microscopic structures of calcite (calcium carbonate), during some phase of their life cycle.</skos:scopeNote>
    <skos:altLabel xml:lang="en">coccoliths</skos:altLabel>
    <skos:broader rdf:resource="http://www.usgs.gov/science/USGSThesaurus/algae"/>
    <skos:related rdf:resource="http://www.usgs.gov/science/USGSThesaurus/micropaleontology"/>
    <skos:related rdf:resource="http://www.usgs.gov/science/USGSThesaurus/phycology"/>
    <skos:related rdf:resource="http://www.usgs.gov/science/USGSThesaurus/plankton"/>
    <skos:related rdf:resource="http://www.usgs.gov/science/USGSThesaurus/phytoplankton"/>
    <skos:inScheme rdf:resource="http://www.usgs.gov/science/USGSThesaurus"/>
  </rdf:Description>
  <rdf:Description about="http://www.usgs.gov/science/USGSThesaurus/diatoms">
    <rdf:type rdf:resource="http://www.w3.org/2004/02/skos/core#Concept"/>
    <skos:prefLabel xml:lang="en">diatoms</skos:prefLabel>
    <skos:scopeNote xml:lang="en">Microscopic, single-celled plants of the class Bacillariophyceae that have siliceous shells called frustules, and which grow in both marine and fresh water.</skos:scopeNote>
    <skos:broader rdf:resource="http://www.usgs.gov/science/USGSThesaurus/algae"/>
    <skos:related rdf:resource="http://www.usgs.gov/science/USGSThesaurus/micropaleontology"/>
    <skos:related rdf:resource="http://www.usgs.gov/science/USGSThesaurus/phycology"/>
    <skos:inScheme rdf:resource="http://www.usgs.gov/science/USGSThesaurus"/>
  </rdf:Description>
  <rdf:Description about="http://www.usgs.gov/science/USGSThesaurus/dinoflagellates">
    <rdf:type rdf:resource="http://www.w3.org/2004/02/skos/core#Concept"/>
    <skos:prefLabel xml:lang="en">dinoflagellates</skos:prefLabel>
    <skos:scopeNote xml:lang="en">Single-celled planktonic organisms, chiefly marine, characterized by twirling motion and whip-like flagella with affinities to both plants and animals.</skos:scopeNote>
    <skos:broader rdf:resource="http://www.usgs.gov/science/USGSThesaurus/algae"/>
    <skos:related rdf:resource="http://www.usgs.gov/science/USGSThesaurus/micropaleontology"/>
    <skos:related rdf:resource="http://www.usgs.gov/science/USGSThesaurus/phycology"/>
    <skos:inScheme rdf:resource="http://www.usgs.gov/science/USGSThesaurus"/>
  </rdf:Description>
  <rdf:Description about="http://www.usgs.gov/science/USGSThesaurus/animals">
    <rdf:type rdf:resource="http://www.w3.org/2004/02/skos/core#Concept"/>
    <skos:prefLabel xml:lang="en">animals</skos:prefLabel>
    <skos:scopeNote xml:lang="en">Multi-celled organisms of the kingdom Animalia with eukaryotic cells (cells with distinct nuclei containing genetic material and bounded by thin membranes) that are heterotrophic (obtaining energy from organic substances produced by other organisms).</skos:scopeNote>
    <skos:altLabel xml:lang="en">fauna</skos:altLabel>
    <skos:broader rdf:resource="http://www.usgs.gov/science/USGSThesaurus/organisms"/>
    <skos:narrower rdf:resource="http://www.usgs.gov/science/USGSThesaurus/invertebrates"/>
    <skos:narrower rdf:resource="http://www.usgs.gov/science/USGSThesaurus/vertebrates"/>
    <skos:related rdf:resource="http://www.usgs.gov/science/USGSThesaurus/wildlife"/>
    <skos:related rdf:resource="http://www.usgs.gov/science/USGSThesaurus/zoology"/>
    <skos:inScheme rdf:resource="http://www.usgs.gov/science/USGSThesaurus"/>
  </rdf:Description>
  <rdf:Description about="http://www.usgs.gov/science/USGSThesaurus/invertebrates">
    <rdf:type rdf:resource="http://www.w3.org/2004/02/skos/core#Concept"/>
    <skos:prefLabel xml:lang="en">invertebrates</skos:prefLabel>
    <skos:scopeNote xml:lang="en">Animals having no backbone or spinal column, such as insects, mollusks, crustaceans, worms, and similar organisms.</skos:scopeNote>
    <skos:broader rdf:resource="http://www.usgs.gov/science/USGSThesaurus/animals"/>
    <skos:narrower rdf:resource="http://www.usgs.gov/science/USGSThesaurus/arthropods"/>
    <skos:narrower rdf:resource="http://www.usgs.gov/science/USGSThesaurus/bryozoans%20and%20brachiopods"/>
    <skos:narrower rdf:resource="http://www.usgs.gov/science/USGSThesaurus/coelenterates"/>
    <skos:narrower rdf:resource="http://www.usgs.gov/science/USGSThesaurus/conodonts"/>
    <skos:narrower rdf:resource="http://www.usgs.gov/science/USGSThesaurus/echinoderms"/>
    <skos:narrower rdf:resource="http://www.usgs.gov/science/USGSThesaurus/mollusks"/>
    <skos:narrower rdf:resource="http://www.usgs.gov/science/USGSThesaurus/sponges"/>
    <skos:narrower rdf:resource="http://www.usgs.gov/science/USGSThesaurus/tunicates"/>
    <skos:narrower rdf:resource="http://www.usgs.gov/science/USGSThesaurus/worms"/>
    <skos:related rdf:resource="http://www.usgs.gov/science/USGSThesaurus/invertebrate%20paleontology"/>
    <skos:related rdf:resource="http://www.usgs.gov/science/USGSThesaurus/invertebrate%20zoology"/>
    <skos:inScheme rdf:resource="http://www.usgs.gov/science/USGSThesaurus"/>
  </rdf:Description>
  <rdf:Description about="http://www.usgs.gov/science/USGSThesaurus/arthropods">
    <rdf:type rdf:resource="http://www.w3.org/2004/02/skos/core#Concept"/>
    <skos:prefLabel xml:lang="en">arthropods</skos:prefLabel>
    <skos:scopeNote xml:lang="en">Invertebrates belonging to the largest phylum of animals, Arthropoda, with an exoskeleton, segmented bodies, and jointed appendages, including many subphyla and classes, such as insects, crustaceans, horseshoe crabs, sea spiders, centipedes, millipedes, and the extinct trilobites.</skos:scopeNote>
    <skos:broader rdf:resource="http://www.usgs.gov/science/USGSThesaurus/invertebrates"/>
    <skos:narrower rdf:resource="http://www.usgs.gov/science/USGSThesaurus/arachnids"/>
    <skos:narrower rdf:resource="http://www.usgs.gov/science/USGSThesaurus/crustaceans"/>
    <skos:narrower rdf:resource="http://www.usgs.gov/science/USGSThesaurus/horseshoe%20crabs"/>
    <skos:narrower rdf:resource="http://www.usgs.gov/science/USGSThesaurus/insects"/>
    <skos:narrower rdf:resource="http://www.usgs.gov/science/USGSThesaurus/trilobites"/>
    <skos:related rdf:resource="http://www.usgs.gov/science/USGSThesaurus/invertebrate%20zoology"/>
    <skos:inScheme rdf:resource="http://www.usgs.gov/science/USGSThesaurus"/>
  </rdf:Description>
  <rdf:Description about="http://www.usgs.gov/science/USGSThesaurus/arachnids">
    <rdf:type rdf:resource="http://www.w3.org/2004/02/skos/core#Concept"/>
    <skos:prefLabel xml:lang="en">arachnids</skos:prefLabel>
    <skos:scopeNote xml:lang="en">Carnivorous arthropods, chiefly terrestrial, of the class Arachnida including spiders, scorpions, mites, ticks, false scorpions, palpigrades, solifugids, and harvestmen.</skos:scopeNote>
    <skos:altLabel xml:lang="en">false scorpions</skos:altLabel>
    <skos:altLabel xml:lang="en">mites</skos:altLabel>
    <skos:altLabel xml:lang="en">spiders</skos:altLabel>
    <skos:altLabel xml:lang="en">ticks</skos:altLabel>
    <skos:broader rdf:resource="http://www.usgs.gov/science/USGSThesaurus/arthropods"/>
    <skos:related rdf:resource="http://www.usgs.gov/science/USGSThesaurus/entomology"/>
    <skos:related rdf:resource="http://www.usgs.gov/science/USGSThesaurus/invertebrate%20zoology"/>
    <skos:inScheme rdf:resource="http://www.usgs.gov/science/USGSThesaurus"/>
  </rdf:Description>
  <rdf:Description about="http://www.usgs.gov/science/USGSThesaurus/crustaceans">
    <rdf:type rdf:resource="http://www.w3.org/2004/02/skos/core#Concept"/>
    <skos:prefLabel xml:lang="en">crustaceans</skos:prefLabel>
    <skos:scopeNote xml:lang="en">Arthropods of class Crustacea, such as crabs, lobsters, shrimp, prawns, or barnacles, with hard shells (exoskeleton) and segmented bodies with pairs of jointed appendages.</skos:scopeNote>
    <skos:broader rdf:resource="http://www.usgs.gov/science/USGSThesaurus/arthropods"/>
    <skos:narrower rdf:resource="http://www.usgs.gov/science/USGSThesaurus/ostracodes"/>
    <skos:related rdf:resource="http://www.usgs.gov/science/USGSThesaurus/invertebrate%20zoology"/>
    <skos:related rdf:resource="http://www.usgs.gov/science/USGSThesaurus/shellfish"/>
    <skos:inScheme rdf:resource="http://www.usgs.gov/science/USGSThesaurus"/>
  </rdf:Description>
  <rdf:Description about="http://www.usgs.gov/science/USGSThesaurus/ostracodes">
    <rdf:type rdf:resource="http://www.w3.org/2004/02/skos/core#Concept"/>
    <skos:prefLabel xml:lang="en">ostracodes</skos:prefLabel>
    <skos:scopeNote xml:lang="en">Small aquatic crustaceans belonging to the subclass Ostracoda, characterized by a bivalve shell.</skos:scopeNote>
    <skos:altLabel xml:lang="en">Ostracoda</skos:altLabel>
    <skos:altLabel xml:lang="en">ostracods</skos:altLabel>
    <skos:broader rdf:resource="http://www.usgs.gov/science/USGSThesaurus/crustaceans"/>
    <skos:related rdf:resource="http://www.usgs.gov/science/USGSThesaurus/invertebrate%20zoology"/>
    <skos:inScheme rdf:resource="http://www.usgs.gov/science/USGSThesaurus"/>
  </rdf:Description>
  <rdf:Description about="http://www.usgs.gov/science/USGSThesaurus/horseshoe%20crabs">
    <rdf:type rdf:resource="http://www.w3.org/2004/02/skos/core#Concept"/>
    <skos:prefLabel xml:lang="en">horseshoe crabs</skos:prefLabel>
    <skos:scopeNote xml:lang="en">Marine arthropods, usually classed as Merostomata, which have a broad crescent (horseshoe-shaped) cephalothorax.</skos:scopeNote>
    <skos:broader rdf:resource="http://www.usgs.gov/science/USGSThesaurus/arthropods"/>
    <skos:related rdf:resource="http://www.usgs.gov/science/USGSThesaurus/invertebrate%20zoology"/>
    <skos:inScheme rdf:resource="http://www.usgs.gov/science/USGSThesaurus"/>
  </rdf:Description>
  <rdf:Description about="http://www.usgs.gov/science/USGSThesaurus/insects">
    <rdf:type rdf:resource="http://www.w3.org/2004/02/skos/core#Concept"/>
    <skos:prefLabel xml:lang="en">insects</skos:prefLabel>
    <skos:scopeNote xml:lang="en">Small arthropod animals of the class Insecta with bodies in 3 segments (head, thorax, and abdomen). They have 3 pairs of legs, 2 antennae, and usually one or two pairs of wings. Includes flies, mosquitoes, beetles, butterflies, bees, crickets, and dragonflies.</skos:scopeNote>
    <skos:altLabel xml:lang="en">bugs</skos:altLabel>
    <skos:broader rdf:resource="http://www.usgs.gov/science/USGSThesaurus/arthropods"/>
    <skos:narrower rdf:resource="http://www.usgs.gov/science/USGSThesaurus/bees%20and%20wasps"/>
    <skos:narrower rdf:resource="http://www.usgs.gov/science/USGSThesaurus/butterflies%20and%20moths"/>
    <skos:related rdf:resource="http://www.usgs.gov/science/USGSThesaurus/entomology"/>
    <skos:inScheme rdf:resource="http://www.usgs.gov/science/USGSThesaurus"/>
  </rdf:Description>
  <rdf:Description about="http://www.usgs.gov/science/USGSThesaurus/bees%20and%20wasps">
    <rdf:type rdf:resource="http://www.w3.org/2004/02/skos/core#Concept"/>
    <skos:prefLabel xml:lang="en">bees and wasps</skos:prefLabel>
    <skos:scopeNote xml:lang="en"></skos:scopeNote>
    <skos:altLabel xml:lang="en">wasps</skos:altLabel>
    <skos:altLabel xml:lang="en">bees</skos:altLabel>
    <skos:broader rdf:resource="http://www.usgs.gov/science/USGSThesaurus/insects"/>
    <skos:inScheme rdf:resource="http://www.usgs.gov/science/USGSThesaurus"/>
  </rdf:Description>
  <rdf:Description about="http://www.usgs.gov/science/USGSThesaurus/butterflies%20and%20moths">
    <rdf:type rdf:resource="http://www.w3.org/2004/02/skos/core#Concept"/>
    <skos:prefLabel xml:lang="en">butterflies and moths</skos:prefLabel>
    <skos:scopeNote xml:lang="en">Insects of the order Lepidoptera that have four wings with overlapping, often highly colored scales. They undergo four life cycle stages: eggs, caterpillar larvae, pupae, and the winged adults.</skos:scopeNote>
    <skos:altLabel xml:lang="en">lepidoptera</skos:altLabel>
    <skos:altLabel xml:lang="en">moths</skos:altLabel>
    <skos:broader rdf:resource="http://www.usgs.gov/science/USGSThesaurus/insects"/>
    <skos:related rdf:resource="http://www.usgs.gov/science/USGSThesaurus/entomology"/>
    <skos:inScheme rdf:resource="http://www.usgs.gov/science/USGSThesaurus"/>
  </rdf:Description>
  <rdf:Description about="http://www.usgs.gov/science/USGSThesaurus/trilobites">
    <rdf:type rdf:resource="http://www.w3.org/2004/02/skos/core#Concept"/>
    <skos:prefLabel xml:lang="en">trilobites</skos:prefLabel>
    <skos:scopeNote xml:lang="en">Extinct marine arthropods of the class Trilobita with segmented bodies and jointed appendages found as Paleozoic fossils in many parts of the world.</skos:scopeNote>
    <skos:broader rdf:resource="http://www.usgs.gov/science/USGSThesaurus/arthropods"/>
    <skos:related rdf:resource="http://www.usgs.gov/science/USGSThesaurus/fossils"/>
    <skos:related rdf:resource="http://www.usgs.gov/science/USGSThesaurus/invertebrate%20paleontology"/>
    <skos:inScheme rdf:resource="http://www.usgs.gov/science/USGSThesaurus"/>
  </rdf:Description>
  <rdf:Description about="http://www.usgs.gov/science/USGSThesaurus/bryozoans%20and%20brachiopods">
    <rdf:type rdf:resource="http://www.w3.org/2004/02/skos/core#Concept"/>
    <skos:prefLabel xml:lang="en">bryozoans and brachiopods</skos:prefLabel>
    <skos:scopeNote xml:lang="en">Aquatic invertebrates, usually marine, belonging to the phyla Bryozoa and Brachiopoda.  Brachiopods, or clam shells, are solitary living invertebrates characterized by two shells and a lophophore, which is a complex food gathering organ.  Bryozoans are colonial and include moss coral and moss polyps.</skos:scopeNote>
    <skos:altLabel xml:lang="en">brachiopods</skos:altLabel>
    <skos:altLabel xml:lang="en">ectoprocta</skos:altLabel>
    <skos:broader rdf:resource="http://www.usgs.gov/science/USGSThesaurus/invertebrates"/>
    <skos:related rdf:resource="http://www.usgs.gov/science/USGSThesaurus/invertebrate%20paleontology"/>
    <skos:related rdf:resource="http://www.usgs.gov/science/USGSThesaurus/invertebrate%20zoology"/>
    <skos:inScheme rdf:resource="http://www.usgs.gov/science/USGSThesaurus"/>
  </rdf:Description>
  <rdf:Description about="http://www.usgs.gov/science/USGSThesaurus/coelenterates">
    <rdf:type rdf:resource="http://www.w3.org/2004/02/skos/core#Concept"/>
    <skos:prefLabel xml:lang="en">coelenterates</skos:prefLabel>
    <skos:scopeNote xml:lang="en">Freshwater and marine invertebrates, such as corals, jellyfish, and sea anemones, belonging to the phylum Coelenterata and living as sedentary polyps or free swimming medusae.</skos:scopeNote>
    <skos:altLabel xml:lang="en">corals</skos:altLabel>
    <skos:altLabel xml:lang="en">jellyfish</skos:altLabel>
    <skos:altLabel xml:lang="en">sea anemones</skos:altLabel>
    <skos:broader rdf:resource="http://www.usgs.gov/science/USGSThesaurus/invertebrates"/>
    <skos:related rdf:resource="http://www.usgs.gov/science/USGSThesaurus/invertebrate%20zoology"/>
    <skos:related rdf:resource="http://www.usgs.gov/science/USGSThesaurus/reef%20ecosystems"/>
    <skos:inScheme rdf:resource="http://www.usgs.gov/science/USGSThesaurus"/>
  </rdf:Description>
  <rdf:Description about="http://www.usgs.gov/science/USGSThesaurus/conodonts">
    <rdf:type rdf:resource="http://www.w3.org/2004/02/skos/core#Concept"/>
    <skos:prefLabel xml:lang="en">conodonts</skos:prefLabel>
    <skos:scopeNote xml:lang="en">Microscopic teeth of primitive, boneless, eel-like animals, similar to modern hagfish, that lived in many of the world's oceans from the Cambrian through Triassic Periods of geologic time (550 to 210 million years ago).</skos:scopeNote>
    <skos:broader rdf:resource="http://www.usgs.gov/science/USGSThesaurus/invertebrates"/>
    <skos:related rdf:resource="http://www.usgs.gov/science/USGSThesaurus/invertebrate%20paleontology"/>
    <skos:related rdf:resource="http://www.usgs.gov/science/USGSThesaurus/micropaleontology"/>
    <skos:inScheme rdf:resource="http://www.usgs.gov/science/USGSThesaurus"/>
  </rdf:Description>
  <rdf:Description about="http://www.usgs.gov/science/USGSThesaurus/echinoderms">
    <rdf:type rdf:resource="http://www.w3.org/2004/02/skos/core#Concept"/>
    <skos:prefLabel xml:lang="en">echinoderms</skos:prefLabel>
    <skos:scopeNote xml:lang="en">Marine invertebrates of the phylum Echinodermata with a radial body and a calcareous exoskeleton. Includes starfishes, brittle stars, sea lilies, sea urchins, and sea cucumbers.</skos:scopeNote>
    <skos:broader rdf:resource="http://www.usgs.gov/science/USGSThesaurus/invertebrates"/>
    <skos:related rdf:resource="http://www.usgs.gov/science/USGSThesaurus/invertebrate%20zoology"/>
    <skos:inScheme rdf:resource="http://www.usgs.gov/science/USGSThesaurus"/>
  </rdf:Description>
  <rdf:Description about="http://www.usgs.gov/science/USGSThesaurus/mollusks">
    <rdf:type rdf:resource="http://www.w3.org/2004/02/skos/core#Concept"/>
    <skos:prefLabel xml:lang="en">mollusks</skos:prefLabel>
    <skos:scopeNote xml:lang="en">Invertebrates belonging to the phylum Mollusca with soft, nonsegmented bodies, often covered by a hard shell.  Includes snails, clams, oysters, whelks, mussels, slugs, octopuses, and squids.</skos:scopeNote>
    <skos:altLabel xml:lang="en">molluscs</skos:altLabel>
    <skos:broader rdf:resource="http://www.usgs.gov/science/USGSThesaurus/invertebrates"/>
    <skos:related rdf:resource="http://www.usgs.gov/science/USGSThesaurus/invertebrate%20zoology"/>
    <skos:related rdf:resource="http://www.usgs.gov/science/USGSThesaurus/shellfish"/>
    <skos:inScheme rdf:resource="http://www.usgs.gov/science/USGSThesaurus"/>
  </rdf:Description>
  <rdf:Description about="http://www.usgs.gov/science/USGSThesaurus/sponges">
    <rdf:type rdf:resource="http://www.w3.org/2004/02/skos/core#Concept"/>
    <skos:prefLabel xml:lang="en">sponges</skos:prefLabel>
    <skos:scopeNote xml:lang="en">Aquatic invertebrates belonging to the phylum Porifera having internal skeletons of silica or collagen, porous body around a cavity or cavities, and usually living in stationary communities.</skos:scopeNote>
    <skos:broader rdf:resource="http://www.usgs.gov/science/USGSThesaurus/invertebrates"/>
    <skos:related rdf:resource="http://www.usgs.gov/science/USGSThesaurus/invertebrate%20zoology"/>
    <skos:inScheme rdf:resource="http://www.usgs.gov/science/USGSThesaurus"/>
  </rdf:Description>
  <rdf:Description about="http://www.usgs.gov/science/USGSThesaurus/tunicates">
    <rdf:type rdf:resource="http://www.w3.org/2004/02/skos/core#Concept"/>
    <skos:prefLabel xml:lang="en">tunicates</skos:prefLabel>
    <skos:scopeNote xml:lang="en">Marine organisms of the subphylum tunicata of the phylum chordata.</skos:scopeNote>
    <skos:altLabel xml:lang="en">sea squirts</skos:altLabel>
    <skos:altLabel xml:lang="en">urochordates</skos:altLabel>
    <skos:broader rdf:resource="http://www.usgs.gov/science/USGSThesaurus/invertebrates"/>
    <skos:inScheme rdf:resource="http://www.usgs.gov/science/USGSThesaurus"/>
  </rdf:Description>
  <rdf:Description about="http://www.usgs.gov/science/USGSThesaurus/worms">
    <rdf:type rdf:resource="http://www.w3.org/2004/02/skos/core#Concept"/>
    <skos:prefLabel xml:lang="en">worms</skos:prefLabel>
    <skos:scopeNote xml:lang="en">Invertebrate animals of the phyla Annelida, Nematoda, Memertea, or Plathyhelminthes, that have long thin rounded or flat bodies without obvious appendages.</skos:scopeNote>
    <skos:broader rdf:resource="http://www.usgs.gov/science/USGSThesaurus/invertebrates"/>
    <skos:narrower rdf:resource="http://www.usgs.gov/science/USGSThesaurus/flatworms"/>
    <skos:narrower rdf:resource="http://www.usgs.gov/science/USGSThesaurus/roundworms"/>
    <skos:narrower rdf:resource="http://www.usgs.gov/science/USGSThesaurus/segmented%20worms"/>
    <skos:related rdf:resource="http://www.usgs.gov/science/USGSThesaurus/invertebrate%20zoology"/>
    <skos:inScheme rdf:resource="http://www.usgs.gov/science/USGSThesaurus"/>
  </rdf:Description>
  <rdf:Description about="http://www.usgs.gov/science/USGSThesaurus/flatworms">
    <rdf:type rdf:resource="http://www.w3.org/2004/02/skos/core#Concept"/>
    <skos:prefLabel xml:lang="en">flatworms</skos:prefLabel>
    <skos:scopeNote xml:lang="en">Soft flat worms of the phylum Platyhelminthes, which are often parasitic. Includes tapeworms and flukes.</skos:scopeNote>
    <skos:broader rdf:resource="http://www.usgs.gov/science/USGSThesaurus/worms"/>
    <skos:related rdf:resource="http://www.usgs.gov/science/USGSThesaurus/invertebrate%20zoology"/>
    <skos:inScheme rdf:resource="http://www.usgs.gov/science/USGSThesaurus"/>
  </rdf:Description>
  <rdf:Description about="http://www.usgs.gov/science/USGSThesaurus/roundworms">
    <rdf:type rdf:resource="http://www.w3.org/2004/02/skos/core#Concept"/>
    <skos:prefLabel xml:lang="en">roundworms</skos:prefLabel>
    <skos:scopeNote xml:lang="en">Worms of the phylum Nematoda, often parasitic, such as hookworms and pinworms, having soft cylindrical bodies without segments.</skos:scopeNote>
    <skos:altLabel xml:lang="en">nematodes</skos:altLabel>
    <skos:broader rdf:resource="http://www.usgs.gov/science/USGSThesaurus/worms"/>
    <skos:related rdf:resource="http://www.usgs.gov/science/USGSThesaurus/invertebrate%20zoology"/>
    <skos:inScheme rdf:resource="http://www.usgs.gov/science/USGSThesaurus"/>
  </rdf:Description>
  <rdf:Description about="http://www.usgs.gov/science/USGSThesaurus/segmented%20worms">
    <rdf:type rdf:resource="http://www.w3.org/2004/02/skos/core#Concept"/>
    <skos:prefLabel xml:lang="en">segmented worms</skos:prefLabel>
    <skos:scopeNote xml:lang="en">Worms belonging to the phylum Annelida, with soft bodies divided into segments and distinct heads. Includes leeches, earthworms, and marine worms.</skos:scopeNote>
    <skos:altLabel xml:lang="en">annelids</skos:altLabel>
    <skos:broader rdf:resource="http://www.usgs.gov/science/USGSThesaurus/worms"/>
    <skos:related rdf:resource="http://www.usgs.gov/science/USGSThesaurus/invertebrate%20zoology"/>
    <skos:inScheme rdf:resource="http://www.usgs.gov/science/USGSThesaurus"/>
  </rdf:Description>
  <rdf:Description about="http://www.usgs.gov/science/USGSThesaurus/vertebrates">
    <rdf:type rdf:resource="http://www.w3.org/2004/02/skos/core#Concept"/>
    <skos:prefLabel xml:lang="en">vertebrates</skos:prefLabel>
    <skos:scopeNote xml:lang="en">Animals possessing a vertebral column or backbone including birds, fishes, amphibians, reptiles, and mammals.</skos:scopeNote>
    <skos:broader rdf:resource="http://www.usgs.gov/science/USGSThesaurus/animals"/>
    <skos:narrower rdf:resource="http://www.usgs.gov/science/USGSThesaurus/amphibians"/>
    <skos:narrower rdf:resource="http://www.usgs.gov/science/USGSThesaurus/birds"/>
    <skos:narrower rdf:resource="http://www.usgs.gov/science/USGSThesaurus/fish"/>
    <skos:narrower rdf:resource="http://www.usgs.gov/science/USGSThesaurus/mammals"/>
    <skos:narrower rdf:resource="http://www.usgs.gov/science/USGSThesaurus/reptiles"/>
    <skos:related rdf:resource="http://www.usgs.gov/science/USGSThesaurus/vertebrate%20paleontology"/>
    <skos:related rdf:resource="http://www.usgs.gov/science/USGSThesaurus/vertebrate%20zoology"/>
    <skos:inScheme rdf:resource="http://www.usgs.gov/science/USGSThesaurus"/>
  </rdf:Description>
  <rdf:Description about="http://www.usgs.gov/science/USGSThesaurus/amphibians">
    <rdf:type rdf:resource="http://www.w3.org/2004/02/skos/core#Concept"/>
    <skos:prefLabel xml:lang="en">amphibians</skos:prefLabel>
    <skos:scopeNote xml:lang="en">Vertebrates of the class Amphibia including frogs and toads (Anura), salamanders (Urodela), caecilians (Apoda) and extinct forms which are cold-blooded and have life stages in water as eggs and larval forms (tadpoles)until they metamorphose as adults.</skos:scopeNote>
    <skos:broader rdf:resource="http://www.usgs.gov/science/USGSThesaurus/vertebrates"/>
    <skos:related rdf:resource="http://www.usgs.gov/science/USGSThesaurus/herpetology"/>
    <skos:inScheme rdf:resource="http://www.usgs.gov/science/USGSThesaurus"/>
  </rdf:Description>
  <rdf:Description about="http://www.usgs.gov/science/USGSThesaurus/birds">
    <rdf:type rdf:resource="http://www.w3.org/2004/02/skos/core#Concept"/>
    <skos:prefLabel xml:lang="en">birds</skos:prefLabel>
    <skos:scopeNote xml:lang="en">Land vertebrates belonging to the class Aves with warm blood, feathers, wings, and reproduction characterized by egg laying.</skos:scopeNote>
    <skos:altLabel xml:lang="en">shorebirds</skos:altLabel>
    <skos:altLabel xml:lang="en">water birds</skos:altLabel>
    <skos:altLabel xml:lang="en">waterfowl</skos:altLabel>
    <skos:broader rdf:resource="http://www.usgs.gov/science/USGSThesaurus/vertebrates"/>
    <skos:related rdf:resource="http://www.usgs.gov/science/USGSThesaurus/ornithology"/>
    <skos:inScheme rdf:resource="http://www.usgs.gov/science/USGSThesaurus"/>
  </rdf:Description>
  <rdf:Description about="http://www.usgs.gov/science/USGSThesaurus/fish">
    <rdf:type rdf:resource="http://www.w3.org/2004/02/skos/core#Concept"/>
    <skos:prefLabel xml:lang="en">fish</skos:prefLabel>
    <skos:scopeNote xml:lang="en">Cold-blooded aquatic vertebrates with fins for swimming, gills for breathing, and usually scales.</skos:scopeNote>
    <!--FOR fish inventories USE fish WITH field sampling-->
    <skos:altLabel xml:lang="en">fish inventories</skos:altLabel>
    <skos:altLabel xml:lang="en">fishes</skos:altLabel>
    <!--FOR anadromous fish USE fish WITH migratory species-->
    <skos:altLabel xml:lang="en">anadromous fish</skos:altLabel>
    <!--FOR diadromous fish USE fish WITH migratory species-->
    <skos:altLabel xml:lang="en">diadromous fish</skos:altLabel>
    <skos:broader rdf:resource="http://www.usgs.gov/science/USGSThesaurus/vertebrates"/>
    <skos:related rdf:resource="http://www.usgs.gov/science/USGSThesaurus/ichthyology"/>
    <skos:inScheme rdf:resource="http://www.usgs.gov/science/USGSThesaurus"/>
  </rdf:Description>
  <rdf:Description about="http://www.usgs.gov/science/USGSThesaurus/mammals">
    <rdf:type rdf:resource="http://www.w3.org/2004/02/skos/core#Concept"/>
    <skos:prefLabel xml:lang="en">mammals</skos:prefLabel>
    <skos:scopeNote xml:lang="en">Vertebrate animals, generally large, with skin covered by hair and large brain cavities.  Females have mammary glands for feeding the young, who are usually born quite mature.</skos:scopeNote>
    <skos:broader rdf:resource="http://www.usgs.gov/science/USGSThesaurus/vertebrates"/>
    <skos:narrower rdf:resource="http://www.usgs.gov/science/USGSThesaurus/bats"/>
    <skos:narrower rdf:resource="http://www.usgs.gov/science/USGSThesaurus/bears"/>
    <skos:narrower rdf:resource="http://www.usgs.gov/science/USGSThesaurus/walruses"/>
    <skos:related rdf:resource="http://www.usgs.gov/science/USGSThesaurus/mammalogy"/>
    <skos:inScheme rdf:resource="http://www.usgs.gov/science/USGSThesaurus"/>
  </rdf:Description>
  <rdf:Description about="http://www.usgs.gov/science/USGSThesaurus/bats">
    <rdf:type rdf:resource="http://www.w3.org/2004/02/skos/core#Concept"/>
    <skos:prefLabel xml:lang="en">bats</skos:prefLabel>
    <skos:scopeNote xml:lang="en">Small flying mammals of the order Chiroptera.</skos:scopeNote>
    <skos:broader rdf:resource="http://www.usgs.gov/science/USGSThesaurus/mammals"/>
    <skos:inScheme rdf:resource="http://www.usgs.gov/science/USGSThesaurus"/>
  </rdf:Description>
  <rdf:Description about="http://www.usgs.gov/science/USGSThesaurus/bears">
    <rdf:type rdf:resource="http://www.w3.org/2004/02/skos/core#Concept"/>
    <skos:prefLabel xml:lang="en">bears</skos:prefLabel>
    <skos:scopeNote xml:lang="en">Large wild mammals of the family Ursidae.  Includes black and brown (grizzly) bears and polar bears.</skos:scopeNote>
    <skos:altLabel xml:lang="en">polar bears</skos:altLabel>
    <skos:altLabel xml:lang="en">grizzly bears</skos:altLabel>
    <skos:altLabel xml:lang="en">black bears</skos:altLabel>
    <skos:broader rdf:resource="http://www.usgs.gov/science/USGSThesaurus/mammals"/>
    <skos:inScheme rdf:resource="http://www.usgs.gov/science/USGSThesaurus"/>
  </rdf:Description>
  <rdf:Description about="http://www.usgs.gov/science/USGSThesaurus/walruses">
    <rdf:type rdf:resource="http://www.w3.org/2004/02/skos/core#Concept"/>
    <skos:prefLabel xml:lang="en">walruses</skos:prefLabel>
    <skos:scopeNote xml:lang="en"></skos:scopeNote>
    <skos:altLabel xml:lang="en">walrus</skos:altLabel>
    <skos:broader rdf:resource="http://www.usgs.gov/science/USGSThesaurus/mammals"/>
    <skos:inScheme rdf:resource="http://www.usgs.gov/science/USGSThesaurus"/>
  </rdf:Description>
  <rdf:Description about="http://www.usgs.gov/science/USGSThesaurus/reptiles">
    <rdf:type rdf:resource="http://www.w3.org/2004/02/skos/core#Concept"/>
    <skos:prefLabel xml:lang="en">reptiles</skos:prefLabel>
    <skos:scopeNote xml:lang="en">Cold-blooded vertebrates of the class Reptilia.  Characterized by skin covered with scales or horny plates and reproduced by eggs. Includes snakes, lizards, crocodiles, alligators, turtles, and extinct species such as dinosaurs.</skos:scopeNote>
    <skos:broader rdf:resource="http://www.usgs.gov/science/USGSThesaurus/vertebrates"/>
    <skos:narrower rdf:resource="http://www.usgs.gov/science/USGSThesaurus/dinosaurs"/>
    <skos:related rdf:resource="http://www.usgs.gov/science/USGSThesaurus/herpetology"/>
    <skos:inScheme rdf:resource="http://www.usgs.gov/science/USGSThesaurus"/>
  </rdf:Description>
  <rdf:Description about="http://www.usgs.gov/science/USGSThesaurus/dinosaurs">
    <rdf:type rdf:resource="http://www.w3.org/2004/02/skos/core#Concept"/>
    <skos:prefLabel xml:lang="en">dinosaurs</skos:prefLabel>
    <skos:scopeNote xml:lang="en">Extinct reptiles, often gigantic, chiefly terrestrial, carnivorous or herbivorous, that lived during the Mesozoic era.</skos:scopeNote>
    <skos:broader rdf:resource="http://www.usgs.gov/science/USGSThesaurus/reptiles"/>
    <skos:related rdf:resource="http://www.usgs.gov/science/USGSThesaurus/vertebrate%20paleontology"/>
    <skos:inScheme rdf:resource="http://www.usgs.gov/science/USGSThesaurus"/>
  </rdf:Description>
  <rdf:Description about="http://www.usgs.gov/science/USGSThesaurus/archaea">
    <rdf:type rdf:resource="http://www.w3.org/2004/02/skos/core#Concept"/>
    <skos:prefLabel xml:lang="en">archaea</skos:prefLabel>
    <skos:scopeNote xml:lang="en">Microscopic organisms of the domain Archaea living on a diet of hydrogen and carbon dioxide, once thought to be bacteria, and often inhabiting extreme environments, such as thermal vents and hot springs, extremely alkaline and acidic waters, hypersaline water, and anoxic habitats.</skos:scopeNote>
    <skos:altLabel xml:lang="en">archaebacteria</skos:altLabel>
    <skos:broader rdf:resource="http://www.usgs.gov/science/USGSThesaurus/organisms"/>
    <skos:related rdf:resource="http://www.usgs.gov/science/USGSThesaurus/microbiology"/>
    <skos:inScheme rdf:resource="http://www.usgs.gov/science/USGSThesaurus"/>
  </rdf:Description>
  <rdf:Description about="http://www.usgs.gov/science/USGSThesaurus/bacteria">
    <rdf:type rdf:resource="http://www.w3.org/2004/02/skos/core#Concept"/>
    <skos:prefLabel xml:lang="en">bacteria</skos:prefLabel>
    <skos:scopeNote xml:lang="en">Single celled microorganisms, beneficial or pathogenic, without a nuclear membrane.</skos:scopeNote>
    <skos:broader rdf:resource="http://www.usgs.gov/science/USGSThesaurus/organisms"/>
    <skos:related rdf:resource="http://www.usgs.gov/science/USGSThesaurus/algae"/>
    <skos:related rdf:resource="http://www.usgs.gov/science/USGSThesaurus/microbiology"/>
    <skos:inScheme rdf:resource="http://www.usgs.gov/science/USGSThesaurus"/>
  </rdf:Description>
  <rdf:Description about="http://www.usgs.gov/science/USGSThesaurus/fungi">
    <rdf:type rdf:resource="http://www.w3.org/2004/02/skos/core#Concept"/>
    <skos:prefLabel xml:lang="en">fungi</skos:prefLabel>
    <skos:scopeNote xml:lang="en">Immobile organisms of the kingdom Fungi that lack chlorophyll and that obtain nutrients from other dead or living organisms. Fungi reproduce by spores and include yeasts, molds, smuts, and mushrooms.</skos:scopeNote>
    <skos:broader rdf:resource="http://www.usgs.gov/science/USGSThesaurus/organisms"/>
    <skos:related rdf:resource="http://www.usgs.gov/science/USGSThesaurus/mycology"/>
    <skos:inScheme rdf:resource="http://www.usgs.gov/science/USGSThesaurus"/>
  </rdf:Description>
  <rdf:Description about="http://www.usgs.gov/science/USGSThesaurus/lichens">
    <rdf:type rdf:resource="http://www.w3.org/2004/02/skos/core#Concept"/>
    <skos:prefLabel xml:lang="en">lichens</skos:prefLabel>
    <skos:scopeNote xml:lang="en">Plants that are composed of a fungus and an alga growing together symbiotically and often found growing on rocks or tree trunks.</skos:scopeNote>
    <skos:broader rdf:resource="http://www.usgs.gov/science/USGSThesaurus/organisms"/>
    <skos:related rdf:resource="http://www.usgs.gov/science/USGSThesaurus/mycology"/>
    <skos:related rdf:resource="http://www.usgs.gov/science/USGSThesaurus/phycology"/>
    <skos:inScheme rdf:resource="http://www.usgs.gov/science/USGSThesaurus"/>
  </rdf:Description>
  <rdf:Description about="http://www.usgs.gov/science/USGSThesaurus/plants%20%28organisms%29">
    <rdf:type rdf:resource="http://www.w3.org/2004/02/skos/core#Concept"/>
    <skos:prefLabel xml:lang="en">plants (organisms)</skos:prefLabel>
    <skos:scopeNote xml:lang="en">Organisms which belong to the plant kingdom. Commonly multicellular, they produce food through photosynthesis.</skos:scopeNote>
    <skos:altLabel xml:lang="en">flora</skos:altLabel>
    <skos:broader rdf:resource="http://www.usgs.gov/science/USGSThesaurus/organisms"/>
    <skos:narrower rdf:resource="http://www.usgs.gov/science/USGSThesaurus/nonvascular%20plants"/>
    <skos:narrower rdf:resource="http://www.usgs.gov/science/USGSThesaurus/vascular%20plants"/>
    <skos:related rdf:resource="http://www.usgs.gov/science/USGSThesaurus/botany"/>
    <skos:related rdf:resource="http://www.usgs.gov/science/USGSThesaurus/palynology"/>
    <skos:related rdf:resource="http://www.usgs.gov/science/USGSThesaurus/vegetation"/>
    <skos:inScheme rdf:resource="http://www.usgs.gov/science/USGSThesaurus"/>
  </rdf:Description>
  <rdf:Description about="http://www.usgs.gov/science/USGSThesaurus/nonvascular%20plants">
    <rdf:type rdf:resource="http://www.w3.org/2004/02/skos/core#Concept"/>
    <skos:prefLabel xml:lang="en">nonvascular plants</skos:prefLabel>
    <skos:scopeNote xml:lang="en">Simple plants which lack conducting tissues known as vascular bundles, a group of specialized cells made up of xylem and phloem.</skos:scopeNote>
    <skos:altLabel xml:lang="en">non-vascular plants</skos:altLabel>
    <skos:broader rdf:resource="http://www.usgs.gov/science/USGSThesaurus/plants%20%28organisms%29"/>
    <skos:narrower rdf:resource="http://www.usgs.gov/science/USGSThesaurus/liverworts%20and%20hornworts"/>
    <skos:narrower rdf:resource="http://www.usgs.gov/science/USGSThesaurus/mosses"/>
    <skos:related rdf:resource="http://www.usgs.gov/science/USGSThesaurus/botany"/>
    <skos:inScheme rdf:resource="http://www.usgs.gov/science/USGSThesaurus"/>
  </rdf:Description>
  <rdf:Description about="http://www.usgs.gov/science/USGSThesaurus/liverworts%20and%20hornworts">
    <rdf:type rdf:resource="http://www.w3.org/2004/02/skos/core#Concept"/>
    <skos:prefLabel xml:lang="en">liverworts and hornworts</skos:prefLabel>
    <skos:scopeNote xml:lang="en">Simple green land plants of the phyla Bryophyta with leaves and a stem and always without roots.</skos:scopeNote>
    <skos:broader rdf:resource="http://www.usgs.gov/science/USGSThesaurus/nonvascular%20plants"/>
    <skos:related rdf:resource="http://www.usgs.gov/science/USGSThesaurus/botany"/>
    <skos:related rdf:resource="http://www.usgs.gov/science/USGSThesaurus/mosses"/>
    <skos:inScheme rdf:resource="http://www.usgs.gov/science/USGSThesaurus"/>
  </rdf:Description>
  <rdf:Description about="http://www.usgs.gov/science/USGSThesaurus/mosses">
    <rdf:type rdf:resource="http://www.w3.org/2004/02/skos/core#Concept"/>
    <skos:prefLabel xml:lang="en">mosses</skos:prefLabel>
    <skos:scopeNote xml:lang="en">Simple green land plants, member of the phyla Bryophyta, along with liverworts and hornworts.  They have leaves and a stem, but always lack roots.</skos:scopeNote>
    <skos:broader rdf:resource="http://www.usgs.gov/science/USGSThesaurus/nonvascular%20plants"/>
    <skos:related rdf:resource="http://www.usgs.gov/science/USGSThesaurus/botany"/>
    <skos:related rdf:resource="http://www.usgs.gov/science/USGSThesaurus/liverworts%20and%20hornworts"/>
    <skos:inScheme rdf:resource="http://www.usgs.gov/science/USGSThesaurus"/>
  </rdf:Description>
  <rdf:Description about="http://www.usgs.gov/science/USGSThesaurus/vascular%20plants">
    <rdf:type rdf:resource="http://www.w3.org/2004/02/skos/core#Concept"/>
    <skos:prefLabel xml:lang="en">vascular plants</skos:prefLabel>
    <skos:scopeNote xml:lang="en">Plants which have a specialized conductive system. Includes xylem and phloem: club mosses, ferns, cycads, gymnosperms, and angiosperms.</skos:scopeNote>
    <skos:broader rdf:resource="http://www.usgs.gov/science/USGSThesaurus/plants%20%28organisms%29"/>
    <skos:narrower rdf:resource="http://www.usgs.gov/science/USGSThesaurus/ferns%20and%20fern%20allies"/>
    <skos:narrower rdf:resource="http://www.usgs.gov/science/USGSThesaurus/flowering%20plants"/>
    <skos:narrower rdf:resource="http://www.usgs.gov/science/USGSThesaurus/gymnosperms"/>
    <skos:related rdf:resource="http://www.usgs.gov/science/USGSThesaurus/botany"/>
    <skos:inScheme rdf:resource="http://www.usgs.gov/science/USGSThesaurus"/>
  </rdf:Description>
  <rdf:Description about="http://www.usgs.gov/science/USGSThesaurus/ferns%20and%20fern%20allies">
    <rdf:type rdf:resource="http://www.w3.org/2004/02/skos/core#Concept"/>
    <skos:prefLabel xml:lang="en">ferns and fern allies</skos:prefLabel>
    <skos:scopeNote xml:lang="en">Spore-bearing, vascular plants having leaves known as fronds.</skos:scopeNote>
    <skos:broader rdf:resource="http://www.usgs.gov/science/USGSThesaurus/vascular%20plants"/>
    <skos:related rdf:resource="http://www.usgs.gov/science/USGSThesaurus/botany"/>
    <skos:inScheme rdf:resource="http://www.usgs.gov/science/USGSThesaurus"/>
  </rdf:Description>
  <rdf:Description about="http://www.usgs.gov/science/USGSThesaurus/flowering%20plants">
    <rdf:type rdf:resource="http://www.w3.org/2004/02/skos/core#Concept"/>
    <skos:prefLabel xml:lang="en">flowering plants</skos:prefLabel>
    <skos:scopeNote xml:lang="en">Plants known as angiosperms which periodically produce flowers which have various parts including sepals, petals, stamens, and carpels.</skos:scopeNote>
    <skos:broader rdf:resource="http://www.usgs.gov/science/USGSThesaurus/vascular%20plants"/>
    <skos:related rdf:resource="http://www.usgs.gov/science/USGSThesaurus/botany"/>
    <skos:inScheme rdf:resource="http://www.usgs.gov/science/USGSThesaurus"/>
  </rdf:Description>
  <rdf:Description about="http://www.usgs.gov/science/USGSThesaurus/gymnosperms">
    <rdf:type rdf:resource="http://www.w3.org/2004/02/skos/core#Concept"/>
    <skos:prefLabel xml:lang="en">gymnosperms</skos:prefLabel>
    <skos:scopeNote xml:lang="en">Seed-bearing woody vascular plants, such as the conifers (pine, spruce, fir, etc.), whose seeds are not enclosed in an ovary or fruit, but are exposed. </skos:scopeNote>
    <skos:broader rdf:resource="http://www.usgs.gov/science/USGSThesaurus/vascular%20plants"/>
    <skos:related rdf:resource="http://www.usgs.gov/science/USGSThesaurus/botany"/>
    <skos:inScheme rdf:resource="http://www.usgs.gov/science/USGSThesaurus"/>
  </rdf:Description>
  <rdf:Description about="http://www.usgs.gov/science/USGSThesaurus/protists">
    <rdf:type rdf:resource="http://www.w3.org/2004/02/skos/core#Concept"/>
    <skos:prefLabel xml:lang="en">protists</skos:prefLabel>
    <skos:scopeNote xml:lang="en">Unicellular eukaryotes (organisms possessing nucleated cells) with affinities to both plants and animals. Classed in the Protista or Potoctista kingdom, they include protozoans, foraminifera, radiolarians, fungi and some algae.</skos:scopeNote>
    <skos:altLabel xml:lang="en">foraminifera</skos:altLabel>
    <skos:altLabel xml:lang="en">protozoans</skos:altLabel>
    <skos:altLabel xml:lang="en">radiolaria</skos:altLabel>
    <skos:broader rdf:resource="http://www.usgs.gov/science/USGSThesaurus/organisms"/>
    <skos:related rdf:resource="http://www.usgs.gov/science/USGSThesaurus/algae"/>
    <skos:related rdf:resource="http://www.usgs.gov/science/USGSThesaurus/microbiology"/>
    <skos:related rdf:resource="http://www.usgs.gov/science/USGSThesaurus/micropaleontology"/>
    <skos:inScheme rdf:resource="http://www.usgs.gov/science/USGSThesaurus"/>
  </rdf:Description>
  <rdf:Description about="http://www.usgs.gov/science/USGSThesaurus/viruses">
    <rdf:type rdf:resource="http://www.w3.org/2004/02/skos/core#Concept"/>
    <skos:prefLabel xml:lang="en">viruses</skos:prefLabel>
    <skos:scopeNote xml:lang="en">Very small particles visible only with an electronic microscope. Considered to be complex molecules and not living organisms, these are often causes of disease in plants, animals, and bacteria.</skos:scopeNote>
    <skos:broader rdf:resource="http://www.usgs.gov/science/USGSThesaurus/organisms"/>
    <skos:related rdf:resource="http://www.usgs.gov/science/USGSThesaurus/virology"/>
    <skos:inScheme rdf:resource="http://www.usgs.gov/science/USGSThesaurus"/>
  </rdf:Description>
  <rdf:Description about="http://www.usgs.gov/science/USGSThesaurus/planetary%20bodies">
    <rdf:type rdf:resource="http://www.w3.org/2004/02/skos/core#Concept"/>
    <skos:prefLabel xml:lang="en">planetary bodies</skos:prefLabel>
    <skos:scopeNote xml:lang="en">Large celestial masses of rock, metal, or gas orbiting around a star.  Use for extraterrestrial bodies.</skos:scopeNote>
    <skos:broader rdf:resource="http://www.usgs.gov/science/USGSThesaurus/topics"/>
    <skos:narrower rdf:resource="http://www.usgs.gov/science/USGSThesaurus/meteorites"/>
    <skos:related rdf:resource="http://www.usgs.gov/science/USGSThesaurus/planetary%20sciences"/>
    <skos:related rdf:resource="http://www.usgs.gov/science/USGSThesaurus/impact%20cratering"/>
    <skos:inScheme rdf:resource="http://www.usgs.gov/science/USGSThesaurus"/>
  </rdf:Description>
  <rdf:Description about="http://www.usgs.gov/science/USGSThesaurus/meteorites">
    <rdf:type rdf:resource="http://www.w3.org/2004/02/skos/core#Concept"/>
    <skos:prefLabel xml:lang="en">meteorites</skos:prefLabel>
    <skos:scopeNote xml:lang="en">Masses of rock or metal from space that reach the earth's surface without burning up.  Use for 'meteors' or 'meteoroids' as well as 'meteorites'. USGS is more likely to have information about 'meteorites' since these are objects found on the earth.</skos:scopeNote>
    <skos:altLabel xml:lang="en">chondrites</skos:altLabel>
    <skos:altLabel xml:lang="en">bolides</skos:altLabel>
    <skos:altLabel xml:lang="en">meteors</skos:altLabel>
    <skos:broader rdf:resource="http://www.usgs.gov/science/USGSThesaurus/planetary%20bodies"/>
    <skos:related rdf:resource="http://www.usgs.gov/science/USGSThesaurus/rocks%20and%20deposits"/>
    <skos:inScheme rdf:resource="http://www.usgs.gov/science/USGSThesaurus"/>
  </rdf:Description>
  <rdf:Description about="http://www.usgs.gov/science/USGSThesaurus/population%20and%20community%20ecology">
    <rdf:type rdf:resource="http://www.w3.org/2004/02/skos/core#Concept"/>
    <skos:prefLabel xml:lang="en">population and community ecology</skos:prefLabel>
    <skos:scopeNote xml:lang="en">Interactions of a single species (population) or an association of different species (community) occupying a particular region, including their biotic and abiotic environments.</skos:scopeNote>
    <skos:altLabel xml:lang="en">life history</skos:altLabel>
    <skos:altLabel xml:lang="en">population energetics</skos:altLabel>
    <!--FOR radar ecology USE population and community ecology WITH doppler radar imaging-->
    <skos:altLabel xml:lang="en">radar ecology</skos:altLabel>
    <skos:broader rdf:resource="http://www.usgs.gov/science/USGSThesaurus/topics"/>
    <skos:narrower rdf:resource="http://www.usgs.gov/science/USGSThesaurus/animal%20behavior"/>
    <skos:narrower rdf:resource="http://www.usgs.gov/science/USGSThesaurus/biodiversity"/>
    <skos:narrower rdf:resource="http://www.usgs.gov/science/USGSThesaurus/biogeography"/>
    <skos:narrower rdf:resource="http://www.usgs.gov/science/USGSThesaurus/community%20ecology"/>
    <skos:narrower rdf:resource="http://www.usgs.gov/science/USGSThesaurus/ecosystems"/>
    <skos:narrower rdf:resource="http://www.usgs.gov/science/USGSThesaurus/habitats"/>
    <skos:narrower rdf:resource="http://www.usgs.gov/science/USGSThesaurus/phenology"/>
    <skos:narrower rdf:resource="http://www.usgs.gov/science/USGSThesaurus/population%20dynamics"/>
    <skos:narrower rdf:resource="http://www.usgs.gov/science/USGSThesaurus/symbiosis"/>
    <skos:related rdf:resource="http://www.usgs.gov/science/USGSThesaurus/biological%20population%20management"/>
    <skos:related rdf:resource="http://www.usgs.gov/science/USGSThesaurus/ecological%20processes"/>
    <skos:related rdf:resource="http://www.usgs.gov/science/USGSThesaurus/ecology"/>
    <skos:related rdf:resource="http://www.usgs.gov/science/USGSThesaurus/ecosystem%20monitoring"/>
    <skos:related rdf:resource="http://www.usgs.gov/science/USGSThesaurus/natural%20resource%20management"/>
    <skos:related rdf:resource="http://www.usgs.gov/science/USGSThesaurus/relative%20abundance%20analysis"/>
    <skos:inScheme rdf:resource="http://www.usgs.gov/science/USGSThesaurus"/>
  </rdf:Description>
  <rdf:Description about="http://www.usgs.gov/science/USGSThesaurus/animal%20behavior">
    <rdf:type rdf:resource="http://www.w3.org/2004/02/skos/core#Concept"/>
    <skos:prefLabel xml:lang="en">animal behavior</skos:prefLabel>
    <skos:scopeNote xml:lang="en">The way animals act or react to conditions in the environment and to other organisms, including life patterns such as migration, hibernation, and nocturnal living.</skos:scopeNote>
    <skos:broader rdf:resource="http://www.usgs.gov/science/USGSThesaurus/population%20and%20community%20ecology"/>
    <skos:related rdf:resource="http://www.usgs.gov/science/USGSThesaurus/ecology"/>
    <skos:related rdf:resource="http://www.usgs.gov/science/USGSThesaurus/migration%20%28organisms%29"/>
    <skos:related rdf:resource="http://www.usgs.gov/science/USGSThesaurus/migratory%20species"/>
    <skos:related rdf:resource="http://www.usgs.gov/science/USGSThesaurus/ethology"/>
    <skos:inScheme rdf:resource="http://www.usgs.gov/science/USGSThesaurus"/>
  </rdf:Description>
  <rdf:Description about="http://www.usgs.gov/science/USGSThesaurus/biodiversity">
    <rdf:type rdf:resource="http://www.w3.org/2004/02/skos/core#Concept"/>
    <skos:prefLabel xml:lang="en">biodiversity</skos:prefLabel>
    <skos:scopeNote xml:lang="en">The variety in form, genetics, and ecological roles of organisms within a specific geographic area.</skos:scopeNote>
    <skos:altLabel xml:lang="en">biological diversity</skos:altLabel>
    <skos:altLabel xml:lang="en">diversity (biological)</skos:altLabel>
    <skos:broader rdf:resource="http://www.usgs.gov/science/USGSThesaurus/population%20and%20community%20ecology"/>
    <skos:narrower rdf:resource="http://www.usgs.gov/science/USGSThesaurus/ecosystem%20diversity"/>
    <skos:narrower rdf:resource="http://www.usgs.gov/science/USGSThesaurus/genetic%20diversity"/>
    <skos:narrower rdf:resource="http://www.usgs.gov/science/USGSThesaurus/species%20diversity"/>
    <skos:related rdf:resource="http://www.usgs.gov/science/USGSThesaurus/biogeography"/>
    <skos:related rdf:resource="http://www.usgs.gov/science/USGSThesaurus/ecological%20competition"/>
    <skos:related rdf:resource="http://www.usgs.gov/science/USGSThesaurus/ecology"/>
    <skos:related rdf:resource="http://www.usgs.gov/science/USGSThesaurus/endangered%20species"/>
    <skos:related rdf:resource="http://www.usgs.gov/science/USGSThesaurus/endemic%20species"/>
    <skos:related rdf:resource="http://www.usgs.gov/science/USGSThesaurus/invasive%20species"/>
    <skos:related rdf:resource="http://www.usgs.gov/science/USGSThesaurus/life%20sciences"/>
    <skos:related rdf:resource="http://www.usgs.gov/science/USGSThesaurus/native%20species"/>
    <skos:related rdf:resource="http://www.usgs.gov/science/USGSThesaurus/nonindigenous%20species"/>
    <skos:inScheme rdf:resource="http://www.usgs.gov/science/USGSThesaurus"/>
  </rdf:Description>
  <rdf:Description about="http://www.usgs.gov/science/USGSThesaurus/ecosystem%20diversity">
    <rdf:type rdf:resource="http://www.w3.org/2004/02/skos/core#Concept"/>
    <skos:prefLabel xml:lang="en">ecosystem diversity</skos:prefLabel>
    <skos:scopeNote xml:lang="en">Measure of the variety of biological communities and habitats important for ecological stability.</skos:scopeNote>
    <skos:broader rdf:resource="http://www.usgs.gov/science/USGSThesaurus/biodiversity"/>
    <skos:narrower rdf:resource="http://www.usgs.gov/science/USGSThesaurus/environmental%20DNA"/>
    <skos:inScheme rdf:resource="http://www.usgs.gov/science/USGSThesaurus"/>
  </rdf:Description>
  <rdf:Description about="http://www.usgs.gov/science/USGSThesaurus/environmental%20DNA">
    <rdf:type rdf:resource="http://www.w3.org/2004/02/skos/core#Concept"/>
    <skos:prefLabel xml:lang="en">environmental DNA</skos:prefLabel>
    <skos:scopeNote xml:lang="en">Nuclear or mitochondrial DNA released into the environment as bodily secretions, hair, or similar materials other than whole individuals.  Used to detect organisms that are not observed directly.</skos:scopeNote>
    <skos:altLabel xml:lang="en">eDNA</skos:altLabel>
    <skos:broader rdf:resource="http://www.usgs.gov/science/USGSThesaurus/ecosystem%20diversity"/>
    <skos:inScheme rdf:resource="http://www.usgs.gov/science/USGSThesaurus"/>
  </rdf:Description>
  <rdf:Description about="http://www.usgs.gov/science/USGSThesaurus/genetic%20diversity">
    <rdf:type rdf:resource="http://www.w3.org/2004/02/skos/core#Concept"/>
    <skos:prefLabel xml:lang="en">genetic diversity</skos:prefLabel>
    <skos:scopeNote xml:lang="en">Measure of the variety of genes within a population pool in a given area.</skos:scopeNote>
    <!--FOR conservation genetics USE genetic diversity WITH biological population management-->
    <skos:altLabel xml:lang="en">conservation genetics</skos:altLabel>
    <skos:broader rdf:resource="http://www.usgs.gov/science/USGSThesaurus/biodiversity"/>
    <skos:narrower rdf:resource="http://www.usgs.gov/science/USGSThesaurus/genotype"/>
    <skos:inScheme rdf:resource="http://www.usgs.gov/science/USGSThesaurus"/>
  </rdf:Description>
  <rdf:Description about="http://www.usgs.gov/science/USGSThesaurus/genotype">
    <rdf:type rdf:resource="http://www.w3.org/2004/02/skos/core#Concept"/>
    <skos:prefLabel xml:lang="en">genotype</skos:prefLabel>
    <skos:scopeNote xml:lang="en">Genetic characteristics of an individual organism.</skos:scopeNote>
    <skos:broader rdf:resource="http://www.usgs.gov/science/USGSThesaurus/genetic%20diversity"/>
    <skos:inScheme rdf:resource="http://www.usgs.gov/science/USGSThesaurus"/>
  </rdf:Description>
  <rdf:Description about="http://www.usgs.gov/science/USGSThesaurus/species%20diversity">
    <rdf:type rdf:resource="http://www.w3.org/2004/02/skos/core#Concept"/>
    <skos:prefLabel xml:lang="en">species diversity</skos:prefLabel>
    <skos:scopeNote xml:lang="en">An ecological concept incorporating both the number of species in a particular sampling area and the evenness with which individuals are distributed among the various species.</skos:scopeNote>
    <skos:broader rdf:resource="http://www.usgs.gov/science/USGSThesaurus/biodiversity"/>
    <skos:inScheme rdf:resource="http://www.usgs.gov/science/USGSThesaurus"/>
  </rdf:Description>
  <rdf:Description about="http://www.usgs.gov/science/USGSThesaurus/biogeography">
    <rdf:type rdf:resource="http://www.w3.org/2004/02/skos/core#Concept"/>
    <skos:prefLabel xml:lang="en">biogeography</skos:prefLabel>
    <skos:scopeNote xml:lang="en">The study of the geographic distributions of plants and animals.</skos:scopeNote>
    <skos:altLabel xml:lang="en">animal distribution</skos:altLabel>
    <skos:altLabel xml:lang="en">distribution of animals</skos:altLabel>
    <skos:altLabel xml:lang="en">distribution of plants</skos:altLabel>
    <skos:altLabel xml:lang="en">distribution of species</skos:altLabel>
    <!--FOR flyways USE biogeography WITH migration (organisms)-->
    <skos:altLabel xml:lang="en">flyways</skos:altLabel>
    <skos:altLabel xml:lang="en">plant distribution</skos:altLabel>
    <!--FOR species distribution maps USE biogeography WITH maps and atlases-->
    <skos:altLabel xml:lang="en">species distribution maps</skos:altLabel>
    <skos:altLabel xml:lang="en">species distribution</skos:altLabel>
    <skos:altLabel xml:lang="en">species geographic range</skos:altLabel>
    <skos:broader rdf:resource="http://www.usgs.gov/science/USGSThesaurus/population%20and%20community%20ecology"/>
    <skos:related rdf:resource="http://www.usgs.gov/science/USGSThesaurus/biodiversity"/>
    <skos:related rdf:resource="http://www.usgs.gov/science/USGSThesaurus/ecology"/>
    <skos:related rdf:resource="http://www.usgs.gov/science/USGSThesaurus/ecosystem%20monitoring"/>
    <skos:related rdf:resource="http://www.usgs.gov/science/USGSThesaurus/migration%20%28organisms%29"/>
    <skos:related rdf:resource="http://www.usgs.gov/science/USGSThesaurus/migratory%20species"/>
    <skos:related rdf:resource="http://www.usgs.gov/science/USGSThesaurus/population%20dynamics"/>
    <skos:related rdf:resource="http://www.usgs.gov/science/USGSThesaurus/wildlife%20population%20management"/>
    <skos:inScheme rdf:resource="http://www.usgs.gov/science/USGSThesaurus"/>
  </rdf:Description>
  <rdf:Description about="http://www.usgs.gov/science/USGSThesaurus/community%20ecology">
    <rdf:type rdf:resource="http://www.w3.org/2004/02/skos/core#Concept"/>
    <skos:prefLabel xml:lang="en">community ecology</skos:prefLabel>
    <skos:scopeNote xml:lang="en">Study of the relationships of species that interact in a common area.</skos:scopeNote>
    <skos:broader rdf:resource="http://www.usgs.gov/science/USGSThesaurus/population%20and%20community%20ecology"/>
    <skos:related rdf:resource="http://www.usgs.gov/science/USGSThesaurus/ecological%20competition"/>
    <skos:related rdf:resource="http://www.usgs.gov/science/USGSThesaurus/ecology"/>
    <skos:inScheme rdf:resource="http://www.usgs.gov/science/USGSThesaurus"/>
  </rdf:Description>
  <rdf:Description about="http://www.usgs.gov/science/USGSThesaurus/ecosystems">
    <rdf:type rdf:resource="http://www.w3.org/2004/02/skos/core#Concept"/>
    <skos:prefLabel xml:lang="en">ecosystems</skos:prefLabel>
    <skos:scopeNote xml:lang="en">The interacting populations of plants, animals, and  microorganisms occupying a certain area, and their relationship to the environment.</skos:scopeNote>
    <skos:altLabel xml:lang="en">biosphere</skos:altLabel>
    <skos:altLabel xml:lang="en">clines</skos:altLabel>
    <skos:altLabel xml:lang="en">ecoclines</skos:altLabel>
    <skos:altLabel xml:lang="en">ecotones</skos:altLabel>
    <skos:broader rdf:resource="http://www.usgs.gov/science/USGSThesaurus/population%20and%20community%20ecology"/>
    <skos:narrower rdf:resource="http://www.usgs.gov/science/USGSThesaurus/aquatic%20ecosystems"/>
    <skos:narrower rdf:resource="http://www.usgs.gov/science/USGSThesaurus/terrestrial%20ecosystems"/>
    <skos:narrower rdf:resource="http://www.usgs.gov/science/USGSThesaurus/wetland%20ecosystems"/>
    <skos:related rdf:resource="http://www.usgs.gov/science/USGSThesaurus/ecology"/>
    <skos:related rdf:resource="http://www.usgs.gov/science/USGSThesaurus/habitats"/>
    <skos:related rdf:resource="http://www.usgs.gov/science/USGSThesaurus/ecosystem%20functions"/>
    <skos:related rdf:resource="http://www.usgs.gov/science/USGSThesaurus/ecosystem%20services%20valuation"/>
    <skos:inScheme rdf:resource="http://www.usgs.gov/science/USGSThesaurus"/>
  </rdf:Description>
  <rdf:Description about="http://www.usgs.gov/science/USGSThesaurus/aquatic%20ecosystems">
    <rdf:type rdf:resource="http://www.w3.org/2004/02/skos/core#Concept"/>
    <skos:prefLabel xml:lang="en">aquatic ecosystems</skos:prefLabel>
    <skos:scopeNote xml:lang="en">Communities of interdependent organisms living primarily in or on water.</skos:scopeNote>
    <!--FOR planktonic ecosystems USE aquatic ecosystems WITH plankton-->
    <skos:altLabel xml:lang="en">planktonic ecosystems</skos:altLabel>
    <skos:broader rdf:resource="http://www.usgs.gov/science/USGSThesaurus/ecosystems"/>
    <skos:narrower rdf:resource="http://www.usgs.gov/science/USGSThesaurus/benthic%20ecosystems"/>
    <skos:narrower rdf:resource="http://www.usgs.gov/science/USGSThesaurus/estuarine%20ecosystems"/>
    <skos:narrower rdf:resource="http://www.usgs.gov/science/USGSThesaurus/freshwater%20ecosystems"/>
    <skos:narrower rdf:resource="http://www.usgs.gov/science/USGSThesaurus/marine%20ecosystems"/>
    <skos:related rdf:resource="http://www.usgs.gov/science/USGSThesaurus/aquatic%20biology"/>
    <skos:related rdf:resource="http://www.usgs.gov/science/USGSThesaurus/coastal%20ecosystems"/>
    <skos:related rdf:resource="http://www.usgs.gov/science/USGSThesaurus/ecology"/>
    <skos:related rdf:resource="http://www.usgs.gov/science/USGSThesaurus/limnology"/>
    <skos:related rdf:resource="http://www.usgs.gov/science/USGSThesaurus/marine%20biology"/>
    <skos:inScheme rdf:resource="http://www.usgs.gov/science/USGSThesaurus"/>
  </rdf:Description>
  <rdf:Description about="http://www.usgs.gov/science/USGSThesaurus/benthic%20ecosystems">
    <rdf:type rdf:resource="http://www.w3.org/2004/02/skos/core#Concept"/>
    <skos:prefLabel xml:lang="en">benthic ecosystems</skos:prefLabel>
    <skos:scopeNote xml:lang="en">Biologic communities and habitats at the bottom of lakes, streams, or oceans.</skos:scopeNote>
    <skos:broader rdf:resource="http://www.usgs.gov/science/USGSThesaurus/aquatic%20ecosystems"/>
    <skos:related rdf:resource="http://www.usgs.gov/science/USGSThesaurus/aquatic%20biology"/>
    <skos:related rdf:resource="http://www.usgs.gov/science/USGSThesaurus/ecology"/>
    <skos:related rdf:resource="http://www.usgs.gov/science/USGSThesaurus/limnology"/>
    <skos:related rdf:resource="http://www.usgs.gov/science/USGSThesaurus/marine%20biology"/>
    <skos:inScheme rdf:resource="http://www.usgs.gov/science/USGSThesaurus"/>
  </rdf:Description>
  <rdf:Description about="http://www.usgs.gov/science/USGSThesaurus/estuarine%20ecosystems">
    <rdf:type rdf:resource="http://www.w3.org/2004/02/skos/core#Concept"/>
    <skos:prefLabel xml:lang="en">estuarine ecosystems</skos:prefLabel>
    <skos:scopeNote xml:lang="en">Biological communities and habitats within sea inlets or the zones where rivers meet the seas which are subject to tidal effects and the mixture of fresh and saltwater.</skos:scopeNote>
    <!--FOR estuarine ecosystem functions USE estuarine ecosystems WITH ecosystem functions-->
    <skos:altLabel xml:lang="en">estuarine ecosystem functions</skos:altLabel>
    <skos:broader rdf:resource="http://www.usgs.gov/science/USGSThesaurus/aquatic%20ecosystems"/>
    <skos:related rdf:resource="http://www.usgs.gov/science/USGSThesaurus/aquatic%20biology"/>
    <skos:related rdf:resource="http://www.usgs.gov/science/USGSThesaurus/ecology"/>
    <skos:inScheme rdf:resource="http://www.usgs.gov/science/USGSThesaurus"/>
  </rdf:Description>
  <rdf:Description about="http://www.usgs.gov/science/USGSThesaurus/freshwater%20ecosystems">
    <rdf:type rdf:resource="http://www.w3.org/2004/02/skos/core#Concept"/>
    <skos:prefLabel xml:lang="en">freshwater ecosystems</skos:prefLabel>
    <skos:scopeNote xml:lang="en">Biological communities and habitats that exist in lakes, rivers, ponds, and other bodies of water that are not salty.</skos:scopeNote>
    <skos:altLabel xml:lang="en">lake ecosystems</skos:altLabel>
    <skos:altLabel xml:lang="en">pond ecosystems</skos:altLabel>
    <!--FOR river ecosystems USE freshwater ecosystems WITH river systems-->
    <skos:altLabel xml:lang="en">river ecosystems</skos:altLabel>
    <skos:altLabel xml:lang="en">spring ecosystems</skos:altLabel>
    <skos:altLabel xml:lang="en">stream ecosystems</skos:altLabel>
    <skos:broader rdf:resource="http://www.usgs.gov/science/USGSThesaurus/aquatic%20ecosystems"/>
    <skos:related rdf:resource="http://www.usgs.gov/science/USGSThesaurus/aquatic%20biology"/>
    <skos:related rdf:resource="http://www.usgs.gov/science/USGSThesaurus/ecology"/>
    <skos:related rdf:resource="http://www.usgs.gov/science/USGSThesaurus/groundwater"/>
    <skos:related rdf:resource="http://www.usgs.gov/science/USGSThesaurus/limnology"/>
    <skos:related rdf:resource="http://www.usgs.gov/science/USGSThesaurus/surface%20water%20%28non-marine%29"/>
    <skos:inScheme rdf:resource="http://www.usgs.gov/science/USGSThesaurus"/>
  </rdf:Description>
  <rdf:Description about="http://www.usgs.gov/science/USGSThesaurus/marine%20ecosystems">
    <rdf:type rdf:resource="http://www.w3.org/2004/02/skos/core#Concept"/>
    <skos:prefLabel xml:lang="en">marine ecosystems</skos:prefLabel>
    <skos:scopeNote xml:lang="en">Biological communities composed of plants and animals living primarily in or on seawater.</skos:scopeNote>
    <skos:broader rdf:resource="http://www.usgs.gov/science/USGSThesaurus/aquatic%20ecosystems"/>
    <skos:narrower rdf:resource="http://www.usgs.gov/science/USGSThesaurus/reef%20ecosystems"/>
    <skos:related rdf:resource="http://www.usgs.gov/science/USGSThesaurus/aquatic%20biology"/>
    <skos:related rdf:resource="http://www.usgs.gov/science/USGSThesaurus/ecology"/>
    <skos:related rdf:resource="http://www.usgs.gov/science/USGSThesaurus/marine%20biology"/>
    <skos:inScheme rdf:resource="http://www.usgs.gov/science/USGSThesaurus"/>
  </rdf:Description>
  <rdf:Description about="http://www.usgs.gov/science/USGSThesaurus/reef%20ecosystems">
    <rdf:type rdf:resource="http://www.w3.org/2004/02/skos/core#Concept"/>
    <skos:prefLabel xml:lang="en">reef ecosystems</skos:prefLabel>
    <skos:scopeNote xml:lang="en">Biological communities formed by the skeletons of calcareous seawater organisms, usually corals.</skos:scopeNote>
    <skos:altLabel xml:lang="en">coral reef ecosystems</skos:altLabel>
    <skos:broader rdf:resource="http://www.usgs.gov/science/USGSThesaurus/marine%20ecosystems"/>
    <skos:related rdf:resource="http://www.usgs.gov/science/USGSThesaurus/coelenterates"/>
    <skos:related rdf:resource="http://www.usgs.gov/science/USGSThesaurus/ecology"/>
    <skos:related rdf:resource="http://www.usgs.gov/science/USGSThesaurus/marine%20biology"/>
    <skos:related rdf:resource="http://www.usgs.gov/science/USGSThesaurus/marine%20fishery%20resources"/>
    <skos:inScheme rdf:resource="http://www.usgs.gov/science/USGSThesaurus"/>
  </rdf:Description>
  <rdf:Description about="http://www.usgs.gov/science/USGSThesaurus/terrestrial%20ecosystems">
    <rdf:type rdf:resource="http://www.w3.org/2004/02/skos/core#Concept"/>
    <skos:prefLabel xml:lang="en">terrestrial ecosystems</skos:prefLabel>
    <skos:scopeNote xml:lang="en">Communities of living organisms in a specific geographical location which exist primarily on land and not in water.</skos:scopeNote>
    <skos:altLabel xml:lang="en">rangeland ecosystems</skos:altLabel>
    <skos:broader rdf:resource="http://www.usgs.gov/science/USGSThesaurus/ecosystems"/>
    <skos:narrower rdf:resource="http://www.usgs.gov/science/USGSThesaurus/coastal%20ecosystems"/>
    <skos:narrower rdf:resource="http://www.usgs.gov/science/USGSThesaurus/desert%20ecosystems"/>
    <skos:narrower rdf:resource="http://www.usgs.gov/science/USGSThesaurus/forest%20ecosystems"/>
    <skos:narrower rdf:resource="http://www.usgs.gov/science/USGSThesaurus/grassland%20ecosystems"/>
    <skos:narrower rdf:resource="http://www.usgs.gov/science/USGSThesaurus/island%20ecosystems"/>
    <skos:narrower rdf:resource="http://www.usgs.gov/science/USGSThesaurus/shrubland%20ecosystems"/>
    <skos:narrower rdf:resource="http://www.usgs.gov/science/USGSThesaurus/tundra%20ecosystems"/>
    <skos:related rdf:resource="http://www.usgs.gov/science/USGSThesaurus/ecology"/>
    <skos:related rdf:resource="http://www.usgs.gov/science/USGSThesaurus/wetland%20ecosystems"/>
    <skos:inScheme rdf:resource="http://www.usgs.gov/science/USGSThesaurus"/>
  </rdf:Description>
  <rdf:Description about="http://www.usgs.gov/science/USGSThesaurus/coastal%20ecosystems">
    <rdf:type rdf:resource="http://www.w3.org/2004/02/skos/core#Concept"/>
    <skos:prefLabel xml:lang="en">coastal ecosystems</skos:prefLabel>
    <skos:scopeNote xml:lang="en">Biological communities and habitats within the narrow zones of land between the margin of oceans or seas and large landmasses.</skos:scopeNote>
    <skos:altLabel xml:lang="en">littoral ecosystems</skos:altLabel>
    <skos:broader rdf:resource="http://www.usgs.gov/science/USGSThesaurus/terrestrial%20ecosystems"/>
    <skos:related rdf:resource="http://www.usgs.gov/science/USGSThesaurus/aquatic%20ecosystems"/>
    <skos:related rdf:resource="http://www.usgs.gov/science/USGSThesaurus/ecology"/>
    <skos:inScheme rdf:resource="http://www.usgs.gov/science/USGSThesaurus"/>
  </rdf:Description>
  <rdf:Description about="http://www.usgs.gov/science/USGSThesaurus/desert%20ecosystems">
    <rdf:type rdf:resource="http://www.w3.org/2004/02/skos/core#Concept"/>
    <skos:prefLabel xml:lang="en">desert ecosystems</skos:prefLabel>
    <skos:scopeNote xml:lang="en">Biological communities and habitats in arid areas with little precipitation, sparse, highly adapted vegetation, and extreme temperatures.</skos:scopeNote>
    <skos:broader rdf:resource="http://www.usgs.gov/science/USGSThesaurus/terrestrial%20ecosystems"/>
    <skos:related rdf:resource="http://www.usgs.gov/science/USGSThesaurus/desertification"/>
    <skos:related rdf:resource="http://www.usgs.gov/science/USGSThesaurus/ecology"/>
    <skos:inScheme rdf:resource="http://www.usgs.gov/science/USGSThesaurus"/>
  </rdf:Description>
  <rdf:Description about="http://www.usgs.gov/science/USGSThesaurus/forest%20ecosystems">
    <rdf:type rdf:resource="http://www.w3.org/2004/02/skos/core#Concept"/>
    <skos:prefLabel xml:lang="en">forest ecosystems</skos:prefLabel>
    <skos:scopeNote xml:lang="en">Biological communities and habitats in geographic areas with dense growths of trees and associated vegetation.</skos:scopeNote>
    <skos:altLabel xml:lang="en">arboreal ecosystems</skos:altLabel>
    <skos:altLabel xml:lang="en">coniferous forests ecosystems</skos:altLabel>
    <skos:altLabel xml:lang="en">deciduous forest ecosystems</skos:altLabel>
    <skos:altLabel xml:lang="en">mixed forest ecosystems</skos:altLabel>
    <skos:altLabel xml:lang="en">taiga ecosystems</skos:altLabel>
    <skos:broader rdf:resource="http://www.usgs.gov/science/USGSThesaurus/terrestrial%20ecosystems"/>
    <skos:related rdf:resource="http://www.usgs.gov/science/USGSThesaurus/ecology"/>
    <skos:related rdf:resource="http://www.usgs.gov/science/USGSThesaurus/forest%20resources"/>
    <skos:inScheme rdf:resource="http://www.usgs.gov/science/USGSThesaurus"/>
  </rdf:Description>
  <rdf:Description about="http://www.usgs.gov/science/USGSThesaurus/grassland%20ecosystems">
    <rdf:type rdf:resource="http://www.w3.org/2004/02/skos/core#Concept"/>
    <skos:prefLabel xml:lang="en">grassland ecosystems</skos:prefLabel>
    <skos:scopeNote xml:lang="en">Biological communities and habitats with ground cover of grasses and other herbaceous plants, but few trees.  Examples include prairies, meadows, and savannas.</skos:scopeNote>
    <skos:altLabel xml:lang="en">mixed grass ecosystems</skos:altLabel>
    <skos:altLabel xml:lang="en">plains ecosystems</skos:altLabel>
    <skos:altLabel xml:lang="en">prairie ecosystems</skos:altLabel>
    <skos:altLabel xml:lang="en">short grass ecosystems</skos:altLabel>
    <skos:altLabel xml:lang="en">tall grass ecosystems</skos:altLabel>
    <skos:broader rdf:resource="http://www.usgs.gov/science/USGSThesaurus/terrestrial%20ecosystems"/>
    <skos:related rdf:resource="http://www.usgs.gov/science/USGSThesaurus/ecology"/>
    <skos:inScheme rdf:resource="http://www.usgs.gov/science/USGSThesaurus"/>
  </rdf:Description>
  <rdf:Description about="http://www.usgs.gov/science/USGSThesaurus/island%20ecosystems">
    <rdf:type rdf:resource="http://www.w3.org/2004/02/skos/core#Concept"/>
    <skos:prefLabel xml:lang="en">island ecosystems</skos:prefLabel>
    <skos:scopeNote xml:lang="en">Communities of living organisms on islands.</skos:scopeNote>
    <skos:altLabel xml:lang="en">insular ecology</skos:altLabel>
    <skos:broader rdf:resource="http://www.usgs.gov/science/USGSThesaurus/terrestrial%20ecosystems"/>
    <skos:inScheme rdf:resource="http://www.usgs.gov/science/USGSThesaurus"/>
  </rdf:Description>
  <rdf:Description about="http://www.usgs.gov/science/USGSThesaurus/shrubland%20ecosystems">
    <rdf:type rdf:resource="http://www.w3.org/2004/02/skos/core#Concept"/>
    <skos:prefLabel xml:lang="en">shrubland ecosystems</skos:prefLabel>
    <skos:scopeNote xml:lang="en">Biological land communities and habitats with sparse, low-growing vegetation.</skos:scopeNote>
    <skos:altLabel xml:lang="en">scrubland ecosystems</skos:altLabel>
    <skos:broader rdf:resource="http://www.usgs.gov/science/USGSThesaurus/terrestrial%20ecosystems"/>
    <skos:related rdf:resource="http://www.usgs.gov/science/USGSThesaurus/ecology"/>
    <skos:inScheme rdf:resource="http://www.usgs.gov/science/USGSThesaurus"/>
  </rdf:Description>
  <rdf:Description about="http://www.usgs.gov/science/USGSThesaurus/tundra%20ecosystems">
    <rdf:type rdf:resource="http://www.w3.org/2004/02/skos/core#Concept"/>
    <skos:prefLabel xml:lang="en">tundra ecosystems</skos:prefLabel>
    <skos:scopeNote xml:lang="en">Biological communities and habitats located in the treeless plains of Arctic regions where the subsoil is permanently frozen.</skos:scopeNote>
    <skos:broader rdf:resource="http://www.usgs.gov/science/USGSThesaurus/terrestrial%20ecosystems"/>
    <skos:related rdf:resource="http://www.usgs.gov/science/USGSThesaurus/ecology"/>
    <skos:inScheme rdf:resource="http://www.usgs.gov/science/USGSThesaurus"/>
  </rdf:Description>
  <rdf:Description about="http://www.usgs.gov/science/USGSThesaurus/wetland%20ecosystems">
    <rdf:type rdf:resource="http://www.w3.org/2004/02/skos/core#Concept"/>
    <skos:prefLabel xml:lang="en">wetland ecosystems</skos:prefLabel>
    <skos:scopeNote xml:lang="en">Ecosystems whose soil is saturated for long periods seasonally or continuously, including marshes, swamps, and ephemeral ponds.  More detailed terms for wetlands can be selected from the FGDC Wetland Classification &lt;http://fgdc.gov/standards/status/sub3_4.html&gt;.</skos:scopeNote>
    <skos:altLabel xml:lang="en">marsh ecosystems</skos:altLabel>
    <skos:altLabel xml:lang="en">marshland ecosystems</skos:altLabel>
    <skos:altLabel xml:lang="en">riparian ecosystems</skos:altLabel>
    <skos:broader rdf:resource="http://www.usgs.gov/science/USGSThesaurus/ecosystems"/>
    <skos:related rdf:resource="http://www.usgs.gov/science/USGSThesaurus/wetland%20functions"/>
    <skos:related rdf:resource="http://www.usgs.gov/science/USGSThesaurus/aquatic%20biology"/>
    <skos:related rdf:resource="http://www.usgs.gov/science/USGSThesaurus/ecology"/>
    <skos:related rdf:resource="http://www.usgs.gov/science/USGSThesaurus/terrestrial%20ecosystems"/>
    <skos:inScheme rdf:resource="http://www.usgs.gov/science/USGSThesaurus"/>
  </rdf:Description>
  <rdf:Description about="http://www.usgs.gov/science/USGSThesaurus/habitats">
    <rdf:type rdf:resource="http://www.w3.org/2004/02/skos/core#Concept"/>
    <skos:prefLabel xml:lang="en">habitats</skos:prefLabel>
    <skos:scopeNote xml:lang="en">Parts of the physical environment where plants and animals live. Use in combination with terms from organisms and organism groupings (non-taxonomic) to indicate the topic of a species or group of species habitat.</skos:scopeNote>
    <skos:broader rdf:resource="http://www.usgs.gov/science/USGSThesaurus/population%20and%20community%20ecology"/>
    <skos:related rdf:resource="http://www.usgs.gov/science/USGSThesaurus/ecosystems"/>
    <skos:inScheme rdf:resource="http://www.usgs.gov/science/USGSThesaurus"/>
  </rdf:Description>
  <rdf:Description about="http://www.usgs.gov/science/USGSThesaurus/phenology">
    <rdf:type rdf:resource="http://www.w3.org/2004/02/skos/core#Concept"/>
    <skos:prefLabel xml:lang="en">phenology</skos:prefLabel>
    <skos:scopeNote xml:lang="en">Study of the response of organisms to seasonal or interannual changes in the environment.</skos:scopeNote>
    <skos:broader rdf:resource="http://www.usgs.gov/science/USGSThesaurus/population%20and%20community%20ecology"/>
    <skos:inScheme rdf:resource="http://www.usgs.gov/science/USGSThesaurus"/>
  </rdf:Description>
  <rdf:Description about="http://www.usgs.gov/science/USGSThesaurus/population%20dynamics">
    <rdf:type rdf:resource="http://www.w3.org/2004/02/skos/core#Concept"/>
    <skos:prefLabel xml:lang="en">population dynamics</skos:prefLabel>
    <skos:scopeNote xml:lang="en">Changes in the size, composition, or structure of aggregates of single or multiple species in a specific area over time.</skos:scopeNote>
    <skos:broader rdf:resource="http://www.usgs.gov/science/USGSThesaurus/population%20and%20community%20ecology"/>
    <skos:related rdf:resource="http://www.usgs.gov/science/USGSThesaurus/algal%20blooms"/>
    <skos:related rdf:resource="http://www.usgs.gov/science/USGSThesaurus/biogeography"/>
    <skos:related rdf:resource="http://www.usgs.gov/science/USGSThesaurus/ecology"/>
    <skos:inScheme rdf:resource="http://www.usgs.gov/science/USGSThesaurus"/>
  </rdf:Description>
  <rdf:Description about="http://www.usgs.gov/science/USGSThesaurus/symbiosis">
    <rdf:type rdf:resource="http://www.w3.org/2004/02/skos/core#Concept"/>
    <skos:prefLabel xml:lang="en">symbiosis</skos:prefLabel>
    <skos:scopeNote xml:lang="en">An intimate, prolonged association between two or more organisms of different species that may or may not benefit each member.</skos:scopeNote>
    <skos:altLabel xml:lang="en">commensalism</skos:altLabel>
    <skos:altLabel xml:lang="en">mutualism</skos:altLabel>
    <skos:altLabel xml:lang="en">parasitism</skos:altLabel>
    <skos:broader rdf:resource="http://www.usgs.gov/science/USGSThesaurus/population%20and%20community%20ecology"/>
    <skos:inScheme rdf:resource="http://www.usgs.gov/science/USGSThesaurus"/>
  </rdf:Description>
  <rdf:Description about="http://www.usgs.gov/science/USGSThesaurus/recreation">
    <rdf:type rdf:resource="http://www.w3.org/2004/02/skos/core#Concept"/>
    <skos:prefLabel xml:lang="en">recreation</skos:prefLabel>
    <skos:scopeNote xml:lang="en">Pursuit of leisure-time activities, typically out of doors.</skos:scopeNote>
    <skos:altLabel xml:lang="en">biking</skos:altLabel>
    <skos:altLabel xml:lang="en">bird watching</skos:altLabel>
    <skos:altLabel xml:lang="en">boating</skos:altLabel>
    <skos:altLabel xml:lang="en">camping</skos:altLabel>
    <skos:altLabel xml:lang="en">canoeing</skos:altLabel>
    <skos:altLabel xml:lang="en">caving</skos:altLabel>
    <skos:altLabel xml:lang="en">climbing</skos:altLabel>
    <skos:altLabel xml:lang="en">fishing (recreational)</skos:altLabel>
    <skos:altLabel xml:lang="en">hiking</skos:altLabel>
    <skos:altLabel xml:lang="en">hunting</skos:altLabel>
    <skos:altLabel xml:lang="en">kayaking</skos:altLabel>
    <skos:broader rdf:resource="http://www.usgs.gov/science/USGSThesaurus/topics"/>
    <skos:inScheme rdf:resource="http://www.usgs.gov/science/USGSThesaurus"/>
  </rdf:Description>
  <rdf:Description about="http://www.usgs.gov/science/USGSThesaurus/scientific%20careers">
    <rdf:type rdf:resource="http://www.w3.org/2004/02/skos/core#Concept"/>
    <skos:prefLabel xml:lang="en">scientific careers</skos:prefLabel>
    <skos:scopeNote xml:lang="en">Professions in which people carry out or support scientific research or monitoring.</skos:scopeNote>
    <skos:altLabel xml:lang="en">careers in science</skos:altLabel>
    <!--FOR scientists-at-work photographs USE scientific careers WITH image collections-->
    <skos:altLabel xml:lang="en">scientists-at-work photographs</skos:altLabel>
    <skos:broader rdf:resource="http://www.usgs.gov/science/USGSThesaurus/topics"/>
    <skos:related rdf:resource="http://www.usgs.gov/science/USGSThesaurus/earth%20sciences"/>
    <skos:related rdf:resource="http://www.usgs.gov/science/USGSThesaurus/engineering%20sciences"/>
    <skos:related rdf:resource="http://www.usgs.gov/science/USGSThesaurus/information%20sciences"/>
    <skos:related rdf:resource="http://www.usgs.gov/science/USGSThesaurus/life%20sciences"/>
    <skos:related rdf:resource="http://www.usgs.gov/science/USGSThesaurus/planetary%20sciences"/>
    <skos:related rdf:resource="http://www.usgs.gov/science/USGSThesaurus/social%20sciences"/>
    <skos:inScheme rdf:resource="http://www.usgs.gov/science/USGSThesaurus"/>
  </rdf:Description>
  <rdf:Description about="http://www.usgs.gov/science/USGSThesaurus/water%20properties">
    <rdf:type rdf:resource="http://www.w3.org/2004/02/skos/core#Concept"/>
    <skos:prefLabel xml:lang="en">water properties</skos:prefLabel>
    <skos:scopeNote xml:lang="en">Measurable physical and chemical characteristics of water from different sources.</skos:scopeNote>
    <skos:broader rdf:resource="http://www.usgs.gov/science/USGSThesaurus/topics"/>
    <skos:narrower rdf:resource="http://www.usgs.gov/science/USGSThesaurus/dissolved%20gases"/>
    <skos:narrower rdf:resource="http://www.usgs.gov/science/USGSThesaurus/dissolved%20metals"/>
    <skos:narrower rdf:resource="http://www.usgs.gov/science/USGSThesaurus/dissolved%20organic%20compounds"/>
    <skos:narrower rdf:resource="http://www.usgs.gov/science/USGSThesaurus/nutrient%20content%20%28water%29"/>
    <skos:narrower rdf:resource="http://www.usgs.gov/science/USGSThesaurus/oxygen%20content%20%28water%29"/>
    <skos:narrower rdf:resource="http://www.usgs.gov/science/USGSThesaurus/salinity"/>
    <skos:narrower rdf:resource="http://www.usgs.gov/science/USGSThesaurus/sound%20velocity"/>
    <skos:narrower rdf:resource="http://www.usgs.gov/science/USGSThesaurus/suspended%20material%20%28water%29"/>
    <skos:narrower rdf:resource="http://www.usgs.gov/science/USGSThesaurus/water%20hardness"/>
    <skos:narrower rdf:resource="http://www.usgs.gov/science/USGSThesaurus/water%20pH"/>
    <skos:narrower rdf:resource="http://www.usgs.gov/science/USGSThesaurus/water%20temperature"/>
    <skos:related rdf:resource="http://www.usgs.gov/science/USGSThesaurus/hydrology"/>
    <skos:related rdf:resource="http://www.usgs.gov/science/USGSThesaurus/water%20chemistry"/>
    <skos:related rdf:resource="http://www.usgs.gov/science/USGSThesaurus/water%20quality"/>
    <skos:inScheme rdf:resource="http://www.usgs.gov/science/USGSThesaurus"/>
  </rdf:Description>
  <rdf:Description about="http://www.usgs.gov/science/USGSThesaurus/dissolved%20gases">
    <rdf:type rdf:resource="http://www.w3.org/2004/02/skos/core#Concept"/>
    <skos:prefLabel xml:lang="en">dissolved gases</skos:prefLabel>
    <skos:scopeNote xml:lang="en">Gases such as ammonia, oxygen, nitrogen, and carbon dioxide in solution measured in a water sample.</skos:scopeNote>
    <skos:broader rdf:resource="http://www.usgs.gov/science/USGSThesaurus/water%20properties"/>
    <skos:inScheme rdf:resource="http://www.usgs.gov/science/USGSThesaurus"/>
  </rdf:Description>
  <rdf:Description about="http://www.usgs.gov/science/USGSThesaurus/dissolved%20metals">
    <rdf:type rdf:resource="http://www.w3.org/2004/02/skos/core#Concept"/>
    <skos:prefLabel xml:lang="en">dissolved metals</skos:prefLabel>
    <skos:scopeNote xml:lang="en">Metal elements in solution, of concern in studies of hazards such as mine drainage and of water resource usability.</skos:scopeNote>
    <skos:broader rdf:resource="http://www.usgs.gov/science/USGSThesaurus/water%20properties"/>
    <skos:inScheme rdf:resource="http://www.usgs.gov/science/USGSThesaurus"/>
  </rdf:Description>
  <rdf:Description about="http://www.usgs.gov/science/USGSThesaurus/dissolved%20organic%20compounds">
    <rdf:type rdf:resource="http://www.w3.org/2004/02/skos/core#Concept"/>
    <skos:prefLabel xml:lang="en">dissolved organic compounds</skos:prefLabel>
    <skos:scopeNote xml:lang="en">Organic compounds present in water, typically as anthropogenic contaminants including pharmaceuticals, pesticides, and herbicides.</skos:scopeNote>
    <skos:broader rdf:resource="http://www.usgs.gov/science/USGSThesaurus/water%20properties"/>
    <skos:inScheme rdf:resource="http://www.usgs.gov/science/USGSThesaurus"/>
  </rdf:Description>
  <rdf:Description about="http://www.usgs.gov/science/USGSThesaurus/nutrient%20content%20%28water%29">
    <rdf:type rdf:resource="http://www.w3.org/2004/02/skos/core#Concept"/>
    <skos:prefLabel xml:lang="en">nutrient content (water)</skos:prefLabel>
    <skos:scopeNote xml:lang="en">Contaminants in water that nourish organisms, especially plants. Includes nitrogen and phosphorus, either of which can lead to the harmful growth of algae and other plants when present to excess in a body of water.</skos:scopeNote>
    <skos:altLabel xml:lang="en">nitrogen content</skos:altLabel>
    <skos:altLabel xml:lang="en">phosphorus content</skos:altLabel>
    <skos:broader rdf:resource="http://www.usgs.gov/science/USGSThesaurus/water%20properties"/>
    <skos:related rdf:resource="http://www.usgs.gov/science/USGSThesaurus/hydrology"/>
    <skos:related rdf:resource="http://www.usgs.gov/science/USGSThesaurus/nutrient%20cycling"/>
    <skos:related rdf:resource="http://www.usgs.gov/science/USGSThesaurus/water%20chemistry"/>
    <skos:inScheme rdf:resource="http://www.usgs.gov/science/USGSThesaurus"/>
  </rdf:Description>
  <rdf:Description about="http://www.usgs.gov/science/USGSThesaurus/oxygen%20content%20%28water%29">
    <rdf:type rdf:resource="http://www.w3.org/2004/02/skos/core#Concept"/>
    <skos:prefLabel xml:lang="en">oxygen content (water)</skos:prefLabel>
    <skos:scopeNote xml:lang="en">Measurement of the concentration of oxygen dissolved in water, which is an important indicator of the condition of a water body.</skos:scopeNote>
    <skos:altLabel xml:lang="en">anoxia</skos:altLabel>
    <skos:altLabel xml:lang="en">dissolved oxygen</skos:altLabel>
    <skos:altLabel xml:lang="en">hypoxia</skos:altLabel>
    <skos:broader rdf:resource="http://www.usgs.gov/science/USGSThesaurus/water%20properties"/>
    <skos:related rdf:resource="http://www.usgs.gov/science/USGSThesaurus/eutrophication"/>
    <skos:related rdf:resource="http://www.usgs.gov/science/USGSThesaurus/hydrology"/>
    <skos:related rdf:resource="http://www.usgs.gov/science/USGSThesaurus/water%20chemistry"/>
    <skos:inScheme rdf:resource="http://www.usgs.gov/science/USGSThesaurus"/>
  </rdf:Description>
  <rdf:Description about="http://www.usgs.gov/science/USGSThesaurus/salinity">
    <rdf:type rdf:resource="http://www.w3.org/2004/02/skos/core#Concept"/>
    <skos:prefLabel xml:lang="en">salinity</skos:prefLabel>
    <skos:scopeNote xml:lang="en">Measure of the concentration of salts dissolved in a solution.</skos:scopeNote>
    <skos:altLabel xml:lang="en">chloride concentration</skos:altLabel>
    <skos:broader rdf:resource="http://www.usgs.gov/science/USGSThesaurus/water%20properties"/>
    <skos:related rdf:resource="http://www.usgs.gov/science/USGSThesaurus/hydrology"/>
    <skos:related rdf:resource="http://www.usgs.gov/science/USGSThesaurus/ocean%20salinity"/>
    <skos:related rdf:resource="http://www.usgs.gov/science/USGSThesaurus/water%20chemistry"/>
    <skos:inScheme rdf:resource="http://www.usgs.gov/science/USGSThesaurus"/>
  </rdf:Description>
  <rdf:Description about="http://www.usgs.gov/science/USGSThesaurus/sound%20velocity">
    <rdf:type rdf:resource="http://www.w3.org/2004/02/skos/core#Concept"/>
    <skos:prefLabel xml:lang="en">sound velocity</skos:prefLabel>
    <skos:scopeNote xml:lang="en">Estimates of the velocity of sound in water, indexed by depth at a specific location, usually calculated from other water properties.</skos:scopeNote>
    <!--FOR sound velocity profiles USE sound velocity WITH profiles-->
    <skos:altLabel xml:lang="en">sound velocity profiles</skos:altLabel>
    <skos:broader rdf:resource="http://www.usgs.gov/science/USGSThesaurus/water%20properties"/>
    <skos:related rdf:resource="http://www.usgs.gov/science/USGSThesaurus/interferometric%20sonar"/>
    <skos:inScheme rdf:resource="http://www.usgs.gov/science/USGSThesaurus"/>
  </rdf:Description>
  <rdf:Description about="http://www.usgs.gov/science/USGSThesaurus/suspended%20material%20%28water%29">
    <rdf:type rdf:resource="http://www.w3.org/2004/02/skos/core#Concept"/>
    <skos:prefLabel xml:lang="en">suspended material (water)</skos:prefLabel>
    <skos:scopeNote xml:lang="en">Sediment or particles of rock, sand, soil, and organic detritus carried in suspension in the water column, in contrast to sediment that moves on or near the streambed.</skos:scopeNote>
    <skos:broader rdf:resource="http://www.usgs.gov/science/USGSThesaurus/water%20properties"/>
    <skos:related rdf:resource="http://www.usgs.gov/science/USGSThesaurus/hydrology"/>
    <skos:related rdf:resource="http://www.usgs.gov/science/USGSThesaurus/water%20chemistry"/>
    <skos:inScheme rdf:resource="http://www.usgs.gov/science/USGSThesaurus"/>
  </rdf:Description>
  <rdf:Description about="http://www.usgs.gov/science/USGSThesaurus/water%20hardness">
    <rdf:type rdf:resource="http://www.w3.org/2004/02/skos/core#Concept"/>
    <skos:prefLabel xml:lang="en">water hardness</skos:prefLabel>
    <skos:scopeNote xml:lang="en">Indicator of the concentration of alkaline salts in water, mainly calcium and magnesium, as a measure of water quality.</skos:scopeNote>
    <skos:altLabel xml:lang="en">hardness (water)</skos:altLabel>
    <skos:broader rdf:resource="http://www.usgs.gov/science/USGSThesaurus/water%20properties"/>
    <skos:related rdf:resource="http://www.usgs.gov/science/USGSThesaurus/hydrology"/>
    <skos:related rdf:resource="http://www.usgs.gov/science/USGSThesaurus/water%20chemistry"/>
    <skos:inScheme rdf:resource="http://www.usgs.gov/science/USGSThesaurus"/>
  </rdf:Description>
  <rdf:Description about="http://www.usgs.gov/science/USGSThesaurus/water%20pH">
    <rdf:type rdf:resource="http://www.w3.org/2004/02/skos/core#Concept"/>
    <skos:prefLabel xml:lang="en">water pH</skos:prefLabel>
    <skos:scopeNote xml:lang="en">The negative logarithm of the hydrogen ion concentration or activity of a water solution. Used for expressing both acidity (pH less than 7) and alkalinity (pH greater than 7), with 7 considered neutral.</skos:scopeNote>
    <skos:altLabel xml:lang="en">pH (water)</skos:altLabel>
    <skos:broader rdf:resource="http://www.usgs.gov/science/USGSThesaurus/water%20properties"/>
    <skos:related rdf:resource="http://www.usgs.gov/science/USGSThesaurus/hydrology"/>
    <skos:related rdf:resource="http://www.usgs.gov/science/USGSThesaurus/water%20chemistry"/>
    <skos:inScheme rdf:resource="http://www.usgs.gov/science/USGSThesaurus"/>
  </rdf:Description>
  <rdf:Description about="http://www.usgs.gov/science/USGSThesaurus/water%20temperature">
    <rdf:type rdf:resource="http://www.w3.org/2004/02/skos/core#Concept"/>
    <skos:prefLabel xml:lang="en">water temperature</skos:prefLabel>
    <skos:scopeNote xml:lang="en">The degrees of heat of water from a given source at a specific time.</skos:scopeNote>
    <skos:altLabel xml:lang="en">temperature (water)</skos:altLabel>
    <skos:broader rdf:resource="http://www.usgs.gov/science/USGSThesaurus/water%20properties"/>
    <skos:related rdf:resource="http://www.usgs.gov/science/USGSThesaurus/hydrology"/>
    <skos:related rdf:resource="http://www.usgs.gov/science/USGSThesaurus/water%20chemistry"/>
    <skos:inScheme rdf:resource="http://www.usgs.gov/science/USGSThesaurus"/>
  </rdf:Description>
  <rdf:Description about="http://www.usgs.gov/science/USGSThesaurus/water%20quality">
    <rdf:type rdf:resource="http://www.w3.org/2004/02/skos/core#Concept"/>
    <skos:prefLabel xml:lang="en">water quality</skos:prefLabel>
    <skos:scopeNote xml:lang="en">The chemical, physical, and biological characteristics of water, usually in respect to its suitability for a particular purpose.</skos:scopeNote>
    <skos:altLabel xml:lang="en">dissolved constituents</skos:altLabel>
    <skos:altLabel xml:lang="en">dissolved contaminants</skos:altLabel>
    <!--FOR water-quality data USE water quality WITH datasets-->
    <skos:altLabel xml:lang="en">water-quality data</skos:altLabel>
    <skos:altLabel xml:lang="en">water-quality</skos:altLabel>
    <skos:broader rdf:resource="http://www.usgs.gov/science/USGSThesaurus/topics"/>
    <skos:narrower rdf:resource="http://www.usgs.gov/science/USGSThesaurus/groundwater%20quality"/>
    <skos:narrower rdf:resource="http://www.usgs.gov/science/USGSThesaurus/marine%20water%20quality"/>
    <skos:narrower rdf:resource="http://www.usgs.gov/science/USGSThesaurus/surface%20water%20quality"/>
    <skos:related rdf:resource="http://www.usgs.gov/science/USGSThesaurus/aquatic%20biology"/>
    <skos:related rdf:resource="http://www.usgs.gov/science/USGSThesaurus/drinking%20water%20use"/>
    <skos:related rdf:resource="http://www.usgs.gov/science/USGSThesaurus/hydrology"/>
    <skos:related rdf:resource="http://www.usgs.gov/science/USGSThesaurus/water%20chemistry"/>
    <skos:related rdf:resource="http://www.usgs.gov/science/USGSThesaurus/water%20properties"/>
    <skos:related rdf:resource="http://www.usgs.gov/science/USGSThesaurus/contamination%20and%20pollution"/>
    <skos:inScheme rdf:resource="http://www.usgs.gov/science/USGSThesaurus"/>
  </rdf:Description>
  <rdf:Description about="http://www.usgs.gov/science/USGSThesaurus/groundwater%20quality">
    <rdf:type rdf:resource="http://www.w3.org/2004/02/skos/core#Concept"/>
    <skos:prefLabel xml:lang="en">groundwater quality</skos:prefLabel>
    <skos:scopeNote xml:lang="en">Fitness of subsurface water for use based on its composition and properties.</skos:scopeNote>
    <skos:altLabel xml:lang="en">ground-water quality</skos:altLabel>
    <skos:broader rdf:resource="http://www.usgs.gov/science/USGSThesaurus/water%20quality"/>
    <skos:related rdf:resource="http://www.usgs.gov/science/USGSThesaurus/groundwater"/>
    <skos:related rdf:resource="http://www.usgs.gov/science/USGSThesaurus/hydrology"/>
    <skos:related rdf:resource="http://www.usgs.gov/science/USGSThesaurus/water%20chemistry"/>
    <skos:inScheme rdf:resource="http://www.usgs.gov/science/USGSThesaurus"/>
  </rdf:Description>
  <rdf:Description about="http://www.usgs.gov/science/USGSThesaurus/marine%20water%20quality">
    <rdf:type rdf:resource="http://www.w3.org/2004/02/skos/core#Concept"/>
    <skos:prefLabel xml:lang="en">marine water quality</skos:prefLabel>
    <skos:scopeNote xml:lang="en">Observed intrinsic characteristics of marine waters affecting their ability to support life or facilitate biological processes such as waste decomposition.</skos:scopeNote>
    <skos:altLabel xml:lang="en">ocean water quality</skos:altLabel>
    <skos:broader rdf:resource="http://www.usgs.gov/science/USGSThesaurus/water%20quality"/>
    <skos:related rdf:resource="http://www.usgs.gov/science/USGSThesaurus/hydrology"/>
    <skos:related rdf:resource="http://www.usgs.gov/science/USGSThesaurus/marine%20chemistry"/>
    <skos:related rdf:resource="http://www.usgs.gov/science/USGSThesaurus/ocean%20sciences"/>
    <skos:inScheme rdf:resource="http://www.usgs.gov/science/USGSThesaurus"/>
  </rdf:Description>
  <rdf:Description about="http://www.usgs.gov/science/USGSThesaurus/surface%20water%20quality">
    <rdf:type rdf:resource="http://www.w3.org/2004/02/skos/core#Concept"/>
    <skos:prefLabel xml:lang="en">surface water quality</skos:prefLabel>
    <skos:scopeNote xml:lang="en">Chemical, physical, and biological characteristics of water in lakes, rivers, or streams related to its fitness for use.</skos:scopeNote>
    <skos:broader rdf:resource="http://www.usgs.gov/science/USGSThesaurus/water%20quality"/>
    <skos:related rdf:resource="http://www.usgs.gov/science/USGSThesaurus/hydrology"/>
    <skos:related rdf:resource="http://www.usgs.gov/science/USGSThesaurus/limnology"/>
    <skos:related rdf:resource="http://www.usgs.gov/science/USGSThesaurus/surface%20water%20%28non-marine%29"/>
    <skos:related rdf:resource="http://www.usgs.gov/science/USGSThesaurus/water%20chemistry"/>
    <skos:inScheme rdf:resource="http://www.usgs.gov/science/USGSThesaurus"/>
  </rdf:Description>
  <rdf:Description about="http://www.usgs.gov/science/USGSThesaurus/water%20supply%20and%20demand">
    <rdf:type rdf:resource="http://www.w3.org/2004/02/skos/core#Concept"/>
    <skos:prefLabel xml:lang="en">water supply and demand</skos:prefLabel>
    <skos:scopeNote xml:lang="en">The quantities of water resources in an area that are easily available and the amount of water that is needed for all uses.</skos:scopeNote>
    <skos:altLabel xml:lang="en">water demand</skos:altLabel>
    <skos:broader rdf:resource="http://www.usgs.gov/science/USGSThesaurus/topics"/>
    <skos:narrower rdf:resource="http://www.usgs.gov/science/USGSThesaurus/wastewater%20discharge"/>
    <skos:narrower rdf:resource="http://www.usgs.gov/science/USGSThesaurus/water%20budget"/>
    <skos:narrower rdf:resource="http://www.usgs.gov/science/USGSThesaurus/water%20use"/>
    <skos:inScheme rdf:resource="http://www.usgs.gov/science/USGSThesaurus"/>
  </rdf:Description>
  <rdf:Description about="http://www.usgs.gov/science/USGSThesaurus/wastewater%20discharge">
    <rdf:type rdf:resource="http://www.w3.org/2004/02/skos/core#Concept"/>
    <skos:prefLabel xml:lang="en">wastewater discharge</skos:prefLabel>
    <skos:scopeNote xml:lang="en">Water that is returned or reused after release from a wastewater treatment plant.</skos:scopeNote>
    <skos:altLabel xml:lang="en">gray water</skos:altLabel>
    <skos:altLabel xml:lang="en">grey water</skos:altLabel>
    <skos:altLabel xml:lang="en">wastewater</skos:altLabel>
    <skos:altLabel xml:lang="en">treated sewage</skos:altLabel>
    <skos:altLabel xml:lang="en">treated wastewater</skos:altLabel>
    <skos:broader rdf:resource="http://www.usgs.gov/science/USGSThesaurus/water%20supply%20and%20demand"/>
    <skos:related rdf:resource="http://www.usgs.gov/science/USGSThesaurus/hydraulic%20engineering"/>
    <skos:related rdf:resource="http://www.usgs.gov/science/USGSThesaurus/hydrology"/>
    <skos:related rdf:resource="http://www.usgs.gov/science/USGSThesaurus/waste%20treatment%20and%20disposal"/>
    <skos:inScheme rdf:resource="http://www.usgs.gov/science/USGSThesaurus"/>
  </rdf:Description>
  <rdf:Description about="http://www.usgs.gov/science/USGSThesaurus/water%20budget">
    <rdf:type rdf:resource="http://www.w3.org/2004/02/skos/core#Concept"/>
    <skos:prefLabel xml:lang="en">water budget</skos:prefLabel>
    <skos:scopeNote xml:lang="en">An accounting of the inflow, outflow, and storage changes of water in a hydrologic unit.</skos:scopeNote>
    <skos:altLabel xml:lang="en">water balance</skos:altLabel>
    <skos:broader rdf:resource="http://www.usgs.gov/science/USGSThesaurus/water%20supply%20and%20demand"/>
    <skos:inScheme rdf:resource="http://www.usgs.gov/science/USGSThesaurus"/>
  </rdf:Description>
  <rdf:Description about="http://www.usgs.gov/science/USGSThesaurus/water%20use">
    <rdf:type rdf:resource="http://www.w3.org/2004/02/skos/core#Concept"/>
    <skos:prefLabel xml:lang="en">water use</skos:prefLabel>
    <skos:scopeNote xml:lang="en">Water withdrawal for a specific purpose, such as domestic use, irrigation, or industrial processing.</skos:scopeNote>
    <skos:altLabel xml:lang="en">consumptive use (water)</skos:altLabel>
    <skos:altLabel xml:lang="en">drawdown</skos:altLabel>
    <skos:altLabel xml:lang="en">water utilities</skos:altLabel>
    <skos:broader rdf:resource="http://www.usgs.gov/science/USGSThesaurus/water%20supply%20and%20demand"/>
    <skos:narrower rdf:resource="http://www.usgs.gov/science/USGSThesaurus/aquaculture%20water%20use"/>
    <skos:narrower rdf:resource="http://www.usgs.gov/science/USGSThesaurus/domestic%20well%20water%20use"/>
    <skos:narrower rdf:resource="http://www.usgs.gov/science/USGSThesaurus/industrial%20water%20use"/>
    <skos:narrower rdf:resource="http://www.usgs.gov/science/USGSThesaurus/irrigation"/>
    <skos:narrower rdf:resource="http://www.usgs.gov/science/USGSThesaurus/mining%20water%20use"/>
    <skos:narrower rdf:resource="http://www.usgs.gov/science/USGSThesaurus/power%20generation%20water%20use"/>
    <skos:narrower rdf:resource="http://www.usgs.gov/science/USGSThesaurus/public%20supply%20water%20use"/>
    <skos:related rdf:resource="http://www.usgs.gov/science/USGSThesaurus/hydraulic%20engineering"/>
    <skos:related rdf:resource="http://www.usgs.gov/science/USGSThesaurus/hydrology"/>
    <skos:inScheme rdf:resource="http://www.usgs.gov/science/USGSThesaurus"/>
  </rdf:Description>
  <rdf:Description about="http://www.usgs.gov/science/USGSThesaurus/aquaculture%20water%20use">
    <rdf:type rdf:resource="http://www.w3.org/2004/02/skos/core#Concept"/>
    <skos:prefLabel xml:lang="en">aquaculture water use</skos:prefLabel>
    <skos:scopeNote xml:lang="en">Use of water to raise aquatic organisms, typically for food, restoration, conservation, or sport.</skos:scopeNote>
    <skos:altLabel xml:lang="en">fish farming</skos:altLabel>
    <skos:broader rdf:resource="http://www.usgs.gov/science/USGSThesaurus/water%20use"/>
    <skos:inScheme rdf:resource="http://www.usgs.gov/science/USGSThesaurus"/>
  </rdf:Description>
  <rdf:Description about="http://www.usgs.gov/science/USGSThesaurus/domestic%20well%20water%20use">
    <rdf:type rdf:resource="http://www.w3.org/2004/02/skos/core#Concept"/>
    <skos:prefLabel xml:lang="en">domestic well water use</skos:prefLabel>
    <skos:scopeNote xml:lang="en">Use of self-supplied water for household purposes, such as drinking, food preparation, bathing, washing clothes and dishes, flushing toilets, and watering lawns and gardens.</skos:scopeNote>
    <skos:altLabel xml:lang="en">self-supplied water use</skos:altLabel>
    <skos:altLabel xml:lang="en">residential well water use</skos:altLabel>
    <skos:broader rdf:resource="http://www.usgs.gov/science/USGSThesaurus/water%20use"/>
    <skos:narrower rdf:resource="http://www.usgs.gov/science/USGSThesaurus/drinking%20water%20use"/>
    <skos:related rdf:resource="http://www.usgs.gov/science/USGSThesaurus/hydraulic%20engineering"/>
    <skos:related rdf:resource="http://www.usgs.gov/science/USGSThesaurus/hydrology"/>
    <skos:inScheme rdf:resource="http://www.usgs.gov/science/USGSThesaurus"/>
  </rdf:Description>
  <rdf:Description about="http://www.usgs.gov/science/USGSThesaurus/drinking%20water%20use">
    <rdf:type rdf:resource="http://www.w3.org/2004/02/skos/core#Concept"/>
    <skos:prefLabel xml:lang="en">drinking water use</skos:prefLabel>
    <skos:scopeNote xml:lang="en"></skos:scopeNote>
    <skos:altLabel xml:lang="en">drinking water</skos:altLabel>
    <skos:altLabel xml:lang="en">potable water</skos:altLabel>
    <skos:broader rdf:resource="http://www.usgs.gov/science/USGSThesaurus/domestic%20well%20water%20use"/>
    <skos:related rdf:resource="http://www.usgs.gov/science/USGSThesaurus/water%20quality"/>
    <skos:inScheme rdf:resource="http://www.usgs.gov/science/USGSThesaurus"/>
  </rdf:Description>
  <rdf:Description about="http://www.usgs.gov/science/USGSThesaurus/industrial%20water%20use">
    <rdf:type rdf:resource="http://www.w3.org/2004/02/skos/core#Concept"/>
    <skos:prefLabel xml:lang="en">industrial water use</skos:prefLabel>
    <skos:scopeNote xml:lang="en">Use of water for industrial purposes such as fabrication, processing, washing, and cooling, and including such industries as steel, chemical and allied products, paper and allied products, mining, and petroleum refining.</skos:scopeNote>
    <skos:broader rdf:resource="http://www.usgs.gov/science/USGSThesaurus/water%20use"/>
    <skos:related rdf:resource="http://www.usgs.gov/science/USGSThesaurus/hydraulic%20engineering"/>
    <skos:related rdf:resource="http://www.usgs.gov/science/USGSThesaurus/hydrology"/>
    <skos:inScheme rdf:resource="http://www.usgs.gov/science/USGSThesaurus"/>
  </rdf:Description>
  <rdf:Description about="http://www.usgs.gov/science/USGSThesaurus/irrigation">
    <rdf:type rdf:resource="http://www.w3.org/2004/02/skos/core#Concept"/>
    <skos:prefLabel xml:lang="en">irrigation</skos:prefLabel>
    <skos:scopeNote xml:lang="en">Artificial application of water on lands to assist in the growing of crops and pastures or to maintain vegetative growth in recreational lands such as parks and golf courses.</skos:scopeNote>
    <skos:altLabel xml:lang="en">spray irrigation</skos:altLabel>
    <skos:altLabel xml:lang="en">microirrigation</skos:altLabel>
    <skos:altLabel xml:lang="en">flood irrigation</skos:altLabel>
    <skos:broader rdf:resource="http://www.usgs.gov/science/USGSThesaurus/water%20use"/>
    <skos:related rdf:resource="http://www.usgs.gov/science/USGSThesaurus/hydraulic%20engineering"/>
    <skos:related rdf:resource="http://www.usgs.gov/science/USGSThesaurus/hydrology"/>
    <skos:inScheme rdf:resource="http://www.usgs.gov/science/USGSThesaurus"/>
  </rdf:Description>
  <rdf:Description about="http://www.usgs.gov/science/USGSThesaurus/mining%20water%20use">
    <rdf:type rdf:resource="http://www.w3.org/2004/02/skos/core#Concept"/>
    <skos:prefLabel xml:lang="en">mining water use</skos:prefLabel>
    <skos:scopeNote xml:lang="en">Water use for the extraction of naturally occurring mineral deposits by mining or quarrying.</skos:scopeNote>
    <skos:broader rdf:resource="http://www.usgs.gov/science/USGSThesaurus/water%20use"/>
    <skos:related rdf:resource="http://www.usgs.gov/science/USGSThesaurus/hydraulic%20engineering"/>
    <skos:related rdf:resource="http://www.usgs.gov/science/USGSThesaurus/hydrology"/>
    <skos:inScheme rdf:resource="http://www.usgs.gov/science/USGSThesaurus"/>
  </rdf:Description>
  <rdf:Description about="http://www.usgs.gov/science/USGSThesaurus/power%20generation%20water%20use">
    <rdf:type rdf:resource="http://www.w3.org/2004/02/skos/core#Concept"/>
    <skos:prefLabel xml:lang="en">power generation water use</skos:prefLabel>
    <skos:scopeNote xml:lang="en">Use of water in the process of producing electric energy by transforming other forms of energy.</skos:scopeNote>
    <skos:altLabel xml:lang="en">hydroelectric power generation water use</skos:altLabel>
    <skos:altLabel xml:lang="en">thermoelectric power generation water use</skos:altLabel>
    <skos:broader rdf:resource="http://www.usgs.gov/science/USGSThesaurus/water%20use"/>
    <skos:related rdf:resource="http://www.usgs.gov/science/USGSThesaurus/hydraulic%20engineering"/>
    <skos:related rdf:resource="http://www.usgs.gov/science/USGSThesaurus/hydrology"/>
    <skos:inScheme rdf:resource="http://www.usgs.gov/science/USGSThesaurus"/>
  </rdf:Description>
  <rdf:Description about="http://www.usgs.gov/science/USGSThesaurus/public%20supply%20water%20use">
    <rdf:type rdf:resource="http://www.w3.org/2004/02/skos/core#Concept"/>
    <skos:prefLabel xml:lang="en">public supply water use</skos:prefLabel>
    <skos:scopeNote xml:lang="en">Provision of water by local governments or private companies for residential, commercial, and light industrial use.</skos:scopeNote>
    <skos:broader rdf:resource="http://www.usgs.gov/science/USGSThesaurus/water%20use"/>
    <skos:inScheme rdf:resource="http://www.usgs.gov/science/USGSThesaurus"/>
  </rdf:Description>
</rdf:RDF>
